@prefix dcterms: <http://purl.org/dc/terms/> .
@prefix ns1: <http://www.opengis.net/def/metamodel/ogc-na/> .
@prefix rdfs: <http://www.w3.org/2000/01/rdf-schema#> .
@prefix skos: <http://www.w3.org/2004/02/skos/core#> .
@prefix xsd: <http://www.w3.org/2001/XMLSchema#> .

<http://www.opengis.net/def/register/> skos:member <http://www.opengis.net/def/namespaces/> .

<http://www.opengis.net/def/namespaces/ogc/1.0/cis> a skos:Concept ;
    rdfs:label "cis" ;
    dcterms:created "2026-01-14T22:50:09.399872"^^xsd:dateTime ;
    skos:definition "Prefix 'cis' for the namespace https://www.opengis.net/def/namespaces/ogc/1.0/cis" ;
    skos:inScheme <http://www.opengis.net/def/namespaces> ;
    skos:notation "http://www.opengis.net/cis/1.1/" ;
    skos:prefLabel "cis" .

<http://www.opengis.net/def/namespaces/ogc/1.0/covjson> a skos:Concept ;
    rdfs:label "covjson" ;
    dcterms:created "2026-01-14T22:50:09.399259"^^xsd:dateTime ;
    skos:definition "Prefix 'covjson' for the namespace https://www.opengis.net/def/namespaces/ogc/1.0/covjson" ;
    skos:inScheme <http://www.opengis.net/def/namespaces> ;
    skos:notation "https://covjson.org/def/core#" ;
    skos:prefLabel "covjson" .

<http://www.opengis.net/def/namespaces/ogc/1.0/covjsondt> a skos:Concept ;
    rdfs:label "covjsondt" ;
    dcterms:created "2026-01-14T22:50:09.399300"^^xsd:dateTime ;
    skos:definition "Prefix 'covjsondt' for the namespace https://www.opengis.net/def/namespaces/ogc/1.0/covjsondt" ;
    skos:inScheme <http://www.opengis.net/def/namespaces> ;
    skos:notation "https://covjson.org/def/domainTypes#" ;
    skos:prefLabel "covjsondt" .

<http://www.opengis.net/def/namespaces/ogc/1.0/dct> a skos:Concept ;
    rdfs:label "dct" ;
    dcterms:created "2026-01-14T22:50:09.399573"^^xsd:dateTime ;
    skos:definition "Prefix 'dct' for the namespace https://www.opengis.net/def/namespaces/ogc/1.0/dct" ;
    skos:inScheme <http://www.opengis.net/def/namespaces> ;
    skos:notation "http://purl.org/dc/terms/" ;
    skos:prefLabel "dct" .

<http://www.opengis.net/def/namespaces/ogc/1.0/hydra> a skos:Concept ;
    rdfs:label "hydra" ;
    dcterms:created "2026-01-14T22:50:09.399618"^^xsd:dateTime ;
    skos:definition "Prefix 'hydra' for the namespace https://www.opengis.net/def/namespaces/ogc/1.0/hydra" ;
    skos:inScheme <http://www.opengis.net/def/namespaces> ;
    skos:notation "http://www.w3.org/namespaces/hydra/core#" ;
    skos:prefLabel "hydra" .

<http://www.opengis.net/def/namespaces/ogc/1.0/ignf> a skos:Concept ;
    rdfs:label "ignf" ;
    dcterms:created "2026-01-14T22:50:09.399705"^^xsd:dateTime ;
    skos:definition "Prefix 'ignf' for the namespace https://www.opengis.net/def/namespaces/ogc/1.0/ignf" ;
    skos:inScheme <http://www.opengis.net/def/namespaces> ;
    skos:notation "http://data.ign.fr/def/ignf#" ;
    skos:prefLabel "ignf" .

<http://www.opengis.net/def/namespaces/ogc/1.0/inspiregloss> a skos:Concept ;
    rdfs:label "inspiregloss" ;
    dcterms:created "2026-01-14T22:50:09.399746"^^xsd:dateTime ;
    skos:definition "Prefix 'inspiregloss' for the namespace https://www.opengis.net/def/namespaces/ogc/1.0/inspiregloss" ;
    skos:inScheme <http://www.opengis.net/def/namespaces> ;
    skos:notation "http://inspire.ec.europa.eu/glossary/" ;
    skos:prefLabel "inspiregloss" .

<http://www.opengis.net/def/namespaces/ogc/1.0/metocean> a skos:Concept ;
    rdfs:label "metocean" ;
    dcterms:created "2026-01-14T22:50:09.399828"^^xsd:dateTime ;
    skos:definition "Prefix 'metocean' for the namespace https://www.opengis.net/def/namespaces/ogc/1.0/metocean" ;
    skos:inScheme <http://www.opengis.net/def/namespaces> ;
    skos:notation "https://api.meteogate.eu/profiles/metocean/covjson" ;
    skos:prefLabel "metocean" .

<http://www.opengis.net/def/namespaces/ogc/1.0/my> a skos:Concept ;
    rdfs:label "my" ;
    dcterms:created "2026-01-14T22:50:09.399045"^^xsd:dateTime ;
    skos:definition "Prefix 'my' for the namespace https://www.opengis.net/def/namespaces/ogc/1.0/my" ;
    skos:inScheme <http://www.opengis.net/def/namespaces> ;
    skos:notation "http://example.org/ApplicationSchema#" ;
    skos:prefLabel "my" .

<http://www.opengis.net/def/namespaces/ogc/1.0/qudt> a skos:Concept ;
    rdfs:label "qudt" ;
    dcterms:created "2026-01-14T22:50:09.399219"^^xsd:dateTime,
        "2026-01-14T22:50:09.399660"^^xsd:dateTime ;
    skos:definition "Prefix 'qudt' for the namespace https://www.opengis.net/def/namespaces/ogc/1.0/qudt" ;
    skos:inScheme <http://www.opengis.net/def/namespaces> ;
    skos:notation "http://qudt.org/schema/qudt#",
        "http://qudt.org/schema/qudt/" ;
    skos:prefLabel "qudt" .

<http://www.opengis.net/def/namespaces/ogc/1.0/rdf> a skos:Concept ;
    rdfs:label "rdf" ;
    dcterms:created "2026-01-14T22:50:09.399092"^^xsd:dateTime ;
    skos:definition "Prefix 'rdf' for the namespace https://www.opengis.net/def/namespaces/ogc/1.0/rdf" ;
    skos:inScheme <http://www.opengis.net/def/namespaces> ;
    skos:notation "http://www.w3.org/1999/02/22-rdf-syntax-ns#" ;
    skos:prefLabel "rdf" .

<http://www.opengis.net/def/namespaces/ogc/1.0/rdfs> a skos:Concept ;
    rdfs:label "rdfs" ;
    dcterms:created "2026-01-14T22:50:09.399133"^^xsd:dateTime ;
    skos:definition "Prefix 'rdfs' for the namespace https://www.opengis.net/def/namespaces/ogc/1.0/rdfs" ;
    skos:inScheme <http://www.opengis.net/def/namespaces> ;
    skos:notation "http://www.w3.org/2000/01/rdf-schema#" ;
    skos:prefLabel "rdfs" .

<http://www.opengis.net/def/namespaces/ogc/1.0/rel> a skos:Concept ;
    rdfs:label "rel" ;
    dcterms:created "2026-01-14T22:50:09.399787"^^xsd:dateTime ;
    skos:definition "Prefix 'rel' for the namespace https://www.opengis.net/def/namespaces/ogc/1.0/rel" ;
    skos:inScheme <http://www.opengis.net/def/namespaces> ;
    skos:notation "http://www.iana.org/assignments/relation/" ;
    skos:prefLabel "rel" .

<http://www.opengis.net/def/namespaces/ogc/1.0/sf> a skos:Concept ;
    rdfs:label "sf" ;
    dcterms:created "2026-01-14T22:50:09.399177"^^xsd:dateTime ;
    skos:definition "Prefix 'sf' for the namespace https://www.opengis.net/def/namespaces/ogc/1.0/sf" ;
    skos:inScheme <http://www.opengis.net/def/namespaces> ;
    skos:notation "http://www.opengis.net/ont/sf#" ;
    skos:prefLabel "sf" .

<http://www.opengis.net/def/namespaces/ogc/1.0/skos> a skos:Concept ;
    rdfs:label "skos" ;
    dcterms:created "2026-01-14T22:50:09.399426"^^xsd:dateTime ;
    skos:definition "Prefix 'skos' for the namespace https://www.opengis.net/def/namespaces/ogc/1.0/skos" ;
    skos:inScheme <http://www.opengis.net/def/namespaces> ;
    skos:notation "http://www.w3.org/2004/02/skos/core#" ;
    skos:prefLabel "skos" .

<http://www.opengis.net/def/namespaces/ogc/1.0/ssn> a skos:Concept ;
    rdfs:label "ssn" ;
    dcterms:created "2026-01-14T22:50:09.399384"^^xsd:dateTime ;
    skos:definition "Prefix 'ssn' for the namespace https://www.opengis.net/def/namespaces/ogc/1.0/ssn" ;
    skos:inScheme <http://www.opengis.net/def/namespaces> ;
    skos:notation "http://www.w3.org/2005/Incubator/ssn/ssnx/ssn#" ;
    skos:prefLabel "ssn" .

<http://www.opengis.net/def/namespaces/ogc/1.0/xsd> a skos:Concept ;
    rdfs:label "xsd" ;
    dcterms:created "2026-01-14T22:50:09.399341"^^xsd:dateTime ;
    skos:definition "Prefix 'xsd' for the namespace https://www.opengis.net/def/namespaces/ogc/1.0/xsd" ;
    skos:inScheme <http://www.opengis.net/def/namespaces> ;
    skos:notation "http://www.w3.org/2001/XMLSchema#" ;
    skos:prefLabel "xsd" .

<http://www.opengis.net/def/namespaces/ogc/1.0/﻿geo> a skos:Concept ;
    rdfs:label "geo" ;
    dcterms:created "2026-01-14T22:50:09.398978"^^xsd:dateTime ;
    skos:definition "Prefix 'geo' for the namespace https://www.opengis.net/def/namespaces/ogc/1.0/geo" ;
    skos:inScheme <http://www.opengis.net/def/namespaces> ;
    skos:notation "http://www.opengis.net/ont/geosparql#" ;
    skos:prefLabel "geo" .

<http://www.opengis.net/def/namespaces/> a skos:Collection ;
    rdfs:label "Namespaces Register" ;
    skos:inScheme <http://www.opengis.net/def/namespaces> ;
    skos:member <http://www.opengis.net/def/namespaces/ogc/1.0/cis>,
        <http://www.opengis.net/def/namespaces/ogc/1.0/covjson>,
        <http://www.opengis.net/def/namespaces/ogc/1.0/covjsondt>,
        <http://www.opengis.net/def/namespaces/ogc/1.0/dct>,
        <http://www.opengis.net/def/namespaces/ogc/1.0/hydra>,
        <http://www.opengis.net/def/namespaces/ogc/1.0/ignf>,
        <http://www.opengis.net/def/namespaces/ogc/1.0/inspiregloss>,
        <http://www.opengis.net/def/namespaces/ogc/1.0/metocean>,
        <http://www.opengis.net/def/namespaces/ogc/1.0/my>,
        <http://www.opengis.net/def/namespaces/ogc/1.0/qudt>,
        <http://www.opengis.net/def/namespaces/ogc/1.0/rdf>,
        <http://www.opengis.net/def/namespaces/ogc/1.0/rdfs>,
        <http://www.opengis.net/def/namespaces/ogc/1.0/rel>,
        <http://www.opengis.net/def/namespaces/ogc/1.0/sf>,
        <http://www.opengis.net/def/namespaces/ogc/1.0/skos>,
        <http://www.opengis.net/def/namespaces/ogc/1.0/ssn>,
        <http://www.opengis.net/def/namespaces/ogc/1.0/xsd>,
        <http://www.opengis.net/def/namespaces/ogc/1.0/﻿geo> ;
    skos:prefLabel "Namespaces Register" .

<http://www.opengis.net/def/namespaces> a skos:ConceptScheme ;
    rdfs:label "Namespaces Register" ;
    ns1:collectionView <http://www.opengis.net/def/namespaces/> ;
    skos:prefLabel "Namespaces Register" .

