<?xml version="1.0" encoding="utf-8"?>
<rdf:RDF
   xmlns:dcterms="http://purl.org/dc/terms/"
   xmlns:ns1="http://www.opengis.net/def/metamodel/ogc-na/"
   xmlns:rdf="http://www.w3.org/1999/02/22-rdf-syntax-ns#"
   xmlns:rdfs="http://www.w3.org/2000/01/rdf-schema#"
   xmlns:skos="http://www.w3.org/2004/02/skos/core#"
>
  <rdf:Description rdf:about="http://www.opengis.net/def/geotiff-tag/dgiwg/2.3/50908">
    <rdf:type rdf:resource="http://www.w3.org/2004/02/skos/core#Concept"/>
    <rdfs:label>TIFF_RSID Tag</rdfs:label>
    <ns1:status rdf:resource="http://www.opengis.net/def/status/valid"/>
    <dcterms:created rdf:datatype="http://www.w3.org/2001/XMLSchema#dateTime">2021-10-14T12:25:02.503220</dcterms:created>
    <rdfs:seeAlso rdf:resource="https://portal.ogc.org/files/95763"/>
    <skos:definition>This tag specifies a File Universal Unique Identifier or RSID according to DGIWG DMF (DGIWG Metadata Foundation) definition.</skos:definition>
    <skos:notation rdf:datatype="http://www.opengis.net/def/encoding/ogc/geotiff">50908</skos:notation>
    <skos:inScheme rdf:resource="http://www.opengis.net/def/geotiff-tag"/>
    <skos:prefLabel>TIFF_RSID Tag</skos:prefLabel>
  </rdf:Description>
  <rdf:Description rdf:about="http://www.opengis.net/def/geotiff-tag/ogc/1.1/34735">
    <rdf:type rdf:resource="http://www.w3.org/2004/02/skos/core#Concept"/>
    <rdfs:label>GeoKeyDirectoryTag</rdfs:label>
    <ns1:status rdf:resource="http://www.opengis.net/def/status/valid"/>
    <dcterms:created rdf:datatype="http://www.w3.org/2001/XMLSchema#dateTime">2021-02-16T12:27:08.805882</dcterms:created>
    <rdfs:seeAlso rdf:resource="http://docs.opengeospatial.org/is/19-008r4/19-008r4.html#_requirements_class_geokeydirectorytag"/>
    <skos:definition>The Keys in GeoTIFF (also called 'GeoKeys') are all referenced from the GeoKeyDirectoryTag tag</skos:definition>
    <skos:notation rdf:datatype="http://www.opengis.net/def/encoding/ogc/geotiff">34735</skos:notation>
    <skos:inScheme rdf:resource="http://www.opengis.net/def/geotiff-tag"/>
    <skos:prefLabel>GeoKeyDirectoryTag</skos:prefLabel>
  </rdf:Description>
  <rdf:Description rdf:about="http://www.opengis.net/def/geotiff-tag/dgiwg/2.3/50909">
    <rdf:type rdf:resource="http://www.w3.org/2004/02/skos/core#Concept"/>
    <rdfs:label>GEO_METADATA Tag</rdfs:label>
    <ns1:status rdf:resource="http://www.opengis.net/def/status/valid"/>
    <dcterms:created rdf:datatype="http://www.w3.org/2001/XMLSchema#dateTime">2021-10-14T12:25:01.803240</dcterms:created>
    <rdfs:seeAlso rdf:resource="https://portal.ogc.org/files/95763"/>
    <skos:definition>This tag may be used for embedding XML-encoded instance documents prepared using 19139-based schema. Note that the type is BYTE instead of ASCII because metadata may contain UTF-8 characters.</skos:definition>
    <skos:notation rdf:datatype="http://www.opengis.net/def/encoding/ogc/geotiff">50909</skos:notation>
    <skos:inScheme rdf:resource="http://www.opengis.net/def/geotiff-tag"/>
    <skos:prefLabel>GEO_METADATA Tag</skos:prefLabel>
  </rdf:Description>
  <rdf:Description rdf:about="http://www.opengis.net/def/geotiff-tag">
    <rdf:type rdf:resource="http://www.w3.org/2004/02/skos/core#ConceptScheme"/>
    <rdfs:label>GeoTIFF Tag Register</rdfs:label>
    <ns1:status rdf:resource="http://www.opengis.net/def/status/valid"/>
    <ns1:collectionView rdf:resource="http://www.opengis.net/def/geotiff-tag/"/>
    <skos:prefLabel>GeoTIFF Tag Register</skos:prefLabel>
    <dcterms:source rdf:resource="http://www.opengis.net/def/entities/bodies/ogcna"/>
    <skos:definition>GeoTIFF Tag Register</skos:definition>
  </rdf:Description>
  <rdf:Description rdf:about="http://www.opengis.net/def/geotiff-tag/ogc/1.1/33550">
    <rdf:type rdf:resource="http://www.w3.org/2004/02/skos/core#Concept"/>
    <rdfs:label>ModelPixelScaleTag</rdfs:label>
    <ns1:status rdf:resource="http://www.opengis.net/def/status/valid"/>
    <dcterms:created rdf:datatype="http://www.w3.org/2001/XMLSchema#dateTime">2021-02-16T12:27:08.804790</dcterms:created>
    <rdfs:seeAlso rdf:resource="http://docs.opengeospatial.org/is/19-008r4/19-008r4.html#_requirements_class_modelpixelscaletag"/>
    <skos:definition>The ModelPixelScaleTag may be used to specify the size of raster pixel spacing in the model space units when the raster space can be embedded in the model space coordinate reference system without rotation</skos:definition>
    <skos:notation rdf:datatype="http://www.opengis.net/def/encoding/ogc/geotiff">33550</skos:notation>
    <skos:inScheme rdf:resource="http://www.opengis.net/def/geotiff-tag"/>
    <skos:prefLabel>ModelPixelScaleTag</skos:prefLabel>
  </rdf:Description>
  <rdf:Description rdf:about="http://www.opengis.net/def/geotiff-tag/ogc/1.1/34737">
    <rdf:type rdf:resource="http://www.w3.org/2004/02/skos/core#Concept"/>
    <rdfs:label>GeoAsciiParamsTag</rdfs:label>
    <ns1:status rdf:resource="http://www.opengis.net/def/status/valid"/>
    <dcterms:created rdf:datatype="http://www.w3.org/2001/XMLSchema#dateTime">2021-02-16T12:27:08.806592</dcterms:created>
    <rdfs:seeAlso rdf:resource="http://docs.opengeospatial.org/is/19-008r4/19-008r4.html#_requirements_class_geoasciiparamstag"/>
    <skos:definition>The GeoAsciiParamsTag supports the storage of parameter values when the values are of type ASCII</skos:definition>
    <skos:notation rdf:datatype="http://www.opengis.net/def/encoding/ogc/geotiff">34737</skos:notation>
    <skos:inScheme rdf:resource="http://www.opengis.net/def/geotiff-tag"/>
    <skos:prefLabel>GeoAsciiParamsTag</skos:prefLabel>
  </rdf:Description>
  <rdf:Description rdf:about="http://www.opengis.net/def/geotiff-tag/ogc/1.1/33922">
    <rdf:type rdf:resource="http://www.w3.org/2004/02/skos/core#Concept"/>
    <rdfs:label>ModelTiepointTag</rdfs:label>
    <ns1:status rdf:resource="http://www.opengis.net/def/status/valid"/>
    <dcterms:created rdf:datatype="http://www.w3.org/2001/XMLSchema#dateTime">2021-02-16T12:27:08.805167</dcterms:created>
    <rdfs:seeAlso rdf:resource="http://docs.opengeospatial.org/is/19-008r4/19-008r4.html#_requirements_class_modeltiepointtag"/>
    <skos:definition>The ModelTiepointTag may be used to help define the transformation between raster space and model space through a set of raster-to-model tiepoints and scaling parameters</skos:definition>
    <skos:notation rdf:datatype="http://www.opengis.net/def/encoding/ogc/geotiff">33922</skos:notation>
    <skos:inScheme rdf:resource="http://www.opengis.net/def/geotiff-tag"/>
    <skos:prefLabel>ModelTiepointTag</skos:prefLabel>
  </rdf:Description>
  <rdf:Description rdf:about="http://www.opengis.net/def/geotiff-tag/">
    <rdf:type rdf:resource="http://www.w3.org/2004/02/skos/core#Collection"/>
    <rdfs:label>GeoTIFF Tag Register</rdfs:label>
    <ns1:status rdf:resource="http://www.opengis.net/def/status/valid"/>
    <skos:inScheme rdf:resource="http://www.opengis.net/def/geotiff-tag"/>
    <skos:member rdf:resource="http://www.opengis.net/def/geotiff-tag/ogc/1.1/33550"/>
    <skos:member rdf:resource="http://www.opengis.net/def/geotiff-tag/ogc/1.1/33922"/>
    <skos:member rdf:resource="http://www.opengis.net/def/geotiff-tag/ogc/1.1/34264"/>
    <skos:member rdf:resource="http://www.opengis.net/def/geotiff-tag/ogc/1.1/34735"/>
    <skos:member rdf:resource="http://www.opengis.net/def/geotiff-tag/ogc/1.1/34736"/>
    <skos:member rdf:resource="http://www.opengis.net/def/geotiff-tag/ogc/1.1/34737"/>
    <skos:member rdf:resource="http://www.opengis.net/def/geotiff-tag/dgiwg/2.3/50909"/>
    <skos:member rdf:resource="http://www.opengis.net/def/geotiff-tag/dgiwg/2.3/50908"/>
    <skos:prefLabel>GeoTIFF Tag Register</skos:prefLabel>
    <skos:definition>GeoTIFF Tag Register</skos:definition>
  </rdf:Description>
  <rdf:Description rdf:about="http://www.opengis.net/def/geotiff-tag/ogc/1.1/34264">
    <rdf:type rdf:resource="http://www.w3.org/2004/02/skos/core#Concept"/>
    <rdfs:label>ModelTransformationTag</rdfs:label>
    <ns1:status rdf:resource="http://www.opengis.net/def/status/valid"/>
    <dcterms:created rdf:datatype="http://www.w3.org/2001/XMLSchema#dateTime">2021-02-16T12:27:08.805526</dcterms:created>
    <rdfs:seeAlso rdf:resource="http://docs.opengeospatial.org/is/19-008r4/19-008r4.html#_requirements_class_modeltransformationtag"/>
    <skos:definition>The ModelTransformationTag may be used to specify the transformation matrix between the raster space (and its dependent pixel-value space) and the (possibly 3D) model space</skos:definition>
    <skos:notation rdf:datatype="http://www.opengis.net/def/encoding/ogc/geotiff">34264</skos:notation>
    <skos:inScheme rdf:resource="http://www.opengis.net/def/geotiff-tag"/>
    <skos:prefLabel>ModelTransformationTag</skos:prefLabel>
  </rdf:Description>
  <rdf:Description rdf:about="http://www.opengis.net/def/geotiff-tag/ogc/1.1/34736">
    <rdf:type rdf:resource="http://www.w3.org/2004/02/skos/core#Concept"/>
    <rdfs:label>GeoDoubleParamsTag</rdfs:label>
    <ns1:status rdf:resource="http://www.opengis.net/def/status/valid"/>
    <dcterms:created rdf:datatype="http://www.w3.org/2001/XMLSchema#dateTime">2021-02-16T12:27:08.806240</dcterms:created>
    <rdfs:seeAlso rdf:resource="http://docs.opengeospatial.org/is/19-008r4/19-008r4.html#_requirements_class_geodoubleparamstag"/>
    <skos:definition>The GeoDoubleParamsTag supports the storage of parameter values when the values are of type Double</skos:definition>
    <skos:notation rdf:datatype="http://www.opengis.net/def/encoding/ogc/geotiff">34736</skos:notation>
    <skos:inScheme rdf:resource="http://www.opengis.net/def/geotiff-tag"/>
    <skos:prefLabel>GeoDoubleParamsTag</skos:prefLabel>
  </rdf:Description>
  <rdf:Description rdf:about="http://www.opengis.net/def/register/">
    <skos:member rdf:resource="http://www.opengis.net/def/geotiff-tag/"/>
  </rdf:Description>
  <rdf:Description rdf:about="http://www.opengis.net/def/entities/bodies/ogcna">
    <rdf:type rdf:resource="http://www.w3.org/2004/02/skos/core#Concept"/>
  </rdf:Description>
</rdf:RDF>
