@prefix dcterms: <http://purl.org/dc/terms/> .
@prefix ns1: <http://www.opengis.net/def/metamodel/ogc-na/> .
@prefix rdfs: <http://www.w3.org/2000/01/rdf-schema#> .
@prefix skos: <http://www.w3.org/2004/02/skos/core#> .
@prefix xsd: <http://www.w3.org/2001/XMLSchema#> .

<http://www.opengis.net/def/register/> skos:member <http://www.opengis.net/def/rel/> .

<http://www.opengis.net/def/entities/bodies/ogcna> a skos:Concept .

<https://www.opengis.net/def/rel/ogc/1.0/legend> a skos:Concept ;
    rdfs:label "legend" ;
    dcterms:created "2024-02-09"^^xsd:date ;
    ns1:status <http://www.opengis.net/def/status/proposed> ;
    rdfs:comment "Not yet registered with IANA" ;
    skos:definition "Refers to a legend for the map."@en ;
    skos:notation "legend" ;
    skos:prefLabel "legend"@en .

<https://www.opengis.net/def/rel/ogc/1.0/map> a skos:Concept ;
    rdfs:label "map" ;
    dcterms:created "2022-04-27"^^xsd:date ;
    ns1:status <http://www.opengis.net/def/status/proposed> ;
    rdfs:comment "Not yet registered with IANA" ;
    skos:definition "Refers to a resource that is map representation of another geospatial resource (e.g. a collection)."@en ;
    skos:notation "map" ;
    skos:prefLabel "map"@en .

<http://www.opengis.net/def/rel/> a skos:Collection ;
    rdfs:label "OGC Link Relation Type Register" ;
    skos:definition "This is a register of link relation types used by OGC standards."@en ;
    skos:inScheme <http://www.opengis.net/def/rel> ;
    skos:member <http://www.opengis.net/def/rel/iana/1.0/alternate>,
        <http://www.opengis.net/def/rel/iana/1.0/collection>,
        <http://www.opengis.net/def/rel/iana/1.0/describedby>,
        <http://www.opengis.net/def/rel/iana/1.0/item>,
        <http://www.opengis.net/def/rel/iana/1.0/license>,
        <http://www.opengis.net/def/rel/iana/1.0/next>,
        <http://www.opengis.net/def/rel/iana/1.0/prev>,
        <http://www.opengis.net/def/rel/iana/1.0/self>,
        <http://www.opengis.net/def/rel/iana/1.0/service-desc>,
        <http://www.opengis.net/def/rel/iana/1.0/service-doc>,
        <http://www.opengis.net/def/rel/iana/1.0/status>,
        <http://www.opengis.net/def/rel/iana/1.0/up>,
        <http://www.opengis.net/def/rel/ogc/1.0/conformance>,
        <http://www.opengis.net/def/rel/ogc/1.0/data>,
        <http://www.opengis.net/def/rel/ogc/1.0/data-meta>,
        <http://www.opengis.net/def/rel/ogc/1.0/dataset>,
        <http://www.opengis.net/def/rel/ogc/1.0/exceptions>,
        <http://www.opengis.net/def/rel/ogc/1.0/execute>,
        <http://www.opengis.net/def/rel/ogc/1.0/geodata>,
        <http://www.opengis.net/def/rel/ogc/1.0/items>,
        <http://www.opengis.net/def/rel/ogc/1.0/job-list>,
        <http://www.opengis.net/def/rel/ogc/1.0/processes>,
        <http://www.opengis.net/def/rel/ogc/1.0/results>,
        <http://www.opengis.net/def/rel/ogc/1.0/tilesets-coverage>,
        <http://www.opengis.net/def/rel/ogc/1.0/tilesets-map>,
        <http://www.opengis.net/def/rel/ogc/1.0/tilesets-vector>,
        <http://www.opengis.net/def/rel/ogc/1.0/tiling-scheme>,
        <http://www.opengis.net/def/rel/ogc/1.0/tiling-schemes>,
        <https://www.opengis.net/def/rel/ogc/1.0/legend>,
        <https://www.opengis.net/def/rel/ogc/1.0/map> ;
    skos:prefLabel "OGC Link Relation Type Register"@en .

<http://www.opengis.net/def/rel/iana/1.0/alternate> a skos:Concept ;
    rdfs:label "alternate" ;
    dcterms:created "2020-06-10"^^xsd:date ;
    ns1:status <http://www.opengis.net/def/status/valid> ;
    rdfs:comment "Registered with IANA" ;
    skos:definition " Refers to a substitute for this context."@en ;
    skos:inScheme <http://www.opengis.net/def/rel> ;
    skos:notation "alternate"^^<https://www.iana.org/assignments/link-relations> ;
    skos:prefLabel "alternate"@en ;
    skos:topConceptOf <http://www.opengis.net/def/rel> .

<http://www.opengis.net/def/rel/iana/1.0/collection> a skos:Concept ;
    rdfs:label "collection" ;
    dcterms:created "2020-06-10"^^xsd:date ;
    ns1:status <http://www.opengis.net/def/status/valid> ;
    rdfs:comment "Registered with IANA" ;
    skos:definition " The target IRI points to a resource which represents the collection resource for the context IRI."@en ;
    skos:inScheme <http://www.opengis.net/def/rel> ;
    skos:notation "collection"^^<https://www.iana.org/assignments/link-relations> ;
    skos:prefLabel "collection"@en ;
    skos:topConceptOf <http://www.opengis.net/def/rel> .

<http://www.opengis.net/def/rel/iana/1.0/describedby> a skos:Concept ;
    rdfs:label "describedby" ;
    dcterms:created "2020-06-10"^^xsd:date ;
    ns1:status <http://www.opengis.net/def/status/valid> ;
    rdfs:comment "Registered with IANA" ;
    skos:definition " Refers to a resource providing information about the link’s context."@en ;
    skos:inScheme <http://www.opengis.net/def/rel> ;
    skos:notation "describedby"^^<https://www.iana.org/assignments/link-relations> ;
    skos:prefLabel "describedby"@en ;
    skos:topConceptOf <http://www.opengis.net/def/rel> .

<http://www.opengis.net/def/rel/iana/1.0/item> a skos:Concept ;
    rdfs:label "item" ;
    dcterms:created "2020-06-10"^^xsd:date ;
    ns1:status <http://www.opengis.net/def/status/valid> ;
    rdfs:comment "Registered with IANA" ;
    skos:definition " The target IRI points to a resource that is a member of the collection represented by the context IRI."@en ;
    skos:inScheme <http://www.opengis.net/def/rel> ;
    skos:notation "item"^^<https://www.iana.org/assignments/link-relations> ;
    skos:prefLabel "item"@en ;
    skos:topConceptOf <http://www.opengis.net/def/rel> .

<http://www.opengis.net/def/rel/iana/1.0/license> a skos:Concept ;
    rdfs:label "license" ;
    dcterms:created "2020-06-10"^^xsd:date ;
    ns1:status <http://www.opengis.net/def/status/valid> ;
    rdfs:comment "Registered with IANA" ;
    skos:definition " Refers to a license associated with this context."@en ;
    skos:inScheme <http://www.opengis.net/def/rel> ;
    skos:notation "license"^^<https://www.iana.org/assignments/link-relations> ;
    skos:prefLabel "license"@en ;
    skos:topConceptOf <http://www.opengis.net/def/rel> .

<http://www.opengis.net/def/rel/iana/1.0/next> a skos:Concept ;
    rdfs:label "next" ;
    dcterms:created "2020-06-10"^^xsd:date ;
    ns1:status <http://www.opengis.net/def/status/valid> ;
    rdfs:comment "Registered with IANA" ;
    skos:definition " Indicates that the link’s context is a part of a series, and that the next in the series is the link target."@en ;
    skos:inScheme <http://www.opengis.net/def/rel> ;
    skos:notation "next"^^<https://www.iana.org/assignments/link-relations> ;
    skos:prefLabel "next"@en ;
    skos:topConceptOf <http://www.opengis.net/def/rel> .

<http://www.opengis.net/def/rel/iana/1.0/prev> a skos:Concept ;
    rdfs:label "prev" ;
    dcterms:created "2020-06-10"^^xsd:date ;
    ns1:status <http://www.opengis.net/def/status/valid> ;
    rdfs:comment "Registered with IANA" ;
    skos:definition " Indicates that the link’s context is a part of a series, and that the previous in the series is the link target. This relation is only used in examples."@en ;
    skos:inScheme <http://www.opengis.net/def/rel> ;
    skos:notation "prev"^^<https://www.iana.org/assignments/link-relations> ;
    skos:prefLabel "prev"@en ;
    skos:topConceptOf <http://www.opengis.net/def/rel> .

<http://www.opengis.net/def/rel/iana/1.0/self> a skos:Concept ;
    rdfs:label "self" ;
    dcterms:created "2020-06-10"^^xsd:date ;
    ns1:status <http://www.opengis.net/def/status/valid> ;
    rdfs:comment "Registered with IANA" ;
    skos:definition " Conveys an identifier for the link’s context."@en ;
    skos:inScheme <http://www.opengis.net/def/rel> ;
    skos:notation "self"^^<https://www.iana.org/assignments/link-relations> ;
    skos:prefLabel "self"@en ;
    skos:topConceptOf <http://www.opengis.net/def/rel> .

<http://www.opengis.net/def/rel/iana/1.0/service-desc> a skos:Concept ;
    rdfs:label "service-desc" ;
    dcterms:created "2020-06-10"^^xsd:date ;
    ns1:status <http://www.opengis.net/def/status/valid> ;
    rdfs:comment "Registered with IANA" ;
    skos:definition " Identifies service description for the context that is primarily intended for consumption by machines. API definitions are considered service descriptions."@en ;
    skos:inScheme <http://www.opengis.net/def/rel> ;
    skos:notation "service-desc"^^<https://www.iana.org/assignments/link-relations> ;
    skos:prefLabel "service-desc"@en ;
    skos:topConceptOf <http://www.opengis.net/def/rel> .

<http://www.opengis.net/def/rel/iana/1.0/service-doc> a skos:Concept ;
    rdfs:label "service-doc" ;
    dcterms:created "2020-06-10"^^xsd:date ;
    ns1:status <http://www.opengis.net/def/status/valid> ;
    rdfs:comment "Registered with IANA" ;
    skos:definition " Identifies service documentation for the context that is primarily intended for human consumption."@en ;
    skos:inScheme <http://www.opengis.net/def/rel> ;
    skos:notation "service-doc"^^<https://www.iana.org/assignments/link-relations> ;
    skos:prefLabel "service-doc"@en ;
    skos:topConceptOf <http://www.opengis.net/def/rel> .

<http://www.opengis.net/def/rel/iana/1.0/status> a skos:Concept ;
    rdfs:label "status" ;
    dcterms:created "2022-04-27"^^xsd:date ;
    ns1:status <http://www.opengis.net/def/status/valid> ;
    rdfs:comment "Registered with IANA" ;
    skos:definition "Identifies a resource that represents the status of the context."@en ;
    skos:inScheme <http://www.opengis.net/def/rel> ;
    skos:notation "status"^^<https://www.iana.org/assignments/link-relations> ;
    skos:prefLabel "status"@en ;
    skos:topConceptOf <http://www.opengis.net/def/rel> .

<http://www.opengis.net/def/rel/iana/1.0/up> a skos:Concept ;
    rdfs:label "up" ;
    dcterms:created "2022-04-27"^^xsd:date ;
    ns1:status <http://www.opengis.net/def/status/valid> ;
    rdfs:comment "Registered with IANA" ;
    skos:definition "Refers to a parent document in a hierarchy of documents."@en ;
    skos:inScheme <http://www.opengis.net/def/rel> ;
    skos:notation "up"^^<https://www.iana.org/assignments/link-relations> ;
    skos:prefLabel "up"@en ;
    skos:topConceptOf <http://www.opengis.net/def/rel> .

<http://www.opengis.net/def/rel/ogc/1.0/conformance> a skos:Concept ;
    rdfs:label "conformance" ;
    dcterms:created "2020-06-10"^^xsd:date ;
    ns1:status <http://www.opengis.net/def/status/proposed> ;
    rdfs:comment "Not yet registered with IANA" ;
    skos:definition " Refers to a resource that identifies the specifications that the link’s context conforms to."@en ;
    skos:inScheme <http://www.opengis.net/def/rel> ;
    skos:notation "conformance" ;
    skos:prefLabel "conformance"@en ;
    skos:topConceptOf <http://www.opengis.net/def/rel> .

<http://www.opengis.net/def/rel/ogc/1.0/data> a skos:Concept ;
    rdfs:label "data" ;
    dcterms:created "2020-06-10"^^xsd:date ;
    ns1:status <http://www.opengis.net/def/status/proposed> ;
    rdfs:comment "Not yet registered with IANA" ;
    skos:definition " Indicates that the link’s context is a distribution of a dataset that is an API and refers to the root resource of the dataset in the API."@en ;
    skos:inScheme <http://www.opengis.net/def/rel> ;
    skos:notation "data" ;
    skos:prefLabel "data"@en ;
    skos:topConceptOf <http://www.opengis.net/def/rel> .

<http://www.opengis.net/def/rel/ogc/1.0/data-meta> a skos:Concept ;
    rdfs:label "data-meta" ;
    dcterms:created "2021-04-28"^^xsd:date ;
    ns1:status <http://www.opengis.net/def/status/proposed> ;
    rdfs:comment "Not yet registered with IANA" ;
    skos:definition "Identifies general metadata for the context (dataset or collection) that is primarily intended for consumption by machines."@en ;
    skos:inScheme <http://www.opengis.net/def/rel> ;
    skos:notation "data-meta" ;
    skos:prefLabel "data-meta"@en ;
    skos:topConceptOf <http://www.opengis.net/def/rel> .

<http://www.opengis.net/def/rel/ogc/1.0/dataset> a skos:Concept ;
    rdfs:label "dataset" ;
    dcterms:created "2022-04-27"^^xsd:date ;
    ns1:status <http://www.opengis.net/def/status/proposed> ;
    rdfs:comment "Not yet registered with IANA" ;
    skos:definition "The target IRI points to a resource representing the dataset (e.g. the root of an OGC Web API)."@en ;
    skos:inScheme <http://www.opengis.net/def/rel> ;
    skos:notation "dataset" ;
    skos:prefLabel "dataset"@en ;
    skos:topConceptOf <http://www.opengis.net/def/rel> .

<http://www.opengis.net/def/rel/ogc/1.0/exceptions> a skos:Concept ;
    rdfs:label "exceptions" ;
    dcterms:created "2020-06-10"^^xsd:date ;
    ns1:status <http://www.opengis.net/def/status/proposed> ;
    rdfs:comment "Not yet registered with IANA" ;
    skos:definition "The target URI points to exceptions of a failed process."@en ;
    skos:inScheme <http://www.opengis.net/def/rel> ;
    skos:notation "exceptions" ;
    skos:prefLabel "exceptions"@en ;
    skos:topConceptOf <http://www.opengis.net/def/rel> .

<http://www.opengis.net/def/rel/ogc/1.0/execute> a skos:Concept ;
    rdfs:label "execute" ;
    dcterms:created "2020-06-10"^^xsd:date ;
    ns1:status <http://www.opengis.net/def/status/proposed> ;
    rdfs:comment "Not yet registered with IANA" ;
    skos:definition "The target URI points to the execution endpoint of the server."@en ;
    skos:inScheme <http://www.opengis.net/def/rel> ;
    skos:notation "execute" ;
    skos:prefLabel "execute"@en ;
    skos:topConceptOf <http://www.opengis.net/def/rel> .

<http://www.opengis.net/def/rel/ogc/1.0/geodata> a skos:Concept ;
    rdfs:label "geodata" ;
    dcterms:created "2022-04-27"^^xsd:date ;
    ns1:status <http://www.opengis.net/def/status/proposed> ;
    rdfs:comment "Not yet registered with IANA" ;
    skos:definition "The target IRI points to a resource representing a collection of geospatial data."@en ;
    skos:inScheme <http://www.opengis.net/def/rel> ;
    skos:notation "geodata" ;
    skos:prefLabel "geodata"@en ;
    skos:topConceptOf <http://www.opengis.net/def/rel> .

<http://www.opengis.net/def/rel/ogc/1.0/items> a skos:Concept ;
    rdfs:label "items" ;
    dcterms:created "2020-06-10"^^xsd:date ;
    ns1:status <http://www.opengis.net/def/status/proposed> ;
    rdfs:comment "Not yet registered with IANA" ;
    skos:definition " Refers to a resource that is comprised of members of the collection represented by the link’s context."@en ;
    skos:inScheme <http://www.opengis.net/def/rel> ;
    skos:notation "items" ;
    skos:prefLabel "items"@en ;
    skos:topConceptOf <http://www.opengis.net/def/rel> .

<http://www.opengis.net/def/rel/ogc/1.0/job-list> a skos:Concept ;
    rdfs:label "job-list" ;
    dcterms:created "2020-06-10"^^xsd:date ;
    ns1:status <http://www.opengis.net/def/status/proposed> ;
    rdfs:comment "Not yet registered with IANA" ;
    skos:definition "The target URI points to the list of jobs."@en ;
    skos:inScheme <http://www.opengis.net/def/rel> ;
    skos:notation "job-list" ;
    skos:prefLabel "job-list"@en ;
    skos:topConceptOf <http://www.opengis.net/def/rel> .

<http://www.opengis.net/def/rel/ogc/1.0/processes> a skos:Concept ;
    rdfs:label "processes" ;
    dcterms:created "2020-06-10"^^xsd:date ;
    ns1:status <http://www.opengis.net/def/status/proposed> ;
    rdfs:comment "Not yet registered with IANA" ;
    skos:definition "The target URI points to the list of processes the API offers."@en ;
    skos:inScheme <http://www.opengis.net/def/rel> ;
    skos:notation "processes" ;
    skos:prefLabel "processes"@en ;
    skos:topConceptOf <http://www.opengis.net/def/rel> .

<http://www.opengis.net/def/rel/ogc/1.0/results> a skos:Concept ;
    rdfs:label "results" ;
    dcterms:created "2020-06-10"^^xsd:date ;
    ns1:status <http://www.opengis.net/def/status/proposed> ;
    rdfs:comment "Not yet registered with IANA" ;
    skos:definition "The target URI points to the results of a job."@en ;
    skos:inScheme <http://www.opengis.net/def/rel> ;
    skos:notation "results" ;
    skos:prefLabel "results"@en ;
    skos:topConceptOf <http://www.opengis.net/def/rel> .

<http://www.opengis.net/def/rel/ogc/1.0/tilesets-coverage> a skos:Concept ;
    rdfs:label "tilesets-coverage" ;
    dcterms:created "2022-04-27"^^xsd:date ;
    ns1:status <http://www.opengis.net/def/status/proposed> ;
    rdfs:comment "Not yet registered with IANA" ;
    skos:definition "The target IRI points to a resource that describes how to provide tile sets of the context resource in coverage format."@en ;
    skos:inScheme <http://www.opengis.net/def/rel> ;
    skos:notation "tilesets-coverage" ;
    skos:prefLabel "tilesets-coverage"@en ;
    skos:topConceptOf <http://www.opengis.net/def/rel> .

<http://www.opengis.net/def/rel/ogc/1.0/tilesets-map> a skos:Concept ;
    rdfs:label "tilesets-map" ;
    dcterms:created "2022-04-27"^^xsd:date ;
    ns1:status <http://www.opengis.net/def/status/proposed> ;
    rdfs:comment "Not yet registered with IANA" ;
    skos:definition "The target IRI points to a resource that describes how to provide tile sets of the context resource in map format."@en ;
    skos:inScheme <http://www.opengis.net/def/rel> ;
    skos:notation "tilesets-map" ;
    skos:prefLabel "tilesets-map"@en ;
    skos:topConceptOf <http://www.opengis.net/def/rel> .

<http://www.opengis.net/def/rel/ogc/1.0/tilesets-vector> a skos:Concept ;
    rdfs:label "tilesets-vector" ;
    dcterms:created "2022-04-27"^^xsd:date ;
    ns1:status <http://www.opengis.net/def/status/proposed> ;
    rdfs:comment "Not yet registered with IANA" ;
    skos:definition "The target IRI points to a resource that describes how to provide tile sets of the context resource in vector format."@en ;
    skos:inScheme <http://www.opengis.net/def/rel> ;
    skos:notation "tilesets-vector" ;
    skos:prefLabel "tilesets-vector"@en ;
    skos:topConceptOf <http://www.opengis.net/def/rel> .

<http://www.opengis.net/def/rel/ogc/1.0/tiling-scheme> a skos:Concept ;
    rdfs:label "tiling-scheme" ;
    dcterms:created "2022-04-27"^^xsd:date ;
    ns1:status <http://www.opengis.net/def/status/proposed> ;
    rdfs:comment "Not yet registered with IANA" ;
    skos:definition "The target IRI points to a resource that describes the TileMatrixSet according to the 2D-TMS standard."@en ;
    skos:inScheme <http://www.opengis.net/def/rel> ;
    skos:notation "tiling-scheme" ;
    skos:prefLabel "tiling-scheme"@en ;
    skos:topConceptOf <http://www.opengis.net/def/rel> .

<http://www.opengis.net/def/rel/ogc/1.0/tiling-schemes> a skos:Concept ;
    rdfs:label "tiling-schemes" ;
    dcterms:created "2022-04-27"^^xsd:date ;
    ns1:status <http://www.opengis.net/def/status/proposed> ;
    rdfs:comment "Not yet registered with IANA" ;
    skos:definition "The target IRI points to a resource that lists one or more TileMatrixSets according to the 2D-TMS standard."@en ;
    skos:inScheme <http://www.opengis.net/def/rel> ;
    skos:notation "tiling-schemes" ;
    skos:prefLabel "tiling-schemes"@en ;
    skos:topConceptOf <http://www.opengis.net/def/rel> .

<http://www.opengis.net/def/rel> a skos:ConceptScheme ;
    rdfs:label "OGC Link Relation Type Register" ;
    dcterms:source <http://www.opengis.net/def/entities/bodies/ogcna> ;
    ns1:collectionView <http://www.opengis.net/def/rel/> ;
    skos:definition "This is a register of link relation types used by OGC standards. "@en ;
    skos:hasTopConcept <http://www.opengis.net/def/rel/iana/1.0/alternate>,
        <http://www.opengis.net/def/rel/iana/1.0/collection>,
        <http://www.opengis.net/def/rel/iana/1.0/describedby>,
        <http://www.opengis.net/def/rel/iana/1.0/item>,
        <http://www.opengis.net/def/rel/iana/1.0/license>,
        <http://www.opengis.net/def/rel/iana/1.0/next>,
        <http://www.opengis.net/def/rel/iana/1.0/prev>,
        <http://www.opengis.net/def/rel/iana/1.0/self>,
        <http://www.opengis.net/def/rel/iana/1.0/service-desc>,
        <http://www.opengis.net/def/rel/iana/1.0/service-doc>,
        <http://www.opengis.net/def/rel/iana/1.0/status>,
        <http://www.opengis.net/def/rel/iana/1.0/up>,
        <http://www.opengis.net/def/rel/ogc/1.0/conformance>,
        <http://www.opengis.net/def/rel/ogc/1.0/data>,
        <http://www.opengis.net/def/rel/ogc/1.0/data-meta>,
        <http://www.opengis.net/def/rel/ogc/1.0/dataset>,
        <http://www.opengis.net/def/rel/ogc/1.0/exceptions>,
        <http://www.opengis.net/def/rel/ogc/1.0/execute>,
        <http://www.opengis.net/def/rel/ogc/1.0/geodata>,
        <http://www.opengis.net/def/rel/ogc/1.0/items>,
        <http://www.opengis.net/def/rel/ogc/1.0/job-list>,
        <http://www.opengis.net/def/rel/ogc/1.0/processes>,
        <http://www.opengis.net/def/rel/ogc/1.0/results>,
        <http://www.opengis.net/def/rel/ogc/1.0/tilesets-coverage>,
        <http://www.opengis.net/def/rel/ogc/1.0/tilesets-map>,
        <http://www.opengis.net/def/rel/ogc/1.0/tilesets-vector>,
        <http://www.opengis.net/def/rel/ogc/1.0/tiling-scheme>,
        <http://www.opengis.net/def/rel/ogc/1.0/tiling-schemes> ;
    skos:prefLabel "OGC Link Relation Type Register"@en .

