@prefix dc: <http://purl.org/dc/elements/1.1/> .
@prefix dcterms: <http://purl.org/dc/terms/> .
@prefix def: <http://www.opengis.net/def/> .
@prefix owl: <http://www.w3.org/2002/07/owl#> .
@prefix policy: <http://www.opengis.net/def/metamodel/ogc-na/> .
@prefix rdfs: <http://www.w3.org/2000/01/rdf-schema#> .
@prefix skos: <http://www.w3.org/2004/02/skos/core#> .
@prefix status: <http://www.opengis.net/def/status/> .
@prefix xsd: <http://www.w3.org/2001/XMLSchema#> .

def:uom a skos:ConceptScheme ;
    rdfs:label "units of measure definitions"^^xsd:string ;
    dcterms:source "OGC Naming Authority on behalf of relevant OGC Working Group" ;
    policy:collectionView <http://www.opengis.net/def/uom/> ;
    skos:prefLabel "units of measure definitions" .

<http://www.opengis.net/def/uom/OGC/1.0> owl:sameAs <http://www.opengis.net/def/uom/OGC/1.0/> .

<http://www.opengis.net/def/uom/UCUM> owl:sameAs <http://www.opengis.net/def/uom/UCUM/> .

<http://www.opengis.net/def/uom/UCUM/0> owl:sameAs <http://www.opengis.net/def/uom/UCUM/0/> .

<http://www.opengis.net/def/uom/> a skos:Collection ;
    rdfs:label "units of measure" ;
    dc:source "ISO 10000"^^xsd:string ;
    dcterms:created "2012-02-14"^^xsd:date ;
    skos:member <http://www.opengis.net/def/uom/EPSG/>,
        <http://www.opengis.net/def/uom/OGC/>,
        <http://www.opengis.net/def/uom/SI/>,
        <http://www.opengis.net/def/uom/UCUM/> .

<http://www.opengis.net/def/uom/EPSG/> a skos:Collection ;
    rdfs:label "EPSG units of measure"^^xsd:string ;
    owl:sameAs <http://www.opengis.net/def/uom/epsg/> .

<http://www.opengis.net/def/uom/OGC/> a skos:Collection ;
    rdfs:label "OGC Units of Measure" ;
    dcterms:created "2012-02-14"^^xsd:date ;
    owl:sameAs <http://www.opengis.net/def/uom/ogc/> ;
    skos:member <http://www.opengis.net/def/uom/OGC/1.0/> .

<http://www.opengis.net/def/uom/SI/ampere> a skos:Concept ;
    rdfs:seeAlso <http://www.bipm.org/en/si/si_brochure/chapter2/2-1/ampere.html> ;
    skos:definition "The ampere is that constant current which, if maintained in two straight parallel conductors of infinite length, of negligible circular cross-section, and placed 1 m apart in vacuum, would produce between these conductors a force equal to 2 x 10â€“7 newton per metre of length."^^xsd:string ;
    skos:exactMatch <http://qudt.org/vocab/unit#Ampere> ;
    skos:notation "A"^^xsd:string .

<http://www.opengis.net/def/uom/SI/candela> a skos:Concept ;
    rdfs:seeAlso <http://www.bipm.org/en/si/si_brochure/chapter2/2-1/candela.html> ;
    skos:definition "The candela is the luminous intensity, in a given direction, of a source that emits monochromatic radiation of frequency 540 x 1012 hertz and that has a radiant intensity in that direction of 1/683 watt per steradian."^^xsd:string ;
    skos:exactMatch <http://qudt.org/vocab/unit#Candela> ;
    skos:notation "cd"^^xsd:string .

<http://www.opengis.net/def/uom/SI/kelvin> a skos:Concept ;
    rdfs:seeAlso <http://www.bipm.org/en/si/si_brochure/chapter2/2-1/kelvin.html> ;
    skos:definition "The kelvin, unit of thermodynamic temperature, is the fraction 1/273.16 of the thermodynamic temperature of the triple point of water."^^xsd:string ;
    skos:exactMatch <http://qudt.org/vocab/unit#Kelvin> ;
    skos:notation "K"^^xsd:string .

<http://www.opengis.net/def/uom/SI/kilogram> a skos:Concept ;
    rdfs:seeAlso <http://www.bipm.org/en/si/si_brochure/chapter2/2-1/kilogram.html> ;
    skos:definition "The kilogram is the unit of mass; it is equal to the mass of the international prototype of the kilogram."^^xsd:string ;
    skos:exactMatch <http://qudt.org/vocab/unit#Kilogram> ;
    skos:notation "kg"^^xsd:string .

<http://www.opengis.net/def/uom/SI/metre> a skos:Concept ;
    rdfs:seeAlso <http://www.bipm.org/en/si/si_brochure/chapter2/2-1/metre.html> ;
    skos:definition "The metre is the length of the path travelled by light in vacuum during a time interval of 1/299 792 458 of a second."^^xsd:string ;
    skos:exactMatch <http://qudt.org/vocab/unit#Meter> ;
    skos:notation "m"^^xsd:string .

<http://www.opengis.net/def/uom/SI/mole> a skos:Concept ;
    rdfs:seeAlso <http://www.bipm.org/en/si/si_brochure/chapter2/2-1/mole.html> ;
    skos:definition """	1.	The mole is the amount of substance of a system which contains as many elementary entities as there are atoms in 0.012 kilogram of carbon 12.\r
2.	When the mole is used, the elementary entities must be specified and may be atoms, molecules, ions, electrons, other particles, or specified groups of such particles."""^^xsd:string ;
    skos:exactMatch <http://qudt.org/vocab/unit#Mole> ;
    skos:notation "mol"^^xsd:string .

<http://www.opengis.net/def/uom/SI/second> a skos:Concept ;
    rdfs:seeAlso <http://www.bipm.org/en/si/si_brochure/chapter2/2-1/second.html> ;
    skos:definition "The second is the duration of 9 192 631 770 periods of the radiation corresponding to the transition between the two hyperfine levels of the ground state of the caesium 133 atom."^^xsd:string ;
    skos:exactMatch <http://qudt.org/vocab/unit#Second> ;
    skos:notation "s"^^xsd:string .

<http://www.opengis.net/def/uom/epsg/> a skos:Collection .

<http://www.opengis.net/def/uom/ogc/> a skos:Collection .

<http://www.opengis.net/def/uom/ogc/1.0/> a skos:Collection .

<http://www.opengis.net/def/uom/ogc/1.0/degree> a skos:Concept ;
    policy:status status:valid ;
    owl:sameAs <http://www.opengis.net/def/uom/OGC/1.0/degree> .

<http://www.opengis.net/def/uom/ogc/1.0/gridspacing> a skos:Concept ;
    policy:status status:valid ;
    owl:sameAs <http://www.opengis.net/def/uom/OGC/1.0/GridSpacing> .

<http://www.opengis.net/def/uom/ogc/1.0/metre> a skos:Concept ;
    policy:status status:valid ;
    owl:sameAs <http://www.opengis.net/def/uom/OGC/1.0/metre> .

<http://www.opengis.net/def/uom/ogc/1.0/radian> a skos:Concept ;
    policy:status status:valid ;
    owl:sameAs <http://www.opengis.net/def/uom/OGC/1.0/radian> .

<http://www.opengis.net/def/uom/ogc/1.0/unity> a skos:Concept ;
    policy:status status:valid ;
    owl:sameAs <http://www.opengis.net/def/uom/OGC/1.0/unity> .

<http://www.opengis.net/def/uom/si/> owl:sameAs <http://www.opengis.net/def/uom/SI/> .

<http://www.opengis.net/def/uom/ucum/> a skos:Collection .

<http://www.opengis.net/def/uom/ucum/0/> a skos:Collection .

<http://www.opengis.net/def/uom/OGC/1.0/> a skos:Collection ;
    rdfs:label "OGC Units of Measure 1.0" ;
    dcterms:created "2012-02-14"^^xsd:date ;
    owl:sameAs <http://www.opengis.net/def/uom/ogc/1.0/> ;
    skos:member <http://www.opengis.net/def/uom/OGC/1.0/GridSpacing>,
        <http://www.opengis.net/def/uom/OGC/1.0/degree>,
        <http://www.opengis.net/def/uom/OGC/1.0/metre>,
        <http://www.opengis.net/def/uom/OGC/1.0/radian>,
        <http://www.opengis.net/def/uom/OGC/1.0/unity> .

<http://www.opengis.net/def/uom/OGC/1.0/GridSpacing> a skos:Concept ;
    rdfs:label "grid spacing"@en ;
    dc:creator "Arliss Whiteside" ;
    dc:date "2010-03-23" ;
    dcterms:created "2010-03-23" ;
    dcterms:modified "2012-02-14"^^xsd:date ;
    policy:status status:valid ;
    owl:sameAs <http://www.opengis.net/def/uom/ogc/1.0/gridspacing> ;
    skos:definition "Spacing between adjacent grid lines, or between centers of adjacent pixels"@en ;
    skos:inScheme def:scheme ;
    skos:prefLabel "grid spacing"@en .

<http://www.opengis.net/def/uom/OGC/1.0/degree> a skos:Concept ;
    rdfs:label "degree"@en ;
    dc:creator "Arliss Whiteside" ;
    dc:date "2010-03-23" ;
    dc:source "OGC 07-092r3 Table 9"^^xsd:string ;
    dcterms:created "2010-03-23" ;
    dcterms:modified "2012-02-14"^^xsd:date ;
    policy:status status:valid ;
    rdfs:seeAlso <http://www.opengis.net/doc/urn-def/1.3#Table-9> ;
    owl:sameAs <http://www.opengis.net/def/uom/UCUM/0/deg>,
        <http://www.opengis.net/def/uom/ogc/1.0/degree> ;
    skos:definition "Angular degree"@en ;
    skos:inScheme def:scheme ;
    skos:prefLabel "degree"@en .

<http://www.opengis.net/def/uom/OGC/1.0/metre> a skos:Concept ;
    rdfs:label "metre"@en,
        "meter"@en-us ;
    dc:creator "Arliss Whiteside" ;
    dc:date "2010-03-23" ;
    dc:source "OGC 07-092r3 Table 9"^^xsd:string ;
    dcterms:created "2010-03-23" ;
    dcterms:modified "2012-02-14"^^xsd:date ;
    policy:status status:valid ;
    rdfs:seeAlso <http://www.opengis.net/doc/urn-def/1.3#Table-9> ;
    owl:sameAs <http://www.opengis.net/def/uom/UCUM/0/m>,
        <http://www.opengis.net/def/uom/ogc/1.0/metre> ;
    skos:definition "The metre is the length of the path travelled by light in vacuum during a time interval of 1/299 792 458 of a second."@en ;
    skos:inScheme def:scheme ;
    skos:prefLabel "metre"@en,
        "meter"@en-us .

<http://www.opengis.net/def/uom/OGC/1.0/radian> a skos:Concept ;
    rdfs:label "radian"@en ;
    dc:creator "Arliss Whiteside" ;
    dc:date "2010-03-23" ;
    dc:source "OGC 07-092r3 Table 9"^^xsd:string ;
    dcterms:created "2010-03-23" ;
    dcterms:modified "2012-02-14"^^xsd:date ;
    policy:status status:valid ;
    rdfs:seeAlso <http://www.opengis.net/doc/urn-def/1.3#Table-9> ;
    owl:sameAs <http://www.opengis.net/def/uom/UCUM/0/radian>,
        <http://www.opengis.net/def/uom/ogc/1.0/radian> ;
    skos:definition "Angular radian"@en ;
    skos:inScheme def:scheme ;
    skos:prefLabel "radian"@en .

<http://www.opengis.net/def/uom/OGC/1.0/unity> a skos:Concept ;
    rdfs:label "unity"@en ;
    dc:creator "Arliss Whiteside" ;
    dc:date "2010-03-23" ;
    dc:source "OGC 07-092r3 Table 9"^^xsd:string ;
    dcterms:created "2010-03-23" ;
    dcterms:modified "2012-02-14"^^xsd:date ;
    policy:status status:valid ;
    rdfs:seeAlso <http://www.opengis.net/doc/urn-def/1.3#Table-9> ;
    owl:sameAs <http://www.opengis.net/def/uom/ogc/1.0/unity> ;
    skos:definition "unitless ratio of two quantities with the same units"@en ;
    skos:inScheme def:scheme ;
    skos:prefLabel "unity"@en .

<http://www.opengis.net/def/uom/SI/> a skos:Collection ;
    rdfs:label "SI units of measure"^^xsd:string ;
    rdfs:seeAlso <http://www.bipm.org/en/si/> ;
    owl:sameAs <http://www.opengis.net/def/uom/si/> ;
    skos:member <http://www.opengis.net/def/uom/SI/ampere>,
        <http://www.opengis.net/def/uom/SI/candela>,
        <http://www.opengis.net/def/uom/SI/kelvin>,
        <http://www.opengis.net/def/uom/SI/kilogram>,
        <http://www.opengis.net/def/uom/SI/metre>,
        <http://www.opengis.net/def/uom/SI/mole>,
        <http://www.opengis.net/def/uom/SI/second> .

<http://www.opengis.net/def/uom/UCUM/> a skos:Collection ;
    rdfs:label "UCUM Units of Measure" ;
    dcterms:created "2012-02-14"^^xsd:date ;
    owl:sameAs <http://www.opengis.net/def/uom/ucum/> ;
    skos:member <http://www.opengis.net/def/uom/UCUM/0/> .

<http://www.opengis.net/def/uom/UCUM/0/> a skos:Collection ;
    rdfs:label "UCUM Units of Measure 0" ;
    dcterms:created "2012-02-14"^^xsd:date ;
    rdfs:seeAlso <http://aurora.regenstrief.org/~ucum/ucum.html> ;
    owl:sameAs <http://www.opengis.net/def/uom/ucum/0/> .

