@prefix : <http://www.opengis.net/ont/geosparql#> .
@prefix conf10core: <http://www.opengis.net/spec/geosparql/1.0/conf/core/> .
@prefix conf10gtx: <http://www.opengis.net/spec/geosparql/1.0/conf/geometry-topology-extension/> .
@prefix conf10gx: <http://www.opengis.net/spec/geosparql/1.0/conf/geometry-extension/> .
@prefix conf10qre: <http://www.opengis.net/spec/geosparql/1.0/conf/query-rewrite-extension/> .
@prefix conf10ree: <http://www.opengis.net/spec/geosparql/1.0/conf/rdfs-entailment-extension/> .
@prefix conf10tve: <http://www.opengis.net/spec/geosparql/1.0/conf/topology-extension/> .
@prefix conf11core: <http://www.opengis.net/spec/geosparql/1.1/conf/core/> .
@prefix conf11gx: <http://www.opengis.net/spec/geosparql/1.1/conf/geometry-extension/> .
@prefix conf11qre: <http://www.opengis.net/spec/geosparql/1.1/conf/query-rewrite-extension/> .
@prefix confs10: <http://www.opengis.net/spec/geosparql/1.0/conf/> .
@prefix confs11: <http://www.opengis.net/spec/geosparql/1.1/conf/> .
@prefix dc: <http://purl.org/dc/elements/1.1/> .
@prefix dcterms: <http://purl.org/dc/terms/> .
@prefix ent: <http://www.w3.org/ns/entailment/> .
@prefix fno: <https://w3id.org/function/ontology#> .
@prefix funcs: <http://www.opengis.net/def/function/geosparql/> .
@prefix ogc: <http://www.opengis.net/> .
@prefix owl: <http://www.w3.org/2002/07/owl#> .
@prefix policy: <http://www.opengis.net/def/metamodel/ogc-na/> .
@prefix prof: <http://www.w3.org/ns/dx/prof/> .
@prefix prov1: <http://www.w3.org/ns/prov-o/> .
@prefix rdf: <http://www.w3.org/1999/02/22-rdf-syntax-ns#> .
@prefix rdfs: <http://www.w3.org/2000/01/rdf-schema#> .
@prefix reqs10: <http://www.opengis.net/spec/geosparql/1.0/req/> .
@prefix reqs10core: <http://www.opengis.net/spec/geosparql/1.0/req/core/> .
@prefix reqs10gtx: <http://www.opengis.net/spec/geosparql/1.0/req/geometry-topology-extension/> .
@prefix reqs10gx: <http://www.opengis.net/spec/geosparql/1.0/req/geometry-extension/> .
@prefix reqs10qre: <http://www.opengis.net/spec/geosparql/1.0/req/query-rewrite-extension/> .
@prefix reqs10ree: <http://www.opengis.net/spec/geosparql/1.0/req/rdfs-entailment-extension/> .
@prefix reqs10tve: <http://www.opengis.net/spec/geosparql/1.0/req/topology-extension/> .
@prefix reqs11core: <http://www.opengis.net/spec/geosparql/1.1/req/core/> .
@prefix reqs11gx: <http://www.opengis.net/spec/geosparql/1.1/req/geometry-extension/> .
@prefix role: <http://www.w3.org/ns/dx/prof/role/> .
@prefix rules: <http://www.opengis.net/def/rule/geosparql/> .
@prefix sd: <http://www.w3.org/ns/sparql-service-description#> .
@prefix sdo: <https://schema.org/> .
@prefix sf: <http://www.opengis.net/ont/sf#> .
@prefix skos: <http://www.w3.org/2004/02/skos/core#> .
@prefix spec: <http://www.opengis.net/def/spec-element/> .
@prefix spec11: <http://www.opengis.net/spec/geosparql/1.1/specification.html#> .
@prefix status: <http://www.opengis.net/def/status/> .
@prefix xsd: <http://www.w3.org/2001/XMLSchema#> .

:Feature a rdfs:Class,
        owl:Class ;
    rdfs:label "Feature"@en ;
    dc:contributor "Matthew Perry" ;
    dc:creator "OGC GeoSPARQL 1.0 Standard Working Group" ;
    dc:date "2011-06-16"^^xsd:date ;
    dc:description """
      This class represents the top-level feature type. This class is
      equivalent to GFI_Feature defined in ISO 19156:2011, and it is
      superclass of all feature types.
    """@en ;
    rdfs:comment """
      This class represents the top-level feature type. This class is
      equivalent to GFI_Feature defined in ISO 19156:2011, and it is
      superclass of all feature types.
    """@en ;
    rdfs:isDefinedBy <http://www.opengis.net/ont/geosparql>,
        :,
        <http://www.opengis.net/spec/geosparql/1.0>,
        reqs10core:feature-class,
        reqs11core:feature-class ;
    rdfs:subClassOf :SpatialObject ;
    owl:disjointWith :Geometry ;
    skos:definition """
      This class represents the top-level feature type. This class is
      equivalent to GFI_Feature defined in ISO 19156:2011, and it is
      superclass of all feature types.
    """@en,
        "A discrete spatial phenomenon in a universe of discourse."@en ;
    skos:example spec11:B.1.1.2.1,
        spec11:B.1.1.2.2,
        spec11:B.1.1.2.3,
        spec11:B.1.1.2.4,
        spec11:B.1.1.2.5,
        spec11:B.1.1.2.6,
        spec11:B.1.1.2.7,
        spec11:B.1.1.2.8,
        spec11:B.1.1.2.9,
        spec11:B.1.1.3.2,
        spec11:B.1.1.3.3,
        spec11:B.1.2.2,
        spec11:B.1.2.3,
        spec11:B.1.2.4 ;
    skos:note "A Feature represents a uniquely identifiable phenomenon, for example a river or an apple. While such phenomena (and therefore the Features used to represent them) are bounded, their boundaries may be crisp (e.g., the declared boundaries of a state), vague (e.g., the delineation of a valley versus its neighboring mountains), and change with time (e.g., a storm front). While discrete in nature, Features may be created from continuous observations, such as an isochrone that determines the region that can be reached by ambulance within 5 minutes."@en ;
    skos:prefLabel "Feature"@en .

:FeatureCollection a rdfs:Class,
        owl:Class ;
    rdfs:isDefinedBy :,
        reqs11core:feature-collection-class ;
    rdfs:subClassOf [ a owl:Restriction ;
            owl:allValuesFrom :Feature ;
            owl:onProperty rdfs:member ],
        :SpatialObjectCollection ;
    skos:definition "A collection of individual Features."@en ;
    skos:example spec11:B.1.1.6 ;
    skos:prefLabel "Feature Collection"@en .

:Geometry a rdfs:Class,
        owl:Class ;
    rdfs:label "Geometry"@en ;
    dc:contributor "Matthew Perry" ;
    dc:creator "OGC GeoSPARQL 1.0 Standard Working Group" ;
    dc:date "2011-06-16"^^xsd:date ;
    dc:description """
      The class represents the top-level geometry type. This class is
      equivalent to the UML class GM_Object defined in ISO 19107, and
      it is superclass of all geometry types.
    """@en ;
    rdfs:comment """
      The class represents the top-level geometry type. This class is
      equivalent to the UML class GM_Object defined in ISO 19107, and
      it is superclass of all geometry types.
    """@en ;
    rdfs:isDefinedBy <http://www.opengis.net/ont/geosparql>,
        :,
        <http://www.opengis.net/spec/geosparql/1.0>,
        reqs10gx:geometry-class,
        reqs11gx:geometry-class ;
    rdfs:subClassOf :SpatialObject ;
    skos:definition """
      The class represents the top-level geometry type. This class is
      equivalent to the UML class GM_Object defined in ISO 19107, and
      it is superclass of all geometry types.
    """@en,
        "A coherent set of direct positions in space. The positions are held within a Spatial Reference System (SRS)."@en ;
    skos:example spec11:B.1.1.2.2,
        spec11:B.1.1.2.3,
        spec11:B.1.1.2.4,
        spec11:B.1.1.2.5,
        spec11:B.1.1.2.6,
        spec11:B.1.1.2.8,
        spec11:B.1.1.3.1,
        spec11:B.1.1.3.2,
        spec11:B.1.1.3.3,
        spec11:B.1.2.2,
        spec11:B.1.2.3,
        spec11:B.1.2.4 ;
    skos:note "Geometry can be used as a representation of the shape, extent or location of a Feature and may exist as a self-contained entity."@en ;
    skos:prefLabel "Geometry"@en .

:GeometryCollection a rdfs:Class,
        owl:Class ;
    rdfs:isDefinedBy :,
        reqs11core:geometry-collection-class ;
    rdfs:subClassOf [ a owl:Restriction ;
            owl:allValuesFrom :Geometry ;
            owl:onProperty rdfs:member ],
        :SpatialObjectCollection ;
    skos:definition "A collection of individual Geometries."@en ;
    skos:example spec11:B.1.1.7 ;
    skos:prefLabel "Geometry Collection"@en .

:SpatialObject a rdfs:Class,
        owl:Class ;
    rdfs:label "SpatialObject"@en ;
    dc:contributor "Matthew Perry" ;
    dc:creator "OGC GeoSPARQL 1.0 Standard Working Group" ;
    dc:date "2011-06-16"^^xsd:date ;
    dc:description """
      The class spatial-object represents everything that can have
      a spatial representation. It is superclass of feature and geometry.
    """@en ;
    rdfs:comment """
      The class spatial-object represents everything that can have
      a spatial representation. It is superclass of feature and geometry.
    """@en ;
    rdfs:isDefinedBy <http://www.opengis.net/ont/geosparql>,
        :,
        <http://www.opengis.net/spec/geosparql/1.0>,
        reqs10core:spatial-object-class,
        reqs11core:spatial-object-class ;
    skos:definition """
      The class spatial-object represents everything that can have
      a spatial representation. It is superclass of feature and geometry.
    """@en,
        "Anything spatial (being or having a shape, position or an extent)."@en ;
    skos:example spec11:B.1.1.1.1,
        spec11:B.1.1.1.2 ;
    skos:note "Subclasses of this class are expected to be used for instance data."@en ;
    skos:prefLabel "Spatial Object"@en,
        "SpatialObject"@en .

:SpatialObjectCollection a rdfs:Class,
        owl:Class ;
    rdfs:isDefinedBy :,
        reqs11core:spatial-object-collection-class ;
    rdfs:subClassOf [ a owl:Restriction ;
            owl:allValuesFrom :SpatialObject ;
            owl:onProperty rdfs:member ],
        rdfs:Container ;
    skos:definition "A collection of individual Spatial Objects."@en ;
    skos:note "This is the superclass of Feature Collection and Geometry Collection."@en ;
    skos:prefLabel "Spatial Object Collection"@en .

sf:Curve a rdfs:Class,
        owl:Class ;
    rdfs:label "Curve"@en ;
    rdfs:comment """A Curve is a 1-dimensional geometric object usually stored as a sequence of Points, with the subtype of Curve specifying the form of the interpolation between Points. This specification defines only one subclass of Curve, LineString, which uses linear interpolation between Points.

A Curve is a 1-dimensional geometric object that is the homeomorphic image of a real, closed, interval.

A Curve is simple if it does not pass through the same Point twice with the possible exception of the two end
points.

A Curve is closed if its start Point is equal to its end Point.

The boundary of a closed Curve is empty.

A Curve that is simple and closed is a Ring.

The boundary of a non-closed Curve consists of its two end Points.

A Curve is defined as topologically closed, that is, it contains its endpoints f(a) and f(b)."""@en ;
    rdfs:isDefinedBy <http://www.opengis.net/ont/sf> ;
    rdfs:subClassOf sf:Geometry ;
    skos:definition """A Curve is a 1-dimensional geometric object usually stored as a sequence of Points, with the subtype of Curve specifying the form of the interpolation between Points. This specification defines only one subclass of Curve, LineString, which uses linear interpolation between Points.

A Curve is a 1-dimensional geometric object that is the homeomorphic image of a real, closed, interval.

A Curve is simple if it does not pass through the same Point twice with the possible exception of the two end
points.

A Curve is closed if its start Point is equal to its end Point.

The boundary of a closed Curve is empty.

A Curve that is simple and closed is a Ring.

The boundary of a non-closed Curve consists of its two end Points.

A Curve is defined as topologically closed, that is, it contains its endpoints f(a) and f(b)."""@en ;
    skos:prefLabel "Curve"@en .

sf:Envelope a rdfs:Class,
        owl:Class ;
    rdfs:isDefinedBy <http://www.opengis.net/ont/sf> ;
    rdfs:subClassOf [ a owl:Restriction ;
            owl:cardinality "1"^^xsd:nonNegativeInteger ;
            owl:onProperty sf:maximum ],
        [ a owl:Restriction ;
            owl:cardinality "1"^^xsd:nonNegativeInteger ;
            owl:onProperty sf:minimum ],
        sf:Polygon ;
    skos:definition """Shape defined by the corner points of the bounding box of a geometry.
The corner points may be in any dimension (usually 2D or 3D) but the two corners must have the same dimension."""@en ;
    skos:prefLabel "Envelope or Bounding Box"@en .

sf:Geometry a rdfs:Class,
        owl:Class ;
    rdfs:label "Geometry"@en ;
    rdfs:comment """Geometry is the root class of the hierarchy.

The instantiable subclasses of Geometry are restricted to 0, 1 and 2-dimensional geometric objects that exist in 2, 3 or 4-dimensional coordinate space (R2, R3 or R4). Geometry values in R2 have points with coordinate values for x and y. Geometry values in R3 have points with coordinate values for x, y and z or for x, y and m. Geometry values in R4 have points with coordinate values for x, y, z and m.

The interpretation of the coordinates is subject to the coordinate reference systems associated to the point. All coordinates within a geometry object should be in the same coordinate reference systems. Each coordinate shall be unambiguously associated to a coordinate reference system either directly or through its containing geometry. The z coordinate of a point is typically, but not necessarily, represents altitude or elevation. The m coordinate represents a measurement.

All Geometry classes described in this specification are defined so that instances of Geometry are topologically closed, i.e. all represented geometries include their boundary as point sets. This does not affect their representation, and open version of the same classes may be used in other circumstances, such as topological representations."""@en ;
    rdfs:isDefinedBy <http://www.opengis.net/ont/sf> ;
    rdfs:subClassOf :Geometry ;
    skos:definition """Geometry is the root class of the hierarchy.

The instantiable subclasses of Geometry are restricted to 0, 1 and 2-dimensional geometric objects that exist in 2, 3 or 4-dimensional coordinate space (R2, R3 or R4). Geometry values in R2 have points with coordinate values for x and y. Geometry values in R3 have points with coordinate values for x, y and z or for x, y and m. Geometry values in R4 have points with coordinate values for x, y, z and m.

The interpretation of the coordinates is subject to the coordinate reference systems associated to the point. All coordinates within a geometry object should be in the same coordinate reference systems. Each coordinate shall be unambiguously associated to a coordinate reference system either directly or through its containing geometry. The z coordinate of a point is typically, but not necessarily, represents altitude or elevation. The m coordinate represents a measurement.

All Geometry classes described in this specification are defined so that instances of Geometry are topologically closed, i.e. all represented geometries include their boundary as point sets. This does not affect their representation, and open versions of the same classes may be used in other circumstances, such as topological representations."""@en ;
    skos:prefLabel "Geometry"@en .

sf:GeometryCollection a rdfs:Class,
        owl:Class ;
    rdfs:label "Geometry Collection"@en ;
    rdfs:comment """A GeometryCollection is a geometric object that is a collection of some number of geometric objects.

All the elements in a GeometryCollection shall be in the same Spatial Reference System. This is also the Spatial Reference System for the GeometryCollection.
GeometryCollection places no other constraints on its elements. Subclasses of GeometryCollection may restrict membership based on dimension and may also place other constraints on the degree of spatial overlap between elements."""@en ;
    rdfs:isDefinedBy <http://www.opengis.net/ont/sf> ;
    rdfs:subClassOf sf:Geometry ;
    skos:definition """A GeometryCollection is a geometric object that is a collection of some number of geometric objects.

All the elements in a GeometryCollection shall be in the same Spatial Reference System. This is also the Spatial Reference System for the GeometryCollection.
GeometryCollection places no other constraints on its elements. Subclasses of GeometryCollection may restrict membership based on dimension and may also place other constraints on the degree of spatial overlap between elements."""@en ;
    skos:prefLabel "Geometry Collection"@en .

sf:Line a rdfs:Class,
        owl:Class ;
    rdfs:label "Line"@en ;
    rdfs:comment "A Line is a LineString with exactly 2 Points."@en ;
    rdfs:isDefinedBy <http://www.opengis.net/ont/sf> ;
    rdfs:subClassOf sf:LineString ;
    skos:definition "A Line is a LineString with exactly 2 Points."@en ;
    skos:prefLabel "Line"@en .

sf:LineString a rdfs:Class,
        owl:Class ;
    rdfs:label "Line String"@en ;
    rdfs:comment "A LineString is a Curve with linear interpolation between Points. Each consecutive pair of Points defines a Line segment."@en ;
    rdfs:isDefinedBy <http://www.opengis.net/ont/sf> ;
    rdfs:subClassOf sf:Curve ;
    skos:definition "A LineString is a Curve with linear interpolation between Points. Each consecutive pair of Points defines a Line segment."@en ;
    skos:prefLabel "Line String"@en .

sf:LinearRing a rdfs:Class,
        owl:Class ;
    rdfs:label "Linear Ring"@en ;
    rdfs:comment "A LinearRing is a LineString that is both closed and simple."@en ;
    rdfs:isDefinedBy <http://www.opengis.net/ont/sf> ;
    rdfs:subClassOf sf:LineString ;
    skos:definition "A LinearRing is a LineString that is both closed and simple."@en ;
    skos:prefLabel "Linear Ring"@en .

sf:MultiCurve a rdfs:Class,
        owl:Class ;
    rdfs:label "Multi Curve"@en ;
    rdfs:comment """A MultiCurve is a 1-dimensional GeometryCollection whose elements are Curves.

A MultiCurve defines a set of methods for its subclasses and is included for reasons of extensibility.

A MultiCurve is simple if and only if all of its elements are simple and the only intersections between any two elements occur at Points that are on the boundaries of both elements.

The boundary of a MultiCurve is obtained by applying the mod 2 union rule: A Point is in the boundary of a MultiCurve if it is in the boundaries of an odd number of elements of the MultiCurve.

A MultiCurve is closed if all of its elements are closed. The boundary of a closed MultiCurve is always empty.

A MultiCurve is defined as topologically closed."""@en ;
    rdfs:isDefinedBy <http://www.opengis.net/ont/sf> ;
    rdfs:subClassOf sf:GeometryCollection ;
    skos:definition """A MultiCurve is a 1-dimensional GeometryCollection whose elements are Curves.

A MultiCurve defines a set of methods for its subclasses and is included for reasons of extensibility.

A MultiCurve is simple if and only if all of its elements are simple and the only intersections between any two elements occur at Points that are on the boundaries of both elements.

The boundary of a MultiCurve is obtained by applying the mod 2 union rule: A Point is in the boundary of a MultiCurve if it is in the boundaries of an odd number of elements of the MultiCurve.

A MultiCurve is closed if all of its elements are closed. The boundary of a closed MultiCurve is always empty.

A MultiCurve is defined as topologically closed."""@en ;
    skos:prefLabel "Multi Curve"@en .

sf:MultiLineString a rdfs:Class,
        owl:Class ;
    rdfs:label "Multi Line String"@en ;
    rdfs:comment "A MultiLineString is a MultiCurve whose elements are LineStrings."@en ;
    rdfs:isDefinedBy <http://www.opengis.net/ont/sf> ;
    rdfs:subClassOf sf:MultiCurve ;
    skos:definition "A MultiLineString is a MultiCurve whose elements are LineStrings."@en ;
    skos:prefLabel "Multi Line String"@en .

sf:MultiPoint a rdfs:Class,
        owl:Class ;
    rdfs:label "Multi Point"@en ;
    rdfs:comment """A MultiPoint is a 0-dimensional GeometryCollection. The elements of a MultiPoint are restricted to Points. ThePoints are not connected or ordered in any semantically important way.

A MultiPoint is simple if no two Points in the MultiPoint are equal (have identical coordinate values in X and Y).

Every MultiPoint is spatially equal to a simple Multipoint.

The boundary of a MultiPoint is the empty set."""@en ;
    rdfs:isDefinedBy <http://www.opengis.net/ont/sf> ;
    rdfs:subClassOf sf:GeometryCollection ;
    skos:definition """A MultiPoint is a 0-dimensional GeometryCollection. The elements of a MultiPoint are restricted to Points. ThePoints are not connected or ordered in any semantically important way.

A MultiPoint is simple if no two Points in the MultiPoint are equal (have identical coordinate values in X and Y).

Every MultiPoint is spatially equal to a simple Multipoint.

The boundary of a MultiPoint is the empty set."""@en ;
    skos:prefLabel "Multi Point"@en .

sf:MultiPolygon a rdfs:Class,
        owl:Class ;
    rdfs:label "Multi Polygon"@en ;
    rdfs:comment """A MultiPolygon is a MultiSurface whose elements are Polygons.

The assertions for MultiPolygons are as follows.

a) The interiors of 2 Polygons that are elements of a MultiPolygon may not intersect.
b) The boundaries of any 2 Polygons that are elements of a MultiPolygon may not cross and may touch at only a finite number of Points.
c) A MultiPolygon is defined as topologically closed.
d) A MultiPolygon may not have cut lines, spikes or punctures, a MultiPolygon is a regular closed Point set,
e) The interior of a MultiPolygon with more than 1 Polygon is not connected; the number of connected components of the interior of a MultiPolygon is equal to the number of Polygons in the MultiPolygon. 

The boundary of a MultiPolygon is a set of closed Curves (LineStrings) corresponding to the boundaries of its element Polygons. Each Curve in the boundary of the MultiPolygon is in the boundary of exactly 1 element Polygon, and every Curve in the boundary of an element Polygon is in the boundary of the MultiPolygon."""@en ;
    rdfs:isDefinedBy <http://www.opengis.net/ont/sf> ;
    rdfs:subClassOf sf:MultiSurface ;
    skos:definition """A MultiPolygon is a MultiSurface whose elements are Polygons.

The assertions for MultiPolygons are as follows.

a) The interiors of 2 Polygons that are elements of a MultiPolygon may not intersect.
b) The boundaries of any 2 Polygons that are elements of a MultiPolygon may not cross and may touch at only a finite number of Points.
c) A MultiPolygon is defined as topologically closed.
d) A MultiPolygon may not have cut lines, spikes or punctures, a MultiPolygon is a regular closed Point set,
e) The interior of a MultiPolygon with more than 1 Polygon is not connected; the number of connected components of the interior of a MultiPolygon is equal to the number of Polygons in the MultiPolygon. 

The boundary of a MultiPolygon is a set of closed Curves (LineStrings) corresponding to the boundaries of its element Polygons. Each Curve in the boundary of the MultiPolygon is in the boundary of exactly 1 element Polygon, and every Curve in the boundary of an element Polygon is in the boundary of the MultiPolygon."""@en ;
    skos:prefLabel "Multi Polygon"@en .

sf:MultiSurface a rdfs:Class,
        owl:Class ;
    rdfs:label "Multi Surface"@en ;
    rdfs:comment """A MultiSurface is a 2-dimensional GeometryCollection whose elements are Surfaces, all using coordinates from the same coordinate reference system. The geometric interiors of any two Surfaces in a MultiSurface may not intersect in the full coordinate system. The boundaries of any two coplanar elements in a MultiSurface may intersect, at most, at a finite number of Points. If they were to meet along a curve, they could be merged into a single surface.

A MultiSurface may be used to represent heterogeneous surfaces collections of polygons and polyhedral surfaces. It defines a set of methods for its subclasses. The subclass of MultiSurface is MultiPolygon corresponding to a collection of Polygons only. Other collections shall use MultiSurface."""@en ;
    rdfs:isDefinedBy <http://www.opengis.net/ont/sf> ;
    rdfs:subClassOf sf:GeometryCollection ;
    skos:definition """A MultiSurface is a 2-dimensional GeometryCollection whose elements are Surfaces, all using coordinates from the same coordinate reference system. The geometric interiors of any two Surfaces in a MultiSurface may not intersect in the full coordinate system. The boundaries of any two coplanar elements in a MultiSurface may intersect, at most, at a finite number of Points. If they were to meet along a curve, they could be merged into a single surface.

A MultiSurface may be used to represent heterogeneous surfaces collections of polygons and polyhedral surfaces. It defines a set of methods for its subclasses. The subclass of MultiSurface is MultiPolygon corresponding to a collection of Polygons only. Other collections shall use MultiSurface."""@en ;
    skos:prefLabel "Multi Surface"@en .

sf:Point a rdfs:Class,
        owl:Class ;
    rdfs:label "Point"@en ;
    rdfs:comment """A Point is a 0-dimensional geometric object and represents a single location in coordinate space. 
A Point has an x-coordinate value, a y-coordinate value. If called for by the associated Spatial Reference System, it may also have coordinate values for z and m.
The boundary of a Point is the empty set."""@en ;
    rdfs:isDefinedBy <http://www.opengis.net/ont/sf> ;
    rdfs:subClassOf sf:Geometry ;
    skos:definition """A Point is a 0-dimensional geometric object and represents a single location in coordinate space. 
A Point has an x-coordinate value, a y-coordinate value. If called for by the associated Spatial Reference System, it may also have coordinate values for z and m.
The boundary of a Point is the empty set."""@en ;
    skos:prefLabel "Point"@en .

sf:Polygon a rdfs:Class,
        owl:Class ;
    rdfs:label "Polygon"@en ;
    rdfs:comment """A Polygon is a planar Surface defined by 1 exterior boundary and 0 or more interior boundaries. Each interior boundary defines a hole in the Polygon.
The exterior boundary LinearRing defines the top of the surface which is the side of the surface from which the exterior boundary appears to traverse the boundary in a counter clockwise direction. The interior LinearRings will have the opposite orientation, and appear as clockwise when viewed from the top,
The assertions for Polygons (the rules that define valid Polygons) are as follows:

a) Polygons are topologically closed;
b) The boundary of a Polygon consists of a set of LinearRings that make up its exterior and interior boundaries;
c) No two Rings in the boundary cross and the Rings in the boundary of a Polygon may intersect at a Point but only as a tangent.
d) A Polygon may not have cut lines, spikes or punctures.
e) The interior of every Polygon is a connected point set;
f) The exterior of a Polygon with 1 or more holes is not connected. Each hole defines a connected component of the exterior."""@en ;
    rdfs:isDefinedBy <http://www.opengis.net/ont/sf> ;
    rdfs:subClassOf sf:Surface ;
    skos:definition """A Polygon is a planar Surface defined by 1 exterior boundary and 0 or more interior boundaries. Each interior boundary defines a hole in the Polygon.
The exterior boundary LinearRing defines the top of the surface which is the side of the surface from which the exterior boundary appears to traverse the boundary in a counter clockwise direction. The interior LinearRings will have the opposite orientation, and appear as clockwise when viewed from the top,
The assertions for Polygons (the rules that define valid Polygons) are as follows:

a) Polygons are topologically closed;
b) The boundary of a Polygon consists of a set of LinearRings that make up its exterior and interior boundaries;
c) No two Rings in the boundary cross and the Rings in the boundary of a Polygon may intersect at a Point but only as a tangent.
d) A Polygon may not have cut lines, spikes or punctures.
e) The interior of every Polygon is a connected point set;
f) The exterior of a Polygon with 1 or more holes is not connected. Each hole defines a connected component of the exterior."""@en ;
    skos:prefLabel "Polygon"@en .

sf:PolyhedralSurface a rdfs:Class,
        owl:Class ;
    rdfs:label "Polyhedral Surface"@en ;
    rdfs:comment """A PolyhedralSurface is a contiguous collection of polygons, which share common boundary segments. For each pair of polygons that touch, the common boundary shall be expressible as a finite collection of LineStrings. Each such LineString shall be part of the boundary of at most 2 Polygon patches. 

For any two polygons that share a common boundary, the top of the polygon shall be consistent. This means that when two LinearRings from these two Polygons traverse the common boundary segment, they do so in opposite directions. Since the Polyhedral surface is contiguous, all polygons will be thus consistently oriented. This means that a non-oriented surface (such as Mbius band) shall not have single surface representations. They may be represented by a MultiSurface.

If each such LineString is the boundary of exactly 2 Polygon patches, then the PolyhedralSurface is a simple, closed polyhedron and is topologically isomorphic to the surface of a sphere. By the Jordan Surface Theorem (Jordans Theorem for 2-spheres), such polyhedrons enclose a solid topologically isomorphic to the interior of a sphere; the ball. In this case, the top of the surface will either point inward or outward of the enclosed finite solid. If outward, the surface is the exterior boundary of the enclosed surface. If inward, the surface is the interior of the infinite complement of the enclosed solid. A Ball with some number of voids (holes) inside can thus be presented as one exterior boundary shell, and some number in interior boundary shells."""@en ;
    rdfs:isDefinedBy <http://www.opengis.net/ont/sf> ;
    rdfs:subClassOf sf:Surface ;
    skos:definition """A PolyhedralSurface is a contiguous collection of polygons, which share common boundary segments. For each pair of polygons that touch, the common boundary shall be expressible as a finite collection of LineStrings. Each such LineString shall be part of the boundary of at most 2 Polygon patches. 

For any two polygons that share a common boundary, the top of the polygon shall be consistent. This means that when two LinearRings from these two Polygons traverse the common boundary segment, they do so in opposite directions. Since the Polyhedral surface is contiguous, all polygons will be thus consistently oriented. This means that a non-oriented surface (such as Mbius band) shall not have single surface representations. They may be represented by a MultiSurface.

If each such LineString is the boundary of exactly 2 Polygon patches, then the PolyhedralSurface is a simple, closed polyhedron and is topologically isomorphic to the surface of a sphere. By the Jordan Surface Theorem (Jordans Theorem for 2-spheres), such polyhedrons enclose a solid topologically isomorphic to the interior of a sphere; the ball. In this case, the top of the surface will either point inward or outward of the enclosed finite solid. If outward, the surface is the exterior boundary of the enclosed surface. If inward, the surface is the interior of the infinite complement of the enclosed solid. A Ball with some number of voids (holes) inside can thus be presented as one exterior boundary shell, and some number in interior boundary shells."""@en ;
    skos:prefLabel "Polyhedral Surface"@en .

sf:Surface a rdfs:Class,
        owl:Class ;
    rdfs:label "Surface"@en ;
    rdfs:comment """A Surface is a 2-dimensional geometric object.
A simple Surface may consists of a single patch that is associated with one exterior boundary and 0 or more interior boundaries. A single such Surface patch in 3-dimensional space is isometric to planar Surfaces, by a simple affine rotation matrix that rotates the patch onto the plane z = 0. If the patch is not vertical, the projection onto the same plane is an isomorphism, and can be represented as a linear transformation, i.e. an affine.

Polyhedral Surfaces are formed by stitching together such simple Surfaces patches along their common boundaries. Such polyhedral Surfaces in a 3-dimensional space may not be planar as a whole, depending on the orientation of their planar normals. If all the patches are in alignment (their normals are parallel), then the whole stitched polyhedral surface is co-planar and can be represented as a single patch if it is connected.

The boundary of a simple Surface is the set of closed Curves corresponding to its exterior and interior boundaries.

A Polygon is a simple Surface that is planar. A PolyhedralSurface is a simple surface, consisting of some number of Polygon patches or facets. If a PolyhedralSurface is closed, then it bounds a solid. A MultiSurface containing a set of closed PolyhedralSurfaces can be used to represent a Solid object with holes."""@en ;
    rdfs:isDefinedBy <http://www.opengis.net/ont/sf> ;
    rdfs:subClassOf sf:Geometry ;
    skos:definition """A Surface is a 2-dimensional geometric object.
A simple Surface may consists of a single patch that is associated with one exterior boundary and 0 or more interior boundaries. A single such Surface patch in 3-dimensional space is isometric to planar Surfaces, by a simple affine rotation matrix that rotates the patch onto the plane z = 0. If the patch is not vertical, the projection onto the same plane is an isomorphism, and can be represented as a linear transformation, i.e. an affine.

Polyhedral Surfaces are formed by stitching together such simple Surfaces patches along their common boundaries. Such polyhedral Surfaces in a 3-dimensional space may not be planar as a whole, depending on the orientation of their planar normals. If all the patches are in alignment (their normals are parallel), then the whole stitched polyhedral surface is co-planar and can be represented as a single patch if it is connected.

The boundary of a simple Surface is the set of closed Curves corresponding to its exterior and interior boundaries.

A Polygon is a simple Surface that is planar. A PolyhedralSurface is a simple surface, consisting of some number of Polygon patches or facets. If a PolyhedralSurface is closed, then it bounds a solid. A MultiSurface containing a set of closed PolyhedralSurfaces can be used to represent a Solid object with holes."""@en ;
    skos:prefLabel "Surface"@en .

sf:TIN a rdfs:Class,
        owl:Class ;
    rdfs:label "Triangulated Irregular Network"@en ;
    rdfs:comment "A TIN (triangulated irregular network) is a PolyhedralSurface consisting only of Triangle patches."@en ;
    rdfs:isDefinedBy <http://www.opengis.net/ont/sf> ;
    rdfs:subClassOf sf:PolyhedralSurface ;
    skos:definition "A TIN (triangulated irregular network) is a PolyhedralSurface consisting only of Triangle patches."@en ;
    skos:prefLabel "Triangulated Irregular Network"@en .

sf:Triangle a rdfs:Class,
        owl:Class ;
    rdfs:label "Triangle"@en ;
    rdfs:comment "A Triangle is a polygon with 3 distinct, non-collinear vertices and no interior boundary."@en ;
    rdfs:isDefinedBy <http://www.opengis.net/ont/sf> ;
    rdfs:subClassOf sf:Polygon ;
    skos:definition "A Triangle is a polygon with 3 distinct, non-collinear vertices and no interior boundary."@en ;
    skos:prefLabel "Triangle"@en .

dc:contributor a owl:AnnotationProperty ;
    rdfs:label "Contributor"@en ;
    dcterms:description "Examples of a Contributor include a person, an organization, or a service. Typically, the name of a Contributor should be used to indicate the entity."@en ;
    dcterms:hasVersion <http://dublincore.org/usage/terms/history/#contributor-006> ;
    dcterms:issued "1999-07-02"^^xsd:date ;
    dcterms:modified "2008-01-14"^^xsd:date ;
    rdfs:comment "An entity responsible for making contributions to the resource."@en ;
    rdfs:isDefinedBy dc: ;
    skos:note "A second property with the same name as this property has been declared in the dcterms: namespace (http://purl.org/dc/terms/).  See the Introduction to the document \"DCMI Metadata Terms\" (http://dublincore.org/documents/dcmi-terms/) for an explanation."@en .

dc:coverage rdfs:label "Coverage"@en ;
    dcterms:description "Spatial topic and spatial applicability may be a named place or a location specified by its geographic coordinates. Temporal topic may be a named period, date, or date range. A jurisdiction may be a named administrative entity or a geographic place to which the resource applies. Recommended best practice is to use a controlled vocabulary such as the Thesaurus of Geographic Names [TGN]. Where appropriate, named places or time periods can be used in preference to numeric identifiers such as sets of coordinates or date ranges."@en ;
    dcterms:hasVersion <http://dublincore.org/usage/terms/history/#coverage-006> ;
    dcterms:issued "1999-07-02"^^xsd:date ;
    dcterms:modified "2008-01-14"^^xsd:date ;
    rdfs:comment "The spatial or temporal topic of the resource, the spatial applicability of the resource, or the jurisdiction under which the resource is relevant."@en ;
    rdfs:isDefinedBy dc: ;
    skos:note "A second property with the same name as this property has been declared in the dcterms: namespace (http://purl.org/dc/terms/).  See the Introduction to the document \"DCMI Metadata Terms\" (http://dublincore.org/documents/dcmi-terms/) for an explanation."@en .

dc:creator a owl:AnnotationProperty ;
    rdfs:label "Creator"@en ;
    dcterms:description "Examples of a Creator include a person, an organization, or a service. Typically, the name of a Creator should be used to indicate the entity."@en ;
    dcterms:hasVersion <http://dublincore.org/usage/terms/history/#creator-006> ;
    dcterms:issued "1999-07-02"^^xsd:date ;
    dcterms:modified "2008-01-14"^^xsd:date ;
    rdfs:comment "An entity primarily responsible for making the resource."@en ;
    rdfs:isDefinedBy dc: ;
    skos:note "A second property with the same name as this property has been declared in the dcterms: namespace (http://purl.org/dc/terms/).  See the Introduction to the document \"DCMI Metadata Terms\" (http://dublincore.org/documents/dcmi-terms/) for an explanation."@en .

dc:date a owl:AnnotationProperty ;
    rdfs:label "Date"@en ;
    dcterms:description "Date may be used to express temporal information at any level of granularity.  Recommended best practice is to use an encoding scheme, such as the W3CDTF profile of ISO 8601 [W3CDTF]."@en ;
    dcterms:hasVersion <http://dublincore.org/usage/terms/history/#date-006> ;
    dcterms:issued "1999-07-02"^^xsd:date ;
    dcterms:modified "2008-01-14"^^xsd:date ;
    rdfs:comment "A point or period of time associated with an event in the lifecycle of the resource."@en ;
    rdfs:isDefinedBy dc: ;
    skos:note "A second property with the same name as this property has been declared in the dcterms: namespace (http://purl.org/dc/terms/).  See the Introduction to the document \"DCMI Metadata Terms\" (http://dublincore.org/documents/dcmi-terms/) for an explanation."@en .

dc:description a owl:AnnotationProperty ;
    rdfs:label "Description"@en ;
    dcterms:description "Description may include but is not limited to: an abstract, a table of contents, a graphical representation, or a free-text account of the resource."@en ;
    dcterms:hasVersion <http://dublincore.org/usage/terms/history/#description-006> ;
    dcterms:issued "1999-07-02"^^xsd:date ;
    dcterms:modified "2008-01-14"^^xsd:date ;
    rdfs:comment "An account of the resource."@en ;
    rdfs:isDefinedBy dc: ;
    skos:note "A second property with the same name as this property has been declared in the dcterms: namespace (http://purl.org/dc/terms/).  See the Introduction to the document \"DCMI Metadata Terms\" (http://dublincore.org/documents/dcmi-terms/) for an explanation."@en .

dc:format rdfs:label "Format"@en ;
    dcterms:description "Examples of dimensions include size and duration. Recommended best practice is to use a controlled vocabulary such as the list of Internet Media Types [MIME]."@en ;
    dcterms:hasVersion <http://dublincore.org/usage/terms/history/#format-007> ;
    dcterms:issued "1999-07-02"^^xsd:date ;
    dcterms:modified "2008-01-14"^^xsd:date ;
    rdfs:comment "The file format, physical medium, or dimensions of the resource."@en ;
    rdfs:isDefinedBy dc: ;
    skos:note "A second property with the same name as this property has been declared in the dcterms: namespace (http://purl.org/dc/terms/).  See the Introduction to the document \"DCMI Metadata Terms\" (http://dublincore.org/documents/dcmi-terms/) for an explanation."@en .

dc:identifier rdfs:label "Identifier"@en ;
    dcterms:description "Recommended best practice is to identify the resource by means of a string conforming to a formal identification system. "@en ;
    dcterms:hasVersion <http://dublincore.org/usage/terms/history/#identifier-006> ;
    dcterms:issued "1999-07-02"^^xsd:date ;
    dcterms:modified "2008-01-14"^^xsd:date ;
    rdfs:comment "An unambiguous reference to the resource within a given context."@en ;
    rdfs:isDefinedBy dc: ;
    skos:note "A second property with the same name as this property has been declared in the dcterms: namespace (http://purl.org/dc/terms/).  See the Introduction to the document \"DCMI Metadata Terms\" (http://dublincore.org/documents/dcmi-terms/) for an explanation."@en .

dc:language rdfs:label "Language"@en ;
    dcterms:description "Recommended best practice is to use a controlled vocabulary such as RFC 4646 [RFC4646]."@en ;
    dcterms:hasVersion <http://dublincore.org/usage/terms/history/#language-007> ;
    dcterms:issued "1999-07-02"^^xsd:date ;
    dcterms:modified "2008-01-14"^^xsd:date ;
    rdfs:comment "A language of the resource."@en ;
    rdfs:isDefinedBy dc: ;
    rdfs:seeAlso <http://www.ietf.org/rfc/rfc4646.txt> ;
    skos:note "A second property with the same name as this property has been declared in the dcterms: namespace (http://purl.org/dc/terms/).  See the Introduction to the document \"DCMI Metadata Terms\" (http://dublincore.org/documents/dcmi-terms/) for an explanation."@en .

dc:publisher rdfs:label "Publisher"@en ;
    dcterms:description "Examples of a Publisher include a person, an organization, or a service. Typically, the name of a Publisher should be used to indicate the entity."@en ;
    dcterms:hasVersion <http://dublincore.org/usage/terms/history/#publisher-006> ;
    dcterms:issued "1999-07-02"^^xsd:date ;
    dcterms:modified "2008-01-14"^^xsd:date ;
    rdfs:comment "An entity responsible for making the resource available."@en ;
    rdfs:isDefinedBy dc: ;
    skos:note "A second property with the same name as this property has been declared in the dcterms: namespace (http://purl.org/dc/terms/).  See the Introduction to the document \"DCMI Metadata Terms\" (http://dublincore.org/documents/dcmi-terms/) for an explanation."@en .

dc:relation rdfs:label "Relation"@en ;
    dcterms:description "Recommended best practice is to identify the related resource by means of a string conforming to a formal identification system. "@en ;
    dcterms:hasVersion <http://dublincore.org/usage/terms/history/#relation-006> ;
    dcterms:issued "1999-07-02"^^xsd:date ;
    dcterms:modified "2008-01-14"^^xsd:date ;
    rdfs:comment "A related resource."@en ;
    rdfs:isDefinedBy dc: ;
    skos:note "A second property with the same name as this property has been declared in the dcterms: namespace (http://purl.org/dc/terms/).  See the Introduction to the document \"DCMI Metadata Terms\" (http://dublincore.org/documents/dcmi-terms/) for an explanation."@en .

dc:rights rdfs:label "Rights"@en ;
    dcterms:description "Typically, rights information includes a statement about various property rights associated with the resource, including intellectual property rights."@en ;
    dcterms:hasVersion <http://dublincore.org/usage/terms/history/#rights-006> ;
    dcterms:issued "1999-07-02"^^xsd:date ;
    dcterms:modified "2008-01-14"^^xsd:date ;
    rdfs:comment "Information about rights held in and over the resource."@en ;
    rdfs:isDefinedBy dc: ;
    skos:note "A second property with the same name as this property has been declared in the dcterms: namespace (http://purl.org/dc/terms/).  See the Introduction to the document \"DCMI Metadata Terms\" (http://dublincore.org/documents/dcmi-terms/) for an explanation."@en .

dc:source rdfs:label "Source"@en ;
    dcterms:description "The described resource may be derived from the related resource in whole or in part. Recommended best practice is to identify the related resource by means of a string conforming to a formal identification system."@en ;
    dcterms:hasVersion <http://dublincore.org/usage/terms/history/#source-006> ;
    dcterms:issued "1999-07-02"^^xsd:date ;
    dcterms:modified "2008-01-14"^^xsd:date ;
    rdfs:comment "A related resource from which the described resource is derived."@en ;
    rdfs:isDefinedBy dc: ;
    skos:note "A second property with the same name as this property has been declared in the dcterms: namespace (http://purl.org/dc/terms/).  See the Introduction to the document \"DCMI Metadata Terms\" (http://dublincore.org/documents/dcmi-terms/) for an explanation."@en .

dc:subject rdfs:label "Subject"@en ;
    dcterms:description "Typically, the subject will be represented using keywords, key phrases, or classification codes. Recommended best practice is to use a controlled vocabulary."@en ;
    dcterms:hasVersion <http://dublincore.org/usage/terms/history/#subject-007> ;
    dcterms:issued "1999-07-02"^^xsd:date ;
    dcterms:modified "2012-06-14"^^xsd:date ;
    rdfs:comment "The topic of the resource."@en ;
    rdfs:isDefinedBy dc: ;
    skos:note "A second property with the same name as this property has been declared in the dcterms: namespace (http://purl.org/dc/terms/).  See the Introduction to the document \"DCMI Metadata Terms\" (http://dublincore.org/documents/dcmi-terms/) for an explanation."@en .

dc:title rdfs:label "Title"@en ;
    dcterms:hasVersion <http://dublincore.org/usage/terms/history/#title-006> ;
    dcterms:issued "1999-07-02"^^xsd:date ;
    dcterms:modified "2008-01-14"^^xsd:date ;
    rdfs:comment "A name given to the resource."@en ;
    rdfs:isDefinedBy dc: ;
    skos:note "A second property with the same name as this property has been declared in the dcterms: namespace (http://purl.org/dc/terms/).  See the Introduction to the document \"DCMI Metadata Terms\" (http://dublincore.org/documents/dcmi-terms/) for an explanation."@en .

dc:type rdfs:label "Type"@en ;
    dcterms:description "Recommended best practice is to use a controlled vocabulary such as the DCMI Type Vocabulary [DCMITYPE]. To describe the file format, physical medium, or dimensions of the resource, use the Format element."@en ;
    dcterms:hasVersion <http://dublincore.org/usage/terms/history/#type-006> ;
    dcterms:issued "1999-07-02"^^xsd:date ;
    dcterms:modified "2008-01-14"^^xsd:date ;
    rdfs:comment "The nature or genre of the resource."@en ;
    rdfs:isDefinedBy dc: ;
    skos:note "A second property with the same name as this property has been declared in the dcterms: namespace (http://purl.org/dc/terms/).  See the Introduction to the document \"DCMI Metadata Terms\" (http://dublincore.org/documents/dcmi-terms/) for an explanation."@en .

dcterms:description a owl:AnnotationProperty .

dcterms:hasVersion a owl:AnnotationProperty .

dcterms:issued a owl:AnnotationProperty .

dcterms:modified a owl:AnnotationProperty .

dcterms:publisher a owl:AnnotationProperty .

dcterms:title a owl:AnnotationProperty .

funcs: a skos:Collection ;
    dcterms:source <http://www.opengis.net/doc/geosparql/1.0>,
        <http://www.opengis.net/doc/geosparql/1.1> ;
    rdfs:seeAlso <http://www.opengis.net/doc/geosparql/1.0>,
        <http://www.opengis.net/doc/geosparql/1.1> ;
    skos:definition "All the GeoSPARQL Functions defined within the GeoSPARQL 1.1 specification"@en ;
    skos:member funcs:area,
        funcs:asDGGS,
        funcs:asGML,
        funcs:asGeoJSON,
        funcs:asKML,
        funcs:asWKT,
        funcs:boundary,
        funcs:boundingCircle,
        funcs:buffer,
        funcs:concaveHull,
        funcs:convexHull,
        funcs:difference,
        funcs:dimension,
        funcs:distance,
        funcs:ehContains,
        funcs:ehCoveredBy,
        funcs:ehCovers,
        funcs:ehDisjoint,
        funcs:ehEquals,
        funcs:ehInside,
        funcs:ehMeet,
        funcs:ehOverlap,
        funcs:envelope,
        funcs:getSRID,
        funcs:intersection,
        funcs:isEmpty,
        funcs:isSimple,
        funcs:length,
        funcs:maxx,
        funcs:maxy,
        funcs:maxz,
        funcs:metricArea,
        funcs:metricBuffer,
        funcs:metricDistance,
        funcs:metricLength,
        funcs:metricPerimeter,
        funcs:minx,
        funcs:miny,
        funcs:minz,
        funcs:perimeter,
        funcs:rcc8dc,
        funcs:rcc8ec,
        funcs:rcc8eq,
        funcs:rcc8ntpp,
        funcs:rcc8ntppi,
        funcs:rcc8po,
        funcs:rcc8tpp,
        funcs:rcc8tppi,
        funcs:relate,
        funcs:sfContains,
        funcs:sfCrosses,
        funcs:sfDisjoint,
        funcs:sfEquals,
        funcs:sfIntersects,
        funcs:sfOverlaps,
        funcs:sfTouches,
        funcs:sfWithin,
        funcs:symDifference,
        funcs:union ;
    skos:prefLabel "GeoSPARQL Functions",
        "GeoSPARQL Functions"@en .

funcs:aggboundingBox a skos:Concept,
        sd:Aggregate ;
    dcterms:date "2021-02-25"^^xsd:date ;
    dcterms:source <http://www.opengis.net/doc/geosparql/1.1> ;
    policy:status status:valid ;
    rdfs:isDefinedBy reqs11gx:sa-functions ;
    rdfs:seeAlso <http://www.opengis.net/doc/geosparql/1.1> ;
    skos:definition "A spatial aggregate function that calculates the minimum bounding box of set of geometries."@en ;
    skos:prefLabel "bounding box"@en .

funcs:aggboundingCircle a skos:Concept,
        sd:Aggregate ;
    dcterms:date "2021-02-25"^^xsd:date ;
    dcterms:source <http://www.opengis.net/doc/geosparql/1.1> ;
    policy:status status:valid ;
    rdfs:isDefinedBy reqs11gx:sa-functions ;
    rdfs:seeAlso <http://www.opengis.net/doc/geosparql/1.1> ;
    skos:definition "A spatial aggregate function that calculates the minimum bounding circle of set of geometries."@en ;
    skos:prefLabel "bounding circle"@en .

funcs:boundingCircle_output a fno:Output ;
    fno:required true ;
    fno:type :dggsLiteral,
        :geoJSONLiteral,
        :gmlLiteral,
        :kmlLiteral,
        :wktLiteral .

funcs:boundingCircle_param1 a fno:Parameter ;
    skos:prefLabel "geom"@en ;
    fno:required true ;
    fno:type :dggsLiteral,
        :geoJSONLiteral,
        :gmlLiteral,
        :kmlLiteral,
        :wktLiteral .

funcs:common a skos:Collection ;
    dcterms:source <http://www.opengis.net/doc/geosparql/1.1> ;
    rdfs:seeAlso <http://www.opengis.net/doc/geosparql/1.1> ;
    skos:definition "All the GeoSPARQL Common Query Functions defined within the GeoSPARQL 1.1 specification"@en ;
    skos:member funcs:relate ;
    skos:prefLabel "GeoSPARQL Common Query Functions"@en .

funcs:eh a skos:Collection ;
    dcterms:source <http://www.opengis.net/doc/geosparql/1.1> ;
    rdfs:seeAlso <http://www.opengis.net/doc/geosparql/1.1> ;
    skos:definition "All the GeoSPARQL Egenhofer Topological Functions defined within the GeoSPARQL 1.1 specification"@en ;
    skos:member funcs:ehContains,
        funcs:ehCoveredBy,
        funcs:ehCovers,
        funcs:ehDisjoint,
        funcs:ehEquals,
        funcs:ehInside,
        funcs:ehMeet,
        funcs:ehOverlap ;
    skos:prefLabel "GeoSPARQL Egenhofer Topological Functions" .

funcs:ehCoveredBy_output a fno:Output ;
    fno:required true ;
    fno:type xsd:boolean .

funcs:nonTopo a skos:Collection ;
    dcterms:source <http://www.opengis.net/doc/geosparql/1.1> ;
    rdfs:seeAlso <http://www.opengis.net/doc/geosparql/1.1> ;
    skos:definition "All the GeoSPARQL Non-topological Query Functions defined within the GeoSPARQL 1.1 specification"@en ;
    skos:member funcs:area,
        funcs:boundary,
        funcs:boundingCircle,
        funcs:buffer,
        funcs:convexHull,
        funcs:difference,
        funcs:dimension,
        funcs:distance,
        funcs:envelope,
        funcs:geometryN,
        funcs:getSRID,
        funcs:intersection,
        funcs:isEmpty,
        funcs:isSimple,
        funcs:length,
        funcs:maxx,
        funcs:maxy,
        funcs:maxz,
        funcs:metricArea,
        funcs:metricBuffer,
        funcs:metricDistance,
        funcs:metricLength,
        funcs:metricPerimeter,
        funcs:minx,
        funcs:miny,
        funcs:minz,
        funcs:numGeometries,
        funcs:perimeter,
        funcs:symDifference,
        funcs:union ;
    skos:prefLabel "GeoSPARQL Non-topological Query Functions"@en .

funcs:rcc a skos:Collection ;
    dcterms:source <http://www.opengis.net/doc/geosparql/1.1> ;
    rdfs:seeAlso <http://www.opengis.net/doc/geosparql/1.1> ;
    skos:definition "All the GeoSPARQL RCC8 Topological Functions defined within the GeoSPARQL 1.1 specification"@en ;
    skos:member funcs:rcc8dc,
        funcs:rcc8ec,
        funcs:rcc8eq,
        funcs:rcc8ntpp,
        funcs:rcc8ntppi,
        funcs:rcc8po,
        funcs:rcc8tpp,
        funcs:rcc8tppi ;
    skos:prefLabel "GeoSPARQL RCC8 Topological Functions"@en .

funcs:sa a skos:Collection ;
    dcterms:source <http://www.opengis.net/doc/geosparql/1.1> ;
    rdfs:seeAlso <http://www.opengis.net/doc/geosparql/1.1> ;
    skos:member funcs:aggBoundingBox,
        funcs:aggBoundingCircle,
        funcs:aggCentroid,
        funcs:aggConcaveHull,
        funcs:aggUnion ;
    skos:prefLabel "GeoSPARQL Spatial Aggregate Functions"@en .

funcs:sf a skos:Collection ;
    dcterms:source <http://www.opengis.net/doc/geosparql/1.1> ;
    rdfs:seeAlso <http://www.opengis.net/doc/geosparql/1.1> ;
    skos:definition "All the GeoSPARQL Simple Features Topological Functions defined within the GeoSPARQL 1.1 specification"@en ;
    skos:member funcs:sfContains,
        funcs:sfCrosses,
        funcs:sfDisjoint,
        funcs:sfEquals,
        funcs:sfIntersects,
        funcs:sfOverlaps,
        funcs:sfTouches,
        funcs:sfWithin ;
    skos:prefLabel "GeoSPARQL Simple Features Functions"@en .

<http://www.opengis.net/def/geosparql> a prof:Profile ;
    dcterms:created "2020-10-11"^^xsd:date,
        "2020-11-20"^^xsd:date ;
    dcterms:creator "OGC GeoSPARQL Standards Working Group" ;
    dcterms:description "This is a 'profile declaration' for the GeoSPARQL 1.0 specification (standard) as originally published in 2012. It describes the multiple parts of the specification and how the standard relates to other standards. It is formulated according to the Profiles Vocabulary."@en,
        "This is a 'profile declaration' for the GeoSPARQL 1.1 specification (standard). It describes the multiple parts of the specification and how the standard relates to other standards. It is formulated according to the Profiles Vocabulary."@en ;
    dcterms:issued "2021"^^xsd:gYear ;
    dcterms:license "https://www.ogc.org/license"^^xsd:anyURI ;
    dcterms:modified "2020-12-22"^^xsd:date,
        "2021-06-16"^^xsd:date ;
    dcterms:publisher [ a sdo:Organization ;
            sdo:name "Open Geospatial Consortium" ;
            sdo:url "https://www.ogc.org"^^xsd:anyURI ],
        <https://ror.org/00fsdxs93> ;
    dcterms:rights "(c) 2021 Open Geospatial Consortium" ;
    dcterms:title "GeoSPARQL 1.0 Profile",
        "GeoSPARQL 1.1 Profile" ;
    owl:versionIRI <http://www.opengis.net/def/geosparql/1.0>,
        <http://www.opengis.net/def/geosparql/1.1> ;
    owl:versionInfo "OGC GeoSPARQL 1.0",
        "OGC GeosPARQL 1.1" ;
    skos:scopeNote "Profile declarations are used to allow data to identify specifications in a way that allows data to make conformance claims to them - a broader conformance claim than that made to individual 'conformance classes' that are commonly found in recent OGC specifications. Profile declarations are also used to describe and relate the often multiple parts of specifications: ontologies, specification 'documents', vocabularies, validators and so on. This declaration describes where those parts are, what form (format) they take, what information models they implement and what roles they play."@en ;
    prof:hasResource <http://www.opengis.net/def/geosparql/extended-examples>,
        <http://www.opengis.net/def/geosparql/funcsrules>,
        <http://www.opengis.net/def/geosparql/geo-jsonldcontext>,
        <http://www.opengis.net/def/geosparql/repository>,
        <http://www.opengis.net/def/geosparql/reqs>,
        <http://www.opengis.net/def/geosparql/safuncs>,
        <http://www.opengis.net/def/geosparql/sf-jsonldcontext>,
        <http://www.opengis.net/def/geosparql/validator>,
        <http://www.opengis.net/doc/IS/geosparql/1.0>,
        <http://www.opengis.net/doc/IS/geosparql/1.1>,
        <http://www.opengis.net/doc/IS/geosparql/1.1.pdf>,
        <http://www.opengis.net/doc/IS/geosparql/release-notes-1.1>,
        <http://www.opengis.net/ont/geosparql>,
        <http://www.opengis.net/ont/geosparql.json>,
        <http://www.opengis.net/ont/sf> .

<http://www.opengis.net/def/geosparql/servicedescallfunctions> a skos:ConceptScheme,
        sd:Service ;
    owl:versionIRI <http://www.opengis.net/def/geosparql/servicedescallfunctions/1.0>,
        <http://www.opengis.net/def/geosparql/servicedescallfunctions/1.1> ;
    owl:versionInfo "OGC GeoSPARQL 1.0",
        "OGC GeoSPARQL 1.1" ;
    skos:prefLabel "GeoSPARQL 1.0 SPARQL Service Description: All Functions",
        "GeoSPARQL 1.1 SPARQL Service Description: All Functions" ;
    sd:defaultEntailmentRegime ent:RDFS ;
    sd:extensionAggregate funcs:aggBoundingCircle,
        funcs:aggCentroid,
        funcs:aggConcaveHull,
        funcs:aggConvexHull,
        funcs:aggUnion ;
    sd:extensionFunction funcs:area,
        funcs:asDGGS,
        funcs:asGML,
        funcs:asGeoJSON,
        funcs:asKML,
        funcs:asWKT,
        funcs:boundary,
        funcs:boundingCircle,
        funcs:buffer,
        funcs:centroid,
        funcs:concaveHull,
        funcs:convexHull,
        funcs:coordinateDimension,
        funcs:difference,
        funcs:dimension,
        funcs:distance,
        funcs:ehContains,
        funcs:ehCoveredBy,
        funcs:ehCovers,
        funcs:ehDisjoint,
        funcs:ehEquals,
        funcs:ehInside,
        funcs:ehMeet,
        funcs:ehOverlap,
        funcs:envelope,
        funcs:geometryN,
        funcs:geometryType,
        funcs:getSRID,
        funcs:intersection,
        funcs:is3D,
        funcs:isEmpty,
        funcs:isMeasured,
        funcs:isSimple,
        funcs:length,
        funcs:maxX,
        funcs:maxY,
        funcs:maxZ,
        funcs:metricBuffer,
        funcs:metricDistance,
        funcs:minX,
        funcs:minY,
        funcs:minZ,
        funcs:numGeometries,
        funcs:rcc8dc,
        funcs:rcc8ec,
        funcs:rcc8eq,
        funcs:rcc8ntpp,
        funcs:rcc8ntppi,
        funcs:rcc8po,
        funcs:rcc8tpp,
        funcs:rcc8tppi,
        funcs:relate,
        funcs:sfContains,
        funcs:sfCrosses,
        funcs:sfDisjoint,
        funcs:sfEquals,
        funcs:sfIntersects,
        funcs:sfOverlaps,
        funcs:sfTouches,
        funcs:sfWithin,
        funcs:spatialDimension,
        funcs:symDifference,
        funcs:transform,
        funcs:union ;
    sd:resultFormat <http://www.w3.org/ns/formats/RDF_XML>,
        <http://www.w3.org/ns/formats/Turtle> ;
    sd:supportedLanguage sd:SPARQL11Query .

<http://www.opengis.net/def/geosparql/servicedescconformanceclasses> a skos:ConceptScheme,
        sd:Service ;
    owl:versionIRI <http://www.opengis.net/def/geosparql/servicedescconformanceclasses/1.0>,
        <http://www.opengis.net/def/geosparql/servicedescconformanceclasses/1.1> ;
    owl:versionInfo "OGC GeoSPARQL 1.0",
        "OGC GeoSPARQL 1.1" ;
    skos:prefLabel "GeoSPARQL 1.0 SPARQL Service Description: All Conformance Classes",
        "GeoSPARQL 1.1 SPARQL Service Description: All Conformance Classes" ;
    sd:defaultEntailmentRegime ent:RDFS ;
    sd:feature conf10core:feature-class,
        conf10core:sparql-protocol,
        conf10core:spatial-object-class,
        conf10gx:feature-properties,
        conf10gx:geometry-as-gml-literal,
        conf10gx:geometry-as-wkt-literal,
        conf10gx:geometry-class,
        conf10gx:geometry-properties,
        conf10gx:gml-literal,
        conf10gx:gml-literal-empty,
        conf10gx:gml-profile,
        conf10gx:query-functions,
        conf10gx:srid-function,
        conf10gx:wkt-axis-order,
        conf10gx:wkt-literal,
        conf10gx:wkt-literal-default-srs,
        conf10gx:wkt-literal-empty,
        conf10gtx:eh-query-functions,
        conf10gtx:rcc8-query-functions,
        conf10gtx:relate-query-function,
        conf10gtx:sf-query-functions,
        conf10qre:eh-query-rewrite,
        conf10qre:rcc8-query-rewrite,
        conf10qre:sf-query-rewrite,
        conf11core:feature-collection-class,
        conf11core:sparql-protocol,
        conf11core:spatial-object-class,
        conf11core:spatial-object-collection-class,
        conf11core:spatial-object-properties,
        conf11gx:dggs-literal,
        conf11gx:dggs-literal-empty,
        conf11gx:dggs-literal-srs,
        conf11gx:feature-properties,
        conf11gx:geojson-literal,
        conf11gx:geojson-literal-empty,
        conf11gx:geojson-literal-srs,
        conf11gx:geometry-as-dggs-function,
        conf11gx:geometry-as-dggs-literal,
        conf11gx:geometry-as-geojson-function,
        conf11gx:geometry-as-geojson-literal,
        conf11gx:geometry-as-gml-function,
        conf11gx:geometry-as-kml-function,
        conf11gx:geometry-as-kml-literal,
        conf11gx:geometry-as-wkt-function,
        conf11gx:geometry-properties,
        conf11gx:kml-literal,
        conf11gx:kml-literal-empty,
        conf11gx:kml-literal-srs,
        conf11gx:query-functions,
        conf11gx:query-functions-dggs,
        conf11gx:query-functions-non-sf,
        conf11gx:query-functions-non-sf-dggs,
        conf11gx:sa-functions ;
    sd:resultFormat <http://www.w3.org/ns/formats/RDF_XML>,
        <http://www.w3.org/ns/formats/Turtle> ;
    sd:supportedLanguage sd:SPARQL11Query .

<http://www.opengis.net/def/geosparql/servicedescextensions> a skos:ConceptScheme,
        sd:Service ;
    owl:versionIRI <http://www.opengis.net/def/geosparql/servicedescextensions/1.0>,
        <http://www.opengis.net/def/geosparql/servicedescextensions/1.1> ;
    owl:versionInfo "OGC GeoSPARQL 1.0",
        "OGC GeoSPARQL 1.1" ;
    skos:prefLabel "GeoSPARQL 1.0 SPARQL Service Description: All Extensions",
        "GeoSPARQL 1.1 SPARQL Service Description: All Extensions" ;
    sd:defaultEntailmentRegime ent:RDFS ;
    sd:feature conf10core:,
        conf10gx:,
        conf10gtx:,
        conf10qre:,
        conf10ree:,
        <http://www.opengis.net/spec/geosparql/1.0/conf/topology-vocab-extension/>,
        conf11core:,
        <http://www.opengis.net/spec/geosparql/1.1/conf/geometry-extension-dggs/>,
        conf11gx:,
        <http://www.opengis.net/spec/geosparql/1.1/conf/geometry-topology-extension/>,
        conf11qre:,
        <http://www.opengis.net/spec/geosparql/1.1/conf/rdfs-entailment-extension/>,
        <http://www.opengis.net/spec/geosparql/1.1/conf/topology-vocab-extension/> ;
    sd:resultFormat <http://www.w3.org/ns/formats/RDF_XML>,
        <http://www.w3.org/ns/formats/Turtle> ;
    sd:supportedLanguage sd:SPARQL11Query .

rules: a skos:Collection ;
    dcterms:source <http://www.opengis.net/doc/geosparql/1.0>,
        <http://www.opengis.net/doc/geosparql/1.1> ;
    rdfs:seeAlso <http://www.opengis.net/doc/geosparql/1.0>,
        <http://www.opengis.net/doc/geosparql/1.1> ;
    skos:definition "All the GeoSPARQL Rules defined within the GeoSPARQL 1.1 specification"@en ;
    skos:member rules:ehContains,
        rules:ehCoveredBy,
        rules:ehCovers,
        rules:ehDisjoint,
        rules:ehEquals,
        rules:ehInside,
        rules:ehMeet,
        rules:ehOverlap,
        rules:rcc8dc,
        rules:rcc8ec,
        rules:rcc8eq,
        rules:rcc8ntpp,
        rules:rcc8ntppi,
        rules:rcc8po,
        rules:rcc8tpp,
        rules:rcc8tppi,
        rules:sfContains,
        rules:sfCrosses,
        rules:sfDisjoint,
        rules:sfEquals,
        rules:sfIntersects,
        rules:sfOverlaps,
        rules:sfTouches,
        rules:sfWithin ;
    skos:prefLabel "GeoSPARQL Rules",
        "GeoSPARQL Rules"@en .

rules:eh a skos:Collection ;
    dcterms:source <http://www.opengis.net/doc/geosparql/1.1> ;
    rdfs:seeAlso <http://www.opengis.net/doc/geosparql/1.1> ;
    skos:definition "All the GeoSPARQL Egenhofer Rules defined within the GeoSPARQL 1.1 specification"@en ;
    skos:member rules:ehContains,
        rules:ehCoveredBy,
        rules:ehCovers,
        rules:ehDisjoint,
        rules:ehEquals,
        rules:ehInside,
        rules:ehMeet,
        rules:ehOverlap ;
    skos:prefLabel "GeoSPARQL Egenhofer Topological Rules"@en .

rules:rcc a skos:Collection ;
    dcterms:source <http://www.opengis.net/doc/geosparql/1.1> ;
    rdfs:seeAlso <http://www.opengis.net/doc/geosparql/1.1> ;
    skos:definition "All the GeoSPARQL RCC8 Rules defined within the GeoSPARQL 1.1 specification"@en ;
    skos:member rules:rcc8dc,
        rules:rcc8ec,
        rules:rcc8eq,
        rules:rcc8ntpp,
        rules:rcc8ntppi,
        rules:rcc8po,
        rules:rcc8tpp,
        rules:rcc8tppi ;
    skos:prefLabel "GeoSPARQL RCC8 Topological Rules"@en .

rules:sf a skos:Collection ;
    dcterms:source <http://www.opengis.net/doc/geosparql/1.1> ;
    rdfs:seeAlso <http://www.opengis.net/doc/geosparql/1.1> ;
    skos:definition "All the GeoSPARQL Simple Features Topological Rules defined within the GeoSPARQL 1.1 specification"@en ;
    skos:member rules:sfContains,
        rules:sfCrosses,
        rules:sfDisjoint,
        rules:sfEquals,
        rules:sfIntersects,
        rules:sfOverlaps,
        rules:sfTouches,
        rules:sfWithin ;
    skos:prefLabel "GeoSPARQL Simple Features Rules"@en .

:asDGGS a rdf:Property,
        owl:DatatypeProperty ;
    rdfs:domain :Geometry ;
    rdfs:isDefinedBy :,
        reqs11gx:geometry-as-dggs-literal ;
    rdfs:range :dggsLiteral ;
    rdfs:subPropertyOf :hasSerialization ;
    skos:definition "The Discrete Global Grid System (DGGS) serialization of a Geometry"@en ;
    skos:example spec11:B.1.2.4 ;
    skos:prefLabel "as DGGS"@en .

:asGML a rdf:Property,
        owl:DatatypeProperty ;
    rdfs:label "asGML"@en ;
    dc:contributor "Matthew Perry" ;
    dc:creator "OGC GeoSPARQL 1.0 Standard Working Group" ;
    dc:date "2011-06-16"^^xsd:date ;
    dc:description """
      The GML serialization of a geometry
    """@en ;
    rdfs:comment """
      The GML serialization of a geometry
    """@en ;
    rdfs:domain :Geometry ;
    rdfs:isDefinedBy <http://www.opengis.net/ont/geosparql>,
        :,
        <http://www.opengis.net/spec/geosparql/1.0>,
        reqs10gx:geometry-as-gml-literal,
        reqs11gx:geometry-as-gml-literal ;
    rdfs:range :gmlLiteral ;
    rdfs:subPropertyOf :hasSerialization ;
    skos:definition """
      The GML serialization of a geometry
    """@en,
        "The GML serialization of a Geometry"@en ;
    skos:example spec11:B.1.2.4 ;
    skos:prefLabel "as GML"@en,
        "asGML"@en .

:asGeoJSON a rdf:Property,
        owl:DatatypeProperty ;
    rdfs:domain :Geometry ;
    rdfs:isDefinedBy :,
        reqs11gx:geometry-as-geojson-literal ;
    rdfs:range :geoJSONLiteral ;
    rdfs:seeAlso <https://tools.ietf.org/html/rfc7946> ;
    rdfs:subPropertyOf :hasSerialization ;
    skos:definition "The GeoJSON serialization of a Geometry"@en ;
    skos:example spec11:B.1.2.4 ;
    skos:prefLabel "as GeoJSON"@en .

:asKML a rdf:Property,
        owl:DatatypeProperty ;
    rdfs:domain :Geometry ;
    rdfs:isDefinedBy :,
        reqs11gx:geometry-as-kml-literal ;
    rdfs:range :kmlLiteral ;
    rdfs:seeAlso <https://www.ogc.org/standards/kml> ;
    rdfs:subPropertyOf :hasSerialization ;
    skos:definition "The KML serialization of a Geometry"@en ;
    skos:example spec11:B.1.2.4 ;
    skos:prefLabel "as KML"@en .

:asWKT a rdf:Property,
        owl:DatatypeProperty ;
    rdfs:label "asWKT"@en ;
    dc:contributor "Matthew Perry" ;
    dc:creator "OGC GeoSPARQL 1.0 Standard Working Group" ;
    dc:date "2011-06-16"^^xsd:date ;
    dc:description """
      The WKT serialization of a geometry
    """@en ;
    rdfs:comment """
      The WKT serialization of a geometry
    """@en ;
    rdfs:domain :Geometry ;
    rdfs:isDefinedBy <http://www.opengis.net/ont/geosparql>,
        :,
        <http://www.opengis.net/spec/geosparql/1.0>,
        reqs10gx:geometry-as-wkt-literal,
        reqs11gx:geometry-as-wkt-literal ;
    rdfs:range :wktLiteral ;
    rdfs:subPropertyOf :hasSerialization ;
    skos:definition """
      The WKT serialization of a geometry
    """@en,
        "The WKT serialization of a Geometry"@en ;
    skos:example spec11:B.1.1.2.2,
        spec11:B.1.1.2.3,
        spec11:B.1.1.2.4,
        spec11:B.1.1.2.5,
        spec11:B.1.1.2.6,
        spec11:B.1.1.2.8,
        spec11:B.1.1.3.1,
        spec11:B.1.1.3.2,
        spec11:B.1.1.3.3,
        spec11:B.1.2.2,
        spec11:B.2.1,
        spec11:B.2.2.4 ;
    skos:prefLabel "as WKT"@en,
        "asWKT"@en .

:coordinateDimension a rdf:Property,
        owl:DatatypeProperty ;
    rdfs:label "coordinateDimension"@en ;
    dc:contributor "Matthew Perry" ;
    dc:creator "OGC GeoSPARQL 1.0 Standard Working Group" ;
    dc:date "2011-06-16"^^xsd:date ;
    dc:description """
      The number of measurements or axes needed to describe the position of this
      geometry in a coordinate system.
    """@en ;
    rdfs:comment """
      The number of measurements or axes needed to describe the position of this
      geometry in a coordinate system.
    """@en ;
    rdfs:domain :Geometry ;
    rdfs:isDefinedBy <http://www.opengis.net/ont/geosparql>,
        :,
        <http://www.opengis.net/spec/geosparql/1.0>,
        reqs11gx:geometry-properties ;
    rdfs:range xsd:integer ;
    skos:definition """
      The number of measurements or axes needed to describe the position of this
      geometry in a coordinate system.
    """@en,
        "The number of measurements or axes needed to describe the position of this Geometry in a coordinate system."@en ;
    skos:example spec11:B.1.2.3 ;
    skos:prefLabel "coordinate dimension"@en,
        "coordinateDimension"@en .

:dimension a rdf:Property,
        owl:DatatypeProperty ;
    rdfs:label "dimension"@en ;
    dc:contributor "Matthew Perry" ;
    dc:creator "OGC GeoSPARQL 1.0 Standard Working Group" ;
    dc:date "2011-06-16"^^xsd:date ;
    dc:description """
      The topological dimension of this geometric object, which
      must be less than or equal to the coordinate dimension.
      In non-homogeneous collections, this will return the largest
      topological dimension of the contained objects.
    """@en ;
    rdfs:comment """
      The topological dimension of this geometric object, which
      must be less than or equal to the coordinate dimension.
      In non-homogeneous collections, this will return the largest
      topological dimension of the contained objects.
    """@en ;
    rdfs:domain :Geometry ;
    rdfs:isDefinedBy <http://www.opengis.net/ont/geosparql>,
        :,
        <http://www.opengis.net/spec/geosparql/1.0>,
        reqs11gx:geometry-properties ;
    rdfs:range xsd:integer ;
    skos:definition """
      The topological dimension of this geometric object, which
      must be less than or equal to the coordinate dimension.
      In non-homogeneous collections, this will return the largest
      topological dimension of the contained objects.
    """@en,
        "The topological dimension of this geometric object, which must be less than or equal to the coordinate dimension. In non-homogeneous collections, this will return the largest topological dimension of the contained objects."@en ;
    skos:example spec11:B.1.2.3 ;
    skos:prefLabel "dimension"@en .

:ehContains a rdf:Property,
        owl:ObjectProperty ;
    rdfs:label "contains"@en ;
    dc:contributor "Matthew Perry" ;
    dc:creator "OGC GeoSPARQL 1.0 Standard Working Group" ;
    dc:date "2011-06-16"^^xsd:date ;
    dc:description """
      Exists if the subject SpatialObject spatially contains the
      object SpatialObject. DE-9IM: T*TFF*FF*
    """@en ;
    rdfs:comment """
      Exists if the subject SpatialObject spatially contains the
      object SpatialObject. DE-9IM: T*TFF*FF*
    """@en ;
    rdfs:domain :SpatialObject ;
    rdfs:isDefinedBy <http://www.opengis.net/ont/geosparql>,
        :,
        <http://www.opengis.net/spec/geosparql/1.0>,
        reqs10gx:eh-spatial-relations,
        reqs11gx:eh-spatial-relations ;
    rdfs:range :SpatialObject ;
    rdfs:seeAlso <http://dbpedia.org/resource/DE-9IM> ;
    skos:definition """
      Exists if the subject SpatialObject spatially contains the
      object SpatialObject. DE-9IM: T*TFF*FF*
    """@en,
        "States that the subject SpatialObject spatially contains the object SpatialObject. DE-9IM: T*TFF*FF*"@en ;
    skos:prefLabel "contains"@en .

:ehCoveredBy a rdf:Property,
        owl:ObjectProperty ;
    rdfs:label "coveredBy"@en ;
    dc:contributor "Matthew Perry" ;
    dc:creator "OGC GeoSPARQL 1.0 Standard Working Group" ;
    dc:date "2011-06-16"^^xsd:date ;
    dc:description """
      Exists if the subject SpatialObject is spatially covered
      by the object SpatialObject. DE-9IM: TFF*TFT**
    """@en ;
    rdfs:comment """
      Exists if the subject SpatialObject is spatially covered
      by the object SpatialObject. DE-9IM: TFF*TFT**
    """@en ;
    rdfs:domain :SpatialObject ;
    rdfs:isDefinedBy <http://www.opengis.net/ont/geosparql>,
        :,
        <http://www.opengis.net/spec/geosparql/1.0>,
        reqs10gx:eh-spatial-relations,
        reqs11gx:eh-spatial-relations ;
    rdfs:range :SpatialObject ;
    rdfs:seeAlso <http://dbpedia.org/resource/DE-9IM> ;
    skos:definition """
      Exists if the subject SpatialObject is spatially covered
      by the object SpatialObject. DE-9IM: TFF*TFT**
    """@en,
        "States that the subject SpatialObject is spatially covered by the object SpatialObject. DE-9IM: TFF*TFT**"@en ;
    skos:prefLabel "covered by"@en,
        "coveredBy"@en .

:ehCovers a rdf:Property,
        owl:ObjectProperty ;
    rdfs:label "covers"@en ;
    dc:contributor "Matthew Perry" ;
    dc:creator "OGC GeoSPARQL 1.0 Standard Working Group" ;
    dc:date "2011-06-16"^^xsd:date ;
    dc:description """
      Exists if the subject SpatialObject spatially covers the
      object SpatialObject. DE-9IM: T*TFT*FF*
    """@en ;
    rdfs:comment """
      Exists if the subject SpatialObject spatially covers the
      object SpatialObject. DE-9IM: T*TFT*FF*
    """@en ;
    rdfs:domain :SpatialObject ;
    rdfs:isDefinedBy <http://www.opengis.net/ont/geosparql>,
        :,
        <http://www.opengis.net/spec/geosparql/1.0>,
        reqs10gx:eh-spatial-relations,
        reqs11gx:eh-spatial-relations ;
    rdfs:range :SpatialObject ;
    rdfs:seeAlso <http://dbpedia.org/resource/DE-9IM> ;
    skos:definition """
      Exists if the subject SpatialObject spatially covers the
      object SpatialObject. DE-9IM: T*TFT*FF*
    """@en,
        "States that the subject SpatialObject spatially covers the object SpatialObject. DE-9IM: T*TFT*FF*"@en ;
    skos:prefLabel "covers"@en .

:ehInside a rdf:Property,
        owl:ObjectProperty ;
    rdfs:label "inside"@en ;
    dc:contributor "Matthew Perry" ;
    dc:creator "OGC GeoSPARQL 1.0 Standard Working Group" ;
    dc:date "2011-06-16"^^xsd:date ;
    dc:description """
      Exists if the subject SpatialObject is spatially inside
      the object SpatialObject. DE-9IM: TFF*FFT**
    """@en ;
    rdfs:comment """
      Exists if the subject SpatialObject is spatially inside
      the object SpatialObject. DE-9IM: TFF*FFT**
    """@en ;
    rdfs:domain :SpatialObject ;
    rdfs:isDefinedBy <http://www.opengis.net/ont/geosparql>,
        :,
        <http://www.opengis.net/spec/geosparql/1.0>,
        reqs10gx:eh-spatial-relations,
        reqs11gx:eh-spatial-relations ;
    rdfs:range :SpatialObject ;
    rdfs:seeAlso <http://dbpedia.org/resource/DE-9IM> ;
    skos:definition """
      Exists if the subject SpatialObject is spatially inside
      the object SpatialObject. DE-9IM: TFF*FFT**
    """@en,
        "States that the subject SpatialObject is spatially inside the object SpatialObject. DE-9IM: TFF*FFT**"@en ;
    skos:prefLabel "inside"@en .

:ehOverlap a rdf:Property,
        owl:ObjectProperty ;
    rdfs:label "overlap"@en ;
    dc:contributor "Matthew Perry" ;
    dc:creator "OGC GeoSPARQL 1.0 Standard Working Group" ;
    dc:date "2011-06-16"^^xsd:date ;
    dc:description """
      Exists if the subject SpatialObject spatially overlaps the
      object SpatialObject. DE-9IM: T*T***T**
    """@en ;
    rdfs:comment """
      Exists if the subject SpatialObject spatially overlaps the
      object SpatialObject. DE-9IM: T*T***T**
    """@en ;
    rdfs:domain :SpatialObject ;
    rdfs:isDefinedBy <http://www.opengis.net/ont/geosparql>,
        :,
        <http://www.opengis.net/spec/geosparql/1.0>,
        reqs10gx:eh-spatial-relations,
        reqs11gx:eh-spatial-relations ;
    rdfs:range :SpatialObject ;
    rdfs:seeAlso <http://dbpedia.org/resource/DE-9IM> ;
    skos:definition """
      Exists if the subject SpatialObject spatially overlaps the
      object SpatialObject. DE-9IM: T*T***T**
    """@en,
        "States that the subject SpatialObject spatially overlaps the object SpatialObject. DE-9IM: T*T***T**"@en ;
    skos:prefLabel "overlap"@en .

:hasArea a rdf:Property,
        owl:ObjectProperty ;
    rdfs:domain :SpatialObject ;
    rdfs:isDefinedBy :,
        reqs11gx:spatial-object-properties ;
    rdfs:subPropertyOf :hasSize ;
    skos:definition "The area of a Spatial Object."@en ;
    skos:example spec11:B.1.1.2.4,
        spec11:B.1.2.2 ;
    skos:prefLabel "has area"@en .

:hasBoundingBox a rdf:Property,
        owl:ObjectProperty ;
    rdfs:domain :Feature ;
    rdfs:isDefinedBy :,
        reqs11gx:feature-properties ;
    rdfs:range :Geometry ;
    rdfs:subPropertyOf :hasGeometry ;
    skos:definition "The minimum or smallest bounding or enclosing box of a given Feature."@en ;
    skos:example spec11:B.1.2.2 ;
    skos:prefLabel "has bounding box"@en ;
    skos:scopeNote "The target is a Geometry that defines a rectilinear region whose edges are aligned with the axes of the coordinate reference system, which exactly contains the Feature, for example an instance of http://www.opengis.net/ont/sf#envelope."@en .

:hasCentroid a rdf:Property,
        owl:ObjectProperty ;
    rdfs:domain :Feature ;
    rdfs:isDefinedBy :,
        reqs11gx:feature-properties ;
    rdfs:range :Geometry ;
    rdfs:subPropertyOf :hasGeometry ;
    skos:definition "The arithmetic mean position of all the Geometry points of a given Feature."@en ;
    skos:example spec11:B.1.2.2 ;
    skos:prefLabel "has centroid"@en ;
    skos:scopeNote "The target Geometry shall describe a point, for example an instance of http://www.opengis.net/ont/sf#Point."@en .

:hasLength a rdf:Property,
        owl:ObjectProperty ;
    rdfs:domain :SpatialObject ;
    rdfs:isDefinedBy :,
        reqs11gx:spatial-object-properties ;
    rdfs:subPropertyOf :hasSize ;
    skos:definition "The length of a Spatial Object."@en ;
    skos:example spec11:B.1.1.2.7,
        spec11:B.1.2.2 ;
    skos:prefLabel "has length"@en .

:hasMetricArea a rdf:Property,
        owl:DatatypeProperty ;
    rdfs:domain :SpatialObject ;
    rdfs:isDefinedBy :,
        reqs11gx:spatial-object-properties ;
    rdfs:range xsd:double ;
    rdfs:subPropertyOf :hasMetricSize ;
    skos:definition "The area of a Spatial Object in square meters."@en ;
    skos:example spec11:B.1.1.2.3,
        spec11:B.1.1.2.9,
        spec11:B.1.1.3.3,
        spec11:B.1.2.2 ;
    skos:prefLabel "has area in square meters"@en .

:hasMetricLength a rdf:Property,
        owl:DatatypeProperty ;
    rdfs:domain :SpatialObject ;
    rdfs:isDefinedBy :,
        reqs11gx:spatial-object-properties ;
    rdfs:range xsd:double ;
    rdfs:subPropertyOf :hasMetricSize ;
    skos:definition "The length of a Spatial Object in meters."@en ;
    skos:example spec11:B.1.2.2 ;
    skos:prefLabel "has length in meters"@en .

:hasMetricPerimeterLength a rdf:Property,
        owl:DatatypeProperty ;
    rdfs:domain :SpatialObject ;
    rdfs:isDefinedBy :,
        reqs11gx:spatial-object-properties ;
    rdfs:range xsd:double ;
    rdfs:subPropertyOf :hasMetricSize ;
    skos:definition "The length of the perimeter of a Spatial Object in meters."@en ;
    skos:example spec11:B.1.1.1.2 ;
    skos:prefLabel "has perimeter length in meters"@en .

:hasMetricSpatialAccuracy a rdf:Property,
        owl:DatatypeProperty ;
    rdfs:domain :Geometry ;
    rdfs:isDefinedBy :,
        reqs11gx:geometry-properties ;
    rdfs:range xsd:double ;
    skos:definition "The positional accuracy of the coordinates of a Geometry in meters."@en ;
    skos:example spec11:B.1.2.3 ;
    skos:note "Spatial accuracy is applicable when a Geometry is used to represent a Feature. It is expressed as a distance that indicates the truthfullness of the positions (coordinates) that define the Geometry. In this case accuracy defines a zone surrounding each coordinate within wich the real positions are known to be. The accuracy value defines this zone as a distance from the coordinate(s) in all directions (e.g. a line, a circle or a sphere, depending on spatial dimension)."@en ;
    skos:prefLabel "has spatial accuracy in meters"@en .

:hasMetricSpatialResolution a rdf:Property,
        owl:DatatypeProperty ;
    rdfs:domain :Geometry ;
    rdfs:isDefinedBy :,
        reqs11gx:geometry-properties ;
    rdfs:range xsd:double ;
    skos:definition "The spatial resolution of a Geometry in meters."@en ;
    skos:example spec11:B.1.1.2.6,
        spec11:B.1.2.2 ;
    skos:note "Spatial resolution specifies the level of detail of a Geometry. It the smallest dinstinguishable distance between spatially adjacent coordinates."@en ;
    skos:prefLabel "has spatial resolution in meters"@en .

:hasMetricVolume a rdf:Property,
        owl:DatatypeProperty ;
    rdfs:domain :SpatialObject ;
    rdfs:isDefinedBy :,
        reqs11gx:spatial-object-properties ;
    rdfs:range xsd:double ;
    rdfs:subPropertyOf :hasMetricSize ;
    skos:definition "The volume of a Spatial Object in cubic meters."@en ;
    skos:example spec11:B.1.1.2.9,
        spec11:B.1.2.2 ;
    skos:prefLabel "has volume in cubic meters"@en .

:hasPerimeterLength a rdf:Property,
        owl:ObjectProperty ;
    rdfs:domain :SpatialObject ;
    rdfs:isDefinedBy :,
        reqs11gx:spatial-object-properties ;
    rdfs:subPropertyOf :hasSize ;
    skos:definition "The length of the perimeter of a Spatial Object."@en ;
    skos:example spec11:B.1.1.1.2 ;
    skos:prefLabel "has perimeter length"@en .

:hasSpatialAccuracy a rdf:Property,
        owl:ObjectProperty ;
    rdfs:domain :Geometry ;
    rdfs:isDefinedBy :,
        reqs11gx:geometry-properties ;
    skos:definition "The positional accuracy of the coordinates of a Geometry."@en ;
    skos:example spec11:B.1.2.3 ;
    skos:note "Spatial accuracy is applicable when a Geometry is used to represent a Feature. It is expressed as a distance that indicates the truthfullness of the positions (coordinates) that define the Geometry. In this case accuracy defines a zone surrounding each coordinate within wich the real positions are known to be. The accuracy value defines this zone as a distance from the coordinate(s) in all directions (e.g. a line, a circle or a sphere, depending on spatial dimension)."@en ;
    skos:prefLabel "has spatial accuracy"@en .

:hasSpatialResolution a rdf:Property,
        owl:ObjectProperty ;
    rdfs:domain :Geometry ;
    rdfs:isDefinedBy :,
        reqs11gx:feature-properties ;
    skos:definition "The spatial resolution of a Geometry."@en ;
    skos:example spec11:B.1.2.2 ;
    skos:note "Spatial resolution specifies the level of detail of a Geometry. It the smallest distinguishable distance between spatially adjacent coordinates."@en ;
    skos:prefLabel "has spatial resolution"@en .

:hasVolume a rdf:Property,
        owl:ObjectProperty ;
    rdfs:domain :SpatialObject ;
    rdfs:isDefinedBy :,
        reqs11gx:spatial-object-properties ;
    rdfs:subPropertyOf :hasSize ;
    skos:definition "The volume of a three-dimensional Spatial Object."@en ;
    skos:example spec11:B.1.2.2 ;
    skos:prefLabel "has volume"@en .

:isEmpty a rdf:Property,
        owl:DatatypeProperty ;
    rdfs:label "isEmpty"@en ;
    dc:contributor "Matthew Perry" ;
    dc:creator "OGC GeoSPARQL 1.0 Standard Working Group" ;
    dc:date "2011-06-16"^^xsd:date ;
    dc:description """
      (true) if this geometric object is the empty Geometry. If
      true, then this geometric object represents the empty point
      set for the coordinate space.
    """@en ;
    rdfs:comment """
      (true) if this geometric object is the empty Geometry. If
      true, then this geometric object represents the empty point
      set for the coordinate space.
    """@en ;
    rdfs:domain :Geometry ;
    rdfs:isDefinedBy <http://www.opengis.net/ont/geosparql>,
        :,
        <http://www.opengis.net/spec/geosparql/1.0>,
        reqs10gx:geometry-properties,
        reqs11gx:geometry-properties ;
    rdfs:range xsd:boolean ;
    skos:definition """
      (true) if this geometric object is the empty Geometry. If
      true, then this geometric object represents the empty point
      set for the coordinate space.
    """@en,
        "(true) if this geometric object is the empty Geometry. If true, then this geometric object represents the empty point set for the coordinate space."@en ;
    skos:example spec11:B.1.2.3 ;
    skos:prefLabel "is empty"@en,
        "isEmpty"@en .

:isSimple a rdf:Property,
        owl:DatatypeProperty ;
    rdfs:label "isSimple"@en ;
    dc:contributor "Matthew Perry" ;
    dc:creator "OGC GeoSPARQL 1.0 Standard Working Group" ;
    dc:date "2011-06-16"^^xsd:date ;
    dc:description """
      (true) if this geometric object has no anomalous geometric
      points, such as self intersection or self tangency.
    """@en ;
    rdfs:comment """
      (true) if this geometric object has no anomalous geometric
      points, such as self intersection or self tangency.
    """@en ;
    rdfs:domain :Geometry ;
    rdfs:isDefinedBy <http://www.opengis.net/ont/geosparql>,
        :,
        <http://www.opengis.net/spec/geosparql/1.0>,
        reqs10gx:geometry-properties,
        reqs11gx:geometry-properties ;
    rdfs:range xsd:boolean ;
    rdfs:seeAlso <https://portal.ogc.org/files/?artifact_id=25355> ;
    skos:definition """
      (true) if this geometric object has no anomalous geometric
      points, such as self intersection or self tangency.
    """@en,
        "(true) if this geometric object has no anomalous geometric points, such as self intersection or self tangency."@en ;
    skos:example spec11:B.1.2.3 ;
    skos:prefLabel "is simple"@en,
        "isSimple"@en .

:rcc8dc a rdf:Property,
        owl:ObjectProperty ;
    rdfs:label "disconnected"@en ;
    dc:contributor "Matthew Perry" ;
    dc:creator "OGC GeoSPARQL 1.0 Standard Working Group" ;
    dc:date "2011-06-16"^^xsd:date ;
    dc:description """
      Exists if the subject SpatialObject is spatially disjoint
      from the object SpatialObject. DE-9IM: FFTFFTTTT
    """@en ;
    rdfs:comment """
      Exists if the subject SpatialObject is spatially disjoint
      from the object SpatialObject. DE-9IM: FFTFFTTTT
    """@en ;
    rdfs:domain :SpatialObject ;
    rdfs:isDefinedBy <http://www.opengis.net/ont/geosparql>,
        :,
        <http://www.opengis.net/spec/geosparql/1.0>,
        <http://www.opengis.net/spec/geosparql/1.0/req/topology-vocab-extension/rcc8-spatial-relations>,
        <http://www.opengis.net/spec/geosparql/1.1/req/topology-vocab-extension/rcc8-spatial-relations> ;
    rdfs:range :SpatialObject ;
    rdfs:seeAlso <http://dbpedia.org/resource/DE-9IM> ;
    skos:definition """
      Exists if the subject SpatialObject is spatially disjoint
      from the object SpatialObject. DE-9IM: FFTFFTTTT
    """@en,
        "States that the subject SpatialObject is spatially disjoint from the object SpatialObject. DE-9IM: FFTFFTTTT"@en ;
    skos:prefLabel "disconnected"@en .

:rcc8ec a rdf:Property,
        owl:ObjectProperty ;
    rdfs:label "externally connected"@en ;
    dc:contributor "Matthew Perry" ;
    dc:creator "OGC GeoSPARQL 1.0 Standard Working Group" ;
    dc:date "2011-06-16"^^xsd:date ;
    dc:description """
      Exists if the subject SpatialObject spatially meets the
      object SpatialObject. DE-9IM: FFTFTTTTT
    """@en ;
    rdfs:comment """
      Exists if the subject SpatialObject spatially meets the
      object SpatialObject. DE-9IM: FFTFTTTTT
    """@en ;
    rdfs:domain :SpatialObject ;
    rdfs:isDefinedBy <http://www.opengis.net/ont/geosparql>,
        :,
        <http://www.opengis.net/spec/geosparql/1.0>,
        <http://www.opengis.net/spec/geosparql/1.0/req/topology-vocab-extension/rcc8-spatial-relations>,
        <http://www.opengis.net/spec/geosparql/1.1/req/topology-vocab-extension/rcc8-spatial-relations> ;
    rdfs:range :SpatialObject ;
    rdfs:seeAlso <http://dbpedia.org/resource/DE-9IM> ;
    skos:definition """
      Exists if the subject SpatialObject spatially meets the
      object SpatialObject. DE-9IM: FFTFTTTTT
    """@en,
        "States that the subject SpatialObject spatially meets the object SpatialObject. DE-9IM: FFTFTTTTT"@en ;
    skos:prefLabel "externally connected"@en .

:rcc8eq a rdf:Property,
        owl:ObjectProperty ;
    rdfs:label "equals"@en ;
    dc:contributor "Matthew Perry" ;
    dc:creator "OGC GeoSPARQL 1.0 Standard Working Group" ;
    dc:date "2011-06-16"^^xsd:date ;
    dc:description """
      Exists if the subject SpatialObject spatially equals the
      object SpatialObject. DE-9IM: TFFFTFFFT
    """@en ;
    rdfs:comment """
      Exists if the subject SpatialObject spatially equals the
      object SpatialObject. DE-9IM: TFFFTFFFT
    """@en ;
    rdfs:domain :SpatialObject ;
    rdfs:isDefinedBy <http://www.opengis.net/ont/geosparql>,
        :,
        <http://www.opengis.net/spec/geosparql/1.0>,
        <http://www.opengis.net/spec/geosparql/1.0/req/topology-vocab-extension/rcc8-spatial-relations>,
        <http://www.opengis.net/spec/geosparql/1.1/req/topology-vocab-extension/rcc8-spatial-relations> ;
    rdfs:range :SpatialObject ;
    rdfs:seeAlso <http://dbpedia.org/resource/DE-9IM> ;
    skos:definition """
      Exists if the subject SpatialObject spatially equals the
      object SpatialObject. DE-9IM: TFFFTFFFT
    """@en,
        "States that the subject SpatialObject spatially equals the object SpatialObject. DE-9IM: TFFFTFFFT"@en ;
    skos:prefLabel "equals"@en .

:rcc8ntpp a rdf:Property,
        owl:ObjectProperty ;
    rdfs:label "non-tangential proper part"@en ;
    dc:contributor "Matthew Perry" ;
    dc:creator "OGC GeoSPARQL 1.0 Standard Working Group" ;
    dc:date "2011-06-16"^^xsd:date ;
    dc:description """
      Exists if the subject SpatialObject is spatially inside
      the object SpatialObject. DE-9IM: TFFTFFTTT
    """@en ;
    rdfs:comment """
      Exists if the subject SpatialObject is spatially inside
      the object SpatialObject. DE-9IM: TFFTFFTTT
    """@en ;
    rdfs:domain :SpatialObject ;
    rdfs:isDefinedBy <http://www.opengis.net/ont/geosparql>,
        :,
        <http://www.opengis.net/spec/geosparql/1.0>,
        <http://www.opengis.net/spec/geosparql/1.0/req/topology-vocab-extension/rcc8-spatial-relations>,
        <http://www.opengis.net/spec/geosparql/1.1/req/topology-vocab-extension/rcc8-spatial-relations> ;
    rdfs:range :SpatialObject ;
    rdfs:seeAlso <http://dbpedia.org/resource/DE-9IM> ;
    skos:definition """
      Exists if the subject SpatialObject is spatially inside
      the object SpatialObject. DE-9IM: TFFTFFTTT
    """@en,
        "States that the subject SpatialObject is spatially inside the object SpatialObject. DE-9IM: TFFTFFTTT"@en ;
    skos:prefLabel "non-tangential proper part"@en .

:rcc8ntppi a rdf:Property,
        owl:ObjectProperty ;
    rdfs:label "non-tangential proper part inverse"@en ;
    dc:contributor "Matthew Perry" ;
    dc:creator "OGC GeoSPARQL 1.0 Standard Working Group" ;
    dc:date "2011-06-16"^^xsd:date ;
    dc:description """
      Exists if the subject SpatialObject spatially contains the
      object SpatialObject. DE-9IM: TTTFFTFFT
    """@en ;
    rdfs:comment """
      Exists if the subject SpatialObject spatially contains the
      object SpatialObject. DE-9IM: TTTFFTFFT
    """@en ;
    rdfs:domain :SpatialObject ;
    rdfs:isDefinedBy <http://www.opengis.net/ont/geosparql>,
        :,
        <http://www.opengis.net/spec/geosparql/1.0>,
        <http://www.opengis.net/spec/geosparql/1.0/req/topology-vocab-extension/rcc8-spatial-relations>,
        <http://www.opengis.net/spec/geosparql/1.1/req/topology-vocab-extension/rcc8-spatial-relations> ;
    rdfs:range :SpatialObject ;
    rdfs:seeAlso <http://dbpedia.org/resource/DE-9IM> ;
    skos:definition """
      Exists if the subject SpatialObject spatially contains the
      object SpatialObject. DE-9IM: TTTFFTFFT
    """@en,
        "States that the subject SpatialObject spatially contains the object SpatialObject. DE-9IM: TTTFFTFFT"@en ;
    skos:prefLabel "non-tangential proper part inverse"@en .

:rcc8po a rdf:Property,
        owl:ObjectProperty ;
    rdfs:label "partially overlapping"@en ;
    dc:contributor "Matthew Perry" ;
    dc:creator "OGC GeoSPARQL 1.0 Standard Working Group" ;
    dc:date "2011-06-16"^^xsd:date ;
    dc:description """
      Exists if the subject SpatialObject spatially overlaps the
      object SpatialObject. DE-9IM: TTTTTTTTT
    """@en ;
    rdfs:comment """
      Exists if the subject SpatialObject spatially overlaps the
      object SpatialObject. DE-9IM: TTTTTTTTT
    """@en ;
    rdfs:domain :SpatialObject ;
    rdfs:isDefinedBy <http://www.opengis.net/ont/geosparql>,
        :,
        <http://www.opengis.net/spec/geosparql/1.0>,
        <http://www.opengis.net/spec/geosparql/1.0/req/topology-vocab-extension/rcc8-spatial-relations>,
        <http://www.opengis.net/spec/geosparql/1.1/req/topology-vocab-extension/rcc8-spatial-relations> ;
    rdfs:range :SpatialObject ;
    rdfs:seeAlso <http://dbpedia.org/resource/DE-9IM> ;
    skos:definition """
      Exists if the subject SpatialObject spatially overlaps the
      object SpatialObject. DE-9IM: TTTTTTTTT
    """@en,
        "States that the subject SpatialObject spatially overlaps the object SpatialObject. DE-9IM: TTTTTTTTT"@en ;
    skos:prefLabel "partially overlapping"@en .

:rcc8tpp a rdf:Property,
        owl:ObjectProperty ;
    rdfs:label "tangential proper part"@en ;
    dc:contributor "Matthew Perry" ;
    dc:creator "OGC GeoSPARQL 1.0 Standard Working Group" ;
    dc:date "2011-06-16"^^xsd:date ;
    dc:description """
      Exists if the subject SpatialObject is spatially covered
      by the object SpatialObject. DE-9IM: TFFTTFTTT
    """@en ;
    rdfs:comment """
      Exists if the subject SpatialObject is spatially covered
      by the object SpatialObject. DE-9IM: TFFTTFTTT
    """@en ;
    rdfs:domain :SpatialObject ;
    rdfs:isDefinedBy <http://www.opengis.net/ont/geosparql>,
        :,
        <http://www.opengis.net/spec/geosparql/1.0>,
        <http://www.opengis.net/spec/geosparql/1.0/req/topology-vocab-extension/rcc8-spatial-relations>,
        <http://www.opengis.net/spec/geosparql/1.1/req/topology-vocab-extension/rcc8-spatial-relations> ;
    rdfs:range :SpatialObject ;
    rdfs:seeAlso <http://dbpedia.org/resource/DE-9IM> ;
    skos:definition """
      Exists if the subject SpatialObject is spatially covered
      by the object SpatialObject. DE-9IM: TFFTTFTTT
    """@en,
        "States that the subject SpatialObject is spatially covered by the object SpatialObject. DE-9IM: TFFTTFTTT"@en ;
    skos:prefLabel "tangential proper part"@en .

:rcc8tppi a rdf:Property,
        owl:ObjectProperty ;
    rdfs:label "tangential proper part inverse"@en ;
    dc:contributor "Matthew Perry" ;
    dc:creator "OGC GeoSPARQL 1.0 Standard Working Group" ;
    dc:date "2011-06-16"^^xsd:date ;
    dc:description """
      Exists if the subject SpatialObject spatially covers the
      object SpatialObject. DE-9IM: TTTFTTFFT
    """@en ;
    rdfs:comment """
      Exists if the subject SpatialObject spatially covers the
      object SpatialObject. DE-9IM: TTTFTTFFT
    """@en ;
    rdfs:domain :SpatialObject ;
    rdfs:isDefinedBy <http://www.opengis.net/ont/geosparql>,
        :,
        <http://www.opengis.net/spec/geosparql/1.0>,
        <http://www.opengis.net/spec/geosparql/1.0/req/topology-vocab-extension/rcc8-spatial-relations>,
        <http://www.opengis.net/spec/geosparql/1.1/req/topology-vocab-extension/rcc8-spatial-relations> ;
    rdfs:range :SpatialObject ;
    rdfs:seeAlso <http://dbpedia.org/resource/DE-9IM> ;
    skos:definition """
      Exists if the subject SpatialObject spatially covers the
      object SpatialObject. DE-9IM: TTTFTTFFT
    """@en,
        "States that the subject SpatialObject spatially covers the object SpatialObject. DE-9IM: TTTFTTFFT"@en ;
    skos:prefLabel "tangential proper part inverse"@en .

:sfContains a rdf:Property,
        owl:ObjectProperty ;
    rdfs:label "contains"@en ;
    dc:contributor "Matthew Perry" ;
    dc:creator "OGC GeoSPARQL 1.0 Standard Working Group" ;
    dc:date "2011-06-16"^^xsd:date ;
    dc:description """
      Exists if the subject SpatialObject spatially contains the
      object SpatialObject. DE-9IM: T*****FF*
    """@en ;
    rdfs:comment """
      Exists if the subject SpatialObject spatially contains the
      object SpatialObject. DE-9IM: T*****FF*
    """@en ;
    rdfs:domain :SpatialObject ;
    rdfs:isDefinedBy <http://www.opengis.net/ont/geosparql>,
        :,
        <http://www.opengis.net/spec/geosparql/1.0>,
        <http://www.opengis.net/spec/geosparql/1.0/req/topology-vocab-extension/rcc8-spatial-relations>,
        <http://www.opengis.net/spec/geosparql/1.1/req/topology-vocab-extension/rcc8-spatial-relations> ;
    rdfs:range :SpatialObject ;
    rdfs:seeAlso <http://dbpedia.org/resource/DE-9IM> ;
    skos:definition """
      Exists if the subject SpatialObject spatially contains the
      object SpatialObject. DE-9IM: T*****FF*
    """@en,
        "States that the subject SpatialObject spatially contains the object SpatialObject. DE-9IM: T*****FF*"@en ;
    skos:prefLabel "contains"@en .

:sfCrosses a rdf:Property,
        owl:ObjectProperty ;
    rdfs:label "crosses"@en ;
    dc:contributor "Matthew Perry" ;
    dc:creator "OGC GeoSPARQL 1.0 Standard Working Group" ;
    dc:date "2011-06-16"^^xsd:date ;
    dc:description """
      Exists if the subject SpatialObject spatially crosses the
      object SpatialObject. DE-9IM: T*T******
    """@en ;
    rdfs:comment """
      Exists if the subject SpatialObject spatially crosses the
      object SpatialObject. DE-9IM: T*T******
    """@en ;
    rdfs:domain :SpatialObject ;
    rdfs:isDefinedBy <http://www.opengis.net/ont/geosparql>,
        :,
        <http://www.opengis.net/spec/geosparql/1.0>,
        <http://www.opengis.net/spec/geosparql/1.0/req/topology-vocab-extension/sf-spatial-relations>,
        <http://www.opengis.net/spec/geosparql/1.1/req/topology-vocab-extension/sf-spatial-relations> ;
    rdfs:range :SpatialObject ;
    rdfs:seeAlso <http://dbpedia.org/resource/DE-9IM> ;
    skos:definition """
      Exists if the subject SpatialObject spatially crosses the
      object SpatialObject. DE-9IM: T*T******
    """@en,
        "States that the subject SpatialObject spatially crosses the object SpatialObject. DE-9IM: T*T******"@en ;
    skos:prefLabel "crosses"@en .

:sfIntersects a rdf:Property,
        owl:ObjectProperty ;
    rdfs:label "intersects"@en ;
    dc:contributor "Matthew Perry" ;
    dc:creator "OGC GeoSPARQL 1.0 Standard Working Group" ;
    dc:date "2011-06-16"^^xsd:date ;
    dc:description """
      Exists if the subject SpatialObject is not spatially disjoint
      from the object SpatialObject.
      DE-9IM: T******** ^ *T******* ^ ***T***** ^ ****T****
    """@en ;
    rdfs:comment """
      Exists if the subject SpatialObject is not spatially disjoint
      from the object SpatialObject.
      DE-9IM: T******** ^ *T******* ^ ***T***** ^ ****T****
    """@en ;
    rdfs:domain :SpatialObject ;
    rdfs:isDefinedBy <http://www.opengis.net/ont/geosparql>,
        :,
        <http://www.opengis.net/spec/geosparql/1.0>,
        <http://www.opengis.net/spec/geosparql/1.0/req/topology-vocab-extension/sf-spatial-relations>,
        <http://www.opengis.net/spec/geosparql/1.1/req/topology-vocab-extension/sf-spatial-relations> ;
    rdfs:range :SpatialObject ;
    rdfs:seeAlso <http://dbpedia.org/resource/DE-9IM> ;
    skos:definition """
      Exists if the subject SpatialObject is not spatially disjoint
      from the object SpatialObject.
      DE-9IM: T******** ^ *T******* ^ ***T***** ^ ****T****
    """@en,
        "States that the subject SpatialObject is not spatially disjoint from the object SpatialObject. DE-9IM: T******** ^ *T******* ^ ***T***** ^ ****T****"@en ;
    skos:prefLabel "intersects"@en .

:sfOverlaps a rdf:Property,
        owl:ObjectProperty ;
    rdfs:label "overlaps"@en ;
    dc:contributor "Matthew Perry" ;
    dc:creator "OGC GeoSPARQL 1.0 Standard Working Group" ;
    dc:date "2011-06-16"^^xsd:date ;
    dc:description """
      Exists if the subject SpatialObject spatially overlaps the
      object SpatialObject. DE-9IM: T*T***T**
    """@en ;
    rdfs:comment """
      Exists if the subject SpatialObject spatially overlaps the
      object SpatialObject. DE-9IM: T*T***T**
    """@en ;
    rdfs:domain :SpatialObject ;
    rdfs:isDefinedBy <http://www.opengis.net/ont/geosparql>,
        :,
        <http://www.opengis.net/spec/geosparql/1.0>,
        <http://www.opengis.net/spec/geosparql/1.0/req/topology-vocab-extension/sf-spatial-relations>,
        <http://www.opengis.net/spec/geosparql/1.1/req/topology-vocab-extension/sf-spatial-relations> ;
    rdfs:range :SpatialObject ;
    rdfs:seeAlso <http://dbpedia.org/resource/DE-9IM> ;
    skos:definition """
      Exists if the subject SpatialObject spatially overlaps the
      object SpatialObject. DE-9IM: T*T***T**
    """@en,
        "States that the subject SpatialObject spatially overlaps the object SpatialObject. DE-9IM: T*T***T**"@en ;
    skos:prefLabel "overlaps"@en .

:sfWithin a rdf:Property,
        owl:ObjectProperty ;
    rdfs:label "within"@en ;
    dc:contributor "Matthew Perry" ;
    dc:creator "OGC GeoSPARQL 1.0 Standard Working Group" ;
    dc:date "2011-06-16"^^xsd:date ;
    dc:description """
      Exists if the subject SpatialObject is spatially within the
      object SpatialObject. DE-9IM: T*F**F***
    """@en ;
    rdfs:comment """
      Exists if the subject SpatialObject is spatially within the
      object SpatialObject. DE-9IM: T*F**F***
    """@en ;
    rdfs:domain :SpatialObject ;
    rdfs:isDefinedBy <http://www.opengis.net/ont/geosparql>,
        :,
        <http://www.opengis.net/spec/geosparql/1.0>,
        <http://www.opengis.net/spec/geosparql/1.0/req/topology-vocab-extension/sf-spatial-relations>,
        <http://www.opengis.net/spec/geosparql/1.1/req/topology-vocab-extension/sf-spatial-relations> ;
    rdfs:range :SpatialObject ;
    rdfs:seeAlso <http://dbpedia.org/resource/DE-9IM> ;
    skos:definition """
      Exists if the subject SpatialObject is spatially within the
      object SpatialObject. DE-9IM: T*F**F***
    """@en,
        "States that the subject SpatialObject is spatially within the object SpatialObject. DE-9IM: T*F**F***"@en ;
    skos:prefLabel "within"@en .

:spatialDimension a rdf:Property,
        owl:DatatypeProperty ;
    rdfs:label "spatialDimension"@en ;
    dc:contributor "Matthew Perry" ;
    dc:creator "OGC GeoSPARQL 1.0 Standard Working Group" ;
    dc:date "2011-06-16"^^xsd:date ;
    dc:description """
      The number of measurements or axes needed to describe the spatial position of
      this geometry in a coordinate system.
    """@en ;
    rdfs:comment """
      The number of measurements or axes needed to describe the spatial position of
      this geometry in a coordinate system.
    """@en ;
    rdfs:domain :Geometry ;
    rdfs:isDefinedBy <http://www.opengis.net/ont/geosparql>,
        :,
        <http://www.opengis.net/spec/geosparql/1.0>,
        reqs10gx:geometry-properties,
        reqs11gx:geometry-properties ;
    rdfs:range xsd:integer ;
    skos:definition """
      The number of measurements or axes needed to describe the spatial position of
      this geometry in a coordinate system.
    """@en,
        "The number of measurements or axes needed to describe the spatial position of this Geometry in a coordinate system."@en ;
    skos:example spec11:B.1.2.3 ;
    skos:prefLabel "spatial dimension"@en,
        "spatialDimension"@en .

<http://www.opengis.net/ont/gml> a prof:ResourceDescriptor ;
    dcterms:conformsTo <http://www.w3.org/TR/owl2-rdf-based-semantics/> ;
    dcterms:description "An OWL ontology (vocabulary) of the GML geometry types"@en ;
    dcterms:format "text/xml" ;
    dcterms:title "GML Geometry Types Vocabulary"@en ;
    prof:hasArtifact "https://schemas.opengis.net/gml/3.2.1/gml_32_geometries.rdf"^^xsd:anyURI ;
    prof:hasRole role:vocabulary .

conf10tve:eh-spatial-relations a spec:ConformanceTest ;
    spec:testPurpose "check conformance with this requirement"@en ;
    spec:testType spec:Capabilities ;
    rdfs:seeAlso reqs10tve:eh-spatial-relations ;
    skos:definition "Verify that queries involving these properties return the correct result for a test dataset"@en ;
    skos:prefLabel "GeoSPARQL 1.0 Conformance Test: EH Spatial Relations"@en .

conf10tve:rcc8-spatial-relations a spec:ConformanceTest ;
    spec:testPurpose "check conformance with this requirement"@en ;
    spec:testType spec:Capabilities ;
    rdfs:seeAlso reqs10tve:rcc8-spatial-relations ;
    skos:definition "Verify that queries involving these properties return the correct result for a test dataset"@en ;
    skos:prefLabel "GeoSPARQL 1.0 Conformance Test: RCC8 Spatial Relations"@en .

conf10tve:sf-spatial-relations a spec:ConformanceTest ;
    spec:testPurpose "check conformance with this requirement"@en ;
    spec:testType spec:Capabilities ;
    rdfs:seeAlso reqs10tve:sf-spatial-relations ;
    skos:definition "Verify that queries involving these properties return the correct result for a test dataset"@en ;
    skos:prefLabel "GeoSPARQL 1.0 Conformance Test: SF Spatial Relations"@en .

reqs10:geosparql10reqs a skos:Collection ;
    skos:definition "All the GeoSPARQL Requirements defined within the GeoSPARQL 1.0 specification"@en ;
    skos:member reqs10core:feature-class,
        reqs10core:sparql-protocol,
        reqs10core:spatial-object-class,
        reqs10gx:feature-properties,
        reqs10gx:geometry-as-gml-literal,
        reqs10gx:geometry-as-wkt-literal,
        reqs10gx:geometry-class,
        reqs10gx:geometry-properties,
        reqs10gx:gml-literal,
        reqs10gx:gml-literal-empty,
        reqs10gx:gml-profile,
        reqs10gx:query-functions,
        reqs10gx:srid-function,
        reqs10gx:wkt-axis-order,
        reqs10gx:wkt-literal,
        reqs10gx:wkt-literal-default-srs,
        reqs10gx:wkt-literal-empty,
        reqs10gtx:eh-query-functions,
        reqs10gtx:rcc8-query-functions,
        reqs10gtx:relate-query-function,
        reqs10gtx:sf-query-functions,
        reqs10qre:eh-query-rewrite,
        reqs10qre:rcc8-query-rewrite,
        reqs10qre:sf-query-rewrite,
        reqs10ree:bgp-rdfs-ent,
        reqs10ree:gml-geometry-types,
        reqs10ree:wkt-geometry-types,
        reqs10tve:eh-spatial-relations,
        reqs10tve:rcc8-spatial-relations,
        reqs10tve:sf-spatial-relations ;
    skos:prefLabel "GeoSPARQL 1.0 Requirements"@en .

reqs10:geosparql11reqs a skos:Collection ;
    skos:definition "All the GeoSPARQL Requirements defined within the GeoSPARQL 1.1 specification"@en ;
    skos:member reqs11core:feature-collection-class,
        reqs11core:geometry-collection-class,
        reqs11core:sparql-protocol,
        reqs11core:spatial-object-collection-class,
        reqs11gx:dggs-literal,
        reqs11gx:dggs-literal-empty,
        reqs11gx:dggs-literal-srs,
        reqs11gx:feature-properties,
        reqs11gx:geojson-literal,
        reqs11gx:geojson-literal-empty,
        reqs11gx:geojson-literal-srs,
        reqs11gx:geometry-as-dggs-literal,
        reqs11gx:geometry-as-geojson-literal,
        reqs11gx:geometry-as-kml-literal,
        reqs11gx:geometry-properties,
        reqs11gx:kml-literal,
        reqs11gx:kml-literal-empty,
        reqs11gx:kml-literal-srs,
        reqs11gx:query-functions,
        reqs11gx:query-functions-dggs,
        reqs11gx:query-functions-non-sf,
        reqs11gx:query-functions-non-sf-dggs,
        <http://www.opengis.net/spec/geosparql/1.1/req/geometry-extension/reqs11gx:sa-functions> ;
    skos:prefLabel "GeoSPARQL 1.1 Requirements"@en .

conf11core:geometry-collection-class a spec:ConformanceTest ;
    spec:testPurpose "check conformance with this requirement"@en ;
    spec:testType spec:Capabilities ;
    skos:definition "Verify that queries involving geo:GeometryCollection return the correct result on a test dataset"@en ;
    skos:prefLabel "GeoSPARQL 1.1 Conformance Test: Geometry Collection Class"@en .

confs11:geometry-extension-dggs a spec:ConformanceClass,
        skos:Collection,
        sd:Feature ;
    dcterms:requires confs11:core ;
    skos:member conf10gx:geometry-class,
        conf10gx:query-functions,
        conf10gx:srid-function,
        conf11gx:dggs-literal,
        conf11gx:dggs-literal-empty,
        conf11gx:dggs-literal-srs,
        conf11gx:feature-properties,
        conf11gx:query-functions,
        conf11gx:query-functions-non-sf,
        conf11gx:sa-functions ;
    skos:prefLabel "GeoSPARQL 1.1 Conformance Class: Geometry Extension - DGGS"@en .

conf11qre:query-rewrite-extension a spec:ConformanceClass,
        skos:Collection,
        sd:Feature ;
    dcterms:requires confs10:query-rewrite-extension,
        confs11:geometry-topology-extension ;
    skos:prefLabel "GeoSPARQL 1.1 Conformance Class: Query Rewrite Extension"@en .

confs11:rdfs-entailment-extension a spec:ConformanceClass,
        skos:Collection,
        sd:Feature ;
    dcterms:requires confs10:rdfs-entailment-extension,
        confs11:geometry-topology-extension ;
    skos:prefLabel "GeoSPARQL 1.1 Conformance Class: RDFS Entailment Extension"@en .

xsd:date a rdfs:Datatype .

skos:definition a owl:AnnotationProperty .

skos:note a owl:AnnotationProperty .

skos:prefLabel a owl:AnnotationProperty .

funcs:area_output a fno:Output ;
    fno:required true ;
    fno:type xsd:integer .

funcs:area_param1 a fno:Parameter ;
    skos:prefLabel "geom"@en ;
    fno:required true ;
    fno:type :dggsLiteral,
        :geoJSONLiteral,
        :gmlLiteral,
        :kmlLiteral,
        :wktLiteral .

funcs:area_param2 a fno:Parameter ;
    skos:prefLabel "units"@en ;
    fno:required true ;
    fno:type xsd:anyURI .

funcs:asDGGS_output a fno:Output ;
    fno:required true ;
    fno:type :dggsLiteral .

funcs:asDGGS_param1 a fno:Parameter ;
    skos:prefLabel "geom"@en ;
    fno:required true ;
    fno:type :dggsLiteral,
        :geoJSONLiteral,
        :gmlLiteral,
        :kmlLiteral,
        :wktLiteral .

funcs:asDGGS_param2 a fno:Parameter ;
    skos:prefLabel "specificDggsDatatype"@en ;
    fno:required true ;
    fno:type xsd:anyURI .

funcs:asGML_output a fno:Output ;
    fno:required true ;
    fno:type :gmlLiteral .

funcs:asGML_param1 a fno:Parameter ;
    skos:prefLabel "geom"@en ;
    fno:required true ;
    fno:type :dggsLiteral,
        :geoJSONLiteral,
        :gmlLiteral,
        :kmlLiteral,
        :wktLiteral .

funcs:asGML_param2 a fno:Parameter ;
    skos:prefLabel "gmlProfile"@en ;
    fno:required true ;
    fno:type xsd:string .

funcs:asGeoJSON_output a fno:Output ;
    fno:required true ;
    fno:type :geoJSONLiteral .

funcs:asGeoJSON_param1 a fno:Parameter ;
    skos:prefLabel "geom"@en ;
    fno:required true ;
    fno:type :dggsLiteral,
        :geoJSONLiteral,
        :gmlLiteral,
        :kmlLiteral,
        :wktLiteral .

funcs:asKML_output a fno:Output ;
    fno:required true ;
    fno:type :kmlLiteral .

funcs:asKML_param1 a fno:Parameter ;
    skos:prefLabel "geom"@en ;
    fno:required true ;
    fno:type :dggsLiteral,
        :geoJSONLiteral,
        :gmlLiteral,
        :kmlLiteral,
        :wktLiteral .

funcs:asWKT_output a fno:Output ;
    fno:required true ;
    fno:type :wktLiteral .

funcs:asWKT_param1 a fno:Parameter ;
    skos:prefLabel "geom"@en ;
    fno:required true ;
    fno:type :dggsLiteral,
        :geoJSONLiteral,
        :gmlLiteral,
        :kmlLiteral,
        :wktLiteral .

funcs:centroid a skos:Concept,
        sd:Function,
        fno:Function ;
    dcterms:date "2021-02-25"^^xsd:date ;
    dcterms:source <http://www.opengis.net/doc/geosparql/1.1> ;
    policy:status status:valid ;
    rdfs:isDefinedBy reqs11gx:sa-functions ;
    rdfs:seeAlso <http://www.opengis.net/doc/geosparql/1.1> ;
    skos:definition "A spatial aggregate function that calculates a centroid of a set of geometries."@en ;
    skos:prefLabel "centroid"@en ;
    fno:expects ( funcs:centroid_param1 ) ;
    fno:returns ( funcs:centroid_output ) .

funcs:centroid_output a fno:Output ;
    fno:required true ;
    fno:type :dggsLiteral,
        :geoJSONLiteral,
        :gmlLiteral,
        :kmlLiteral,
        :wktLiteral .

funcs:centroid_param1 a fno:Parameter ;
    skos:prefLabel "geom"@en ;
    fno:required true ;
    fno:type :dggsLiteral,
        :geoJSONLiteral,
        :gmlLiteral,
        :kmlLiteral,
        :wktLiteral .

funcs:concaveHull_output a fno:Output ;
    fno:required true ;
    fno:type :dggsLiteral,
        :geoJSONLiteral,
        :gmlLiteral,
        :kmlLiteral,
        :wktLiteral .

funcs:concaveHull_param1 a fno:Parameter ;
    skos:prefLabel "geom"@en ;
    fno:required true ;
    fno:type :dggsLiteral,
        :geoJSONLiteral,
        :gmlLiteral,
        :kmlLiteral,
        :wktLiteral .

funcs:dimension_output a fno:Output ;
    fno:required true ;
    fno:type xsd:integer .

funcs:dimension_param1 a fno:Parameter ;
    skos:prefLabel "geom"@en ;
    fno:required true ;
    fno:type :dggsLiteral,
        :geoJSONLiteral,
        :gmlLiteral,
        :kmlLiteral,
        :wktLiteral .

funcs:geometryN_output a fno:Output ;
    fno:required true ;
    fno:type :dggsLiteral,
        :geoJSONLiteral,
        :gmlLiteral,
        :kmlLiteral,
        :wktLiteral .

funcs:geometryN_param1 a fno:Parameter ;
    skos:prefLabel "geom"@en ;
    fno:required true ;
    fno:type :dggsLiteral,
        :geoJSONLiteral,
        :gmlLiteral,
        :kmlLiteral,
        :wktLiteral .

funcs:geometryN_param2 a fno:Parameter ;
    skos:prefLabel "geomindex"@en ;
    fno:required true ;
    fno:type xsd:int .

funcs:isEmpty_output a fno:Output ;
    fno:required true ;
    fno:type xsd:boolean .

funcs:isEmpty_param1 a fno:Parameter ;
    skos:prefLabel "geom1"@en ;
    fno:required true ;
    fno:type :dggsLiteral,
        :geoJSONLiteral,
        :gmlLiteral,
        :kmlLiteral,
        :wktLiteral .

funcs:isSimple_output a fno:Output ;
    fno:required true ;
    fno:type xsd:boolean .

funcs:isSimple_param1 a fno:Parameter ;
    skos:prefLabel "geom1"@en ;
    fno:required true ;
    fno:type :dggsLiteral,
        :geoJSONLiteral,
        :gmlLiteral,
        :kmlLiteral,
        :wktLiteral .

funcs:length_output a fno:Output ;
    fno:required true ;
    fno:type xsd:double .

funcs:length_param1 a fno:Parameter ;
    skos:prefLabel "geom"@en ;
    fno:required true ;
    fno:type :dggsLiteral,
        :geoJSONLiteral,
        :gmlLiteral,
        :kmlLiteral,
        :wktLiteral,
        xsd:anyURI .

funcs:maxx_output a fno:Output ;
    fno:required true ;
    fno:type xsd:double .

funcs:maxx_param1 a fno:Parameter ;
    skos:prefLabel "geom1"@en ;
    fno:required true ;
    fno:type :dggsLiteral,
        :geoJSONLiteral,
        :gmlLiteral,
        :kmlLiteral,
        :wktLiteral .

funcs:maxy_output a fno:Output ;
    fno:required true ;
    fno:type xsd:double .

funcs:maxy_param1 a fno:Parameter ;
    skos:prefLabel "geom1"@en ;
    fno:required true ;
    fno:type :dggsLiteral,
        :geoJSONLiteral,
        :gmlLiteral,
        :kmlLiteral,
        :wktLiteral .

funcs:maxz_output a fno:Output ;
    fno:required true ;
    fno:type xsd:double .

funcs:maxz_param1 a fno:Parameter ;
    skos:prefLabel "geom1"@en ;
    fno:required true ;
    fno:type :dggsLiteral,
        :geoJSONLiteral,
        :gmlLiteral,
        :kmlLiteral,
        :wktLiteral .

funcs:metricArea_output a fno:Output ;
    fno:required true ;
    fno:type xsd:integer .

funcs:metricArea_param1 a fno:Parameter ;
    skos:prefLabel "geom"@en ;
    fno:required true ;
    fno:type :dggsLiteral,
        :geoJSONLiteral,
        :gmlLiteral,
        :kmlLiteral,
        :wktLiteral .

funcs:metricBuffer_output a fno:Output ;
    fno:required true ;
    fno:type :dggsLiteral,
        :geoJSONLiteral,
        :gmlLiteral,
        :kmlLiteral,
        :wktLiteral .

funcs:metricBuffer_param1 a fno:Parameter ;
    skos:prefLabel "geom"@en ;
    fno:required true ;
    fno:type :dggsLiteral,
        :geoJSONLiteral,
        :gmlLiteral,
        :kmlLiteral,
        :wktLiteral .

funcs:metricBuffer_param2 a fno:Parameter ;
    skos:prefLabel "radius"@en ;
    fno:required true ;
    fno:type xsd:double .

funcs:metricDistance_output a fno:Output ;
    fno:required true ;
    fno:type xsd:double .

funcs:metricDistance_param1 a fno:Parameter ;
    skos:prefLabel "geom"@en ;
    fno:required true ;
    fno:type :dggsLiteral,
        :geoJSONLiteral,
        :gmlLiteral,
        :kmlLiteral,
        :wktLiteral .

funcs:metricDistance_param2 a fno:Parameter ;
    skos:prefLabel "geom"@en ;
    fno:required true ;
    fno:type :dggsLiteral,
        :geoJSONLiteral,
        :gmlLiteral,
        :kmlLiteral,
        :wktLiteral .

funcs:metricLength_output a fno:Output ;
    fno:required true ;
    fno:type xsd:double .

funcs:metricLength_param1 a fno:Parameter ;
    skos:prefLabel "geom"@en ;
    fno:required true ;
    fno:type :dggsLiteral,
        :geoJSONLiteral,
        :gmlLiteral,
        :kmlLiteral,
        :wktLiteral .

funcs:metricPerimeter_output a fno:Output ;
    fno:required true ;
    fno:type xsd:double .

funcs:metricPerimeter_param1 a fno:Parameter ;
    skos:prefLabel "geom"@en ;
    fno:required true ;
    fno:type :dggsLiteral,
        :geoJSONLiteral,
        :gmlLiteral,
        :kmlLiteral,
        :wktLiteral .

funcs:minx_output a fno:Output ;
    fno:required true ;
    fno:type xsd:double .

funcs:minx_param1 a fno:Parameter ;
    skos:prefLabel "geom1"@en ;
    fno:required true ;
    fno:type :dggsLiteral,
        :geoJSONLiteral,
        :gmlLiteral,
        :kmlLiteral,
        :wktLiteral .

funcs:miny_output a fno:Output ;
    fno:required true ;
    fno:type xsd:double .

funcs:miny_param1 a fno:Parameter ;
    skos:prefLabel "geom1"@en ;
    fno:required true ;
    fno:type :dggsLiteral,
        :geoJSONLiteral,
        :gmlLiteral,
        :kmlLiteral,
        :wktLiteral .

funcs:minz_output a fno:Output ;
    fno:required true ;
    fno:type xsd:double .

funcs:minz_param1 a fno:Parameter ;
    skos:prefLabel "geom1"@en ;
    fno:required true ;
    fno:type :dggsLiteral,
        :geoJSONLiteral,
        :gmlLiteral,
        :kmlLiteral,
        :wktLiteral .

funcs:numGeometries_output a fno:Output ;
    fno:required true ;
    fno:type xsd:integer .

funcs:numGeometries_param1 a fno:Parameter ;
    skos:prefLabel "geom"@en ;
    fno:required true ;
    fno:type :dggsLiteral,
        :geoJSONLiteral,
        :gmlLiteral,
        :kmlLiteral,
        :wktLiteral .

funcs:perimeter_output a fno:Output ;
    fno:required true ;
    fno:type xsd:double .

funcs:perimeter_param1 a fno:Parameter ;
    skos:prefLabel "geom"@en ;
    fno:required true ;
    fno:type :dggsLiteral,
        :geoJSONLiteral,
        :gmlLiteral,
        :kmlLiteral,
        :wktLiteral .

funcs:perimeter_param2 a fno:Parameter ;
    skos:prefLabel "unit"@en ;
    fno:required true ;
    fno:type xsd:anyURI .

funcs:transform_output a fno:Output ;
    fno:required true ;
    fno:type :dggsLiteral,
        :geoJSONLiteral,
        :gmlLiteral,
        :kmlLiteral,
        :wktLiteral .

funcs:transform_param1 a fno:Parameter ;
    skos:prefLabel "geom"@en ;
    fno:required true ;
    fno:type :dggsLiteral,
        :geoJSONLiteral,
        :gmlLiteral,
        :kmlLiteral,
        :wktLiteral .

funcs:transform_param2 a fno:Parameter ;
    skos:prefLabel "srsIRI"@en ;
    fno:required true ;
    fno:type xsd:anyURI .

<http://www.opengis.net/def/geosparql/extended-examples> a prof:ResourceDescriptor ;
    dcterms:description "Examples that are too long to sensibly fit within the Specification's Annex B. They are presented as individual files within a version control repository directory."@en ;
    dcterms:title "Extended Examples"@en ;
    prof:hasArtifact "https://github.com/opengeospatial/ogc-geosparql/tree/master/1.1/examples"^^xsd:anyURI ;
    prof:hasRole role:example .

<http://www.opengis.net/def/geosparql/funcsrules> a owl:Ontology,
        skos:ConceptScheme,
        prof:ResourceDescriptor ;
    dcterms:conformsTo <https://www.w3.org/TR/skos-reference/> ;
    dcterms:creator "OGC GeoSPARQL Standards Working Group" ;
    dcterms:description "all GeoSPARQL functions and rules presented as a SKOS vocabulary"@en ;
    dcterms:format "text/turtle" ;
    dcterms:license "https://www.ogc.org/license"^^xsd:anyURI ;
    dcterms:modified "2020-11-20"^^xsd:date,
        "2021-06-16"^^xsd:date ;
    dcterms:publisher [ a sdo:Organization ;
            sdo:name "Open Geospatial Consortium" ;
            sdo:url "https://www.ogc.org"^^xsd:anyURI ] ;
    dcterms:rights "(c) 2022 Open Geospatial Consortium" ;
    dcterms:title "GeoSPARQL Functions & Rules vocabulary"@en ;
    rdfs:seeAlso <http://www.opengis.net/doc/geosparql/1.0>,
        <http://www.opengis.net/doc/geosparql/1.1> ;
    owl:imports <http://www.opengis.net/def/ogc-na> ;
    owl:versionIRI <http://www.opengis.net/def/geosparql/funcsrules/1.0>,
        <http://www.opengis.net/def/geosparql/funcsrules/1.1> ;
    owl:versionInfo "OGC GeoSPARQL 1.0",
        "OGC GeoSPARQL 1.1" ;
    skos:definition "A vocabulary (taxonomy) of the functions and rules defined within the GeoSPARQL 1.0 ontology"@en,
        "A vocabulary (taxonomy) of the functions and rules defined within the GeoSPARQL 1.1 specification"@en ;
    skos:hasTopConcept funcs:area,
        funcs:asDGGS,
        funcs:asGML,
        funcs:asGeoJSON,
        funcs:asKML,
        funcs:asWKT,
        funcs:boundary,
        funcs:boundingCircle,
        funcs:buffer,
        funcs:convexHull,
        funcs:difference,
        funcs:dimension,
        funcs:distance,
        funcs:ehContains,
        funcs:ehCoveredBy,
        funcs:ehCovers,
        funcs:ehDisjoint,
        funcs:ehEquals,
        funcs:ehInside,
        funcs:ehMeet,
        funcs:ehOverlap,
        funcs:envelope,
        funcs:geometryN,
        funcs:getSRID,
        funcs:intersection,
        funcs:isEmpty,
        funcs:isSimple,
        funcs:maxx,
        funcs:maxy,
        funcs:maxz,
        funcs:metricArea,
        funcs:metricBuffer,
        funcs:metricDistance,
        funcs:metricPerimeter,
        funcs:minx,
        funcs:miny,
        funcs:minz,
        funcs:numGeometries,
        funcs:perimeter,
        funcs:rcc8dc,
        funcs:rcc8ec,
        funcs:rcc8eq,
        funcs:rcc8ntpp,
        funcs:rcc8ntppi,
        funcs:rcc8po,
        funcs:rcc8tpp,
        funcs:rcc8tppi,
        funcs:relate,
        funcs:sfContains,
        funcs:sfCrosses,
        funcs:sfDisjoint,
        funcs:sfEquals,
        funcs:sfIntersects,
        funcs:sfOverlaps,
        funcs:sfTouches,
        funcs:sfWithin,
        funcs:symDifference,
        funcs:transform,
        funcs:union,
        rules:ehContains,
        rules:ehCoveredBy,
        rules:ehCovers,
        rules:ehDisjoint,
        rules:ehEquals,
        rules:ehInside,
        rules:ehMeet,
        rules:ehOverlap,
        rules:rcc8dc,
        rules:rcc8ec,
        rules:rcc8eq,
        rules:rcc8ntpp,
        rules:rcc8ntppi,
        rules:rcc8po,
        rules:rcc8tpp,
        rules:rcc8tppi,
        rules:sfContains,
        rules:sfCrosses,
        rules:sfDisjoint,
        rules:sfEquals,
        rules:sfIntersects,
        rules:sfOverlaps,
        rules:sfTouches,
        rules:sfWithin ;
    skos:prefLabel "GeoSPARQL Functions and Rules Register",
        "GeoSPARQL Functions and Rules Register"@en ;
    prof:hasArtifact <http://defs-dev.opengis.net/static/definitions/conceptschemes/functions_geosparql.ttl>,
        "http://defs-dev.opengis.net/static/definitions/conceptschemes/functions_geosparql.ttl"^^xsd:anyURI ;
    prof:hasRole role:vocabulary .

<http://www.opengis.net/def/geosparql/geo-jsonldcontext> a prof:ResourceDescriptor ;
    dcterms:description "This is a JSON-LD context which can be used to incorporate the GeoSPARQL vocabulary in a JSON-LD file"@en ;
    dcterms:format "text/json" ;
    dcterms:title "JSON-LD context for the GeoSPARQL ontology"@en ;
    prof:hasArtifact "https://github.com/opengeospatial/ogc-geosparql/blob/master/1.1/contexts/geo-context.json"^^xsd:anyURI ;
    prof:hasRole role:specification .

<http://www.opengis.net/def/geosparql/repository> a prof:ResourceDescriptor ;
    dcterms:description "Code repository storing all Profile artifacts"@en ;
    dcterms:title "Profile code repository"@en ;
    prof:hasArtifact "https://github.com/opengeospatial/ogc-geosparql"^^xsd:anyURI ;
    prof:hasRole role:repository .

<http://www.opengis.net/def/geosparql/reqs> a skos:ConceptScheme,
        prof:ResourceDescriptor ;
    dcterms:conformsTo <https://www.w3.org/TR/skos-reference/> ;
    dcterms:created "2021-06-28"^^xsd:date ;
    dcterms:creator "OGC GeoSPARQL Standards Working Group" ;
    dcterms:description "A vocabulary of the requirements and conformance classes in the GeoSPARQL 1.1 specification"@en ;
    dcterms:format "text/turtle" ;
    dcterms:license "https://www.ogc.org/license"^^xsd:anyURI ;
    dcterms:modified "2022-06-16"^^xsd:date ;
    dcterms:publisher [ a sdo:Organization ;
            sdo:name "Open Geospatial Consortium" ;
            sdo:url "https://www.ogc.org"^^xsd:anyURI ] ;
    dcterms:rights "(c) 2022 Open Geospatial Consortium" ;
    dcterms:title "GeoSPARQL 1.1 Requirement and Conformance Class Vocabulary"@en ;
    rdfs:seeAlso <http://www.opengis.net/doc/geosparql/1.1> ;
    owl:versionIRI <http://www.opengis.net/def/geosparql/reqs/1.1> ;
    owl:versionInfo "OGC GeoSPARQL 1.1" ;
    skos:definition "A vocabulary of the requirements and conformance classes in the GeoSPARQL 1.1 specification"@en ;
    skos:prefLabel "GeoSPARQL 1.1 Requirements and Conformance Class Register"@en ;
    prof:hasArtifact "https://github.com/opengeospatial/ogc-geosparql/blob/master/1.1/reqs.ttl"^^xsd:anyURI ;
    prof:hasRole role:specification .

<http://www.opengis.net/def/geosparql/safuncs> a prof:ResourceDescriptor ;
    dcterms:conformsTo <https://www.w3.org/TR/skos-reference/> ;
    dcterms:description "all GeoSPARQL Spatial Aggregate functions presented as a SKOS vocabulary"@en ;
    dcterms:format "text/turtle" ;
    dcterms:title "GeoSPARQL Spatial Aggregate Functions"@en ;
    prof:hasArtifact "http://defs-dev.opengis.net/static/definitions/conceptschemes/sa_functions.ttl"^^xsd:anyURI ;
    prof:hasRole role:vocabulary .

<http://www.opengis.net/def/geosparql/sf-jsonldcontext> a prof:ResourceDescriptor ;
    dcterms:description "This is a JSON-LD context which can be used to incorporate the Simple Features vocabulary in a JSON-LD file"@en ;
    dcterms:format "text/json" ;
    dcterms:title "JSON-LD context for the Simple Features vocabulary"@en ;
    prof:hasArtifact "https://github.com/opengeospatial/ogc-geosparql/blob/master/1.1/contexts/sf-context.json"^^xsd:anyURI ;
    prof:hasRole role:specification .

<http://www.opengis.net/def/geosparql/validator> a prof:ResourceDescriptor ;
    dcterms:conformsTo <https://www.w3.org/TR/shacl/> ;
    dcterms:description "A [Shapes Constraint Language (SHACL)](https://www.w3.org/TR/shacl/) file that specifies rules for RDF data that can be used to test the conformance of data to the GeoSPARQL standard."@en ;
    dcterms:format "text/turtle" ;
    dcterms:title "GeoSPARQL RDF Shapes Validator"@en ;
    prof:hasArtifact "https://github.com/opengeospatial/ogc-geosparql/master/1.1/validator.ttl"^^xsd:anyURI ;
    prof:hasRole role:validation .

<http://www.opengis.net/doc/IS/geosparql/1.1.pdf> a prof:ResourceDescriptor ;
    dcterms:format "application/pdf" ;
    dcterms:title "GeoSPARQL Specification Document as a PDF"@en ;
    prof:hasArtifact "https://github.com/opengeospatial/ogc-geosparql/master/1.1/spec/_11-052r4.pdf"^^xsd:anyURI ;
    prof:hasRole role:specification .

:defaultGeometry a rdf:Property,
        owl:ObjectProperty ;
    rdfs:label "defaultGeometry"@en ;
    dc:contributor "Matthew Perry" ;
    dc:creator "OGC GeoSPARQL 1.0 Standard Working Group" ;
    dc:date "2011-06-16"^^xsd:date ;
    dc:description """
      The default geometry to be used in spatial calculations.
      It is Usually the most detailed geometry.
    """@en ;
    rdfs:comment """
      The default geometry to be used in spatial calculations.
      It is Usually the most detailed geometry.
    """@en ;
    rdfs:domain :Feature ;
    rdfs:isDefinedBy <http://www.opengis.net/ont/geosparql>,
        :,
        <http://www.opengis.net/spec/geosparql/1.0>,
        reqs11gx:feature-properties ;
    rdfs:range :Geometry ;
    rdfs:subPropertyOf :hasGeometry ;
    owl:equivalentProperty :hasDefaultGeometry ;
    skos:definition """
      The default geometry to be used in spatial calculations.
      It is Usually the most detailed geometry.
    """@en,
        "The default Geometry to be used in spatial calculations. It is usually the most detailed Geometry."@en ;
    skos:example spec11:B.1.2.2,
        spec11:B.2.1 ;
    skos:note "Duplicate properties defaultGeometry and hasDefaultGeometry exist because of an inconsistency between ontology and documentation in GeoSPARQL 1.0. Only hasDefaultGeometry is described in the documention."@en ;
    skos:prefLabel "default geometry"@en,
        "defaultGeometry"@en .

:ehDisjoint a rdf:Property,
        owl:ObjectProperty ;
    rdfs:label "disjoint"@en ;
    dc:contributor "Matthew Perry" ;
    dc:creator "OGC GeoSPARQL 1.0 Standard Working Group" ;
    dc:date "2011-06-16"^^xsd:date ;
    dc:description """
      Exists if the subject SpatialObject is spatially disjoint
      from the object SpatialObject. DE-9IM: FF*FF****
    """@en ;
    rdfs:comment """
      Exists if the subject SpatialObject is spatially disjoint
      from the object SpatialObject. DE-9IM: FF*FF****
    """@en ;
    rdfs:domain :SpatialObject ;
    rdfs:isDefinedBy <http://www.opengis.net/ont/geosparql>,
        :,
        <http://www.opengis.net/spec/geosparql/1.0>,
        reqs10gx:eh-spatial-relations,
        reqs11gx:eh-spatial-relations ;
    rdfs:range :SpatialObject ;
    rdfs:seeAlso <http://dbpedia.org/resource/DE-9IM> ;
    owl:equivalentProperty :sfDisjoint ;
    skos:definition """
      Exists if the subject SpatialObject is spatially disjoint
      from the object SpatialObject. DE-9IM: FF*FF****
    """@en,
        "States that the subject SpatialObject is spatially disjoint from the object SpatialObject. DE-9IM: FF*FF****"@en ;
    skos:prefLabel "disjoint"@en .

:ehEquals a rdf:Property,
        owl:ObjectProperty ;
    rdfs:label "equals"@en ;
    dc:contributor "Matthew Perry" ;
    dc:creator "OGC GeoSPARQL 1.0 Standard Working Group" ;
    dc:date "2011-06-16"^^xsd:date ;
    dc:description """
      Exists if the subject SpatialObject spatially equals the
      object SpatialObject. DE-9IM: TFFFTFFFT
    """@en ;
    rdfs:comment """
      Exists if the subject SpatialObject spatially equals the
      object SpatialObject. DE-9IM: TFFFTFFFT
    """@en ;
    rdfs:domain :SpatialObject ;
    rdfs:isDefinedBy <http://www.opengis.net/ont/geosparql>,
        :,
        <http://www.opengis.net/spec/geosparql/1.0>,
        reqs10gx:eh-spatial-relations,
        reqs11gx:eh-spatial-relations ;
    rdfs:range :SpatialObject ;
    rdfs:seeAlso <http://dbpedia.org/resource/DE-9IM> ;
    owl:equivalentProperty :sfEquals ;
    skos:definition """
      Exists if the subject SpatialObject spatially equals the
      object SpatialObject. DE-9IM: TFFFTFFFT
    """@en,
        "States that the subject SpatialObject spatially equals the object SpatialObject. DE-9IM: TFFFTFFFT"@en ;
    skos:prefLabel "equals"@en .

:ehMeet a rdf:Property,
        owl:ObjectProperty ;
    rdfs:label "meet"@en ;
    dc:contributor "Matthew Perry" ;
    dc:creator "OGC GeoSPARQL 1.0 Standard Working Group" ;
    dc:date "2011-06-16"^^xsd:date ;
    dc:description """
      Exists if the subject SpatialObject spatially meets the
      object SpatialObject.
      DE-9IM: FT******* ^ F**T***** ^ F***T****
    """@en ;
    rdfs:comment """
      Exists if the subject SpatialObject spatially meets the
      object SpatialObject.
      DE-9IM: FT******* ^ F**T***** ^ F***T****
    """@en ;
    rdfs:domain :SpatialObject ;
    rdfs:isDefinedBy <http://www.opengis.net/ont/geosparql>,
        :,
        <http://www.opengis.net/spec/geosparql/1.0>,
        reqs10gx:eh-spatial-relations,
        reqs11gx:eh-spatial-relations ;
    rdfs:range :SpatialObject ;
    rdfs:seeAlso <http://dbpedia.org/resource/DE-9IM> ;
    owl:equivalentProperty :sfTouches ;
    skos:definition """
      Exists if the subject SpatialObject spatially meets the
      object SpatialObject.
      DE-9IM: FT******* ^ F**T***** ^ F***T****
    """@en,
        "States that the subject SpatialObject spatially meets the object SpatialObject. DE-9IM: FT******* ^ F**T***** ^ F***T****"@en ;
    skos:prefLabel "meet"@en .

:hasDefaultGeometry a rdf:Property,
        owl:ObjectProperty ;
    rdfs:domain :Feature ;
    rdfs:isDefinedBy :,
        reqs10gx:feature-properties,
        reqs11gx:feature-properties ;
    rdfs:range :Geometry ;
    rdfs:subPropertyOf :hasGeometry ;
    owl:equivalentProperty :defaultGeometry ;
    skos:definition "The default Geometry to be used in spatial calculations. It is usually the most detailed Geometry."@en ;
    skos:note "Duplicate properties defaultGeometry and hasDefaultGeometry exist because of an inconsistency between ontology and documentation in GeoSPARQL 1.0. Only hasDefaultGeometry is described in the documention."@en ;
    skos:prefLabel "has default geometry"@en .

:sfDisjoint a rdf:Property,
        owl:ObjectProperty ;
    rdfs:label "disjoint"@en ;
    dc:contributor "Matthew Perry" ;
    dc:creator "OGC GeoSPARQL 1.0 Standard Working Group" ;
    dc:date "2011-06-16"^^xsd:date ;
    dc:description """
      Exists if the subject SpatialObject is spatially disjoint
      from the object SpatialObject. DE-9IM: FF*FF****
    """@en ;
    rdfs:comment """
      Exists if the subject SpatialObject is spatially disjoint
      from the object SpatialObject. DE-9IM: FF*FF****
    """@en ;
    rdfs:domain :SpatialObject ;
    rdfs:isDefinedBy <http://www.opengis.net/ont/geosparql>,
        :,
        <http://www.opengis.net/spec/geosparql/1.0>,
        <http://www.opengis.net/spec/geosparql/1.0/req/topology-vocab-extension/sf-spatial-relations>,
        <http://www.opengis.net/spec/geosparql/1.1/req/topology-vocab-extension/sf-spatial-relations> ;
    rdfs:range :SpatialObject ;
    rdfs:seeAlso <http://dbpedia.org/resource/DE-9IM> ;
    owl:equivalentProperty :ehDisjoint ;
    skos:definition """
      Exists if the subject SpatialObject is spatially disjoint
      from the object SpatialObject. DE-9IM: FF*FF****
    """@en,
        "States that the subject SpatialObject is spatially disjoint from the object SpatialObject. DE-9IM: FF*FF****"@en ;
    skos:prefLabel "disjoint"@en .

:sfEquals a rdf:Property,
        owl:ObjectProperty ;
    rdfs:label "equals"@en ;
    dc:contributor "Matthew Perry" ;
    dc:creator "OGC GeoSPARQL 1.0 Standard Working Group" ;
    dc:date "2011-06-16"^^xsd:date ;
    dc:description """
      Exists if the subject SpatialObject spatially equals the
      object SpatialObject. DE-9IM: TFFFTFFFT
    """@en ;
    rdfs:comment """
      Exists if the subject SpatialObject spatially equals the
      object SpatialObject. DE-9IM: TFFFTFFFT
    """@en ;
    rdfs:domain :SpatialObject ;
    rdfs:isDefinedBy <http://www.opengis.net/ont/geosparql>,
        :,
        <http://www.opengis.net/spec/geosparql/1.0>,
        <http://www.opengis.net/spec/geosparql/1.0/req/topology-vocab-extension/sf-spatial-relations>,
        <http://www.opengis.net/spec/geosparql/1.1/req/topology-vocab-extension/sf-spatial-relations> ;
    rdfs:range :SpatialObject ;
    rdfs:seeAlso <http://dbpedia.org/resource/DE-9IM> ;
    owl:equivalentProperty :ehEquals ;
    skos:definition """
      Exists if the subject SpatialObject spatially equals the
      object SpatialObject. DE-9IM: TFFFTFFFT
    """@en,
        "States that the subject SpatialObject spatially equals the object SpatialObject. DE-9IM: TFFFTFFFT"@en ;
    skos:prefLabel "equals"@en .

:sfTouches a rdf:Property,
        owl:ObjectProperty ;
    rdfs:label "touches"@en ;
    dc:contributor "Matthew Perry" ;
    dc:creator "OGC GeoSPARQL 1.0 Standard Working Group" ;
    dc:date "2011-06-16"^^xsd:date ;
    dc:description """
      Exists if the subject SpatialObject spatially touches the
      object SpatialObject.
      DE-9IM: FT******* ^ F**T***** ^ F***T****
    """@en ;
    rdfs:comment """
      Exists if the subject SpatialObject spatially touches the
      object SpatialObject.
      DE-9IM: FT******* ^ F**T***** ^ F***T****
    """@en ;
    rdfs:domain :SpatialObject ;
    rdfs:isDefinedBy <http://www.opengis.net/ont/geosparql>,
        :,
        <http://www.opengis.net/spec/geosparql/1.0>,
        <http://www.opengis.net/spec/geosparql/1.0/req/topology-vocab-extension/sf-spatial-relations>,
        <http://www.opengis.net/spec/geosparql/1.1/req/topology-vocab-extension/sf-spatial-relations> ;
    rdfs:range :SpatialObject ;
    rdfs:seeAlso <http://dbpedia.org/resource/DE-9IM> ;
    owl:equivalentProperty :ehMeet ;
    skos:definition """
      Exists if the subject SpatialObject spatially touches the
      object SpatialObject.
      DE-9IM: FT******* ^ F**T***** ^ F***T****
    """@en,
        "States that the subject SpatialObject spatially touches the object SpatialObject. DE-9IM: FT******* ^ F**T***** ^ F***T****"@en ;
    skos:prefLabel "touches"@en .

<http://www.opengis.net/ont/geosparql.json> a prof:ResourceDescriptor ;
    dcterms:description "The GeoSPARQL 1.1 ontology in RDF (JSON-LD)"@en ;
    dcterms:format "application/ld+json" ;
    dcterms:title "GeoSPARQL Ontology"@en ;
    prof:hasArtifact "https://github.com/opengeospatial/ogc-geosparql/master/1.1/geo.json"^^xsd:anyURI ;
    prof:hasRole role:schema .

sf:maximum a owl:ObjectProperty ;
    rdfs:domain sf:Envelope ;
    rdfs:isDefinedBy <http://www.opengis.net/ont/sf> ;
    rdfs:range sf:Point ;
    skos:definition "Point containing the maximum values of the coordinates of an envelope or bounding box"@en ;
    skos:prefLabel "maximum"@en .

sf:minimum a owl:ObjectProperty ;
    rdfs:domain sf:Envelope ;
    rdfs:isDefinedBy <http://www.opengis.net/ont/sf> ;
    rdfs:range sf:Point ;
    skos:definition "Point containing the minimum values of the coordinates of an envelope or bounding box"@en ;
    skos:prefLabel "minimum"@en .

confs10:query-rewrite-extension a spec:ConformanceClass,
        skos:Collection,
        sd:Feature ;
    dcterms:requires confs10:geometry-topology-extension ;
    skos:member conf10qre:eh-query-rewrite,
        conf10qre:rcc8-query-rewrite,
        conf10qre:sf-query-rewrite ;
    skos:notation "" ;
    skos:prefLabel "GeoSPARQL 1.0 Conformance Class: Query Rewrite Extension"@en .

confs10:rdfs-entailment-extension a spec:ConformanceClass,
        skos:Collection,
        sd:Feature ;
    dcterms:requires confs10:geometry-topology-extension ;
    skos:member conf10ree:bgp-rdfs-ent,
        conf10ree:gml-geometry-types,
        conf10ree:wkt-geometry-types ;
    skos:prefLabel "GeoSPARQL 1.0 Conformance Class: RDFS Entailment Extension"@en .

conf10ree:bgp-rdfs-ent a spec:ConformanceTest ;
    spec:testPurpose "check conformance with this requirement"@en ;
    spec:testType spec:Capabilities ;
    rdfs:seeAlso reqs10ree:bgp-rdfs-ent ;
    skos:definition "Verify that a set of SPARQL queries involving entailed RDF triples returns the correct result for a test dataset using the specified serialization, version and relation_family"@en ;
    skos:prefLabel "GeoSPARQL 1.0 Conformance Test: BGP RDFS Entailment"@en .

conf10ree:gml-geometry-types a spec:ConformanceTest ;
    spec:testPurpose "check conformance with this requirement"@en ;
    spec:testType spec:Capabilities ;
    rdfs:seeAlso reqs10ree:gml-geometry-types ;
    skos:definition "Verify that a set of SPARQL queries involving GML Geometry types returns the correct result for a test dataset using the specified version of GML"@en ;
    skos:prefLabel "GeoSPARQL 1.0 Conformance Test: GML Geometry Types"@en .

conf10ree:wkt-geometry-types a spec:ConformanceTest ;
    spec:testPurpose "check conformance with this requirement"@en ;
    spec:testType spec:Capabilities ;
    rdfs:seeAlso reqs10ree:wkt-geometry-types ;
    skos:definition "Verify that a set of SPARQL queries involving WKT Geometry types returns the correct result for a test dataset using the specified version of Simple Features"@en ;
    skos:prefLabel "GeoSPARQL 1.0 Conformance Test: WKT Geometry Types"@en .

confs11:geometry-extension a spec:ConformanceClass,
        skos:Collection,
        sd:Feature ;
    dcterms:requires confs10:geometry-extension,
        confs11:core ;
    skos:member conf11gx:geojson-literal,
        conf11gx:geojson-literal-empty,
        conf11gx:geojson-literal-srs,
        conf11gx:geometry-as-geojson-literal,
        conf11gx:geometry-as-kml-literal,
        conf11gx:geometry-properties,
        conf11gx:kml-literal,
        conf11gx:kml-literal-empty,
        conf11gx:kml-literal-srs,
        conf11gx:query-functions,
        conf11gx:query-functions-non-sf,
        conf11gx:sa-functions ;
    skos:prefLabel "GeoSPARQL 1.1 Conformance Class: Geometry Extension"@en .

conf11gx:geometry-as-dggs-function a spec:ConformanceTest ;
    spec:testPurpose "check conformance with this requirement"@en ;
    spec:testType spec:Capabilities ;
    rdfs:seeAlso reqs11gx:geometry-as-dggs-function ;
    skos:definition "Verify that a set of SPARQL queries involving the geof:asDGGS function returns the correct result for a test dataset when using the specified serialization and version"@en ;
    skos:prefLabel "GeoSPARQL 1.1 Conformance Test: asDGGS Function"@en .

conf11gx:geometry-as-dggs-literal a spec:ConformanceTest ;
    spec:testPurpose "check conformance with this requirement" ;
    spec:testType spec:Capabilities ;
    rdfs:seeAlso reqs11gx:geometry-as-dggs-literal ;
    skos:definition "Verify that queries involving the geo:asDGGS property return the correct result for a test dataset"@en ;
    skos:prefLabel "GeoSPARQL 1.1 Conformance Test: Geometry asDGGS Literal"@en .

conf11gx:geometry-as-geojson-function a spec:ConformanceTest ;
    spec:testPurpose "check conformance with this requirement"@en ;
    spec:testType spec:Capabilities ;
    rdfs:seeAlso reqs11gx:geometry-as-geojson-function ;
    skos:definition "Verify that a set of SPARQL queries involving the geof:asGeoJSON function returns the correct result for a test dataset when using the specified serialization and version"@en ;
    skos:prefLabel "GeoSPARQL 1.1 Conformance Test: asGeoJSON Function"@en .

conf11gx:geometry-as-gml-function a spec:ConformanceTest ;
    spec:testPurpose "check conformance with this requirement"@en ;
    spec:testType spec:Capabilities ;
    rdfs:seeAlso reqs11gx:geometry-as-gml-function ;
    skos:definition "Verify that a set of SPARQL queries involving the geof:asGML function returns the correct result for a test dataset when using the specified serialization and version"@en ;
    skos:prefLabel "GeoSPARQL 1.1 Conformance Test: asGML Function"@en .

conf11gx:geometry-as-kml-function a spec:ConformanceTest ;
    spec:testPurpose "check conformance with this requirement"@en ;
    spec:testType spec:Capabilities ;
    rdfs:seeAlso reqs11gx:geometry-as-kml-function ;
    skos:definition "Verify that a set of SPARQL queries involving the geof:asKML function returns the correct result for a test dataset when using the specified serialization and version"@en ;
    skos:prefLabel "GeoSPARQL 1.1 Conformance Test: asKML Function"@en .

conf11gx:geometry-as-wkt-function a spec:ConformanceTest ;
    spec:testPurpose "check conformance with this requirement"@en ;
    spec:testType spec:Capabilities ;
    rdfs:seeAlso reqs11gx:geometry-as-wkt-function ;
    skos:definition "Verify that a set of SPARQL queries involving the geof:asWKT function returns the correct result for a test dataset when using the specified serialization and version"@en ;
    skos:prefLabel "GeoSPARQL 1.1 Conformance Test: asWKT Function"@en .

conf11gx:query-functions-dggs a spec:ConformanceTest ;
    spec:testPurpose "check conformance with this requirement"@en ;
    spec:testType spec:Capabilities ;
    rdfs:seeAlso reqs11gx:query-functions-dggs ;
    skos:definition "Verify that a set of SPARQL queries involving each of the following functions returns the correct result for a test dataset when using the specified serialization and version: geof:boundary geof:buffer, geof:convexHull, geof:coordinateDimension, geof:difference, geof:dimension, geof:distance, geof:envelope, geof:geometryType, geof:getSRID, geof:intersection, geof:is3D, geof:isEmpty, geof:isMeasured, geof:isSimple, geof:spatialDimension, geof:symDifference, geof:transform and geof:union for DGGS geometry literals"@en ;
    skos:prefLabel "GeoSPARQL 1.1 Conformance Test: Query Functions, DGGS"@en .

conf11gx:query-functions-non-sf-dggs a spec:ConformanceTest ;
    spec:testPurpose "check conformance with this requirement"@en ;
    spec:testType spec:Capabilities ;
    rdfs:seeAlso reqs11gx:query-functions-non-sf-dggs ;
    skos:definition "Verify that a set of SPARQL queries involving each of the following functions returns the correct result for a test dataset when using the specified serialization and version: geof:area, geof:geometryN, geof:length, geof:maxX, geof:maxY, geof:maxZ, geof:minX, geof:minY, geof:minZ, geof:numGeometries and geof:projectTo for DGGS geometry literals"@en ;
    skos:prefLabel "GeoSPARQL 1.1 Conformance Test: Query Functions, non Simple Features, DGGS"@en .

confs11:topology-extension a spec:ConformanceClass,
        skos:Collection,
        sd:Feature ;
    dcterms:requires confs10:topology-extension,
        confs11:core ;
    skos:prefLabel "GeoSPARQL 1.1 Conformance Class: Topology Extension"@en .

<https://ror.org/00fsdxs93> a owl:NamedIndividual,
        sdo:Organization ;
    sdo:name "Open Geospatial Consortium" ;
    sdo:url <https://www.ogc.org> .

funcs:aggConcaveHull a skos:Concept,
        sd:Aggregate ;
    dcterms:date "2021-02-25"^^xsd:date ;
    dcterms:source <http://www.opengis.net/doc/geosparql/1.1> ;
    policy:status status:valid ;
    rdfs:isDefinedBy reqs11gx:sa-functions ;
    rdfs:seeAlso <http://www.opengis.net/doc/geosparql/1.1> ;
    skos:definition "A spatial aggregate function that calculates the concave hull of a set of geometries."@en ;
    skos:prefLabel "concave hull"@en .

funcs:aggUnion a skos:Concept,
        sd:Aggregate ;
    dcterms:source <http://www.opengis.net/doc/geosparql/1.1> ;
    policy:status status:valid ;
    rdfs:isDefinedBy reqs11gx:sa-functions ;
    rdfs:seeAlso <http://www.opengis.net/doc/geosparql/1.1> ;
    skos:definition "A spatial aggregate function that calculates the union of a set of geometries."@en ;
    skos:prefLabel "aggregate union"@en .

funcs:boundary_output a fno:Output ;
    fno:required true ;
    fno:type ogc:gmlLiteral,
        :dggsLiteral,
        :geoJSONLiteral,
        :gmlLiteral,
        :kmlLiteral,
        :wktLiteral,
        ogc:wktLiteral .

funcs:boundary_param1 a fno:Parameter ;
    skos:prefLabel "geom"@en ;
    fno:required true ;
    fno:type ogc:gmlLiteral,
        :dggsLiteral,
        :geoJSONLiteral,
        :gmlLiteral,
        :kmlLiteral,
        :wktLiteral,
        ogc:wktLiteral .

funcs:buffer_output a fno:Output ;
    fno:required true ;
    fno:type ogc:gmlLiteral,
        :dggsLiteral,
        :geoJSONLiteral,
        :gmlLiteral,
        :kmlLiteral,
        :wktLiteral,
        ogc:wktLiteral .

funcs:buffer_param1 a fno:Parameter ;
    skos:prefLabel "geom"@en ;
    fno:required true ;
    fno:type ogc:gmlLiteral,
        :dggsLiteral,
        :geoJSONLiteral,
        :gmlLiteral,
        :kmlLiteral,
        :wktLiteral,
        ogc:wktLiteral .

funcs:buffer_param2 a fno:Parameter ;
    skos:prefLabel "radius"@en ;
    fno:required true ;
    fno:type xsd:double .

funcs:buffer_param3 a fno:Parameter ;
    skos:prefLabel "units"@en ;
    fno:required true ;
    fno:type xsd:anyURI .

funcs:concaveHull a skos:Concept,
        sd:Function,
        fno:Function ;
    dcterms:date "2021-02-25"^^xsd:date ;
    dcterms:source <http://www.opengis.net/doc/geosparql/1.1> ;
    policy:status status:valid ;
    rdfs:isDefinedBy reqs11gx:sa-functions ;
    rdfs:seeAlso <http://www.opengis.net/doc/geosparql/1.1> ;
    skos:definition "A query function that calculates the concave hull of a set of geometries."@en ;
    skos:prefLabel "concave hull"@en ;
    fno:expects ( funcs:concaveHull_param1 ) ;
    fno:returns ( funcs:concaveHull_output ) .

funcs:convexHull_output a fno:Output ;
    fno:required true ;
    fno:type ogc:gmlLiteral,
        :dggsLiteral,
        :geoJSONLiteral,
        :gmlLiteral,
        :kmlLiteral,
        :wktLiteral,
        ogc:wktLiteral .

funcs:convexHull_param1 a fno:Parameter ;
    skos:prefLabel "geom"@en ;
    fno:required true ;
    fno:type ogc:gmlLiteral,
        :dggsLiteral,
        :geoJSONLiteral,
        :gmlLiteral,
        :kmlLiteral,
        :wktLiteral,
        ogc:wktLiteral .

funcs:difference_output a fno:Output ;
    fno:required true ;
    fno:type ogc:gmlLiteral,
        :dggsLiteral,
        :geoJSONLiteral,
        :gmlLiteral,
        :kmlLiteral,
        :wktLiteral,
        ogc:wktLiteral .

funcs:difference_param1 a fno:Parameter ;
    skos:prefLabel "geom"@en ;
    fno:required true ;
    fno:type ogc:gmlLiteral,
        :dggsLiteral,
        :geoJSONLiteral,
        :gmlLiteral,
        :kmlLiteral,
        :wktLiteral,
        ogc:wktLiteral .

funcs:difference_param2 a fno:Parameter ;
    skos:prefLabel "geom2"@en ;
    fno:required true ;
    fno:type ogc:gmlLiteral,
        :dggsLiteral,
        :geoJSONLiteral,
        :gmlLiteral,
        :kmlLiteral,
        :wktLiteral,
        ogc:wktLiteral .

funcs:distance_output a fno:Output ;
    fno:required true ;
    fno:type xsd:double .

funcs:distance_param1 a fno:Parameter ;
    skos:prefLabel "geom"@en ;
    fno:required true ;
    fno:type ogc:gmlLiteral,
        :dggsLiteral,
        :geoJSONLiteral,
        :gmlLiteral,
        :kmlLiteral,
        :wktLiteral,
        ogc:wktLiteral .

funcs:distance_param2 a fno:Parameter ;
    skos:prefLabel "geom2"@en ;
    fno:required true ;
    fno:type ogc:gmlLiteral,
        :dggsLiteral,
        :geoJSONLiteral,
        :gmlLiteral,
        :kmlLiteral,
        :wktLiteral,
        ogc:wktLiteral .

funcs:distance_param3 a fno:Parameter ;
    skos:prefLabel "units"@en ;
    fno:required true ;
    fno:type xsd:anyURI .

funcs:ehContains_output a fno:Output ;
    fno:required true ;
    fno:type xsd:boolean .

funcs:ehContains_param1 a fno:Parameter ;
    skos:prefLabel "geom1"@en ;
    fno:required true ;
    fno:type ogc:gmlLiteral,
        :dggsLiteral,
        :geoJSONLiteral,
        :gmlLiteral,
        :kmlLiteral,
        :wktLiteral,
        ogc:wktLiteral .

funcs:ehContains_param2 a fno:Parameter ;
    skos:prefLabel "geom2"@en ;
    fno:required true ;
    fno:type ogc:gmlLiteral,
        :dggsLiteral,
        :geoJSONLiteral,
        :gmlLiteral,
        :kmlLiteral,
        :wktLiteral,
        ogc:wktLiteral .

funcs:ehCoveredBy_param1 a fno:Parameter ;
    skos:prefLabel "geom1"@en ;
    fno:required true ;
    fno:type ogc:gmlLiteral,
        :dggsLiteral,
        :geoJSONLiteral,
        :gmlLiteral,
        :kmlLiteral,
        :wktLiteral,
        ogc:wktLiteral .

funcs:ehCoveredBy_param2 a fno:Parameter ;
    skos:prefLabel "geom2"@en ;
    fno:required true ;
    fno:type ogc:gmlLiteral,
        :dggsLiteral,
        :geoJSONLiteral,
        :gmlLiteral,
        :kmlLiteral,
        :wktLiteral,
        ogc:wktLiteral .

funcs:ehCovers_output a fno:Output ;
    fno:required true ;
    fno:type xsd:boolean .

funcs:ehCovers_param1 a fno:Parameter ;
    skos:prefLabel "geom1"@en ;
    fno:required true ;
    fno:type ogc:gmlLiteral,
        :dggsLiteral,
        :geoJSONLiteral,
        :gmlLiteral,
        :kmlLiteral,
        :wktLiteral,
        ogc:wktLiteral .

funcs:ehCovers_param2 a fno:Parameter ;
    skos:prefLabel "geom2"@en ;
    fno:required true ;
    fno:type ogc:gmlLiteral,
        :dggsLiteral,
        :geoJSONLiteral,
        :gmlLiteral,
        :kmlLiteral,
        :wktLiteral,
        ogc:wktLiteral .

funcs:ehDisjoint_output a fno:Output ;
    fno:required true ;
    fno:type xsd:boolean .

funcs:ehDisjoint_param1 a fno:Parameter ;
    skos:prefLabel "geom1"@en ;
    fno:required true ;
    fno:type ogc:gmlLiteral,
        :dggsLiteral,
        :geoJSONLiteral,
        :gmlLiteral,
        :kmlLiteral,
        :wktLiteral,
        ogc:wktLiteral .

funcs:ehDisjoint_param2 a fno:Parameter ;
    skos:prefLabel "geom2"@en ;
    fno:required true ;
    fno:type ogc:gmlLiteral,
        :dggsLiteral,
        :geoJSONLiteral,
        :gmlLiteral,
        :kmlLiteral,
        :wktLiteral,
        ogc:wktLiteral .

funcs:ehEquals_output a fno:Output ;
    fno:required true ;
    fno:type xsd:boolean .

funcs:ehEquals_param1 a fno:Parameter ;
    skos:prefLabel "geom1"@en ;
    fno:required true ;
    fno:type ogc:gmlLiteral,
        :dggsLiteral,
        :geoJSONLiteral,
        :gmlLiteral,
        :kmlLiteral,
        :wktLiteral,
        ogc:wktLiteral .

funcs:ehEquals_param2 a fno:Parameter ;
    skos:prefLabel "geom2"@en ;
    fno:required true ;
    fno:type ogc:gmlLiteral,
        :dggsLiteral,
        :geoJSONLiteral,
        :gmlLiteral,
        :kmlLiteral,
        :wktLiteral,
        ogc:wktLiteral .

funcs:ehInside_output a fno:Output ;
    fno:required true ;
    fno:type xsd:boolean .

funcs:ehInside_param1 a fno:Parameter ;
    skos:prefLabel "geom1"@en ;
    fno:required true ;
    fno:type ogc:gmlLiteral,
        :dggsLiteral,
        :geoJSONLiteral,
        :gmlLiteral,
        :kmlLiteral,
        :wktLiteral,
        ogc:wktLiteral .

funcs:ehInside_param2 a fno:Parameter ;
    skos:prefLabel "geom2"@en ;
    fno:required true ;
    fno:type ogc:gmlLiteral,
        :dggsLiteral,
        :geoJSONLiteral,
        :gmlLiteral,
        :kmlLiteral,
        :wktLiteral,
        ogc:wktLiteral .

funcs:ehMeet_output a fno:Output ;
    fno:required true ;
    fno:type xsd:boolean .

funcs:ehMeet_param1 a fno:Parameter ;
    skos:prefLabel "geom1"@en ;
    fno:required true ;
    fno:type ogc:gmlLiteral,
        :dggsLiteral,
        :geoJSONLiteral,
        :gmlLiteral,
        :kmlLiteral,
        :wktLiteral,
        ogc:wktLiteral .

funcs:ehMeet_param2 a fno:Parameter ;
    skos:prefLabel "geom2"@en ;
    fno:required true ;
    fno:type ogc:gmlLiteral,
        :dggsLiteral,
        :geoJSONLiteral,
        :gmlLiteral,
        :kmlLiteral,
        :wktLiteral,
        ogc:wktLiteral .

funcs:ehOverlap_output a fno:Output ;
    fno:required true ;
    fno:type xsd:boolean .

funcs:ehOverlap_param1 a fno:Parameter ;
    skos:prefLabel "geom1"@en ;
    fno:required true ;
    fno:type ogc:gmlLiteral,
        :dggsLiteral,
        :geoJSONLiteral,
        :gmlLiteral,
        :kmlLiteral,
        :wktLiteral,
        ogc:wktLiteral .

funcs:ehOverlap_param2 a fno:Parameter ;
    skos:prefLabel "geom2"@en ;
    fno:required true ;
    fno:type ogc:gmlLiteral,
        :dggsLiteral,
        :geoJSONLiteral,
        :gmlLiteral,
        :kmlLiteral,
        :wktLiteral,
        ogc:wktLiteral .

funcs:envelope_output a fno:Output ;
    fno:required true ;
    fno:type ogc:gmlLiteral,
        :dggsLiteral,
        :geoJSONLiteral,
        :gmlLiteral,
        :kmlLiteral,
        :wktLiteral,
        ogc:wktLiteral .

funcs:envelope_param1 a fno:Parameter ;
    skos:prefLabel "geom1"@en ;
    fno:required true ;
    fno:type ogc:gmlLiteral,
        :dggsLiteral,
        :geoJSONLiteral,
        :gmlLiteral,
        :kmlLiteral,
        :wktLiteral,
        ogc:wktLiteral .

funcs:getSRID_output a fno:Output ;
    fno:required true ;
    fno:type xsd:anyURI .

funcs:getSRID_param1 a fno:Parameter ;
    skos:prefLabel "geom1"@en ;
    fno:required true ;
    fno:type ogc:gmlLiteral,
        :dggsLiteral,
        :geoJSONLiteral,
        :gmlLiteral,
        :kmlLiteral,
        :wktLiteral,
        ogc:wktLiteral .

funcs:intersection_output a fno:Output ;
    fno:required true ;
    fno:type ogc:gmlLiteral,
        :dggsLiteral,
        :geoJSONLiteral,
        :gmlLiteral,
        :kmlLiteral,
        :wktLiteral,
        ogc:wktLiteral .

funcs:intersection_param1 a fno:Parameter ;
    skos:prefLabel "geom1"@en ;
    fno:required true ;
    fno:type ogc:gmlLiteral,
        :dggsLiteral,
        :geoJSONLiteral,
        :gmlLiteral,
        :kmlLiteral,
        :wktLiteral,
        ogc:wktLiteral .

funcs:intersection_param2 a fno:Parameter ;
    skos:prefLabel "geom2"@en ;
    fno:required true ;
    fno:type ogc:gmlLiteral,
        :dggsLiteral,
        :geoJSONLiteral,
        :gmlLiteral,
        :kmlLiteral,
        :wktLiteral,
        ogc:wktLiteral .

funcs:metricLength a skos:Concept,
        sd:Function,
        fno:Function ;
    dcterms:source <http://www.opengis.net/doc/geosparql/1.1> ;
    policy:status status:valid ;
    rdfs:isDefinedBy reqs11gx:query-functions ;
    rdfs:seeAlso <http://www.opengis.net/doc/geosparql/1.1> ;
    skos:definition "Returns the length of a geometry in meters."@en ;
    skos:prefLabel "metric length"@en ;
    fno:expects ( funcs:metricLength_param1 ) ;
    fno:returns ( funcs:metricLength_output ) .

funcs:rcc8dc_output a fno:Output ;
    fno:required true ;
    fno:type xsd:boolean .

funcs:rcc8dc_param1 a fno:Parameter ;
    skos:prefLabel "geom1"@en ;
    fno:required true ;
    fno:type ogc:gmlLiteral,
        :dggsLiteral,
        :geoJSONLiteral,
        :gmlLiteral,
        :kmlLiteral,
        :wktLiteral,
        ogc:wktLiteral .

funcs:rcc8dc_param2 a fno:Parameter ;
    skos:prefLabel "geom2"@en ;
    fno:required true ;
    fno:type ogc:gmlLiteral,
        :dggsLiteral,
        :geoJSONLiteral,
        :gmlLiteral,
        :kmlLiteral,
        :wktLiteral,
        ogc:wktLiteral .

funcs:rcc8ec_output a fno:Output ;
    fno:required true ;
    fno:type xsd:boolean .

funcs:rcc8ec_param1 a fno:Parameter ;
    skos:prefLabel "geom1"@en ;
    fno:required true ;
    fno:type ogc:gmlLiteral,
        :dggsLiteral,
        :geoJSONLiteral,
        :gmlLiteral,
        :kmlLiteral,
        :wktLiteral,
        ogc:wktLiteral .

funcs:rcc8ec_param2 a fno:Parameter ;
    skos:prefLabel "geom2"@en ;
    fno:required true ;
    fno:type ogc:gmlLiteral,
        :dggsLiteral,
        :geoJSONLiteral,
        :gmlLiteral,
        :kmlLiteral,
        :wktLiteral,
        ogc:wktLiteral .

funcs:rcc8eq_output a fno:Output ;
    fno:required true ;
    fno:type xsd:boolean .

funcs:rcc8eq_param1 a fno:Parameter ;
    skos:prefLabel "geom1"@en ;
    fno:required true ;
    fno:type ogc:gmlLiteral,
        :dggsLiteral,
        :geoJSONLiteral,
        :gmlLiteral,
        :kmlLiteral,
        :wktLiteral,
        ogc:wktLiteral .

funcs:rcc8eq_param2 a fno:Parameter ;
    skos:prefLabel "geom2"@en ;
    fno:required true ;
    fno:type ogc:gmlLiteral,
        :dggsLiteral,
        :geoJSONLiteral,
        :gmlLiteral,
        :kmlLiteral,
        :wktLiteral,
        ogc:wktLiteral .

funcs:rcc8ntpp_output a fno:Output ;
    fno:required true ;
    fno:type xsd:boolean .

funcs:rcc8ntpp_param1 a fno:Parameter ;
    skos:prefLabel "geom1"@en ;
    fno:required true ;
    fno:type ogc:gmlLiteral,
        :dggsLiteral,
        :geoJSONLiteral,
        :gmlLiteral,
        :kmlLiteral,
        :wktLiteral,
        ogc:wktLiteral .

funcs:rcc8ntpp_param2 a fno:Parameter ;
    skos:prefLabel "geom2"@en ;
    fno:required true ;
    fno:type ogc:gmlLiteral,
        :dggsLiteral,
        :geoJSONLiteral,
        :gmlLiteral,
        :kmlLiteral,
        :wktLiteral,
        ogc:wktLiteral .

funcs:rcc8ntppi_output a fno:Output ;
    fno:required true ;
    fno:type xsd:boolean .

funcs:rcc8ntppi_param1 a fno:Parameter ;
    skos:prefLabel "geom1"@en ;
    fno:required true ;
    fno:type ogc:gmlLiteral,
        :dggsLiteral,
        :geoJSONLiteral,
        :gmlLiteral,
        :kmlLiteral,
        :wktLiteral,
        ogc:wktLiteral .

funcs:rcc8ntppi_param2 a fno:Parameter ;
    skos:prefLabel "geom2"@en ;
    fno:required true ;
    fno:type ogc:gmlLiteral,
        :dggsLiteral,
        :geoJSONLiteral,
        :gmlLiteral,
        :kmlLiteral,
        :wktLiteral,
        ogc:wktLiteral .

funcs:rcc8po_output a fno:Output ;
    fno:required true ;
    fno:type xsd:boolean .

funcs:rcc8po_param1 a fno:Parameter ;
    skos:prefLabel "geom1"@en ;
    fno:required true ;
    fno:type ogc:gmlLiteral,
        :dggsLiteral,
        :geoJSONLiteral,
        :gmlLiteral,
        :kmlLiteral,
        :wktLiteral,
        ogc:wktLiteral .

funcs:rcc8po_param2 a fno:Parameter ;
    skos:prefLabel "geom2"@en ;
    fno:required true ;
    fno:type ogc:gmlLiteral,
        :dggsLiteral,
        :geoJSONLiteral,
        :gmlLiteral,
        :kmlLiteral,
        :wktLiteral,
        ogc:wktLiteral .

funcs:rcc8tpp_output a fno:Output ;
    fno:required true ;
    fno:type xsd:boolean .

funcs:rcc8tpp_param1 a fno:Parameter ;
    skos:prefLabel "geom1"@en ;
    fno:required true ;
    fno:type ogc:gmlLiteral,
        :dggsLiteral,
        :geoJSONLiteral,
        :gmlLiteral,
        :kmlLiteral,
        :wktLiteral,
        ogc:wktLiteral .

funcs:rcc8tpp_param2 a fno:Parameter ;
    skos:prefLabel "geom2"@en ;
    fno:required true ;
    fno:type ogc:gmlLiteral,
        :dggsLiteral,
        :geoJSONLiteral,
        :gmlLiteral,
        :kmlLiteral,
        :wktLiteral,
        ogc:wktLiteral .

funcs:rcc8tppi_output a fno:Output ;
    fno:required true ;
    fno:type xsd:boolean .

funcs:rcc8tppi_param1 a fno:Parameter ;
    skos:prefLabel "geom1"@en ;
    fno:required true ;
    fno:type ogc:gmlLiteral,
        :dggsLiteral,
        :geoJSONLiteral,
        :gmlLiteral,
        :kmlLiteral,
        :wktLiteral,
        ogc:wktLiteral .

funcs:rcc8tppi_param2 a fno:Parameter ;
    skos:prefLabel "geom2"@en ;
    fno:required true ;
    fno:type ogc:gmlLiteral,
        :dggsLiteral,
        :geoJSONLiteral,
        :gmlLiteral,
        :kmlLiteral,
        :wktLiteral,
        ogc:wktLiteral .

funcs:relate_output a fno:Output ;
    fno:required true ;
    fno:type xsd:boolean .

funcs:relate_param1 a fno:Parameter ;
    skos:prefLabel "geom1"@en ;
    fno:required true ;
    fno:type ogc:gmlLiteral,
        :dggsLiteral,
        :geoJSONLiteral,
        :gmlLiteral,
        :kmlLiteral,
        :wktLiteral,
        ogc:wktLiteral .

funcs:relate_param2 a fno:Parameter ;
    skos:prefLabel "geom2"@en ;
    fno:required true ;
    fno:type ogc:gmlLiteral,
        :dggsLiteral,
        :geoJSONLiteral,
        :gmlLiteral,
        :kmlLiteral,
        :wktLiteral,
        ogc:wktLiteral .

funcs:relate_param3 a fno:Parameter ;
    skos:prefLabel "pattern-matrix"@en ;
    fno:required true ;
    fno:type xsd:string .

funcs:sfContains_output a fno:Output ;
    fno:required true ;
    fno:type xsd:boolean .

funcs:sfContains_param1 a fno:Parameter ;
    skos:prefLabel "geom1"@en ;
    fno:required true ;
    fno:type ogc:gmlLiteral,
        :dggsLiteral,
        :geoJSONLiteral,
        :gmlLiteral,
        :kmlLiteral,
        :wktLiteral,
        ogc:wktLiteral .

funcs:sfContains_param2 a fno:Parameter ;
    skos:prefLabel "geom2"@en ;
    fno:required true ;
    fno:type ogc:gmlLiteral,
        :dggsLiteral,
        :geoJSONLiteral,
        :gmlLiteral,
        :kmlLiteral,
        :wktLiteral,
        ogc:wktLiteral .

funcs:sfCrosses_output a fno:Output ;
    fno:required true ;
    fno:type xsd:boolean .

funcs:sfCrosses_param1 a fno:Parameter ;
    skos:prefLabel "geom1"@en ;
    fno:required true ;
    fno:type ogc:gmlLiteral,
        :dggsLiteral,
        :geoJSONLiteral,
        :gmlLiteral,
        :kmlLiteral,
        :wktLiteral,
        ogc:wktLiteral .

funcs:sfCrosses_param2 a fno:Parameter ;
    skos:prefLabel "geom2"@en ;
    fno:required true ;
    fno:type ogc:gmlLiteral,
        :dggsLiteral,
        :geoJSONLiteral,
        :gmlLiteral,
        :kmlLiteral,
        :wktLiteral,
        ogc:wktLiteral .

funcs:sfDisjoint_output a fno:Output ;
    fno:required true ;
    fno:type xsd:boolean .

funcs:sfDisjoint_param1 a fno:Parameter ;
    skos:prefLabel "geom1"@en ;
    fno:required true ;
    fno:type ogc:gmlLiteral,
        :dggsLiteral,
        :geoJSONLiteral,
        :gmlLiteral,
        :kmlLiteral,
        :wktLiteral,
        ogc:wktLiteral .

funcs:sfDisjoint_param2 a fno:Parameter ;
    skos:prefLabel "geom2"@en ;
    fno:required true ;
    fno:type ogc:gmlLiteral,
        :dggsLiteral,
        :geoJSONLiteral,
        :gmlLiteral,
        :kmlLiteral,
        :wktLiteral,
        ogc:wktLiteral .

funcs:sfEquals_output a fno:Output ;
    fno:required true ;
    fno:type xsd:boolean .

funcs:sfEquals_param1 a fno:Parameter ;
    skos:prefLabel "geom1"@en ;
    fno:required true ;
    fno:type ogc:gmlLiteral,
        :dggsLiteral,
        :geoJSONLiteral,
        :gmlLiteral,
        :kmlLiteral,
        :wktLiteral,
        ogc:wktLiteral .

funcs:sfEquals_param2 a fno:Parameter ;
    skos:prefLabel "geom2"@en ;
    fno:required true ;
    fno:type ogc:gmlLiteral,
        :dggsLiteral,
        :geoJSONLiteral,
        :gmlLiteral,
        :kmlLiteral,
        :wktLiteral,
        ogc:wktLiteral .

funcs:sfIntersects_output a fno:Output ;
    fno:required true ;
    fno:type xsd:boolean .

funcs:sfIntersects_param1 a fno:Parameter ;
    skos:prefLabel "geom1"@en ;
    fno:required true ;
    fno:type ogc:gmlLiteral,
        :dggsLiteral,
        :geoJSONLiteral,
        :gmlLiteral,
        :kmlLiteral,
        :wktLiteral,
        ogc:wktLiteral .

funcs:sfIntersects_param2 a fno:Parameter ;
    skos:prefLabel "geom2"@en ;
    fno:required true ;
    fno:type ogc:gmlLiteral,
        :dggsLiteral,
        :geoJSONLiteral,
        :gmlLiteral,
        :kmlLiteral,
        :wktLiteral,
        ogc:wktLiteral .

funcs:sfOverlaps_output a fno:Output ;
    fno:required true ;
    fno:type xsd:boolean .

funcs:sfOverlaps_param1 a fno:Parameter ;
    skos:prefLabel "geom1"@en ;
    fno:required true ;
    fno:type ogc:gmlLiteral,
        :dggsLiteral,
        :geoJSONLiteral,
        :gmlLiteral,
        :kmlLiteral,
        :wktLiteral,
        ogc:wktLiteral .

funcs:sfOverlaps_param2 a fno:Parameter ;
    skos:prefLabel "geom2"@en ;
    fno:required true ;
    fno:type ogc:gmlLiteral,
        :dggsLiteral,
        :geoJSONLiteral,
        :gmlLiteral,
        :kmlLiteral,
        :wktLiteral,
        ogc:wktLiteral .

funcs:sfTouches_output a fno:Output ;
    fno:required true ;
    fno:type xsd:boolean .

funcs:sfTouches_param1 a fno:Parameter ;
    skos:prefLabel "geom1"@en ;
    fno:required true ;
    fno:type ogc:gmlLiteral,
        :dggsLiteral,
        :geoJSONLiteral,
        :gmlLiteral,
        :kmlLiteral,
        :wktLiteral,
        ogc:wktLiteral .

funcs:sfTouches_param2 a fno:Parameter ;
    skos:prefLabel "geom2"@en ;
    fno:required true ;
    fno:type ogc:gmlLiteral,
        :dggsLiteral,
        :geoJSONLiteral,
        :gmlLiteral,
        :kmlLiteral,
        :wktLiteral,
        ogc:wktLiteral .

funcs:sfWithin_output a fno:Output ;
    fno:required true ;
    fno:type xsd:boolean .

funcs:sfWithin_param1 a fno:Parameter ;
    skos:prefLabel "geom1"@en ;
    fno:required true ;
    fno:type ogc:gmlLiteral,
        :dggsLiteral,
        :geoJSONLiteral,
        :gmlLiteral,
        :kmlLiteral,
        :wktLiteral,
        ogc:wktLiteral .

funcs:sfWithin_param2 a fno:Parameter ;
    skos:prefLabel "geom2"@en ;
    fno:required true ;
    fno:type ogc:gmlLiteral,
        :dggsLiteral,
        :geoJSONLiteral,
        :gmlLiteral,
        :kmlLiteral,
        :wktLiteral,
        ogc:wktLiteral .

funcs:symDifference_output a fno:Output ;
    fno:required true ;
    fno:type ogc:gmlLiteral,
        :dggsLiteral,
        :geoJSONLiteral,
        :gmlLiteral,
        :kmlLiteral,
        :wktLiteral,
        ogc:wktLiteral .

funcs:symDifference_param1 a fno:Parameter ;
    skos:prefLabel "geom1"@en ;
    fno:required true ;
    fno:type ogc:gmlLiteral,
        :dggsLiteral,
        :geoJSONLiteral,
        :gmlLiteral,
        :kmlLiteral,
        :wktLiteral,
        ogc:wktLiteral .

funcs:symDifference_param2 a fno:Parameter ;
    skos:prefLabel "geom2"@en ;
    fno:required true ;
    fno:type ogc:gmlLiteral,
        :dggsLiteral,
        :geoJSONLiteral,
        :gmlLiteral,
        :kmlLiteral,
        :wktLiteral,
        ogc:wktLiteral .

funcs:transform a skos:Concept,
        sd:Function,
        fno:Function ;
    dcterms:source <http://www.opengis.net/doc/geosparql/1.1> ;
    policy:status status:valid ;
    rdfs:isDefinedBy reqs11gx:query-functions ;
    rdfs:seeAlso <http://www.opengis.net/doc/geosparql/1.1> ;
    skos:definition "A query function that converts a given geometry to a spatial reference system defined by an IRI. The function raises an error if a transformation is not mathematically possible."@en ;
    skos:prefLabel "transform"@en ;
    fno:expects ( funcs:transform_param1 funcs:transform_param2 ) ;
    fno:returns ( funcs:transform_output ) .

funcs:union_output a fno:Output ;
    fno:required true ;
    fno:type ogc:gmlLiteral,
        :dggsLiteral,
        :geoJSONLiteral,
        :gmlLiteral,
        :kmlLiteral,
        :wktLiteral,
        ogc:wktLiteral .

funcs:union_param1 a fno:Parameter ;
    skos:prefLabel "geom1"@en ;
    fno:required true ;
    fno:type ogc:gmlLiteral,
        :dggsLiteral,
        :geoJSONLiteral,
        :gmlLiteral,
        :kmlLiteral,
        :wktLiteral,
        ogc:wktLiteral .

funcs:union_param2 a fno:Parameter ;
    skos:prefLabel "geom2"@en ;
    fno:required true ;
    fno:type ogc:gmlLiteral,
        :dggsLiteral,
        :geoJSONLiteral,
        :gmlLiteral,
        :kmlLiteral,
        :wktLiteral,
        ogc:wktLiteral .

conf10core:feature-class a spec:ConformanceTest ;
    spec:testPurpose "check conformance with this requirement"@en ;
    spec:testType spec:Capabilities ;
    rdfs:seeAlso reqs10core:feature-class ;
    skos:definition "Verify that queries involving geo:Feature return the correct result on a test dataset"@en ;
    skos:prefLabel "GeoSPARQL 1.0 Conformance Test: Feature Class"@en .

conf10core:spatial-object-class a spec:ConformanceTest ;
    spec:testPurpose "check conformance with this requirement"@en ;
    spec:testType spec:Capabilities ;
    rdfs:seeAlso reqs10core:spatial-object-class ;
    skos:definition "Verify that queries involving geo:SpatialObject return the correct result on a test dataset"@en ;
    skos:prefLabel "GeoSPARQL 1.0 Conformance Test: Spatial Object Class"@en .

confs10:geometry-extension a spec:ConformanceClass,
        skos:Collection,
        sd:Feature ;
    dcterms:requires confs10:core ;
    skos:member conf10gx:feature-properties,
        conf10gx:geometry-as-gml-literal,
        conf10gx:geometry-as-wkt-literal,
        conf10gx:geometry-properties,
        conf10gx:gml-literal,
        conf10gx:gml-literal-empty,
        conf10gx:gml-profile,
        conf10gx:query-functions,
        conf10gx:srid-function,
        conf10gx:wkt-axis-order,
        conf10gx:wkt-literal,
        conf10gx:wkt-literal-default-srs,
        conf10gx:wkt-literal-empty ;
    skos:prefLabel "GeoSPARQL 1.0 Conformance Class: Geometry Extension"@en .

conf10gx:feature-properties a spec:ConformanceTest ;
    spec:testPurpose "check conformance with this requirement"@en ;
    spec:testType spec:Capabilities ;
    rdfs:seeAlso reqs10gx:feature-properties ;
    skos:definition "Verify that queries involving these properties return the correct result for a test dataset"@en ;
    skos:prefLabel "GeoSPARQL 1.0 Conformance Test: Feature Properties"@en .

conf10gx:geometry-as-gml-literal a spec:ConformanceTest ;
    spec:testPurpose "check conformance with this requirement"@en ;
    spec:testType spec:Capabilities ;
    rdfs:seeAlso reqs10gx:geometry-as-gml-literal ;
    skos:definition "Verify that queries involving the geo:asGML property return the correct result for a test dataset"@en ;
    skos:prefLabel "GeoSPARQL 1.0 Conformance Test: Geometry asGML Literal"@en .

conf10gx:geometry-as-wkt-literal a spec:ConformanceTest ;
    spec:testPurpose "check conformance with this requirement"@en ;
    spec:testType spec:Capabilities ;
    rdfs:seeAlso reqs10gx:geometry-as-wkt-literal ;
    skos:definition "Verify that queries involving geo:wktLiteral values return the correct result for a test dataset"@en ;
    skos:prefLabel "GeoSPARQL 1.0 Conformance Test: Geometry asWKT Literal"@en .

conf10gx:geometry-class a spec:ConformanceTest ;
    spec:testPurpose "check conformance with this requirement"@en ;
    spec:testType spec:Capabilities ;
    rdfs:seeAlso reqs10gx:geometry-class ;
    skos:definition "Verify that queries involving geo:Geometry return the correct result on a test dataset"@en ;
    skos:prefLabel "GeoSPARQL 1.0 Conformance Test: Geometry Class"@en .

conf10gx:geometry-properties a spec:ConformanceTest ;
    spec:testPurpose "check conformance with this requirement"@en ;
    spec:testType spec:Capabilities ;
    rdfs:seeAlso reqs10gx:geometry-properties ;
    skos:definition "Verify that queries involving these properties return the correct result for a test dataset"@en ;
    skos:prefLabel "GeoSPARQL 1.0 Conformance Test: Geometry Properties"@en .

conf10gx:gml-literal a spec:ConformanceTest ;
    spec:testPurpose "check conformance with this requirement"@en ;
    spec:testType spec:Capabilities ;
    rdfs:seeAlso reqs10gx:gml-literal ;
    skos:definition "Verify that queries involving geo:gmlLiteral values return the correct result for a test dataset"@en ;
    skos:prefLabel "GeoSPARQL 1.0 Conformance Test: GML Literal"@en .

conf10gx:gml-literal-empty a spec:ConformanceTest ;
    spec:testPurpose "check conformance with this requirement"@en ;
    spec:testType spec:Capabilities ;
    rdfs:seeAlso reqs10gx:gml-literal-empty ;
    skos:definition "Verify that queries involving empty geo:gmlLiteral values return the correct result for a test dataset"@en ;
    skos:prefLabel "GeoSPARQL 1.0 Conformance Test: GML Literal Empty"@en .

conf10gx:gml-profile a spec:ConformanceTest ;
    spec:testPurpose "check conformance with this requirement"@en ;
    spec:testType spec:Capabilities ;
    rdfs:seeAlso reqs10gx:gml-profile ;
    skos:definition "Examine the implementations documentation to verify that the supported GML profiles are documented"@en ;
    skos:prefLabel "GeoSPARQL 1.0 Conformance Test: GML Profile"@en .

conf10gx:wkt-axis-order a spec:ConformanceTest ;
    spec:testPurpose "check conformance with this requirement"@en ;
    spec:testType spec:Capabilities ;
    rdfs:seeAlso reqs10gx:wkt-axis-order ;
    skos:definition "Verify that queries involving geo:wktLiteral values return the correct result for a test dataset"@en ;
    skos:prefLabel "GeoSPARQL 1.0 Conformance Test: WKT Axis Order"@en .

conf10gx:wkt-literal a spec:ConformanceTest ;
    spec:testPurpose "check conformance with this requirement"@en ;
    spec:testType spec:Capabilities ;
    rdfs:seeAlso reqs10gx:wkt-literal ;
    skos:definition "Verify that queries involving geo:wktLiteral values return the correct result for a test dataset"@en ;
    skos:prefLabel "GeoSPARQL 1.0 Conformance Test: WKT Literal"@en .

conf10gx:wkt-literal-default-srs a spec:ConformanceTest ;
    spec:testPurpose "check conformance with this requirement"@en ;
    spec:testType spec:Capabilities ;
    rdfs:seeAlso reqs10gx:wkt-literal-default-srs ;
    skos:definition "Verify that queries involving geo:wktLiteral values without an explicit encoded spatial reference system URI return the correct result for a test dataset"@en ;
    skos:prefLabel "GeoSPARQL 1.0 Conformance Test: WKT Literal Default SRS"@en .

conf10gx:wkt-literal-empty a spec:ConformanceTest ;
    spec:testPurpose "check conformance with this requirement"@en ;
    spec:testType spec:Capabilities ;
    rdfs:seeAlso reqs10gx:wkt-literal-empty ;
    skos:definition "Verify that queries involving geo:wktLiteral values return the correct result for a test dataset"@en ;
    skos:prefLabel "GeoSPARQL 1.0 Conformance Test: WKT Literal Empty"@en .

conf10qre:eh-query-rewrite a spec:ConformanceTest ;
    spec:testPurpose "check conformance with this requirement"@en ;
    spec:testType spec:Capabilities ;
    rdfs:seeAlso reqs10qre:eh-query-rewrite ;
    skos:definition "Verify that queries involving the following query transformation rules return the correct result for a test dataset when using the specified serialization and version: geor:ehEquals, geor:ehDisjoint, geor:ehMeet, geor:ehOverlap, geor:ehCovers, geor:ehCoveredBy, geor:ehInside, geor:ehContains"@en ;
    skos:prefLabel "GeoSPARQL 1.0 Conformance Test: EH Query Rewrite"@en .

conf10qre:rcc8-query-rewrite a spec:ConformanceTest ;
    spec:testPurpose "check conformance with this requirement"@en ;
    spec:testType spec:Capabilities ;
    rdfs:seeAlso reqs10qre:rcc8-query-rewrite ;
    skos:definition "Verify that queries involving the following query transformation rules return the correct result for a test dataset when using the specified serialization and version: geor:rcc8eq, geor:rcc8dc, geor:rcc8ec, geor:rcc8po, geor:rcc8tppi, geor:rcc8tpp, geor:rcc8ntpp, geor:rcc8ntppi"@en ;
    skos:prefLabel "GeoSPARQL 1.0 Conformance Test: RCC8 Query Rewrite"@en .

conf10qre:sf-query-rewrite a spec:ConformanceTest ;
    spec:testPurpose "check conformance with this requirement"@en ;
    spec:testType spec:Capabilities ;
    rdfs:seeAlso reqs10qre:sf-query-rewrite ;
    skos:definition "Verify that queries involving the following query transformation rules return the correct result for a test dataset when using the specified serialization and version: geor:sfEquals, geor:sfDisjoint, geor:sfIntersects, geor:sfTouches, geor:sfCrosses, geor:sfWithin, geor:sfContains and geor:sfOverlaps"@en ;
    skos:prefLabel "GeoSPARQL 1.0 Conformance Test: SF Query Rewrite"@en .

confs10:topology-extension a spec:ConformanceClass,
        skos:Collection,
        sd:Feature ;
    dcterms:requires confs10:core ;
    skos:member conf10gtx:eh-query-functions,
        conf10gtx:rcc8-query-functions,
        conf10gtx:relate-query-function,
        conf10gtx:sf-query-functions ;
    skos:prefLabel "GeoSPARQL 1.0 Conformance Class: Topology Extension"@en .

reqs10gx:gml-literal-empty a spec:Requirement ;
    skos:definition "An empty geo:gmlLiteral shall be interpreted as an empty geometry"@en ;
    skos:prefLabel "GeoSPARQL 1.0 Requirement: GML Literal Empty"@en ;
    skos:requires reqs10gx:gml-literal .

reqs10gx:gml-profile a spec:Requirement ;
    skos:definition "Implementations shall document supported GML profiles"@en ;
    skos:prefLabel "GeoSPARQL 1.0 Requirement: GML Profile"@en .

reqs10gx:srid-function a spec:Requirement ;
    skos:definition "Implementations shall support geof:getSRID as a SPARQL extension function"@en ;
    skos:prefLabel "GeoSPARQL 1.0 Requirement: SRID Function"@en .

reqs10gx:wkt-axis-order a spec:Requirement ;
    skos:definition "Coordinate tuples within geo:wktLiterals shall be interpreted using the axis order defined in the spatial reference system used"@en ;
    skos:prefLabel "GeoSPARQL 1.0 Requirement: WKT Axis Order"@en .

reqs10gx:wkt-literal-default-srs a spec:Requirement ;
    skos:definition "The URI <http://www.opengis.net/def/crs/OGC/1.3/CRS84> shall be assumed as the spatial reference system for geo:wktLiterals that do not specify an explicit spatial reference system URI" ;
    skos:prefLabel "GeoSPARQL 1.0 Requirement: WKT Literal Default SRS"@en .

reqs10gx:wkt-literal-empty a spec:Requirement ;
    skos:definition "An empty RDFS Literal of type geo:wktLiteral shall be interpreted as an empty geometry"@en ;
    skos:prefLabel "GeoSPARQL 1.0 Requirement: WKT Literal Empty"@en .

reqs10gtx:eh-query-functions a spec:Requirement ;
    skos:definition "Implementations shall support geof:ehEquals, geof:ehDisjoint, geof:ehMeet, geof:ehOverlap, geof:ehCovers, geof:ehCoveredBy, geof:ehInside, geof:ehContains as SPARQL extension functions, consistent with their corresponding DE9IM intersection patterns, as defined by Simple Features [ISO 19125-1]"@en ;
    skos:prefLabel "GeoSPARQL 1.0 Requirement: EH Query Functions"@en .

reqs10gtx:rcc8-query-functions a spec:Requirement ;
    skos:definition "Implementations shall support geof:rcc8eq, geof:rcc8dc, geof:rcc8ec, geof:rcc8po, geof:rcc8tppi, geof:rcc8tpp, geof:rcc8ntpp, geof:rcc8ntppi as SPARQL extension functions, consistent with their corresponding DE-9IM intersection patterns, as defined by Simple Features [ISO 19125-1]"@en ;
    skos:prefLabel "GeoSPARQL 1.0 Requirement: RCC8 Query Functions"@en .

reqs10gtx:relate-query-function a spec:Requirement ;
    skos:definition "Implementations shall support geof:relate as a SPARQL extension function, consistent with the relate operator defined in Simple Features [ISO 19125-1]"@en ;
    skos:prefLabel "GeoSPARQL 1.0 Requirement: Relate Query Function"@en .

reqs10gtx:sf-query-functions a spec:Requirement ;
    skos:definition "Implementations shall support geof:sfEquals, geof:sfDisjoint, geof:sfIntersects, geof:sfTouches, geof:sfCrosses, geof:sfWithin, geof:sfContains, geof:sfOverlaps as  SPARQL extension functions, consistent with their corresponding DE9IM intersection patterns, as defined by Simple Features [ISO 19125-1]"@en ;
    skos:prefLabel "GeoSPARQL 1.0 Requirement: SF Query Functions"@en .

reqs10qre:eh-query-rewrite a spec:Requirement ;
    skos:definition "Basic graph pattern matching shall use the semantics defined by the RIF Core Entailment Regime [W3C SPARQL Entailment] for the RIF rules [W3C RIF Core] geor:ehEquals, geor:ehDisjoint, geor:ehMeet, geor:ehOverlap, geor:ehCovers, geor:ehCoveredBy, geor:ehInside, geor:ehContains"@en ;
    skos:prefLabel "GeoSPARQL 1.0 Requirement: EH Query Rewrite"@en .

reqs10qre:rcc8-query-rewrite a spec:Requirement ;
    skos:definition "Basic graph pattern matching shall use the semantics defined by the RIF Core Entailment Regime [W3C SPARQL Entailment] for the RIF rules [W3C RIF Core] geor:rcc8eq, geor:rcc8dc, geor:rcc8ec, geor:rcc8po, geor:rcc8tppi, geor:rcc8tpp, geor:rcc8ntpp, geor:rcc8ntppi"@en ;
    skos:prefLabel "GeoSPARQL 1.0 Requirement: RCC8 Query Rewrite"@en .

reqs10qre:sf-query-rewrite a spec:Requirement ;
    skos:definition "Basic graph pattern matching shall use the semantics defined by the RIF Core Entailment Regime [W3C SPARQL Entailment] for the RIF rules [W3C RIF Core] geor:sfEquals, geor:sfDisjoint, geor:sfIntersects, geor:sfTouches, geor:sfCrosses, geor:sfWithin, geor:sfContains, geor:sfOverlaps"@en ;
    skos:prefLabel "GeoSPARQL 1.0 Requirement: SF Query Rewrite"@en .

reqs10ree:bgp-rdfs-ent a spec:Requirement ;
    skos:definition "Basic graph pattern matching shall use the semantics defined by the RDFS Entailment Regime [W3C SPARQL Entailment]"@en ;
    skos:prefLabel "GeoSPARQL 1.0 Requirement: BGP RDFS Entailment"@en .

reqs10ree:gml-geometry-types a spec:Requirement ;
    skos:definition "Implementations shall support graph patterns involving terms from an RDFS/OWL class hierarchy of geometry types consistent with the GML schema that implements GM_Object using the specified version of GML [OGC 07-036]"@en ;
    skos:prefLabel "GeoSPARQL 1.0 Requirement: GML Geometry Types"@en .

reqs10ree:wkt-geometry-types a spec:Requirement ;
    skos:definition "Implementations shall support graph patterns involving terms from an RDFS/OWL class hierarchy of geometry types consistent with the one in the specified version of Simple Features [ISO 19125-1]"@en ;
    skos:prefLabel "GeoSPARQL 1.0 Requirement: WKT Geometry Types"@en .

reqs10tve:eh-spatial-relations a spec:Requirement ;
    skos:definition "Implementations shall allow the properties geo:ehEquals, geo:ehDisjoint, geo:ehMeet, geo:ehOverlap, geo:ehCovers, geo:ehCoveredBy, geo:ehInside, geo:ehContains to be used in SPARQL graph patterns"@en ;
    skos:prefLabel "GeoSPARQL 1.0 Requirement: EH Spatial Relations"@en .

reqs10tve:rcc8-spatial-relations a spec:Requirement ;
    skos:definition "Implementations shall allow the properties geo:rcc8eq, geo:rcc8dc, geo:rcc8ec, geo:rcc8po, geo:rcc8tppi, geo:rcc8tpp, geo:rcc8ntpp, geo:rcc8ntppi to be used in SPARQL graph patterns"@en ;
    skos:prefLabel "GeoSPARQL 1.0 Requirement: RCC8 Spatial Relations"@en .

reqs10tve:sf-spatial-relations a spec:Requirement ;
    skos:definition "Implementations shall allow the properties geo:sfEquals, geo:sfDisjoint, geo:sfIntersects, geo:sfTouches, geo:sfCrosses, geo:sfWithin, geo:sfContains, geo:sfOverlaps to be used in SPARQL graph patterns"@en ;
    skos:prefLabel "GeoSPARQL 1.0 Requirement: SF Spatial Relations"@en .

conf11core:feature-collection-class a spec:ConformanceTest ;
    spec:testPurpose "check conformance with this requirement"@en ;
    spec:testType spec:Capabilities ;
    skos:definition "Verify that queries involving geo:FeatureCollection return the correct result on a test dataset"@en ;
    skos:prefLabel "GeoSPARQL 1.1 Conformance Test: Feature Collection Class"@en .

conf11core:sparql-protocol a spec:ConformanceTest ;
    spec:testPurpose "check conformance with this requirement"@en ;
    spec:testType spec:Capabilities ;
    rdfs:seeAlso reqs11core:sparql-protocol ;
    skos:definition "Verify that the implementation accepts SPARQL queries and returns the correct results in the correct format, according to the SPARQL Query Language for RDF, the SPARQL Protocol for RDF and SPARQL Query Results XML Format W3C specifications"@en ;
    skos:prefLabel "GeoSPARQL 1.1 Conformance Test: SPARQL Protocol"@en ;
    prov1:wasDerivedFrom conf10core:sparql-protocol .

conf11core:spatial-object-collection-class a spec:ConformanceTest ;
    spec:testPurpose "check conformance with this requirement"@en ;
    spec:testType spec:Capabilities ;
    skos:definition "Verify that queries involving geo:SpatialObjectCollection return the correct result on a test dataset"@en ;
    skos:prefLabel "GeoSPARQL 1.1 Conformance Test: Spatial Object Collection Class"@en .

conf11core:spatial-object-properties a spec:ConformanceTest ;
    spec:testPurpose "check conformance with this requirement"@en ;
    spec:testType spec:Capabilities ;
    rdfs:seeAlso reqs11core:spatial-object-properties ;
    skos:definition "Verify that queries involving these properties return the correct result for a test dataset"@en ;
    skos:prefLabel "GeoSPARQL 1.1 Conformance Test: Spatial Object Properties"@en .

conf11gx:dggs-literal a spec:ConformanceTest ;
    spec:testPurpose "check conformance with this requirement"@en ;
    spec:testType spec:Capabilities ;
    rdfs:seeAlso reqs11gx:dggs-literal ;
    skos:definition "Verify that queries do not use use this datatype but instead use specializations of it"@en ;
    skos:prefLabel "GeoSPARQL 1.1 Conformance Test: DGGS Literal"@en .

conf11gx:dggs-literal-empty a spec:ConformanceTest ;
    spec:testPurpose "check conformance with this requirement"@en ;
    spec:testType spec:Capabilities ;
    rdfs:seeAlso reqs11gx:dggs-literal-empty ;
    skos:definition "Verify that queries involving empty geo:dggsLiteral values return the correct result for a test dataset"@en ;
    skos:prefLabel "GeoSPARQL 1.1 Conformance Test: DGGS Literal Empty"@en .

conf11gx:feature-properties a spec:ConformanceTest ;
    spec:testPurpose "check conformance with this requirement"@en ;
    spec:testType spec:Capabilities ;
    rdfs:seeAlso reqs11gx:feature-properties ;
    skos:definition "Verify that queries involving these properties return the correct result for a test dataset"@en ;
    skos:prefLabel "GeoSPARQL 1.1 Conformance Test: Feature Properties"@en .

conf11gx:geojson-literal a spec:ConformanceTest ;
    spec:testPurpose "check conformance with this requirement"@en ;
    spec:testType spec:Capabilities ;
    rdfs:seeAlso reqs11gx:geojson-literal ;
    skos:definition "Verify that queries involving geo:geoJSONLiteral values return the correct result for a test dataset"@en ;
    skos:prefLabel "GeoSPARQL 1.1 Conformance Test: GeoJSON Literal"@en .

conf11gx:geojson-literal-empty a spec:ConformanceTest ;
    spec:testPurpose "check conformance with this requirement"@en ;
    spec:testType spec:Capabilities ;
    rdfs:seeAlso reqs11gx:geojson-literal-empty ;
    skos:definition "Verify that queries involving empty geo:kmlLiteral values return the correct result for a test dataset"@en ;
    skos:prefLabel "GeoSPARQL 1.1 Conformance Test: KML Literal Empty"@en .

conf11gx:geojson-literal-srs a spec:ConformanceTest ;
    spec:testPurpose "check conformance with this requirement"@en ;
    spec:testType spec:Capabilities ;
    rdfs:seeAlso reqs11gx:geojson-literal-srs ;
    skos:definition "Verify that queries involving geo:geoJSONLiteral values return the correct result for a test dataset"@en ;
    skos:prefLabel "GeoSPARQL 1.1 Conformance Test: GeoJSON Literal Default SRS"@en .

conf11gx:geometry-as-geojson-literal a spec:ConformanceTest ;
    spec:testPurpose "check conformance with this requirement"@en ;
    spec:testType spec:Capabilities ;
    rdfs:seeAlso reqs11gx:geometry-as-geojson-literal ;
    skos:definition "Verify that queries involving the geo:asGeoJSON property return the correct result for a test dataset"@en ;
    skos:prefLabel "GeoSPARQL 1.1 Conformance Test: Geometry asGeoJSON Literal"@en .

conf11gx:geometry-as-kml-literal a spec:ConformanceTest ;
    spec:testPurpose "check conformance with this requirement"@en ;
    spec:testType spec:Capabilities ;
    rdfs:seeAlso reqs11gx:geometry-as-kml-literal ;
    skos:definition "Verify that queries involving the geo:asKML property return the correct result for a test dataset"@en ;
    skos:prefLabel "GeoSPARQL 1.1 Conformance Test: Geometry asKML Literal"@en .

conf11gx:geometry-properties a spec:ConformanceTest ;
    spec:testPurpose "check conformance with this requirement"@en ;
    spec:testType spec:Capabilities ;
    rdfs:seeAlso reqs11gx:geometry-properties ;
    skos:definition "Verify that queries involving these properties return the correct result for a test dataset"@en ;
    skos:prefLabel "GeoSPARQL 1.1 Conformance Test: Geometry Properties"@en .

conf11gx:kml-literal a spec:ConformanceTest ;
    spec:testPurpose "check conformance with this requirement"@en ;
    spec:testType spec:Capabilities ;
    rdfs:seeAlso reqs11gx:kml-literal ;
    skos:definition "Verify that queries involving geo:kmlLiteral values return the correct result for a test dataset"@en ;
    skos:prefLabel "GeoSPARQL 1.1 Conformance Test: KML Literal"@en .

conf11gx:kml-literal-empty a spec:ConformanceTest ;
    spec:testPurpose "check conformance with this requirement"@en ;
    spec:testType spec:Capabilities ;
    rdfs:seeAlso reqs11gx:kml-literal-empty ;
    skos:definition "Verify that queries involving empty geo:geoJSONLiteral return the correct result for a test dataset"@en ;
    skos:prefLabel "GeoSPARQL 1.1 Conformance Test: GeoJSON Literal Empty"@en .

conf11gx:kml-literal-srs a spec:ConformanceTest ;
    spec:testPurpose "check conformance with this requirement"@en ;
    spec:testType spec:Capabilities ;
    rdfs:seeAlso reqs11gx:kml-literal-srs ;
    skos:definition "Verify that queries involving geo:kmlLiteral values return the correct result for a test dataset"@en ;
    skos:prefLabel "GeoSPARQL 1.1 Conformance Test: KML Literal Default SRS"@en .

confs11:geometry-topology-extension a spec:ConformanceClass,
        skos:Collection,
        sd:Feature ;
    dcterms:requires confs10:geometry-topology-extension,
        confs11:geometry-extension,
        confs11:topology-extension ;
    skos:prefLabel "GeoSPARQL 1.1 Conformance Class: Geometry Topology Extension"@en .

reqs11core:feature-collection-class a spec:Requirement ;
    skos:definition "Implementations shall allow the RDFS class geo:FeatureCollection to be used in SPARQL graph patterns"@en ;
    skos:prefLabel "GeoSPARQL 1.1 Requirement: Feature Collection Class"@en .

reqs11core:geometry-collection-class a spec:Requirement ;
    skos:definition "Implementations shall allow the RDFS class geo:GeometryCollection to be used in SPARQL graph patterns"@en ;
    skos:prefLabel "GeoSPARQL 1.1 Requirement: Geometry Collection Class"@en .

reqs11core:sparql-protocol a spec:Requirement ;
    skos:definition "Implementations shall support the SPARQL Query Language for RDF [SPARQL], the SPARQL Protocol [SPARQLPROT] and the SPARQL Query Results XML [SPARQLRESX] and JSON [SPARQLRESJ] Formats"@en ;
    skos:prefLabel "GeoSPARQL 1.1 Requirement: SPARQL Protocol"@en ;
    prov1:wasDerivedFrom reqs10core:sparql-protocol .

reqs11core:spatial-object-collection-class a spec:Requirement ;
    skos:definition "Implementations shall allow the RDFS class geo:SpatialObjectCollection to be used in SPARQL graph patterns"@en ;
    skos:prefLabel "GeoSPARQL 1.1 Requirement: Spatial Object Collection Class"@en .

reqs11gx:dggs-literal-empty a spec:Requirement ;
    skos:definition "An empty geo:dggsLiteral shall be interpreted as an empty geometry"@en ;
    skos:prefLabel "GeoSPARQL 1.1 Requirement: DGGS Literal Empty"@en .

reqs11gx:geojson-literal-empty a spec:Requirement ;
    skos:definition "An empty geo:kmlLiteral shall be interpreted as an empty geometry"@en ;
    skos:prefLabel "GeoSPARQL 1.1 Requirement: KML Literal Empty"@en .

reqs11gx:geojson-literal-srs a spec:Requirement ;
    skos:definition "RDFS Literals of type geo:geoJSONLiteral do not contain a SRS definition. All literals of this type shall, according to the GeoJSON specification, be encoded only in, and be assumed to use, the WGS84 geodetic longitude-latitude spatial reference system (http://www.opengis.net/def/crs/OGC/1.3/CRS84)"@en ;
    skos:prefLabel "GeoSPARQL 1.1 Requirement: GeoJSON Literal Default SRS"@en .

reqs11gx:geometry-as-dggs-function a spec:Requirement ;
    skos:definition "Implementations shall support geof:asDGGS, as a SPARQL extension function"@en ;
    skos:prefLabel "GeoSPARQL 1.1 Requirement: asDGGS Function"@en .

reqs11gx:geometry-as-geojson-function a spec:Requirement ;
    skos:definition "Implementations shall support geof:asGeoJSON, as a SPARQL extension function"@en ;
    skos:prefLabel "GeoSPARQL 1.1 Requirement: asGeoJSON Function"@en .

reqs11gx:geometry-as-gml-function a spec:Requirement ;
    skos:definition "Implementations shall support geof:asGML, as a SPARQL extension function"@en ;
    skos:prefLabel "GeoSPARQL 1.1 Requirement: asGML Function"@en .

reqs11gx:geometry-as-kml-function a spec:Requirement ;
    skos:definition "Implementations shall support geof:asKML, as a SPARQL extension function"@en ;
    skos:prefLabel "GeoSPARQL 1.1 Requirement: asKML Function"@en .

reqs11gx:geometry-as-wkt-function a spec:Requirement ;
    skos:definition "Implementations shall support geof:asWKT, as a SPARQL extension function"@en ;
    skos:prefLabel "GeoSPARQL 1.1 Requirement: asWKT Function"@en .

reqs11gx:kml-literal-empty a spec:Requirement ;
    skos:definition "An empty geo:geoJSONLiteral shall be interpreted as an empty geometry"@en ;
    skos:prefLabel "GeoSPARQL 1.1 Requirement: GeoJSON Literal Empty"@en .

reqs11gx:kml-literal-srs a spec:Requirement ;
    skos:definition "The IRI http://www.opengis.net/def/crs/OGC/1.3/CRS84 shall be assumed as the SRS for geo:kmlLiterals that do not specify an explicit SRS IRI"@en ;
    skos:prefLabel "GeoSPARQL 1.1 Requirement: KML Literal Default SRS"@en .

reqs11gx:query-functions-dggs a spec:Requirement ;
    skos:definition "Implementations shall support the functions of Requirement 40 for DGGS geometry literals as SPARQL extension functions, consistent with definitions of these functions in Simple Features <<ISO19125-1>>, for non-DGGS geometry literals"@en ;
    skos:prefLabel "GeoSPARQL 1.1 Requirement: Query Functions"@en ;
    prov1:wasDerivedFrom reqs10gx:query-functions .

reqs11gx:query-functions-non-sf a spec:Requirement ;
    skos:definition "Implementations shall support the functions geof:area, geof:geometryN, geof:length, geof:maxX, geof:maxY, geof:maxZ, geof:minX, geof:minY, geof:minZ, geof:numGeometries and geof:projectTo as SPARQL extension functions which are defined in this standard, for non-DGGS geometry literals"@en ;
    skos:prefLabel "GeoSPARQL 1.1 Requirement: Query Functions"@en ;
    prov1:wasDerivedFrom reqs10gx:query-functions .

reqs11gx:query-functions-non-sf-dggs a spec:Requirement ;
    skos:definition "Implementations shall support the functions of Requirement 41 for DGGS geometry literals as SPARQL extension functions which are defined in this standard, for non-DGGS geometry literals"@en ;
    skos:prefLabel "GeoSPARQL 1.1 Requirement: Query Functions"@en ;
    prov1:wasDerivedFrom reqs10gx:query-functions .

funcs:asDGGS a skos:Concept,
        sd:Function,
        fno:Function ;
    dcterms:source <http://www.opengis.net/doc/geosparql/1.1> ;
    policy:status status:valid ;
    rdfs:isDefinedBy reqs11gx:geometry-as-dggs-function ;
    rdfs:seeAlso <http://www.opengis.net/doc/geosparql/1.1> ;
    skos:definition "Converts a given geometry to an equivalent DGGS representation, formulated according to the specific DGGS literal indicated using the specificDggsDatatype parameter."@en ;
    skos:prefLabel "asDGGS"@en ;
    fno:expects ( funcs:asDGGS_param1 funcs:asDGGS_param2 ) ;
    fno:returns ( funcs:asDGGS_output ) .

funcs:asGML a skos:Concept,
        sd:Function,
        fno:Function ;
    dcterms:source <http://www.opengis.net/doc/geosparql/1.1> ;
    policy:status status:valid ;
    rdfs:isDefinedBy reqs11gx:geometry-as-gml-function ;
    rdfs:seeAlso <http://www.opengis.net/doc/geosparql/1.1> ;
    skos:definition "Converts a given geometry to an equivalent GML representation defined by a gmlProfile version string preserving the coordinate reference system."@en ;
    skos:prefLabel "asGML"@en ;
    fno:expects ( funcs:asGML_param1 funcs:asGML_param2 ) ;
    fno:returns ( funcs:asGML_output ) .

funcs:asGeoJSON a skos:Concept,
        sd:Function,
        fno:Function ;
    dcterms:contributor "Timo Homburg" ;
    dcterms:creator "OGC GeoSPARQL 2.0 Standard Working Group" ;
    dcterms:date "2021-05-20"^^xsd:date ;
    dcterms:source <http://www.opengis.net/doc/geosparql/1.1> ;
    policy:status status:valid ;
    rdfs:isDefinedBy reqs11gx:geometry-as-geojson-function ;
    rdfs:seeAlso <http://www.opengis.net/doc/geosparql/1.1> ;
    skos:definition "Converts a given geometry to an equivalent GeoJSON representation. Coordinates are converted to the CRS84 coordinate system, the only valid coordinate system to be used in a GeoJSON literal."@en ;
    skos:prefLabel "asGeoJSON"@en ;
    fno:expects ( funcs:asGeoJSON_param1 ) ;
    fno:returns ( funcs:asGeoJSON_output ) .

funcs:asKML a skos:Concept,
        sd:Function,
        fno:Function ;
    dcterms:source <http://www.opengis.net/doc/geosparql/1.1> ;
    policy:status status:valid ;
    rdfs:isDefinedBy reqs11gx:geometry-as-kml-function ;
    rdfs:seeAlso <http://www.opengis.net/doc/geosparql/1.1> ;
    skos:definition "Converts a given geometry to an equivalent KML representation. Coordinates are converted to the CRS84 coordinate system, the only valid coordinate system to be used in a KML literal."@en ;
    skos:prefLabel "asKML"@en ;
    fno:expects ( funcs:asKML_param1 ) ;
    fno:returns ( funcs:asKML_output ) .

funcs:asWKT a skos:Concept,
        sd:Function,
        fno:Function ;
    dcterms:source <http://www.opengis.net/doc/geosparql/1.1> ;
    policy:status status:valid ;
    rdfs:isDefinedBy reqs11gx:geometry-as-wkt-function ;
    rdfs:seeAlso <http://www.opengis.net/doc/geosparql/1.1> ;
    skos:definition "Converts a given geometry to an equivalent WKT representation preserving the coordinate reference system and geometry type, if possible."@en ;
    skos:prefLabel "asWKT"@en ;
    fno:expects ( funcs:asWKT_param1 ) ;
    fno:returns ( funcs:asWKT_output ) .

funcs:geometryN a skos:Concept,
        sd:Function,
        fno:Function ;
    dcterms:source <http://www.opengis.net/doc/geosparql/1.1> ;
    policy:status status:valid ;
    rdfs:isDefinedBy reqs11gx:query-functions ;
    rdfs:seeAlso <http://www.opengis.net/doc/geosparql/1.1> ;
    skos:definition "A query function that returns the the nth geometry if the given geometry literal contains a GeometryCollection."@en ;
    skos:prefLabel "geometryN"@en ;
    fno:expects ( funcs:geometryN_param1 funcs:geometryN_param2 ) ;
    fno:returns ( funcs:geometryN_output ) .

funcs:length a skos:Concept,
        sd:Function,
        fno:Function ;
    dcterms:source <http://www.opengis.net/doc/geosparql/1.1> ;
    policy:status status:valid ;
    rdfs:isDefinedBy reqs11gx:query-functions ;
    rdfs:seeAlso <http://www.opengis.net/doc/geosparql/1.1> ;
    skos:definition "Returns the length of a geometry in meters."@en ;
    skos:prefLabel "length"@en ;
    fno:expects ( funcs:length_param1 funcs:length_param2 ) ;
    fno:returns ( funcs:length_output ) .

funcs:maxx a skos:Concept,
        sd:Function,
        fno:Function ;
    dcterms:source <http://www.opengis.net/doc/geosparql/1.1> ;
    policy:status status:valid ;
    rdfs:isDefinedBy reqs11gx:sa-functions ;
    rdfs:seeAlso <http://www.opengis.net/doc/geosparql/1.1> ;
    skos:definition "A query function that returns the maximum x coordinate of the input geometry."@en ;
    skos:prefLabel "maxX"@en ;
    skos:scopeNote "X indicates the first dimension as indicated by the spatial reference system"@en ;
    fno:expects ( funcs:maxx_param1 ) ;
    fno:returns ( funcs:maxx_output ) .

funcs:maxy a skos:Concept,
        sd:Function,
        fno:Function ;
    dcterms:source <http://www.opengis.net/doc/geosparql/1.1> ;
    policy:status status:valid ;
    rdfs:isDefinedBy reqs11gx:sa-functions ;
    rdfs:seeAlso <http://www.opengis.net/doc/geosparql/1.1> ;
    skos:definition "A query function that returns the maximum y coordinate of the input geometry."@en ;
    skos:prefLabel "maxY"@en ;
    skos:scopeNote "Y indicates the second dimension as indicated by the spatial reference system"@en ;
    fno:expects ( funcs:maxy_param1 ) ;
    fno:returns ( funcs:maxy_output ) .

funcs:maxz a skos:Concept,
        sd:Function,
        fno:Function ;
    dcterms:source <http://www.opengis.net/doc/geosparql/1.1> ;
    policy:status status:valid ;
    rdfs:isDefinedBy reqs11gx:sa-functions ;
    rdfs:seeAlso <http://www.opengis.net/doc/geosparql/1.1> ;
    skos:definition "A query function that returns the maximum z coordinate of the input geometry."@en ;
    skos:prefLabel "maxZ"@en ;
    skos:scopeNote "Z indicates the third dimension as indicated by the spatial reference system"@en ;
    fno:expects ( funcs:maxz_param1 ) ;
    fno:returns ( funcs:maxz_output ) .

funcs:metricArea a skos:Concept,
        sd:Function,
        fno:Function ;
    dcterms:source <http://www.opengis.net/doc/geosparql/1.1> ;
    policy:status status:valid ;
    rdfs:isDefinedBy reqs11gx:query-functions ;
    rdfs:seeAlso <http://www.opengis.net/doc/geosparql/1.1> ;
    skos:definition "Returns the area of a geometry in squaremeters."@en ;
    skos:prefLabel "metric area"@en ;
    fno:expects ( funcs:metricArea_param1 ) ;
    fno:returns ( funcs:metricArea_output ) .

funcs:metricPerimeter a skos:Concept,
        sd:Function,
        fno:Function ;
    dcterms:source <http://www.opengis.net/doc/geosparql/1.1> ;
    policy:status status:valid ;
    rdfs:isDefinedBy reqs11gx:query-functions ;
    rdfs:seeAlso <http://www.opengis.net/doc/geosparql/1.1> ;
    skos:definition "Returns the perimeter of a geometry in meters."@en ;
    skos:prefLabel "metric perimeter"@en ;
    fno:expects ( funcs:metricPerimeter_param1 ) ;
    fno:returns ( funcs:metricPerimeter_output ) .

funcs:minx a skos:Concept,
        sd:Function,
        fno:Function ;
    dcterms:source <http://www.opengis.net/doc/geosparql/1.1> ;
    policy:status status:valid ;
    rdfs:isDefinedBy reqs11gx:sa-functions ;
    rdfs:seeAlso <http://www.opengis.net/doc/geosparql/1.1> ;
    skos:definition "A query function that returns the minimum x coordinate of the input geometry."@en ;
    skos:prefLabel "minX"@en ;
    skos:scopeNote "X indicates the first dimension as indicated by the spatial reference system"@en ;
    fno:expects ( funcs:minx_param1 ) ;
    fno:returns ( funcs:minx_output ) .

funcs:miny a skos:Concept,
        sd:Function,
        fno:Function ;
    dcterms:source <http://www.opengis.net/doc/geosparql/1.1> ;
    policy:status status:valid ;
    rdfs:isDefinedBy reqs11gx:sa-functions ;
    rdfs:seeAlso <http://www.opengis.net/doc/geosparql/1.1> ;
    skos:definition "A query function that returns the minimum y coordinate of the input geometry."@en ;
    skos:prefLabel "minY"@en ;
    skos:scopeNote "Y indicates the second dimension as indicated by the spatial reference system"@en ;
    fno:expects ( funcs:miny_param1 ) ;
    fno:returns ( funcs:miny_output ) .

funcs:minz a skos:Concept,
        sd:Function,
        fno:Function ;
    dcterms:source <http://www.opengis.net/doc/geosparql/1.1> ;
    policy:status status:valid ;
    rdfs:isDefinedBy reqs11gx:sa-functions ;
    rdfs:seeAlso <http://www.opengis.net/doc/geosparql/1.1> ;
    skos:definition "A query function that returns the minimum z coordinate of the input geometry."@en ;
    skos:prefLabel "minZ"@en ;
    skos:scopeNote "Z indicates the third dimension as indicated by the spatial reference system"@en ;
    fno:expects ( funcs:minz_param1 ) ;
    fno:returns ( funcs:minz_output ) .

funcs:numGeometries a skos:Concept,
        sd:Function,
        fno:Function ;
    dcterms:source <http://www.opengis.net/doc/geosparql/1.1> ;
    policy:status status:valid ;
    rdfs:isDefinedBy reqs11gx:query-functions ;
    rdfs:seeAlso <http://www.opengis.net/doc/geosparql/1.1> ;
    skos:definition "A query function that returns the number of geometries if the given geometry literal contains a GeometryCollection."@en ;
    skos:prefLabel "numGeometries"@en ;
    fno:expects ( funcs:numGeometries_param1 ) ;
    fno:returns ( funcs:numGeometries_output ) .

funcs:perimeter a skos:Concept,
        sd:Function,
        fno:Function ;
    dcterms:source <http://www.opengis.net/doc/geosparql/1.1> ;
    policy:status status:valid ;
    rdfs:isDefinedBy reqs11gx:query-functions ;
    rdfs:seeAlso <http://www.opengis.net/doc/geosparql/1.1> ;
    skos:definition "Returns the perimeter of a geometry in meters."@en ;
    skos:prefLabel "perimeter"@en ;
    fno:expects ( funcs:perimeter_param1 funcs:perimeter_param2 ) ;
    fno:returns ( funcs:perimeter_output ) .

rules:ehContains a skos:Concept ;
    dcterms:contributor "Matthew Perry" ;
    dcterms:creator "OGC GeoSPARQL 1.0 Standard Working Group" ;
    dcterms:date "2011-06-16"^^xsd:date ;
    dcterms:source <http://www.opengis.net/doc/geosparql/1.0>,
        <http://www.opengis.net/doc/geosparql/1.1> ;
    policy:status status:valid ;
    rdfs:isDefinedBy <http://www.opengis.net/spec/geosparql/1.0>,
        <http://www.opengis.net/spec/geosparql/1.1/req/query-rewrite-extension/eh-query-rewrite> ;
    rdfs:seeAlso <http://www.opengis.net/doc/geosparql/1.0>,
        <http://www.opengis.net/doc/geosparql/1.1> ;
    skos:definition "A query rewrite rule used to determine if one spatial object contains another spatial object based on their associated primary geometry objects."@en ;
    skos:prefLabel "contains"@en .

rules:ehCoveredBy a skos:Concept ;
    dcterms:contributor "Matthew Perry" ;
    dcterms:creator "OGC GeoSPARQL 1.0 Standard Working Group" ;
    dcterms:date "2011-06-16"^^xsd:date ;
    dcterms:source <http://www.opengis.net/doc/geosparql/1.0>,
        <http://www.opengis.net/doc/geosparql/1.1> ;
    policy:status status:valid ;
    rdfs:isDefinedBy <http://www.opengis.net/spec/geosparql/1.0>,
        <http://www.opengis.net/spec/geosparql/1.1/req/query-rewrite-extension/eh-query-rewrite> ;
    rdfs:seeAlso <http://www.opengis.net/doc/geosparql/1.0>,
        <http://www.opengis.net/doc/geosparql/1.1> ;
    skos:definition "A query rewrite rule used to determine if one spatial object is covered by another spatial object based on their associated primary geometry objects."@en ;
    skos:prefLabel "covered by"@en .

rules:ehCovers a skos:Concept ;
    dcterms:contributor "Matthew Perry" ;
    dcterms:creator "OGC GeoSPARQL 1.0 Standard Working Group" ;
    dcterms:date "2011-06-16"^^xsd:date ;
    dcterms:source <http://www.opengis.net/doc/geosparql/1.0>,
        <http://www.opengis.net/doc/geosparql/1.1> ;
    policy:status status:valid ;
    rdfs:isDefinedBy <http://www.opengis.net/spec/geosparql/1.0>,
        <http://www.opengis.net/spec/geosparql/1.1/req/query-rewrite-extension/eh-query-rewrite> ;
    rdfs:seeAlso <http://www.opengis.net/doc/geosparql/1.0>,
        <http://www.opengis.net/doc/geosparql/1.1> ;
    skos:definition "A query rewrite rule used to determine if one spatial object covers another spatial object based on their associated primary geometry objects."@en ;
    skos:prefLabel "covers"@en .

rules:ehDisjoint a skos:Concept ;
    dcterms:contributor "Matthew Perry" ;
    dcterms:creator "OGC GeoSPARQL 1.0 Standard Working Group" ;
    dcterms:date "2011-06-16"^^xsd:date ;
    dcterms:source <http://www.opengis.net/doc/geosparql/1.0>,
        <http://www.opengis.net/doc/geosparql/1.1> ;
    policy:status status:valid ;
    rdfs:isDefinedBy <http://www.opengis.net/spec/geosparql/1.0>,
        <http://www.opengis.net/spec/geosparql/1.1/req/query-rewrite-extension/eh-query-rewrite> ;
    rdfs:seeAlso <http://www.opengis.net/doc/geosparql/1.0>,
        <http://www.opengis.net/doc/geosparql/1.1> ;
    skos:definition "A query rewrite rule used to determine if two spatial objects are disjoint based on their associated primary geometry objects."@en ;
    skos:prefLabel "disjoint"@en .

rules:ehEquals a skos:Concept ;
    dcterms:contributor "Matthew Perry" ;
    dcterms:creator "OGC GeoSPARQL 1.0 Standard Working Group" ;
    dcterms:date "2011-06-16"^^xsd:date ;
    dcterms:source <http://www.opengis.net/doc/geosparql/1.0>,
        <http://www.opengis.net/doc/geosparql/1.1> ;
    policy:status status:valid ;
    rdfs:isDefinedBy <http://www.opengis.net/spec/geosparql/1.0>,
        <http://www.opengis.net/spec/geosparql/1.1/req/query-rewrite-extension/eh-query-rewrite> ;
    rdfs:seeAlso <http://www.opengis.net/doc/geosparql/1.0>,
        <http://www.opengis.net/doc/geosparql/1.1> ;
    skos:definition "A query rewrite rule used to determine if two spatial objects are equal based on their associated primary geometry objects."@en ;
    skos:prefLabel "equals"@en .

rules:ehInside a skos:Concept ;
    dcterms:contributor "Matthew Perry" ;
    dcterms:creator "OGC GeoSPARQL 1.0 Standard Working Group" ;
    dcterms:date "2011-06-16"^^xsd:date ;
    dcterms:source <http://www.opengis.net/doc/geosparql/1.0>,
        <http://www.opengis.net/doc/geosparql/1.1> ;
    policy:status status:valid ;
    rdfs:isDefinedBy <http://www.opengis.net/spec/geosparql/1.0>,
        <http://www.opengis.net/spec/geosparql/1.1/req/query-rewrite-extension/eh-query-rewrite> ;
    rdfs:seeAlso <http://www.opengis.net/doc/geosparql/1.0>,
        <http://www.opengis.net/doc/geosparql/1.1> ;
    skos:definition "A query rewrite rule used to determine if one spatial object is inside another spatial object based on their associated primary geometry objects."@en ;
    skos:prefLabel "inside"@en .

rules:ehMeet a skos:Concept ;
    dcterms:contributor "Matthew Perry" ;
    dcterms:creator "OGC GeoSPARQL 1.0 Standard Working Group" ;
    dcterms:date "2011-06-16"^^xsd:date ;
    dcterms:source <http://www.opengis.net/doc/geosparql/1.0>,
        <http://www.opengis.net/doc/geosparql/1.1> ;
    policy:status status:valid ;
    rdfs:isDefinedBy <http://www.opengis.net/spec/geosparql/1.0>,
        <http://www.opengis.net/spec/geosparql/1.1/req/query-rewrite-extension/eh-query-rewrite> ;
    rdfs:seeAlso <http://www.opengis.net/doc/geosparql/1.0>,
        <http://www.opengis.net/doc/geosparql/1.1> ;
    skos:definition "A query rewrite rule used to determine if two spatial objects meet based on their associated primary geometry objects."@en ;
    skos:prefLabel "meet"@en .

rules:ehOverlap a skos:Concept ;
    dcterms:contributor "Matthew Perry" ;
    dcterms:creator "OGC GeoSPARQL 1.0 Standard Working Group" ;
    dcterms:date "2011-06-16"^^xsd:date ;
    dcterms:source <http://www.opengis.net/doc/geosparql/1.0>,
        <http://www.opengis.net/doc/geosparql/1.1> ;
    policy:status status:valid ;
    rdfs:isDefinedBy <http://www.opengis.net/spec/geosparql/1.0>,
        <http://www.opengis.net/spec/geosparql/1.1/req/query-rewrite-extension/eh-query-rewrite> ;
    rdfs:seeAlso <http://www.opengis.net/doc/geosparql/1.0>,
        <http://www.opengis.net/doc/geosparql/1.1> ;
    skos:definition "A query rewrite rule used to determine if two spatial objects overlap based on their associated primary geometry objects."@en ;
    skos:prefLabel "overlap"@en .

rules:rcc8dc a skos:Concept ;
    dcterms:contributor "Matthew Perry" ;
    dcterms:creator "OGC GeoSPARQL 1.0 Standard Working Group" ;
    dcterms:date "2011-06-16"^^xsd:date ;
    dcterms:source <http://www.opengis.net/doc/geosparql/1.0>,
        <http://www.opengis.net/doc/geosparql/1.1> ;
    policy:status status:valid ;
    rdfs:isDefinedBy <http://www.opengis.net/spec/geosparql/1.0>,
        <http://www.opengis.net/spec/geosparql/1.1/req/query-rewrite-extension/rcc8-query-rewrite> ;
    rdfs:seeAlso <http://www.opengis.net/doc/geosparql/1.0>,
        <http://www.opengis.net/doc/geosparql/1.1> ;
    skos:definition "A query rewrite rule used to determine if two spatial objects are disjoint based on their associated primary geometry objects."@en ;
    skos:prefLabel "disconnected"@en .

rules:rcc8ec a skos:Concept ;
    dcterms:contributor "Matthew Perry" ;
    dcterms:creator "OGC GeoSPARQL 1.0 Standard Working Group" ;
    dcterms:date "2011-06-16"^^xsd:date ;
    dcterms:source <http://www.opengis.net/doc/geosparql/1.0>,
        <http://www.opengis.net/doc/geosparql/1.1> ;
    policy:status status:valid ;
    rdfs:isDefinedBy <http://www.opengis.net/spec/geosparql/1.0>,
        <http://www.opengis.net/spec/geosparql/1.1/req/query-rewrite-extension/rcc8-query-rewrite> ;
    rdfs:seeAlso <http://www.opengis.net/doc/geosparql/1.0>,
        <http://www.opengis.net/doc/geosparql/1.1> ;
    skos:definition "A query rewrite rule used to determine if two spatial objects are externally connected based on their associated primary geometry objects."@en ;
    skos:prefLabel "externally connected"@en .

rules:rcc8eq a skos:Concept ;
    dcterms:contributor "Matthew Perry" ;
    dcterms:creator "OGC GeoSPARQL 1.0 Standard Working Group" ;
    dcterms:date "2011-06-16"^^xsd:date ;
    dcterms:source <http://www.opengis.net/doc/geosparql/1.0>,
        <http://www.opengis.net/doc/geosparql/1.1> ;
    policy:status status:valid ;
    rdfs:isDefinedBy <http://www.opengis.net/spec/geosparql/1.0>,
        <http://www.opengis.net/spec/geosparql/1.1/req/query-rewrite-extension/rcc8-query-rewrite> ;
    rdfs:seeAlso <http://www.opengis.net/doc/geosparql/1.0>,
        <http://www.opengis.net/doc/geosparql/1.1> ;
    skos:definition "A query rewrite rule used to determine two spatial objects are equal based on their associated primary geometry objects."@en ;
    skos:prefLabel "equals"@en .

rules:rcc8ntpp a skos:Concept ;
    dcterms:contributor "Matthew Perry" ;
    dcterms:creator "OGC GeoSPARQL 1.0 Standard Working Group" ;
    dcterms:date "2011-06-16"^^xsd:date ;
    dcterms:source <http://www.opengis.net/doc/geosparql/1.0>,
        <http://www.opengis.net/doc/geosparql/1.1> ;
    policy:status status:valid ;
    rdfs:isDefinedBy <http://www.opengis.net/spec/geosparql/1.0>,
        <http://www.opengis.net/spec/geosparql/1.1/req/query-rewrite-extension/rcc8-query-rewrite> ;
    rdfs:seeAlso <http://www.opengis.net/doc/geosparql/1.0>,
        <http://www.opengis.net/spec/geosparql/1.1> ;
    skos:definition "A query rewrite rule used to determine if one spatial object is a non-tangential proper part of another spatial object based on their associated primary geometry objects."@en ;
    skos:prefLabel "non-tangential proper part"@en .

rules:rcc8ntppi a skos:Concept ;
    dcterms:contributor "Matthew Perry" ;
    dcterms:creator "OGC GeoSPARQL 1.0 Standard Working Group" ;
    dcterms:date "2011-06-16"^^xsd:date ;
    dcterms:source <http://www.opengis.net/doc/geosparql/1.0>,
        <http://www.opengis.net/doc/geosparql/1.1> ;
    policy:status status:valid ;
    rdfs:isDefinedBy <http://www.opengis.net/spec/geosparql/1.0>,
        <http://www.opengis.net/spec/geosparql/1.1/req/query-rewrite-extension/rcc8-query-rewrite> ;
    rdfs:seeAlso <http://www.opengis.net/doc/geosparql/1.0>,
        <http://www.opengis.net/doc/geosparql/1.1> ;
    skos:definition "A query rewrite rule used to determine if one spatial object is a non-tangential proper part inverse of another spatial object based on their associated primary geometry objects."@en ;
    skos:prefLabel "non-tangential proper part inverse"@en .

rules:rcc8po a skos:Concept ;
    dcterms:contributor "Matthew Perry" ;
    dcterms:creator "OGC GeoSPARQL 1.0 Standard Working Group" ;
    dcterms:date "2011-06-16"^^xsd:date ;
    dcterms:source <http://www.opengis.net/doc/geosparql/1.0>,
        <http://www.opengis.net/doc/geosparql/1.1> ;
    policy:status status:valid ;
    rdfs:isDefinedBy <http://www.opengis.net/spec/geosparql/1.0>,
        <http://www.opengis.net/spec/geosparql/1.1/req/query-rewrite-extension/rcc8-query-rewrite> ;
    rdfs:seeAlso <http://www.opengis.net/doc/geosparql/1.0>,
        <http://www.opengis.net/doc/geosparql/1.1> ;
    skos:definition "A query rewrite rule used to determine if two spatial objects partially overlap based on their associated primary geometry objects."@en ;
    skos:prefLabel "partially overlapping"@en .

rules:rcc8tpp a skos:Concept ;
    dcterms:contributor "Matthew Perry" ;
    dcterms:creator "OGC GeoSPARQL 1.0 Standard Working Group" ;
    dcterms:date "2011-06-16"^^xsd:date ;
    dcterms:source <http://www.opengis.net/doc/geosparql/1.0>,
        <http://www.opengis.net/doc/geosparql/1.1> ;
    policy:status status:valid ;
    rdfs:isDefinedBy <http://www.opengis.net/spec/geosparql/1.0>,
        <http://www.opengis.net/spec/geosparql/1.1/req/query-rewrite-extension/rcc8-query-rewrite> ;
    rdfs:seeAlso <http://www.opengis.net/doc/geosparql/1.0>,
        <http://www.opengis.net/doc/geosparql/1.1> ;
    skos:definition "A query rewrite rule used to determine if one spatial object is a tangential proper part of another spatial object based on their associated geometry objects."@en ;
    skos:prefLabel "tangential proper part"@en .

rules:rcc8tppi a skos:Concept ;
    dcterms:contributor "Matthew Perry" ;
    dcterms:creator "OGC GeoSPARQL 1.0 Standard Working Group" ;
    dcterms:date "2011-06-16"^^xsd:date ;
    dcterms:source <http://www.opengis.net/doc/geosparql/1.0>,
        <http://www.opengis.net/doc/geosparql/1.1> ;
    policy:status status:valid ;
    rdfs:isDefinedBy <http://www.opengis.net/spec/geosparql/1.0>,
        <http://www.opengis.net/spec/geosparql/1.1/req/query-rewrite-extension/rcc8-query-rewrite> ;
    rdfs:seeAlso <http://www.opengis.net/doc/geosparql/1.0>,
        <http://www.opengis.net/doc/geosparql/1.1> ;
    skos:definition "A query rewrite rule used to determine if one spatial object is a tangential proper part inverse of another spatial object based on their associated primary geometry objects."@en ;
    skos:prefLabel "tangential proper part inverse"@en .

rules:sfContains a skos:Concept ;
    dcterms:contributor "Matthew Perry" ;
    dcterms:creator "OGC GeoSPARQL 1.0 Standard Working Group" ;
    dcterms:date "2011-06-16"^^xsd:date ;
    dcterms:source <http://www.opengis.net/doc/geosparql/1.0>,
        <http://www.opengis.net/doc/geosparql/1.1> ;
    policy:status status:valid ;
    rdfs:isDefinedBy <http://www.opengis.net/spec/geosparql/1.0>,
        <http://www.opengis.net/spec/geosparql/1.1/req/query-rewrite-extension/sf-query-rewrite> ;
    rdfs:seeAlso <http://www.opengis.net/doc/geosparql/1.0>,
        <http://www.opengis.net/doc/geosparql/1.1> ;
    skos:definition "A query rewrite rule used to determine if one spatial object contains another spatial object based on their associated primary geometry objects."@en ;
    skos:prefLabel "contains"@en .

rules:sfCrosses a skos:Concept ;
    dcterms:contributor "Matthew Perry" ;
    dcterms:creator "OGC GeoSPARQL 1.0 Standard Working Group" ;
    dcterms:date "2011-06-16"^^xsd:date ;
    dcterms:source <http://www.opengis.net/doc/geosparql/1.0>,
        <http://www.opengis.net/doc/geosparql/1.1> ;
    policy:status status:valid ;
    rdfs:isDefinedBy <http://www.opengis.net/spec/geosparql/1.0>,
        <http://www.opengis.net/spec/geosparql/1.1/req/query-rewrite-extension/sf-query-rewrite> ;
    rdfs:seeAlso <http://www.opengis.net/doc/geosparql/1.0>,
        <http://www.opengis.net/doc/geosparql/1.1> ;
    skos:definition "A query rewrite rule used to determine if two spatial objects cross based their associated primary geometry objects."@en ;
    skos:prefLabel "crosses"@en .

rules:sfDisjoint a skos:Concept ;
    dcterms:contributor "Matthew Perry" ;
    dcterms:creator "OGC GeoSPARQL 1.0 Standard Working Group" ;
    dcterms:date "2011-06-16"^^xsd:date ;
    dcterms:source <http://www.opengis.net/doc/geosparql/1.0>,
        <http://www.opengis.net/doc/geosparql/1.1> ;
    policy:status status:valid ;
    rdfs:isDefinedBy <http://www.opengis.net/spec/geosparql/1.0>,
        <http://www.opengis.net/spec/geosparql/1.1/req/query-rewrite-extension/sf-query-rewrite> ;
    rdfs:seeAlso <http://www.opengis.net/doc/geosparql/1.0>,
        <http://www.opengis.net/doc/geosparql/1.1> ;
    skos:definition "A query rewrite rule used to determine if two spatial objects are disjoint based on their associated primary geometry objects."@en ;
    skos:prefLabel "disjoint"@en .

rules:sfEquals a skos:Concept ;
    dcterms:contributor "Matthew Perry" ;
    dcterms:creator "OGC GeoSPARQL 1.0 Standard Working Group" ;
    dcterms:date "2011-06-16"^^xsd:date ;
    dcterms:source <http://www.opengis.net/doc/geosparql/1.0>,
        <http://www.opengis.net/doc/geosparql/1.1> ;
    policy:status status:valid ;
    rdfs:isDefinedBy <http://www.opengis.net/spec/geosparql/1.0>,
        <http://www.opengis.net/spec/geosparql/1.1/req/query-rewrite-extension/sf-query-rewrite> ;
    rdfs:seeAlso <http://www.opengis.net/doc/geosparql/1.0>,
        <http://www.opengis.net/doc/geosparql/1.1> ;
    skos:definition "A query rewrite rule used to determine if two spatial objects are equal based on their associated primary geometry objects."@en ;
    skos:prefLabel "equals"@en .

rules:sfIntersects a skos:Concept ;
    dcterms:contributor "Matthew Perry" ;
    dcterms:creator "OGC GeoSPARQL 1.0 Standard Working Group" ;
    dcterms:date "2011-06-16"^^xsd:date ;
    dcterms:source <http://www.opengis.net/doc/geosparql/1.0>,
        <http://www.opengis.net/doc/geosparql/1.1> ;
    policy:status status:valid ;
    rdfs:isDefinedBy <http://www.opengis.net/spec/geosparql/1.0>,
        <http://www.opengis.net/spec/geosparql/1.1/req/query-rewrite-extension/sf-query-rewrite> ;
    rdfs:seeAlso <http://www.opengis.net/doc/geosparql/1.0>,
        <http://www.opengis.net/doc/geosparql/1.1> ;
    skos:definition "A query rewrite rule used to determine if two spatial objects intersect based on their associated primary geometry objects."@en ;
    skos:prefLabel "intersects"@en .

rules:sfOverlaps a skos:Concept ;
    dcterms:contributor "Matthew Perry" ;
    dcterms:creator "OGC GeoSPARQL 1.0 Standard Working Group" ;
    dcterms:date "2011-06-16"^^xsd:date ;
    dcterms:source <http://www.opengis.net/doc/geosparql/1.0>,
        <http://www.opengis.net/doc/geosparql/1.1> ;
    policy:status status:valid ;
    rdfs:isDefinedBy <http://www.opengis.net/spec/geosparql/1.0>,
        <http://www.opengis.net/spec/geosparql/1.1/req/query-rewrite-extension/sf-query-rewrite> ;
    rdfs:seeAlso <http://www.opengis.net/doc/geosparql/1.0>,
        <http://www.opengis.net/doc/geosparql/1.1> ;
    skos:definition "A query rewrite rule used to determine if two spatial objects overlap based on their associated primary geometry objects."@en ;
    skos:example spec11:B.2.2.5 ;
    skos:prefLabel "overlaps"@en .

rules:sfTouches a skos:Concept ;
    dcterms:contributor "Matthew Perry" ;
    dcterms:creator "OGC GeoSPARQL 1.0 Standard Working Group" ;
    dcterms:date "2011-06-16"^^xsd:date ;
    dcterms:source <http://www.opengis.net/doc/geosparql/1.0>,
        <http://www.opengis.net/doc/geosparql/1.1> ;
    policy:status status:valid ;
    rdfs:isDefinedBy <http://www.opengis.net/spec/geosparql/1.0>,
        <http://www.opengis.net/spec/geosparql/1.1/req/query-rewrite-extension/sf-query-rewrite> ;
    rdfs:seeAlso <http://www.opengis.net/doc/geosparql/1.0>,
        <http://www.opengis.net/doc/geosparql/1.1> ;
    skos:definition "A query rewrite rule used to determine if two spatial objects touch based on their associated primary geometry objects."@en ;
    skos:prefLabel "touches"@en .

rules:sfWithin a skos:Concept ;
    dcterms:contributor "Matthew Perry" ;
    dcterms:creator "OGC GeoSPARQL 1.0 Standard Working Group" ;
    dcterms:date "2011-06-16"^^xsd:date ;
    dcterms:source <http://www.opengis.net/doc/geosparql/1.0>,
        <http://www.opengis.net/doc/geosparql/1.1> ;
    policy:status status:valid ;
    rdfs:isDefinedBy <http://www.opengis.net/spec/geosparql/1.0>,
        <http://www.opengis.net/spec/geosparql/1.1/req/query-rewrite-extension/sf-query-rewrite> ;
    rdfs:seeAlso <http://www.opengis.net/doc/geosparql/1.0>,
        <http://www.opengis.net/doc/geosparql/1.1> ;
    skos:definition "A query rewrite rule used to determine if one spatial object is within another spatial object based on their associated geometry objects."@en ;
    skos:prefLabel "within"@en .

<http://www.opengis.net/doc/IS/geosparql/1.0> dcterms:format "application/pdf" ;
    dcterms:title "GeoSPARQL Specification Document as a PDF"@en ;
    prof:hasArtifact <https://portal.ogc.org/files/?artifact_id=47664> ;
    prof:hasRole role:specification .

<http://www.opengis.net/doc/IS/geosparql/1.1> a prof:ResourceDescriptor ;
    dcterms:format "text/html" ;
    dcterms:title "GeoSPARQL 1.1 Release Notes"@en,
        "GeoSPARQL Specification online"@en ;
    prof:hasArtifact "https://github.com/opengeospatial/ogc-geosparql/master/1.1/spec/_11-052r4.html"^^xsd:anyURI,
        "https://opengeospatial.github.io/ogc-geosparql/geosparql11/releasenotes.html"^^xsd:anyURI ;
    prof:hasRole role:specification .

confs10:core a spec:ConformanceClass,
        skos:Collection,
        sd:Feature ;
    skos:member conf10core:feature-class,
        conf10core:sparql-protocol,
        conf10core:spatial-object-class ;
    skos:prefLabel "GeoSPARQL 1.0 Conformance Class: Core"@en .

conf10core:sparql-protocol a spec:ConformanceTest ;
    spec:testPurpose "check conformance with this requirement"@en ;
    spec:testType spec:Capabilities ;
    rdfs:seeAlso reqs10core:sparql-protocol ;
    skos:definition "Verify that the implementation accepts SPARQL queries and returns the correct results in the correct format, according to the SPARQL Query Language for RDF, the SPARQL Protocol for RDF and SPARQL Query Results XML Format W3C specifications"@en ;
    skos:prefLabel "GeoSPARQL 1.0 Conformance Test: SPARQL Protocol"@en .

conf10gx:query-functions a spec:ConformanceTest ;
    spec:testPurpose "check conformance with this requirement"@en ;
    spec:testType spec:Capabilities ;
    rdfs:seeAlso reqs10gx:query-functions ;
    skos:definition "Verify that a set of SPARQL queries involving each of the following functions returns the correct result for a test dataset when using the specified serialization and version: geof:distance, geof:buffer, geof:convexHull, geof:intersection, geof:union, geof:difference,geof:symDifference, geof:envelope and geof:boundary"@en ;
    skos:prefLabel "GeoSPARQL 1.0 Conformance Test: Query Functions"@en .

conf10gx:srid-function a spec:ConformanceTest ;
    spec:testPurpose "check conformance with this requirement"@en ;
    spec:testType spec:Capabilities ;
    rdfs:seeAlso reqs10gx:srid-function ;
    skos:definition "Verify that a SPARQL query involving the geof:getSRID function returns the correct result for a test dataset when using the specified serialization and version"@en ;
    skos:prefLabel "GeoSPARQL 1.0 Conformance Test: SRID Function"@en .

confs10:geometry-topology-extension a spec:ConformanceClass,
        skos:Collection,
        sd:Feature ;
    dcterms:requires confs10:geometry-extension,
        confs10:topology-extension ;
    skos:member conf10gtx:eh-query-functions,
        conf10gtx:rcc8-query-functions,
        conf10gtx:relate-query-function,
        conf10gtx:sf-query-functions ;
    skos:prefLabel "GeoSPARQL 1.0 Conformance Class: Geometry Topology Extension"@en .

conf10gtx:eh-query-functions a spec:ConformanceTest ;
    spec:testPurpose "check conformance with this requirement"@en ;
    spec:testType spec:Capabilities ;
    rdfs:seeAlso reqs10gtx:eh-query-functions ;
    skos:definition "Verify that a set of SPARQL queries involving each of the following functions returns the correct result for a test dataset when using the specified serialization and version: geof:ehEquals, geof:ehDisjoint, geof:ehMeet, geof:ehOverlap, geof:ehCovers, geof:ehCoveredBy, geof:ehInside, geof:ehContains"@en ;
    skos:prefLabel "GeoSPARQL 1.0 Conformance Test: EH Query Functions"@en .

conf10gtx:rcc8-query-functions a spec:ConformanceTest ;
    spec:testPurpose "check conformance with this requirement"@en ;
    spec:testType spec:Capabilities ;
    rdfs:seeAlso reqs10gtx:rcc8-query-functions ;
    skos:definition "Verify that a set of SPARQL queries involving each of the following functions returns the correct result for a test dataset when using the specified serialization and version: geof:rcc8eq, geof:rcc8dc, geof:rcc8ec, geof:rcc8po, geof:rcc8tppi, geof:rcc8tpp, geof:rcc8ntpp, geof:rcc8ntppi"@en ;
    skos:prefLabel "GeoSPARQL 1.0 Conformance Test: RCC8 Query Functions"@en .

conf10gtx:relate-query-function a spec:ConformanceTest ;
    spec:testPurpose "check conformance with this requirement"@en ;
    spec:testType spec:Capabilities ;
    rdfs:seeAlso reqs10gtx:relate-query-function ;
    skos:definition "Verify that a set of SPARQL queries involving the geof:relate function returns the correct result for a test dataset when using the specified serialization and version"@en ;
    skos:prefLabel "GeoSPARQL 1.0 Conformance Test: Relate Query Function"@en .

conf10gtx:sf-query-functions a spec:ConformanceTest ;
    spec:testPurpose "check conformance with this requirement"@en ;
    spec:testType spec:Capabilities ;
    rdfs:seeAlso reqs10gtx:sf-query-functions ;
    skos:definition "Verify that a set of SPARQL queries involving each of the following functions returns the correct result for a test dataset when using the specified serialization and version: geof:sfEquals, geof:sfDisjoint, geof:sfIntersects, geof:sfTouches, geof:sfCrosses, geof:sfWithin, geof:sfContains, geof:sfOverlaps"@en ;
    skos:prefLabel "GeoSPARQL 1.0 Conformance Test: SF Query Functions"@en .

reqs10core:feature-class a spec:Requirement ;
    skos:definition "Implementations shall allow the RDFS class geo:Feature to be used in SPARQL graph patterns"@en ;
    skos:prefLabel "GeoSPARQL 1.0 Requirement: Feature Class"@en .

reqs10core:sparql-protocol a spec:Requirement ;
    skos:definition "Implementations shall support the SPARQL Query Language for RDF, the SPARQL Protocol for RDF and the SPARQL Query Results XML Format"@en ;
    skos:prefLabel "GeoSPARQL 1.0 Requirement: SPARQL Protocol"@en .

reqs10core:spatial-object-class a spec:Requirement ;
    skos:definition "Implementations shall allow the RDFS class geo:SpatialObject to be used in SPARQL graph patterns"@en ;
    skos:prefLabel "GeoSPARQL 1.0 Requirement: Spatial Object Class"@en .

reqs10gx:geometry-as-gml-literal a spec:Requirement ;
    skos:definition "Implementations shall allow the RDF property geo:asGML to be used in SPARQL graph patterns"@en ;
    skos:prefLabel "GeoSPARQL 1.0 Requirement:  Geometry asGML Literal"@en .

reqs10gx:geometry-as-wkt-literal a spec:Requirement ;
    skos:definition "Implementations shall allow the RDF property geo:asWKT to be used in SPARQL graph patterns"@en ;
    skos:prefLabel "GeoSPARQL 1.0 Requirement: Geometry asWKT Literal"@en .

reqs10gx:geometry-class a spec:Requirement ;
    skos:definition "Implementations shall allow the RDFS class geo:Geometry to be used in SPARQL graph patterns"@en ;
    skos:prefLabel "GeoSPARQL 1.0 Requirement: Geometry Class"@en .

reqs10gx:wkt-literal a spec:Requirement ;
    skos:definition "All RDFS Literals of type geo:wktLiteral shall consist of an optional URI identifying the coordinate reference system followed by Simple Features Well Known Text (WKT) describing a geometric value. Valid geo:wktLiterals are formed by concatenating a valid, absolute URI as defined in [RFC 2396], one or more spaces U+0020 character) as a separator, and a WKT string as defined in Simple Features [ISO 19125-1]"@en ;
    skos:prefLabel "GeoSPARQL 1.0 Requirement: WKT Literal"@en .

confs11:core a spec:ConformanceClass,
        skos:Collection,
        sd:Feature ;
    dcterms:requires confs10:core ;
    skos:member conf11core:feature-collection-class,
        conf11core:sparql-protocol,
        conf11core:spatial-object-class,
        conf11core:spatial-object-collection-class,
        conf11core:spatial-object-properties ;
    skos:prefLabel "GeoSPARQL 1.1 Conformance Class: Core"@en .

conf11gx:query-functions a spec:ConformanceTest ;
    spec:testPurpose "check conformance with this requirement"@en ;
    spec:testType spec:Capabilities ;
    rdfs:seeAlso reqs11gx:query-functions ;
    skos:definition "Verify that a set of SPARQL queries involving each of the following functions returns the correct result for a test dataset when using the specified serialization and version: geof:boundary geof:buffer, geof:convexHull, geof:coordinateDimension, geof:difference, geof:dimension, geof:distance, geof:envelope, geof:geometryType, geof:getSRID, geof:intersection, geof:is3D, geof:isEmpty, geof:isMeasured, geof:isSimple, geof:spatialDimension, geof:symDifference, geof:transform and geof:union  for non-DGGS geometry literals"@en ;
    skos:prefLabel "GeoSPARQL 1.1 Conformance Test: Query Functions"@en .

conf11gx:query-functions-non-sf a spec:ConformanceTest ;
    spec:testPurpose "check conformance with this requirement"@en ;
    spec:testType spec:Capabilities ;
    rdfs:seeAlso reqs11gx:query-functions-non-sf ;
    skos:definition "Verify that a set of SPARQL queries involving each of the following functions returns the correct result for a test dataset when using the specified serialization and version: geof:area, geof:geometryN, geof:length, geof:maxX, geof:maxY, geof:maxZ, geof:minX, geof:minY, geof:minZ, geof:numGeometries and geof:projectTo for non-DGGS geometry literals" ;
    skos:prefLabel "GeoSPARQL 1.1 Conformance Test: Query Functions, non Simple Features"@en .

conf11gx:sa-functions a spec:ConformanceTest ;
    spec:testPurpose "check conformance with this requirement" ;
    spec:testType spec:Capabilities ;
    rdfs:seeAlso reqs11gx:sa-functions ;
    skos:definition "Verify that queries involving these functions return the correct result for a test dataset"@en ;
    skos:prefLabel "GeoSPARQL 1.1 Conformance Test: Spatial Aggregate Functions"@en .

reqs11gx:dggs-literal a spec:Requirement ;
    skos:definition "All RDFS Literals of type geo:dggsLiteral shall consist of a DGGS geometry serialization formulated according to a specific DGGS literal type identified by a datatype specializing this generic datatype"@en ;
    skos:prefLabel "GeoSPARQL 1.1 Requirement: DGGS Literal"@en .

reqs11gx:geojson-literal a spec:Requirement ;
    skos:definition "All geo:geoJSONLiteral instances shall consist of the Geometry objects as defined in the GeoJSON specification [GEOJSON]"@en ;
    skos:prefLabel "GeoSPARQL 1.1 Requirement: GeoJSON Literal"@en .

reqs11gx:geometry-as-dggs-literal a spec:Requirement ;
    skos:definition "Implementations shall allow the RDF property geo:asDGGS to be used in SPARQL graph patterns"@en ;
    skos:prefLabel "GeoSPARQL 1.1 Requirement: Geometry asDGGS Literal"@en .

reqs11gx:geometry-as-geojson-literal a spec:Requirement ;
    skos:definition "Implementations shall allow the RDF property geo:asGeoJSON to be used in SPARQL graph patterns"@en ;
    skos:prefLabel "GeoSPARQL 1.1 Requirement: Geometry asGeoJSON Literal"@en .

reqs11gx:geometry-as-kml-literal a spec:Requirement ;
    skos:definition "Implementations shall allow the RDF property geo:asKML to be used in SPARQL graph patterns"@en ;
    skos:prefLabel "GeoSPARQL 1.1 Requirement: Geometry asKML Literal"@en .

reqs11gx:kml-literal a spec:Requirement ;
    skos:definition "All geo:kmlLiteral instances shall consist of the Geometry objects as defined in the KML specification [OGCKML]"@en ;
    skos:prefLabel "GeoSPARQL 1.1 Requirement: KML Literal"@en .

funcs:area a skos:Concept,
        sd:Function,
        fno:Function ;
    dcterms:source <http://www.opengis.net/doc/geosparql/1.1> ;
    policy:status status:valid ;
    rdfs:isDefinedBy reqs11gx:query-functions ;
    rdfs:seeAlso <http://www.opengis.net/doc/geosparql/1.1> ;
    skos:definition "Returns the area of a geometry in square meters."@en ;
    skos:prefLabel "area"@en ;
    fno:expects ( funcs:area_param1 funcs:area_param2 ) ;
    fno:returns ( funcs:area_output ) .

funcs:boundary a skos:Concept,
        sd:Function,
        fno:Function ;
    dcterms:contributor "Matthew Perry" ;
    dcterms:creator "OGC GeoSPARQL 1.0 Standard Working Group" ;
    dcterms:date "2011-06-16"^^xsd:date ;
    dcterms:source <http://www.opengis.net/doc/geosparql/1.0>,
        <http://www.opengis.net/doc/geosparql/1.1> ;
    policy:status status:valid ;
    rdfs:isDefinedBy <http://www.opengis.net/spec/geosparql/1.0>,
        reqs11gx:query-functions ;
    rdfs:seeAlso <http://www.opengis.net/doc/geosparql/1.0>,
        <http://www.opengis.net/doc/geosparql/1.1> ;
    skos:definition "A query function that returns the boundary of the input geometry."@en ;
    skos:prefLabel "boundary"@en ;
    fno:expects ( funcs:boundary_param1 ),
        ( funcs:boundary_param1 ) ;
    fno:returns ( funcs:boundary_output ),
        ( funcs:boundary_output ) .

funcs:boundingCircle a skos:Concept,
        sd:Function,
        fno:Function ;
    dcterms:date "2021-02-25"^^xsd:date ;
    dcterms:source <http://www.opengis.net/doc/geosparql/1.1> ;
    policy:status status:valid ;
    rdfs:isDefinedBy reqs11gx:sa-functions ;
    rdfs:seeAlso <http://www.opengis.net/doc/geosparql/1.1> ;
    skos:definition "A query function that calculates the minimum bounding circle of set of geometries."@en ;
    skos:prefLabel "bounding circle"@en .

funcs:buffer a skos:Concept,
        sd:Function,
        fno:Function ;
    dcterms:contributor "Matthew Perry" ;
    dcterms:creator "OGC GeoSPARQL 1.0 Standard Working Group" ;
    dcterms:date "2011-06-16"^^xsd:date ;
    dcterms:source <http://www.opengis.net/doc/geosparql/1.0>,
        <http://www.opengis.net/doc/geosparql/1.1> ;
    policy:status status:valid ;
    rdfs:isDefinedBy <http://www.opengis.net/spec/geosparql/1.0>,
        reqs11gx:query-functions ;
    rdfs:seeAlso <http://www.opengis.net/doc/geosparql/1.0>,
        <http://www.opengis.net/doc/geosparql/1.1> ;
    skos:definition "A query function that returns a buffer around the input geometry."@en ;
    skos:prefLabel "buffer"@en ;
    fno:expects ( funcs:buffer_param1 funcs:buffer_param2 funcs:buffer_param3 ),
        ( funcs:buffer_param1 funcs:buffer_param2 funcs:buffer_param3 ) ;
    fno:returns ( funcs:buffer_output ),
        ( funcs:buffer_output ) .

funcs:convexHull a skos:Concept,
        sd:Function,
        fno:Function ;
    dcterms:contributor "Matthew Perry" ;
    dcterms:creator "OGC GeoSPARQL 1.0 Standard Working Group" ;
    dcterms:date "2011-06-16"^^xsd:date ;
    dcterms:source <http://www.opengis.net/doc/geosparql/1.0>,
        <http://www.opengis.net/doc/geosparql/1.1> ;
    policy:status status:valid ;
    rdfs:isDefinedBy <http://www.opengis.net/spec/geosparql/1.0>,
        reqs11gx:query-functions ;
    rdfs:seeAlso <http://www.opengis.net/doc/geosparql/1.0>,
        <http://www.opengis.net/doc/geosparql/1.1> ;
    skos:definition "A query function that returns the convex hull of the input geometry."@en ;
    skos:prefLabel "convex hull"@en ;
    fno:expects ( funcs:convexHull_param1 ),
        ( funcs:convexHull_param1 ) ;
    fno:returns ( funcs:convexHull_output ),
        ( funcs:convexHull_output ) .

funcs:difference a skos:Concept,
        sd:Function,
        fno:Function ;
    dcterms:contributor "Matthew Perry" ;
    dcterms:creator "OGC GeoSPARQL 1.0 Standard Working Group" ;
    dcterms:date "2011-06-16"^^xsd:date ;
    dcterms:source <http://www.opengis.net/doc/geosparql/1.0>,
        <http://www.opengis.net/doc/geosparql/1.1> ;
    policy:status status:valid ;
    rdfs:isDefinedBy <http://www.opengis.net/spec/geosparql/1.0>,
        reqs11gx:query-functions ;
    rdfs:seeAlso <http://www.opengis.net/doc/geosparql/1.0>,
        <http://www.opengis.net/doc/geosparql/1.1> ;
    skos:definition "A query function that returns a geometry consisting of all points that are part of the first geometry but not the second geometry."@en ;
    skos:prefLabel "difference"@en ;
    fno:expects ( funcs:difference_param1 funcs:difference_param2 ),
        ( funcs:difference_param1 funcs:difference_param2 ) ;
    fno:returns ( funcs:difference_output ),
        ( funcs:difference_output ) .

funcs:dimension a skos:Concept,
        sd:Function,
        fno:Function ;
    dcterms:source <http://www.opengis.net/doc/geosparql/1.1> ;
    policy:status status:valid ;
    rdfs:isDefinedBy reqs11gx:query-functions ;
    rdfs:seeAlso <http://www.opengis.net/doc/geosparql/1.1> ;
    skos:definition "Returns the dimension of a geometry."@en ;
    skos:prefLabel "area"@en ;
    fno:expects ( funcs:dimension_param1 ) ;
    fno:returns ( funcs:dimension_output ) .

funcs:distance a skos:Concept,
        sd:Function,
        fno:Function ;
    dcterms:contributor "Matthew Perry" ;
    dcterms:creator "OGC GeoSPARQL 1.0 Standard Working Group" ;
    dcterms:date "2011-06-16"^^xsd:date ;
    dcterms:source <http://www.opengis.net/doc/geosparql/1.0>,
        <http://www.opengis.net/doc/geosparql/1.1> ;
    policy:status status:valid ;
    rdfs:isDefinedBy <http://www.opengis.net/spec/geosparql/1.0>,
        reqs11gx:query-functions ;
    rdfs:seeAlso <http://www.opengis.net/doc/geosparql/1.0>,
        <http://www.opengis.net/doc/geosparql/1.1> ;
    skos:definition "A query function that returns the distance between the two closest points of the input geometries."@en ;
    skos:example spec11:B.2.2.4 ;
    skos:prefLabel "distance"@en ;
    fno:expects ( funcs:distance_param1 funcs:distance_param2 funcs:distance_param3 ),
        ( funcs:distance_param1 funcs:distance_param2 funcs:distance_param3 ) ;
    fno:returns ( funcs:distance_output ),
        ( funcs:distance_output ) .

funcs:ehContains a skos:Concept,
        sd:Function,
        fno:Function ;
    dcterms:contributor "Matthew Perry" ;
    dcterms:creator "OGC GeoSPARQL 1.0 Standard Working Group" ;
    dcterms:date "2011-06-16"^^xsd:date ;
    dcterms:source <http://www.opengis.net/doc/geosparql/1.0>,
        <http://www.opengis.net/doc/geosparql/1.1> ;
    policy:status status:valid ;
    rdfs:isDefinedBy <http://www.opengis.net/spec/geosparql/1.0>,
        <http://www.opengis.net/spec/geosparql/1.1/req/geometry-topology-extension/eh-query-functions> ;
    rdfs:seeAlso <http://www.opengis.net/doc/geosparql/1.0>,
        <http://www.opengis.net/doc/geosparql/1.1> ;
    skos:definition """A query function that returns true if the first geometry argument spatially contains the second geometry argument. 
      
DE-9IM: T*TFF*FF*"""@en,
        """A query function that returns true if the first geometry argument spatially contains the second geometry argument. \r
      \r
DE-9IM: T*TFF*FF*"""@en ;
    skos:prefLabel "contains"@en ;
    fno:expects ( funcs:ehContains_param1 funcs:ehContains_param2 ),
        ( funcs:ehContains_param1 funcs:ehContains_param2 ) ;
    fno:returns ( funcs:ehContains_output ),
        ( funcs:ehContains_output ) .

funcs:ehCoveredBy a skos:Concept,
        sd:Function,
        fno:Function ;
    dcterms:contributor "Matthew Perry" ;
    dcterms:creator "OGC GeoSPARQL 1.0 Standard Working Group" ;
    dcterms:date "2011-06-16"^^xsd:date ;
    dcterms:source <http://www.opengis.net/doc/geosparql/1.0>,
        <http://www.opengis.net/doc/geosparql/1.1> ;
    policy:status status:valid ;
    rdfs:isDefinedBy <http://www.opengis.net/spec/geosparql/1.0>,
        <http://www.opengis.net/spec/geosparql/1.1/req/geometry-topology-extension/eh-query-functions> ;
    rdfs:seeAlso <http://www.opengis.net/doc/geosparql/1.0>,
        <http://www.opengis.net/doc/geosparql/1.1> ;
    skos:definition """A query function that returns true if the first geometry argument is spatially covered by the second geometry argument.

DE-9IM: TFF*TFT**"""@en,
        """A query function that returns true if the first geometry argument is spatially covered by the second geometry argument.\r
\r
DE-9IM: TFF*TFT**"""@en ;
    skos:prefLabel "covered by"@en ;
    fno:expects ( funcs:ehCoveredBy_param1 funcs:ehCoveredBy_param2 ),
        ( funcs:ehCoveredBy_param1 funcs:ehCoveredBy_param2 ) ;
    fno:returns ( funcs:ehConveredBy_output ),
        ( funcs:ehConveredBy_output ) .

funcs:ehCovers a skos:Concept,
        sd:Function,
        fno:Function ;
    dcterms:contributor "Matthew Perry" ;
    dcterms:creator "OGC GeoSPARQL 1.0 Standard Working Group" ;
    dcterms:date "2011-06-16"^^xsd:date ;
    dcterms:source <http://www.opengis.net/doc/geosparql/1.0>,
        <http://www.opengis.net/doc/geosparql/1.1> ;
    policy:status status:valid ;
    rdfs:isDefinedBy <http://www.opengis.net/spec/geosparql/1.0>,
        <http://www.opengis.net/spec/geosparql/1.1/req/geometry-topology-extension/eh-query-functions> ;
    rdfs:seeAlso <http://www.opengis.net/doc/geosparql/1.0>,
        <http://www.opengis.net/doc/geosparql/1.1> ;
    skos:definition """A query function that returns true if the first geometry argument spatially covers the second geometry argument.

DE-9IM: T*TFT*FF*"""@en,
        """A query function that returns true if the first geometry argument spatially covers the second geometry argument.\r
\r
DE-9IM: T*TFT*FF*"""@en ;
    skos:prefLabel "covers"@en ;
    fno:expects ( funcs:ehCovers_param1 funcs:ehCovers_param2 ),
        ( funcs:ehCovers_param1 funcs:ehCovers_param2 ) ;
    fno:returns ( funcs:ehCovers_output ),
        ( funcs:ehCovers_output ) .

funcs:ehDisjoint a skos:Concept,
        sd:Function,
        fno:Function ;
    dcterms:contributor "Matthew Perry" ;
    dcterms:creator "OGC GeoSPARQL 1.0 Standard Working Group" ;
    dcterms:date "2011-06-16"^^xsd:date ;
    dcterms:source <http://www.opengis.net/doc/geosparql/1.0>,
        <http://www.opengis.net/doc/geosparql/1.1> ;
    policy:status status:valid ;
    rdfs:isDefinedBy <http://www.opengis.net/spec/geosparql/1.0>,
        <http://www.opengis.net/spec/geosparql/1.1/req/geometry-topology-extension/eh-query-functions> ;
    rdfs:seeAlso <http://www.opengis.net/doc/geosparql/1.0>,
        <http://www.opengis.net/doc/geosparql/1.1> ;
    skos:definition """A query function that returns true if the input geometries are disjoint. 

DE-9IM: FF*FF****"""@en,
        """A query function that returns true if the input geometries are disjoint. \r
\r
DE-9IM: FF*FF****"""@en ;
    skos:prefLabel "disjoint"@en ;
    fno:expects ( funcs:ehDisjoint_param1 funcs:ehDisjoint_param2 ),
        ( funcs:ehDisjoint_param1 funcs:ehDisjoint_param2 ) ;
    fno:returns ( funcs:ehDisjoint_output ),
        ( funcs:ehDisjoint_output ) .

funcs:ehEquals a skos:Concept,
        sd:Function,
        fno:Function ;
    dcterms:contributor "Matthew Perry" ;
    dcterms:creator "OGC GeoSPARQL 1.0 Standard Working Group" ;
    dcterms:date "2011-06-16"^^xsd:date ;
    dcterms:source <http://www.opengis.net/doc/geosparql/1.0>,
        <http://www.opengis.net/doc/geosparql/1.1> ;
    policy:status status:valid ;
    rdfs:isDefinedBy <http://www.opengis.net/spec/geosparql/1.0>,
        <http://www.opengis.net/spec/geosparql/1.1/req/geometry-topology-extension/eh-query-functions> ;
    rdfs:seeAlso <http://www.opengis.net/doc/geosparql/1.0>,
        <http://www.opengis.net/doc/geosparql/1.1> ;
    skos:definition """A query function that returns true if the input geometries are equal. 

DE-9IM: TFFFTFFFT"""@en,
        """A query function that returns true if the input geometries are equal. \r
\r
DE-9IM: TFFFTFFFT"""@en ;
    skos:prefLabel "equals"@en ;
    fno:expects ( funcs:ehEquals_param1 funcs:ehEquals_param2 ),
        ( funcs:ehEquals_param1 funcs:ehEquals_param2 ) ;
    fno:returns ( funcs:ehEquals_output ),
        ( funcs:ehEquals_output ) .

funcs:ehInside a skos:Concept,
        sd:Function,
        fno:Function ;
    dcterms:contributor "Matthew Perry" ;
    dcterms:creator "OGC GeoSPARQL 1.0 Standard Working Group" ;
    dcterms:date "2011-06-16"^^xsd:date ;
    dcterms:source <http://www.opengis.net/doc/geosparql/1.0>,
        <http://www.opengis.net/doc/geosparql/1.1> ;
    policy:status status:valid ;
    rdfs:isDefinedBy <http://www.opengis.net/spec/geosparql/1.0>,
        <http://www.opengis.net/spec/geosparql/1.1/req/geometry-topology-extension/eh-query-functions> ;
    rdfs:seeAlso <http://www.opengis.net/doc/geosparql/1.0>,
        <http://www.opengis.net/doc/geosparql/1.1> ;
    skos:definition """A query function that returns true if the first geometry argument is spatially inside the second geometry argument.

DE-9IM: TFF*FFT**"""@en,
        """A query function that returns true if the first geometry argument is spatially inside the second geometry argument.\r
\r
DE-9IM: TFF*FFT**"""@en ;
    skos:prefLabel "inside"@en ;
    fno:expects ( funcs:ehInside_param1 funcs:ehInside_param2 ),
        ( funcs:ehInside_param1 funcs:ehInside_param2 ) ;
    fno:returns ( funcs:ehInside_output ),
        ( funcs:ehInside_output ) .

funcs:ehMeet a skos:Concept,
        sd:Function,
        fno:Function ;
    dcterms:contributor "Matthew Perry" ;
    dcterms:creator "OGC GeoSPARQL 1.0 Standard Working Group" ;
    dcterms:date "2011-06-16"^^xsd:date ;
    dcterms:source <http://www.opengis.net/doc/geosparql/1.0>,
        <http://www.opengis.net/doc/geosparql/1.1> ;
    policy:status status:valid ;
    rdfs:isDefinedBy <http://www.opengis.net/spec/geosparql/1.0>,
        <http://www.opengis.net/spec/geosparql/1.1/req/geometry-topology-extension/eh-query-functions> ;
    rdfs:seeAlso <http://www.opengis.net/doc/geosparql/1.0>,
        <http://www.opengis.net/doc/geosparql/1.1> ;
    skos:definition """A query function that returns true if the input geometries meet.

DE-9IM: FT******* ^ F**T***** ^ F***T****"""@en,
        """A query function that returns true if the input geometries meet.\r
\r
DE-9IM: FT******* ^ F**T***** ^ F***T****"""@en ;
    skos:prefLabel "meet"@en ;
    fno:expects ( funcs:ehMeet_param1 funcs:ehMeet_param2 ),
        ( funcs:ehMeet_param1 funcs:ehMeet_param2 ) ;
    fno:returns ( funcs:ehMeet_output ),
        ( funcs:ehMeet_output ) .

funcs:ehOverlap a skos:Concept,
        sd:Function,
        fno:Function ;
    dcterms:contributor "Matthew Perry" ;
    dcterms:creator "OGC GeoSPARQL 1.0 Standard Working Group" ;
    dcterms:date "2011-06-16"^^xsd:date ;
    dcterms:source <http://www.opengis.net/doc/geosparql/1.0>,
        <http://www.opengis.net/doc/geosparql/1.1> ;
    policy:status status:valid ;
    rdfs:isDefinedBy <http://www.opengis.net/spec/geosparql/1.0>,
        <http://www.opengis.net/spec/geosparql/1.1/req/geometry-topology-extension/eh-query-functions> ;
    rdfs:seeAlso <http://www.opengis.net/doc/geosparql/1.0>,
        <http://www.opengis.net/doc/geosparql/1.1> ;
    skos:definition """A query function that returns true if the input geometries overlap.

DE-9IM: T*T***T**"""@en,
        """A query function that returns true if the input geometries overlap.\r
\r
DE-9IM: T*T***T**"""@en ;
    skos:prefLabel "overlap"@en ;
    fno:expects ( funcs:ehOverlap_param1 funcs:ehOverlap_param2 ),
        ( funcs:ehOverlap_param1 funcs:ehOverlap_param2 ) ;
    fno:returns ( funcs:ehOverlap_output ),
        ( funcs:ehOverlap_output ) .

funcs:envelope a skos:Concept,
        sd:Function,
        fno:Function ;
    dcterms:contributor "Matthew Perry" ;
    dcterms:creator "OGC GeoSPARQL 1.0 Standard Working Group" ;
    dcterms:date "2011-06-16"^^xsd:date ;
    dcterms:source <http://www.opengis.net/doc/geosparql/1.0>,
        <http://www.opengis.net/doc/geosparql/1.1> ;
    policy:status status:valid ;
    rdfs:isDefinedBy <http://www.opengis.net/spec/geosparql/1.0>,
        reqs11gx:query-functions ;
    rdfs:seeAlso <http://www.opengis.net/doc/geosparql/1.0>,
        <http://www.opengis.net/doc/geosparql/1.1> ;
    skos:definition "A query function that returns the minimum bounding rectangle of the input geometry."@en ;
    skos:prefLabel "envelope"@en ;
    fno:expects ( funcs:envelope_param1 ),
        ( funcs:envelope_param1 ) ;
    fno:returns ( funcs:envelope_output ),
        ( funcs:envelope_output ) .

funcs:getSRID a skos:Concept,
        sd:Function,
        fno:Function ;
    dcterms:contributor "Matthew Perry" ;
    dcterms:creator "OGC GeoSPARQL 1.0 Standard Working Group" ;
    dcterms:date "2011-06-16"^^xsd:date ;
    dcterms:source <http://www.opengis.net/doc/geosparql/1.0>,
        <http://www.opengis.net/doc/geosparql/1.1> ;
    policy:status status:valid ;
    rdfs:isDefinedBy <http://www.opengis.net/spec/geosparql/1.0>,
        reqs11gx:srid-function ;
    rdfs:seeAlso <http://www.opengis.net/doc/geosparql/1.0>,
        <http://www.opengis.net/doc/geosparql/1.1> ;
    skos:definition "A query function that returns the spatial reference system URI of the input geometry."@en ;
    skos:prefLabel "getSRID"@en ;
    fno:expects ( funcs:getSRID_param1 ),
        ( funcs:getSRID_param1 ) ;
    fno:returns ( funcs:getSRID_output ),
        ( funcs:getSRID_output ) .

funcs:intersection a skos:Concept,
        sd:Function,
        fno:Function ;
    dcterms:contributor "Matthew Perry" ;
    dcterms:creator "OGC GeoSPARQL 1.0 Standard Working Group" ;
    dcterms:date "2011-06-16"^^xsd:date ;
    dcterms:source <http://www.opengis.net/doc/geosparql/1.0>,
        <http://www.opengis.net/doc/geosparql/1.1> ;
    policy:status status:valid ;
    rdfs:isDefinedBy <http://www.opengis.net/spec/geosparql/1.0>,
        reqs11gx:query-functions ;
    rdfs:seeAlso <http://www.opengis.net/doc/geosparql/1.0>,
        <http://www.opengis.net/doc/geosparql/1.1> ;
    skos:definition "A query function that returns a geometry consisting of all points that are part of both input geometries."@en ;
    skos:prefLabel "intersection"@en ;
    fno:expects ( funcs:intersection_param1 funcs:intersection_param2 ),
        ( funcs:intersection_param1 funcs:intersection_param2 ) ;
    fno:returns ( funcs:intersection_output ),
        ( funcs:intersection_output ) .

funcs:isEmpty a skos:Concept,
        sd:Function,
        fno:Function ;
    dcterms:source <http://www.opengis.net/doc/geosparql/1.1> ;
    policy:status status:valid ;
    rdfs:isDefinedBy reqs11gx:query-functions ;
    rdfs:seeAlso <http://www.opengis.net/doc/geosparql/1.1> ;
    skos:definition "A query function that returns true if the input geometry is empty."@en ;
    skos:prefLabel "isEmpty"@en ;
    fno:expects ( funcs:isEmpty_param1 ) ;
    fno:returns ( funcs:isEmpty_output ) .

funcs:isSimple a skos:Concept,
        sd:Function,
        fno:Function ;
    dcterms:source <http://www.opengis.net/doc/geosparql/1.1> ;
    policy:status status:valid ;
    rdfs:isDefinedBy reqs11gx:query-functions ;
    rdfs:seeAlso <http://www.opengis.net/doc/geosparql/1.1> ;
    skos:definition "A query function that returns true if the input geometry is a simple geometry."@en ;
    skos:prefLabel "isSimple"@en ;
    fno:expects ( funcs:isSimple_param1 ) ;
    fno:returns ( funcs:isSimple_output ) .

funcs:metricBuffer a skos:Concept,
        sd:Function,
        fno:Function ;
    dcterms:date "2022-04-20"^^xsd:date ;
    dcterms:source <http://www.opengis.net/doc/geosparql/1.1> ;
    policy:status status:valid ;
    rdfs:isDefinedBy reqs11gx:query-functions ;
    rdfs:seeAlso <http://www.opengis.net/doc/geosparql/1.1> ;
    skos:definition "A query function that returns a buffer around the input geometry, using a distance in meters."@en ;
    skos:prefLabel "metric buffer"@en ;
    fno:expects ( funcs:metricBuffer_param1 funcs:metricBuffer_param2 ) ;
    fno:returns ( funcs:metricBuffer_output ) .

funcs:metricDistance a skos:Concept,
        sd:Function,
        fno:Function ;
    dcterms:source <http://www.opengis.net/doc/geosparql/1.1> ;
    policy:status status:valid ;
    rdfs:isDefinedBy reqs11gx:query-functions ;
    rdfs:seeAlso <http://www.opengis.net/doc/geosparql/1.1> ;
    skos:definition "A query function that returns the distance in meters between the two closest points of the input geometries."@en ;
    skos:prefLabel "metric distance"@en ;
    fno:expects ( funcs:metricDistance_param1 funcs:metricDistance_param2 ) ;
    fno:returns ( funcs:metricDistance_output ) .

funcs:rcc8dc a skos:Concept,
        sd:Function,
        fno:Function ;
    dcterms:contributor "Matthew Perry" ;
    dcterms:creator "OGC GeoSPARQL 1.0 Standard Working Group" ;
    dcterms:date "2011-06-16"^^xsd:date ;
    dcterms:source <http://www.opengis.net/doc/geosparql/1.0>,
        <http://www.opengis.net/doc/geosparql/1.1> ;
    policy:status status:valid ;
    rdfs:isDefinedBy <http://www.opengis.net/spec/geosparql/1.0>,
        <http://www.opengis.net/spec/geosparql/1.1/req/geometry-topology-extension/rcc8-query-functions> ;
    rdfs:seeAlso <http://www.opengis.net/doc/geosparql/1.0>,
        <http://www.opengis.net/doc/geosparql/1.1> ;
    skos:definition """A query function that returns true if the input geometries are disjoint. 

DE-9IM: FFTFFTTTT"""@en,
        """A query function that returns true if the input geometries are disjoint. \r
\r
DE-9IM: FFTFFTTTT"""@en ;
    skos:prefLabel "disconnected"@en ;
    fno:expects ( funcs:rcc8dc_param1 funcs:rcc8dc_param2 ),
        ( funcs:rcc8dc_param1 funcs:rcc8dc_param2 ) ;
    fno:returns ( funcs:rcc8dc_output ),
        ( funcs:rcc8dc_output ) .

funcs:rcc8ec a skos:Concept,
        sd:Function,
        fno:Function ;
    dcterms:contributor "Matthew Perry" ;
    dcterms:creator "OGC GeoSPARQL 1.0 Standard Working Group" ;
    dcterms:date "2011-06-16"^^xsd:date ;
    dcterms:source <http://www.opengis.net/doc/geosparql/1.0>,
        <http://www.opengis.net/doc/geosparql/1.1> ;
    policy:status status:valid ;
    rdfs:isDefinedBy <http://www.opengis.net/spec/geosparql/1.0>,
        <http://www.opengis.net/spec/geosparql/1.1/req/geometry-topology-extension/rcc8-query-functions> ;
    rdfs:seeAlso <http://www.opengis.net/doc/geosparql/1.0>,
        <http://www.opengis.net/doc/geosparql/1.1> ;
    skos:definition """A query function that returns true if the input geometries meet. 

DE-9IM: FFTFTTTTT"""@en,
        """A query function that returns true if the input geometries meet. \r
\r
DE-9IM: FFTFTTTTT"""@en ;
    skos:prefLabel "externally connected"@en ;
    fno:expects ( funcs:rcc8ec_param1 funcs:rcc8ec_param2 ),
        ( funcs:rcc8ec_param1 funcs:rcc8ec_param2 ) ;
    fno:returns ( funcs:rcc8ec_output ),
        ( funcs:rcc8ec_output ) .

funcs:rcc8eq a skos:Concept,
        sd:Function,
        fno:Function ;
    dcterms:contributor "Matthew Perry" ;
    dcterms:creator "OGC GeoSPARQL 1.0 Standard Working Group" ;
    dcterms:date "2011-06-16"^^xsd:date ;
    dcterms:source <http://www.opengis.net/doc/geosparql/1.0>,
        <http://www.opengis.net/doc/geosparql/1.1> ;
    policy:status status:valid ;
    rdfs:isDefinedBy <http://www.opengis.net/spec/geosparql/1.0>,
        <http://www.opengis.net/spec/geosparql/1.1/req/geometry-topology-extension/rcc8-query-functions> ;
    rdfs:seeAlso <http://www.opengis.net/doc/geosparql/1.0>,
        <http://www.opengis.net/doc/geosparql/1.1> ;
    skos:definition """A query function that returns true if the input geometries are equal. 
      
DE-9IM: TFFFTFFFT"""@en,
        """A query function that returns true if the input geometries are equal. \r
      \r
DE-9IM: TFFFTFFFT"""@en ;
    skos:prefLabel "equals"@en ;
    fno:expects ( funcs:rcc8eq_param1 funcs:rcc8eq_param2 ),
        ( funcs:rcc8eq_param1 funcs:rcc8eq_param2 ) ;
    fno:returns ( funcs:rcc8eq_output ),
        ( funcs:rcc8eq_output ) .

funcs:rcc8ntpp a skos:Concept,
        sd:Function,
        fno:Function ;
    dcterms:contributor "Matthew Perry" ;
    dcterms:creator "OGC GeoSPARQL 1.0 Standard Working Group" ;
    dcterms:date "2011-06-16"^^xsd:date ;
    dcterms:source <http://www.opengis.net/doc/geosparql/1.0>,
        <http://www.opengis.net/doc/geosparql/1.1> ;
    policy:status status:valid ;
    rdfs:isDefinedBy <http://www.opengis.net/spec/geosparql/1.0>,
        <http://www.opengis.net/spec/geosparql/1.1/req/geometry-topology-extension/rcc8-query-functions> ;
    rdfs:seeAlso <http://www.opengis.net/doc/geosparql/1.0>,
        <http://www.opengis.net/doc/geosparql/1.1> ;
    skos:definition """A query function that returns true if the first geometry argument is spatially inside the second geometry argument.

DE-9IM: TFFTFFTTT"""@en,
        """A query function that returns true if the first geometry argument is spatially inside the second geometry argument.\r
\r
DE-9IM: TFFTFFTTT"""@en ;
    skos:prefLabel "non-tangential proper part"@en ;
    fno:expects ( funcs:rcc8ntpp_param1 funcs:rcc8ntpp_param2 ),
        ( funcs:rcc8ntpp_param1 funcs:rcc8ntpp_param2 ) ;
    fno:returns ( funcs:rcc8ntpp_output ),
        ( funcs:rcc8ntpp_output ) .

funcs:rcc8ntppi a skos:Concept,
        sd:Function,
        fno:Function ;
    dcterms:contributor "Matthew Perry" ;
    dcterms:creator "OGC GeoSPARQL 1.0 Standard Working Group" ;
    dcterms:date "2011-06-16"^^xsd:date ;
    dcterms:source <http://www.opengis.net/doc/geosparql/1.0>,
        <http://www.opengis.net/doc/geosparql/1.1> ;
    policy:status status:valid ;
    rdfs:isDefinedBy <http://www.opengis.net/spec/geosparql/1.0>,
        <http://www.opengis.net/spec/geosparql/1.1/req/geometry-topology-extension/rcc8-query-functions> ;
    rdfs:seeAlso <http://www.opengis.net/doc/geosparql/1.0>,
        <http://www.opengis.net/doc/geosparql/1.1> ;
    skos:definition """A query function that returns true if the first geometry argument spatially contains the second geometry argument.

DE-9IM: TTTFFTFFT"""@en,
        """A query function that returns true if the first geometry argument spatially contains the second geometry argument.\r
\r
DE-9IM: TTTFFTFFT"""@en ;
    skos:prefLabel "non-tangential proper part inverse"@en ;
    fno:expects ( funcs:rcc8ntppi_param1 funcs:rcc8ntppi_param2 ),
        ( funcs:rcc8ntppi_param1 funcs:rcc8ntppi_param2 ) ;
    fno:returns ( funcs:rcc8ntppi_output ),
        ( funcs:rcc8ntppi_output ) .

funcs:rcc8po a skos:Concept,
        sd:Function,
        fno:Function ;
    dcterms:contributor "Matthew Perry" ;
    dcterms:creator "OGC GeoSPARQL 1.0 Standard Working Group" ;
    dcterms:date "2011-06-16"^^xsd:date ;
    dcterms:source <http://www.opengis.net/doc/geosparql/1.0>,
        <http://www.opengis.net/doc/geosparql/1.1> ;
    policy:status status:valid ;
    rdfs:isDefinedBy <http://www.opengis.net/spec/geosparql/1.0>,
        <http://www.opengis.net/spec/geosparql/1.1/req/geometry-topology-extension/rcc8-query-functions> ;
    rdfs:seeAlso <http://www.opengis.net/doc/geosparql/1.0>,
        <http://www.opengis.net/doc/geosparql/1.1> ;
    skos:definition """A query function that returns true if the input geometries overlap.

DE-9IM: TTTTTTTTT"""@en,
        """A query function that returns true if the input geometries overlap.\r
\r
DE-9IM: TTTTTTTTT"""@en ;
    skos:prefLabel "partially overlapping"@en ;
    fno:expects ( funcs:rcc8po_param1 funcs:rcc8po_param2 ),
        ( funcs:rcc8po_param1 funcs:rcc8po_param2 ) ;
    fno:returns ( funcs:rcc8po_output ),
        ( funcs:rcc8po_output ) .

funcs:rcc8tpp a skos:Concept,
        sd:Function,
        fno:Function ;
    dcterms:contributor "Matthew Perry" ;
    dcterms:creator "OGC GeoSPARQL 1.0 Standard Working Group" ;
    dcterms:date "2011-06-16"^^xsd:date ;
    dcterms:source <http://www.opengis.net/doc/geosparql/1.0>,
        <http://www.opengis.net/doc/geosparql/1.1> ;
    policy:status status:valid ;
    rdfs:isDefinedBy <http://www.opengis.net/spec/geosparql/1.0>,
        <http://www.opengis.net/spec/geosparql/1.1/req/geometry-topology-extension/rcc8-query-functions> ;
    rdfs:seeAlso <http://www.opengis.net/doc/geosparql/1.0>,
        <http://www.opengis.net/doc/geosparql/1.1> ;
    skos:definition """A query function that returns true if the first geometry argument is spatially covered by the second geometry argument.

DE-9IM: TFFTTFTTT"""@en,
        """A query function that returns true if the first geometry argument is spatially covered by the second geometry argument.\r
\r
DE-9IM: TFFTTFTTT"""@en ;
    skos:prefLabel "tangential proper part"@en ;
    fno:expects ( funcs:rcc8tpp_param1 funcs:rcc8tpp_param2 ),
        ( funcs:rcc8tpp_param1 funcs:rcc8tpp_param2 ) ;
    fno:returns ( funcs:rcc8tpp_output ),
        ( funcs:rcc8tpp_output ) .

funcs:rcc8tppi a skos:Concept,
        sd:Function,
        fno:Function ;
    dcterms:contributor "Matthew Perry" ;
    dcterms:creator "OGC GeoSPARQL 1.0 Standard Working Group" ;
    dcterms:date "2011-06-16"^^xsd:date ;
    dcterms:source <http://www.opengis.net/doc/geosparql/1.0>,
        <http://www.opengis.net/doc/geosparql/1.1> ;
    policy:status status:valid ;
    rdfs:isDefinedBy <http://www.opengis.net/spec/geosparql/1.0>,
        <http://www.opengis.net/spec/geosparql/1.1/req/geometry-topology-extension/rcc8-query-functions> ;
    rdfs:seeAlso <http://www.opengis.net/doc/geosparql/1.0>,
        <http://www.opengis.net/doc/geosparql/1.1> ;
    skos:definition """A query function that returns true if the first geometry argument spatially covers the second geometry argument.

DE-9IM: TTTFTTFFT"""@en,
        """A query function that returns true if the first geometry argument spatially covers the second geometry argument.\r
\r
DE-9IM: TTTFTTFFT"""@en ;
    skos:prefLabel "tangential proper part inverse"@en ;
    fno:expects ( funcs:rcc8tppi_param1 funcs:rcc8tppi_param2 ),
        ( funcs:rcc8tppi_param1 funcs:rcc8tppi_param2 ) ;
    fno:returns ( funcs:rcc8tppi_output ),
        ( funcs:rcc8tppi_output ) .

funcs:relate a skos:Concept,
        sd:Function,
        fno:Function ;
    dcterms:contributor "Matthew Perry" ;
    dcterms:creator "OGC GeoSPARQL 1.0 Standard Working Group" ;
    dcterms:date "2011-06-16"^^xsd:date ;
    dcterms:source <http://www.opengis.net/doc/geosparql/1.0>,
        <http://www.opengis.net/doc/geosparql/1.1> ;
    policy:status status:valid ;
    rdfs:isDefinedBy <http://www.opengis.net/spec/geosparql/1.0>,
        <http://www.opengis.net/spec/geosparql/1.1/req/geometry-topology-extension/relate-query-function> ;
    rdfs:seeAlso <http://www.opengis.net/doc/geosparql/1.0>,
        <http://www.opengis.net/doc/geosparql/1.1> ;
    skos:definition "A query function that returns true if the spatial relationship between the two input geometries corresponds to one with acceptable values for the specified DE-9IM pattern matrix."@en ;
    skos:prefLabel "relate"@en ;
    fno:expects ( funcs:relate_param1 funcs:relate_param2 funcs:relate_param3 ),
        ( funcs:relate_param1 funcs:relate_param2 funcs:relate_param3 ) ;
    fno:returns ( funcs:relate_output ),
        ( funcs:relate_output ) .

funcs:sfContains a skos:Concept,
        sd:Function,
        fno:Function ;
    dcterms:contributor "Matthew Perry" ;
    dcterms:creator "OGC GeoSPARQL 1.0 Standard Working Group" ;
    dcterms:date "2011-06-16"^^xsd:date ;
    dcterms:source <http://www.opengis.net/doc/geosparql/1.0>,
        <http://www.opengis.net/doc/geosparql/1.1> ;
    policy:status status:valid ;
    rdfs:isDefinedBy <http://www.opengis.net/spec/geosparql/1.0>,
        <http://www.opengis.net/spec/geosparql/1.1/req/geometry-topology-extension/sf-query-functions> ;
    rdfs:seeAlso <http://www.opengis.net/doc/geosparql/1.0>,
        <http://www.opengis.net/doc/geosparql/1.1> ;
    skos:definition """A query function that returns true if the first geometry argument spatially contains the second geometry argument.

DE-9IM: T*****FF*"""@en,
        """A query function that returns true if the first geometry argument spatially contains the second geometry argument.\r
\r
DE-9IM: T*****FF*"""@en ;
    skos:example spec11:B.2.2.1 ;
    skos:prefLabel "contains"@en ;
    fno:expects ( funcs:sfContains_param1 funcs:sfContains_param2 ),
        ( funcs:sfContains_param1 funcs:sfContains_param2 ) ;
    fno:returns ( funcs:sfContains_output ),
        ( funcs:sfContains_output ) .

funcs:sfCrosses a skos:Concept,
        sd:Function,
        fno:Function ;
    dcterms:contributor "Matthew Perry" ;
    dcterms:creator "OGC GeoSPARQL 1.0 Standard Working Group" ;
    dcterms:date "2011-06-16"^^xsd:date ;
    dcterms:source <http://www.opengis.net/doc/geosparql/1.0>,
        <http://www.opengis.net/doc/geosparql/1.1> ;
    policy:status status:valid ;
    rdfs:isDefinedBy <http://www.opengis.net/spec/geosparql/1.0>,
        <http://www.opengis.net/spec/geosparql/1.1/req/geometry-topology-extension/sf-query-functions> ;
    rdfs:seeAlso <http://www.opengis.net/doc/geosparql/1.0>,
        <http://www.opengis.net/doc/geosparql/1.1> ;
    skos:definition """A query function that returns true if the first geometry argument spatially crosses the second geometry argument.

DE-9IM: T*T***T**"""@en,
        """A query function that returns true if the first geometry argument spatially crosses the second geometry argument.\r
\r
DE-9IM: T*T***T**"""@en ;
    skos:prefLabel "crosses"@en ;
    fno:expects ( funcs:sfCrosses_param1 funcs:sfCrosses_param2 ),
        ( funcs:sfCrosses_param1 funcs:sfCrosses_param2 ) ;
    fno:returns ( funcs:sfCrosses_output ),
        ( funcs:sfCrosses_output ) .

funcs:sfDisjoint a skos:Concept,
        sd:Function,
        fno:Function ;
    dcterms:date "2011-06-16"^^xsd:date ;
    dcterms:source <http://www.opengis.net/doc/geosparql/1.0>,
        <http://www.opengis.net/doc/geosparql/1.1> ;
    policy:status status:valid ;
    rdfs:isDefinedBy <http://www.opengis.net/spec/geosparql/1.0>,
        <http://www.opengis.net/spec/geosparql/1.1/req/geometry-topology-extension/sf-query-functions> ;
    rdfs:seeAlso <http://www.opengis.net/doc/geosparql/1.0>,
        <http://www.opengis.net/doc/geosparql/1.1> ;
    skos:definition """A query function that returns true if the input geometries are disjoint. 
      
DE-9IM: FF*FF****"""@en,
        """A query function that returns true if the input geometries are disjoint. \r
      \r
DE-9IM: FF*FF****"""@en ;
    skos:prefLabel "disjoint"@en ;
    fno:expects ( funcs:sfDisjoint_param1 funcs:sfDisjoint_param2 ),
        ( funcs:sfDisjoint_param1 funcs:sfDisjoint_param2 ) ;
    fno:returns ( funcs:sfDisjoint_output ),
        ( funcs:sfDisjoint_output ) .

funcs:sfEquals a skos:Concept,
        sd:Function,
        fno:Function ;
    dcterms:contributor "Matthew Perry" ;
    dcterms:creator "OGC GeoSPARQL 1.0 Standard Working Group" ;
    dcterms:date "2011-06-16"^^xsd:date ;
    dcterms:source <http://www.opengis.net/doc/geosparql/1.0>,
        <http://www.opengis.net/doc/geosparql/1.1> ;
    policy:status status:valid ;
    rdfs:isDefinedBy <http://www.opengis.net/spec/geosparql/1.0>,
        <http://www.opengis.net/spec/geosparql/1.1/req/geometry-topology-extension/sf-query-functions> ;
    rdfs:seeAlso <http://www.opengis.net/doc/geosparql/1.0>,
        <http://www.opengis.net/doc/geosparql/1.1> ;
    skos:definition """A query function that returns true if the input geometries are equal. 

DE-9IM: TFFFTFFFT"""@en,
        """A query function that returns true if the input geometries are equal. \r
\r
DE-9IM: TFFFTFFFT"""@en ;
    skos:prefLabel "equals"@en ;
    fno:expects ( funcs:sfEquals_param1 funcs:sfEquals_param2 ),
        ( funcs:sfEquals_param1 funcs:sfEquals_param2 ) ;
    fno:returns ( funcs:sfEquals_output ),
        ( funcs:sfEquals_output ) .

funcs:sfIntersects a skos:Concept,
        sd:Function,
        fno:Function ;
    dcterms:contributor "Matthew Perry" ;
    dcterms:creator "OGC GeoSPARQL 1.0 Standard Working Group" ;
    dcterms:date "2011-06-16"^^xsd:date ;
    dcterms:source <http://www.opengis.net/doc/geosparql/1.0>,
        <http://www.opengis.net/doc/geosparql/1.1> ;
    policy:status status:valid ;
    rdfs:isDefinedBy <http://www.opengis.net/spec/geosparql/1.0>,
        <http://www.opengis.net/spec/geosparql/1.1/req/geometry-topology-extension/sf-query-functions> ;
    rdfs:seeAlso <http://www.opengis.net/doc/geosparql/1.0>,
        <http://www.opengis.net/doc/geosparql/1.1> ;
    skos:definition """A query function that returns true if the input geometries intersect.

DE-9IM: T******** ^ *T******* ^ ***T***** ^ ****T**** """@en,
        """A query function that returns true if the input geometries intersect.\r
\r
DE-9IM: T******** ^ *T******* ^ ***T***** ^ ****T**** """@en ;
    skos:prefLabel "intersects"@en ;
    fno:expects ( funcs:sfIntersects_param1 funcs:sfIntersects_param2 ),
        ( funcs:sfIntersects_param1 funcs:sfIntersects_param2 ) ;
    fno:returns ( funcs:sfIntersects_output ),
        ( funcs:sfIntersects_output ) .

funcs:sfOverlaps a skos:Concept,
        sd:Function,
        fno:Function ;
    dcterms:contributor "Matthew Perry" ;
    dcterms:creator "OGC GeoSPARQL 1.0 Standard Working Group" ;
    dcterms:date "2011-06-16"^^xsd:date ;
    dcterms:source <http://www.opengis.net/doc/geosparql/1.0>,
        <http://www.opengis.net/doc/geosparql/1.1> ;
    policy:status status:valid ;
    rdfs:isDefinedBy <http://www.opengis.net/spec/geosparql/1.0>,
        <http://www.opengis.net/spec/geosparql/1.1/req/geometry-topology-extension/sf-query-functions> ;
    rdfs:seeAlso <http://www.opengis.net/doc/geosparql/1.0>,
        <http://www.opengis.net/doc/geosparql/1.1> ;
    skos:definition """A query function that returns true if the first geometry argument spatially overlaps the second geometry argument.

DE-9IM: T*T***T** """@en,
        """A query function that returns true if the first geometry argument spatially overlaps the second geometry argument.\r
\r
DE-9IM: T*T***T** """@en ;
    skos:prefLabel "overlaps"@en ;
    fno:expects ( funcs:sfOverlaps_param1 funcs:sfOverlaps_param2 ),
        ( funcs:sfOverlaps_param1 funcs:sfOverlaps_param2 ) ;
    fno:returns ( funcs:sfOverlaps_output ),
        ( funcs:sfOverlaps_output ) .

funcs:sfTouches a skos:Concept,
        sd:Function,
        fno:Function ;
    dcterms:contributor "Matthew Perry" ;
    dcterms:creator "OGC GeoSPARQL 1.0 Standard Working Group" ;
    dcterms:date "2011-06-16"^^xsd:date ;
    dcterms:source <http://www.opengis.net/doc/geosparql/1.0>,
        <http://www.opengis.net/doc/geosparql/1.1> ;
    policy:status status:valid ;
    rdfs:isDefinedBy <http://www.opengis.net/spec/geosparql/1.0>,
        <http://www.opengis.net/spec/geosparql/1.1/req/geometry-topology-extension/sf-query-functions> ;
    rdfs:seeAlso <http://www.opengis.net/doc/geosparql/1.0>,
        <http://www.opengis.net/doc/geosparql/1.1> ;
    skos:definition """A query function that returns true if the input geometries touch.

DE-9IM: FT******* ^ F**T***** ^ F***T****"""@en,
        """A query function that returns true if the input geometries touch.\r
\r
DE-9IM: FT******* ^ F**T***** ^ F***T****"""@en ;
    skos:example spec11:B.2.2.3 ;
    skos:prefLabel "touches"@en ;
    fno:expects ( funcs:sfTouches_param1 funcs:sfTouches_param2 ),
        ( funcs:sfTouches_param1 funcs:sfTouches_param2 ) ;
    fno:returns ( funcs:sfTouches_output ),
        ( funcs:sfTouches_output ) .

funcs:sfWithin a skos:Concept,
        sd:Function,
        fno:Function ;
    dcterms:contributor "Matthew Perry" ;
    dcterms:creator "OGC GeoSPARQL 1.0 Standard Working Group" ;
    dcterms:date "2011-06-16"^^xsd:date ;
    dcterms:source <http://www.opengis.net/doc/geosparql/1.0>,
        <http://www.opengis.net/doc/geosparql/1.1> ;
    policy:status status:valid ;
    rdfs:isDefinedBy <http://www.opengis.net/spec/geosparql/1.0>,
        <http://www.opengis.net/spec/geosparql/1.1/req/geometry-topology-extension/sf-query-functions> ;
    rdfs:seeAlso <http://www.opengis.net/doc/geosparql/1.0>,
        <http://www.opengis.net/doc/geosparql/1.1> ;
    skos:definition """A query function that returns true if the first geometry argument is spatially within the second geometry argument. 

DE-9IM: T*F**F***"""@en,
        """A query function that returns true if the first geometry argument is spatially within the second geometry argument. \r
\r
DE-9IM: T*F**F***"""@en ;
    skos:example spec11:B.2.2.2 ;
    skos:prefLabel "within"@en ;
    fno:expects ( funcs:sfWithin_param1 funcs:sfWithin_param2 ),
        ( funcs:sfWithin_param1 funcs:sfWithin_param2 ) ;
    fno:returns ( funcs:sfWithin_output ),
        ( funcs:sfWithin_output ) .

funcs:symDifference a skos:Concept,
        sd:Function,
        fno:Function ;
    dcterms:contributor "Matthew Perry" ;
    dcterms:creator "OGC GeoSPARQL 1.0 Standard Working Group" ;
    dcterms:date "2011-06-16"^^xsd:date ;
    dcterms:source <http://www.opengis.net/doc/geosparql/1.0>,
        <http://www.opengis.net/doc/geosparql/1.1> ;
    policy:status status:valid ;
    rdfs:isDefinedBy <http://www.opengis.net/spec/geosparql/1.0>,
        reqs11gx:query-functions ;
    rdfs:seeAlso <http://www.opengis.net/doc/geosparql/1.0>,
        <http://www.opengis.net/doc/geosparql/1.1> ;
    skos:definition "A query function that returns a geometry consisting of all points that are part of only one input geometry."@en ;
    skos:prefLabel "symmetric difference"@en ;
    fno:expects ( funcs:symDifference_param1 funcs:symDifference_param2 ),
        ( funcs:symDifference_param1 funcs:symDifference_param2 ) ;
    fno:returns ( funcs:symDifference_output ),
        ( funcs:symDifference_output ) .

funcs:union a skos:Concept,
        sd:Function,
        fno:Function ;
    dcterms:contributor "Matthew Perry" ;
    dcterms:creator "OGC GeoSPARQL 1.0 Standard Working Group" ;
    dcterms:date "2011-06-16"^^xsd:date ;
    dcterms:source <http://www.opengis.net/doc/geosparql/1.0>,
        <http://www.opengis.net/doc/geosparql/1.1> ;
    policy:status status:valid ;
    rdfs:isDefinedBy <http://www.opengis.net/spec/geosparql/1.0>,
        reqs11gx:query-functions ;
    rdfs:seeAlso <http://www.opengis.net/doc/geosparql/1.0>,
        <http://www.opengis.net/doc/geosparql/1.1> ;
    skos:definition "A query function that returns a geometry consisting of all points that are part of at least one input geometry."@en ;
    skos:example spec11:B.2.2.3 ;
    skos:prefLabel "union"@en ;
    fno:expects ( funcs:union_param1 funcs:union_param2 ),
        ( funcs:union_param1 funcs:union_param2 ) ;
    fno:returns ( funcs:union_output ),
        ( funcs:union_output ) .

:hasGeometry a rdf:Property,
        owl:ObjectProperty ;
    rdfs:label "hasGeometry"@en ;
    dc:contributor "Matthew Perry" ;
    dc:creator "OGC GeoSPARQL 1.0 Standard Working Group" ;
    dc:date "2011-06-16"^^xsd:date ;
    dc:description """
      A spatial representation for a given feature.
    """@en ;
    rdfs:comment """
      A spatial representation for a given feature.
    """@en ;
    rdfs:domain :Feature ;
    rdfs:isDefinedBy <http://www.opengis.net/ont/geosparql>,
        :,
        <http://www.opengis.net/spec/geosparql/1.0>,
        reqs10gx:feature-properties,
        reqs11gx:feature-properties ;
    rdfs:range :Geometry ;
    skos:definition """
      A spatial representation for a given feature.
    """@en,
        "A spatial representation for a given Feature."@en ;
    skos:example spec11:B.1.1.2.2,
        spec11:B.1.1.2.3,
        spec11:B.1.1.2.4,
        spec11:B.1.1.2.5,
        spec11:B.1.1.2.6,
        spec11:B.1.1.2.8,
        spec11:B.1.1.3.2,
        spec11:B.1.1.3.3,
        spec11:B.1.2.2,
        spec11:B.1.2.3,
        spec11:B.1.2.4,
        spec11:B.2 ;
    skos:prefLabel "has geometry"@en,
        "hasGeometry"@en .

:hasMetricSize a rdf:Property,
        owl:DatatypeProperty ;
    rdfs:domain :SpatialObject ;
    rdfs:isDefinedBy :,
        reqs11gx:spatial-object-properties ;
    rdfs:range xsd:double ;
    skos:definition "Subproperties of this property are used to indicate the size of a Spatial Object, as a measurement or estimate of one or more dimensions of the Spatial Object's spatial presence. Units are always metric (meter, square meter or cubic meter)."@en ;
    skos:prefLabel "has metric size"@en .

:hasSize a rdf:Property,
        owl:ObjectProperty ;
    rdfs:domain :SpatialObject ;
    rdfs:isDefinedBy :,
        <http://www.opengis.net/spec/geosparql/1.0/req/topology-vocab-extension/spatial-object-properties>,
        <http://www.opengis.net/spec/geosparql/1.1/req/topology-vocab-extension/spatial-object-properties> ;
    skos:definition "Subproperties of this property are used to indicate the size of a Spatial Object as a measurement or estimate of one or more dimensions of the Spatial Object's spatial presence."@en ;
    skos:note "The recommended way to specify size is by using a subproperty of hasMetricSize. Subproperties of hasSize can be used if more complex expressions are necessary, for example if the unit of length can not be converted to meter, or if additional data are needed to describe the measurement or estimate."@en ;
    skos:prefLabel "has size"@en .

reqs10gx:gml-literal a spec:Requirement ;
    skos:definition "All geo:gmlLiterals shall consist of a valid element from the GML schema that implements a subtype of GM_Object as defined in [OGC 07-036]"@en ;
    skos:prefLabel "GeoSPARQL 1.0 Requirement: GML Literal"@en .

:hasSerialization a rdf:Property,
        owl:DatatypeProperty ;
    rdfs:label "has serialization"@en ;
    dc:contributor "Matthew Perry" ;
    dc:creator "OGC GeoSPARQL 1.0 Standard Working Group" ;
    dc:date "2011-06-16"^^xsd:date ;
    dc:description """
      Connects a geometry object with its text-based serialization.
    """@en ;
    rdfs:comment """
      Connects a geometry object with its text-based serialization.
    """@en ;
    rdfs:domain :Geometry ;
    rdfs:isDefinedBy <http://www.opengis.net/ont/geosparql>,
        :,
        <http://www.opengis.net/spec/geosparql/1.0>,
        reqs10gx:geometry-properties,
        reqs11gx:geometry-properties ;
    rdfs:range rdfs:Literal ;
    skos:definition """
      Connects a geometry object with its text-based serialization.
    """@en,
        "Connects a Geometry object with its text-based serialization."@en ;
    skos:example spec11:B.1.2.3 ;
    skos:prefLabel "has serialization"@en .

reqs10gx:feature-properties a spec:Requirement ;
    skos:definition "Implementations shall allow the properties geo:hasGeometry and geo:hasDefaultGeometry to be used in SPARQL graph patterns"@en ;
    skos:prefLabel "GeoSPARQL 1.0 Requirement: Feature Properties"@en .

reqs10gx:query-functions a spec:Requirement ;
    skos:definition "Implementations shall support geof:distance, geof:buffer, geof:convexHull, geof:intersection, geof:union, geof:difference, geof:symDifference, geof:envelope and geof:boundary as SPARQL extension functions, consistent with the definitions of the corresponding functions (distance, buffer, convexHull, intersection, difference, symDifference, envelope and boundary respectively) in Simple Features [ISO 19125-1]"@en ;
    skos:prefLabel "GeoSPARQL 1.0 Requirement: Query Functions"@en .

reqs10gx:geometry-properties a spec:Requirement ;
    skos:definition "Implementations shall allow the properties geo:dimension, geo:coordinateDimension, geo:spatialDimension, geo:isEmpty, geo:isSimple, geo:hasSerialization to be used in SPARQL graph patterns"@en ;
    skos:prefLabel "GeoSPARQL 1.0 Requirement: Geometry Properties"@en .

reqs11gx:feature-properties a spec:Requirement ;
    skos:definition "Implementations shall allow the properties geo:hasGeometry, geo:hasDefaultGeometry, geo:hasLength, geo:hasArea, geo:hasVolume geo:hasCentroid, geo:hasBoundingBox and geo:hasSpatialResolution to be used in SPARQL graph patterns"@en ;
    skos:prefLabel "GeoSPARQL 1.1 Requirement: Feature Properties"@en ;
    prov1:wasDerivedFrom reqs10gx:feature-properties .

reqs11gx:geometry-properties a spec:Requirement ;
    skos:definition "Implementations shall allow the properties geo:dimension, geo:coordinateDimension, geo:spatialDimension, geo:isEmpty, geo:isSimple, geo:hasSerialization to be used in SPARQL graph patterns"@en ;
    skos:prefLabel "GeoSPARQL 1.1 Requirement: Geometry Properties"@en ;
    prov1:wasDerivedFrom reqs10gx:geometry-properties .

reqs11gx:sa-functions a spec:Requirement ;
    skos:definition "Implementations shall support geof:concaveHull, geof:boundingCircle, geof:union2, geof:concatLines, geof:centroid, geof:maxX, geof:maxY, geof:maxZ, geof:minX, geof:minY and geof:minZ as a SPARQL extension functions."@en ;
    skos:prefLabel "GeoSPARQL 1.1 Requirement: Spatial Aggregate Functions"@en .

dc: dcterms:modified "2012-06-14"^^xsd:date ;
    dcterms:publisher <http://purl.org/dc/aboutdcmi#DCMI> ;
    dcterms:title "Dublin Core Metadata Element Set, Version 1.1"@en .

<http://www.opengis.net/ont/sf> a owl:Ontology,
        prof:ResourceDescriptor ;
    dc:creator "Open Geospatial Consortium" ;
    dc:date "2012-09-11"^^xsd:date ;
    dc:description "An RDF/OWL vocabulary for defining SimpleFeature geometry types" ;
    dc:title "Simple Features Vocabulary" ;
    dcterms:conformsTo <http://www.w3.org/TR/owl2-rdf-based-semantics/> ;
    dcterms:creator "OGC GeoSPARQL Standards Working Group" ;
    dcterms:description "An RDF/OWL vocabulary for defining SimpleFeature geometry types",
        "An OWL ontology (vocabulary) of the Simple Features geometry types"@en ;
    dcterms:format "text/turtle",
        "text/xml" ;
    dcterms:license "https://www.ogc.org/license"^^xsd:anyURI ;
    dcterms:modified "2022-06-16"^^xsd:date ;
    dcterms:publisher [ a sdo:Organization ;
            sdo:name "Open Geospatial Consortium" ;
            sdo:url "https://www.ogc.org"^^xsd:anyURI ] ;
    dcterms:rights "(c) 2022 Open Geospatial Consortium" ;
    dcterms:title "Simple Features Vocabulary",
        "Simple Features Vocabulary"@en ;
    rdfs:comment "A Turtle format artifact for this Resource is present in the GeoSPARQL 1.0 profile repository. It includes ontology annotations (title, date etc.) not present in the online artifact referenced here."@en ;
    owl:imports <http://www.opengis.net/ont/geosparql> ;
    owl:versionIRI <http://www.opengis.net/ont/sf/1.0>,
        <http://www.opengis.net/ont/sf/1.1> ;
    owl:versionInfo "OGC GeoSPARQL 1.0",
        "OGC GeoSPARQL 1.1" ;
    prof:hasArtifact <http://schemas.opengis.net/sf/1.0/simple_features_geometries.rdf>,
        "https://github.com/opengeospatial/ogc-geosparql/blob/master/1.1/sf_geometries.ttl"^^xsd:anyURI ;
    prof:hasRole role:vocabulary .

reqs11gx:query-functions a spec:Requirement ;
    skos:definition "Implementations shall support the functions geof:boundary geof:buffer, geof:convexHull, geof:coordinateDimension, geof:difference, geof:dimension, geof:distance, geof:envelope, geof:geometryType, geof:getSRID, geof:intersection, geof:is3D, geof:isEmpty, geof:isMeasured, geof:isSimple, geof:spatialDimension, geof:symDifference, geof:transform and geof:union as SPARQL extension functions, consistent with definitions of these functions in Simple Features [ISO19125-1], for non-DGGS geometry literals"@en ;
    skos:prefLabel "GeoSPARQL 1.1 Requirement: Query Functions"@en ;
    prov1:wasDerivedFrom reqs10gx:query-functions .

<http://www.opengis.net/ont/geosparql> a owl:Ontology,
        prof:ResourceDescriptor ;
    dc:creator "Open Geospatial Consortium" ;
    dc:date "2012-04-30"^^xsd:date ;
    dc:description "An RDF/OWL vocabulary for representing spatial information" ;
    dc:source <http://www.opengis.net/doc/IS/geosparql/1.0>,
        "OGC GeoSPARQL  A Geographic Query Language for RDF Data OGC 11-052r5" ;
    dc:title "GeoSPARQL Ontology" ;
    dcterms:conformsTo <http://www.w3.org/TR/owl2-rdf-based-semantics/> ;
    dcterms:contributor [ a sdo:Person ;
            sdo:affiliation "Oracle Corporation" ;
            sdo:email "matthew.perry@oracle.com"^^xsd:anyURI ;
            sdo:name "Matthew Perry" ;
            sdo:url "https://orcid.org/0000-0003-1988-462X"^^xsd:anyURI ],
        [ a sdo:Person ;
            sdo:affiliation "Oracle Corporation" ;
            sdo:email "john.herring@oracle.com"^^xsd:anyURI ;
            sdo:name "John Herring" ],
        [ a sdo:Person ;
            sdo:affiliation "Australian National University",
                "SURROUND Australia Pty Ltd" ;
            sdo:email "nicholas.car@surroundaustralia.com"^^xsd:anyURI ;
            sdo:name "Nicholas J. Car" ;
            sdo:url "https://orcid.org/0000-0002-8742-7730"^^xsd:anyURI ],
        [ a sdo:Person ;
            sdo:affiliation "Geoscape Australia" ;
            sdo:email "joseph.abhayaratna@geoscape.com.au"^^xsd:anyURI ;
            sdo:name "Joseph Abhayaratna" ;
            sdo:url "https://orcid.org/0000-0001-5075-6234"^^xsd:anyURI ],
        [ a sdo:Person ;
            sdo:affiliation "Mainz University Of Applied Sciences" ;
            sdo:email "timo.homburg@hs-mainz.de"^^xsd:anyURI ;
            sdo:name "Timo Homburg" ;
            sdo:url "https://orcid.org/0000-0002-9499-5840"^^xsd:anyURI ],
        [ a sdo:Person ;
            sdo:affiliation "CSIRO Australia" ;
            sdo:email "simon.cox@csiro.au"^^xsd:anyURI ;
            sdo:name "Simon J D Cox" ;
            sdo:url "https://orcid.org/0000-0002-3884-3420"^^xsd:anyURI ],
        [ a sdo:Person ;
            sdo:email "fjknibbe@gmail.com"^^xsd:anyURI ;
            sdo:name "Frans Knibbe" ;
            sdo:url "https://orcid.org/0000-0003-3789-2260"^^xsd:anyURI ],
        [ a sdo:Person ;
            sdo:affiliation "KU Leuven",
                "Neanex Technologies" ;
            sdo:email "mathias.bonduel@neanex.com"^^xsd:anyURI ;
            sdo:name "Mathias Bonduel" ;
            sdo:url "https://orcid.org/0000-0002-3313-924X"^^xsd:anyURI ] ;
    dcterms:created "2020-09-09"^^xsd:date ;
    dcterms:creator "OGC GeoSPARQL Standards Working Group" ;
    dcterms:description "An RDF/OWL vocabulary for representing spatial information"@en,
        "The GeoSPARQL 1.1 ontology in RDF (turtle)"@en ;
    dcterms:format "application/rdf+xml",
        "text/turtle" ;
    dcterms:license "https://www.ogc.org/license"^^xsd:anyURI ;
    dcterms:modified "2021-10-27"^^xsd:date ;
    dcterms:publisher [ a sdo:Organization ;
            sdo:name "Open Geospatial Consortium" ;
            sdo:url "https://www.ogc.org"^^xsd:anyURI ] ;
    dcterms:replaces <http://www.opengis.net/ont/geosparql/1.0> ;
    dcterms:rights "(c) 2021 Open Geospatial Consortium" ;
    dcterms:source <http://www.opengis.net/doc/IS/geosparql/1.1>,
        "OGC GeoSPARQL - A Geographic Query Language for RDF Data OGC 11-052r5"@en ;
    dcterms:title "GeoSPARQL Ontology",
        "GeoSPARQL Ontology"@en ;
    rdfs:seeAlso <http://www.opengis.net/def/function/ogc-geosparql/1.0>,
        <http://www.opengis.net/def/rule/ogc-geosparql/1.0>,
        <http://www.opengis.net/doc/IS/geosparql/1.0>,
        <http://www.opengis.net/doc/IS/geosparql/1.1> ;
    owl:versionIRI <http://www.opengis.net/ont/geosparql/1.0>,
        <http://www.opengis.net/ont/geosparql/1.1> ;
    owl:versionInfo "OGC GeoSPARQL 1.0",
        "OGC GeoSPARQL 1.1" ;
    prof:hasArtifact <http://schemas.opengis.net/geosparql/1.0/geosparql_vocab_all.rdf>,
        "https://github.com/opengeospatial/ogc-geosparql/master/1.1/geo.ttl"^^xsd:anyURI ;
    prof:hasRole role:schema,
        role:scheme .

:dggsLiteral a rdfs:Datatype ;
    rdfs:isDefinedBy :,
        reqs11gx:dggs-literal ;
    rdfs:seeAlso <http://www.opengis.net/doc/AS/dggs/2.0> ;
    skos:definition "A textual serialization of a Discrete Global Grid (DGGS) Geometry object."@en ;
    skos:example spec11:B.1.2.4,
        " \"<https://w3id.org/dggs/auspix> OrdinateList (R3234)\"^^<http://www.opengis.net/ont/geosparql#dggsLiteral>" ;
    skos:prefLabel "DGGS Literal"@en ;
    skos:scopeNote "This datatype is not expected to be used directly but to serve as an abstract datatype for a series of specific DGGS literal types, for specific DGGS implementations"@en .

:geoJSONLiteral a rdfs:Datatype ;
    rdfs:isDefinedBy :,
        reqs11gx:geojson-literal ;
    rdfs:seeAlso <https://tools.ietf.org/html/rfc7946> ;
    skos:definition "A GeoJSON serialization of a Geometry object."@en ;
    skos:example spec11:B.1.2.4 ;
    skos:prefLabel "GeoJSON Literal"@en .

:gmlLiteral a rdfs:Datatype ;
    rdfs:label "GML Literal"@en ;
    dc:contributor "Matthew Perry" ;
    dc:creator "OGC GeoSPARQL 1.0 Standard Working Group" ;
    dc:date "2011-06-16"^^xsd:date ;
    dc:description """
      A GML serialization of a geometry object.
    """@en ;
    rdfs:comment """
      A GML serialization of a geometry object.
    """@en ;
    rdfs:isDefinedBy <http://www.opengis.net/ont/geosparql>,
        :,
        <http://www.opengis.net/spec/geosparql/1.0>,
        reqs10gx:gml-literal,
        reqs11gx:gml-literal ;
    rdfs:seeAlso <https://portal.ogc.org/files/?artifact_id=20509> ;
    skos:definition """
      A GML serialization of a geometry object.
    """@en,
        "A GML serialization of a Geometry object."@en ;
    skos:example spec11:B.1.2.4 ;
    skos:prefLabel "GML Literal"@en .

:kmlLiteral a rdfs:Datatype ;
    rdfs:isDefinedBy :,
        reqs11gx:kml-literal ;
    rdfs:seeAlso <https://www.ogc.org/standards/kml/> ;
    skos:definition "A KML serialization of a Geometry object."@en ;
    skos:example spec11:B.1.2.4 ;
    skos:prefLabel "KML Literal"@en .

:wktLiteral a rdfs:Datatype ;
    rdfs:label "Well-known Text Literal"@en ;
    dc:contributor "Matthew Perry" ;
    dc:creator "OGC GeoSPARQL 1.0 Standard Working Group" ;
    dc:date "2011-06-16"^^xsd:date ;
    dc:description """
      A Well-known Text serialization of a geometry object.
    """@en ;
    rdfs:comment """
      A Well-known Text serialization of a geometry object.
    """@en ;
    rdfs:isDefinedBy <http://www.opengis.net/ont/geosparql>,
        :,
        <http://www.opengis.net/spec/geosparql/1.0>,
        reqs10gx:wkt-literal,
        reqs11gx:wkt-literal ;
    rdfs:seeAlso <https://portal.ogc.org/files/?artifact_id=25355> ;
    skos:definition """
      A Well-known Text serialization of a geometry object.
    """@en,
        "A Well-known Text serialization of a Geometry object."@en ;
    skos:example spec11:B.2.2.2 ;
    skos:prefLabel "Well-known Text Literal"@en .

