<?xml version="1.0" encoding="UTF-8"?>
<rdf:RDF xmlns:rdf="http://www.w3.org/1999/02/22-rdf-syntax-ns#" xmlns:rdfs="http://www.w3.org/2000/01/rdf-schema#" xmlns:skos="http://www.w3.org/2004/02/skos/core#" xmlns:dc="http://purl.org/dc/elements/1.1/" xmlns:dct="http://purl.org/dc/terms/" xml:lang="en">

# This file includes the CaLAThe concept scheme part of the 5th version of CaLAThe, which is available online at cadastralvocabulary.org/CaLAThe.rdf
The present CaLAThe concept scheme part and the corresponding CaLATheCodeList concept scheme part are provided in separate files. #



	<skos:ConceptScheme rdf:about="https://www.opengis.net/def/CaLAThe/5.0">
		<skos:prefLabel>CaLAThe 5.0</skos:prefLabel>
		<dc:title>CaLAThe - Cadastre and Land Administration Thesaurus, version 5.0</dc:title>
		<skos:description>The Thesaurus for the domain of Cadastre and Land Administration, CaLAThe, regards the surveying and mapping of land, more specifically the boundaries of land parcels and individually owned buildings and building parts (condominiums), as performed by the profession of surveyors. From a public point of view, the domain provides the administrative and technical base for taxation of land and buildings, and for land use planning; from a private point of view, the domain supports security in ownership and other land-related rights. CaLAThe lies partly within the technical domains of civil engineering and computer science, partly within social science domains, including law and public administration</skos:description>
		<dc:description>The Cadastre and Land Administration Thesaurus, CaLAThe, is a controlled vocabulary, recorded at http://www.cadastralvocabulary.org. The initial 2011 version of CaLAThe was prepared based on terms and term relationships derived from DIS version of the ISO 19152:2012 Land Administration Domain Model (LADM). Moreover, it referred to existing thesauri, primarily the GEMET thesaurus, the AGROVOC thesaurus, and the STW Thesaurus for Economics. Terms rendering dynamic or temporal aspects of the domain were added in version 2, while version 3 was supplemented with terms from the OGC Land and Infrastructure Conceptual Model Standard (LandInfra). Version 4 added code lists names and values from both standards, specified within its own skos:ConceptScheme. The code list values refer to CaLAThe thesaurus terms when possible in a meaningful way. Version 5 started a multi-lingual itinerary by adding terms (skos:prefLabel) in Danish and Turkish, the native language of the authors. The corresponding code list part, version 2, includes code lists specified in Land and Survey parts of OGC LandInfra. Also, a skos:Collection statement was added to specify relations between the two skos:ConceptSchemes. - The content of the present file may be queried by means of the SKOS Play facility at http://labs.sparna.fr/skos-play/. SKOS Play offers presentation of each of the two concept schemes, as well as each of the three languages. Validated through http://demo.seco.tkk.fi/skosify/skosify</dc:description>
		<dc:creator>Erik Stubkjær</dc:creator>
		<dc:creator> Volkan Çağdaş</dc:creator>
		<dc:date>2021-09-06</dc:date>
		<dct:issued>2021-09-06</dct:issued>
		<skos:hasTopConcept rdf:resource="https://www.opengis.net/def/CaLAThe/5.0/Party"/>
		<skos:hasTopConcept rdf:resource="https://www.opengis.net/def/CaLAThe/5.0/Law"/>
		<skos:hasTopConcept rdf:resource="https://www.opengis.net/def/CaLAThe/5.0/Information"/>
		<skos:hasTopConcept rdf:resource="https://www.opengis.net/def/CaLAThe/5.0/Land"/>
		<skos:hasTopConcept rdf:resource="https://www.opengis.net/def/CaLAThe/5.0/Activity"/>
		<skos:hasTopConcept rdf:resource="https://www.opengis.net/def/CaLAThe/5.0/Survey"/>
	</skos:ConceptScheme>

	<skos:Concept rdf:about="https://www.opengis.net/def/CaLAThe/5.0/2D">
		<skos:prefLabel xml:lang="en">2D</skos:prefLabel>
		<skos:prefLabel xml:lang="da">2D</skos:prefLabel>
		<skos:prefLabel xml:lang="tr">2B</skos:prefLabel>
		<skos:scopeNote>OGC LandInfra / InfraGML term</skos:scopeNote>
		<skos:definition>Dimension type, cf. OGC LandInfra 7.10.6 SpatialUnit</skos:definition>
		<skos:changeNote>Established with version 4</skos:changeNote>
		<skos:inScheme rdf:resource="https://www.opengis.net/def/CaLAThe/5.0"/>
		<skos:broader rdf:resource="https://www.opengis.net/def/CaLAThe/5.0/DimensionType"/>
	</skos:Concept>
	<skos:Concept rdf:about="https://www.opengis.net/def/CaLAThe/5.0/3D">
		<skos:prefLabel xml:lang="en">3D</skos:prefLabel>
		<skos:prefLabel xml:lang="da">3D</skos:prefLabel>
		<skos:prefLabel xml:lang="tr">3B</skos:prefLabel>
		<skos:scopeNote>OGC LandInfra / InfraGML term</skos:scopeNote>
		<skos:definition>Dimension type, cf. OGC LandInfra 7.10.6 SpatialUnit</skos:definition>
		<skos:changeNote>Established with version 4</skos:changeNote>
		<skos:inScheme rdf:resource="https://www.opengis.net/def/CaLAThe/5.0"/>
		<skos:broader rdf:resource="https://www.opengis.net/def/CaLAThe/5.0/DimensionType"/>
	</skos:Concept>
	<skos:Concept rdf:about="https://www.opengis.net/def/CaLAThe/5.0/Activity">
		<skos:prefLabel xml:lang="en">Activity</skos:prefLabel>
		<skos:prefLabel xml:lang="da">Aktivitet</skos:prefLabel>
		<skos:prefLabel xml:lang="tr">Aktivite</skos:prefLabel>
		<skos:scopeNote>EULIS / ELRA glossary term</skos:scopeNote>
		<skos:definition>The act by which land or property rights are registered (Source: EULIS / ELRA glossary).</skos:definition>
		<skos:changeNote>Established with version 2. Narrower ParcelEstablishment added with version 3. Survey with version 4.</skos:changeNote>
		<skos:inScheme rdf:resource="https://www.opengis.net/def/CaLAThe/5.0"/>
		<skos:topConceptOf rdf:resource="https://www.opengis.net/def/CaLAThe/5.0"/>
		<skos:altLabel>Transaction</skos:altLabel>
		<skos:altLabel>Registration</skos:altLabel>
		<skos:narrower rdf:resource="https://www.opengis.net/def/CaLAThe/5.0/Exchange"/>
		<skos:narrower rdf:resource="https://www.opengis.net/def/CaLAThe/5.0/PropertyFormation"/>
		<skos:narrower rdf:resource="https://www.opengis.net/def/CaLAThe/5.0/Transfer"/>
	</skos:Concept>
	<skos:Concept rdf:about="https://www.opengis.net/def/CaLAThe/5.0/AdministrativeUnit">
		<skos:prefLabel xml:lang="en">Administrative unit</skos:prefLabel>
		<skos:prefLabel xml:lang="da">Administrativ inddeling</skos:prefLabel>
		<skos:prefLabel xml:lang="tr">İdari birim</skos:prefLabel>
		<skos:scopeNote>GEMET term</skos:scopeNote>
		<skos:definition>Unit of administration where a Member State has and/or exercises jurisdictional rights, for local, regional and national governance (Source: INSPIRE feature concept dictionary).</skos:definition>
		<skos:changeNote>Established with version 1. Edited with version 3 and 4. Definition is revised in version 5.</skos:changeNote>
		<skos:exactMatch rdf:resource="http://inspire.ec.europa.eu/featureconcept/AdministrativeUnit"/>
	<skos:exactMatch rdf:resource="http://eurovoc.europa.eu/362"/>
		<skos:inScheme rdf:resource="https://www.opengis.net/def/CaLAThe/5.0"/>
		<skos:altLabel>Jurisdiction</skos:altLabel>
		<skos:altLabel>LA_SpatialUnitGroup</skos:altLabel>
		<skos:altLabel>Administrative division</skos:altLabel>
		<skos:broader rdf:resource="https://www.opengis.net/def/CaLAThe/5.0/LandDivision"/>
		<skos:narrower rdf:resource="https://www.opengis.net/def/CaLAThe/5.0/NUTSRegion"/>
		<skos:narrower rdf:resource="https://www.opengis.net/def/CaLAThe/5.0/ProtectedSite"/>
		<skos:narrower rdf:resource="https://www.opengis.net/def/CaLAThe/5.0/Site"/>
	</skos:Concept>
	<skos:Concept rdf:about="https://www.opengis.net/def/CaLAThe/5.0/AdversePossession">
		<skos:prefLabel xml:lang="en">Adverse possession</skos:prefLabel>
		<skos:prefLabel xml:lang="da">Ejendomshævd</skos:prefLabel>
		<skos:prefLabel xml:lang="tr">Kazandırıcı zaman aşımı</skos:prefLabel>
		<skos:changeNote>Established with version 2.</skos:changeNote>
		<skos:inScheme rdf:resource="https://www.opengis.net/def/CaLAThe/5.0"/>
		<skos:altLabel>Prescriptive acquisition</skos:altLabel>
		<skos:broader rdf:resource="https://www.opengis.net/def/CaLAThe/5.0/Ownership"/>
	</skos:Concept>
	<skos:Concept rdf:about="https://www.opengis.net/def/CaLAThe/5.0/AerialPhotograph">
		<skos:prefLabel xml:lang="en">Aerial photograph</skos:prefLabel>
		<skos:prefLabel xml:lang="da">Luftfoto</skos:prefLabel>
		<skos:prefLabel xml:lang="tr">Hava fotoğrafı</skos:prefLabel>
		<skos:scopeNote>GEMET term</skos:scopeNote>
		<skos:definition>An image of the ground surface made on a light-sensitive material and taken at a high altitude from an aircraft, spacecraft or rocket (Source: GEMET).</skos:definition>
		<skos:changeNote>Established with version 1.</skos:changeNote>
		<skos:exactMatch rdf:resource="http://aims.fao.org/aos/agrovoc/c_be37a91c"/>
		<skos:inScheme rdf:resource="https://www.opengis.net/def/CaLAThe/5.0"/>
		<skos:broader rdf:resource="https://www.opengis.net/def/CaLAThe/5.0/DigitalImagery"/>
	</skos:Concept>
	<skos:Concept rdf:about="https://www.opengis.net/def/CaLAThe/5.0/Amalgamation">
		<skos:prefLabel xml:lang="en">Amalgamation</skos:prefLabel>
		<skos:prefLabel xml:lang="da">Sammenlægning</skos:prefLabel>
		<skos:prefLabel xml:lang="tr">Birleştirme, tevhit</skos:prefLabel>
		<skos:changeNote>Established with version 2.</skos:changeNote>
		<skos:inScheme rdf:resource="https://www.opengis.net/def/CaLAThe/5.0"/>
		<skos:broader rdf:resource="https://www.opengis.net/def/CaLAThe/5.0/PropertyFormation"/>
	</skos:Concept>
	<skos:Concept rdf:about="https://www.opengis.net/def/CaLAThe/5.0/AngelObservation">
		<skos:prefLabel xml:lang="en">Angle observation</skos:prefLabel>
		<skos:prefLabel xml:lang="da">Vinkelobservation</skos:prefLabel>
		<skos:prefLabel xml:lang="tr">Açı gözlemi</skos:prefLabel>
		<skos:changeNote>Established with version 4</skos:changeNote>
		<skos:inScheme rdf:resource="https://www.opengis.net/def/CaLAThe/5.0"/>
		<skos:broader rdf:resource="https://www.opengis.net/def/CaLAThe/5.0/Observation"/>
		<skos:broader rdf:resource="https://www.opengis.net/def/CaLAThe/5.0/Theodolite"/>
	</skos:Concept>
	<skos:Concept rdf:about="https://www.opengis.net/def/CaLAThe/5.0/Association">
		<skos:prefLabel xml:lang="en">Association</skos:prefLabel>
		<skos:prefLabel xml:lang="da">Forening</skos:prefLabel>
		<skos:prefLabel xml:lang="tr">Birlik</skos:prefLabel>
		<skos:scopeNote>GEMET term</skos:scopeNote>
		<skos:definition>A body of persons associated for the regulation of a common economic activity by means of a special organization (Source: GEMET).</skos:definition>
		<skos:changeNote>Established with version 1.</skos:changeNote>
		<skos:exactMatch rdf:resource="http://www.eionet.europa.eu/gemet/concept/607"/>
		<skos:exactMatch rdf:resource="http://eurovoc.europa.eu/2944"/>
		<skos:inScheme rdf:resource="https://www.opengis.net/def/CaLAThe/5.0"/>
		<skos:broader rdf:resource="https://www.opengis.net/def/CaLAThe/5.0/Organisation"/>
		<skos:narrower rdf:resource="https://www.opengis.net/def/CaLAThe/5.0/ProfessionalSociety"/>
	</skos:Concept>
	<skos:Concept rdf:about="https://www.opengis.net/def/CaLAThe/5.0/Bank">
		<skos:prefLabel xml:lang="en">Bank</skos:prefLabel>
		<skos:prefLabel xml:lang="da">Bank</skos:prefLabel>
		<skos:prefLabel xml:lang="tr">Banka</skos:prefLabel>
		<skos:scopeNote>ISO LADM term</skos:scopeNote>
		<skos:changeNote>Established with version 1.</skos:changeNote>
		<skos:exactMatch rdf:resource="http://zbw.eu/stw/descriptor/13283-4"/>
		<skos:exactMatch rdf:resource="http://aims.fao.org/aos/agrovoc/c_812"/>
		<skos:exactMatch rdf:resource="http://eurovoc.europa.eu/4738"/>
		<skos:inScheme rdf:resource="https://www.opengis.net/def/CaLAThe/5.0"/>
		<skos:broader rdf:resource="https://www.opengis.net/def/CaLAThe/5.0/Corporation"/>
	</skos:Concept>
	<skos:Concept rdf:about="https://www.opengis.net/def/CaLAThe/5.0/BEString">
		<skos:prefLabel xml:lang="en">BEString</skos:prefLabel>
		<skos:prefLabel xml:lang="da">.</skos:prefLabel>
		<skos:prefLabel xml:lang="tr">.</skos:prefLabel>
		<skos:scopeNote>OGC LandInfra / InfraGML term</skos:scopeNote>
		<skos:definition>A one-dimensional geometric string representation, limited to curves of type LineString; CircularString; CompoundCurve constructed from LineStrings, CircularStrings, and/or other CompoundCurves; or MultiCurve of any of the previously specified types. (LandInfra 7.10.7)</skos:definition>
		<skos:changeNote>Established with version 4</skos:changeNote>
		<skos:inScheme rdf:resource="https://www.opengis.net/def/CaLAThe/5.0"/>
		<skos:broader rdf:resource="https://www.opengis.net/def/CaLAThe/5.0/BoundingElement"/>
		<skos:narrower rdf:resource="https://www.opengis.net/def/CaLAThe/5.0/StringType"/>
		<skos:narrower rdf:resource="https://www.opengis.net/def/CaLAThe/5.0/LineString"/>
	</skos:Concept>
	<skos:Concept rdf:about="https://www.opengis.net/def/CaLAThe/5.0/Boundary">
		<skos:prefLabel xml:lang="en">Boundary</skos:prefLabel>
		<skos:prefLabel xml:lang="da">Grænse, Matrikelskel</skos:prefLabel>
		<skos:prefLabel xml:lang="tr">Sınır</skos:prefLabel>
		<skos:scopeNote>ISO LADM and OGC LandInfra / InfraGML term</skos:scopeNote>
		<skos:definition>Set that represents the limit of an entity. Note 1 to entry: Boundary is most commonly used in the context of geometry, where the set is a collection of points or a collection of objects that represent those points. In other arenas, the term is used metaphorically to describe the transition between an entity and the rest of its domain of discourse (Source: OGC LandInfra 4.8.3, referring to ISO 19107:2003, 4.4; ISO 19152:2012 4.1.3).</skos:definition>
		<skos:changeNote>Established with version 2. Definition added with version 3.</skos:changeNote>
		<skos:inScheme rdf:resource="https://www.opengis.net/def/CaLAThe/5.0"/>
		<skos:altLabel>LA_Boundary</skos:altLabel>
		<skos:broader rdf:resource="https://www.opengis.net/def/CaLAThe/5.0/LandDivision"/>
		<skos:narrower rdf:resource="https://www.opengis.net/def/CaLAThe/5.0/BoundaryMark"/>
	</skos:Concept>
	<skos:Concept rdf:about="https://www.opengis.net/def/CaLAThe/5.0/BoundaryMark">
		<skos:prefLabel xml:lang="en">Boundary mark</skos:prefLabel>
		<skos:prefLabel xml:lang="da">Skelmærke, Grænsesten</skos:prefLabel>
		<skos:prefLabel xml:lang="tr">Sınır işareti</skos:prefLabel>
		<skos:definition>Physical object which by its form defines a point on the surface of the Earth, which is stably located, and which is recorded in a statement. It may carry a symbol of authority, which communicates its purpose, e.g. marking of the legal boundary between two Land parcels according to jurisdiction-specific provisions (Source: OGC LandInfra, 4.8.16; 7.10.5.1).</skos:definition>
		<skos:changeNote>Established with version 1. Definition with version 3.</skos:changeNote>
		<skos:inScheme rdf:resource="https://www.opengis.net/def/CaLAThe/5.0"/>
		<skos:altLabel>Boundary monument</skos:altLabel>
		<skos:broader rdf:resource="https://www.opengis.net/def/CaLAThe/5.0/Boundary"/>
		<skos:broader rdf:resource="https://www.opengis.net/def/CaLAThe/5.0/SurveyMark"/>
		<skos:related rdf:resource="https://www.opengis.net/def/CaLAThe/5.0/CadastralParcel"/>
	</skos:Concept>
	<skos:Concept rdf:about="https://www.opengis.net/def/CaLAThe/5.0/BoundaryRe-measurement">
		<skos:prefLabel xml:lang="en">Boundary re-measurement</skos:prefLabel>
		<skos:prefLabel xml:lang="da">Teknisk ændring</skos:prefLabel>
		<skos:prefLabel xml:lang="tr">.</skos:prefLabel>
		<skos:changeNote>Established with version 2.</skos:changeNote>
		<skos:inScheme rdf:resource="https://www.opengis.net/def/CaLAThe/5.0"/>
		<skos:broader rdf:resource="https://www.opengis.net/def/CaLAThe/5.0/BoundarySurveyAndMarking"/>
	</skos:Concept>
	<skos:Concept rdf:about="https://www.opengis.net/def/CaLAThe/5.0/BoundaryRectification">
		<skos:prefLabel xml:lang="en">Boundary rectification</skos:prefLabel>
		<skos:prefLabel xml:lang="da">Ejendomsberigtigelse</skos:prefLabel>
		<skos:prefLabel xml:lang="tr">Sınır düzeltmesi</skos:prefLabel>
		<skos:changeNote>Established with version 2.</skos:changeNote>
		<skos:inScheme rdf:resource="https://www.opengis.net/def/CaLAThe/5.0"/>
		<skos:broader rdf:resource="https://www.opengis.net/def/CaLAThe/5.0/BoundarySurveyAndMarking"/>
	</skos:Concept>
	<skos:Concept rdf:about="https://www.opengis.net/def/CaLAThe/5.0/BoundarySurveyAndMarking">
		<skos:prefLabel xml:lang="en">Boundary survey and marking</skos:prefLabel>
		<skos:prefLabel xml:lang="da">Afmærkning og indmåling af ske</skos:prefLabel>
		<skos:prefLabel xml:lang="tr">Sınırlandırma ve ölçme</skos:prefLabel>
		<skos:changeNote>Established with version 2.0. Narrower added in version 3.</skos:changeNote>
		<skos:inScheme rdf:resource="https://www.opengis.net/def/CaLAThe/5.0"/>
		<skos:broader rdf:resource="https://www.opengis.net/def/CaLAThe/5.0/Subdivision"/>
		<skos:narrower rdf:resource="https://www.opengis.net/def/CaLAThe/5.0/BoundaryRectification"/>
		<skos:narrower rdf:resource="https://www.opengis.net/def/CaLAThe/5.0/LegalBoundaryDetermination"/>
		<skos:narrower rdf:resource="https://www.opengis.net/def/CaLAThe/5.0/BoundaryRe-measurement"/>
		<skos:narrower rdf:resource="https://www.opengis.net/def/CaLAThe/5.0/SurveyMonumentEstablishment"/>
	</skos:Concept>
	<skos:Concept rdf:about="https://www.opengis.net/def/CaLAThe/5.0/BoundingElement">
		<skos:prefLabel xml:lang="en">Bounding element</skos:prefLabel>
		<skos:prefLabel xml:lang="da">Begrænsende element</skos:prefLabel>
		<skos:prefLabel xml:lang="tr">Sınırlandırıcı eleman</skos:prefLabel>
		<skos:scopeNote>OGC LandInfra / InfraGML term</skos:scopeNote>
		<skos:definition>A Bounding element describe or define all or part of the geometry and location of the a Spatial unit (OGC LandInfra, 7.10.7).</skos:definition>
		<skos:changeNote>Established with version 3.</skos:changeNote>
		<skos:inScheme rdf:resource="https://www.opengis.net/def/CaLAThe/5.0"/>
		<skos:broader rdf:resource="https://www.opengis.net/def/CaLAThe/5.0/SpatialUnit"/>
		<skos:narrower rdf:resource="https://www.opengis.net/def/CaLAThe/5.0/BEString"/>
		<skos:narrower rdf:resource="https://www.opengis.net/def/CaLAThe/5.0/LA_BoundaryFaceString"/>
	</skos:Concept>
	<skos:Concept rdf:about="https://www.opengis.net/def/CaLAThe/5.0/BuildingUsePart">
		<skos:prefLabel xml:lang="en">Building use part</skos:prefLabel>
		<skos:prefLabel xml:lang="da">Ejerlejlighedslod</skos:prefLabel>
		<skos:prefLabel xml:lang="tr">Bina kullanım bölümü</skos:prefLabel>
		<skos:scopeNote>OGC LandInfra / InfraGML term</skos:scopeNote>
		<skos:definition>Part of a floor of a multi-storage building, subdivided according to management and use by a lawful process (Source: OGC LandInfra, 4.8.2; Compares to ISO 19152:2012 4.1.6 building unit, and to Ifc 5.4.3.51 SpatialZone).</skos:definition>
		<skos:changeNote>Established with version 1. Definition added with version 3.</skos:changeNote>
		<skos:inScheme rdf:resource="https://www.opengis.net/def/CaLAThe/5.0"/>
		<skos:altLabel>Building part</skos:altLabel>
		<skos:broader rdf:resource="https://www.opengis.net/def/CaLAThe/5.0/Condominium"/>
		<skos:broader rdf:resource="https://www.opengis.net/def/CaLAThe/5.0/CondominiumBuilding"/>
	</skos:Concept>
	<skos:Concept rdf:about="https://www.opengis.net/def/CaLAThe/5.0/Buyer">
		<skos:prefLabel xml:lang="en">Buyer</skos:prefLabel>
		<skos:prefLabel xml:lang="da">Køber</skos:prefLabel>
		<skos:prefLabel xml:lang="tr">Alıcı</skos:prefLabel>
		<skos:scopeNote>OGC LandInfra / InfraGML term</skos:scopeNote>
		<skos:changeNote>Established with version 4</skos:changeNote>
		<skos:inScheme rdf:resource="https://www.opengis.net/def/CaLAThe/5.0"/>
		<skos:broader rdf:resource="https://www.opengis.net/def/CaLAThe/5.0/Signatory"/>
	</skos:Concept>
	<skos:Concept rdf:about="https://www.opengis.net/def/CaLAThe/5.0/CadastralAccount">
		<skos:prefLabel xml:lang="en">Cadastral account</skos:prefLabel>
		<skos:prefLabel xml:lang="da">Skematisk redegørelse</skos:prefLabel>
		<skos:prefLabel xml:lang="tr">Tescil bildirimi</skos:prefLabel>
		<skos:scopeNote>OGC LandInfra / InfraGML term</skos:scopeNote>
		<skos:definition>Land surveyors account of parcel and boundary changes, with references to pertinent legislation, intended for recording body (land administration agency, cadastral authority) (Source: OGC LandInfra, 7.10.4.1).</skos:definition>
		<skos:changeNote>Established with version 3.</skos:changeNote>
		<skos:inScheme rdf:resource="https://www.opengis.net/def/CaLAThe/5.0"/>
		<skos:broader rdf:resource="https://www.opengis.net/def/CaLAThe/5.0/Document"/>
	</skos:Concept>
	<skos:Concept rdf:about="https://www.opengis.net/def/CaLAThe/5.0/CadastralMap">
		<skos:prefLabel xml:lang="en">Cadastral map</skos:prefLabel>
		<skos:prefLabel xml:lang="da">Matrikelkort</skos:prefLabel>
		<skos:prefLabel xml:lang="tr">Kadastral harita</skos:prefLabel>
		<skos:definition>A map showing land (cadastral) parcel boundaries (Source: UNECE, 1996).</skos:definition>
		<skos:exactMatch rdf:resource="http://aims.fao.org/aos/agrovoc/c_fdee7675"/>
		<skos:inScheme rdf:resource="https://www.opengis.net/def/CaLAThe/5.0"/>
		<skos:broader rdf:resource="https://www.opengis.net/def/CaLAThe/5.0/Map"/>
		<skos:broader rdf:resource="https://www.opengis.net/def/CaLAThe/5.0/Cadastre"/>
	</skos:Concept>
	<skos:Concept rdf:about="https://www.opengis.net/def/CaLAThe/5.0/CadastralParcel">
		<skos:prefLabel xml:lang="en">Cadastral parcel</skos:prefLabel>
		<skos:prefLabel xml:lang="da">Jordstykke, lod</skos:prefLabel>
		<skos:prefLabel xml:lang="tr">Kadastral parsel</skos:prefLabel>
		<skos:scopeNote>INSPIRE theme</skos:scopeNote>
		<skos:definition>Contiguous part of the surface of the Earth, as specified through lawful process (Source: OGC LandInfra / InfraGML, 4.8.11).</skos:definition>
		<skos:changeNote>Established with version 1. Definition and Land parcel alternative term with version 3.</skos:changeNote>
		<skos:exactMatch rdf:resource="http://inspire.ec.europa.eu/featureconcept/CadastralParcel"/>
		<skos:inScheme rdf:resource="https://www.opengis.net/def/CaLAThe/5.0"/>
		<skos:altLabel>Land parcel</skos:altLabel>
		<skos:altLabel>Parcel</skos:altLabel>
		<skos:broader rdf:resource="https://www.opengis.net/def/CaLAThe/5.0/RealProperty"/>
		<skos:narrower rdf:resource="https://www.opengis.net/def/CaLAThe/5.0/CarrierParcel"/>
		<skos:narrower rdf:resource="https://www.opengis.net/def/CaLAThe/5.0/MainParcel"/>
		<skos:related rdf:resource="https://www.opengis.net/def/CaLAThe/5.0/BoundaryMark"/>
	</skos:Concept>
	<skos:Concept rdf:about="https://www.opengis.net/def/CaLAThe/5.0/CadastralSurveyDocument">
		<skos:prefLabel xml:lang="en">Cadastral survey document</skos:prefLabel>
		<skos:prefLabel xml:lang="da">Måleblad</skos:prefLabel>
		<skos:prefLabel xml:lang="tr">Kadastral ölçü belgesi</skos:prefLabel>
		<skos:definition>Land surveyors account of changes, with references to pertinent legislation, intended for recording body (land administration agency, cadastral authority) (Motivated by OGC LandInfra / InfraGML 7.10.4.1).</skos:definition>
		<skos:changeNote>Established with version 1. Definition added in version 3.</skos:changeNote>
		<skos:inScheme rdf:resource="https://www.opengis.net/def/CaLAThe/5.0"/>
		<skos:broader rdf:resource="https://www.opengis.net/def/CaLAThe/5.0/Document"/>
		<skos:related rdf:resource="https://www.opengis.net/def/CaLAThe/5.0/Registrar"/>
		<skos:related rdf:resource="https://www.opengis.net/def/CaLAThe/5.0/Cadastre"/>
	</skos:Concept>
	<skos:Concept rdf:about="https://www.opengis.net/def/CaLAThe/5.0/CadastralSystem">
		<skos:prefLabel xml:lang="en">Cadastral system</skos:prefLabel>
		<skos:prefLabel xml:lang="da">Matrikel-og tinglysningssystem</skos:prefLabel>
		<skos:prefLabel xml:lang="tr">Kadastral sistem</skos:prefLabel>
		<skos:definition>Combination of land register and cadastre (Source: Adopted from https://doi.org/10.1016/S0198-9715(00)00051-X)</skos:definition>
		<skos:changeNote>Established with version 1.</skos:changeNote>
		<skos:inScheme rdf:resource="https://www.opengis.net/def/CaLAThe/5.0"/>
		<skos:broader rdf:resource="https://www.opengis.net/def/CaLAThe/5.0/Cadastre"/>
		<skos:broader rdf:resource="https://www.opengis.net/def/CaLAThe/5.0/LandRegister"/>
	</skos:Concept>
	<skos:Concept rdf:about="https://www.opengis.net/def/CaLAThe/5.0/Cadastre">
		<skos:prefLabel xml:lang="en">Cadastre</skos:prefLabel>
		<skos:prefLabel xml:lang="da">Matrikel, Matrikelregister</skos:prefLabel>
		<skos:prefLabel xml:lang="tr">Kadastro</skos:prefLabel>
		<skos:scopeNote>AGROVOC Multilingual Thesaurus term</skos:scopeNote>
		<skos:definition>A public record, survey, or map of the value, extent, and ownership of land as a basis of taxation (AGROVOC Multilingual Thesaurus).</skos:definition>
		<skos:changeNote>Established with version 1.</skos:changeNote>
		<skos:exactMatch rdf:resource="http://aims.fao.org/aos/agrovoc/c_1177"/>
		<skos:inScheme rdf:resource="https://www.opengis.net/def/CaLAThe/5.0"/>
		<skos:broader rdf:resource="https://www.opengis.net/def/CaLAThe/5.0/Registry"/>
		<skos:broader rdf:resource="https://www.opengis.net/def/CaLAThe/5.0/GeographicalInformationSystem"/>
		<skos:narrower rdf:resource="https://www.opengis.net/def/CaLAThe/5.0/CadastralMap"/>
		<skos:narrower rdf:resource="https://www.opengis.net/def/CaLAThe/5.0/CadastralSystem"/>
	</skos:Concept>
	<skos:Concept rdf:about="https://www.opengis.net/def/CaLAThe/5.0/Camera">
		<skos:prefLabel xml:lang="en">Camera</skos:prefLabel>
		<skos:prefLabel xml:lang="da">Kamera</skos:prefLabel>
		<skos:prefLabel xml:lang="tr">Kamera</skos:prefLabel>
		<skos:changeNote>Established with version 4</skos:changeNote>
		<skos:inScheme rdf:resource="https://www.opengis.net/def/CaLAThe/5.0"/>
		<skos:broader rdf:resource="https://www.opengis.net/def/CaLAThe/5.0/SurveyingInstrument"/>
		<skos:narrower rdf:resource="https://www.opengis.net/def/CaLAThe/5.0/Image"/>
	</skos:Concept>
	<skos:Concept rdf:about="https://www.opengis.net/def/CaLAThe/5.0/CarrierParcel">
		<skos:prefLabel xml:lang="en">Carrier parcel</skos:prefLabel>
		<skos:prefLabel xml:lang="da">Reference-parcel</skos:prefLabel>
		<skos:prefLabel xml:lang="tr">Yüklü parsel</skos:prefLabel>
		<skos:scopeNote>OGC LandInfra / InfraGML term</skos:scopeNote>
		<skos:definition>Land parcel on which a condominium building is located or which carries a superficies, that is a building or construction, established and owned by a person on land leased from another person (Source: OGC LandInfra, 7.10.2.4).</skos:definition>
		<skos:changeNote>Established with version 3.</skos:changeNote>
		<skos:inScheme rdf:resource="https://www.opengis.net/def/CaLAThe/5.0"/>
		<skos:broader rdf:resource="https://www.opengis.net/def/CaLAThe/5.0/CadastralParcel"/>
		<skos:related rdf:resource="https://www.opengis.net/def/CaLAThe/5.0/CondominiumBuilding"/>
		<skos:related rdf:resource="https://www.opengis.net/def/CaLAThe/5.0/SuperficieObject"/>
	</skos:Concept>
	<skos:Concept rdf:about="https://www.opengis.net/def/CaLAThe/5.0/Certificate">
		<skos:prefLabel xml:lang="en">Certificate</skos:prefLabel>
		<skos:prefLabel xml:lang="da">Certifikat</skos:prefLabel>
		<skos:prefLabel xml:lang="tr">Sertifika</skos:prefLabel>
		<skos:changeNote>Established with version 1.</skos:changeNote>
		<skos:inScheme rdf:resource="https://www.opengis.net/def/CaLAThe/5.0"/>
		<skos:broader rdf:resource="https://www.opengis.net/def/CaLAThe/5.0/Document"/>
		<skos:narrower rdf:resource="https://www.opengis.net/def/CaLAThe/5.0/PropertyEnquiryCertificate"/>
	</skos:Concept>
	<skos:Concept rdf:about="https://www.opengis.net/def/CaLAThe/5.0/ChangeOfPropertyUnitType">
		<skos:prefLabel xml:lang="en">Change of property unit type</skos:prefLabel>
		<skos:prefLabel xml:lang="da">Ændring af ejendomstype</skos:prefLabel>
		<skos:prefLabel xml:lang="tr">Cins değişikliği</skos:prefLabel>
		<skos:changeNote>Established with version 2.</skos:changeNote>
		<skos:inScheme rdf:resource="https://www.opengis.net/def/CaLAThe/5.0"/>
		<skos:broader rdf:resource="https://www.opengis.net/def/CaLAThe/5.0/PropertyFormation"/>
		<skos:narrower rdf:resource="https://www.opengis.net/def/CaLAThe/5.0/CondominiumSubdivision"/>
	</skos:Concept>
	<skos:Concept rdf:about="https://www.opengis.net/def/CaLAThe/5.0/Chief">
		<skos:prefLabel xml:lang="en">Chief</skos:prefLabel>
		<skos:prefLabel xml:lang="da">Høvding</skos:prefLabel>
		<skos:prefLabel xml:lang="tr">Şef</skos:prefLabel>
		<skos:scopeNote>ISO LADM term</skos:scopeNote>
		<skos:changeNote>Established with version 1.</skos:changeNote>
		<skos:inScheme rdf:resource="https://www.opengis.net/def/CaLAThe/5.0"/>
		<skos:broader rdf:resource="https://www.opengis.net/def/CaLAThe/5.0/SocietalRole"/>
	</skos:Concept>
	<skos:Concept rdf:about="https://www.opengis.net/def/CaLAThe/5.0/CoOwnership">
		<skos:prefLabel xml:lang="en">Co-ownership</skos:prefLabel>
		<skos:prefLabel xml:lang="da">Sameje</skos:prefLabel>
		<skos:prefLabel xml:lang="tr">Paylı mülkiyet</skos:prefLabel>
		<skos:definition>Divided or undivided concurrent ownership exercised towards a property (Source: Legal Dictionary of Property in Canada - Dualjuridik). Where two or more people own the same property (Source: EULIS / ELRA glossary).</skos:definition>
		<skos:changeNote>Replaced to Shared ownership in version 3.</skos:changeNote>
		<skos:inScheme rdf:resource="https://www.opengis.net/def/CaLAThe/5.0"/>
		<skos:altLabel>Shared ownership</skos:altLabel>
		<skos:broader rdf:resource="https://www.opengis.net/def/CaLAThe/5.0/Ownership"/>
		<skos:narrower rdf:resource="https://www.opengis.net/def/CaLAThe/5.0/CondominiumRight"/>
		<skos:narrower rdf:resource="https://www.opengis.net/def/CaLAThe/5.0/TimeshareRight"/>
		<skos:narrower rdf:resource="https://www.opengis.net/def/CaLAThe/5.0/CoOwnershipShare"/>
		<skos:narrower rdf:resource="https://www.opengis.net/def/CaLAThe/5.0/RightOfSuperficie"/>
	</skos:Concept>
	<skos:Concept rdf:about="https://www.opengis.net/def/CaLAThe/5.0/CoOwnershipShare">
		<skos:prefLabel xml:lang="en">Co-ownership share</skos:prefLabel>
		<skos:prefLabel xml:lang="da">Andel i fælleseje</skos:prefLabel>
		<skos:prefLabel xml:lang="tr">Mülkiyet payı</skos:prefLabel>
		<skos:changeNote>Established with version 3.</skos:changeNote>
		<skos:inScheme rdf:resource="https://www.opengis.net/def/CaLAThe/5.0"/>
		<skos:broader rdf:resource="https://www.opengis.net/def/CaLAThe/5.0/CoOwnership"/>
		<skos:narrower rdf:resource="https://www.opengis.net/def/CaLAThe/5.0/PartyShare"/>
		<skos:narrower rdf:resource="https://www.opengis.net/def/CaLAThe/5.0/CondominiumShare"/>
	</skos:Concept>
	<skos:Concept rdf:about="https://www.opengis.net/def/CaLAThe/5.0/CollectiveOwnership">
		<skos:prefLabel xml:lang="en">Collective ownership</skos:prefLabel>
		<skos:prefLabel xml:lang="da">Ejendomsfællesskab</skos:prefLabel>
		<skos:prefLabel xml:lang="tr">Birlikte mülkiyet</skos:prefLabel>
		<skos:changeNote>Established with version 3.</skos:changeNote>
		<skos:exactMatch rdf:resource="http://aims.fao.org/aos/agrovoc/c_29157"/>
		<skos:inScheme rdf:resource="https://www.opengis.net/def/CaLAThe/5.0"/>
		<skos:broader rdf:resource="https://www.opengis.net/def/CaLAThe/5.0/CustomaryLaw"/>
	</skos:Concept>
	<skos:Concept rdf:about="https://www.opengis.net/def/CaLAThe/5.0/Compass">
		<skos:prefLabel xml:lang="en">Compass</skos:prefLabel>
		<skos:prefLabel xml:lang="da">Kompas</skos:prefLabel>
		<skos:prefLabel xml:lang="tr">Pusula</skos:prefLabel>
		<skos:scopeNote>OGC LandInfra / InfraGML term</skos:scopeNote>
		<skos:changeNote>Established with version 4</skos:changeNote>
		<skos:inScheme rdf:resource="https://www.opengis.net/def/CaLAThe/5.0"/>
		<skos:broader rdf:resource="https://www.opengis.net/def/CaLAThe/5.0/SurveyingInstrument"/>
	</skos:Concept>
	<skos:Concept rdf:about="https://www.opengis.net/def/CaLAThe/5.0/Condominium">
		<skos:prefLabel xml:lang="en">Condominium</skos:prefLabel>
		<skos:prefLabel xml:lang="da">Ejerlejlighed, ej.hedskompleks</skos:prefLabel>
		<skos:prefLabel xml:lang="tr">Bağımsız bölüm</skos:prefLabel>
		<skos:scopeNote>OGC LandInfra / InfraGML term</skos:scopeNote>
		<skos:definition>Concurrent ownership of real property that has been divided into private and common portions (Legal Dictionary of Property in Canada - Dualjuridik). Note 1 to entry: Condominium unit owners must be members of a mandatory owners  association and engage in the maintenance of joint facilities according to a specified share (Source: OGC LandInfra, 4.8.4).</skos:definition>
		<skos:changeNote>Established with version 3.</skos:changeNote>
		<skos:inScheme rdf:resource="https://www.opengis.net/def/CaLAThe/5.0"/>
		<skos:altLabel>Condominium unit</skos:altLabel>
		<skos:broader rdf:resource="https://www.opengis.net/def/CaLAThe/5.0/RealProperty"/>
		<skos:narrower rdf:resource="https://www.opengis.net/def/CaLAThe/5.0/BuildingUsePart"/>
		<skos:related rdf:resource="https://www.opengis.net/def/CaLAThe/5.0/CondominiumRight"/>
		<skos:related rdf:resource="https://www.opengis.net/def/CaLAThe/5.0/CondominiumScheme"/>
	</skos:Concept>
	<skos:Concept rdf:about="https://www.opengis.net/def/CaLAThe/5.0/CondominiumAcquisition">
		<skos:prefLabel xml:lang="en">Condominium acquisition</skos:prefLabel>
		<skos:prefLabel xml:lang="da">Erhvervelse af ejerlejlighed</skos:prefLabel>
		<skos:prefLabel xml:lang="tr">Bağısmsız bölüm edinimi</skos:prefLabel>
		<skos:scopeNote>OGC LandInfra / InfraGML term</skos:scopeNote>
		<skos:definition>Transfer of ownership from a seller to a buyer, where seller is either the owner of the original Property unit or the owner of a Condominium unit (Source: OGC LandInfra, 7.10.4.1).</skos:definition>
		<skos:changeNote>Established with version 3.</skos:changeNote>
		<skos:inScheme rdf:resource="https://www.opengis.net/def/CaLAThe/5.0"/>
		<skos:broader rdf:resource="https://www.opengis.net/def/CaLAThe/5.0/Conveyance"/>
	</skos:Concept>
	<skos:Concept rdf:about="https://www.opengis.net/def/CaLAThe/5.0/CondominiumBuilding">
		<skos:prefLabel xml:lang="en">Condominium building</skos:prefLabel>
		<skos:prefLabel xml:lang="da">Bygning, opdelt i ejerlejlighe</skos:prefLabel>
		<skos:prefLabel xml:lang="tr">Kat mülkiyetine konu bina</skos:prefLabel>
		<skos:scopeNote>OGC LandInfra / InfraGML term</skos:scopeNote>
		<skos:definition>A Building containing Condominium units subject to a single CondominiumScheme (Source: OGC LandInfra, 7.11.3).</skos:definition>
		<skos:changeNote>Established with version 3.</skos:changeNote>
		<skos:inScheme rdf:resource="https://www.opengis.net/def/CaLAThe/5.0"/>
		<skos:broader rdf:resource="https://www.opengis.net/def/CaLAThe/5.0/Construction"/>
		<skos:narrower rdf:resource="https://www.opengis.net/def/CaLAThe/5.0/BuildingUsePart"/>
		<skos:narrower rdf:resource="https://www.opengis.net/def/CaLAThe/5.0/LA_LegalSpaceBuildingUnit"/>
		<skos:related rdf:resource="https://www.opengis.net/def/CaLAThe/5.0/CarrierParcel"/>
	</skos:Concept>
	<skos:Concept rdf:about="https://www.opengis.net/def/CaLAThe/5.0/CondominiumRight">
		<skos:prefLabel xml:lang="en">Condominium right</skos:prefLabel>
		<skos:prefLabel xml:lang="da">Ejerlejlighedsadkomst</skos:prefLabel>
		<skos:prefLabel xml:lang="tr">Kat mülkiyeti</skos:prefLabel>
		<skos:definition>Type of co-ownership right.</skos:definition>
		<skos:changeNote>Established with version 1, changed and defined with version 3.</skos:changeNote>
		<skos:inScheme rdf:resource="https://www.opengis.net/def/CaLAThe/5.0"/>
		<skos:altLabel>Apartment ownership</skos:altLabel>
		<skos:broader rdf:resource="https://www.opengis.net/def/CaLAThe/5.0/CoOwnership"/>
		<skos:related rdf:resource="https://www.opengis.net/def/CaLAThe/5.0/Condominium"/>
	</skos:Concept>
	<skos:Concept rdf:about="https://www.opengis.net/def/CaLAThe/5.0/CondominiumScheme">
		<skos:prefLabel xml:lang="en">Condominium scheme</skos:prefLabel>
		<skos:prefLabel xml:lang="da">Ejerlejlighedsfortegnelse mv</skos:prefLabel>
		<skos:prefLabel xml:lang="tr">(Kat mülkiyeti) Yönetim planı</skos:prefLabel>
		<skos:scopeNote>OGC LandInfra / InfraGML term</skos:scopeNote>
		<skos:definition>Documentation of interest in land in terms of a statement concerning the building parts which make up a number of condominium units and the share of joint facilities of each condominium unit (Source: OGC LandInfra, 4.8.5).</skos:definition>
		<skos:changeNote>Established with version 3.</skos:changeNote>
		<skos:inScheme rdf:resource="https://www.opengis.net/def/CaLAThe/5.0"/>
		<skos:broader rdf:resource="https://www.opengis.net/def/CaLAThe/5.0/Document"/>
	</skos:Concept>
	<skos:Concept rdf:about="https://www.opengis.net/def/CaLAThe/5.0/CondominiumShare">
		<skos:prefLabel xml:lang="en">Condominium share</skos:prefLabel>
		<skos:prefLabel xml:lang="da">Fordelingstal</skos:prefLabel>
		<skos:prefLabel xml:lang="tr">Arsa payı</skos:prefLabel>
		<skos:changeNote>Established with version 3.</skos:changeNote>
		<skos:inScheme rdf:resource="https://www.opengis.net/def/CaLAThe/5.0"/>
		<skos:broader rdf:resource="https://www.opengis.net/def/CaLAThe/5.0/CoOwnershipShare"/>
	</skos:Concept>
	<skos:Concept rdf:about="https://www.opengis.net/def/CaLAThe/5.0/CondominiumSubdivision">
		<skos:prefLabel xml:lang="en">Condominium subdivision</skos:prefLabel>
		<skos:prefLabel xml:lang="da">Opdeling i ejerlejligheder</skos:prefLabel>
		<skos:prefLabel xml:lang="tr">Bağımsız bölüm ifrazı</skos:prefLabel>
		<skos:scopeNote>OGC LandInfra / InfraGML term</skos:scopeNote>
		<skos:definition>Subdivision of a multi-storage building into ownership units through a scheme, which for each unit specifies one or more Building use parts and a share in the joint facilities. (Source: OGC LandInfra, 7.10.4.1).</skos:definition>
		<skos:changeNote>Established with version 2. Definition added with version 3.</skos:changeNote>
		<skos:inScheme rdf:resource="https://www.opengis.net/def/CaLAThe/5.0"/>
		<skos:broader rdf:resource="https://www.opengis.net/def/CaLAThe/5.0/Subdivision"/>
		<skos:broader rdf:resource="https://www.opengis.net/def/CaLAThe/5.0/ChangeOfPropertyUnitType"/>
	</skos:Concept>
	<skos:Concept rdf:about="https://www.opengis.net/def/CaLAThe/5.0/Construction">
		<skos:prefLabel xml:lang="en">Construction</skos:prefLabel>
		<skos:prefLabel xml:lang="da">Teknisk anlæg</skos:prefLabel>
		<skos:prefLabel xml:lang="tr">İnşaat</skos:prefLabel>
		<skos:scopeNote>OGC LandInfra / InfraGML term</skos:scopeNote>
		<skos:definition>Assembled or complete part of construction works that results from work on-site [ISO 6707-1:2014] (Source: OGC LandInfra, 4.2.4).</skos:definition>
		<skos:changeNote>Established with version 3.</skos:changeNote>
		<skos:inScheme rdf:resource="https://www.opengis.net/def/CaLAThe/5.0"/>
		<skos:altLabel>Building</skos:altLabel>
		<skos:broader rdf:resource="https://www.opengis.net/def/CaLAThe/5.0/TopographicalFeature"/>
		<skos:narrower rdf:resource="https://www.opengis.net/def/CaLAThe/5.0/CondominiumBuilding"/>
		<skos:narrower rdf:resource="https://www.opengis.net/def/CaLAThe/5.0/SuperficieObject"/>
	</skos:Concept>
	<skos:Concept rdf:about="https://www.opengis.net/def/CaLAThe/5.0/ControlPointMonument">
		<skos:prefLabel xml:lang="en">Control point monument</skos:prefLabel>
		<skos:prefLabel xml:lang="da">Fikspunktmærke</skos:prefLabel>
		<skos:prefLabel xml:lang="tr">Kontrol noktası tesisi</skos:prefLabel>
		<skos:changeNote>Established with version 1.</skos:changeNote>
		<skos:inScheme rdf:resource="https://www.opengis.net/def/CaLAThe/5.0"/>
		<skos:altLabel>Survey monument</skos:altLabel>
		<skos:broader rdf:resource="https://www.opengis.net/def/CaLAThe/5.0/SurveyMark"/>
	</skos:Concept>
	<skos:Concept rdf:about="https://www.opengis.net/def/CaLAThe/5.0/Conveyance">
		<skos:prefLabel xml:lang="en">Conveyance</skos:prefLabel>
		<skos:prefLabel xml:lang="da">Overdragelse</skos:prefLabel>
		<skos:prefLabel xml:lang="tr">Devir</skos:prefLabel>
		<skos:changeNote>Established with version 2.</skos:changeNote>
		<skos:inScheme rdf:resource="https://www.opengis.net/def/CaLAThe/5.0"/>
		<skos:altLabel>Sale</skos:altLabel>
		<skos:altLabel>Purchase</skos:altLabel>
		<skos:broader rdf:resource="https://www.opengis.net/def/CaLAThe/5.0/Exchange"/>
		<skos:narrower rdf:resource="https://www.opengis.net/def/CaLAThe/5.0/CondominiumAcquisition"/>
		<skos:narrower rdf:resource="https://www.opengis.net/def/CaLAThe/5.0/ParcelAcquisition"/>
	</skos:Concept>
	<skos:Concept rdf:about="https://www.opengis.net/def/CaLAThe/5.0/Coordinate">
		<skos:prefLabel xml:lang="en">Coordinate</skos:prefLabel>
		<skos:prefLabel xml:lang="da">Koordinat</skos:prefLabel>
		<skos:prefLabel xml:lang="tr">Koordinat</skos:prefLabel>
		<skos:definition>One of a sequence of n numbers designating the position of a point in n-dimensional space. Note to entry: In a coordinate reference system, the coordinate numbers are qualified by units. (Geolexica, ISO 19111:2007)</skos:definition>
		<skos:changeNote>Established with version 4</skos:changeNote>
		<skos:exactMatch rdf:resource="https://isotc211.geolexica.org/concepts/2038/"/>
		<skos:inScheme rdf:resource="https://www.opengis.net/def/CaLAThe/5.0"/>
		<skos:broader rdf:resource="https://www.opengis.net/def/CaLAThe/5.0/CoordinateReferenceSystem"/>
	</skos:Concept>
	<skos:Concept rdf:about="https://www.opengis.net/def/CaLAThe/5.0/CoordinateReferenceSystem">
		<skos:prefLabel xml:lang="en">Coordinate reference system</skos:prefLabel>
		<skos:prefLabel xml:lang="da">Koordinatreferencesystem</skos:prefLabel>
		<skos:prefLabel xml:lang="tr">Koordinat referans sistemi</skos:prefLabel>
		<skos:scopeNote>INSPIRE term</skos:scopeNote>
		<skos:definition>1) Systems for uniquely referencing spatial information in space as a set of coordinates (x, y, z) and/or latitude and longitude and height, based on a geodetic horizontal and vertical datum (Source: INSPIRE glossary). 2) Coordinate system that is related to an object by a datum (Source: ISO 19111:2019, (E), 3.1.9).</skos:definition>
		<skos:changeNote>Established with version 1.</skos:changeNote>
		<skos:exactMatch rdf:resource="http://inspire.ec.europa.eu/glossary/CRS"/>
		<skos:exactMatch rdf:resource="https://isotc211.geolexica.org/concepts/703/"/>
		<skos:inScheme rdf:resource="https://www.opengis.net/def/CaLAThe/5.0"/>
		<skos:broader rdf:resource="https://www.opengis.net/def/CaLAThe/5.0/SpatialReference"/>
		<skos:narrower rdf:resource="https://www.opengis.net/def/CaLAThe/5.0/Coordinate"/>
		<skos:narrower rdf:resource="https://www.opengis.net/def/CaLAThe/5.0/Datum"/>
		<skos:narrower rdf:resource="https://www.opengis.net/def/CaLAThe/5.0/CoordinateTuple"/>
	</skos:Concept>
	<skos:Concept rdf:about="https://www.opengis.net/def/CaLAThe/5.0/CoordinateTuple">
		<skos:prefLabel xml:lang="en">Coordinate tuple</skos:prefLabel>
		<skos:prefLabel xml:lang="da">Koordinat tupel</skos:prefLabel>
		<skos:prefLabel xml:lang="tr">Koordinat üçlüsü</skos:prefLabel>
		<skos:scopeNote>Geolexica term</skos:scopeNote>
		<skos:definition>Tuple composed of a sequence of coordinates. Note to entry: The number of coordinates in the coordinate tuple equals the dimension of the coordinate system; the order of coordinates in the coordinate tuple is identical to the order of the axes of the coordinate system. (ISO 19111:2019, (E), 3.1.13)</skos:definition>
		<skos:changeNote>Established with version 4</skos:changeNote>
		<skos:exactMatch rdf:resource="https://isotc211.geolexica.org/concepts/735/"/>
		<skos:inScheme rdf:resource="https://www.opengis.net/def/CaLAThe/5.0"/>
		<skos:broader rdf:resource="https://www.opengis.net/def/CaLAThe/5.0/CoordinateReferenceSystem"/>
	</skos:Concept>
	<skos:Concept rdf:about="https://www.opengis.net/def/CaLAThe/5.0/Corporation">
		<skos:prefLabel xml:lang="en">Corporation</skos:prefLabel>
		<skos:prefLabel xml:lang="da">Virksomhed, aktieselskab</skos:prefLabel>
		<skos:prefLabel xml:lang="tr">İşletme</skos:prefLabel>
		<skos:scopeNote>STW Thesaurus for Economics term</skos:scopeNote>
		<skos:changeNote>Established with version 1.</skos:changeNote>
		<skos:exactMatch rdf:resource="http://zbw.eu/stw/descriptor/12186-0"/>
		<skos:inScheme rdf:resource="https://www.opengis.net/def/CaLAThe/5.0"/>
		<skos:broader rdf:resource="https://www.opengis.net/def/CaLAThe/5.0/Organisation"/>
		<skos:narrower rdf:resource="https://www.opengis.net/def/CaLAThe/5.0/Bank"/>
	</skos:Concept>
	<skos:Concept rdf:about="https://www.opengis.net/def/CaLAThe/5.0/Correction">
		<skos:prefLabel xml:lang="en">Correction</skos:prefLabel>
		<skos:prefLabel xml:lang="da">Korrektion</skos:prefLabel>
		<skos:prefLabel xml:lang="tr">Düzeltme</skos:prefLabel>
		<skos:scopeNote>OGC LandInfra / InfraGML term</skos:scopeNote>
		<skos:changeNote>Established with version 4</skos:changeNote>
		<skos:inScheme rdf:resource="https://www.opengis.net/def/CaLAThe/5.0"/>
		<skos:broader rdf:resource="https://www.opengis.net/def/CaLAThe/5.0/Observation"/>
	</skos:Concept>
	<skos:Concept rdf:about="https://www.opengis.net/def/CaLAThe/5.0/Curve">
		<skos:prefLabel xml:lang="en">Curve</skos:prefLabel>
		<skos:prefLabel xml:lang="da">Kurve</skos:prefLabel>
		<skos:prefLabel xml:lang="tr">Eğri</skos:prefLabel>
		<skos:scopeNote>Geolexica term</skos:scopeNote>
		<skos:definition>1-dimensional geometric primitive, representing the continuous image of a line. Note to entry: The boundary of a curve is the set of points at either end of the curve. If the curve is a cycle, the two ends are identical, and the curve (if topologically closed) is considered to not have a boundary. The first point is called the start point, and the last is the end point. Connectivity of the curve is guaranteed by the "continuous image of a line" clause. A topological theorem states that a continuous image of a connected set is connected. (Geolexica ISO 19107:2003)</skos:definition>
		<skos:changeNote>Established with version 4</skos:changeNote>
		<skos:exactMatch rdf:resource="https://isotc211.geolexica.org/concepts/101/"/>
		<skos:inScheme rdf:resource="https://www.opengis.net/def/CaLAThe/5.0"/>
		<skos:broader rdf:resource="https://www.opengis.net/def/CaLAThe/5.0/GeometricPrimitive"/>
		<skos:broader rdf:resource="https://www.opengis.net/def/CaLAThe/5.0/Polygon"/>
		<skos:narrower rdf:resource="https://www.opengis.net/def/CaLAThe/5.0/LineString"/>
	</skos:Concept>
	<skos:Concept rdf:about="https://www.opengis.net/def/CaLAThe/5.0/CustomaryLaw">
		<skos:prefLabel xml:lang="en">Customary law</skos:prefLabel>
		<skos:prefLabel xml:lang="da">Sædvaneret</skos:prefLabel>
		<skos:prefLabel xml:lang="tr">Geleneksel hukuk</skos:prefLabel>
		<skos:changeNote>Established with version 1. Custom made preferred term with version 3.</skos:changeNote>
		<skos:exactMatch rdf:resource="http://aims.fao.org/aos/agrovoc/c_10222"/>
		<skos:inScheme rdf:resource="https://www.opengis.net/def/CaLAThe/5.0"/>
		<skos:altLabel>Informal right</skos:altLabel>
		<skos:altLabel>Indigenous right</skos:altLabel>
		<skos:altLabel>Custom</skos:altLabel>
		<skos:broader rdf:resource="https://www.opengis.net/def/CaLAThe/5.0/Law"/>
		<skos:narrower rdf:resource="https://www.opengis.net/def/CaLAThe/5.0/CollectiveOwnership"/>
	</skos:Concept>
	<skos:Concept rdf:about="https://www.opengis.net/def/CaLAThe/5.0/Datum">
		<skos:prefLabel xml:lang="en">Datum</skos:prefLabel>
		<skos:prefLabel xml:lang="da">Datum</skos:prefLabel>
		<skos:prefLabel xml:lang="tr">Datum</skos:prefLabel>
		<skos:scopeNote>Geolexica term</skos:scopeNote>
		<skos:definition>Parameter or set of parameters that realize the position of the origin, the scale, and the orientation of a coordinate system (Geolexica ISO 19111:2019).</skos:definition>
		<skos:changeNote>Established with version 4</skos:changeNote>
		<skos:exactMatch rdf:resource="https://isotc211.geolexica.org/concepts/2376/"/>
		<skos:inScheme rdf:resource="https://www.opengis.net/def/CaLAThe/5.0"/>
		<skos:broader rdf:resource="https://www.opengis.net/def/CaLAThe/5.0/CoordinateReferenceSystem"/>
	</skos:Concept>
	<skos:Concept rdf:about="https://www.opengis.net/def/CaLAThe/5.0/Deed">
		<skos:prefLabel xml:lang="en">Deed</skos:prefLabel>
		<skos:prefLabel xml:lang="da">Beseglet dokument, skøde</skos:prefLabel>
		<skos:prefLabel xml:lang="tr">Sözleşme</skos:prefLabel>
		<skos:changeNote>Established with version 1.</skos:changeNote>
		<skos:exactMatch rdf:resource="http://aims.fao.org/aos/agrovoc/c_c10cdeb5"/>
		<skos:exactMatch rdf:resource="http://eurovoc.europa.eu/164"/>
		<skos:inScheme rdf:resource="https://www.opengis.net/def/CaLAThe/5.0"/>
		<skos:broader rdf:resource="https://www.opengis.net/def/CaLAThe/5.0/Document"/>
		<skos:narrower rdf:resource="https://www.opengis.net/def/CaLAThe/5.0/MortgageDeed"/>
		<skos:narrower rdf:resource="https://www.opengis.net/def/CaLAThe/5.0/TitleDeed"/>
		<skos:narrower rdf:resource="https://www.opengis.net/def/CaLAThe/5.0/RestrictionDeed"/>
	</skos:Concept>
	<skos:Concept rdf:about="https://www.opengis.net/def/CaLAThe/5.0/CodeList">
		<skos:prefLabel xml:lang="en">Code list</skos:prefLabel>
		<skos:prefLabel xml:lang="da">Kodeliste </skos:prefLabel>
		<skos:prefLabel xml:lang="tr">Kod listesi</skos:prefLabel>
		<skos:definition>1. Value domain including a code for each permissible value (Geolexica ISO 19136:2007)
			2. Complete set of data element values of a coded simple data element (ADMS Controlled Vocabularies ISO 9735-1:2002, 4.14)
			- A code list is identified by a name and comprises a set of values</skos:definition>
		<skos:narrower rdf:resource="https://www.opengis.net/def/CaLAThe/5.0/UserDefinedValue"/>
		<skos:changeNote>Established with version 5.</skos:changeNote>
		<skos:inScheme rdf:resource="https://www.opengis.net/def/CaLAThe/5.0"/>
		<skos:broader rdf:resource="https://www.opengis.net/def/CaLAThe/5.0/Information"/>
	</skos:Concept>
	<skos:Concept rdf:about="https://www.opengis.net/def/CaLAThe/5.0/DesignPoint">
		<skos:prefLabel xml:lang="en">Design point</skos:prefLabel>
		<skos:prefLabel xml:lang="da">Designkoordinat</skos:prefLabel>
		<skos:prefLabel xml:lang="tr">.</skos:prefLabel>
		<skos:scopeNote>OGC LandInfra / InfraGML term</skos:scopeNote>
		<skos:changeNote>Established with version 4</skos:changeNote>
		<skos:inScheme rdf:resource="https://www.opengis.net/def/CaLAThe/5.0"/>
		<skos:broader rdf:resource="https://www.opengis.net/def/CaLAThe/5.0/GNSSsensor"/>
		<skos:broader rdf:resource="https://www.opengis.net/def/CaLAThe/5.0/TotalStation"/>
		<skos:narrower rdf:resource="https://www.opengis.net/def/CaLAThe/5.0/Stakeout"/>
	</skos:Concept>
	<skos:Concept rdf:about="https://www.opengis.net/def/CaLAThe/5.0/DigitalImagery">
		<skos:prefLabel xml:lang="en">Digital imagery</skos:prefLabel>
		<skos:prefLabel xml:lang="da">Digitalt billedmateriale</skos:prefLabel>
		<skos:prefLabel xml:lang="tr">Sayısal görüntü</skos:prefLabel>
		<skos:definition>Raster graphics image</skos:definition>
		<skos:changeNote>Established with version 1. Edited with version 4</skos:changeNote>
		<skos:inScheme rdf:resource="https://www.opengis.net/def/CaLAThe/5.0"/>
		<skos:broader rdf:resource="https://www.opengis.net/def/CaLAThe/5.0/GeolocatedInformation"/>
		<skos:narrower rdf:resource="https://www.opengis.net/def/CaLAThe/5.0/SatelliteImage"/>
		<skos:narrower rdf:resource="https://www.opengis.net/def/CaLAThe/5.0/AerialPhotograph"/>
		<skos:narrower rdf:resource="https://www.opengis.net/def/CaLAThe/5.0/Orthoimagery"/>
	</skos:Concept>
	<skos:Concept rdf:about="https://www.opengis.net/def/CaLAThe/5.0/DimensionType">
		<skos:prefLabel xml:lang="en">Dimension type</skos:prefLabel>
		<skos:prefLabel xml:lang="da">Dimensionstype</skos:prefLabel>
		<skos:prefLabel xml:lang="tr">Boyut türü</skos:prefLabel>
		<skos:scopeNote>OGC LandInfra / InfraGML term</skos:scopeNote>
		<skos:changeNote>Established with version 4</skos:changeNote>
		<skos:inScheme rdf:resource="https://www.opengis.net/def/CaLAThe/5.0"/>
		<skos:broader rdf:resource="https://www.opengis.net/def/CaLAThe/5.0/SpatialUnit"/>
		<skos:narrower rdf:resource="https://www.opengis.net/def/CaLAThe/5.0/2D"/>
		<skos:narrower rdf:resource="https://www.opengis.net/def/CaLAThe/5.0/3D"/>
		<skos:narrower rdf:resource="https://www.opengis.net/def/CaLAThe/5.0/Liminal"/>
	</skos:Concept>
	<skos:Concept rdf:about="https://www.opengis.net/def/CaLAThe/5.0/DistanceObservation">
		<skos:prefLabel xml:lang="en">Distance observation</skos:prefLabel>
		<skos:prefLabel xml:lang="da">Afstandsobservation</skos:prefLabel>
		<skos:prefLabel xml:lang="tr">Mesafe gözlemi</skos:prefLabel>
		<skos:scopeNote>OGC LandInfra / InfraGML term</skos:scopeNote>
		<skos:changeNote>Established with version 4</skos:changeNote>
		<skos:inScheme rdf:resource="https://www.opengis.net/def/CaLAThe/5.0"/>
		<skos:broader rdf:resource="https://www.opengis.net/def/CaLAThe/5.0/Observation"/>
		<skos:broader rdf:resource="https://www.opengis.net/def/CaLAThe/5.0/MeasuringTape"/>
		<skos:broader rdf:resource="https://www.opengis.net/def/CaLAThe/5.0/EletronicDistanceMeter"/>
	</skos:Concept>
	<skos:Concept rdf:about="https://www.opengis.net/def/CaLAThe/5.0/Document">
		<skos:prefLabel xml:lang="en">Document</skos:prefLabel>
		<skos:prefLabel xml:lang="da">Dokument</skos:prefLabel>
		<skos:prefLabel xml:lang="tr">Belge</skos:prefLabel>
		<skos:scopeNote>GEMET term</skos:scopeNote>
		<skos:definition>Material of any kind, regardless of physical form, which furnishes information, evidence or ideas, including items such as contracts, bills of sale, letters, audio and video recordings, and machine readable data files  (Source: GEMET). Information in permanent form which is approved by one or more signatures (Source: OGC LandInfra, 4.1.7, Compares to ISO 19152:2012 4.1.21 source).</skos:definition>
		<skos:changeNote>Established with version 1. Definition edited and alternative term added with version 3.</skos:changeNote>
		<skos:exactMatch rdf:resource="http://www.eionet.europa.eu/gemet/concept/2282"/>
		<skos:exactMatch rdf:resource="http://aims.fao.org/aos/agrovoc/c_4f435f4f"/>
		<skos:exactMatch rdf:resource="http://eurovoc.europa.eu/486"/>
		<skos:inScheme rdf:resource="https://www.opengis.net/def/CaLAThe/5.0"/>
		<skos:altLabel>Statement</skos:altLabel>
		<skos:broader rdf:resource="https://www.opengis.net/def/CaLAThe/5.0/Information"/>
		<skos:narrower rdf:resource="https://www.opengis.net/def/CaLAThe/5.0/Deed"/>
		<skos:narrower rdf:resource="https://www.opengis.net/def/CaLAThe/5.0/CadastralSurveyDocument"/>
		<skos:narrower rdf:resource="https://www.opengis.net/def/CaLAThe/5.0/Certificate"/>
		<skos:narrower rdf:resource="https://www.opengis.net/def/CaLAThe/5.0/CondominiumScheme"/>
		<skos:narrower rdf:resource="https://www.opengis.net/def/CaLAThe/5.0/SuperficieObjectScheme"/>
		<skos:narrower rdf:resource="https://www.opengis.net/def/CaLAThe/5.0/EasementDeed"/>
		<skos:narrower rdf:resource="https://www.opengis.net/def/CaLAThe/5.0/CadastralAccount"/>
		<skos:narrower rdf:resource="https://www.opengis.net/def/CaLAThe/5.0/LA_Source"/>
		<skos:related rdf:resource="https://www.opengis.net/def/CaLAThe/5.0/Drafter"/>
	</skos:Concept>
	<skos:Concept rdf:about="https://www.opengis.net/def/CaLAThe/5.0/DominantPropertyUnit">
		<skos:prefLabel xml:lang="en">Dominant property unit</skos:prefLabel>
		<skos:prefLabel xml:lang="da">Herskende ejendom</skos:prefLabel>
		<skos:prefLabel xml:lang="tr">Hakim taşınmaz</skos:prefLabel>
		<skos:definition>Land (Property unit) for which a servitude is granted (Source: Legal Dictionary of Property in Canada - Dualjuridik).</skos:definition>
		<skos:changeNote>Established with version 3.</skos:changeNote>
		<skos:inScheme rdf:resource="https://www.opengis.net/def/CaLAThe/5.0"/>
		<skos:broader rdf:resource="https://www.opengis.net/def/CaLAThe/5.0/Easement"/>
	</skos:Concept>
	<skos:Concept rdf:about="https://www.opengis.net/def/CaLAThe/5.0/Drafter">
		<skos:prefLabel xml:lang="en">Drafter</skos:prefLabel>
		<skos:prefLabel xml:lang="da">Koncipist</skos:prefLabel>
		<skos:prefLabel xml:lang="tr">.</skos:prefLabel>
		<skos:scopeNote>OGC LandInfra / InfraGML term</skos:scopeNote>
		<skos:definition>The professional (lawyer, notary, landSurveyor, ..) who prepared (drafted) a Document (Source: OGC LandInfra, 7.10.4).</skos:definition>
		<skos:changeNote>Established as Draftsman in version 3, revised as Drafter in Version 5.</skos:changeNote>
		<skos:inScheme rdf:resource="https://www.opengis.net/def/CaLAThe/5.0"/>
		<skos:broader rdf:resource="https://www.opengis.net/def/CaLAThe/5.0/Professional"/>
		<skos:related rdf:resource="https://www.opengis.net/def/CaLAThe/5.0/Document"/>
	</skos:Concept>
	<skos:Concept rdf:about="https://www.opengis.net/def/CaLAThe/5.0/Easement">
		<skos:prefLabel xml:lang="en">Easement</skos:prefLabel>
		<skos:prefLabel xml:lang="da">Servitut</skos:prefLabel>
		<skos:prefLabel xml:lang="tr">İrtifak hakkı</skos:prefLabel>
		<skos:scopeNote>GEMET term. Compares to ISO LADM 4.1.19 restriction</skos:scopeNote>
		<skos:definition>The rights of use over the property of another; a burden on a piece of land causing the owner to suffer access by another (Source: GEMET). Accessory interest in land which advantages dominant land or other beneficiary (Source: Legal Dictionary of Property in Canada - Dualjuridik; cf. OGC LandInfra, 4.8.6).</skos:definition>
		<skos:changeNote>Established with version 1. Changed with version 3.</skos:changeNote>
		<skos:exactMatch rdf:resource="http://www.eionet.europa.eu/gemet/concept/11536"/>
		<skos:inScheme rdf:resource="https://www.opengis.net/def/CaLAThe/5.0"/>
		<skos:broader rdf:resource="https://www.opengis.net/def/CaLAThe/5.0/LimitedRight"/>
		<skos:narrower rdf:resource="https://www.opengis.net/def/CaLAThe/5.0/PrivateLawRestriction"/>
		<skos:narrower rdf:resource="https://www.opengis.net/def/CaLAThe/5.0/ServientPropertyUnit"/>
		<skos:narrower rdf:resource="https://www.opengis.net/def/CaLAThe/5.0/PublicLawRestriction"/>
		<skos:narrower rdf:resource="https://www.opengis.net/def/CaLAThe/5.0/DominantPropertyUnit"/>
	</skos:Concept>
	<skos:Concept rdf:about="https://www.opengis.net/def/CaLAThe/5.0/EasementCreation">
		<skos:prefLabel xml:lang="en">Easement creation</skos:prefLabel>
		<skos:prefLabel xml:lang="da">Stiftelse af servitut</skos:prefLabel>
		<skos:prefLabel xml:lang="tr">İrtifak hakkı tesisi</skos:prefLabel>
		<skos:changeNote>Established with version 2. Scope note and relations added with version 3.</skos:changeNote>
		<skos:inScheme rdf:resource="https://www.opengis.net/def/CaLAThe/5.0"/>
		<skos:broader rdf:resource="https://www.opengis.net/def/CaLAThe/5.0/Exchange"/>
		<skos:related rdf:resource="https://www.opengis.net/def/CaLAThe/5.0/DominantPropertyUnit"/>
		<skos:related rdf:resource="https://www.opengis.net/def/CaLAThe/5.0/ServientPropertyUnit"/>
		<skos:related rdf:resource="https://www.opengis.net/def/CaLAThe/5.0/CondominiumScheme"/>
	</skos:Concept>
	<skos:Concept rdf:about="https://www.opengis.net/def/CaLAThe/5.0/EasementDeed">
		<skos:prefLabel xml:lang="en">Easement deed</skos:prefLabel>
		<skos:prefLabel xml:lang="da">Deklaration, Servitutdokument</skos:prefLabel>
		<skos:prefLabel xml:lang="tr">İrtifak hakkı sözleşmesi</skos:prefLabel>
		<skos:scopeNote>OGC LandInfra / InfraGML term</skos:scopeNote>
		<skos:changeNote>Established with version 3 as Easement scheme, and changed as Easement deed in version 5.</skos:changeNote>
		<skos:inScheme rdf:resource="https://www.opengis.net/def/CaLAThe/5.0"/>
		<skos:broader rdf:resource="https://www.opengis.net/def/CaLAThe/5.0/Document"/>
	</skos:Concept>
	<skos:Concept rdf:about="https://www.opengis.net/def/CaLAThe/5.0/Edge">
		<skos:prefLabel xml:lang="en">Edge</skos:prefLabel>
		<skos:prefLabel xml:lang="da">Kant</skos:prefLabel>
		<skos:prefLabel xml:lang="tr">Kenar</skos:prefLabel>
		<skos:scopeNote>Geolexica term</skos:scopeNote>
		<skos:definition>1-dimensional topological primitive. Note to entry: The geometric realization of an edge is a curve. The boundary of an edge is the set of one or two nodes associated to the edge within a topological complex. (Geolexica, ISO 19107:2003)</skos:definition>
		<skos:changeNote>Introduced with version 4</skos:changeNote>
		<skos:exactMatch rdf:resource="https://isotc211.geolexica.org/concepts/146/"/>
		<skos:inScheme rdf:resource="https://www.opengis.net/def/CaLAThe/5.0"/>
		<skos:broader rdf:resource="https://www.opengis.net/def/CaLAThe/5.0/TopologicalPrimitive"/>
		<skos:narrower rdf:resource="https://www.opengis.net/def/CaLAThe/5.0/LA_EdgeBasedSpatialUnit"/>
	</skos:Concept>
	<skos:Concept rdf:about="https://www.opengis.net/def/CaLAThe/5.0/EletronicDistanceMeter">
		<skos:prefLabel xml:lang="en">Electronic distance meter</skos:prefLabel>
		<skos:prefLabel xml:lang="da">Elektrooptisk distancemåler</skos:prefLabel>
		<skos:prefLabel xml:lang="tr">Elektronik uzunluk ölçer</skos:prefLabel>
		<skos:scopeNote>OGC LandInfra / InfraGML term</skos:scopeNote>
		<skos:definition>Instrument for directly measuring distances between the instrument and the sighting points, comprising a transmitter and a receiver (OGC LandInfra 4.6.3, referring to ISO 9849-1:2000).</skos:definition>
		<skos:changeNote>Established with version 4</skos:changeNote>
		<skos:inScheme rdf:resource="https://www.opengis.net/def/CaLAThe/5.0"/>
		<skos:broader rdf:resource="https://www.opengis.net/def/CaLAThe/5.0/SurveyingInstrument"/>
		<skos:narrower rdf:resource="https://www.opengis.net/def/CaLAThe/5.0/DistanceObservation"/>
	</skos:Concept>
	<skos:Concept rdf:about="https://www.opengis.net/def/CaLAThe/5.0/Elevation">
		<skos:prefLabel xml:lang="en">Elevation</skos:prefLabel>
		<skos:prefLabel xml:lang="da">Højde</skos:prefLabel>
		<skos:prefLabel xml:lang="tr">Yükseklik</skos:prefLabel>
		<skos:scopeNote>INSPIRE term</skos:scopeNote>
		<skos:definition>Height above sea level.</skos:definition>
		<skos:changeNote>Established with version 1. Definition is added in version 5.</skos:changeNote>
		<skos:inScheme rdf:resource="https://www.opengis.net/def/CaLAThe/5.0"/>
		<skos:broader rdf:resource="https://www.opengis.net/def/CaLAThe/5.0/TopographicalFeature"/>
	</skos:Concept>
	<skos:Concept rdf:about="https://www.opengis.net/def/CaLAThe/5.0/Engineer">
		<skos:prefLabel xml:lang="en">Engineer</skos:prefLabel>
		<skos:prefLabel xml:lang="da">Ingeniør</skos:prefLabel>
		<skos:prefLabel xml:lang="tr">Mühendis</skos:prefLabel>
		<skos:changeNote>Established with version 3.</skos:changeNote>
		<skos:exactMatch rdf:resource="http://eurovoc.europa.eu/1435"/>
		<skos:exactMatch rdf:resource="http://aims.fao.org/aos/agrovoc/c_2573"/>
		<skos:inScheme rdf:resource="https://www.opengis.net/def/CaLAThe/5.0"/>
		<skos:broader rdf:resource="https://www.opengis.net/def/CaLAThe/5.0/Professional"/>
	</skos:Concept>
	<skos:Concept rdf:about="https://www.opengis.net/def/CaLAThe/5.0/Exchange">
		<skos:prefLabel xml:lang="en">Exchange</skos:prefLabel>
		<skos:prefLabel xml:lang="da">Ejendomsdispositioner</skos:prefLabel>
		<skos:prefLabel xml:lang="tr">Temlik</skos:prefLabel>
		<skos:changeNote>Established with version 2.</skos:changeNote>
		<skos:inScheme rdf:resource="https://www.opengis.net/def/CaLAThe/5.0"/>
		<skos:broader rdf:resource="https://www.opengis.net/def/CaLAThe/5.0/Activity"/>
		<skos:narrower rdf:resource="https://www.opengis.net/def/CaLAThe/5.0/Conveyance"/>
		<skos:narrower rdf:resource="https://www.opengis.net/def/CaLAThe/5.0/Lease"/>
		<skos:narrower rdf:resource="https://www.opengis.net/def/CaLAThe/5.0/Rent"/>
		<skos:narrower rdf:resource="https://www.opengis.net/def/CaLAThe/5.0/Mortgaging"/>
		<skos:narrower rdf:resource="https://www.opengis.net/def/CaLAThe/5.0/ForcedSale"/>
		<skos:narrower rdf:resource="https://www.opengis.net/def/CaLAThe/5.0/EasementCreation"/>
	</skos:Concept>
	<skos:Concept rdf:about="https://www.opengis.net/def/CaLAThe/5.0/Expropriation">
		<skos:prefLabel xml:lang="en">Expropriation</skos:prefLabel>
		<skos:prefLabel xml:lang="da">Ekspropriation</skos:prefLabel>
		<skos:prefLabel xml:lang="tr">Kamulaştırma</skos:prefLabel>
		<skos:scopeNote>GEMET term</skos:scopeNote>
		<skos:definition>To deprive an owner of property, especially by taking it for public use (Source: Collins English Dictionary, 1994).</skos:definition>
		<skos:changeNote>Established with version 2.</skos:changeNote>
		<skos:exactMatch rdf:resource="http://aims.fao.org/aos/agrovoc/c_1798"/>
		<skos:exactMatch rdf:resource="https://www.eionet.europa.eu/gemet/en/concept/3071"/>
		<skos:exactMatch rdf:resource="http://eurovoc.europa.eu/948"/>
		<skos:exactMatch rdf:resource="http://zbw.eu/stw/descriptor/11771-1"/>
		<skos:inScheme rdf:resource="https://www.opengis.net/def/CaLAThe/5.0"/>
		<skos:broader rdf:resource="https://www.opengis.net/def/CaLAThe/5.0/PropertyRestructuring"/>
	</skos:Concept>
	<skos:Concept rdf:about="https://www.opengis.net/def/CaLAThe/5.0/Face">
		<skos:prefLabel xml:lang="en">Face</skos:prefLabel>
		<skos:prefLabel xml:lang="da">Flade</skos:prefLabel>
		<skos:prefLabel xml:lang="tr">Yüz</skos:prefLabel>
		<skos:scopeNote>Geolexica term</skos:scopeNote>
		<skos:definition>2-dimensional topological primitive. Note to entry: The geometric realization of a face is a surface. The boundary of a face is the set of directed edges within the same topological complex that are associated to the face via the boundary relations. These can be organized as rings. (Geolexica, ISO 19107:2003)</skos:definition>
		<skos:changeNote>Introduced with version 4</skos:changeNote>
		<skos:exactMatch rdf:resource="https://isotc211.geolexica.org/concepts/165/"/>
		<skos:inScheme rdf:resource="https://www.opengis.net/def/CaLAThe/5.0"/>
		<skos:broader rdf:resource="https://www.opengis.net/def/CaLAThe/5.0/TopologicalPrimitive"/>
		<skos:narrower rdf:resource="https://www.opengis.net/def/CaLAThe/5.0/LA_FaceBasedSpatialUnit"/>
	</skos:Concept>
	<skos:Concept rdf:about="https://www.opengis.net/def/CaLAThe/5.0/Family">
		<skos:prefLabel xml:lang="en">Family</skos:prefLabel>
		<skos:prefLabel xml:lang="da">Familie</skos:prefLabel>
		<skos:prefLabel xml:lang="tr">Aile</skos:prefLabel>
		<skos:scopeNote>GEMET term</skos:scopeNote>
		<skos:definition>A group comprising parents, offsprings and others closely related or associated with them (Source: Lincoln, Boxshall and Clark, 1982).</skos:definition>
		<skos:changeNote>Established with version 1.</skos:changeNote>
		<skos:exactMatch rdf:resource="http://www.eionet.europa.eu/gemet/concept/3117"/>
		<skos:exactMatch rdf:resource="http://eurovoc.europa.eu/965"/>
		<skos:inScheme rdf:resource="https://www.opengis.net/def/CaLAThe/5.0"/>
		<skos:broader rdf:resource="https://www.opengis.net/def/CaLAThe/5.0/SocialGroup"/>
	</skos:Concept>
	<skos:Concept rdf:about="https://www.opengis.net/def/CaLAThe/5.0/Farmer">
		<skos:prefLabel xml:lang="en">Farmer</skos:prefLabel>
		<skos:prefLabel xml:lang="da">Landmand</skos:prefLabel>
		<skos:prefLabel xml:lang="tr">Çiftçi</skos:prefLabel>
		<skos:scopeNote>ISO LADM term</skos:scopeNote>
		<skos:changeNote>Established with version 4. Broader edited with ver. 5.</skos:changeNote>
		<skos:exactMatch rdf:resource="http://aims.fao.org/aos/agrovoc/c_2805"/>
		<skos:exactMatch rdf:resource="http://eurovoc.europa.eu/936"/>
		<skos:inScheme rdf:resource="https://www.opengis.net/def/CaLAThe/5.0"/>
		<skos:broader rdf:resource="https://www.opengis.net/def/CaLAThe/5.0/SocietalRole"/>
	</skos:Concept>
	<skos:Concept rdf:about="https://www.opengis.net/def/CaLAThe/5.0/ForcedSale">
		<skos:prefLabel xml:lang="en">Forced sale</skos:prefLabel>
		<skos:prefLabel xml:lang="da">Tvangsauktion</skos:prefLabel>
		<skos:prefLabel xml:lang="tr">Zoraki satış</skos:prefLabel>
		<skos:scopeNote>AGROVOC Multilingual Thesaurus term</skos:scopeNote>
		<skos:changeNote>Established with version 2. Close match http://www.eionet.europa.eu/gemet/concept/3401 deleted with version 4</skos:changeNote>
		<skos:exactMatch rdf:resource="http://aims.fao.org/aos/agrovoc/c_15683"/>
		<skos:inScheme rdf:resource="https://www.opengis.net/def/CaLAThe/5.0"/>
		<skos:altLabel>Foreclosure</skos:altLabel>
		<skos:altLabel>Compulsory purchase</skos:altLabel>
		<skos:altLabel>Repossesion</skos:altLabel>
		<skos:broader rdf:resource="https://www.opengis.net/def/CaLAThe/5.0/Exchange"/>
	</skos:Concept>
	<skos:Concept rdf:about="https://www.opengis.net/def/CaLAThe/5.0/Gazetteer">
		<skos:prefLabel xml:lang="en">Gazetteer</skos:prefLabel>
		<skos:prefLabel xml:lang="da">Stednavnefortegnelse</skos:prefLabel>
		<skos:prefLabel xml:lang="tr">Yer adları dizini</skos:prefLabel>
		<skos:scopeNote>AGROVOC Multilingual Thesaurus term</skos:scopeNote>
		<skos:definition>A vocabulary consisting of identifiers, location descriptions, and attributes for a set of geospatial features (Source: Breitman, Casanova and  Truszkowski, 2007).</skos:definition>
		<skos:changeNote>Established with version 1.</skos:changeNote>
		<skos:exactMatch rdf:resource="http://aims.fao.org/aos/agrovoc/c_49853"/>
		<skos:inScheme rdf:resource="https://www.opengis.net/def/CaLAThe/5.0"/>
		<skos:broader rdf:resource="https://www.opengis.net/def/CaLAThe/5.0/SpatialDataInfrastructure"/>
		<skos:narrower rdf:resource="https://www.opengis.net/def/CaLAThe/5.0/PlaceName"/>
	</skos:Concept>
	<skos:Concept rdf:about="https://www.opengis.net/def/CaLAThe/5.0/GeographicalGridSystem">
		<skos:prefLabel xml:lang="en">Geographical grid system</skos:prefLabel>
		<skos:prefLabel xml:lang="da">Geografiske kvadratnetsystemer</skos:prefLabel>
		<skos:prefLabel xml:lang="tr">Coğrafi grid sistemi</skos:prefLabel>
		<skos:scopeNote>INSPIRE term</skos:scopeNote>
		<skos:definition>Harmonised multi-resolution grid with a common point of origin and standardised location and size of grid cells [INSPIRE Directive] (Source: INSPIRE glossary).</skos:definition>
		<skos:changeNote>Established with version 1.</skos:changeNote>
		<skos:exactMatch rdf:resource="http://inspire.ec.europa.eu/glossary/GeographicalGridSystem"/>
		<skos:inScheme rdf:resource="https://www.opengis.net/def/CaLAThe/5.0"/>
		<skos:broader rdf:resource="https://www.opengis.net/def/CaLAThe/5.0/SpatialReference"/>
	</skos:Concept>
	<skos:Concept rdf:about="https://www.opengis.net/def/CaLAThe/5.0/GeographicalInformationSystem">
		<skos:prefLabel xml:lang="en">Geographical information system</skos:prefLabel>
		<skos:prefLabel xml:lang="da">Geografisk informations system</skos:prefLabel>
		<skos:prefLabel xml:lang="tr">Coğrafi bilgi sistemi</skos:prefLabel>
		<skos:scopeNote>AGROVOC Multilingual Thesaurus term</skos:scopeNote>
		<skos:changeNote>Established with version 1.</skos:changeNote>
		<skos:exactMatch rdf:resource="http://aims.fao.org/aos/agrovoc/c_35131"/>
		<skos:exactMatch rdf:resource="http://eurovoc.europa.eu/7218"/>
		<skos:inScheme rdf:resource="https://www.opengis.net/def/CaLAThe/5.0"/>
		<skos:broader rdf:resource="https://www.opengis.net/def/CaLAThe/5.0/SpatialDataInfrastructure"/>
		<skos:narrower rdf:resource="https://www.opengis.net/def/CaLAThe/5.0/Cadastre"/>
	</skos:Concept>
	<skos:Concept rdf:about="https://www.opengis.net/def/CaLAThe/5.0/GeolocatedInformation">
		<skos:prefLabel xml:lang="en">Geolocated information</skos:prefLabel>
		<skos:prefLabel xml:lang="da">Stedbestemt information</skos:prefLabel>
		<skos:prefLabel xml:lang="tr">Coğrafi konumlandırılmış bilgi</skos:prefLabel>
		<skos:definition>Information which is localized on the surface of the Earth through nominal, ordinal or metric means (cf Stevens, 1946; Stubkjær, 1992)</skos:definition>
		<skos:changeNote>Introduced with version 4</skos:changeNote>
		<skos:inScheme rdf:resource="https://www.opengis.net/def/CaLAThe/5.0"/>
		<skos:broader rdf:resource="https://www.opengis.net/def/CaLAThe/5.0/Information"/>
		<skos:narrower rdf:resource="https://www.opengis.net/def/CaLAThe/5.0/PlaceName"/>
		<skos:narrower rdf:resource="https://www.opengis.net/def/CaLAThe/5.0/SpatialDataInfrastructure"/>
		<skos:narrower rdf:resource="https://www.opengis.net/def/CaLAThe/5.0/TopologicalLocalization"/>
		<skos:narrower rdf:resource="https://www.opengis.net/def/CaLAThe/5.0/Map"/>
		<skos:narrower rdf:resource="https://www.opengis.net/def/CaLAThe/5.0/DigitalImagery"/>
		<skos:narrower rdf:resource="https://www.opengis.net/def/CaLAThe/5.0/SpatialUnit"/>
	</skos:Concept>
	<skos:Concept rdf:about="https://www.opengis.net/def/CaLAThe/5.0/GeometricPrimitive">
		<skos:prefLabel xml:lang="en">Geometric primitive</skos:prefLabel>
		<skos:prefLabel xml:lang="da">Geometrisk objekt</skos:prefLabel>
		<skos:prefLabel xml:lang="tr">Geometrik temel şekiller</skos:prefLabel>
		<skos:scopeNote>Geolexica term</skos:scopeNote>
		<skos:definition>Geometric object representing a single, connected, homogeneous (isotropic) element of space (ISO 19107:2019, (E), 3.50).</skos:definition>
		<skos:changeNote>Established with version 1.</skos:changeNote>
		<skos:exactMatch rdf:resource="https://isotc211.geolexica.org/concepts/2164/"/>
		<skos:inScheme rdf:resource="https://www.opengis.net/def/CaLAThe/5.0"/>
		<skos:broader rdf:resource="https://www.opengis.net/def/CaLAThe/5.0/SpatialUnit"/>
		<skos:narrower rdf:resource="https://www.opengis.net/def/CaLAThe/5.0/LA_PointBasedSpatialUnit"/>
		<skos:narrower rdf:resource="https://www.opengis.net/def/CaLAThe/5.0/LA_LineBasedSpatialUnit"/>
		<skos:narrower rdf:resource="https://www.opengis.net/def/CaLAThe/5.0/PolygonBasedSpatialUnit"/>
		<skos:narrower rdf:resource="https://www.opengis.net/def/CaLAThe/5.0/Curve"/>
		<skos:narrower rdf:resource="https://www.opengis.net/def/CaLAThe/5.0/Surface"/>
		<skos:narrower rdf:resource="https://www.opengis.net/def/CaLAThe/5.0/Point"/>
		<skos:narrower rdf:resource="https://www.opengis.net/def/CaLAThe/5.0/LA_Point"/>
	</skos:Concept>
	<skos:Concept rdf:about="https://www.opengis.net/def/CaLAThe/5.0/Gift">
		<skos:prefLabel xml:lang="en">Gift</skos:prefLabel>
		<skos:prefLabel xml:lang="da">Gave</skos:prefLabel>
		<skos:prefLabel xml:lang="tr">Bağış</skos:prefLabel>
		<skos:changeNote>Established with version 2.</skos:changeNote>
		<skos:exactMatch rdf:resource="http://eurovoc.europa.eu/501"/>
		<skos:inScheme rdf:resource="https://www.opengis.net/def/CaLAThe/5.0"/>
		<skos:broader rdf:resource="https://www.opengis.net/def/CaLAThe/5.0/Transfer"/>
	</skos:Concept>
	<skos:Concept rdf:about="https://www.opengis.net/def/CaLAThe/5.0/GNSSobservation">
		<skos:prefLabel xml:lang="en">GNSS observation</skos:prefLabel>
		<skos:prefLabel xml:lang="da">GNSSobservation</skos:prefLabel>
		<skos:prefLabel xml:lang="tr">GNSS gözlemi</skos:prefLabel>
		<skos:definition>GNSS observation contains all observations to one or more satellite systems. When using differential GNSS, also the information on the reference stations are included. (OGC LandInfra 7.8.3.9)</skos:definition>
		<skos:changeNote>Established with version 4</skos:changeNote>
		<skos:exactMatch rdf:resource="http://docs.opengeospatial.org/is/15-111r1/15-111r1.html#121"/>
		<skos:inScheme rdf:resource="https://www.opengis.net/def/CaLAThe/5.0"/>
		<skos:broader rdf:resource="https://www.opengis.net/def/CaLAThe/5.0/Observation"/>
		<skos:broader rdf:resource="https://www.opengis.net/def/CaLAThe/5.0/GNSSsensor"/>
		<skos:narrower rdf:resource="https://www.opengis.net/def/CaLAThe/5.0/TargetPoint"/>
	</skos:Concept>
	<skos:Concept rdf:about="https://www.opengis.net/def/CaLAThe/5.0/GNSSsensor">
		<skos:prefLabel xml:lang="en">GNSS sensor</skos:prefLabel>
		<skos:prefLabel xml:lang="da">GNSS modtager</skos:prefLabel>
		<skos:prefLabel xml:lang="tr">GNSS alıcısı</skos:prefLabel>
		<skos:scopeNote>OGC LandInfra / InfraGML term</skos:scopeNote>
		<skos:definition>GNSS sensors receive the signals from different satellite systems to determine a 3d location of the TargetPoint. External antennas could be also used. If differential GNSS was used GNSS sensor may also contain the sensor information of the reference station. GNSS class will then contain the reference aggregation of a GNNS reference sensor. (OGC LandInfra 7.8.5.13)</skos:definition>
		<skos:changeNote>Established with version 4</skos:changeNote>
		<skos:exactMatch rdf:resource="http://docs.opengeospatial.org/is/15-111r1/15-111r1.html#148"/>
		<skos:inScheme rdf:resource="https://www.opengis.net/def/CaLAThe/5.0"/>
		<skos:broader rdf:resource="https://www.opengis.net/def/CaLAThe/5.0/SurveyingInstrument"/>
		<skos:narrower rdf:resource="https://www.opengis.net/def/CaLAThe/5.0/GNSSobservation"/>
	</skos:Concept>
	<skos:Concept rdf:about="https://www.opengis.net/def/CaLAThe/5.0/GoodFaith">
		<skos:prefLabel xml:lang="en">Good faith</skos:prefLabel>
		<skos:prefLabel xml:lang="da">God tro</skos:prefLabel>
		<skos:prefLabel xml:lang="tr">İyi niyet</skos:prefLabel>
		<skos:definition>Principle of honesty or sincerity of intention.</skos:definition>
		<skos:changeNote>Established with version 3.</skos:changeNote>
		<skos:inScheme rdf:resource="https://www.opengis.net/def/CaLAThe/5.0"/>
		<skos:broader rdf:resource="https://www.opengis.net/def/CaLAThe/5.0/RightsHolder"/>
	</skos:Concept>
	<skos:Concept rdf:about="https://www.opengis.net/def/CaLAThe/5.0/GovernmentalOrganisation">
		<skos:prefLabel xml:lang="en">Governmental organisation</skos:prefLabel>
		<skos:prefLabel xml:lang="da">Offentlig forvaltning</skos:prefLabel>
		<skos:prefLabel xml:lang="tr">Devlet kuruluşu</skos:prefLabel>
		<skos:scopeNote>AGROVOC Multilingual Thesaurus term</skos:scopeNote>
		<skos:definition>Any governmental agency or organization charged with managing and implementing regulations, laws and government policies (Source: AGROVOC).</skos:definition>
		<skos:changeNote>Established with version 1. Edited with version 4. Agency added with ver. 5.</skos:changeNote>
		<skos:exactMatch rdf:resource="http://aims.fao.org/aos/agrovoc/c_50225"/>
		<skos:exactMatch rdf:resource="http://eurovoc.europa.eu/77"/>
		<skos:inScheme rdf:resource="https://www.opengis.net/def/CaLAThe/5.0"/>
		<skos:altLabel>Administrative body</skos:altLabel>
		<skos:altLabel>Agency</skos:altLabel>
		<skos:broader rdf:resource="https://www.opengis.net/def/CaLAThe/5.0/Organisation"/>
		<skos:narrower rdf:resource="https://www.opengis.net/def/CaLAThe/5.0/NationalSurveyAndCadastre"/>
		<skos:narrower rdf:resource="https://www.opengis.net/def/CaLAThe/5.0/LandRegister"/>
	</skos:Concept>
	<skos:Concept rdf:about="https://www.opengis.net/def/CaLAThe/5.0/GroupParty">
		<skos:prefLabel xml:lang="en">Group party</skos:prefLabel>
		<skos:prefLabel xml:lang="da">Gruppe</skos:prefLabel>
		<skos:prefLabel xml:lang="tr">Grup</skos:prefLabel>
		<skos:scopeNote>ISO LADM term</skos:scopeNote>
		<skos:definition>Any number of parties, forming together a distinct entity, with each party registered (Source: ISO LADM, 4.1.8).</skos:definition>
		<skos:changeNote>Established with version 1.</skos:changeNote>
		<skos:inScheme rdf:resource="https://www.opengis.net/def/CaLAThe/5.0"/>
		<skos:altLabel>LA_GroupParty</skos:altLabel>
		<skos:broader rdf:resource="https://www.opengis.net/def/CaLAThe/5.0/PartyType"/>
		<skos:narrower rdf:resource="https://www.opengis.net/def/CaLAThe/5.0/SocialGroup"/>
		<skos:narrower rdf:resource="https://www.opengis.net/def/CaLAThe/5.0/PlaceBoundParty"/>
	</skos:Concept>
	<skos:Concept rdf:about="https://www.opengis.net/def/CaLAThe/5.0/Hydrography">
		<skos:prefLabel xml:lang="en">Hydrography</skos:prefLabel>
		<skos:prefLabel xml:lang="da">Hydrografi</skos:prefLabel>
		<skos:prefLabel xml:lang="tr">Hidroğrafya</skos:prefLabel>
		<skos:scopeNote>GEMET term</skos:scopeNote>
		<skos:definition>Science which deals with the measurement and description of the physical features of the oceans, lakes, rivers, and their adjoining coastal areas, with particular reference to their control and utilization (Source: GEMET).</skos:definition>
		<skos:changeNote>Established with version 1.</skos:changeNote>
		<skos:exactMatch rdf:resource="https://www.eionet.europa.eu/gemet/en/concept/4109"/>
		<skos:exactMatch rdf:resource="http://aims.fao.org/aos/agrovoc/c_3727"/>
		<skos:inScheme rdf:resource="https://www.opengis.net/def/CaLAThe/5.0"/>
		<skos:broader rdf:resource="https://www.opengis.net/def/CaLAThe/5.0/TopographicalFeature"/>
	</skos:Concept>
	<skos:Concept rdf:about="https://www.opengis.net/def/CaLAThe/5.0/Image">
		<skos:prefLabel xml:lang="en">Image</skos:prefLabel>
		<skos:prefLabel xml:lang="da">Billede, Digitalbillede</skos:prefLabel>
		<skos:prefLabel xml:lang="tr">Görüntü</skos:prefLabel>
		<skos:scopeNote>OGC LandInfra / InfraGML term</skos:scopeNote>
		<skos:definition>Image is the result of an ImageObservation (OCG LandInfra 7.8.7.8)</skos:definition>
		<skos:changeNote>Established with version 4</skos:changeNote>
		<skos:exactMatch rdf:resource="https://isotc211.geolexica.org/concepts/551/"/>
		<skos:inScheme rdf:resource="https://www.opengis.net/def/CaLAThe/5.0"/>
		<skos:broader rdf:resource="https://www.opengis.net/def/CaLAThe/5.0/Camera"/>
		<skos:broader rdf:resource="https://www.opengis.net/def/CaLAThe/5.0/SurveyResult"/>
	</skos:Concept>
	<skos:Concept rdf:about="https://www.opengis.net/def/CaLAThe/5.0/IndividualOwnership">
		<skos:prefLabel xml:lang="en">Individual ownership</skos:prefLabel>
		<skos:prefLabel xml:lang="da">Selveje</skos:prefLabel>
		<skos:prefLabel xml:lang="tr">Bireysel mülkiyet</skos:prefLabel>
		<skos:definition>Exercise of ownership towards property by an individual (Source: Legal Dictionary of Property in Canada - Dualjuridik).</skos:definition>
		<skos:changeNote>Established with version 1. Definition added with version 3.</skos:changeNote>
		<skos:inScheme rdf:resource="https://www.opengis.net/def/CaLAThe/5.0"/>
		<skos:broader rdf:resource="https://www.opengis.net/def/CaLAThe/5.0/Ownership"/>
	</skos:Concept>
	<skos:Concept rdf:about="https://www.opengis.net/def/CaLAThe/5.0/Information">
		<skos:prefLabel xml:lang="en">Information</skos:prefLabel>
		<skos:prefLabel xml:lang="da">Information</skos:prefLabel>
		<skos:prefLabel xml:lang="tr">Bilgi</skos:prefLabel>
		<skos:scopeNote>GEMET General Multilingual Environmental Thesaurus term</skos:scopeNote>
		<skos:definition>All facts, ideas or imaginative works of the mind which have been communicated, published or distributed formally or informally in any format, or the knowledge that is communicated or received.</skos:definition>
		<skos:changeNote>Established as Documentation with version 1. Edited to Information in version 4.</skos:changeNote>
		<skos:exactMatch rdf:resource="https://www.eionet.europa.eu/gemet/en/concept/4303"/>
		<skos:exactMatch rdf:resource="http://zbw.eu/stw/descriptor/16754-4"/>
		<skos:exactMatch rdf:resource="http://aims.fao.org/aos/agrovoc/c_330966"/>
		<skos:exactMatch rdf:resource="http://eurovoc.europa.eu/1422"/>
		<skos:inScheme rdf:resource="https://www.opengis.net/def/CaLAThe/5.0"/>
		<skos:topConceptOf rdf:resource="https://www.opengis.net/def/CaLAThe/5.0"/>
		<skos:narrower rdf:resource="https://www.opengis.net/def/CaLAThe/5.0/Document"/>
		<skos:narrower rdf:resource="https://www.opengis.net/def/CaLAThe/5.0/Metadata"/>
		<skos:narrower rdf:resource="https://www.opengis.net/def/CaLAThe/5.0/GeolocatedInformation"/>
		<skos:narrower rdf:resource="https://www.opengis.net/def/CaLAThe/5.0/SpatialReference"/>
		<skos:narrower rdf:resource="https://www.opengis.net/def/CaLAThe/5.0/Registry"/>
		<skos:narrower rdf:resource="https://www.opengis.net/def/CaLAThe/5.0/CodeList"/>
	</skos:Concept>
	<skos:Concept rdf:about="https://www.opengis.net/def/CaLAThe/5.0/Inheritance">
		<skos:prefLabel xml:lang="en">Inheritance</skos:prefLabel>
		<skos:prefLabel xml:lang="da">Arv</skos:prefLabel>
		<skos:prefLabel xml:lang="tr">Miras</skos:prefLabel>
		<skos:changeNote>Established with version 2.</skos:changeNote>
		<skos:exactMatch rdf:resource="http://zbw.eu/stw/descriptor/16028-5"/>
		<skos:exactMatch rdf:resource="http://eurovoc.europa.eu/3934"/>
		<skos:inScheme rdf:resource="https://www.opengis.net/def/CaLAThe/5.0"/>
		<skos:broader rdf:resource="https://www.opengis.net/def/CaLAThe/5.0/Transfer"/>
	</skos:Concept>
	<skos:Concept rdf:about="https://www.opengis.net/def/CaLAThe/5.0/Judiciary">
		<skos:prefLabel xml:lang="en">Judiciary</skos:prefLabel>
		<skos:prefLabel xml:lang="da">Retsvæsen</skos:prefLabel>
		<skos:prefLabel xml:lang="tr">Yargı</skos:prefLabel>
		<skos:scopeNote>STW Thesaurus for Economics term</skos:scopeNote>
		<skos:changeNote>Established with version 1.</skos:changeNote>
		<skos:exactMatch rdf:resource="http://zbw.eu/stw/descriptor/19841-1"/>
		<skos:inScheme rdf:resource="https://www.opengis.net/def/CaLAThe/5.0"/>
		<skos:broader rdf:resource="https://www.opengis.net/def/CaLAThe/5.0/Organisation"/>
	</skos:Concept>
	<skos:Concept rdf:about="https://www.opengis.net/def/CaLAThe/5.0/Land">
		<skos:prefLabel xml:lang="en">Land</skos:prefLabel>
		<skos:prefLabel xml:lang="da">Land</skos:prefLabel>
		<skos:prefLabel xml:lang="tr">Arazi</skos:prefLabel>
		<skos:definition>The area of earth&#39;s surface, excluding the oceans, usually marked off by natural or political boundaries, or boundaries of ownership (ISO 6707-1:2014).</skos:definition>
		<skos:changeNote>Established with version 1.</skos:changeNote>
		<skos:exactMatch rdf:resource="http://zbw.eu/stw/descriptor/12015-6"/>
		<skos:exactMatch rdf:resource="https://www.eionet.europa.eu/gemet/en/concept/4599"/>
		<skos:exactMatch rdf:resource="http://aims.fao.org/aos/agrovoc/c_4172"/>
		<skos:inScheme rdf:resource="https://www.opengis.net/def/CaLAThe/5.0"/>
		<skos:narrower rdf:resource="https://www.opengis.net/def/CaLAThe/5.0/SpatialFeatureType"/>
	</skos:Concept>
	<skos:Concept rdf:about="https://www.opengis.net/def/CaLAThe/5.0/LandAdministration">
		<skos:prefLabel xml:lang="en">Land administration</skos:prefLabel>
		<skos:prefLabel xml:lang="da">Forvaltning af ejendomsdata</skos:prefLabel>
		<skos:prefLabel xml:lang="tr">Arazi bilgi yönetimi</skos:prefLabel>
		<skos:scopeNote>ISO LADM term</skos:scopeNote>
		<skos:definition>The process of determining, recording and disseminating information about the relationship between people and land (ISO LADM, 4.1.10).</skos:definition>
		<skos:changeNote>Established with version 3.</skos:changeNote>
		<skos:exactMatch rdf:resource="http://aims.fao.org/aos/agrovoc/c_9000091"/>
			<skos:exactMatch rdf:resource="https://isotc211.geolexica.org/concepts/1300/"/>
		<skos:inScheme rdf:resource="https://www.opengis.net/def/CaLAThe/5.0"/>
		<skos:topConceptOf rdf:resource="https://www.opengis.net/def/CaLAThe/5.0"/>
	</skos:Concept>
	<skos:Concept rdf:about="https://www.opengis.net/def/CaLAThe/5.0/LandConsolidation">
		<skos:prefLabel xml:lang="en">Land consolidation</skos:prefLabel>
		<skos:prefLabel xml:lang="da">Jordfordeling</skos:prefLabel>
		<skos:prefLabel xml:lang="tr">Arazi toplulaştırması</skos:prefLabel>
		<skos:definition>Joining small plots of land together to form larger farms or large fields (Source: GEMET cited from Collin, 1995).</skos:definition>
		<skos:changeNote>Established with version 2.</skos:changeNote>
		<skos:exactMatch rdf:resource="http://aims.fao.org/aos/agrovoc/c_4173"/>
		<skos:exactMatch rdf:resource="https://www.eionet.europa.eu/gemet/en/concept/4611"/>
		<skos:inScheme rdf:resource="https://www.opengis.net/def/CaLAThe/5.0"/>
		<skos:broader rdf:resource="https://www.opengis.net/def/CaLAThe/5.0/PropertyRestructuring"/>
		<skos:narrower rdf:resource="https://www.opengis.net/def/CaLAThe/5.0/Reallotment"/>
	</skos:Concept>
	<skos:Concept rdf:about="https://www.opengis.net/def/CaLAThe/5.0/LandDivision">
		<skos:prefLabel xml:lang="en">Land division</skos:prefLabel>
		<skos:prefLabel xml:lang="da">Geografisk opdeling</skos:prefLabel>
		<skos:prefLabel xml:lang="tr">Coğrafi bölüm</skos:prefLabel>
		<skos:scopeNote>OGC LandInfra / InfraGML term</skos:scopeNote>
		<skos:definition>Land division may be public (political, judicial, or executive) or private in nature, the latter delimiting ownership in land or in alternative terms: boundaries of real estate, of real property or of immovable property (Source: OGC LandInfra, 7.10.1).</skos:definition>
		<skos:changeNote>Established with version 1. Term changed with version 3 to Land division, and definition added.</skos:changeNote>
		<skos:inScheme rdf:resource="https://www.opengis.net/def/CaLAThe/5.0"/>
		<skos:altLabel>Administrative feature</skos:altLabel>
		<skos:broader rdf:resource="https://www.opengis.net/def/CaLAThe/5.0/SpatialFeatureType"/>
		<skos:narrower rdf:resource="https://www.opengis.net/def/CaLAThe/5.0/AdministrativeUnit"/>
		<skos:narrower rdf:resource="https://www.opengis.net/def/CaLAThe/5.0/RealProperty"/>
		<skos:narrower rdf:resource="https://www.opengis.net/def/CaLAThe/5.0/Marker"/>
		<skos:narrower rdf:resource="https://www.opengis.net/def/CaLAThe/5.0/PlaceName"/>
		<skos:narrower rdf:resource="https://www.opengis.net/def/CaLAThe/5.0/Boundary"/>
	</skos:Concept>
	<skos:Concept rdf:about="https://www.opengis.net/def/CaLAThe/5.0/LandLaw">
		<skos:prefLabel xml:lang="en">Land law</skos:prefLabel>
		<skos:prefLabel xml:lang="da">Ejendomsret (til fast ejendom)</skos:prefLabel>
		<skos:prefLabel xml:lang="tr">Taşınmaz (gayrimenkul) hukuku</skos:prefLabel>
		<skos:definition>Positive law concerning real estate / immovable property, including property formation, land development, and implementation of spatial planning  (Cf. Mattsson, 2001).</skos:definition>
		<skos:changeNote>Established with version 3.</skos:changeNote>
		<skos:exactMatch rdf:resource="http://aims.fao.org/aos/agrovoc/c_573abb9f"/>
		<skos:inScheme rdf:resource="https://www.opengis.net/def/CaLAThe/5.0"/>
		<skos:altLabel>Property law</skos:altLabel>
		<skos:broader rdf:resource="https://www.opengis.net/def/CaLAThe/5.0/PositiveLaw"/>
		<skos:narrower rdf:resource="https://www.opengis.net/def/CaLAThe/5.0/RealRight"/>
		<skos:narrower rdf:resource="https://www.opengis.net/def/CaLAThe/5.0/PlanningLaw"/>
		<skos:narrower rdf:resource="https://www.opengis.net/def/CaLAThe/5.0/LA_RRR"/>
		<skos:narrower rdf:resource="https://www.opengis.net/def/CaLAThe/5.0/LawOfObligation"/>
	</skos:Concept>
	<skos:Concept rdf:about="https://www.opengis.net/def/CaLAThe/5.0/LandReadjustment">
		<skos:prefLabel xml:lang="en">Land readjustment</skos:prefLabel>
		<skos:prefLabel xml:lang="da">Multifunktionel jordfordeling</skos:prefLabel>
		<skos:prefLabel xml:lang="tr">Arazi ve arsa düzenlemesi</skos:prefLabel>
		<skos:changeNote>Established with version 2.</skos:changeNote>
		<skos:exactMatch rdf:resource="http://aims.fao.org/aos/agrovoc/c_57156ff8"/>
		<skos:inScheme rdf:resource="https://www.opengis.net/def/CaLAThe/5.0"/>
		<skos:broader rdf:resource="https://www.opengis.net/def/CaLAThe/5.0/PropertyRestructuring"/>
		<skos:narrower rdf:resource="https://www.opengis.net/def/CaLAThe/5.0/Reallotment"/>
	</skos:Concept>
	<skos:Concept rdf:about="https://www.opengis.net/def/CaLAThe/5.0/LandRegister">
		<skos:prefLabel xml:lang="en">Land register</skos:prefLabel>
		<skos:prefLabel xml:lang="da">Tinglysningsrettens register</skos:prefLabel>
		<skos:prefLabel xml:lang="tr">Tapu sicili</skos:prefLabel>
		<skos:changeNote>Established with version 1.</skos:changeNote>
		<skos:exactMatch rdf:resource="http://aims.fao.org/aos/agrovoc/c_a72beecd"/>
		<skos:exactMatch rdf:resource="http://www.eionet.europa.eu/gemet/concept/4644"/>
		<skos:inScheme rdf:resource="https://www.opengis.net/def/CaLAThe/5.0"/>
		<skos:altLabel>Land registry</skos:altLabel>
		<skos:broader rdf:resource="https://www.opengis.net/def/CaLAThe/5.0/Registry"/>
		<skos:narrower rdf:resource="https://www.opengis.net/def/CaLAThe/5.0/CadastralSystem"/>
	</skos:Concept>
	<skos:Concept rdf:about="https://www.opengis.net/def/CaLAThe/5.0/Law">
		<skos:prefLabel xml:lang="en">Law</skos:prefLabel>
		<skos:prefLabel xml:lang="da">Lov, jura, ret</skos:prefLabel>
		<skos:prefLabel xml:lang="tr">Hukuk</skos:prefLabel>
		<skos:scopeNote>STW Thesaurus for Economics term</skos:scopeNote>
		<skos:changeNote>Established with version 1.</skos:changeNote>
		<skos:exactMatch rdf:resource="http://zbw.eu/stw/descriptor/15966-1"/>
		<skos:exactMatch rdf:resource="http://aims.fao.org/aos/agrovoc/c_12106"/>
		<skos:exactMatch rdf:resource="https://www.eionet.europa.eu/gemet/en/concept/4719"/>
		<skos:exactMatch rdf:resource="http://eurovoc.europa.eu/3935"/>
		<skos:inScheme rdf:resource="https://www.opengis.net/def/CaLAThe/5.0"/>
		<skos:topConceptOf rdf:resource="https://www.opengis.net/def/CaLAThe/5.0"/>
		<skos:narrower rdf:resource="https://www.opengis.net/def/CaLAThe/5.0/PartyRoleType"/>
		<skos:narrower rdf:resource="https://www.opengis.net/def/CaLAThe/5.0/CustomaryLaw"/>
		<skos:narrower rdf:resource="https://www.opengis.net/def/CaLAThe/5.0/PositiveLaw"/>
		<skos:narrower rdf:resource="https://www.opengis.net/def/CaLAThe/5.0/NaturalLaw"/>
	</skos:Concept>
	<skos:Concept rdf:about="https://www.opengis.net/def/CaLAThe/5.0/LawOfObligation">
		<skos:prefLabel xml:lang="en">Law of obligation</skos:prefLabel>
		<skos:prefLabel xml:lang="da">Obligationsret</skos:prefLabel>
		<skos:prefLabel xml:lang="tr">Borçlar Hukuku</skos:prefLabel>
		<skos:scopeNote>Added in version 5 to represent personal rights (cf. Swiss Civil Law, article 959) that can be entered into land book.</skos:scopeNote>
		<skos:inScheme rdf:resource="https://www.opengis.net/def/CaLAThe/5.0"/>
		<skos:broader rdf:resource="https://www.opengis.net/def/CaLAThe/5.0/LandLaw"/>
		<skos:narrower rdf:resource="https://www.opengis.net/def/CaLAThe/5.0/OptionToPurchase"/>
		<skos:narrower rdf:resource="https://www.opengis.net/def/CaLAThe/5.0/PreemptionRight"/>
	</skos:Concept>
	<skos:Concept rdf:about="https://www.opengis.net/def/CaLAThe/5.0/Lawyer">
		<skos:prefLabel xml:lang="en">Lawyer</skos:prefLabel>
		<skos:prefLabel xml:lang="da">Advokat</skos:prefLabel>
		<skos:prefLabel xml:lang="tr">Hukukçu</skos:prefLabel>
		<skos:changeNote>Established with version 3.</skos:changeNote>
		<skos:exactMatch rdf:resource="http://eurovoc.europa.eu/5141"/>
		<skos:inScheme rdf:resource="https://www.opengis.net/def/CaLAThe/5.0"/>
		<skos:broader rdf:resource="https://www.opengis.net/def/CaLAThe/5.0/Professional"/>
		<skos:narrower rdf:resource="https://www.opengis.net/def/CaLAThe/5.0/LegalAdvisor"/>
	</skos:Concept>
	<skos:Concept rdf:about="https://www.opengis.net/def/CaLAThe/5.0/LA_AdministrativeSource">
		<skos:prefLabel xml:lang="en">LA_AdministrativeSource</skos:prefLabel>
		<skos:scopeNote>ISO LADM term</skos:scopeNote>
		<skos:definition>Source (4.1.21) with the administrative description (where applicable) of the parties (4.1.13) involved, the rights (4.1.20), restrictions (4.1.19) and responsibilities (4.1.18) created and the basic administrative units (4.1.2) affected (Source: ISO LADM, 4.1.1).</skos:definition>
		<skos:changeNote>Established with version 3.</skos:changeNote>
		<skos:exactMatch rdf:resource="https://isotc211.geolexica.org/concepts/1286/"/>
		<skos:inScheme rdf:resource="https://www.opengis.net/def/CaLAThe/5.0"/>
		<skos:broader rdf:resource="https://www.opengis.net/def/CaLAThe/5.0/LA_Source"/>
	</skos:Concept>
	<skos:Concept rdf:about="https://www.opengis.net/def/CaLAThe/5.0/LA_BAUnit">
		<skos:prefLabel xml:lang="en">LA_BAUnit</skos:prefLabel>
		<skos:prefLabel xml:lang="da">.</skos:prefLabel>
		<skos:prefLabel xml:lang="tr">.</skos:prefLabel>
		<skos:scopeNote>ISO LADM term</skos:scopeNote>
		<skos:definition>Administrative entity, subject to registration, consisting of zero or more spatial units (4.1.23) against which (one or more) unique and homogeneous rights [e.g. ownership right or land (4.1.9) use right], responsibilities (4.1.18) or restrictions (4.1.19) are associated to the whole entity (Source: ISO LADM, 4.1.2 - here simplified)</skos:definition>
		<skos:changeNote>Established with version 1.</skos:changeNote>
		<skos:exactMatch rdf:resource="http://aims.fao.org/aos/agrovoc/c_3022da1f"/>
		<skos:exactMatch rdf:resource="https://isotc211.geolexica.org/concepts/1570/"/>
		<skos:inScheme rdf:resource="https://www.opengis.net/def/CaLAThe/5.0"/>
		<skos:broader rdf:resource="https://www.opengis.net/def/CaLAThe/5.0/RealProperty"/>
	</skos:Concept>
	<skos:Concept rdf:about="https://www.opengis.net/def/CaLAThe/5.0/LA_BoundaryFaceString">
		<skos:prefLabel xml:lang="en">LA_BoundaryFaceString</skos:prefLabel>
		<skos:prefLabel xml:lang="da">.</skos:prefLabel>
		<skos:prefLabel xml:lang="tr">.</skos:prefLabel>
		<skos:scopeNote>ISO LADM term</skos:scopeNote>
		<skos:changeNote>Established with version 3. Relation edited with version 4.</skos:changeNote>
		<skos:exactMatch rdf:resource="http://aims.fao.org/aos/agrovoc/c_c9ac54c9"/>
		<skos:exactMatch rdf:resource="https://isotc211.geolexica.org/concepts/1289/"/>
		<skos:inScheme rdf:resource="https://www.opengis.net/def/CaLAThe/5.0"/>
		<skos:broader rdf:resource="https://www.opengis.net/def/CaLAThe/5.0/BoundingElement"/>
	</skos:Concept>
	<skos:Concept rdf:about="https://www.opengis.net/def/CaLAThe/5.0/LA_CertifiedSurveyor">
		<skos:prefLabel xml:lang="en">LA_CertifiedSurveyor</skos:prefLabel>
		<skos:prefLabel xml:lang="da">.</skos:prefLabel>
		<skos:prefLabel xml:lang="tr">.</skos:prefLabel>
		<skos:scopeNote>ISO LADM</skos:scopeNote>
		<skos:changeNote>Established with version 4</skos:changeNote>
		<skos:inScheme rdf:resource="https://www.opengis.net/def/CaLAThe/5.0"/>
		<skos:broader rdf:resource="https://www.opengis.net/def/CaLAThe/5.0/Surveyor"/>
	</skos:Concept>
	<skos:Concept rdf:about="https://www.opengis.net/def/CaLAThe/5.0/LA_EdgeBasedSpatialUnit">
		<skos:prefLabel xml:lang="en">LA_Edge based spatial unit</skos:prefLabel>
		<skos:prefLabel xml:lang="da">.</skos:prefLabel>
		<skos:prefLabel xml:lang="tr">.</skos:prefLabel>
		<skos:scopeNote>ISO LADM term</skos:scopeNote>
		<skos:changeNote>Established with version 1. Edited with version 4</skos:changeNote>
		<skos:exactMatch rdf:resource="http://aims.fao.org/aos/agrovoc/c_268654bb"/>
		<skos:inScheme rdf:resource="https://www.opengis.net/def/CaLAThe/5.0"/>
		<skos:broader rdf:resource="https://www.opengis.net/def/CaLAThe/5.0/Edge"/>
	</skos:Concept>
	<skos:Concept rdf:about="https://www.opengis.net/def/CaLAThe/5.0/LA_FaceBasedSpatialUnit">
		<skos:prefLabel xml:lang="en">LA_Face based spatial unit</skos:prefLabel>
		<skos:prefLabel xml:lang="da">.</skos:prefLabel>
		<skos:prefLabel xml:lang="tr">.</skos:prefLabel>
		<skos:scopeNote>ISO LADM term</skos:scopeNote>
		<skos:changeNote>Established with version 1. Edited with version 4.</skos:changeNote>
		<skos:exactMatch rdf:resource="http://aims.fao.org/aos/agrovoc/c_9e450562"/>
		<skos:inScheme rdf:resource="https://www.opengis.net/def/CaLAThe/5.0"/>
		<skos:broader rdf:resource="https://www.opengis.net/def/CaLAThe/5.0/Face"/>
	</skos:Concept>
	<skos:Concept rdf:about="https://www.opengis.net/def/CaLAThe/5.0/LA_LegalSpaceBuildingUnit">
		<skos:prefLabel xml:lang="en">LA_LegalSpaceBuildingUnit</skos:prefLabel>
		<skos:prefLabel xml:lang="da">.</skos:prefLabel>
		<skos:prefLabel xml:lang="tr">.</skos:prefLabel>
		<skos:scopeNote>ISO LADM term</skos:scopeNote>
		<skos:definition>Component of building (the legal, recorded or informal space of the physical entity) (Source: ISO LADM, 4.1.6).</skos:definition>
		<skos:changeNote>Established with version 3.</skos:changeNote>
		<skos:inScheme rdf:resource="https://www.opengis.net/def/CaLAThe/5.0"/>
		<skos:broader rdf:resource="https://www.opengis.net/def/CaLAThe/5.0/CondominiumBuilding"/>
	</skos:Concept>
	<skos:Concept rdf:about="https://www.opengis.net/def/CaLAThe/5.0/LA_LineBasedSpatialUnit">
		<skos:prefLabel xml:lang="en">LA_Line based spatial unit</skos:prefLabel>
		<skos:prefLabel xml:lang="da">.</skos:prefLabel>
		<skos:prefLabel xml:lang="tr">.</skos:prefLabel>
		<skos:scopeNote>ISO LADM term</skos:scopeNote>
		<skos:changeNote>Established with version 1. Edited to LA_Line .. with version 4</skos:changeNote>
		<skos:inScheme rdf:resource="https://www.opengis.net/def/CaLAThe/5.0"/>
		<skos:broader rdf:resource="https://www.opengis.net/def/CaLAThe/5.0/GeometricPrimitive"/>
	</skos:Concept>
	<skos:Concept rdf:about="https://www.opengis.net/def/CaLAThe/5.0/LA_NodeBasedSpatialUnit">
		<skos:prefLabel xml:lang="en">LA_Node based spatial unit</skos:prefLabel>
		<skos:prefLabel xml:lang="da">.</skos:prefLabel>
		<skos:prefLabel xml:lang="tr">.</skos:prefLabel>
		<skos:scopeNote>ISO LADM term</skos:scopeNote>
		<skos:changeNote>Introduced with version 1. Edited with version 4</skos:changeNote>
		<skos:exactMatch rdf:resource="http://aims.fao.org/aos/agrovoc/c_4be99d5b"/>
		<skos:inScheme rdf:resource="https://www.opengis.net/def/CaLAThe/5.0"/>
		<skos:broader rdf:resource="https://www.opengis.net/def/CaLAThe/5.0/Node"/>
	</skos:Concept>
	<skos:Concept rdf:about="https://www.opengis.net/def/CaLAThe/5.0/LA_Point">
		<skos:prefLabel xml:lang="en">LA_Point</skos:prefLabel>
		<skos:prefLabel xml:lang="da">.</skos:prefLabel>
		<skos:prefLabel xml:lang="tr">.</skos:prefLabel>
		<skos:scopeNote>LADM term</skos:scopeNote>
		<skos:definition>0-dimensional geometric primitive, representing a position [ISO 19107:2003, 4.61] (Source: ISO LADM, 4.1.15).</skos:definition>
		<skos:changeNote>Established with version 3.</skos:changeNote>
		<skos:exactMatch rdf:resource="http://aims.fao.org/aos/agrovoc/c_b12823a4"/>
		<skos:inScheme rdf:resource="https://www.opengis.net/def/CaLAThe/5.0"/>
		<skos:broader rdf:resource="https://www.opengis.net/def/CaLAThe/5.0/GeometricPrimitive"/>
	</skos:Concept>
	<skos:Concept rdf:about="https://www.opengis.net/def/CaLAThe/5.0/LA_PointBasedSpatialUnit">
		<skos:prefLabel xml:lang="en">LA_Point based spatial unit</skos:prefLabel>
		<skos:prefLabel xml:lang="da">.</skos:prefLabel>
		<skos:prefLabel xml:lang="tr">.</skos:prefLabel>
		<skos:scopeNote>ISO LADM term</skos:scopeNote>
		<skos:changeNote>Established with version 1.0. Changed to LA_Point... with version 4</skos:changeNote>
		<skos:inScheme rdf:resource="https://www.opengis.net/def/CaLAThe/5.0"/>
		<skos:broader rdf:resource="https://www.opengis.net/def/CaLAThe/5.0/GeometricPrimitive"/>
	</skos:Concept>
	<skos:Concept rdf:about="https://www.opengis.net/def/CaLAThe/5.0/PolygonBasedSpatialUnit">
		<skos:prefLabel xml:lang="en">LA_Polygon based spatial unit</skos:prefLabel>
		<skos:prefLabel xml:lang="da">.</skos:prefLabel>
		<skos:prefLabel xml:lang="tr">.</skos:prefLabel>
		<skos:scopeNote>ISO LADM term</skos:scopeNote>
		<skos:changeNote>Established with version 1.0. Edited to LA_Polygon.. with version 4</skos:changeNote>
		<skos:inScheme rdf:resource="https://www.opengis.net/def/CaLAThe/5.0"/>
		<skos:broader rdf:resource="https://www.opengis.net/def/CaLAThe/5.0/GeometricPrimitive"/>
	</skos:Concept>
	<skos:Concept rdf:about="https://www.opengis.net/def/CaLAThe/5.0/LA_RequiredRelationship">
		<skos:prefLabel xml:lang="en">LA_RequiredRelationship</skos:prefLabel>
		<skos:prefLabel xml:lang="da">.</skos:prefLabel>
		<skos:prefLabel xml:lang="tr">.</skos:prefLabel>
		<skos:scopeNote>LADM term</skos:scopeNote>
		<skos:changeNote>Established with version 3, revised as concept in version 5.</skos:changeNote>
		<skos:exactMatch rdf:resource="https://isotc211.geolexica.org/concepts/1362/"/>
		<skos:inScheme rdf:resource="https://www.opengis.net/def/CaLAThe/5.0"/>
		<skos:broader rdf:resource="https://www.opengis.net/def/CaLAThe/5.0/RealProperty"/>
	</skos:Concept>
	<skos:Concept rdf:about="https://www.opengis.net/def/CaLAThe/5.0/LA_Restriction">
		<skos:prefLabel xml:lang="en">LA_Restriction</skos:prefLabel>
		<skos:prefLabel xml:lang="da">.</skos:prefLabel>
		<skos:prefLabel xml:lang="tr">.</skos:prefLabel>
		<skos:scopeNote>ISO LADM term</skos:scopeNote>
		<skos:definition>Formal or informal obligation to refrain from doing something (Source: ISO LADM, 4.1.18).</skos:definition>
		<skos:changeNote>Established with version 3.</skos:changeNote>
		<skos:exactMatch rdf:resource="https://isotc211.geolexica.org/concepts/1573/"/>
		<skos:inScheme rdf:resource="https://www.opengis.net/def/CaLAThe/5.0"/>
		<skos:broader rdf:resource="https://www.opengis.net/def/CaLAThe/5.0/LimitedRight"/>
	</skos:Concept>
	<skos:Concept rdf:about="https://www.opengis.net/def/CaLAThe/5.0/LA_Right">
		<skos:prefLabel xml:lang="en">LA_Right</skos:prefLabel>
		<skos:prefLabel xml:lang="da">.</skos:prefLabel>
		<skos:prefLabel xml:lang="tr">.</skos:prefLabel>
		<skos:scopeNote>ISO LADM term</skos:scopeNote>
		<skos:definition>Action, activity or class of actions that a system participant may perform on or using an associated resource [ISO 19132:2007, 4.38] (Source: ISO LADM, 4.1.20).</skos:definition>
		<skos:changeNote>Established with version 3.</skos:changeNote>
		<skos:exactMatch rdf:resource="https://isotc211.geolexica.org/concepts/680/"/>
		<skos:inScheme rdf:resource="https://www.opengis.net/def/CaLAThe/5.0"/>
		<skos:broader rdf:resource="https://www.opengis.net/def/CaLAThe/5.0/RealRight"/>
	</skos:Concept>
	<skos:Concept rdf:about="https://www.opengis.net/def/CaLAThe/5.0/LA_RRR">
		<skos:prefLabel xml:lang="en">LA_RRR</skos:prefLabel>
		<skos:prefLabel xml:lang="da">.</skos:prefLabel>
		<skos:prefLabel xml:lang="tr">.</skos:prefLabel>
		<skos:scopeNote>ISO LADM term</skos:scopeNote>
		<skos:definition>LA_RRR is an abstract class with three specialization classes: LA_Right, with rights as instances, LA_Restriction, with restrictions as instances, and LA_Responsibility, with responsibilities as instances. In principle, all rights, restrictions and responsibilities are based on an administrative source, as instances from class LA_AdministrativeSource (Source: ISO LADM, 5.4).</skos:definition>
		<skos:changeNote>Established with version 3.</skos:changeNote>
		<skos:inScheme rdf:resource="https://www.opengis.net/def/CaLAThe/5.0"/>
		<skos:broader rdf:resource="https://www.opengis.net/def/CaLAThe/5.0/LandLaw"/>
	</skos:Concept>
	<skos:Concept rdf:about="https://www.opengis.net/def/CaLAThe/5.0/LA_Source">
		<skos:prefLabel xml:lang="en">LA_Source</skos:prefLabel>
		<skos:prefLabel xml:lang="da">.</skos:prefLabel>
		<skos:prefLabel xml:lang="tr">.</skos:prefLabel>
		<skos:scopeNote>ISO LADM term</skos:scopeNote>
		<skos:definition>Document providing legal and/or administrative facts on which the land administration (LA) object [right (4.1.20), restriction (4.1.19), responsibility (4.1.18), basic administrative unit (4.1.2), party (4.1.13), or spatial unit (4.1.23)] is based on (Source: ISO LADM, 4.1.21).</skos:definition>
		<skos:changeNote>Established with version 3.</skos:changeNote>
		<skos:exactMatch rdf:resource="http://aims.fao.org/aos/agrovoc/c_10265135"/>
		<skos:exactMatch rdf:resource="https://isotc211.geolexica.org/concepts/1574/"/>
		<skos:inScheme rdf:resource="https://www.opengis.net/def/CaLAThe/5.0"/>
		<skos:broader rdf:resource="https://www.opengis.net/def/CaLAThe/5.0/Document"/>
		<skos:narrower rdf:resource="https://www.opengis.net/def/CaLAThe/5.0/LA_AdministrativeSource"/>
		<skos:narrower rdf:resource="https://www.opengis.net/def/CaLAThe/5.0/LA_SpatialSource"/>
	</skos:Concept>
	<skos:Concept rdf:about="https://www.opengis.net/def/CaLAThe/5.0/LA_SpatialSource">
		<skos:prefLabel xml:lang="en">LA_SpatialSource</skos:prefLabel>
		<skos:prefLabel xml:lang="da">.</skos:prefLabel>
		<skos:prefLabel xml:lang="tr">.</skos:prefLabel>
		<skos:scopeNote>ISO LADM term</skos:scopeNote>
		<skos:definition>Source (4.1.21) with the spatial representation of one (part of) or more spatial units (4.1.23) (Source: LADM, 2012, 4.1.22).</skos:definition>
		<skos:changeNote>Established with version 3.</skos:changeNote>
		<skos:exactMatch rdf:resource="http://aims.fao.org/aos/agrovoc/c_cf5b0fc7"/>
		<skos:exactMatch rdf:resource="https://isotc211.geolexica.org/concepts/1316/"/>
		<skos:inScheme rdf:resource="https://www.opengis.net/def/CaLAThe/5.0"/>
		<skos:broader rdf:resource="https://www.opengis.net/def/CaLAThe/5.0/LA_Source"/>
	</skos:Concept>
	<skos:Concept rdf:about="https://www.opengis.net/def/CaLAThe/5.0/Lease">
		<skos:prefLabel xml:lang="en">Lease</skos:prefLabel>
		<skos:prefLabel xml:lang="da">Lejemål, forpagtning</skos:prefLabel>
		<skos:prefLabel xml:lang="tr">.</skos:prefLabel>
		<skos:changeNote>Established with version 2. Relation to Leasehold added with version 3.</skos:changeNote>
		<skos:exactMatch rdf:resource="http://aims.fao.org/aos/agrovoc/c_4240"/>
		<skos:exactMatch rdf:resource="https://www.eionet.europa.eu/gemet/en/concept/11611"/>
		<skos:exactMatch rdf:resource="http://eurovoc.europa.eu/4598"/>
		<skos:exactMatch rdf:resource="https://isotc211.geolexica.org/concepts/1230/"/>
		<skos:inScheme rdf:resource="https://www.opengis.net/def/CaLAThe/5.0"/>
		<skos:broader rdf:resource="https://www.opengis.net/def/CaLAThe/5.0/Exchange"/>
		<skos:related rdf:resource="https://www.opengis.net/def/CaLAThe/5.0/Leasehold"/>
	</skos:Concept>
	<skos:Concept rdf:about="https://www.opengis.net/def/CaLAThe/5.0/Leasehold">
		<skos:prefLabel xml:lang="en">Leasehold</skos:prefLabel>
		<skos:prefLabel xml:lang="da">Forpagtning</skos:prefLabel>
		<skos:prefLabel xml:lang="tr">.</skos:prefLabel>
		<skos:scopeNote>EULIS / ELRA term</skos:scopeNote>
		<skos:definition>The right to possess immovable property for an agreed period of time in return for an agreed consideration  (Source: EULIS / ELRA glossary).</skos:definition>
		<skos:changeNote>Established with version 3.</skos:changeNote>
		<skos:exactMatch rdf:resource="http://aims.fao.org/aos/agrovoc/c_d80e0cd0"/>
		<skos:inScheme rdf:resource="https://www.opengis.net/def/CaLAThe/5.0"/>
		<skos:broader rdf:resource="https://www.opengis.net/def/CaLAThe/5.0/RealRight"/>
		<skos:related rdf:resource="https://www.opengis.net/def/CaLAThe/5.0/Lease"/>
	</skos:Concept>
	<skos:Concept rdf:about="https://www.opengis.net/def/CaLAThe/5.0/LegalAdvisor">
		<skos:prefLabel xml:lang="en">Legal advisor</skos:prefLabel>
		<skos:prefLabel xml:lang="da">Juridisk rådgiver</skos:prefLabel>
		<skos:prefLabel xml:lang="tr">Yasal danışman</skos:prefLabel>
		<skos:changeNote>Established with version 1.</skos:changeNote>
		<skos:exactMatch rdf:resource="http://eurovoc.europa.eu/3989"/>
		<skos:inScheme rdf:resource="https://www.opengis.net/def/CaLAThe/5.0"/>
		<skos:broader rdf:resource="https://www.opengis.net/def/CaLAThe/5.0/Lawyer"/>
	</skos:Concept>
	<skos:Concept rdf:about="https://www.opengis.net/def/CaLAThe/5.0/LegalBoundaryDetermination">
		<skos:prefLabel xml:lang="en">Legal boundary determination</skos:prefLabel>
		<skos:prefLabel xml:lang="da">Skelforretning</skos:prefLabel>
		<skos:prefLabel xml:lang="tr">Hükmen sınır belirleme</skos:prefLabel>
		<skos:changeNote>Established with version 2.</skos:changeNote>
		<skos:inScheme rdf:resource="https://www.opengis.net/def/CaLAThe/5.0"/>
		<skos:broader rdf:resource="https://www.opengis.net/def/CaLAThe/5.0/BoundarySurveyAndMarking"/>
	</skos:Concept>
	<skos:Concept rdf:about="https://www.opengis.net/def/CaLAThe/5.0/LegalPerson">
		<skos:prefLabel xml:lang="en">Legal person</skos:prefLabel>
		<skos:prefLabel xml:lang="da">Juridisk person</skos:prefLabel>
		<skos:prefLabel xml:lang="tr">Tüzel kişi</skos:prefLabel>
		<skos:definition>Public or private institution endowed with a legal personality (Source: Legal Dictionary of Property in Canada - Dualjuridik).</skos:definition>
		<skos:changeNote>Established with version 1. Definition and relation to Organisation added with version 3. Broader edited with version 4.</skos:changeNote>
		<skos:exactMatch rdf:resource="http://eurovoc.europa.eu/2337"/>
		<skos:inScheme rdf:resource="https://www.opengis.net/def/CaLAThe/5.0"/>
		<skos:broader rdf:resource="https://www.opengis.net/def/CaLAThe/5.0/Organisation"/>
	</skos:Concept>
	<skos:Concept rdf:about="https://www.opengis.net/def/CaLAThe/5.0/LegalPersonality">
		<skos:prefLabel xml:lang="en">Legal personality</skos:prefLabel>
		<skos:prefLabel xml:lang="da">Retsevne, Retlig status</skos:prefLabel>
		<skos:prefLabel xml:lang="tr">Kişisel hak</skos:prefLabel>
		<skos:changeNote>Established with version 1.0. Edited from Personal right to Legal personality with version 5 to comply with dictionaries, incl EuroVoc</skos:changeNote>
		<skos:exactMatch rdf:resource="http://eurovoc.europa.eu/4274"/>
		<skos:inScheme rdf:resource="https://www.opengis.net/def/CaLAThe/5.0"/>
		<skos:broader rdf:resource="https://www.opengis.net/def/CaLAThe/5.0/NaturalPersonRole"/>
		<skos:narrower rdf:resource="https://www.opengis.net/def/CaLAThe/5.0/Signatory"/>
	</skos:Concept>
	<skos:Concept rdf:about="https://www.opengis.net/def/CaLAThe/5.0/Lessee">
		<skos:prefLabel xml:lang="en">Lessee</skos:prefLabel>
		<skos:prefLabel xml:lang="da">Forpagter</skos:prefLabel>
		<skos:prefLabel xml:lang="tr">Kiracı</skos:prefLabel>
		<skos:scopeNote>EULIS / ELRA term</skos:scopeNote>
		<skos:definition>A person to whom a lease is granted (Source: EULIS / ELRA glossary).</skos:definition>
		<skos:changeNote>Established with version 3.</skos:changeNote>
		<skos:inScheme rdf:resource="https://www.opengis.net/def/CaLAThe/5.0"/>
		<skos:broader rdf:resource="https://www.opengis.net/def/CaLAThe/5.0/RightsHolder"/>
	</skos:Concept>
	<skos:Concept rdf:about="https://www.opengis.net/def/CaLAThe/5.0/Lessor">
		<skos:prefLabel xml:lang="en">Lessor</skos:prefLabel>
		<skos:prefLabel xml:lang="da">Bortforpagter</skos:prefLabel>
		<skos:prefLabel xml:lang="tr">Kiraya veren</skos:prefLabel>
		<skos:scopeNote>EULIS / ELRA term</skos:scopeNote>
		<skos:definition>A person who grants a lease (Source: EULIS / ELRA glossary).</skos:definition>
		<skos:changeNote>Established with version 3.</skos:changeNote>
		<skos:inScheme rdf:resource="https://www.opengis.net/def/CaLAThe/5.0"/>
		<skos:broader rdf:resource="https://www.opengis.net/def/CaLAThe/5.0/RightsHolder"/>
	</skos:Concept>
	<skos:Concept rdf:about="https://www.opengis.net/def/CaLAThe/5.0/LevelObservation">
		<skos:prefLabel xml:lang="en">Level observation</skos:prefLabel>
		<skos:prefLabel xml:lang="da">Højdemåling</skos:prefLabel>
		<skos:prefLabel xml:lang="tr">Düzey gözlemi</skos:prefLabel>
		<skos:scopeNote>OGC LandInfra / InfraGML term</skos:scopeNote>
		<skos:changeNote>Established with version 4</skos:changeNote>
		<skos:inScheme rdf:resource="https://www.opengis.net/def/CaLAThe/5.0"/>
		<skos:broader rdf:resource="https://www.opengis.net/def/CaLAThe/5.0/LevelingInstrument"/>
		<skos:broader rdf:resource="https://www.opengis.net/def/CaLAThe/5.0/Observation"/>
	</skos:Concept>
	<skos:Concept rdf:about="https://www.opengis.net/def/CaLAThe/5.0/LevelingInstrument">
		<skos:prefLabel xml:lang="en">Leveling instrument</skos:prefLabel>
		<skos:prefLabel xml:lang="da">Nivellerinstrument</skos:prefLabel>
		<skos:prefLabel xml:lang="tr">Nivo</skos:prefLabel>
		<skos:definition>Level sensors are used to determine the height difference between two locations (OGC LandInfra 7.8.5.11)</skos:definition>
		<skos:changeNote>Established with version 4</skos:changeNote>
		<skos:exactMatch rdf:resource="http://docs.opengeospatial.org/is/15-111r1/15-111r1.html#146"/>
		<skos:inScheme rdf:resource="https://www.opengis.net/def/CaLAThe/5.0"/>
		<skos:broader rdf:resource="https://www.opengis.net/def/CaLAThe/5.0/SurveyingInstrument"/>
		<skos:narrower rdf:resource="https://www.opengis.net/def/CaLAThe/5.0/LevelObservation"/>
	</skos:Concept>
	<skos:Concept rdf:about="https://www.opengis.net/def/CaLAThe/5.0/LicensedSurveyor">
		<skos:prefLabel xml:lang="en">Licensed surveyor</skos:prefLabel>
		<skos:prefLabel xml:lang="da">Landinspektør med beskikkelse</skos:prefLabel>
		<skos:prefLabel xml:lang="tr">Lisanslı haritacı</skos:prefLabel>
		<skos:scopeNote>OGC LandInfra / InfraGML term</skos:scopeNote>
		<skos:definition>Surveyor, who through a license is bound to act according to the standards of a professional association (cf. OGC LandInfra, 4.1.19)</skos:definition>
		<skos:changeNote>Established with version 1.  Definition with version 4</skos:changeNote>
		<skos:inScheme rdf:resource="https://www.opengis.net/def/CaLAThe/5.0"/>
		<skos:broader rdf:resource="https://www.opengis.net/def/CaLAThe/5.0/Surveyor"/>
	</skos:Concept>
	<skos:Concept rdf:about="https://www.opengis.net/def/CaLAThe/5.0/Lien">
		<skos:prefLabel xml:lang="en">Lien</skos:prefLabel>
		<skos:prefLabel xml:lang="da">Tilbageholdsret</skos:prefLabel>
		<skos:prefLabel xml:lang="tr">Haciz hakkı</skos:prefLabel>
		<skos:changeNote>Established with version 3.</skos:changeNote>
		<skos:inScheme rdf:resource="https://www.opengis.net/def/CaLAThe/5.0"/>
		<skos:broader rdf:resource="https://www.opengis.net/def/CaLAThe/5.0/Mortgage"/>
	</skos:Concept>
	<skos:Concept rdf:about="https://www.opengis.net/def/CaLAThe/5.0/Liminal">
		<skos:prefLabel xml:lang="en">Liminal</skos:prefLabel>
		<skos:prefLabel xml:lang="da">.</skos:prefLabel>
		<skos:prefLabel xml:lang="tr">.</skos:prefLabel>
		<skos:scopeNote>OGC LandInfra / InfraGML term</skos:scopeNote>
		<skos:definition>Dimension type, cf. OGC LandInfra 7.10.6 SpatialUnit</skos:definition>
		<skos:changeNote>Established with version 4</skos:changeNote>
		<skos:inScheme rdf:resource="https://www.opengis.net/def/CaLAThe/5.0"/>
		<skos:broader rdf:resource="https://www.opengis.net/def/CaLAThe/5.0/DimensionType"/>
	</skos:Concept>
	<skos:Concept rdf:about="https://www.opengis.net/def/CaLAThe/5.0/LimitedRight">
		<skos:prefLabel xml:lang="en">Limited right</skos:prefLabel>
		<skos:prefLabel xml:lang="da">Begrænset ejendomsret</skos:prefLabel>
		<skos:prefLabel xml:lang="tr">Sınırlı ayni hak</skos:prefLabel>
		<skos:changeNote>Established with version 3.</skos:changeNote>
		<skos:inScheme rdf:resource="https://www.opengis.net/def/CaLAThe/5.0"/>
		<skos:broader rdf:resource="https://www.opengis.net/def/CaLAThe/5.0/RealRight"/>
		<skos:narrower rdf:resource="https://www.opengis.net/def/CaLAThe/5.0/Usufruct"/>
		<skos:narrower rdf:resource="https://www.opengis.net/def/CaLAThe/5.0/Easement"/>
		<skos:narrower rdf:resource="https://www.opengis.net/def/CaLAThe/5.0/SecurityInterest"/>
		<skos:narrower rdf:resource="https://www.opengis.net/def/CaLAThe/5.0/LA_Restriction"/>
	</skos:Concept>
	<skos:Concept rdf:about="https://www.opengis.net/def/CaLAThe/5.0/LineString">
		<skos:prefLabel xml:lang="en">Line string</skos:prefLabel>
		<skos:prefLabel xml:lang="da">Kurve, dannet af retlinede seg</skos:prefLabel>
		<skos:prefLabel xml:lang="tr">Düz çizgi</skos:prefLabel>
		<skos:scopeNote>Geolexica term</skos:scopeNote>
		<skos:definition>Curve composed of straight-line segments (Geolexica ISO 19136:2007)</skos:definition>
		<skos:changeNote>Established with version 4</skos:changeNote>
		<skos:exactMatch rdf:resource="https://isotc211.geolexica.org/concepts/270/"/>
		<skos:inScheme rdf:resource="https://www.opengis.net/def/CaLAThe/5.0"/>
		<skos:broader rdf:resource="https://www.opengis.net/def/CaLAThe/5.0/Curve"/>
		<skos:broader rdf:resource="https://www.opengis.net/def/CaLAThe/5.0/BEString"/>
		<skos:narrower rdf:resource="https://www.opengis.net/def/CaLAThe/5.0/Point"/>
	</skos:Concept>
	<skos:Concept rdf:about="https://www.opengis.net/def/CaLAThe/5.0/LI_LandSurveyor">
		<skos:prefLabel xml:lang="en">LI_LandSurveyor</skos:prefLabel>
		<skos:prefLabel xml:lang="da">.</skos:prefLabel>
		<skos:prefLabel xml:lang="tr">.</skos:prefLabel>
		<skos:scopeNote>OGC LandInfra</skos:scopeNote>
		<skos:changeNote>Established with version 4</skos:changeNote>
		<skos:inScheme rdf:resource="https://www.opengis.net/def/CaLAThe/5.0"/>
		<skos:broader rdf:resource="https://www.opengis.net/def/CaLAThe/5.0/Surveyor"/>
		<skos:broader rdf:resource="https://www.opengis.net/def/CaLAThe/5.0/Signatory"/>
	</skos:Concept>
	<skos:Concept rdf:about="https://www.opengis.net/def/CaLAThe/5.0/LI_Sensor">
		<skos:prefLabel xml:lang="en">LI_Sensor</skos:prefLabel>
		<skos:prefLabel xml:lang="da">.</skos:prefLabel>
		<skos:prefLabel xml:lang="tr">.</skos:prefLabel>
		<skos:scopeNote>OGC LandInfra / InfraGML term</skos:scopeNote>
		<skos:definition>Element of a measuring system that is directly affected by a phenomenon, body, or substance carrying a quantity to be measured (Source: ISO/TC 211 Glossary of Terms - English).</skos:definition>
		<skos:changeNote>Established with version 4</skos:changeNote>
		<skos:exactMatch rdf:resource="https://isotc211.geolexica.org/concepts/1108/"/>
		<skos:inScheme rdf:resource="https://www.opengis.net/def/CaLAThe/5.0"/>
		<skos:broader rdf:resource="https://www.opengis.net/def/CaLAThe/5.0/SurveyingInstrument"/>
	</skos:Concept>
	<skos:Concept rdf:about="https://www.opengis.net/def/CaLAThe/5.0/MainParcel">
		<skos:prefLabel xml:lang="en">Main Parcel</skos:prefLabel>
		<skos:prefLabel xml:lang="da">Hovedparcel</skos:prefLabel>
		<skos:prefLabel xml:lang="tr">Ana parcel (taşınmaz)</skos:prefLabel>
		<skos:scopeNote>OGC LandInfra / InfraGML term</skos:scopeNote>
		<skos:definition>Optional indication of a current LandParcel which is part of a LandPropertyUnit with more LandParcels, and which is chosen as reference for all LandParcels in the LandPropertyUnit. May be applied in jurisdictions where legal provisions do not recognize the concept of LandPropertyUnit (LandInfra 7.10.2.5)</skos:definition>
		<skos:changeNote>Established with version 4</skos:changeNote>
		<skos:inScheme rdf:resource="https://www.opengis.net/def/CaLAThe/5.0"/>
		<skos:broader rdf:resource="https://www.opengis.net/def/CaLAThe/5.0/CadastralParcel"/>
	</skos:Concept>
	<skos:Concept rdf:about="https://www.opengis.net/def/CaLAThe/5.0/Map">
		<skos:prefLabel xml:lang="en">Map</skos:prefLabel>
		<skos:prefLabel xml:lang="da">Kort, landkort</skos:prefLabel>
		<skos:prefLabel xml:lang="tr">Harita</skos:prefLabel>
		<skos:scopeNote>GEMET term</skos:scopeNote>
		<skos:definition>A representation, normally on a flat medium, that displays the physical and political features of a surface area of the earth, showing them in their respective forms, sizes and relationships according to some convention of representation (Source: Random House, 1997).</skos:definition>
		<skos:changeNote>Established with version 1.</skos:changeNote>
		<skos:exactMatch rdf:resource="http://www.eionet.europa.eu/gemet/concept/5011"/>
		<skos:exactMatch rdf:resource="http://aims.fao.org/aos/agrovoc/c_b43d8acf"/>
		<skos:exactMatch rdf:resource="http://zbw.eu/stw/descriptor/14814-1"/>
		<skos:inScheme rdf:resource="https://www.opengis.net/def/CaLAThe/5.0"/>
		<skos:broader rdf:resource="https://www.opengis.net/def/CaLAThe/5.0/GeolocatedInformation"/>
		<skos:narrower rdf:resource="https://www.opengis.net/def/CaLAThe/5.0/CadastralMap"/>
		<skos:narrower rdf:resource="https://www.opengis.net/def/CaLAThe/5.0/TopographicMap"/>
	</skos:Concept>
	<skos:Concept rdf:about="https://www.opengis.net/def/CaLAThe/5.0/Marker">
		<skos:prefLabel xml:lang="en">Marker</skos:prefLabel>
		<skos:prefLabel xml:lang="da">Markør</skos:prefLabel>
		<skos:prefLabel xml:lang="tr">Sınır noktası</skos:prefLabel>
		<skos:definition>Pole, plate, or other, used for marking and/or naming a location.</skos:definition>
		<skos:changeNote>Established with version 1. Definition is added in version 5.</skos:changeNote>
		<skos:inScheme rdf:resource="https://www.opengis.net/def/CaLAThe/5.0"/>
		<skos:broader rdf:resource="https://www.opengis.net/def/CaLAThe/5.0/LandDivision"/>
		<skos:narrower rdf:resource="https://www.opengis.net/def/CaLAThe/5.0/SurveyMark"/>
		<skos:narrower rdf:resource="https://www.opengis.net/def/CaLAThe/5.0/StreetSign"/>
	</skos:Concept>
	<skos:Concept rdf:about="https://www.opengis.net/def/CaLAThe/5.0/MeasuringTape">
		<skos:prefLabel xml:lang="en">Measuring tape</skos:prefLabel>
		<skos:prefLabel xml:lang="da">Målebånd</skos:prefLabel>
		<skos:prefLabel xml:lang="tr">Şerit metre</skos:prefLabel>
		<skos:changeNote>Established with version 4</skos:changeNote>
		<skos:inScheme rdf:resource="https://www.opengis.net/def/CaLAThe/5.0"/>
		<skos:broader rdf:resource="https://www.opengis.net/def/CaLAThe/5.0/SurveyingInstrument"/>
		<skos:narrower rdf:resource="https://www.opengis.net/def/CaLAThe/5.0/DistanceObservation"/>
	</skos:Concept>
	<skos:Concept rdf:about="https://www.opengis.net/def/CaLAThe/5.0/Metadata">
		<skos:prefLabel xml:lang="en">Metadata</skos:prefLabel>
		<skos:prefLabel xml:lang="da">Metadata</skos:prefLabel>
		<skos:prefLabel xml:lang="tr">Metaveri</skos:prefLabel>
		<skos:definition>Information about a resource</skos:definition>
		<skos:changeNote>Established with version 2. Broader relation changed with version 3 and 4</skos:changeNote>
		<skos:exactMatch rdf:resource="https://www.geolexica.org/concepts/1650/"/>
		<skos:exactMatch rdf:resource="http://aims.fao.org/aos/agrovoc/c_49829"/>
		<skos:exactMatch rdf:resource="http://eurovoc.europa.eu/c_40f54e0c"/>
		<skos:inScheme rdf:resource="https://www.opengis.net/def/CaLAThe/5.0"/>
		<skos:broader rdf:resource="https://www.opengis.net/def/CaLAThe/5.0/Information"/>
	</skos:Concept>
	<skos:Concept rdf:about="https://www.opengis.net/def/CaLAThe/5.0/Mortgage">
		<skos:prefLabel xml:lang="en">Mortgage</skos:prefLabel>
		<skos:prefLabel xml:lang="da">Pantehæftelse</skos:prefLabel>
		<skos:prefLabel xml:lang="tr">İpotek</skos:prefLabel>
		<skos:scopeNote>STW Thesaurus for Economics term</skos:scopeNote>
		<skos:definition>A security right to secure payment of a debt or other financial obligation (Source: EULIS / ELRA glossary).</skos:definition>
		<skos:changeNote>Established with version 1. Changed with v3 as narrower of Security right.</skos:changeNote>
		<skos:exactMatch rdf:resource="http://zbw.eu/stw/descriptor/13775-4"/>
		<skos:exactMatch rdf:resource="http://aims.fao.org/aos/agrovoc/c_4946"/>
		<skos:exactMatch rdf:resource="http://eurovoc.europa.eu/1281"/>
		<skos:inScheme rdf:resource="https://www.opengis.net/def/CaLAThe/5.0"/>
		<skos:altLabel>LA_Mortgage</skos:altLabel>
		<skos:broader rdf:resource="https://www.opengis.net/def/CaLAThe/5.0/SecurityInterest"/>
		<skos:narrower rdf:resource="https://www.opengis.net/def/CaLAThe/5.0/Lien"/>
	</skos:Concept>
	<skos:Concept rdf:about="https://www.opengis.net/def/CaLAThe/5.0/MortgageDeed">
		<skos:prefLabel xml:lang="en">Mortgage deed</skos:prefLabel>
		<skos:prefLabel xml:lang="da">Pantebrev</skos:prefLabel>
		<skos:prefLabel xml:lang="tr">İpotek sözleşmesi</skos:prefLabel>
		<skos:changeNote>Established with version 1.</skos:changeNote>
		<skos:inScheme rdf:resource="https://www.opengis.net/def/CaLAThe/5.0"/>
		<skos:broader rdf:resource="https://www.opengis.net/def/CaLAThe/5.0/Deed"/>
	</skos:Concept>
	<skos:Concept rdf:about="https://www.opengis.net/def/CaLAThe/5.0/Mortgagee">
		<skos:prefLabel xml:lang="en">Mortgagee</skos:prefLabel>
		<skos:prefLabel xml:lang="da">Panthaver</skos:prefLabel>
		<skos:prefLabel xml:lang="tr">İpotek alacaklısı</skos:prefLabel>
		<skos:changeNote>Established with version 1.</skos:changeNote>
		<skos:inScheme rdf:resource="https://www.opengis.net/def/CaLAThe/5.0"/>
		<skos:broader rdf:resource="https://www.opengis.net/def/CaLAThe/5.0/RightsHolder"/>
	</skos:Concept>
	<skos:Concept rdf:about="https://www.opengis.net/def/CaLAThe/5.0/Mortgaging">
		<skos:prefLabel xml:lang="en">Mortgaging</skos:prefLabel>
		<skos:prefLabel xml:lang="da">Pantsætning</skos:prefLabel>
		<skos:prefLabel xml:lang="tr">İpotek tesisi</skos:prefLabel>
		<skos:changeNote>Established with version 2.</skos:changeNote>
		<skos:inScheme rdf:resource="https://www.opengis.net/def/CaLAThe/5.0"/>
		<skos:broader rdf:resource="https://www.opengis.net/def/CaLAThe/5.0/Exchange"/>
	</skos:Concept>
	<skos:Concept rdf:about="https://www.opengis.net/def/CaLAThe/5.0/Mortgagor">
		<skos:prefLabel xml:lang="en">Mortgagor</skos:prefLabel>
		<skos:prefLabel xml:lang="da">Låntager</skos:prefLabel>
		<skos:prefLabel xml:lang="tr">İpotek borçlusu</skos:prefLabel>
		<skos:changeNote>Established with version 2.</skos:changeNote>
		<skos:inScheme rdf:resource="https://www.opengis.net/def/CaLAThe/5.0"/>
		<skos:broader rdf:resource="https://www.opengis.net/def/CaLAThe/5.0/RightsHolder"/>
	</skos:Concept>
	<skos:Concept rdf:about="https://www.opengis.net/def/CaLAThe/5.0/NationalSurveyAndCadastre">
		<skos:prefLabel xml:lang="en">National survey and cadastre</skos:prefLabel>
		<skos:prefLabel xml:lang="da">Geodatastyrelsen</skos:prefLabel>
		<skos:prefLabel xml:lang="tr">Tapu ve Kadastro G.M.</skos:prefLabel>
		<skos:changeNote>Established with version 1.</skos:changeNote>
		<skos:inScheme rdf:resource="https://www.opengis.net/def/CaLAThe/5.0"/>
		<skos:broader rdf:resource="https://www.opengis.net/def/CaLAThe/5.0/GovernmentalOrganisation"/>
	</skos:Concept>
	<skos:Concept rdf:about="https://www.opengis.net/def/CaLAThe/5.0/NaturalLaw">
		<skos:prefLabel xml:lang="en">Natural law</skos:prefLabel>
		<skos:prefLabel xml:lang="da">Naturret</skos:prefLabel>
		<skos:prefLabel xml:lang="tr">Doğal hukuk</skos:prefLabel>
		<skos:definition>Determinism qualifying the law in a State where the legal order is not established by convention (Source: Legal Dictionary of Property in Canada - Dualjuridik).</skos:definition>
		<skos:changeNote>Established with version 3.</skos:changeNote>
		<skos:exactMatch rdf:resource="http://zbw.eu/stw/descriptor/15965-3"/>
		<skos:exactMatch rdf:resource="http://eurovoc.europa.eu/7399"/>
		<skos:inScheme rdf:resource="https://www.opengis.net/def/CaLAThe/5.0"/>
		<skos:broader rdf:resource="https://www.opengis.net/def/CaLAThe/5.0/Law"/>
	</skos:Concept>
	<skos:Concept rdf:about="https://www.opengis.net/def/CaLAThe/5.0/NaturalPerson">
		<skos:prefLabel xml:lang="en">Natural person</skos:prefLabel>
		<skos:prefLabel xml:lang="da">Fysisk person</skos:prefLabel>
		<skos:prefLabel xml:lang="tr">Gerçek kişi</skos:prefLabel>
		<skos:changeNote>Established with version 1. Narrower to Legal subject deleted with ver. 5; replaced by Legal personality.</skos:changeNote>
		<skos:exactMatch rdf:resource="http://eurovoc.europa.eu/2338"/>
		<skos:inScheme rdf:resource="https://www.opengis.net/def/CaLAThe/5.0"/>
		<skos:broader rdf:resource="https://www.opengis.net/def/CaLAThe/5.0/PartyType"/>
	</skos:Concept>
	<skos:Concept rdf:about="https://www.opengis.net/def/CaLAThe/5.0/NaturalPersonRole">
		<skos:prefLabel xml:lang="en">Natural person role</skos:prefLabel>
		<skos:prefLabel xml:lang="da">Rolle for fysisk person</skos:prefLabel>
		<skos:prefLabel xml:lang="tr">Gerçek kişi rolü</skos:prefLabel>
		<skos:changeNote>Established with version 1.</skos:changeNote>
		<skos:inScheme rdf:resource="https://www.opengis.net/def/CaLAThe/5.0"/>
		<skos:broader rdf:resource="https://www.opengis.net/def/CaLAThe/5.0/PartyRoleType"/>
		<skos:narrower rdf:resource="https://www.opengis.net/def/CaLAThe/5.0/OfficialRole"/>
		<skos:narrower rdf:resource="https://www.opengis.net/def/CaLAThe/5.0/SocietalRole"/>
		<skos:narrower rdf:resource="https://www.opengis.net/def/CaLAThe/5.0/Professional"/>
		<skos:narrower rdf:resource="https://www.opengis.net/def/CaLAThe/5.0/LegalPersonality"/>
	</skos:Concept>
	<skos:Concept rdf:about="https://www.opengis.net/def/CaLAThe/5.0/Neighbor">
		<skos:prefLabel xml:lang="en">Neighbor</skos:prefLabel>
		<skos:prefLabel xml:lang="da">Nabo</skos:prefLabel>
		<skos:prefLabel xml:lang="tr">Komşu</skos:prefLabel>
		<skos:changeNote>Established with version 4. Context changed with ver. 5 (no relation to Signatory)</skos:changeNote>
		<skos:inScheme rdf:resource="https://www.opengis.net/def/CaLAThe/5.0"/>
		<skos:broader rdf:resource="https://www.opengis.net/def/CaLAThe/5.0/SocietalRole"/>
	</skos:Concept>
	<skos:Concept rdf:about="https://www.opengis.net/def/CaLAThe/5.0/Node">
		<skos:prefLabel xml:lang="en">Node</skos:prefLabel>
		<skos:prefLabel xml:lang="da">Knude</skos:prefLabel>
		<skos:prefLabel xml:lang="tr">Düğüm noktası</skos:prefLabel>
		<skos:scopeNote>ISO LADM term</skos:scopeNote>
		<skos:changeNote>Established with version 1. Edited with version 4</skos:changeNote>
		<skos:exactMatch rdf:resource="https://isotc211.geolexica.org/concepts/309/"/>
		<skos:exactMatch rdf:resource="http://aims.fao.org/aos/agrovoc/c_5204"/>
		<skos:inScheme rdf:resource="https://www.opengis.net/def/CaLAThe/5.0"/>
		<skos:broader rdf:resource="https://www.opengis.net/def/CaLAThe/5.0/TopologicalPrimitive"/>
		<skos:narrower rdf:resource="https://www.opengis.net/def/CaLAThe/5.0/LA_NodeBasedSpatialUnit"/>
	</skos:Concept>
	<skos:Concept rdf:about="https://www.opengis.net/def/CaLAThe/5.0/Notary">
		<skos:prefLabel xml:lang="en">Notary</skos:prefLabel>
		<skos:prefLabel xml:lang="da">Notar</skos:prefLabel>
		<skos:prefLabel xml:lang="tr">Noter</skos:prefLabel>
		<skos:changeNote>Established with version 1.</skos:changeNote>
		<skos:exactMatch rdf:resource="http://aims.fao.org/aos/agrovoc/c_72efbdb8"/>
		<skos:exactMatch rdf:resource="http://eurovoc.europa.eu/2085"/>
		<skos:inScheme rdf:resource="https://www.opengis.net/def/CaLAThe/5.0"/>
		<skos:broader rdf:resource="https://www.opengis.net/def/CaLAThe/5.0/Professional"/>
	</skos:Concept>
	<skos:Concept rdf:about="https://www.opengis.net/def/CaLAThe/5.0/NUTSRegion">
		<skos:prefLabel xml:lang="en">NUTS Region</skos:prefLabel>
		<skos:prefLabel xml:lang="da">Regional statistikenhed</skos:prefLabel>
		<skos:prefLabel xml:lang="tr">İstatistiki Bölge Birimleri</skos:prefLabel>
		<skos:scopeNote>INSPIRE term</skos:scopeNote>
		<skos:definition>Territorial unit for statistics defined in the framework of the Regulation (EC) No 1059/2003 of the European Parliament and of the Council of 26 May 2003 (INSPIRE feature concept dictionary).</skos:definition>
		<skos:changeNote>Established with version 2.</skos:changeNote>
		<skos:exactMatch rdf:resource="http://inspire.ec.europa.eu/featureconcept/NUTSRegion"/>
		<skos:inScheme rdf:resource="https://www.opengis.net/def/CaLAThe/5.0"/>
		<skos:broader rdf:resource="https://www.opengis.net/def/CaLAThe/5.0/AdministrativeUnit"/>
	</skos:Concept>
	<skos:Concept rdf:about="https://www.opengis.net/def/CaLAThe/5.0/Observation">
		<skos:prefLabel xml:lang="en">Observation</skos:prefLabel>
		<skos:prefLabel xml:lang="da">Observation</skos:prefLabel>
		<skos:prefLabel xml:lang="tr">Gözlem</skos:prefLabel>
		<skos:scopeNote>OGC LandInfra / InfraGML term</skos:scopeNote>
		<skos:changeNote>Established with version 4</skos:changeNote>
		<skos:exactMatch rdf:resource="http://aims.fao.org/aos/agrovoc/c_fc54b25b"/>
		<skos:exactMatch rdf:resource="http://eurovoc.europa.eu/2085"/>
		<skos:inScheme rdf:resource="https://www.opengis.net/def/CaLAThe/5.0"/>
		<skos:broader rdf:resource="https://www.opengis.net/def/CaLAThe/5.0/SurveyingInstrument"/>
		<skos:narrower rdf:resource="https://www.opengis.net/def/CaLAThe/5.0/DistanceObservation"/>
		<skos:narrower rdf:resource="https://www.opengis.net/def/CaLAThe/5.0/AngelObservation"/>
		<skos:narrower rdf:resource="https://www.opengis.net/def/CaLAThe/5.0/TPSobservation"/>
		<skos:narrower rdf:resource="https://www.opengis.net/def/CaLAThe/5.0/LevelObservation"/>
		<skos:narrower rdf:resource="https://www.opengis.net/def/CaLAThe/5.0/GNSSobservation"/>
		<skos:narrower rdf:resource="https://www.opengis.net/def/CaLAThe/5.0/Correction"/>
	</skos:Concept>
	<skos:Concept rdf:about="https://www.opengis.net/def/CaLAThe/5.0/OfficialRole">
		<skos:prefLabel xml:lang="en">Official role</skos:prefLabel>
		<skos:prefLabel xml:lang="da">Embedsmand</skos:prefLabel>
		<skos:prefLabel xml:lang="tr">Resmi rol</skos:prefLabel>
		<skos:changeNote>Established with version 1. Alternative label with version 3. Removed with version 4</skos:changeNote>
		<skos:inScheme rdf:resource="https://www.opengis.net/def/CaLAThe/5.0"/>
		<skos:broader rdf:resource="https://www.opengis.net/def/CaLAThe/5.0/NaturalPersonRole"/>
		<skos:narrower rdf:resource="https://www.opengis.net/def/CaLAThe/5.0/Registrar"/>
	</skos:Concept>
	<skos:Concept rdf:about="https://www.opengis.net/def/CaLAThe/5.0/OptionToPurchase">
		<skos:prefLabel xml:lang="en">Option to purchase</skos:prefLabel>
		<skos:prefLabel xml:lang="da">Køberet</skos:prefLabel>
		<skos:prefLabel xml:lang="tr">Alım hakkı</skos:prefLabel>
		<skos:scopeNote>EULIS / ELRA term.</skos:scopeNote>
		<skos:definition>A right that entitles a person to compel the owner to sell or grant the property, but does not impose on him any duty to buy (EULIS / ELRA glossary).</skos:definition>
		<skos:changeNote>Established with version 3.</skos:changeNote>
		<skos:inScheme rdf:resource="https://www.opengis.net/def/CaLAThe/5.0"/>
		<skos:broader rdf:resource="https://www.opengis.net/def/CaLAThe/5.0/LawOfObligation"/>
	</skos:Concept>
	<skos:Concept rdf:about="https://www.opengis.net/def/CaLAThe/5.0/OrdinalReferenceFrame">
		<skos:prefLabel xml:lang="en">Ordinal reference frame</skos:prefLabel>
		<skos:prefLabel xml:lang="da">Ordinal referenceramme</skos:prefLabel>
		<skos:prefLabel xml:lang="tr">Sıralı referans çatkısı</skos:prefLabel>
		<skos:changeNote>Established with version 1.</skos:changeNote>
		<skos:inScheme rdf:resource="https://www.opengis.net/def/CaLAThe/5.0"/>
		<skos:broader rdf:resource="https://www.opengis.net/def/CaLAThe/5.0/SpatialReference"/>
	</skos:Concept>
	<skos:Concept rdf:about="https://www.opengis.net/def/CaLAThe/5.0/Organisation">
		<skos:prefLabel xml:lang="en">Organisation</skos:prefLabel>
		<skos:prefLabel xml:lang="da">Organisation</skos:prefLabel>
		<skos:prefLabel xml:lang="tr">Kuruluş</skos:prefLabel>
		<skos:scopeNote>GEMET term</skos:scopeNote>
		<skos:definition>Term used in commercial law, including a corporation, government or governmental subdivision or agency, business trust, estate, trust, partnership or association, two or more persons having a joint or common interest, or any other legal or commercial entity (Source: Black, 1991). A collection of people organized together into a community or other social, commercial or political structure. The group has some common purpose or reason for existence which goes beyond the set of people belonging to it and can act as an Agent. Organizations are often decomposable into hierarchical structures (Source: W3C Organization Ontology).</skos:definition>
		<skos:changeNote>Established with version 1. Relation to Legal person added in version 3 and edited to Narrower in version44. Definition supplemented in version 4.</skos:changeNote>
		<skos:exactMatch rdf:resource="http://aims.fao.org/aos/agrovoc/c_37968"/>
		<skos:exactMatch rdf:resource="http://www.eionet.europa.eu/gemet/concept/13286"/>
		<skos:exactMatch rdf:resource="http://zbw.eu/stw/descriptor/12091-4"/>
		<skos:inScheme rdf:resource="https://www.opengis.net/def/CaLAThe/5.0"/>
		<skos:broader rdf:resource="https://www.opengis.net/def/CaLAThe/5.0/PartyType"/>
		<skos:narrower rdf:resource="https://www.opengis.net/def/CaLAThe/5.0/GovernmentalOrganisation"/>
		<skos:narrower rdf:resource="https://www.opengis.net/def/CaLAThe/5.0/Judiciary"/>
		<skos:narrower rdf:resource="https://www.opengis.net/def/CaLAThe/5.0/Corporation"/>
		<skos:narrower rdf:resource="https://www.opengis.net/def/CaLAThe/5.0/Association"/>
		<skos:narrower rdf:resource="https://www.opengis.net/def/CaLAThe/5.0/LegalPerson"/>
	</skos:Concept>
	<skos:Concept rdf:about="https://www.opengis.net/def/CaLAThe/5.0/Orthoimagery">
		<skos:prefLabel xml:lang="en">Orthoimagery</skos:prefLabel>
		<skos:prefLabel xml:lang="da">Ortofoto</skos:prefLabel>
		<skos:prefLabel xml:lang="tr">Ortogörüntü</skos:prefLabel>
		<skos:scopeNote>INSPIRE term</skos:scopeNote>
		<skos:changeNote>Established with version 1.</skos:changeNote>
		<skos:exactMatch rdf:resource="http://aims.fao.org/aos/agrovoc/c_2f78f962"/>
		<skos:inScheme rdf:resource="https://www.opengis.net/def/CaLAThe/5.0"/>
		<skos:broader rdf:resource="https://www.opengis.net/def/CaLAThe/5.0/DigitalImagery"/>
	</skos:Concept>
	<skos:Concept rdf:about="https://www.opengis.net/def/CaLAThe/5.0/Owner">
		<skos:prefLabel xml:lang="en">Owner</skos:prefLabel>
		<skos:prefLabel xml:lang="da">Ejer</skos:prefLabel>
		<skos:prefLabel xml:lang="tr">Malik; Sahip</skos:prefLabel>
		<skos:scopeNote>STW Thesaurus for Economics term</skos:scopeNote>
		<skos:definition>Subject of ownership and holder of the prerogatives that are attached to it (Source: Legal Dictionary of Property in Canada - Dualjuridik).</skos:definition>
		<skos:changeNote>Established with version 1. Definition added with version 3.</skos:changeNote>
		<skos:exactMatch rdf:resource="http://zbw.eu/stw/descriptor/19161-2"/>
		<skos:exactMatch rdf:resource="http://data.europa.eu/snb/verification/1faf8d450f"/>
		<skos:exactMatch rdf:resource="https://isotc211.geolexica.org/concepts/1241/"/>
		<skos:inScheme rdf:resource="https://www.opengis.net/def/CaLAThe/5.0"/>
		<skos:broader rdf:resource="https://www.opengis.net/def/CaLAThe/5.0/RightsHolder"/>
		<skos:broader rdf:resource="https://www.opengis.net/def/CaLAThe/5.0/Signatory"/>
		<skos:narrower rdf:resource="https://www.opengis.net/def/CaLAThe/5.0/Title"/>
	</skos:Concept>
	<skos:Concept rdf:about="https://www.opengis.net/def/CaLAThe/5.0/Ownership">
		<skos:prefLabel xml:lang="en">Ownership</skos:prefLabel>
		<skos:prefLabel xml:lang="da">Ejendomsret (til fast ejendom)</skos:prefLabel>
		<skos:prefLabel xml:lang="tr">Mülkiyet</skos:prefLabel>
		<skos:scopeNote>GEMET term</skos:scopeNote>
		<skos:definition>Collection of rights to use and enjoy property, including right to transmit it to others. The complete dominion, title, or proprietary right in a thing or claim (Source: Black, 1991). Possessive relationship with a title established between an owner and their property (Source: Legal Dictionary of Property in Canada - Dualjuridik).  Includes the right to grant a lease, an easement, or a security interest and other lesser rights. Ownership in land includes buildings and fixture on the land parcel, unless lawful process is performed in terms of establishment of condominium units  (Source: OGC LandInfra, 4.8.13)</skos:definition>
		<skos:changeNote>Established with version 1. Changed and defined with version 3.</skos:changeNote>
		<skos:exactMatch rdf:resource="http://aims.fao.org/aos/agrovoc/c_5466"/>
		<skos:exactMatch rdf:resource="https://www.eionet.europa.eu/gemet/en/concept/5971"/>
		<skos:exactMatch rdf:resource="http://zbw.eu/stw/descriptor/10005-5"/>
		<skos:exactMatch rdf:resource="http://eurovoc.europa.eu/3929"/>
		<skos:inScheme rdf:resource="https://www.opengis.net/def/CaLAThe/5.0"/>
		<skos:altLabel>Freehold</skos:altLabel>
		<skos:altLabel>Private ownership</skos:altLabel>
		<skos:broader rdf:resource="https://www.opengis.net/def/CaLAThe/5.0/RealRight"/>
		<skos:narrower rdf:resource="https://www.opengis.net/def/CaLAThe/5.0/IndividualOwnership"/>
		<skos:narrower rdf:resource="https://www.opengis.net/def/CaLAThe/5.0/PublicOwnership"/>
		<skos:narrower rdf:resource="https://www.opengis.net/def/CaLAThe/5.0/CoOwnership"/>
		<skos:narrower rdf:resource="https://www.opengis.net/def/CaLAThe/5.0/AdversePossession"/>
	</skos:Concept>
	<skos:Concept rdf:about="https://www.opengis.net/def/CaLAThe/5.0/ParcelAcquisition">
		<skos:prefLabel xml:lang="en">Parcel acquisition</skos:prefLabel>
		<skos:prefLabel xml:lang="da">Erhvervelse af del af fast eje</skos:prefLabel>
		<skos:prefLabel xml:lang="tr">Parsel edinimi</skos:prefLabel>
		<skos:scopeNote>OGC LandIfra / InfraGML term</skos:scopeNote>
		<skos:definition>Transfer of ownership to a LandParcel from the seller to the buyer (Source: OGC LandInfra, 7.10.4.1)</skos:definition>
		<skos:changeNote>Established with version 3.</skos:changeNote>
		<skos:inScheme rdf:resource="https://www.opengis.net/def/CaLAThe/5.0"/>
		<skos:broader rdf:resource="https://www.opengis.net/def/CaLAThe/5.0/Conveyance"/>
	</skos:Concept>
	<skos:Concept rdf:about="https://www.opengis.net/def/CaLAThe/5.0/ParcelEstablishment">
		<skos:prefLabel xml:lang="en">Parcel establishment</skos:prefLabel>
		<skos:prefLabel xml:lang="da">Matrikulering</skos:prefLabel>
		<skos:prefLabel xml:lang="tr">Parsel oluşturma</skos:prefLabel>
		<skos:scopeNote>OGC LandInfra / InfraGML term</skos:scopeNote>
		<skos:definition>The initial cadastral survey, or the creation of a new Cadastral parcel through change of existing parcels (Source: OGC 7.10.4.1).</skos:definition>
		<skos:changeNote>Established with version 3. Edited to refer to Property formation only in version 4</skos:changeNote>
		<skos:inScheme rdf:resource="https://www.opengis.net/def/CaLAThe/5.0"/>
		<skos:broader rdf:resource="https://www.opengis.net/def/CaLAThe/5.0/PropertyFormation"/>
	</skos:Concept>
	<skos:Concept rdf:about="https://www.opengis.net/def/CaLAThe/5.0/Partition">
		<skos:prefLabel xml:lang="en">Partition</skos:prefLabel>
		<skos:prefLabel xml:lang="da">Skifte, fraskillelse</skos:prefLabel>
		<skos:prefLabel xml:lang="tr">Taksim</skos:prefLabel>
		<skos:scopeNote>EULIS / ELRA term</skos:scopeNote>
		<skos:definition>Division of a register unit in specific proportions between the co-owners. (Source: EULIS / ELRA glossary).</skos:definition>
		<skos:changeNote>Established with version 3.</skos:changeNote>
		<skos:inScheme rdf:resource="https://www.opengis.net/def/CaLAThe/5.0"/>
		<skos:broader rdf:resource="https://www.opengis.net/def/CaLAThe/5.0/Transfer"/>
	</skos:Concept>
	<skos:Concept rdf:about="https://www.opengis.net/def/CaLAThe/5.0/Party">
		<skos:prefLabel xml:lang="en">Party</skos:prefLabel>
		<skos:prefLabel xml:lang="da">Aktør</skos:prefLabel>
		<skos:prefLabel xml:lang="tr">Taraf</skos:prefLabel>
		<skos:scopeNote>ISO LADM and OGC LandInfra / InfraGML term</skos:scopeNote>
		<skos:definition>A person or organization that plays a role in a lawful process.  Compares to ISO 19152:2012 4.1.13 party (OGC LandInfra, 4.1.15).</skos:definition>
		<skos:changeNote>Established with version 1.</skos:changeNote>
		<skos:exactMatch rdf:resource="https://isotc211.geolexica.org/concepts/1242/"/>
		<skos:inScheme rdf:resource="https://www.opengis.net/def/CaLAThe/5.0"/>
		<skos:topConceptOf rdf:resource="https://www.opengis.net/def/CaLAThe/5.0"/>
		<skos:altLabel>LA_Party</skos:altLabel>
		<skos:narrower rdf:resource="https://www.opengis.net/def/CaLAThe/5.0/PartyRoleType"/>
		<skos:narrower rdf:resource="https://www.opengis.net/def/CaLAThe/5.0/PartyType"/>
	</skos:Concept>
	<skos:Concept rdf:about="https://www.opengis.net/def/CaLAThe/5.0/PartyMember">
		<skos:prefLabel xml:lang="en">Party member</skos:prefLabel>
		<skos:prefLabel xml:lang="da">Gruppemedlem</skos:prefLabel>
		<skos:prefLabel xml:lang="tr">.</skos:prefLabel>
		<skos:scopeNote>ISO LADM term</skos:scopeNote>
		<skos:changeNote>Established with version 1.</skos:changeNote>
		<skos:exactMatch rdf:resource="https://isotc211.geolexica.org/concepts/1310/"/>
		<skos:inScheme rdf:resource="https://www.opengis.net/def/CaLAThe/5.0"/>
		<skos:altLabel>LA_PartyMember</skos:altLabel>
		<skos:broader rdf:resource="https://www.opengis.net/def/CaLAThe/5.0/RightsHolder"/>
		<skos:related rdf:resource="https://www.opengis.net/def/CaLAThe/5.0/PlaceBoundParty"/>
	</skos:Concept>
	<skos:Concept rdf:about="https://www.opengis.net/def/CaLAThe/5.0/PartyRoleType">
		<skos:prefLabel xml:lang="en">Party role type</skos:prefLabel>
		<skos:prefLabel xml:lang="da">Aktørrolle</skos:prefLabel>
		<skos:prefLabel xml:lang="tr">Taraf rolü</skos:prefLabel>
		<skos:scopeNote>ISO LADM term</skos:scopeNote>
		<skos:changeNote>Established with version 1.</skos:changeNote>
		<skos:inScheme rdf:resource="https://www.opengis.net/def/CaLAThe/5.0"/>
		<skos:broader rdf:resource="https://www.opengis.net/def/CaLAThe/5.0/Party"/>
		<skos:broader rdf:resource="https://www.opengis.net/def/CaLAThe/5.0/Law"/>
		<skos:narrower rdf:resource="https://www.opengis.net/def/CaLAThe/5.0/RightsHolder"/>
		<skos:narrower rdf:resource="https://www.opengis.net/def/CaLAThe/5.0/NaturalPersonRole"/>
	</skos:Concept>
	<skos:Concept rdf:about="https://www.opengis.net/def/CaLAThe/5.0/PartyShare">
		<skos:prefLabel xml:lang="en">Party share</skos:prefLabel>
		<skos:prefLabel xml:lang="da">Andel</skos:prefLabel>
		<skos:prefLabel xml:lang="tr">Pay</skos:prefLabel>
		<skos:changeNote>Established with version 1 and specified as narrower of Co-ownership share in version 3.</skos:changeNote>
		<skos:inScheme rdf:resource="https://www.opengis.net/def/CaLAThe/5.0"/>
		<skos:broader rdf:resource="https://www.opengis.net/def/CaLAThe/5.0/CoOwnershipShare"/>
		<skos:related rdf:resource="https://www.opengis.net/def/CaLAThe/5.0/PartyMember"/>
	</skos:Concept>
	<skos:Concept rdf:about="https://www.opengis.net/def/CaLAThe/5.0/PartyType">
		<skos:prefLabel xml:lang="en">Party type</skos:prefLabel>
		<skos:prefLabel xml:lang="da">Aktørtype</skos:prefLabel>
		<skos:prefLabel xml:lang="tr">Taraf türü</skos:prefLabel>
		<skos:scopeNote>ISO LADM term</skos:scopeNote>
		<skos:changeNote>Established with version 1.0</skos:changeNote>
		<skos:inScheme rdf:resource="https://www.opengis.net/def/CaLAThe/5.0"/>
		<skos:broader rdf:resource="https://www.opengis.net/def/CaLAThe/5.0/Party"/>
		<skos:narrower rdf:resource="https://www.opengis.net/def/CaLAThe/5.0/NaturalPerson"/>
		<skos:narrower rdf:resource="https://www.opengis.net/def/CaLAThe/5.0/GroupParty"/>
		<skos:narrower rdf:resource="https://www.opengis.net/def/CaLAThe/5.0/Organisation"/>
	</skos:Concept>
	<skos:Concept rdf:about="https://www.opengis.net/def/CaLAThe/5.0/PlaceBoundParty">
		<skos:prefLabel xml:lang="en">Place bound party</skos:prefLabel>
		<skos:prefLabel xml:lang="da">Stedbestemt gruppe</skos:prefLabel>
		<skos:prefLabel xml:lang="tr">.</skos:prefLabel>
		<skos:changeNote>Established with version 1.0</skos:changeNote>
		<skos:inScheme rdf:resource="https://www.opengis.net/def/CaLAThe/5.0"/>
		<skos:broader rdf:resource="https://www.opengis.net/def/CaLAThe/5.0/GroupParty"/>
		<skos:related rdf:resource="https://www.opengis.net/def/CaLAThe/5.0/PartyMember"/>
	</skos:Concept>
	<skos:Concept rdf:about="https://www.opengis.net/def/CaLAThe/5.0/PlaceName">
		<skos:prefLabel xml:lang="en">Place name</skos:prefLabel>
		<skos:prefLabel xml:lang="da">Stednavn</skos:prefLabel>
		<skos:prefLabel xml:lang="tr">Yer adı</skos:prefLabel>
		<skos:definition>One or several proper nouns used to identify a real world entity.</skos:definition>
		<skos:changeNote>Established with version 2. Definition added with version 4</skos:changeNote>
		<skos:inScheme rdf:resource="https://www.opengis.net/def/CaLAThe/5.0"/>
		<skos:altLabel>Geographical name</skos:altLabel>
		<skos:broader rdf:resource="https://www.opengis.net/def/CaLAThe/5.0/Gazetteer"/>
		<skos:broader rdf:resource="https://www.opengis.net/def/CaLAThe/5.0/LandDivision"/>
		<skos:broader rdf:resource="https://www.opengis.net/def/CaLAThe/5.0/GeolocatedInformation"/>
		<skos:narrower rdf:resource="https://www.opengis.net/def/CaLAThe/5.0/PostalAddress"/>
	</skos:Concept>
	<skos:Concept rdf:about="https://www.opengis.net/def/CaLAThe/5.0/PlanningLaw">
		<skos:prefLabel xml:lang="en">Planning law</skos:prefLabel>
		<skos:prefLabel xml:lang="da">Arealplanlægning</skos:prefLabel>
		<skos:prefLabel xml:lang="tr">Planlama hukuku</skos:prefLabel>
		<skos:scopeNote>GEMET term</skos:scopeNote>
		<skos:definition>A binding rule or body of rules prescribed by a government to organize, designate and regulate land use within its domain through zoning laws, subdivision regulations, rent and sign controls, growth management and other measures designed to protect human health and ecological integrity (Source: GEMET)</skos:definition>
		<skos:changeNote>Established with version 1.0. Broader relation changed from Property law to Land law with version 3.</skos:changeNote>
		<skos:inScheme rdf:resource="https://www.opengis.net/def/CaLAThe/5.0"/>
		<skos:broader rdf:resource="https://www.opengis.net/def/CaLAThe/5.0/LandLaw"/>
		<skos:narrower rdf:resource="https://www.opengis.net/def/CaLAThe/5.0/PublicLawRestriction"/>
	</skos:Concept>
	<skos:Concept rdf:about="https://www.opengis.net/def/CaLAThe/5.0/Point">
		<skos:prefLabel xml:lang="en">Point</skos:prefLabel>
		<skos:prefLabel xml:lang="da">Punkt</skos:prefLabel>
		<skos:prefLabel xml:lang="tr">Nokta</skos:prefLabel>
		<skos:scopeNote>Geolexica term</skos:scopeNote>
		<skos:definition>0-dimensional geometric primitive, representing a position (Geolexica, ISO 19107:2003)</skos:definition>
		<skos:changeNote>Established with version 4</skos:changeNote>
		<skos:exactMatch rdf:resource="https://isotc211.geolexica.org/concepts/336/"/>
		<skos:inScheme rdf:resource="https://www.opengis.net/def/CaLAThe/5.0"/>
		<skos:broader rdf:resource="https://www.opengis.net/def/CaLAThe/5.0/GeometricPrimitive"/>
		<skos:broader rdf:resource="https://www.opengis.net/def/CaLAThe/5.0/LineString"/>
	</skos:Concept>
	<skos:Concept rdf:about="https://www.opengis.net/def/CaLAThe/5.0/PointCloud">
		<skos:prefLabel xml:lang="en">Point cloud</skos:prefLabel>
		<skos:prefLabel xml:lang="da">Punktsky</skos:prefLabel>
		<skos:prefLabel xml:lang="tr">Nokta bulutu</skos:prefLabel>
		<skos:scopeNote>OGC LandInfra / InfraGML term</skos:scopeNote>
		<skos:definition>PointCloud is the result of a PointCloudObservation (OGC LandInfra 7.8.7.9)</skos:definition>
		<skos:changeNote>Established with version 4</skos:changeNote>
		<skos:exactMatch rdf:resource="https://isotc211.geolexica.org/concepts/1408/"/>
		<skos:inScheme rdf:resource="https://www.opengis.net/def/CaLAThe/5.0"/>
		<skos:broader rdf:resource="https://www.opengis.net/def/CaLAThe/5.0/TerrestrialLaserScanner"/>
		<skos:broader rdf:resource="https://www.opengis.net/def/CaLAThe/5.0/SurveyResult"/>
	</skos:Concept>
	<skos:Concept rdf:about="https://www.opengis.net/def/CaLAThe/5.0/Polygon">
		<skos:prefLabel xml:lang="en">Polygon</skos:prefLabel>
		<skos:prefLabel xml:lang="da">Polygon</skos:prefLabel>
		<skos:prefLabel xml:lang="tr">Poligon; Çoklu doğru</skos:prefLabel>
		<skos:scopeNote>Geolexica term</skos:scopeNote>
		<skos:definition>Planar surface defined by 1 exterior boundary and 0 or more interior boundaries (Geolexica, ISO 19136:2007)</skos:definition>
		<skos:changeNote>Established with version 4</skos:changeNote>
		<skos:exactMatch rdf:resource="https://isotc211.geolexica.org/concepts/695/"/>
		<skos:inScheme rdf:resource="https://www.opengis.net/def/CaLAThe/5.0"/>
		<skos:broader rdf:resource="https://www.opengis.net/def/CaLAThe/5.0/Surface"/>
		<skos:narrower rdf:resource="https://www.opengis.net/def/CaLAThe/5.0/Curve"/>
	</skos:Concept>
	<skos:Concept rdf:about="https://www.opengis.net/def/CaLAThe/5.0/PositiveLaw">
		<skos:prefLabel xml:lang="en">Positive law</skos:prefLabel>
		<skos:prefLabel xml:lang="da">Positiv ret</skos:prefLabel>
		<skos:prefLabel xml:lang="tr">Pozitif hukuk</skos:prefLabel>
		<skos:definition>Conventional legal order prevailing in a State and expressing itself through statutes and jurisprudence (Source: Legal Dictionary of Property in Canada - Dualjuridik).</skos:definition>
		<skos:changeNote>Established with version 3.</skos:changeNote>
		<skos:inScheme rdf:resource="https://www.opengis.net/def/CaLAThe/5.0"/>
		<skos:altLabel>Legal basis</skos:altLabel>
		<skos:altLabel>Formal right</skos:altLabel>
		<skos:broader rdf:resource="https://www.opengis.net/def/CaLAThe/5.0/Law"/>
		<skos:narrower rdf:resource="https://www.opengis.net/def/CaLAThe/5.0/LandLaw"/>
	</skos:Concept>
	<skos:Concept rdf:about="https://www.opengis.net/def/CaLAThe/5.0/PostalAddress">
		<skos:prefLabel xml:lang="en">Postal address</skos:prefLabel>
		<skos:prefLabel xml:lang="da">Postadresse</skos:prefLabel>
		<skos:prefLabel xml:lang="tr">Posta adresi</skos:prefLabel>
		<skos:scopeNote>INSPIRE term</skos:scopeNote>
		<skos:definition>Set of information which, for a postal item, allows the unambiguous determination of an actual or potential delivery point, usually combined with the specification of an addressee and/or mailee. (INSPIRE Source: Universal Postal Union 2006).  Structured information that allows the unambiguous determination of an [real world] object for purposes of identification and location (Geolexica)</skos:definition>
		<skos:changeNote>Established with version 1. Edited in version 3 as Postal address to comply with INPSIRE specifications. Definitions edited with version 4</skos:changeNote>
		<skos:exactMatch rdf:resource="http://inspire.ec.europa.eu/glossary/PostalAddress"/>
		<skos:exactMatch rdf:resource="http://publications.europa.eu/resource/authority/address-type/ADR_POSTAL"/>
	 	<skos:exactMatch rdf:resource="https://isotc211.geolexica.org/concepts/2117/"/>
		<skos:inScheme rdf:resource="https://www.opengis.net/def/CaLAThe/5.0"/>
		<skos:altLabel>Address</skos:altLabel>
		<skos:broader rdf:resource="https://www.opengis.net/def/CaLAThe/5.0/PlaceName"/>
		<skos:broader rdf:resource="https://www.opengis.net/def/CaLAThe/5.0/RoadNetwork"/>
		<skos:narrower rdf:resource="https://www.opengis.net/def/CaLAThe/5.0/StreetSign"/>
	</skos:Concept>
	<skos:Concept rdf:about="https://www.opengis.net/def/CaLAThe/5.0/PreemptionRight">
		<skos:prefLabel xml:lang="en">Pre-emption right</skos:prefLabel>
		<skos:prefLabel xml:lang="da">Forkøbsret</skos:prefLabel>
		<skos:prefLabel xml:lang="tr">Ön alım hakkı</skos:prefLabel>
		<skos:definition>The owner of land has contracted that if he decides to sell the land he first will offer it to the other contracting party.</skos:definition>
		<skos:exactMatch rdf:resource="http://aims.fao.org/aos/agrovoc/c_9c081fdc"/>
		<skos:exactMatch rdf:resource="https://www.eionet.europa.eu/gemet/en/concept/11623"/>
		<skos:exactMatch rdf:resource="http://eurovoc.europa.eu/546"/>
		<skos:inScheme rdf:resource="https://www.opengis.net/def/CaLAThe/5.0"/>
		<skos:broader rdf:resource="https://www.opengis.net/def/CaLAThe/5.0/LawOfObligation"/>
	</skos:Concept>
	<skos:Concept rdf:about="https://www.opengis.net/def/CaLAThe/5.0/PrivateLawRestriction">
		<skos:prefLabel xml:lang="en">Private law restriction</skos:prefLabel>
		<skos:prefLabel xml:lang="da">Privatretlig regulering</skos:prefLabel>
		<skos:prefLabel xml:lang="tr">Özel hukuk kısıtlaması</skos:prefLabel>
		<skos:changeNote>Established with version 1.</skos:changeNote>
		<skos:inScheme rdf:resource="https://www.opengis.net/def/CaLAThe/5.0"/>
		<skos:broader rdf:resource="https://www.opengis.net/def/CaLAThe/5.0/Easement"/>
		<skos:narrower rdf:resource="https://www.opengis.net/def/CaLAThe/5.0/RightOfWay"/>
	</skos:Concept>
	<skos:Concept rdf:about="https://www.opengis.net/def/CaLAThe/5.0/Professional">
		<skos:prefLabel xml:lang="en">Professional</skos:prefLabel>
		<skos:prefLabel xml:lang="da">Professionel</skos:prefLabel>
		<skos:prefLabel xml:lang="tr">Profesyonel</skos:prefLabel>
		<skos:scopeNote>OGC LandInfra / InfraGML term</skos:scopeNote>
		<skos:definition>Person, generally with tertiary education, who through a license is bound to act according to the standards of a professional association.  Note 1 to entry: In common usage, the term professional includes a much broader scope of individuals.  Here, it only refers to those who are licensed, such as land surveyors (OGC LandInfra, 4.1.17)</skos:definition>
		<skos:changeNote>Established with version 3.</skos:changeNote>
		<skos:inScheme rdf:resource="https://www.opengis.net/def/CaLAThe/5.0"/>
		<skos:altLabel>Professional role</skos:altLabel>
		<skos:broader rdf:resource="https://www.opengis.net/def/CaLAThe/5.0/NaturalPersonRole"/>
		<skos:narrower rdf:resource="https://www.opengis.net/def/CaLAThe/5.0/Notary"/>
		<skos:narrower rdf:resource="https://www.opengis.net/def/CaLAThe/5.0/Surveyor"/>
		<skos:narrower rdf:resource="https://www.opengis.net/def/CaLAThe/5.0/Drafter"/>
		<skos:narrower rdf:resource="https://www.opengis.net/def/CaLAThe/5.0/Lawyer"/>
		<skos:narrower rdf:resource="https://www.opengis.net/def/CaLAThe/5.0/Engineer"/>
	</skos:Concept>
	<skos:Concept rdf:about="https://www.opengis.net/def/CaLAThe/5.0/ProfessionalSociety">
		<skos:prefLabel xml:lang="en">Professional society</skos:prefLabel>
		<skos:prefLabel xml:lang="da">Professionsforening</skos:prefLabel>
		<skos:prefLabel xml:lang="tr">Profesyonel cemiyet</skos:prefLabel>
		<skos:scopeNote>GEMET term</skos:scopeNote>
		<skos:definition>A group of persons engaged in the same profession, business, trade or craft that is organized or formally structured to attain common ends (Source: Random House, 1997).</skos:definition>
		<skos:changeNote>Established with version 3.</skos:changeNote>
		<skos:exactMatch rdf:resource="http://www.eionet.europa.eu/gemet/concept/14847"/>
		<skos:exactMatch rdf:resource="http://aims.fao.org/aos/agrovoc/c_50290"/>
		<skos:inScheme rdf:resource="https://www.opengis.net/def/CaLAThe/5.0"/>
		<skos:altLabel>Professional association</skos:altLabel>
		<skos:broader rdf:resource="https://www.opengis.net/def/CaLAThe/5.0/Association"/>
	</skos:Concept>
	<skos:Concept rdf:about="https://www.opengis.net/def/CaLAThe/5.0/PropertyEnquiryCertificate">
		<skos:prefLabel xml:lang="en">Property enquiry certificate</skos:prefLabel>
		<skos:scopeNote>esd-toolkit term</skos:scopeNote>
		<skos:definition>When a property is being sold a solicitor will carry out conveyancing duties which normally include a property search. The local authority can carry out these searches and provide a Property Enquiry Certificate detailing issues relating to Planning, Building Control, Environmental Health, Housing, Roads, etc (Source: esd-toolkit).</skos:definition>
		<skos:changeNote>Established with version 1.</skos:changeNote>
		<skos:exactMatch rdf:resource="http://id.esd-toolkit.eu/service/1060"/>
		<skos:inScheme rdf:resource="https://www.opengis.net/def/CaLAThe/5.0"/>
		<skos:broader rdf:resource="https://www.opengis.net/def/CaLAThe/5.0/Certificate"/>
	</skos:Concept>
	<skos:Concept rdf:about="https://www.opengis.net/def/CaLAThe/5.0/PropertyFormation">
		<skos:prefLabel xml:lang="en">Property formation</skos:prefLabel>
		<skos:prefLabel xml:lang="da">Ejendomsdannelse</skos:prefLabel>
		<skos:prefLabel xml:lang="tr">Taşınmaz oluşturma</skos:prefLabel>
		<skos:changeNote>Established with version 2.0. Related to ParcelEstablishment with version 3. ParcelEstablishment made narrower with version 4</skos:changeNote>
		<skos:inScheme rdf:resource="https://www.opengis.net/def/CaLAThe/5.0"/>
		<skos:altLabel>Cadastral activity</skos:altLabel>
		<skos:broader rdf:resource="https://www.opengis.net/def/CaLAThe/5.0/Activity"/>
		<skos:narrower rdf:resource="https://www.opengis.net/def/CaLAThe/5.0/ChangeOfPropertyUnitType"/>
		<skos:narrower rdf:resource="https://www.opengis.net/def/CaLAThe/5.0/TransferOfPartOfProperty"/>
		<skos:narrower rdf:resource="https://www.opengis.net/def/CaLAThe/5.0/Amalgamation"/>
		<skos:narrower rdf:resource="https://www.opengis.net/def/CaLAThe/5.0/Subdivision"/>
		<skos:narrower rdf:resource="https://www.opengis.net/def/CaLAThe/5.0/PropertyRestructuring"/>
		<skos:narrower rdf:resource="https://www.opengis.net/def/CaLAThe/5.0/SuperficieObjectEstablishment"/>
		<skos:narrower rdf:resource="https://www.opengis.net/def/CaLAThe/5.0/ParcelEstablishment"/>
	</skos:Concept>
	<skos:Concept rdf:about="https://www.opengis.net/def/CaLAThe/5.0/PropertyRestructuring">
		<skos:prefLabel xml:lang="en">Property restructuring</skos:prefLabel>
		<skos:prefLabel xml:lang="da">Områdevis ejendomsændring</skos:prefLabel>
		<skos:prefLabel xml:lang="tr">.</skos:prefLabel>
		<skos:changeNote>Established with version 2.0.</skos:changeNote>
		<skos:inScheme rdf:resource="https://www.opengis.net/def/CaLAThe/5.0"/>
		<skos:broader rdf:resource="https://www.opengis.net/def/CaLAThe/5.0/PropertyFormation"/>
		<skos:narrower rdf:resource="https://www.opengis.net/def/CaLAThe/5.0/LandConsolidation"/>
		<skos:narrower rdf:resource="https://www.opengis.net/def/CaLAThe/5.0/LandReadjustment"/>
		<skos:narrower rdf:resource="https://www.opengis.net/def/CaLAThe/5.0/Expropriation"/>
	</skos:Concept>
	<skos:Concept rdf:about="https://www.opengis.net/def/CaLAThe/5.0/PropertyUnitType">
		<skos:prefLabel xml:lang="en">Property unit type</skos:prefLabel>
		<skos:prefLabel xml:lang="da">Ejendomstype</skos:prefLabel>
		<skos:prefLabel xml:lang="tr">Taşınmaz cinsi</skos:prefLabel>
		<skos:definition>Code list of admitted property unit types within a jurisdiction (Adopted from LA_BAUnitType).</skos:definition>
		<skos:changeNote>Established with version 1. Definition is added in version 5.</skos:changeNote>
		<skos:inScheme rdf:resource="https://www.opengis.net/def/CaLAThe/5.0"/>
		<skos:broader rdf:resource="https://www.opengis.net/def/CaLAThe/5.0/RealProperty"/>
	</skos:Concept>
	<skos:Concept rdf:about="https://www.opengis.net/def/CaLAThe/5.0/ProtectedSite">
		<skos:prefLabel xml:lang="en">Protected site</skos:prefLabel>
		<skos:prefLabel xml:lang="da">Beskyttet lokalitet</skos:prefLabel>
		<skos:prefLabel xml:lang="tr">Korunan alan</skos:prefLabel>
		<skos:scopeNote>INSPIRE term</skos:scopeNote>
		<skos:definition>An area designated or managed according to jurisdiction legislation to achieve specific conservation objectives (Adopted from INSPIRE, http://inspire.ec.europa.eu/featureconcept/ProtectedSite).</skos:definition>
		<skos:changeNote>Established with version 2. Definition is added in version 5.</skos:changeNote>
		<skos:exactMatch rdf:resource="http://inspire.ec.europa.eu/glossary/ProtectedSite"/>
		<skos:exactMatch rdf:resource="http://aims.fao.org/aos/agrovoc/c_37952"/>
		<skos:exactMatch rdf:resource="https://www.eionet.europa.eu/gemet/en/concept/6740"/>
		<skos:exactMatch rdf:resource="http://zbw.eu/stw/descriptor/19628-1"/>
		<skos:exactMatch rdf:resource="http://eurovoc.europa.eu/4801"/>
		<skos:inScheme rdf:resource="https://www.opengis.net/def/CaLAThe/5.0"/>
		<skos:broader rdf:resource="https://www.opengis.net/def/CaLAThe/5.0/AdministrativeUnit"/>
	</skos:Concept>
	<skos:Concept rdf:about="https://www.opengis.net/def/CaLAThe/5.0/PublicLawRestriction">
		<skos:prefLabel xml:lang="en">Public law restriction</skos:prefLabel>
		<skos:prefLabel xml:lang="da">Offentligretlig regulering</skos:prefLabel>
		<skos:prefLabel xml:lang="tr">Kamu hukuku kısıtlaması</skos:prefLabel>
		<skos:changeNote>Established with version 1.</skos:changeNote>
		<skos:inScheme rdf:resource="https://www.opengis.net/def/CaLAThe/5.0"/>
		<skos:broader rdf:resource="https://www.opengis.net/def/CaLAThe/5.0/Easement"/>
		<skos:broader rdf:resource="https://www.opengis.net/def/CaLAThe/5.0/PlanningLaw"/>
		<skos:narrower rdf:resource="https://www.opengis.net/def/CaLAThe/5.0/RightOfWay"/>
	</skos:Concept>
	<skos:Concept rdf:about="https://www.opengis.net/def/CaLAThe/5.0/PublicOwnership">
		<skos:prefLabel xml:lang="en">Public ownership</skos:prefLabel>
		<skos:prefLabel xml:lang="da">Offentlig ejendom</skos:prefLabel>
		<skos:prefLabel xml:lang="tr">Kamu mülkiyeti</skos:prefLabel>
		<skos:scopeNote>AGROVOC Multilingual Thesaurus term</skos:scopeNote>
		<skos:changeNote>Established with version 1.</skos:changeNote>
		<skos:exactMatch rdf:resource="http://aims.fao.org/aos/agrovoc/c_6350"/>
		<skos:exactMatch rdf:resource="http://eurovoc.europa.eu/2812"/>
		<skos:inScheme rdf:resource="https://www.opengis.net/def/CaLAThe/5.0"/>
		<skos:broader rdf:resource="https://www.opengis.net/def/CaLAThe/5.0/Ownership"/>
	</skos:Concept>
	<skos:Concept rdf:about="https://www.opengis.net/def/CaLAThe/5.0/RealProperty">
		<skos:prefLabel xml:lang="en">Real property</skos:prefLabel>
		<skos:prefLabel xml:lang="da">Bestemt fast ejendom</skos:prefLabel>
		<skos:prefLabel xml:lang="tr">Taşınmaz; Gayrimenkul</skos:prefLabel>
		<skos:definition>1. One or more Cadastral parcels, which are owned by the same party, and recorded as a unit according jurisdiction provisions, or 2. Condominium, or 3. Superficie object</skos:definition>
		<skos:changeNote>Established with version 1.0. Changed narrower from Building use part to Condominium with version 3. Definition is added in version 5, and the concept is renamed Real property, while the previous term Property unit is maintained as altLabel.</skos:changeNote>
		<skos:inScheme rdf:resource="https://www.opengis.net/def/CaLAThe/5.0"/>
		<skos:altLabel>Real estate</skos:altLabel>
		<skos:altLabel>Basic property unit</skos:altLabel>
		<skos:altLabel>Immovable property</skos:altLabel>
		<skos:altLabel>Property unit</skos:altLabel>
		<skos:broader rdf:resource="https://www.opengis.net/def/CaLAThe/5.0/LandDivision"/>
		<skos:narrower rdf:resource="https://www.opengis.net/def/CaLAThe/5.0/CadastralParcel"/>
		<skos:narrower rdf:resource="https://www.opengis.net/def/CaLAThe/5.0/PropertyUnitType"/>
		<skos:narrower rdf:resource="https://www.opengis.net/def/CaLAThe/5.0/Condominium"/>
		<skos:narrower rdf:resource="https://www.opengis.net/def/CaLAThe/5.0/SuperficieObject"/>
		<skos:narrower rdf:resource="https://www.opengis.net/def/CaLAThe/5.0/LA_BAUnit"/>
		<skos:narrower rdf:resource="https://www.opengis.net/def/CaLAThe/5.0/LA_RequiredRelationship"/>
	</skos:Concept>
	<skos:Concept rdf:about="https://www.opengis.net/def/CaLAThe/5.0/RealRight">
		<skos:prefLabel xml:lang="en">Real right</skos:prefLabel>
		<skos:prefLabel xml:lang="da">Ejendomsret</skos:prefLabel>
		<skos:prefLabel xml:lang="tr">Ayni hak</skos:prefLabel>
		<skos:scopeNote>EULIS / ELRA term</skos:scopeNote>
		<skos:definition>Prerogative that can be opposed to all, conferring a direct or indirect access to property. (Source: Dualjuridik). A right relating to land that is binding on third parties even if they are unaware of it. (ius in rem) (Source: EULIS / ELRA glossary)</skos:definition>
		<skos:changeNote>Established with version 1. Term changed and definitions added with version 3.</skos:changeNote>
		<skos:inScheme rdf:resource="https://www.opengis.net/def/CaLAThe/5.0"/>
		<skos:altLabel>Interest in land</skos:altLabel>
		<skos:altLabel>Estate</skos:altLabel>
		<skos:broader rdf:resource="https://www.opengis.net/def/CaLAThe/5.0/LandLaw"/>
		<skos:narrower rdf:resource="https://www.opengis.net/def/CaLAThe/5.0/Ownership"/>
		<skos:narrower rdf:resource="https://www.opengis.net/def/CaLAThe/5.0/Leasehold"/>
		<skos:narrower rdf:resource="https://www.opengis.net/def/CaLAThe/5.0/LimitedRight"/>
		<skos:narrower rdf:resource="https://www.opengis.net/def/CaLAThe/5.0/LA_Right"/>
	</skos:Concept>
	<skos:Concept rdf:about="https://www.opengis.net/def/CaLAThe/5.0/Reallotment">
		<skos:prefLabel xml:lang="en">Reallotment</skos:prefLabel>
		<skos:prefLabel xml:lang="da">Arealoverførsel</skos:prefLabel>
		<skos:prefLabel xml:lang="tr">Dağıtım; Tahsis</skos:prefLabel>
		<skos:inScheme rdf:resource="https://www.opengis.net/def/CaLAThe/5.0"/>
		<skos:broader rdf:resource="https://www.opengis.net/def/CaLAThe/5.0/LandConsolidation"/>
		<skos:broader rdf:resource="https://www.opengis.net/def/CaLAThe/5.0/LandReadjustment"/>
		<skos:broader rdf:resource="https://www.opengis.net/def/CaLAThe/5.0/TransferOfPartOfProperty"/>
	</skos:Concept>
	<skos:Concept rdf:about="https://www.opengis.net/def/CaLAThe/5.0/Registrar">
		<skos:prefLabel xml:lang="en">Registrar</skos:prefLabel>
		<skos:prefLabel xml:lang="da">Registrator</skos:prefLabel>
		<skos:prefLabel xml:lang="tr">Tapu sicil muhafızı</skos:prefLabel>
		<skos:changeNote>Established with version 1.</skos:changeNote>
		<skos:exactMatch rdf:resource="http://publications.europa.eu/resource/authority/role/REGISTRAR"/>
		<skos:inScheme rdf:resource="https://www.opengis.net/def/CaLAThe/5.0"/>
		<skos:broader rdf:resource="https://www.opengis.net/def/CaLAThe/5.0/OfficialRole"/>
	</skos:Concept>
	<skos:Concept rdf:about="https://www.opengis.net/def/CaLAThe/5.0/Registry">
		<skos:prefLabel xml:lang="en">Registry</skos:prefLabel>
		<skos:prefLabel xml:lang="da">Registerforvaltning</skos:prefLabel>
		<skos:prefLabel xml:lang="tr">Sicil</skos:prefLabel>
		<skos:scopeNote>Public administration</skos:scopeNote>
		<skos:definition>1. Official records of people or things relating to a business or other activity 2. Organization or place that keeps official records (Source: Adopted from Cambridge Dictionary, Business English)</skos:definition>
		<skos:changeNote>Added in version 5.</skos:changeNote>
		<skos:inScheme rdf:resource="https://www.opengis.net/def/CaLAThe/5.0"/>
		<skos:broader rdf:resource="https://www.opengis.net/def/CaLAThe/5.0/Information"/>
		<skos:narrower rdf:resource="https://www.opengis.net/def/CaLAThe/5.0/LandRegister"/>
		<skos:narrower rdf:resource="https://www.opengis.net/def/CaLAThe/5.0/Cadastre"/>
	</skos:Concept>
	<skos:Concept rdf:about="https://www.opengis.net/def/CaLAThe/5.0/Rent">
		<skos:prefLabel xml:lang="en">Rent</skos:prefLabel>
		<skos:prefLabel xml:lang="da">Leje</skos:prefLabel>
		<skos:prefLabel xml:lang="tr">Kira</skos:prefLabel>
		<skos:changeNote>Established with version 2.</skos:changeNote>
		<skos:exactMatch rdf:resource="http://aims.fao.org/aos/agrovoc/c_6503"/>
		<skos:inScheme rdf:resource="https://www.opengis.net/def/CaLAThe/5.0"/>
		<skos:broader rdf:resource="https://www.opengis.net/def/CaLAThe/5.0/Exchange"/>
	</skos:Concept>
	<skos:Concept rdf:about="https://www.opengis.net/def/CaLAThe/5.0/Representation">
		<skos:prefLabel xml:lang="en">Representation</skos:prefLabel>
		<skos:prefLabel xml:lang="da">Repræsentation</skos:prefLabel>
		<skos:prefLabel xml:lang="tr">Temsiliyet</skos:prefLabel>
		<skos:scopeNote>GEMET term</skos:scopeNote>
		<skos:definition>Any conduct or action undertaken on behalf of a person, group, business or government, often as an elected or appointed voice (Source: Random House, 1997).</skos:definition>
		<skos:changeNote>Established with version 1.</skos:changeNote>
		<skos:exactMatch rdf:resource="http://www.eionet.europa.eu/gemet/concept/7118"/>
		<skos:inScheme rdf:resource="https://www.opengis.net/def/CaLAThe/5.0"/>
		<skos:broader rdf:resource="https://www.opengis.net/def/CaLAThe/5.0/RightsHolder"/>
	</skos:Concept>
	<skos:Concept rdf:about="https://www.opengis.net/def/CaLAThe/5.0/RestrictionDeed">
		<skos:prefLabel xml:lang="en">Restriction deed</skos:prefLabel>
		<skos:prefLabel xml:lang="da">Servitutdokument</skos:prefLabel>
		<skos:prefLabel xml:lang="tr">.</skos:prefLabel>
		<skos:changeNote>Established with version 1.</skos:changeNote>
		<skos:inScheme rdf:resource="https://www.opengis.net/def/CaLAThe/5.0"/>
		<skos:broader rdf:resource="https://www.opengis.net/def/CaLAThe/5.0/Deed"/>
	</skos:Concept>
	<skos:Concept rdf:about="https://www.opengis.net/def/CaLAThe/5.0/RightOfSuperficie">
		<skos:prefLabel xml:lang="en">Right of superficies</skos:prefLabel>
		<skos:prefLabel xml:lang="da">Superficiærfæste</skos:prefLabel>
		<skos:prefLabel xml:lang="tr">Üst hakkı</skos:prefLabel>
		<skos:scopeNote>OGC LandInfra / InfraGML term</skos:scopeNote>
		<skos:definition>Real property right which enables its proprietor - the âsuperficiaryâ - to have or acquire for himself buildings, constructions or plants (vegetation) in, on or above an immovable thing owned by someone else (Dutch Civil Code Article 5:101; http://www.dutchcivillaw.com/legislation/dcctitle5588.htm)</skos:definition>
		<skos:changeNote>Established with version 3. Definition is added in version 5.</skos:changeNote>
		<skos:inScheme rdf:resource="https://www.opengis.net/def/CaLAThe/5.0"/>
		<skos:altLabel>Building lease</skos:altLabel>
		<skos:broader rdf:resource="https://www.opengis.net/def/CaLAThe/5.0/CoOwnership"/>
		<skos:related rdf:resource="https://www.opengis.net/def/CaLAThe/5.0/SuperficieObject"/>
	</skos:Concept>
	<skos:Concept rdf:about="https://www.opengis.net/def/CaLAThe/5.0/RightOfWay">
		<skos:prefLabel xml:lang="en">Right of way</skos:prefLabel>
		<skos:prefLabel xml:lang="da">Vejret</skos:prefLabel>
		<skos:prefLabel xml:lang="tr">Geçit hakkı</skos:prefLabel>
		<skos:definition>Right to circulate given to the holder of the ownership of dominant land (Source: Legal Dictionary of Property in Canada - Dualjuridik).</skos:definition>
		<skos:changeNote>Established with version 1. Definition added with ver. 3.</skos:changeNote>
		<skos:inScheme rdf:resource="https://www.opengis.net/def/CaLAThe/5.0"/>
		<skos:broader rdf:resource="https://www.opengis.net/def/CaLAThe/5.0/PrivateLawRestriction"/>
		<skos:broader rdf:resource="https://www.opengis.net/def/CaLAThe/5.0/PublicLawRestriction"/>
	</skos:Concept>
	<skos:Concept rdf:about="https://www.opengis.net/def/CaLAThe/5.0/RightsHolder">
		<skos:prefLabel xml:lang="en">Rights holder</skos:prefLabel>
		<skos:prefLabel xml:lang="da">Rettighedshaver</skos:prefLabel>
		<skos:prefLabel xml:lang="tr">Hak sahibi</skos:prefLabel>
		<skos:changeNote>Established with version 2. Alternative relation with version 3. Changed from Rightholder to Rights holder in version 5.</skos:changeNote>
		<skos:inScheme rdf:resource="https://www.opengis.net/def/CaLAThe/5.0"/>
		<skos:altLabel>Holder</skos:altLabel>
		<skos:broader rdf:resource="https://www.opengis.net/def/CaLAThe/5.0/PartyRoleType"/>
		<skos:narrower rdf:resource="https://www.opengis.net/def/CaLAThe/5.0/Owner"/>
		<skos:narrower rdf:resource="https://www.opengis.net/def/CaLAThe/5.0/Mortgagee"/>
		<skos:narrower rdf:resource="https://www.opengis.net/def/CaLAThe/5.0/Representation"/>
		<skos:narrower rdf:resource="https://www.opengis.net/def/CaLAThe/5.0/PartyMember"/>
		<skos:narrower rdf:resource="https://www.opengis.net/def/CaLAThe/5.0/LegalPerson"/>
		<skos:narrower rdf:resource="https://www.opengis.net/def/CaLAThe/5.0/Mortgagor"/>
		<skos:narrower rdf:resource="https://www.opengis.net/def/CaLAThe/5.0/Lessor"/>
		<skos:narrower rdf:resource="https://www.opengis.net/def/CaLAThe/5.0/Lessee"/>
		<skos:narrower rdf:resource="https://www.opengis.net/def/CaLAThe/5.0/GoodFaith"/>
		<skos:related rdf:resource="https://www.opengis.net/def/CaLAThe/5.0/Document"/>
	</skos:Concept>
	<skos:Concept rdf:about="https://www.opengis.net/def/CaLAThe/5.0/RoadNetwork">
		<skos:prefLabel xml:lang="en">Road network</skos:prefLabel>
		<skos:prefLabel xml:lang="da">Vejnet</skos:prefLabel>
		<skos:prefLabel xml:lang="tr">Yol ağı</skos:prefLabel>
		<skos:scopeNote>INSPIRE theme</skos:scopeNote>
		<skos:changeNote>Established with version 4</skos:changeNote>
		<skos:exactMatch rdf:resource="http://eurovoc.europa.eu/3438"/>
		<skos:inScheme rdf:resource="https://www.opengis.net/def/CaLAThe/5.0"/>
		<skos:broader rdf:resource="https://www.opengis.net/def/CaLAThe/5.0/TopologicalLocalization"/>
		<skos:narrower rdf:resource="https://www.opengis.net/def/CaLAThe/5.0/PostalAddress"/>
	</skos:Concept>
	<skos:Concept rdf:about="https://www.opengis.net/def/CaLAThe/5.0/SatelliteImage">
		<skos:prefLabel xml:lang="en">Satellite image</skos:prefLabel>
		<skos:prefLabel xml:lang="da">Satellitbillede</skos:prefLabel>
		<skos:prefLabel xml:lang="tr">Uydu görüntüsü</skos:prefLabel>
		<skos:scopeNote>GEMET term</skos:scopeNote>
		<skos:definition>A pictorial representation of data projected onto a two-dimensional grid of individual picture elements (pixels) and acquired from a human-made vessel placed in orbit round a planet, moon or star (Source: GEMET).</skos:definition>
		<skos:changeNote>Established with version 1.</skos:changeNote>
		<skos:exactMatch rdf:resource="http://www.eionet.europa.eu/gemet/concept/6253"/>
		<skos:inScheme rdf:resource="https://www.opengis.net/def/CaLAThe/5.0"/>
		<skos:broader rdf:resource="https://www.opengis.net/def/CaLAThe/5.0/DigitalImagery"/>
	</skos:Concept>
	<skos:Concept rdf:about="https://www.opengis.net/def/CaLAThe/5.0/SecurityInterest">
		<skos:prefLabel xml:lang="en">Security interest</skos:prefLabel>
		<skos:prefLabel xml:lang="da">Sikkerhedsret</skos:prefLabel>
		<skos:prefLabel xml:lang="tr">Rehin hakkı</skos:prefLabel>
		<skos:changeNote>Established with version 3.</skos:changeNote>
		<skos:inScheme rdf:resource="https://www.opengis.net/def/CaLAThe/5.0"/>
		<skos:broader rdf:resource="https://www.opengis.net/def/CaLAThe/5.0/LimitedRight"/>
		<skos:narrower rdf:resource="https://www.opengis.net/def/CaLAThe/5.0/Mortgage"/>
	</skos:Concept>
	<skos:Concept rdf:about="https://www.opengis.net/def/CaLAThe/5.0/Seller">
		<skos:prefLabel xml:lang="en">Seller</skos:prefLabel>
		<skos:prefLabel xml:lang="da">Sælger</skos:prefLabel>
		<skos:prefLabel xml:lang="tr">Satıcı</skos:prefLabel>
		<skos:scopeNote>OGC LandInfra / InfraGML term</skos:scopeNote>
		<skos:changeNote>Established with version 4</skos:changeNote>
		<skos:inScheme rdf:resource="https://www.opengis.net/def/CaLAThe/5.0"/>
		<skos:broader rdf:resource="https://www.opengis.net/def/CaLAThe/5.0/Signatory"/>
	</skos:Concept>
	<skos:Concept rdf:about="https://www.opengis.net/def/CaLAThe/5.0/ServientPropertyUnit">
		<skos:prefLabel xml:lang="en">Servient property unit</skos:prefLabel>
		<skos:prefLabel xml:lang="da">Tjenende ejendom</skos:prefLabel>
		<skos:prefLabel xml:lang="tr">Yükümlü taşınmaz</skos:prefLabel>
		<skos:definition>Land (Property unit) submitted to a servitude to benefit a dominant land (Source: Legal Dictionary of Property in Canada - Dualjuridik).</skos:definition>
		<skos:changeNote>Established with version 1. Definition and alt. relation added with version 3.</skos:changeNote>
		<skos:inScheme rdf:resource="https://www.opengis.net/def/CaLAThe/5.0"/>
		<skos:altLabel>Servient land</skos:altLabel>
		<skos:broader rdf:resource="https://www.opengis.net/def/CaLAThe/5.0/Easement"/>
	</skos:Concept>
	<skos:Concept rdf:about="https://www.opengis.net/def/CaLAThe/5.0/Signatory">
		<skos:prefLabel xml:lang="en">Signatory</skos:prefLabel>
		<skos:prefLabel xml:lang="da">Underskriver</skos:prefLabel>
		<skos:prefLabel xml:lang="tr">İmza sahibi</skos:prefLabel>
		<skos:scopeNote>OGC LandInfra / InfraGML term</skos:scopeNote>
		<skos:definition>The person who signs a document (Source: OGC LandInfra, 7.10). A person who signs and is bound by a document (EU, Authority tables, Role)</skos:definition>
		<skos:changeNote>Added with version 3. Context modified in ver. 5, with introduction of Legal personality.</skos:changeNote>
		<skos:exactMatch rdf:resource="http://publications.europa.eu/resource/authority/role/SIGN"/>
		<skos:inScheme rdf:resource="https://www.opengis.net/def/CaLAThe/5.0"/>
		<skos:altLabel>LI_SigningRole</skos:altLabel>
		<skos:broader rdf:resource="https://www.opengis.net/def/CaLAThe/5.0/LegalPersonality"/>
		<skos:narrower rdf:resource="https://www.opengis.net/def/CaLAThe/5.0/Buyer"/>
		<skos:narrower rdf:resource="https://www.opengis.net/def/CaLAThe/5.0/Seller"/>
		<skos:narrower rdf:resource="https://www.opengis.net/def/CaLAThe/5.0/Owner"/>
	</skos:Concept>
	<skos:Concept rdf:about="https://www.opengis.net/def/CaLAThe/5.0/Site">
		<skos:prefLabel xml:lang="en">Site</skos:prefLabel>
		<skos:prefLabel xml:lang="da">Lokalitet</skos:prefLabel>
		<skos:prefLabel xml:lang="tr">Şantiye</skos:prefLabel>
		<skos:scopeNote>OGC LandInfra / InfraGML term</skos:scopeNote>
		<skos:definition>The area of land or water where construction work or other development is undertaken [ISO 6707-1:2014] (OGC LandInfra, 4.2.9).</skos:definition>
		<skos:changeNote>Established with version 3.</skos:changeNote>
		<skos:inScheme rdf:resource="https://www.opengis.net/def/CaLAThe/5.0"/>
		<skos:broader rdf:resource="https://www.opengis.net/def/CaLAThe/5.0/AdministrativeUnit"/>
	</skos:Concept>
	<skos:Concept rdf:about="https://www.opengis.net/def/CaLAThe/5.0/SocialGroup">
		<skos:prefLabel xml:lang="en">Social group</skos:prefLabel>
		<skos:prefLabel xml:lang="da">Samfundsgruppe</skos:prefLabel>
		<skos:prefLabel xml:lang="tr">Sosyal grup</skos:prefLabel>
		<skos:scopeNote>GEMET term</skos:scopeNote>
		<skos:definition>A collection of people who interact with one another and share a certain feeling of unity (GEMET)</skos:definition>
		<skos:changeNote>Established with version 1.</skos:changeNote>
		<skos:exactMatch rdf:resource="http://aims.fao.org/aos/agrovoc/c_15520"/>
		<skos:exactMatch rdf:resource="http://www.eionet.europa.eu/gemet/concept/7796"/>
		<skos:exactMatch rdf:resource="http://zbw.eu/stw/descriptor/15714-0"/>
		<skos:inScheme rdf:resource="https://www.opengis.net/def/CaLAThe/5.0"/>
		<skos:broader rdf:resource="https://www.opengis.net/def/CaLAThe/5.0/GroupParty"/>
		<skos:narrower rdf:resource="https://www.opengis.net/def/CaLAThe/5.0/Family"/>
		<skos:narrower rdf:resource="https://www.opengis.net/def/CaLAThe/5.0/Tribe"/>
		<skos:related rdf:resource="https://www.opengis.net/def/CaLAThe/5.0/Association"/>
	</skos:Concept>
	<skos:Concept rdf:about="https://www.opengis.net/def/CaLAThe/5.0/SocietalRole">
		<skos:prefLabel xml:lang="en">Societal role</skos:prefLabel>
		<skos:prefLabel xml:lang="da">Rolle i samfundet</skos:prefLabel>
		<skos:prefLabel xml:lang="tr">Toplumsal rol</skos:prefLabel>
		<skos:changeNote>Established with version 2.0. Farmer and Neighbor added to narrower with ver. 5.</skos:changeNote>
		<skos:inScheme rdf:resource="https://www.opengis.net/def/CaLAThe/5.0"/>
		<skos:broader rdf:resource="https://www.opengis.net/def/CaLAThe/5.0/NaturalPersonRole"/>
		<skos:narrower rdf:resource="https://www.opengis.net/def/CaLAThe/5.0/Chief"/>
		<skos:narrower rdf:resource="https://www.opengis.net/def/CaLAThe/5.0/Farmer"/>
		<skos:narrower rdf:resource="https://www.opengis.net/def/CaLAThe/5.0/Neighbor"/>
	</skos:Concept>
	<skos:Concept rdf:about="https://www.opengis.net/def/CaLAThe/5.0/SpatialDataInfrastructure">
		<skos:prefLabel xml:lang="en">Spatial data infrastructure</skos:prefLabel>
		<skos:prefLabel xml:lang="da">Geografisk infrastruktur</skos:prefLabel>
		<skos:prefLabel xml:lang="tr">Coğrafi veri altyapısı</skos:prefLabel>
		<skos:changeNote>Established with version 1.</skos:changeNote>
		<skos:inScheme rdf:resource="https://www.opengis.net/def/CaLAThe/5.0"/>
		<skos:broader rdf:resource="https://www.opengis.net/def/CaLAThe/5.0/GeolocatedInformation"/>
		<skos:narrower rdf:resource="https://www.opengis.net/def/CaLAThe/5.0/GeographicalInformationSystem"/>
		<skos:narrower rdf:resource="https://www.opengis.net/def/CaLAThe/5.0/Gazetteer"/>
	</skos:Concept>
	<skos:Concept rdf:about="https://www.opengis.net/def/CaLAThe/5.0/SpatialFeatureType">
		<skos:prefLabel xml:lang="en">Spatial feature type</skos:prefLabel>
		<skos:prefLabel xml:lang="da">Geografiske objekter</skos:prefLabel>
		<skos:prefLabel xml:lang="tr">Coğrafi detay türü</skos:prefLabel>
		<skos:definition>Classification of spatial objects.</skos:definition>
		<skos:changeNote>Established with version 1. Edited with version 4.</skos:changeNote>
		<skos:inScheme rdf:resource="https://www.opengis.net/def/CaLAThe/5.0"/>
		<skos:broader rdf:resource="https://www.opengis.net/def/CaLAThe/5.0/Land"/>
		<skos:narrower rdf:resource="https://www.opengis.net/def/CaLAThe/5.0/LandDivision"/>
		<skos:narrower rdf:resource="https://www.opengis.net/def/CaLAThe/5.0/TopographicalFeature"/>
	</skos:Concept>
	<skos:Concept rdf:about="https://www.opengis.net/def/CaLAThe/5.0/SpatialReference">
		<skos:prefLabel xml:lang="en">Spatial reference</skos:prefLabel>
		<skos:prefLabel xml:lang="da">Rumlig reference</skos:prefLabel>
		<skos:prefLabel xml:lang="tr">Coğrafi referans</skos:prefLabel>
		<skos:scopeNote>Geolexica and INSPIRE term</skos:scopeNote>
		<skos:definition>Description of position in the real world. Note to entry: This may take the form of a label, code or coordinate tuple. (Geolexica ISO 19111:2007)</skos:definition>
		<skos:changeNote>Established with version 1. Edited with version 4 to comply with Geolexica</skos:changeNote>
		<skos:exactMatch rdf:resource="https://isotc211.geolexica.org/concepts/421/"/>
		<skos:inScheme rdf:resource="https://www.opengis.net/def/CaLAThe/5.0"/>
		<skos:broader rdf:resource="https://www.opengis.net/def/CaLAThe/5.0/Information"/>
		<skos:narrower rdf:resource="https://www.opengis.net/def/CaLAThe/5.0/OrdinalReferenceFrame"/>
		<skos:narrower rdf:resource="https://www.opengis.net/def/CaLAThe/5.0/GeographicalGridSystem"/>
		<skos:narrower rdf:resource="https://www.opengis.net/def/CaLAThe/5.0/CoordinateReferenceSystem"/>
	</skos:Concept>
	<skos:Concept rdf:about="https://www.opengis.net/def/CaLAThe/5.0/SpatialUnit">
		<skos:prefLabel xml:lang="en">Spatial unit</skos:prefLabel>
		<skos:prefLabel xml:lang="da">Rumlig enhed</skos:prefLabel>
		<skos:prefLabel xml:lang="tr">Konumsal birim</skos:prefLabel>
		<skos:scopeNote>ISO LADM and OGC LandInfra / InfraGML term</skos:scopeNote>
		<skos:definition>Contiguous geometrical entity, which is delimited and located on or close to the surface of the Earth through the bounding elements of its boundary. Compares to ISO 19152:2012 4.1.23 spatial unit (Source: OGC LandInfra, 4.8.14).</skos:definition>
		<skos:changeNote>Established with version 1.0. Replaced by SpatialType with version 3. Narrower of Geolocated information with version 4</skos:changeNote>
		<skos:exactMatch rdf:resource="http://aims.fao.org/aos/agrovoc/c_9df6243d"/>
		<skos:exactMatch rdf:resource="https://isotc211.geolexica.org/concepts/1363/"/>
		<skos:inScheme rdf:resource="https://www.opengis.net/def/CaLAThe/5.0"/>
		<skos:altLabel>LA_SpatialUnit</skos:altLabel>
		<skos:broader rdf:resource="https://www.opengis.net/def/CaLAThe/5.0/GeolocatedInformation"/>
		<skos:narrower rdf:resource="https://www.opengis.net/def/CaLAThe/5.0/TextLabelType"/>
		<skos:narrower rdf:resource="https://www.opengis.net/def/CaLAThe/5.0/GeometricPrimitive"/>
		<skos:narrower rdf:resource="https://www.opengis.net/def/CaLAThe/5.0/BoundingElement"/>
		<skos:narrower rdf:resource="https://www.opengis.net/def/CaLAThe/5.0/DimensionType"/>
		<skos:narrower rdf:resource="https://www.opengis.net/def/CaLAThe/5.0/TopologicalPrimitive"/>
	</skos:Concept>
	<skos:Concept rdf:about="https://www.opengis.net/def/CaLAThe/5.0/Stakeout">
		<skos:prefLabel xml:lang="en">Stakeout</skos:prefLabel>
		<skos:prefLabel xml:lang="da">Afsætning</skos:prefLabel>
		<skos:prefLabel xml:lang="tr">Aplikasyon</skos:prefLabel>
		<skos:scopeNote>OGC LandInfra / InfraGML term</skos:scopeNote>
		<skos:definition>Stakeout results contains the differences between the design and the resulted TargetPoint. The design point geometry is hold in the DesignPoint (OGC LandInfra 7.8.7.4)</skos:definition>
		<skos:changeNote>Established with version 4</skos:changeNote>
		<skos:exactMatch rdf:resource="http://docs.opengeospatial.org/is/15-111r1/15-111r1.html#162"/>
		<skos:inScheme rdf:resource="https://www.opengis.net/def/CaLAThe/5.0"/>
		<skos:broader rdf:resource="https://www.opengis.net/def/CaLAThe/5.0/TargetPoint"/>
		<skos:broader rdf:resource="https://www.opengis.net/def/CaLAThe/5.0/DesignPoint"/>
	</skos:Concept>
	<skos:Concept rdf:about="https://www.opengis.net/def/CaLAThe/5.0/StreetSign">
		<skos:prefLabel xml:lang="en">Street sign</skos:prefLabel>
		<skos:prefLabel xml:lang="da">Gadeskilt</skos:prefLabel>
		<skos:prefLabel xml:lang="tr">Sokak tabelası</skos:prefLabel>
		<skos:definition>A sign that designates a street and is placed at intersections during a street addressing project (Source: Farvacque-Vitkovic et al, 2005)</skos:definition>
		<skos:changeNote>Established with version 1. Edited with version 4.</skos:changeNote>
		<skos:exactMatch rdf:resource="http://vocabulary.worldbank.org/thesaurus/1935900"/>
		<skos:exactMatch rdf:resource="http://data.europa.eu/cpv/cpv/34992300"/>
		<skos:inScheme rdf:resource="https://www.opengis.net/def/CaLAThe/5.0"/>
		<skos:altLabel>Plate</skos:altLabel>
		<skos:broader rdf:resource="https://www.opengis.net/def/CaLAThe/5.0/Marker"/>
		<skos:broader rdf:resource="https://www.opengis.net/def/CaLAThe/5.0/PostalAddress"/>
	</skos:Concept>
	<skos:Concept rdf:about="https://www.opengis.net/def/CaLAThe/5.0/StringDirection">
		<skos:prefLabel xml:lang="en">String direction</skos:prefLabel>
		<skos:prefLabel xml:lang="da">.</skos:prefLabel>
		<skos:prefLabel xml:lang="tr">.</skos:prefLabel>
		<skos:scopeNote>OGC LandInfra / InfraGML term</skos:scopeNote>
		<skos:definition>For exterior boundary elements, the direction shall be counterclockwise (anti-clockwise) and for interior boundary elements (holes), the direction shall be clockwise. (OGC LandInfra 7.10.7)</skos:definition>
		<skos:inScheme rdf:resource="https://www.opengis.net/def/CaLAThe/5.0"/>
		<skos:broader rdf:resource="https://www.opengis.net/def/CaLAThe/5.0/BEString"/>
	</skos:Concept>
	<skos:Concept rdf:about="https://www.opengis.net/def/CaLAThe/5.0/StringType">
		<skos:prefLabel xml:lang="en">String type</skos:prefLabel>
		<skos:prefLabel xml:lang="da">.</skos:prefLabel>
		<skos:prefLabel xml:lang="tr">.</skos:prefLabel>
		<skos:changeNote>Established with version 4</skos:changeNote>
		<skos:inScheme rdf:resource="https://www.opengis.net/def/CaLAThe/5.0"/>
		<skos:broader rdf:resource="https://www.opengis.net/def/CaLAThe/5.0/BEString"/>
		<skos:narrower rdf:resource="https://www.opengis.net/def/CaLAThe/5.0/LineString"/>
	</skos:Concept>
	<skos:Concept rdf:about="https://www.opengis.net/def/CaLAThe/5.0/Subdivision">
		<skos:prefLabel xml:lang="en">Subdivision</skos:prefLabel>
		<skos:prefLabel xml:lang="da">Udstykning</skos:prefLabel>
		<skos:prefLabel xml:lang="tr">Ayırma; İfraz</skos:prefLabel>
		<skos:changeNote>Established with version 2.</skos:changeNote>
		<skos:inScheme rdf:resource="https://www.opengis.net/def/CaLAThe/5.0"/>
		<skos:broader rdf:resource="https://www.opengis.net/def/CaLAThe/5.0/PropertyFormation"/>
		<skos:narrower rdf:resource="https://www.opengis.net/def/CaLAThe/5.0/CondominiumSubdivision"/>
		<skos:narrower rdf:resource="https://www.opengis.net/def/CaLAThe/5.0/BoundarySurveyAndMarking"/>
	</skos:Concept>
	<skos:Concept rdf:about="https://www.opengis.net/def/CaLAThe/5.0/Sublease">
		<skos:prefLabel xml:lang="en">Sublease</skos:prefLabel>
		<skos:prefLabel xml:lang="da">Fremleje</skos:prefLabel>
		<skos:prefLabel xml:lang="tr">Devren kiralama</skos:prefLabel>
		<skos:definition>A lease granted by a lessee.</skos:definition>
		<skos:inScheme rdf:resource="https://www.opengis.net/def/CaLAThe/5.0"/>
		<skos:broader rdf:resource="https://www.opengis.net/def/CaLAThe/5.0/Leasehold"/>
	</skos:Concept>
	<skos:Concept rdf:about="https://www.opengis.net/def/CaLAThe/5.0/SuperficieObject">
		<skos:prefLabel xml:lang="en">Superficie object</skos:prefLabel>
		<skos:prefLabel xml:lang="da">Bygning på fremmed grund mv</skos:prefLabel>
		<skos:prefLabel xml:lang="tr">Üst hakkı nesnesi</skos:prefLabel>
		<skos:scopeNote>OGC LandInfra / InfraGML term</skos:scopeNote>
		<skos:definition>A SuperficieObject comprises a building or other construction, including pipes, cables or tunnels, established and owned by a party (other than the owner of the LandParcels on which the superficie object is constructed) according to a granting Statement. (Source: OGC LandInfra 7.10.2.6, referring to http://www.dutchcivillaw.com/content/dutchcivillaw022.htm).</skos:definition>
		<skos:changeNote>Established with version 3.</skos:changeNote>
		<skos:inScheme rdf:resource="https://www.opengis.net/def/CaLAThe/5.0"/>
		<skos:altLabel>3D object</skos:altLabel>
		<skos:broader rdf:resource="https://www.opengis.net/def/CaLAThe/5.0/Construction"/>
		<skos:broader rdf:resource="https://www.opengis.net/def/CaLAThe/5.0/RealProperty"/>
		<skos:related rdf:resource="https://www.opengis.net/def/CaLAThe/5.0/CarrierParcel"/>
		<skos:related rdf:resource="https://www.opengis.net/def/CaLAThe/5.0/RightOfSuperficie"/>
	</skos:Concept>
	<skos:Concept rdf:about="https://www.opengis.net/def/CaLAThe/5.0/SuperficieObjectEstablishment">
		<skos:prefLabel xml:lang="en">Superficie object establishment</skos:prefLabel>
		<skos:prefLabel xml:lang="da">Etablering af superficieobjekt</skos:prefLabel>
		<skos:prefLabel xml:lang="tr">Üst hakkı tesisi</skos:prefLabel>
		<skos:scopeNote>OGC LandInfra / InfraGML term</skos:scopeNote>
		<skos:changeNote>Established with version 3.</skos:changeNote>
		<skos:inScheme rdf:resource="https://www.opengis.net/def/CaLAThe/5.0"/>
		<skos:altLabel>3D object identification</skos:altLabel>
		<skos:broader rdf:resource="https://www.opengis.net/def/CaLAThe/5.0/PropertyFormation"/>
	</skos:Concept>
	<skos:Concept rdf:about="https://www.opengis.net/def/CaLAThe/5.0/SuperficieObjectScheme">
		<skos:prefLabel xml:lang="en">Superficie object scheme</skos:prefLabel>
		<skos:prefLabel xml:lang="da">Dokument om superficieobjekt</skos:prefLabel>
		<skos:prefLabel xml:lang="tr">Üst hakkı sözleşmesi</skos:prefLabel>
		<skos:scopeNote>OGC LandInfra / InfraGML term</skos:scopeNote>
		<skos:changeNote>Established with version 3.</skos:changeNote>
		<skos:inScheme rdf:resource="https://www.opengis.net/def/CaLAThe/5.0"/>
		<skos:altLabel>3D object scheme</skos:altLabel>
		<skos:broader rdf:resource="https://www.opengis.net/def/CaLAThe/5.0/Document"/>
	</skos:Concept>
	<skos:Concept rdf:about="https://www.opengis.net/def/CaLAThe/5.0/Surface">
		<skos:prefLabel xml:lang="en">Surface</skos:prefLabel>
		<skos:prefLabel xml:lang="da">Overflade</skos:prefLabel>
		<skos:prefLabel xml:lang="tr">Yüzey</skos:prefLabel>
		<skos:scopeNote>Geolexica term</skos:scopeNote>
		<skos:definition>2-dimensional geometric primitive, locally representing a continuous image of a region of a plane. Note to entry: The boundary of a surface is the set of oriented, closed curves that delineate the limits of the surface. Surfaces that are isomorphic to a sphere, or to an n-torus (a topological sphere with n "handles") have no boundary. Such surfaces are called cycles. (Geolexica, ISO 19107:2003)</skos:definition>
		<skos:changeNote>Established with version 4.</skos:changeNote>
		<skos:exactMatch rdf:resource="https://isotc211.geolexica.org/concepts/437/"/>
		<skos:inScheme rdf:resource="https://www.opengis.net/def/CaLAThe/5.0"/>
		<skos:broader rdf:resource="https://www.opengis.net/def/CaLAThe/5.0/GeometricPrimitive"/>
		<skos:narrower rdf:resource="https://www.opengis.net/def/CaLAThe/5.0/Polygon"/>
	</skos:Concept>
	<skos:Concept rdf:about="https://www.opengis.net/def/CaLAThe/5.0/Survey">
		<skos:prefLabel xml:lang="en">Survey</skos:prefLabel>
		<skos:prefLabel xml:lang="da">Opmåling, landmåling</skos:prefLabel>
		<skos:prefLabel xml:lang="tr">Ölçme</skos:prefLabel>
		<skos:scopeNote>OGC LandInfra / InfraGML term</skos:scopeNote>
		<skos:definition>An examination of facts or conditions to provide information on a situation, conducted through on-site observations (cf GEMET: Survey)</skos:definition>
		<skos:changeNote>Established with version 4</skos:changeNote>
		<skos:exactMatch rdf:resource="https://www.eionet.europa.eu/gemet/en/concept/8240"/>
		<skos:inScheme rdf:resource="https://www.opengis.net/def/CaLAThe/5.0"/>
		<skos:topConceptOf rdf:resource="https://www.opengis.net/def/CaLAThe/5.0"/>
		<skos:narrower rdf:resource="https://www.opengis.net/def/CaLAThe/5.0/SurveyingInstrument"/>
		<skos:narrower rdf:resource="https://www.opengis.net/def/CaLAThe/5.0/SurveyResult"/>
	</skos:Concept>
	<skos:Concept rdf:about="https://www.opengis.net/def/CaLAThe/5.0/SurveyMark">
		<skos:prefLabel xml:lang="en">Survey mark</skos:prefLabel>
		<skos:prefLabel xml:lang="da">Afmærket punkt</skos:prefLabel>
		<skos:prefLabel xml:lang="tr">Ölçü noktası</skos:prefLabel>
		<skos:scopeNote>OGC LandInfra / InfraGML term</skos:scopeNote>
		<skos:definition>Physical object which by its form defines a point on the surface of the Earth (Source: OGC LandInfra, 4.1.22).</skos:definition>
		<skos:changeNote>Established with version 3.</skos:changeNote>
		<skos:inScheme rdf:resource="https://www.opengis.net/def/CaLAThe/5.0"/>
		<skos:broader rdf:resource="https://www.opengis.net/def/CaLAThe/5.0/Marker"/>
		<skos:narrower rdf:resource="https://www.opengis.net/def/CaLAThe/5.0/BoundaryMark"/>
		<skos:narrower rdf:resource="https://www.opengis.net/def/CaLAThe/5.0/ControlPointMonument"/>
		<skos:narrower rdf:resource="https://www.opengis.net/def/CaLAThe/5.0/TrigonometricMark"/>
	</skos:Concept>
	<skos:Concept rdf:about="https://www.opengis.net/def/CaLAThe/5.0/SurveyMonumentEstablishment">
		<skos:prefLabel xml:lang="en">Survey monument establishment</skos:prefLabel>
		<skos:prefLabel xml:lang="da">Afmærkning af skel</skos:prefLabel>
		<skos:prefLabel xml:lang="tr">Ölçü noktası tesisi</skos:prefLabel>
		<skos:scopeNote>OGC LandInfra / InfraGML term</skos:scopeNote>
		<skos:changeNote>Established with version 3.</skos:changeNote>
		<skos:inScheme rdf:resource="https://www.opengis.net/def/CaLAThe/5.0"/>
		<skos:broader rdf:resource="https://www.opengis.net/def/CaLAThe/5.0/BoundarySurveyAndMarking"/>
	</skos:Concept>
	<skos:Concept rdf:about="https://www.opengis.net/def/CaLAThe/5.0/SurveyResult">
		<skos:prefLabel xml:lang="en">Survey result</skos:prefLabel>
		<skos:prefLabel xml:lang="da">Opmålingsresultat</skos:prefLabel>
		<skos:prefLabel xml:lang="tr">Ölçü sonucu</skos:prefLabel>
		<skos:scopeNote>OGC LandInfra / InfraGML term</skos:scopeNote>
		<skos:changeNote>Established with version 4</skos:changeNote>
		<skos:inScheme rdf:resource="https://www.opengis.net/def/CaLAThe/5.0"/>
		<skos:broader rdf:resource="https://www.opengis.net/def/CaLAThe/5.0/Survey"/>
		<skos:narrower rdf:resource="https://www.opengis.net/def/CaLAThe/5.0/Observation"/>
		<skos:narrower rdf:resource="https://www.opengis.net/def/CaLAThe/5.0/PointCloud"/>
		<skos:narrower rdf:resource="https://www.opengis.net/def/CaLAThe/5.0/Image"/>
		<skos:narrower rdf:resource="https://www.opengis.net/def/CaLAThe/5.0/TargetPoint"/>
		<skos:narrower rdf:resource="https://www.opengis.net/def/CaLAThe/5.0/DesignPoint"/>
	</skos:Concept>
	<skos:Concept rdf:about="https://www.opengis.net/def/CaLAThe/5.0/SurveyingInstrument">
		<skos:prefLabel xml:lang="en">Surveying instrument</skos:prefLabel>
		<skos:prefLabel xml:lang="da">Instrument</skos:prefLabel>
		<skos:prefLabel xml:lang="tr">Ölçme aleti</skos:prefLabel>
		<skos:changeNote>Established with version 4</skos:changeNote>
		<skos:inScheme rdf:resource="https://www.opengis.net/def/CaLAThe/5.0"/>
		<skos:broader rdf:resource="https://www.opengis.net/def/CaLAThe/5.0/Survey"/>
		<skos:narrower rdf:resource="https://www.opengis.net/def/CaLAThe/5.0/Camera"/>
		<skos:narrower rdf:resource="https://www.opengis.net/def/CaLAThe/5.0/Compass"/>
		<skos:narrower rdf:resource="https://www.opengis.net/def/CaLAThe/5.0/LI_Sensor"/>
		<skos:narrower rdf:resource="https://www.opengis.net/def/CaLAThe/5.0/MeasuringTape"/>
		<skos:narrower rdf:resource="https://www.opengis.net/def/CaLAThe/5.0/EletronicDistanceMeter"/>
		<skos:narrower rdf:resource="https://www.opengis.net/def/CaLAThe/5.0/Theodolite"/>
		<skos:narrower rdf:resource="https://www.opengis.net/def/CaLAThe/5.0/GNSSsensor"/>
		<skos:narrower rdf:resource="https://www.opengis.net/def/CaLAThe/5.0/TerrestrialLaserScanner"/>
		<skos:narrower rdf:resource="https://www.opengis.net/def/CaLAThe/5.0/TotalStation"/>
	</skos:Concept>
	<skos:Concept rdf:about="https://www.opengis.net/def/CaLAThe/5.0/Surveyor">
		<skos:prefLabel xml:lang="en">Surveyor</skos:prefLabel>
		<skos:prefLabel xml:lang="da">Landinspektør med beskikkelse</skos:prefLabel>
		<skos:prefLabel xml:lang="tr">Haritacı</skos:prefLabel>
		<skos:changeNote>Established with version 1.</skos:changeNote>
		<skos:exactMatch rdf:resource="http://aims.fao.org/aos/agrovoc/c_26e30c73"/>
		<skos:inScheme rdf:resource="https://www.opengis.net/def/CaLAThe/5.0"/>
		<skos:broader rdf:resource="https://www.opengis.net/def/CaLAThe/5.0/Professional"/>
		<skos:narrower rdf:resource="https://www.opengis.net/def/CaLAThe/5.0/LicensedSurveyor"/>
		<skos:narrower rdf:resource="https://www.opengis.net/def/CaLAThe/5.0/LI_LandSurveyor"/>
		<skos:narrower rdf:resource="https://www.opengis.net/def/CaLAThe/5.0/LA_CertifiedSurveyor"/>
	</skos:Concept>
	<skos:Concept rdf:about="https://www.opengis.net/def/CaLAThe/5.0/TargetPoint">
		<skos:prefLabel xml:lang="en">Target point</skos:prefLabel>
		<skos:prefLabel xml:lang="da">Sigtepunkt</skos:prefLabel>
		<skos:prefLabel xml:lang="tr">Hedef noktası</skos:prefLabel>
		<skos:scopeNote>OGC LandInfra / InfraGML term</skos:scopeNote>
		<skos:definition>TargetPoint is the value of a geometry of the feature of interest that has been estimated from the raw observations (OGC LandInfra 7.8.7.2)</skos:definition>
		<skos:changeNote>Established with version 4</skos:changeNote>
		<skos:inScheme rdf:resource="https://www.opengis.net/def/CaLAThe/5.0"/>
		<skos:broader rdf:resource="https://www.opengis.net/def/CaLAThe/5.0/SurveyResult"/>
		<skos:broader rdf:resource="https://www.opengis.net/def/CaLAThe/5.0/TPSobservation"/>
		<skos:broader rdf:resource="https://www.opengis.net/def/CaLAThe/5.0/GNSSobservation"/>
		<skos:narrower rdf:resource="https://www.opengis.net/def/CaLAThe/5.0/Stakeout"/>
	</skos:Concept>
	<skos:Concept rdf:about="https://www.opengis.net/def/CaLAThe/5.0/TerrestrialLaserScanner">
		<skos:prefLabel xml:lang="en">Terrestrial Laser Scanner</skos:prefLabel>
		<skos:prefLabel xml:lang="da">Terrestisk laserscanner</skos:prefLabel>
		<skos:prefLabel xml:lang="tr">Yersel lazer tarama</skos:prefLabel>
		<skos:scopeNote>OGC LandInfra / InfraGML term</skos:scopeNote>
		<skos:definition>Terrestrial LaserScanner sensors are used to measure point clouds with the controlled steering of laser beams followed by a distance measurement at every pointing direction. (OGC LandInfra 7.8.5.12)</skos:definition>
		<skos:changeNote>Established with version 4</skos:changeNote>
		<skos:inScheme rdf:resource="https://www.opengis.net/def/CaLAThe/5.0"/>
		<skos:altLabel>Laser scanner</skos:altLabel>
		<skos:broader rdf:resource="https://www.opengis.net/def/CaLAThe/5.0/SurveyingInstrument"/>
		<skos:narrower rdf:resource="https://www.opengis.net/def/CaLAThe/5.0/PointCloud"/>
	</skos:Concept>
	<skos:Concept rdf:about="https://www.opengis.net/def/CaLAThe/5.0/TextLabelType">
		<skos:prefLabel xml:lang="en">Textlabel type</skos:prefLabel>
		<skos:prefLabel xml:lang="da">.</skos:prefLabel>
		<skos:prefLabel xml:lang="tr">.</skos:prefLabel>
		<skos:changeNote>Established with version 1.</skos:changeNote>
		<skos:inScheme rdf:resource="https://www.opengis.net/def/CaLAThe/5.0"/>
		<skos:broader rdf:resource="https://www.opengis.net/def/CaLAThe/5.0/SpatialUnit"/>
	</skos:Concept>
	<skos:Concept rdf:about="https://www.opengis.net/def/CaLAThe/5.0/Theodolite">
		<skos:prefLabel xml:lang="en">Theodolite</skos:prefLabel>
		<skos:prefLabel xml:lang="da">Teodolit</skos:prefLabel>
		<skos:prefLabel xml:lang="tr">Teodolit</skos:prefLabel>
		<skos:scopeNote>OGC LandInfra / InfraGML term</skos:scopeNote>
		<skos:definition>Instrument for measuring horizontal directions or horizontal directions and vertical angles, whose main components are the horizontal circle and the vertical circle, the telescope and additional devices for reading the graduated circles and for setting up the vertical axis (OGC LandInfra 4.6.18, referring to ISO 9849-1:2000)</skos:definition>
		<skos:changeNote>Established with version 4</skos:changeNote>
		<skos:inScheme rdf:resource="https://www.opengis.net/def/CaLAThe/5.0"/>
		<skos:broader rdf:resource="https://www.opengis.net/def/CaLAThe/5.0/SurveyingInstrument"/>
		<skos:narrower rdf:resource="https://www.opengis.net/def/CaLAThe/5.0/AngelObservation"/>
	</skos:Concept>
	<skos:Concept rdf:about="https://www.opengis.net/def/CaLAThe/5.0/TimeshareRight">
		<skos:prefLabel xml:lang="en">Timeshare right</skos:prefLabel>
		<skos:prefLabel xml:lang="da">Timeshare rettighed</skos:prefLabel>
		<skos:prefLabel xml:lang="tr">Devre mülk hakkı</skos:prefLabel>
		<skos:changeNote>Established with v1.</skos:changeNote>
		<skos:inScheme rdf:resource="https://www.opengis.net/def/CaLAThe/5.0"/>
		<skos:broader rdf:resource="https://www.opengis.net/def/CaLAThe/5.0/CoOwnership"/>
	</skos:Concept>
	<skos:Concept rdf:about="https://www.opengis.net/def/CaLAThe/5.0/Title">
		<skos:prefLabel xml:lang="en">Title</skos:prefLabel>
		<skos:prefLabel xml:lang="da">Adkomst</skos:prefLabel>
		<skos:prefLabel xml:lang="tr">Tapu</skos:prefLabel>
		<skos:scopeNote>EULIS / ELRA term</skos:scopeNote>
		<skos:definition>Proof of right related to land (Source: EULIS / ELRA glossary)</skos:definition>
		<skos:changeNote>Established with version 3.</skos:changeNote>
		<skos:inScheme rdf:resource="https://www.opengis.net/def/CaLAThe/5.0"/>
		<skos:broader rdf:resource="https://www.opengis.net/def/CaLAThe/5.0/Owner"/>
	</skos:Concept>
	<skos:Concept rdf:about="https://www.opengis.net/def/CaLAThe/5.0/TitleDeed">
		<skos:prefLabel xml:lang="en">Title deed</skos:prefLabel>
		<skos:prefLabel xml:lang="da">Skøde</skos:prefLabel>
		<skos:prefLabel xml:lang="tr">Tapu senedi</skos:prefLabel>
		<skos:changeNote>Established with version 1.</skos:changeNote>
		<skos:exactMatch rdf:resource="http://aims.fao.org/aos/agrovoc/c_b769471e"/>
		<skos:inScheme rdf:resource="https://www.opengis.net/def/CaLAThe/5.0"/>
		<skos:broader rdf:resource="https://www.opengis.net/def/CaLAThe/5.0/Deed"/>
	</skos:Concept>
	<skos:Concept rdf:about="https://www.opengis.net/def/CaLAThe/5.0/TopographicMap">
		<skos:prefLabel xml:lang="en">Topographic map</skos:prefLabel>
		<skos:prefLabel xml:lang="da">Topografisk kort</skos:prefLabel>
		<skos:prefLabel xml:lang="tr">Topoğrafik harita</skos:prefLabel>
		<skos:changeNote>Established with version 2.0</skos:changeNote>
		<skos:inScheme rdf:resource="https://www.opengis.net/def/CaLAThe/5.0"/>
		<skos:broader rdf:resource="https://www.opengis.net/def/CaLAThe/5.0/Map"/>
	</skos:Concept>
	<skos:Concept rdf:about="https://www.opengis.net/def/CaLAThe/5.0/TopographicalFeature">
		<skos:prefLabel xml:lang="en">Topographical feature</skos:prefLabel>
		<skos:prefLabel xml:lang="da">Topografisk objekt</skos:prefLabel>
		<skos:prefLabel xml:lang="tr">Topoğrafik detay</skos:prefLabel>
		<skos:definition>Land and objects, described from a physical (non-administrative) perspective.</skos:definition>
		<skos:changeNote>Established with version 1. Definition is added in version 5.</skos:changeNote>
		<skos:inScheme rdf:resource="https://www.opengis.net/def/CaLAThe/5.0"/>
		<skos:broader rdf:resource="https://www.opengis.net/def/CaLAThe/5.0/SpatialFeatureType"/>
		<skos:narrower rdf:resource="https://www.opengis.net/def/CaLAThe/5.0/Hydrography"/>
		<skos:narrower rdf:resource="https://www.opengis.net/def/CaLAThe/5.0/Elevation"/>
		<skos:narrower rdf:resource="https://www.opengis.net/def/CaLAThe/5.0/TransportNetwork"/>
		<skos:narrower rdf:resource="https://www.opengis.net/def/CaLAThe/5.0/Construction"/>
	</skos:Concept>
	<skos:Concept rdf:about="https://www.opengis.net/def/CaLAThe/5.0/TopologicalLocalization">
		<skos:prefLabel xml:lang="en">Topological localization</skos:prefLabel>
		<skos:prefLabel xml:lang="da">Topologisk stedbestemmelse</skos:prefLabel>
		<skos:prefLabel xml:lang="tr">.</skos:prefLabel>
		<skos:definition>Topological localization is achieved through the topological primitive: node representing location, while the topological primitive: edge represents the adjacency relationship between locations (cf. Ulrich, Nourbakhsh, 2000)</skos:definition>
		<skos:changeNote>Introduced with version 4</skos:changeNote>
		<skos:inScheme rdf:resource="https://www.opengis.net/def/CaLAThe/5.0"/>
		<skos:broader rdf:resource="https://www.opengis.net/def/CaLAThe/5.0/GeolocatedInformation"/>
		<skos:narrower rdf:resource="https://www.opengis.net/def/CaLAThe/5.0/RoadNetwork"/>
	</skos:Concept>
	<skos:Concept rdf:about="https://www.opengis.net/def/CaLAThe/5.0/TopologicalPrimitive">
		<skos:prefLabel xml:lang="en">Topological primitive</skos:prefLabel>
		<skos:prefLabel xml:lang="da">Topologisk objekt</skos:prefLabel>
		<skos:prefLabel xml:lang="tr">Topolojik temel şekiller</skos:prefLabel>
		<skos:scopeNote>ISO/PDTS 19104 term</skos:scopeNote>
		<skos:definition>A topological object that represents a single, non-decomposable element. (Source: ISO 19104:2016).</skos:definition>
		<skos:changeNote>Established with version 1.</skos:changeNote>
		<skos:exactMatch rdf:resource="https://isotc211.geolexica.org/concepts/2254/"/>
		<skos:inScheme rdf:resource="https://www.opengis.net/def/CaLAThe/5.0"/>
		<skos:broader rdf:resource="https://www.opengis.net/def/CaLAThe/5.0/SpatialUnit"/>
		<skos:narrower rdf:resource="https://www.opengis.net/def/CaLAThe/5.0/Node"/>
		<skos:narrower rdf:resource="https://www.opengis.net/def/CaLAThe/5.0/Edge"/>
		<skos:narrower rdf:resource="https://www.opengis.net/def/CaLAThe/5.0/Face"/>
	</skos:Concept>
	<skos:Concept rdf:about="https://www.opengis.net/def/CaLAThe/5.0/TotalStation">
		<skos:prefLabel xml:lang="en">Total station</skos:prefLabel>
		<skos:prefLabel xml:lang="da">Totalstation</skos:prefLabel>
		<skos:prefLabel xml:lang="tr">Totalstation</skos:prefLabel>
		<skos:scopeNote>OGC LandInfra / InfraGML term</skos:scopeNote>
		<skos:changeNote>Established with version 4</skos:changeNote>
		<skos:inScheme rdf:resource="https://www.opengis.net/def/CaLAThe/5.0"/>
		<skos:broader rdf:resource="https://www.opengis.net/def/CaLAThe/5.0/SurveyingInstrument"/>
		<skos:narrower rdf:resource="https://www.opengis.net/def/CaLAThe/5.0/TPSobservation"/>
	</skos:Concept>
	<skos:Concept rdf:about="https://www.opengis.net/def/CaLAThe/5.0/TPSobservation">
		<skos:prefLabel xml:lang="en">TPSobservation</skos:prefLabel>
		<skos:prefLabel xml:lang="da">Vinkel- og afstandsmåling</skos:prefLabel>
		<skos:prefLabel xml:lang="tr">.</skos:prefLabel>
		<skos:scopeNote>OGC LandInfra / InfraGML term</skos:scopeNote>
		<skos:changeNote>Established with version 4</skos:changeNote>
		<skos:inScheme rdf:resource="https://www.opengis.net/def/CaLAThe/5.0"/>
		<skos:broader rdf:resource="https://www.opengis.net/def/CaLAThe/5.0/TotalStation"/>
		<skos:broader rdf:resource="https://www.opengis.net/def/CaLAThe/5.0/Observation"/>
		<skos:narrower rdf:resource="https://www.opengis.net/def/CaLAThe/5.0/TargetPoint"/>
	</skos:Concept>
	<skos:Concept rdf:about="https://www.opengis.net/def/CaLAThe/5.0/Transfer">
		<skos:prefLabel xml:lang="en">Transfer</skos:prefLabel>
		<skos:prefLabel xml:lang="da">Overdragelse</skos:prefLabel>
		<skos:prefLabel xml:lang="tr">İntikal</skos:prefLabel>
		<skos:changeNote>Established with version 2.</skos:changeNote>
		<skos:exactMatch rdf:resource="http://eurovoc.europa.eu/4503"/>
		<skos:inScheme rdf:resource="https://www.opengis.net/def/CaLAThe/5.0"/>
		<skos:broader rdf:resource="https://www.opengis.net/def/CaLAThe/5.0/Activity"/>
		<skos:narrower rdf:resource="https://www.opengis.net/def/CaLAThe/5.0/Gift"/>
		<skos:narrower rdf:resource="https://www.opengis.net/def/CaLAThe/5.0/Inheritance"/>
		<skos:narrower rdf:resource="https://www.opengis.net/def/CaLAThe/5.0/Partition"/>
	</skos:Concept>
	<skos:Concept rdf:about="https://www.opengis.net/def/CaLAThe/5.0/TransferOfPartOfProperty">
		<skos:prefLabel xml:lang="en">Transfer of part of property</skos:prefLabel>
		<skos:prefLabel xml:lang="da">Arealoverførsel</skos:prefLabel>
		<skos:prefLabel xml:lang="tr">İfrazen devir</skos:prefLabel>
		<skos:changeNote>Established with version 2.0.</skos:changeNote>
		<skos:inScheme rdf:resource="https://www.opengis.net/def/CaLAThe/5.0"/>
		<skos:broader rdf:resource="https://www.opengis.net/def/CaLAThe/5.0/PropertyFormation"/>
		<skos:narrower rdf:resource="https://www.opengis.net/def/CaLAThe/5.0/Reallotment"/>
	</skos:Concept>
	<skos:Concept rdf:about="https://www.opengis.net/def/CaLAThe/5.0/TransportNetwork">
		<skos:prefLabel xml:lang="en">Transport network</skos:prefLabel>
		<skos:prefLabel xml:lang="da">Transportnet</skos:prefLabel>
		<skos:prefLabel xml:lang="tr">Ulaşım ağı</skos:prefLabel>
		<skos:scopeNote>INSPIRE theme</skos:scopeNote>
		<skos:definition>Road, rail, air and water transport networks and related infrastructure. Includes links between different networks. Also includes the trans-European transport network as defined in Decision No 1692/96/EC of the European Parliament and of the Council of 23 July 1996 on Community Guidelines for the development of the trans-European transport network (1) and future revisions of that Decision (Source: INSPIRE theme register).</skos:definition>
		<skos:changeNote>Established with version 1.</skos:changeNote>
		<skos:exactMatch rdf:resource="http://inspire.ec.europa.eu/theme/tn"/>
		<skos:exactMatch rdf:resource="https://isotc211.geolexica.org/concepts/1621/"/>
		<skos:inScheme rdf:resource="https://www.opengis.net/def/CaLAThe/5.0"/>
		<skos:broader rdf:resource="https://www.opengis.net/def/CaLAThe/5.0/TopographicalFeature"/>
	</skos:Concept>
	<skos:Concept rdf:about="https://www.opengis.net/def/CaLAThe/5.0/Tribe">
		<skos:prefLabel xml:lang="en">Tribe</skos:prefLabel>
		<skos:prefLabel xml:lang="da">Stamme</skos:prefLabel>
		<skos:prefLabel xml:lang="tr">Aşiret; Kabile</skos:prefLabel>
		<skos:changeNote>Established with version 1.</skos:changeNote>
		<skos:exactMatch rdf:resource="http://aims.fao.org/aos/agrovoc/c_331526"/>
		<skos:inScheme rdf:resource="https://www.opengis.net/def/CaLAThe/5.0"/>
		<skos:broader rdf:resource="https://www.opengis.net/def/CaLAThe/5.0/SocialGroup"/>
	</skos:Concept>
	<skos:Concept rdf:about="https://www.opengis.net/def/CaLAThe/5.0/TrigonometricMark">
		<skos:prefLabel xml:lang="en">Trigonometric mark</skos:prefLabel>
		<skos:prefLabel xml:lang="da">Trigonometrisk postament</skos:prefLabel>
		<skos:prefLabel xml:lang="tr">Trigonometrik işaret</skos:prefLabel>
		<skos:scopeNote>OGC LandInfra / InfraGML term</skos:scopeNote>
		<skos:definition>Marks an observation point of geodetic significance (Source: OGC LandInfra, 7.10.5.1)</skos:definition>
		<skos:changeNote>Established with version 3.</skos:changeNote>
		<skos:inScheme rdf:resource="https://www.opengis.net/def/CaLAThe/5.0"/>
		<skos:broader rdf:resource="https://www.opengis.net/def/CaLAThe/5.0/SurveyMark"/>
	</skos:Concept>
	<skos:Concept rdf:about="https://www.opengis.net/def/CaLAThe/5.0/UserDefinedValue">
		<skos:prefLabel xml:lang="en">User defined value</skos:prefLabel>
		<skos:prefLabel xml:lang="da">Brugerdefineret værdi</skos:prefLabel>
		<skos:prefLabel xml:lang="tr">Özel değer</skos:prefLabel>
		<skos:inScheme rdf:resource="https://www.opengis.net/def/CaLAThe/5.0"/>
		<skos:broader rdf:resource="https://www.opengis.net/def/CaLAThe/5.0/CodeList"/>
	</skos:Concept>
	<skos:Concept rdf:about="https://www.opengis.net/def/CaLAThe/5.0/Usufruct">
		<skos:prefLabel xml:lang="en">Usufruct</skos:prefLabel>
		<skos:prefLabel xml:lang="da">Brugsret</skos:prefLabel>
		<skos:prefLabel xml:lang="tr">Yararlanma (intifa) hakkı</skos:prefLabel>
		<skos:scopeNote>EULIS / ELRA term</skos:scopeNote>
		<skos:definition>Temporary right to use and enjoy the benefit and gain of the property of another, without changing the character of the property. (Source: EULIS / ELRA glossary)</skos:definition>
		<skos:exactMatch rdf:resource="http://aims.fao.org/aos/agrovoc/c_28784"/>
		<skos:exactMatch rdf:resource="http://eurovoc.europa.eu/4625"/>
		<skos:inScheme rdf:resource="https://www.opengis.net/def/CaLAThe/5.0"/>
		<skos:broader rdf:resource="https://www.opengis.net/def/CaLAThe/5.0/LimitedRight"/>
	</skos:Concept>

	</rdf:RDF>
