@prefix dcterms: <http://purl.org/dc/terms/> .
@prefix rdfs: <http://www.w3.org/2000/01/rdf-schema#> .
@prefix skos: <http://www.w3.org/2004/02/skos/core#> .
@prefix xsd: <http://www.w3.org/2001/XMLSchema#> .

<http://www.opengis.net/def/glossary/term/Collection> a skos:Concept ;
    rdfs:label "Collection" ;
    dcterms:created "2023-10-13T16:54:05.345735"^^xsd:dateTime ;
    rdfs:seeAlso <https://docs.ogc.org/is/19-086r6/19-086r6.html> ;
    skos:definition "body of resources that belong or are used together. An aggregate, set, or group of related resources" ;
    skos:inScheme <http://www.opengis.net/def/glossary> ;
    skos:prefLabel "Collection" .

<http://www.opengis.net/def/glossary/term/Conformance> a skos:Concept ;
    rdfs:label "Conformance" ;
    dcterms:created "2023-10-13T16:54:05.345962"^^xsd:dateTime ;
    rdfs:seeAlso <https://www.iso.org/obp/ui/en/#iso:std:iso:19105:ed-2:v1:en> ;
    skos:definition "fulfilment of a requirement" ;
    skos:inScheme <http://www.opengis.net/def/glossary> ;
    skos:prefLabel "Conformance" .

<http://www.opengis.net/def/glossary/term/DCAT> a skos:Concept ;
    rdfs:label "Data Catalog Vocabulary" ;
    dcterms:created "2023-10-13T16:54:05.346122"^^xsd:dateTime ;
    rdfs:seeAlso <https://www.w3.org/TR/vocab-dcat-3/> ;
    skos:altLabel "DCAT" ;
    skos:definition "an RDF vocabulary designed to facilitate interoperability between data catalogs published on the Web" ;
    skos:inScheme <http://www.opengis.net/def/glossary> ;
    skos:prefLabel "Data Catalog Vocabulary" .

<http://www.opengis.net/def/glossary/term/DCAT-AP> a skos:Concept ;
    rdfs:label "DCAT Application Profile for Data Portals in Europe" ;
    dcterms:created "2023-10-13T16:54:05.346264"^^xsd:dateTime ;
    rdfs:seeAlso <https://ec.europa.eu/isa2/solutions/dcat-application-profile-data-portals-europe_en/> ;
    skos:altLabel "DCAT-AP" ;
    skos:definition "an extension of the Data Catalog Vocabulary (DCAT) which is an RDF vocabulary for describing datasets and data catalogs on the web" ;
    skos:inScheme <http://www.opengis.net/def/glossary> ;
    skos:prefLabel "DCAT Application Profile for Data Portals in Europe" .

<http://www.opengis.net/def/glossary/term/DiscoveryService> a skos:Concept ;
    rdfs:label "Discovery service" ;
    dcterms:created "2023-10-13T16:54:05.346388"^^xsd:dateTime ;
    rdfs:seeAlso <https://eur-lex.europa.eu/legal-content/EN/TXT/?uri=CELEX%3A02007L0002-20190626> ;
    skos:definition "a service that makes it possible to search for spatial data sets and services on the basis of the content of the corresponding metadata and to display the content of the metadata" ;
    skos:inScheme <http://www.opengis.net/def/glossary> ;
    skos:prefLabel "Discovery service" .

<http://www.opengis.net/def/glossary/term/DownloadService> a skos:Concept ;
    rdfs:label "Download service" ;
    dcterms:created "2023-10-13T16:54:05.346529"^^xsd:dateTime ;
    rdfs:seeAlso <https://eur-lex.europa.eu/legal-content/EN/TXT/?uri=CELEX%3A02007L0002-20190626> ;
    skos:definition "a service enabling copies of spatial data sets, or parts of such sets, to be downloaded, and, where practicable, accessed directly" ;
    skos:inScheme <http://www.opengis.net/def/glossary> ;
    skos:prefLabel "Download service" .

<http://www.opengis.net/def/glossary/term/DraftStandard> a skos:Concept ;
    rdfs:label "Draft Standard" ;
    dcterms:created "2023-10-13T16:54:05.346653"^^xsd:dateTime ;
    rdfs:seeAlso <https://docs.ogc.org/pol/05-020r29/05-020r29.html#the-two-track-Standards-process-characteristics> ;
    skos:definition "a document developed by the OGC membership for which there is no evidence of implementation or CITE tests. However, the members wish to approve the document as an official OGC document in order to have developers and organizations implement the Draft Standard and provide feedback." ;
    skos:inScheme <http://www.opengis.net/def/glossary> ;
    skos:prefLabel "Draft Standard" .

<http://www.opengis.net/def/glossary/term/EDP> a skos:Concept ;
    rdfs:label "European Data Portal" ;
    dcterms:created "2023-10-13T16:54:05.347054"^^xsd:dateTime ;
    rdfs:seeAlso <https://data.europa.eu/fi> ;
    skos:altLabel "EDP" ;
    skos:definition "European Data Portal (EDP) gathers Public Sector Information that can be freely reused for any purpose (i.e. Open Data) of European Member States and EFTA countries. On the portal, only metadata is shown, which is directly harvested from the existing portals with the aim of providing one single access point to all this data." ;
    skos:inScheme <http://www.opengis.net/def/glossary> ;
    skos:prefLabel "European Data Portal" .

<http://www.opengis.net/def/glossary/term/Encoding> a skos:Concept ;
    rdfs:label "Encoding" ;
    dcterms:created "2023-10-13T16:54:05.346774"^^xsd:dateTime ;
    rdfs:seeAlso <https://docs.ogc.org/pol/05-020r29/05-020r29.html#annex-a-terms-and-definitions> ;
    skos:definition "encodings provide the format (arrangement of data elements) and syntax of the data and messages, or data sent to and by a server" ;
    skos:inScheme <http://www.opengis.net/def/glossary> ;
    skos:prefLabel "Encoding" .

<http://www.opengis.net/def/glossary/term/ExtractTransformLoad> a skos:Concept ;
    rdfs:label "Extract-Transform-Load" ;
    dcterms:created "2023-10-13T16:54:05.346912"^^xsd:dateTime ;
    rdfs:seeAlso <https://en.wikipedia.org/wiki/Extract,_transform,_load> ;
    skos:altLabel "ETL" ;
    skos:definition "a data integration process that extracts (typically heterogenous) data from a multitude and variety of sources, combines and transforms the data into a single entity, and then loads the data into a database or other data repository." ;
    skos:inScheme <http://www.opengis.net/def/glossary> ;
    skos:prefLabel "Extract-Transform-Load" .

<http://www.opengis.net/def/glossary/term/FAIR> a skos:Concept ;
    rdfs:label "Findable, Accessible, Interoperable, Reusable" ;
    dcterms:created "2023-10-13T16:54:05.347198"^^xsd:dateTime ;
    rdfs:seeAlso <https://doi.org/10.1038/sdata.2016.18> ;
    skos:altLabel "FAIR" ;
    skos:definition "a set of principles that serve to guide data producers and publishers as they endevour to maximize the added-value gained by contemporary and formal digital publishing" ;
    skos:inScheme <http://www.opengis.net/def/glossary> ;
    skos:prefLabel "Findable, Accessible, Interoperable, Reusable" .

<http://www.opengis.net/def/glossary/term/HVD> a skos:Concept ;
    rdfs:label "High-Value Datasets" ;
    dcterms:created "2023-10-13T16:54:05.347325"^^xsd:dateTime ;
    rdfs:seeAlso <https://eur-lex.europa.eu/legal-content/EN/TXT/PDF/?uri=CELEX:32023R0138&from=EN> ;
    skos:definition "documents that are associated with important benefits for society, the environment and the economy, in particular because of their suitability for the creation of value-added services, applications, new, high-quality jobs, and of the number of potential beneficiaries of the value-added services and applications based on those datasets." ;
    skos:inScheme <http://www.opengis.net/def/glossary> ;
    skos:prefLabel "High-Value Datasets" .

<http://www.opengis.net/def/glossary/term/LandingPage> a skos:Concept ;
    rdfs:label "Landing page " ;
    dcterms:created "2023-10-13T16:54:05.347488"^^xsd:dateTime ;
    rdfs:seeAlso <https://docs.ogc.org/is/17-069r4/17-069r4.html> ;
    skos:definition "a web resource whose primary purpose is to contain a description of something else. " ;
    skos:inScheme <http://www.opengis.net/def/glossary> ;
    skos:prefLabel "Landing page " .

<http://www.opengis.net/def/glossary/term/OGCAPI> a skos:Concept ;
    rdfs:label "OGC API" ;
    dcterms:created "2023-10-13T16:54:05.347625"^^xsd:dateTime ;
    rdfs:seeAlso <https://docs.ogc.org/is/19-072/19-072.html> ;
    skos:altLabel "OGC Web API" ;
    skos:definition "a Web API that implements one or more Conformance Classes from an OGC API Standard." ;
    skos:inScheme <http://www.opengis.net/def/glossary> ;
    skos:prefLabel "OGC API" .

<http://www.opengis.net/def/glossary/term/OpenAPI> a skos:Concept ;
    rdfs:label "OpenAPI" ;
    dcterms:created "2023-10-13T16:54:05.347762"^^xsd:dateTime ;
    rdfs:seeAlso <https://spec.openapis.org/oas/v3.0.3> ;
    skos:altLabel "OAS" ;
    skos:definition "a specification of a standard, language-agnostic interface to RESTful APIs which allows both humans and computers to discover and understand the capabilities of the service without access to source code, documentation, or through network traffic inspection." ;
    skos:inScheme <http://www.opengis.net/def/glossary> ;
    skos:prefLabel "OpenAPI" .

<http://www.opengis.net/def/glossary/term/REST> a skos:Concept ;
    rdfs:label "Representational State Transfer" ;
    dcterms:created "2023-10-13T16:54:05.348145"^^xsd:dateTime ;
    rdfs:seeAlso <https://ics.uci.edu/~fielding/pubs/dissertation/rest_arch_style.htm> ;
    skos:altLabel "REST" ;
    skos:definition "The Representational State Transfer (REST) style is an abstraction of the architectural elements within a distributed hypermedia system. REST focuses on the roles of components, the constraints upon their interaction with other components, and their interpretation of significant data elements. It encompasses the fundamental constraints upon components, connectors, and data that define the basis of the Web architecture, and thus the essence of its behavior as a network-based application. An API that conforms to the REST architectural principles/constraints is called a RESTful API." ;
    skos:inScheme <http://www.opengis.net/def/glossary> ;
    skos:prefLabel "Representational State Transfer" .

<http://www.opengis.net/def/glossary/term/RESTfulArchitecture> a skos:Concept ;
    rdfs:label "RESTful architecture" ;
    dcterms:created "2023-10-13T16:54:05.348268"^^xsd:dateTime ;
    rdfs:seeAlso <https://ics.uci.edu/~fielding/pubs/dissertation/rest_arch_style.htm> ;
    skos:definition "an architecture that follows REST principles" ;
    skos:inScheme <http://www.opengis.net/def/glossary> ;
    skos:prefLabel "RESTful architecture" .

<http://www.opengis.net/def/glossary/term/Record> a skos:Concept ;
    rdfs:label "Record" ;
    dcterms:created "2023-10-13T16:54:05.347883"^^xsd:dateTime ;
    rdfs:seeAlso <https://docs.ogc.org/DRAFTS/20-004.html#record-def> ;
    skos:definition "atomic unit of information of a catalog that is used to provide information about a particular resource" ;
    skos:inScheme <http://www.opengis.net/def/glossary> ;
    skos:prefLabel "Record" .

<http://www.opengis.net/def/glossary/term/Resource> a skos:Concept ;
    rdfs:label "Resource" ;
    dcterms:created "2023-10-13T16:54:05.347998"^^xsd:dateTime ;
    rdfs:seeAlso <https://www.iso.org/obp/ui/#iso:std:iso:15836:-2:ed-1:v1:en:fn:3> ;
    skos:definition "entity that might be identified" ;
    skos:inScheme <http://www.opengis.net/def/glossary> ;
    skos:prefLabel "Resource" .

<http://www.opengis.net/def/glossary/term/Tile> a skos:Concept ;
    rdfs:label "Tile" ;
    dcterms:created "2023-10-13T16:54:05.348394"^^xsd:dateTime ;
    rdfs:seeAlso <https://docs.ogc.org/is/17-083r4/17-083r4.html> ;
    skos:definition "a geometric shape with known properties that may or may not be the result of a tiling (tessellation) process. A tile consists of a single connected “piece” without “holes” or “lines” (topological disc). " ;
    skos:inScheme <http://www.opengis.net/def/glossary> ;
    skos:prefLabel "Tile" .

<http://www.opengis.net/def/glossary/term/UML> a skos:Concept ;
    rdfs:label "Unified Modeling Language" ;
    dcterms:created "2023-10-13T16:54:05.348533"^^xsd:dateTime ;
    rdfs:seeAlso <https://www.omg.org/spec/UML/2.5.1/About-UML> ;
    skos:altLabel "UML" ;
    skos:definition "a specification defining a graphical language for visualizing, specifying, constructing, and documenting the artifacts of distributed object systems." ;
    skos:inScheme <http://www.opengis.net/def/glossary> ;
    skos:prefLabel "Unified Modeling Language" .

<http://www.opengis.net/def/glossary/term/URL> a skos:Concept ;
    rdfs:label "Uniform Resource Locator" ;
    dcterms:created "2023-10-13T16:54:05.348672"^^xsd:dateTime ;
    rdfs:seeAlso <https://datatracker.ietf.org/doc/html/rfc1738> ;
    skos:altLabel "URL" ;
    skos:definition "the syntax and semantics of formalized information for location and access of resources via the Internet." ;
    skos:inScheme <http://www.opengis.net/def/glossary> ;
    skos:prefLabel "Uniform Resource Locator" .

<http://www.opengis.net/def/glossary/term/YAML> a skos:Concept ;
    rdfs:label "YAML Ain't Markup Language" ;
    dcterms:created "2023-10-13T16:54:05.348824"^^xsd:dateTime ;
    rdfs:seeAlso <https://yaml.org/> ;
    skos:altLabel "YAML" ;
    skos:definition "A data serialization language" ;
    skos:inScheme <http://www.opengis.net/def/glossary> ;
    skos:prefLabel "YAML Ain't Markup Language" .

