@prefix dcterms: <http://purl.org/dc/terms/> .
@prefix ns1: <http://www.opengis.net/def/metamodel/ogc-na/> .
@prefix rdfs: <http://www.w3.org/2000/01/rdf-schema#> .
@prefix skos: <http://www.w3.org/2004/02/skos/core#> .
@prefix xsd: <http://www.w3.org/2001/XMLSchema#> .

<http://www.opengis.net/def/register/> skos:member <http://www.opengis.net/def/geotiff-tag/> .

<http://www.opengis.net/def/geotiff-tag> a skos:ConceptScheme ;
    rdfs:label "GeoTIFF Tag Register" ;
    <http://www.opengis.net/def/metamodel/ogc-na/status>
            <http://www.opengis.net/def/status/valid> ;
    ns1:collectionView <http://www.opengis.net/def/geotiff-tag/> ;
    skos:prefLabel "GeoTIFF Tag Register" .

<http://www.opengis.net/def/geotiff-tag/ogc/1.1/33550> a skos:Concept ;
    rdfs:label "ModelPixelScaleTag" ;
    <http://www.opengis.net/def/metamodel/ogc-na/status>
            <http://www.opengis.net/def/status/valid> ;
    dcterms:created "2021-02-16T12:27:08.804790"^^xsd:dateTime ;
    rdfs:seeAlso <http://docs.opengeospatial.org/is/19-008r4/19-008r4.html#_requirements_class_modelpixelscaletag> ;
    skos:definition "The ModelPixelScaleTag may be used to specify the size of raster pixel spacing in the model space units when the raster space can be embedded in the model space coordinate reference system without rotation" ;
    skos:notation "33550"^^<http://www.opengis.net/def/encoding/ogc/geotiff> ;
    skos:inScheme <http://www.opengis.net/def/geotiff-tag> ;
    skos:prefLabel "ModelPixelScaleTag" .

<http://www.opengis.net/def/geotiff-tag/ogc/1.1/33922> a skos:Concept ;
    rdfs:label "ModelTiepointTag" ;
    <http://www.opengis.net/def/metamodel/ogc-na/status>
            <http://www.opengis.net/def/status/valid> ;
    dcterms:created "2021-02-16T12:27:08.805167"^^xsd:dateTime ;
    rdfs:seeAlso <http://docs.opengeospatial.org/is/19-008r4/19-008r4.html#_requirements_class_modeltiepointtag> ;
    skos:definition "The ModelTiepointTag may be used to help define the transformation between raster space and model space through a set of raster-to-model tiepoints and scaling parameters" ;
    skos:notation "33922"^^<http://www.opengis.net/def/encoding/ogc/geotiff> ;
    skos:inScheme <http://www.opengis.net/def/geotiff-tag> ;
    skos:prefLabel "ModelTiepointTag" .

<http://www.opengis.net/def/geotiff-tag/ogc/1.1/34264> a skos:Concept ;
    rdfs:label "ModelTransformationTag" ;
    <http://www.opengis.net/def/metamodel/ogc-na/status>
            <http://www.opengis.net/def/status/valid> ;
    dcterms:created "2021-02-16T12:27:08.805526"^^xsd:dateTime ;
    rdfs:seeAlso <http://docs.opengeospatial.org/is/19-008r4/19-008r4.html#_requirements_class_modeltransformationtag> ;
    skos:definition "The ModelTransformationTag may be used to specify the transformation matrix between the raster space (and its dependent pixel-value space) and the (possibly 3D) model space" ;
    skos:notation "34264"^^<http://www.opengis.net/def/encoding/ogc/geotiff> ;
    skos:inScheme <http://www.opengis.net/def/geotiff-tag> ;
    skos:prefLabel "ModelTransformationTag" .

<http://www.opengis.net/def/geotiff-tag/ogc/1.1/34735> a skos:Concept ;
    rdfs:label "GeoKeyDirectoryTag" ;
    <http://www.opengis.net/def/metamodel/ogc-na/status>
            <http://www.opengis.net/def/status/valid> ;
    dcterms:created "2021-02-16T12:27:08.805882"^^xsd:dateTime ;
    rdfs:seeAlso <http://docs.opengeospatial.org/is/19-008r4/19-008r4.html#_requirements_class_geokeydirectorytag> ;
    skos:definition "The Keys in GeoTIFF (also called 'GeoKeys') are all referenced from the GeoKeyDirectoryTag tag" ;
    skos:notation "34735"^^<http://www.opengis.net/def/encoding/ogc/geotiff> ;
    skos:inScheme <http://www.opengis.net/def/geotiff-tag> ;
    skos:prefLabel "GeoKeyDirectoryTag" .

<http://www.opengis.net/def/geotiff-tag/ogc/1.1/34736> a skos:Concept ;
    rdfs:label "GeoDoubleParamsTag" ;
    <http://www.opengis.net/def/metamodel/ogc-na/status>
            <http://www.opengis.net/def/status/valid> ;
    dcterms:created "2021-02-16T12:27:08.806240"^^xsd:dateTime ;
    rdfs:seeAlso <http://docs.opengeospatial.org/is/19-008r4/19-008r4.html#_requirements_class_geodoubleparamstag> ;
    skos:definition "The GeoDoubleParamsTag supports the storage of parameter values when the values are of type Double" ;
    skos:notation "34736"^^<http://www.opengis.net/def/encoding/ogc/geotiff> ;
    skos:inScheme <http://www.opengis.net/def/geotiff-tag> ;
    skos:prefLabel "GeoDoubleParamsTag" .

<http://www.opengis.net/def/geotiff-tag/ogc/1.1/34737> a skos:Concept ;
    rdfs:label "GeoAsciiParamsTag" ;
    <http://www.opengis.net/def/metamodel/ogc-na/status>
            <http://www.opengis.net/def/status/valid> ;
    dcterms:created "2021-02-16T12:27:08.806592"^^xsd:dateTime ;
    rdfs:seeAlso <http://docs.opengeospatial.org/is/19-008r4/19-008r4.html#_requirements_class_geoasciiparamstag> ;
    skos:definition "The GeoAsciiParamsTag supports the storage of parameter values when the values are of type ASCII" ;
    skos:notation "34737"^^<http://www.opengis.net/def/encoding/ogc/geotiff> ;
    skos:inScheme <http://www.opengis.net/def/geotiff-tag> ;
    skos:prefLabel "GeoAsciiParamsTag" .

<http://www.opengis.net/def/geotiff-tag/dgiwg/2.3/50909> a skos:Concept ;
    rdfs:label "GEO_METADATA Tag" ;
    <http://www.opengis.net/def/metamodel/ogc-na/status>
            <http://www.opengis.net/def/status/valid> ;
    dcterms:created "2021-10-14T12:25:01.803240"^^xsd:dateTime ;
    rdfs:seeAlso <https://portal.ogc.org/files/95763> ;
    skos:definition "This tag may be used for embedding XML-encoded instance documents prepared using 19139-based schema. Note that the type is BYTE instead of ASCII because metadata may contain UTF-8 characters." ;
    skos:notation "50909"^^<http://www.opengis.net/def/encoding/ogc/geotiff> ;
    skos:inScheme <http://www.opengis.net/def/geotiff-tag> ;
    skos:prefLabel "GEO_METADATA Tag" .


<http://www.opengis.net/def/geotiff-tag/dgiwg/2.3/50908> a skos:Concept ;
    rdfs:label "TIFF_RSID Tag" ;
    <http://www.opengis.net/def/metamodel/ogc-na/status>
            <http://www.opengis.net/def/status/valid> ;
    dcterms:created "2021-10-14T12:25:02.503220"^^xsd:dateTime ;
    rdfs:seeAlso <https://portal.ogc.org/files/95763> ;
    skos:definition "This tag specifies a File Universal Unique Identifier or RSID according to DGIWG DMF (DGIWG Metadata Foundation) definition." ;
    skos:notation "50908"^^<http://www.opengis.net/def/encoding/ogc/geotiff> ;
    skos:inScheme <http://www.opengis.net/def/geotiff-tag> ;
    skos:prefLabel "TIFF_RSID Tag" .

<http://www.opengis.net/def/geotiff-tag/> a skos:Collection ;
    rdfs:label "GeoTIFF Tag Register" ;
    <http://www.opengis.net/def/metamodel/ogc-na/status>
            <http://www.opengis.net/def/status/valid> ;
    skos:inScheme <http://www.opengis.net/def/geotiff-tag> ;
    skos:member <http://www.opengis.net/def/geotiff-tag/ogc/1.1/33550>,
        <http://www.opengis.net/def/geotiff-tag/ogc/1.1/33922>,
        <http://www.opengis.net/def/geotiff-tag/ogc/1.1/34264>,
        <http://www.opengis.net/def/geotiff-tag/ogc/1.1/34735>,
        <http://www.opengis.net/def/geotiff-tag/ogc/1.1/34736>,
        <http://www.opengis.net/def/geotiff-tag/ogc/1.1/34737>,
        <http://www.opengis.net/def/geotiff-tag/dgiwg/2.3/50909>,
        <http://www.opengis.net/def/geotiff-tag/dgiwg/2.3/50908>;
    skos:prefLabel "GeoTIFF Tag Register" .
