@prefix dcterms: <http://purl.org/dc/terms/> .
@prefix rdfs: <http://www.w3.org/2000/01/rdf-schema#> .
@prefix skos: <http://www.w3.org/2004/02/skos/core#> .
@prefix xsd: <http://www.w3.org/2001/XMLSchema#> .

<http://www.opengis.net/def/ogc/> skos:member <http://www.opengis.net/def/profile/ogc/2.0/gml-sf/> .

<http://www.opengis.net/def/profile/ogc/2.0/gml-sf> a skos:ConceptScheme ;
    rdfs:label "Levels of the Geography Markup Language (GML) simple features profile" ;
    <http://www.opengis.net/def/metamodel/ogc-na/status>
            <http://www.opengis.net/def/status/valid> ;
    ns1:collectionView <http://www.opengis.net/def/profile/ogc/2.0/gml-sf/> ;
    skos:prefLabel "Levels of the Geography Markup Language (GML) simple features profile" .

<http://www.opengis.net/def/profile/ogc/2.0/gml-sf0> a skos:Concept ;
    rdfs:label "Geography Markup Language (GML) Simple Features Compliance Level SF-0" ;
    <http://www.opengis.net/def/metamodel/ogc-na/status>
            <http://www.opengis.net/def/status/valid> ;
    dcterms:created "2021-04-28T16:23:42.732904"^^xsd:dateTime ;
    rdfs:seeAlso <https://portal.ogc.org/files/?artifact_id=42729> ;
    skos:definition "Compliance level SF-0 limits the property types of both spatial and non-spatial properties." ;
    skos:notation "gml-sf0"^^<http://www.opengis.net/def/encoding/ogc/gml> ;
    skos:prefLabel "Geography Markup Language (GML) Simple Features Compliance Level SF-0" .

<http://www.opengis.net/def/profile/ogc/2.0/gml-sf1> a skos:Concept ;
    rdfs:label "Geography Markup Language (GML) Simple Features Compliance Level SF-1" ;
    <http://www.opengis.net/def/metamodel/ogc-na/status>
            <http://www.opengis.net/def/status/valid> ;
    dcterms:created "2021-04-28T16:23:42.733243"^^xsd:dateTime ;
    rdfs:seeAlso <https://portal.ogc.org/files/?artifact_id=42729> ;
    skos:definition "Compliance level SF-1 supports everything in compliance level SF-0 but removes the restriction on value cardinality and allows user defined non-spatial property types to be used." ;
    skos:notation "gml-sf1"^^<http://www.opengis.net/def/encoding/ogc/gml> ;
    skos:prefLabel "Geography Markup Language (GML) Simple Features Compliance Level SF-1" .

<http://www.opengis.net/def/profile/ogc/2.0/gml-sf2> a skos:Concept ;
    rdfs:label "Geography Markup Language (GML) Simple Features Compliance Level SF-2" ;
    <http://www.opengis.net/def/metamodel/ogc-na/status>
            <http://www.opengis.net/def/status/valid> ;
    dcterms:created "2021-04-28T16:23:42.733569"^^xsd:dateTime ;
    rdfs:seeAlso <https://portal.ogc.org/files/?artifact_id=42729> ;
    skos:definition "Compliance level SF-2 essentially corresponds to the OGC Simple Features specification. There are no restrictions placed on non-spatial properties but there are restrictions on spatial properties." ;
    skos:notation "gml-sf2"^^<http://www.opengis.net/def/encoding/ogc/gml> ;
    skos:prefLabel "Geography Markup Language (GML) Simple Features Compliance Level SF-2" .

<http://www.opengis.net/def/profile/ogc/2.0/gml-sf/> a skos:Collection ;
    rdfs:label "Levels of the Geography Markup Language (GML) simple features profile" ;
    <http://www.opengis.net/def/metamodel/ogc-na/status>
            <http://www.opengis.net/def/status/valid> ;      
    skos:inScheme <http://www.opengis.net/def/profile/ogc/2.0/gml-sf> ;
    skos:member <http://www.opengis.net/def/profile/ogc/2.0/gml-sf0>,
        <http://www.opengis.net/def/profile/ogc/2.0/gml-sf1>,
        <http://www.opengis.net/def/profile/ogc/2.0/gml-sf2> ;
    skos:prefLabel "Levels of the Geography Markup Language (GML) simple features profile" .
