@prefix dcterms: <http://purl.org/dc/terms/> .
@prefix ns1: <http://www.opengis.net/def/metamodel/ogc-na/> .
@prefix rdfs: <http://www.w3.org/2000/01/rdf-schema#> .
@prefix skos: <http://www.w3.org/2004/02/skos/core#> .
@prefix xsd: <http://www.w3.org/2001/XMLSchema#> .

<http://www.opengis.net/def/register/> skos:member <https://www.opengis.net/def/dggrs/> .

<https://www.opengis.net/def/dggrs/OGC/1.0/GNOSISGlobalGrid> a skos:Concept ;
    rdfs:label "GNOSISGlobalGrid" ;
    dcterms:created "2026-02-02T18:20:15.417809"^^xsd:dateTime ;
    rdfs:seeAlso <https://raw.githubusercontent.com/opengeospatial/ogcapi-discrete-global-grid-systems/refs/heads/master/registry/dggrs/OGC/1.0/GNOSISGlobalGrid.json> ;
    skos:definition "A Discrete Global Grid Reference System based on the GNOSIS Global Grid 2D Tile Matrix Set, a {hexLevel}-{hexRow}-{hexCol} indexing system, and scanline-based sub-zone ordering. Making use of variable matrix widths, zones are divided by 4, unless they touch the pole, in which case the half touching the pole is not split longitude-wise. The error budget is ~-25.8/+66.0% from mean zone size (+/- 45.9% from median) up to level 25 (~849 cm² mean zones)." ;
    skos:inScheme <https://www.opengis.net/def/dggrs> ;
    skos:prefLabel "GNOSISGlobalGrid" .

<https://www.opengis.net/def/dggrs/OGC/1.0/HEALPix> a skos:Concept ;
    rdfs:label "HEALPix" ;
    dcterms:created "2026-02-02T18:20:15.418566"^^xsd:dateTime ;
    rdfs:seeAlso <https://raw.githubusercontent.com/opengeospatial/ogcapi-discrete-global-grid-systems/refs/heads/master/registry/dggrs/OGC/1.0/HEALPix.json> ;
    skos:definition "A HEALPix Discrete Global Grid Reference System using a refinement ratio of 4, a 0° East prime meridian, the WGS84 ellipsoid model, grid configuration Nφ (H) = 4, Nθ (K) = 3, indexing based on 12 root rhombuses numbered 0 to B (hex) from West to East, North to South, and a hexadecimal sub-index in row-major, bottom-left to top-right, top-left to bottom-right scanlines, with sub-zone order also based on the same scanlines." ;
    skos:inScheme <https://www.opengis.net/def/dggrs> ;
    skos:prefLabel "HEALPix" .

<https://www.opengis.net/def/dggrs/OGC/1.0/ISEA3H> a skos:Concept ;
    rdfs:label "ISEA3H" ;
    dcterms:created "2026-02-02T18:20:15.419110"^^xsd:dateTime ;
    rdfs:seeAlso <https://raw.githubusercontent.com/opengeospatial/ogcapi-discrete-global-grid-systems/refs/heads/master/registry/dggrs/OGC/1.0/ISEA3H.json> ;
    skos:definition "An ISEA3H Discrete Global Grid Reference System using an ISEA orientation symmetric about the equator with a single vertex on land, and WGS84 authalic sphere (a WGS84 geodetic latitude is mapped to the sphere by converting it to an authalic latitude), a zone indexing system based on an ISEA9R, and a scanline-based sub-zone ordering" ;
    skos:inScheme <https://www.opengis.net/def/dggrs> ;
    skos:prefLabel "ISEA3H" .

<https://www.opengis.net/def/dggrs/OGC/1.0/ISEA7H> a skos:Concept ;
    rdfs:label "ISEA7H" ;
    dcterms:created "2026-02-02T18:20:15.419760"^^xsd:dateTime ;
    rdfs:seeAlso <https://raw.githubusercontent.com/opengeospatial/ogcapi-discrete-global-grid-systems/refs/heads/master/registry/dggrs/OGC/1.0/ISEA7H.json> ;
    skos:definition "An ISEA7H Discrete Global Grid Reference System using an orientation symmetric about the equator with a single vertex on land, and WGS84 authalic sphere (a WGS84 geodetic latitude is mapped to the sphere by converting it to an authalic latitude), a zone indexing system based on dividing root rhombuses into 7^(level/2)^2 sub-rhombuses for even levels, and a scanline-based sub-zone ordering" ;
    skos:inScheme <https://www.opengis.net/def/dggrs> ;
    skos:prefLabel "ISEA7H" .

<https://www.opengis.net/def/dggrs/OGC/1.0/ISEA9R> a skos:Concept ;
    rdfs:label "ISEA9R" ;
    dcterms:created "2026-02-02T18:20:15.419510"^^xsd:dateTime ;
    rdfs:seeAlso <https://raw.githubusercontent.com/opengeospatial/ogcapi-discrete-global-grid-systems/refs/heads/master/registry/dggrs/OGC/1.0/ISEA9R.json> ;
    skos:definition "An ISEA9R Discrete Global Grid Reference System using an ISEA orientation symmetric about the equator with a single vertex on land, and WGS84 authalic sphere (a WGS84 geodetic latitude is mapped to the sphere by converting it to an authalic latitude), a {level}{rootRhombus}-{hexSubZone} indexing system, and scanline-based sub-zone ordering. The ten root rhombuses are formed by combining two icosahedron triangles at their base. Depending on whether the ISEA planar CRS is rotated, sheared and scaled or not, the geometries of the zones are either squares or rhombuses, and the zone edges are either axis-aligned, or the angles and distances are preserved. In either case, the topology, indexing and surface geometry on the Earth model remains the same. The ISEA9R DGGH is a dual of the ISEA3H DGGH even levels (a vertex/node in ISEA9R is the centroid of an ISEA3H zone)." ;
    skos:inScheme <https://www.opengis.net/def/dggrs> ;
    skos:prefLabel "ISEA9R" .

<https://www.opengis.net/def/dggrs/OGC/1.0/IVEA3H> a skos:Concept ;
    rdfs:label "IVEA3H" ;
    dcterms:created "2026-02-02T18:20:15.418461"^^xsd:dateTime ;
    rdfs:seeAlso <https://raw.githubusercontent.com/opengeospatial/ogcapi-discrete-global-grid-systems/refs/heads/master/registry/dggrs/OGC/1.0/IVEA3H.json> ;
    skos:definition "An IVEA3H Discrete Global Grid Reference System using the Icosahedral Vertex-oriented Equal-Area (IVEA) projection as described in the 2006 'Slice & Dice' publication (equivalent to applying the 1992 Snyder polyhedral projection to the dodecahedron when considering the barycentric coordinates within the projection of the spherical disdyakis triacontahedron triangles constituting full spherical icosahedral symmetry), an orientation symmetric about the equator with a single vertex on land, and WGS84 authalic sphere (a WGS84 geodetic latitude is mapped to the sphere by converting it to an authalic latitude), a zone indexing system based on an IVEA9R, and a scanline-based sub-zone ordering" ;
    skos:inScheme <https://www.opengis.net/def/dggrs> ;
    skos:prefLabel "IVEA3H" .

<https://www.opengis.net/def/dggrs/OGC/1.0/IVEA7H> a skos:Concept ;
    rdfs:label "IVEA7H" ;
    dcterms:created "2026-02-02T18:20:15.419010"^^xsd:dateTime ;
    rdfs:seeAlso <https://raw.githubusercontent.com/opengeospatial/ogcapi-discrete-global-grid-systems/refs/heads/master/registry/dggrs/OGC/1.0/IVEA7H.json> ;
    skos:definition "An IVEA7H Discrete Global Grid Reference System using the Icosahedral Vertex-oriented Equal-Area (IVEA) projection as described in the 2006 'Slice & Dice' publication (equivalent to applying the 1992 Snyder polyhedral projection to the dodecahedron when considering the barycentric coordinates within the projection of the spherical disdyakis triacontahedron triangles constituting full spherical icosahedral symmetry), an orientation symmetric about the equator with a single vertex on land, and WGS84 authalic sphere (a WGS84 geodetic latitude is mapped to the sphere by converting it to an authalic latitude), a zone indexing system based on dividing root rhombuses into 7^(level/2)^2 sub-rhombuses for even levels, and a scanline-based sub-zone ordering" ;
    skos:inScheme <https://www.opengis.net/def/dggrs> ;
    skos:prefLabel "IVEA7H" .

<https://www.opengis.net/def/dggrs/OGC/1.0/IVEA9R> a skos:Concept ;
    rdfs:label "IVEA9R" ;
    dcterms:created "2026-02-02T18:20:15.418777"^^xsd:dateTime ;
    rdfs:seeAlso <https://raw.githubusercontent.com/opengeospatial/ogcapi-discrete-global-grid-systems/refs/heads/master/registry/dggrs/OGC/1.0/IVEA9R.json> ;
    skos:definition "An IVEA9R Discrete Global Grid Reference System using the Icosahedral Vertex-oriented Equal-Area (IVEA) projection as described in the 2006 'Slice & Dice' publication (equivalent to applying the 1992 Snyder polyhedral projection to the dodecahedron when considering the barycentric coordinates within the projection of the spherical disdyakis triacontahedron triangles constituting full spherical icosahedral symmetry), an orientation symmetric about the equator with a single vertex on land, and WGS84 authalic sphere (a WGS84 geodetic latitude is mapped to the sphere by converting it to an authalic latitude), a {level}{rootRhombus}-{hexSubZone} indexing system, and scanline-based sub-zone ordering. The ten root rhombuses are formed by combining two icosahedron triangles at their base. Depending on whether the IVEA planar CRS is rotated, sheared and scaled or not, the geometries of the zones are either squares or rhombuses, and the zone edges are either axis-aligned, or the angles and distances are preserved. In either case, the topology, indexing and surface geometry on the Earth model remains the same. The IVEA9R DGGH is a dual of the IVEA3H DGGH even levels (a vertex/node in IVEA9R is the centroid of an IVEA3H zone)." ;
    skos:inScheme <https://www.opengis.net/def/dggrs> ;
    skos:prefLabel "IVEA9R" .

<https://www.opengis.net/def/dggrs/OGC/1.0/rHEALPix> a skos:Concept ;
    rdfs:label "rHEALPix" ;
    dcterms:created "2026-02-02T18:20:15.418224"^^xsd:dateTime ;
    rdfs:seeAlso <https://raw.githubusercontent.com/opengeospatial/ogcapi-discrete-global-grid-systems/refs/heads/master/registry/dggrs/OGC/1.0/rHEALPix.json> ;
    skos:definition "An rHEALPix Discrete Global Grid Reference System using a refinement ratio of 9, a 50° East prime meridian, the WGS84 ellipsoid model, hierarchical indexing with level 0 zones named N,O,P,Q,R,S and further refined zones adding numbers 0-8, and a sub-zone ordering using non-hierarchical row-major, top-to-bottom, left-to-right scanlines." ;
    skos:inScheme <https://www.opengis.net/def/dggrs> ;
    skos:prefLabel "rHEALPix" .

<https://www.opengis.net/def/dggrs/> a skos:Collection ;
    rdfs:label "DGGRS Register" ;
    skos:inScheme <https://www.opengis.net/def/dggrs> ;
    skos:member <https://www.opengis.net/def/dggrs/OGC/1.0/GNOSISGlobalGrid>,
        <https://www.opengis.net/def/dggrs/OGC/1.0/HEALPix>,
        <https://www.opengis.net/def/dggrs/OGC/1.0/ISEA3H>,
        <https://www.opengis.net/def/dggrs/OGC/1.0/ISEA7H>,
        <https://www.opengis.net/def/dggrs/OGC/1.0/ISEA9R>,
        <https://www.opengis.net/def/dggrs/OGC/1.0/IVEA3H>,
        <https://www.opengis.net/def/dggrs/OGC/1.0/IVEA7H>,
        <https://www.opengis.net/def/dggrs/OGC/1.0/IVEA9R>,
        <https://www.opengis.net/def/dggrs/OGC/1.0/rHEALPix> ;
    skos:prefLabel "DGGRS Register" .

<https://www.opengis.net/def/dggrs> a skos:ConceptScheme ;
    rdfs:label "DGGRS Register" ;
    ns1:collectionView <https://www.opengis.net/def/dggrs/> ;
    skos:prefLabel "DGGRS Register" .

