@prefix adms: <http://www.w3.org/ns/adms#> .
@prefix dcat: <http://www.w3.org/ns/dcat#> .
@prefix dct: <http://purl.org/dc/terms/> .
@prefix na: <http://www.opengis.net/def/metamodel/ogc-na/> .
@prefix ogcdt: <http://www.opengis.net/def/doc-type/> .
@prefix owl: <http://www.w3.org/2002/07/owl#> .
@prefix reg: <http://purl.org/linked-data/registry#> .
@prefix skos: <http://www.w3.org/2004/02/skos/core#> .
@prefix spec: <http://www.opengis.net/def/ont/modspec/> .
@prefix specrel: <http://www.opengis.net/def/ont/specrel/> .
@prefix xsd: <http://www.w3.org/2001/XMLSchema#> .
@prefix dcterms: <http://purl.org/dc/terms/> .

<http://www.opengis.net/spec/docs/20-082r2-anno> a owl:Ontology .



<http://www.opengis.net/def/docs/20-082r2> a spec:Specification ;
    dcterms:creator "Kathi Schleidt" ;
    dcterms:dateAccepted "2099-08-02"^^xsd:date ;
    dcterms:dateSubmitted "2021-07-08"^^xsd:date ;
    dcterms:identifier "http://www.opengis.net/doc/is/OMS/3.0" ;
    reg:status reg:statusValid ;
    na:doctype ogcdt:ip ;
    spec:authority "Open Geospatial Consortium" ;
    spec:class <http://www.opengis.net/spec/OMS/3.0/conf/obs-basic>,
		<http://www.opengis.net/spec/OMS/3.0/conf/obs-basic/Deployment>,
		<http://www.opengis.net/spec/OMS/3.0/conf/obs-basic/GenericDomainFeature>,
		<http://www.opengis.net/spec/OMS/3.0/conf/obs-basic/Host>,
		<http://www.opengis.net/spec/OMS/3.0/conf/obs-basic/ObservableProperty>,
		<http://www.opengis.net/spec/OMS/3.0/conf/obs-basic/Observation>,
		<http://www.opengis.net/spec/OMS/3.0/conf/obs-basic/ObservationCharacteristics>,
		<http://www.opengis.net/spec/OMS/3.0/conf/obs-basic/ObservationCollection>,
		<http://www.opengis.net/spec/OMS/3.0/conf/obs-basic/Observer>,
		<http://www.opengis.net/spec/OMS/3.0/conf/obs-basic/ObservingCapability>,
		<http://www.opengis.net/spec/OMS/3.0/conf/obs-basic/ObservingProcedure>,
		<http://www.opengis.net/spec/OMS/3.0/conf/obs-core>,
		<http://www.opengis.net/spec/OMS/3.0/conf/obs-core/AbstractDeployment>,
		<http://www.opengis.net/spec/OMS/3.0/conf/obs-core/AbstractHost>,
		<http://www.opengis.net/spec/OMS/3.0/conf/obs-core/AbstractObservableProperty>,
		<http://www.opengis.net/spec/OMS/3.0/conf/obs-core/AbstractObservation>,
		<http://www.opengis.net/spec/OMS/3.0/conf/obs-core/AbstractObservationCharacteristics>,
		<http://www.opengis.net/spec/OMS/3.0/conf/obs-core/AbstractObserver>,
		<http://www.opengis.net/spec/OMS/3.0/conf/obs-core/AbstractObservingProcedure>,
		<http://www.opengis.net/spec/OMS/3.0/conf/obs-core/NamedValue>,
		<http://www.opengis.net/spec/OMS/3.0/conf/obs-cpt>,
		<http://www.opengis.net/spec/OMS/3.0/conf/obs-cpt/Deployment>,
		<http://www.opengis.net/spec/OMS/3.0/conf/obs-cpt/Host>,
		<http://www.opengis.net/spec/OMS/3.0/conf/obs-cpt/ObservableProperty>,
		<http://www.opengis.net/spec/OMS/3.0/conf/obs-cpt/Observation>,
		<http://www.opengis.net/spec/OMS/3.0/conf/obs-cpt/Observer>,
		<http://www.opengis.net/spec/OMS/3.0/conf/obs-cpt/ObservingProcedure>,
		<http://www.opengis.net/spec/OMS/3.0/conf/obs-cpt/Procedure>,
		<http://www.opengis.net/spec/OMS/3.0/conf/sam-basic>,
		<http://www.opengis.net/spec/OMS/3.0/conf/sam-basic/MaterialSample>,
		<http://www.opengis.net/spec/OMS/3.0/conf/sam-basic/NamedLocation>,
		<http://www.opengis.net/spec/OMS/3.0/conf/sam-basic/PhysicalDimension>,
		<http://www.opengis.net/spec/OMS/3.0/conf/sam-basic/Sample>,
		<http://www.opengis.net/spec/OMS/3.0/conf/sam-basic/SampleCollection>,
		<http://www.opengis.net/spec/OMS/3.0/conf/sam-basic/Sampler>,
		<http://www.opengis.net/spec/OMS/3.0/conf/sam-basic/Sampling>,
		<http://www.opengis.net/spec/OMS/3.0/conf/sam-basic/SpatialSample>,
		<http://www.opengis.net/spec/OMS/3.0/conf/sam-basic/StatisticalClassification>,
		<http://www.opengis.net/spec/OMS/3.0/conf/sam-basic/StatisticalSample>,
		<http://www.opengis.net/spec/OMS/3.0/conf/sam-core>,
		<http://www.opengis.net/spec/OMS/3.0/conf/sam-core/AbstractPreparationProcedure>,
		<http://www.opengis.net/spec/OMS/3.0/conf/sam-core/AbstractPreparationStep>,
		<http://www.opengis.net/spec/OMS/3.0/conf/sam-core/AbstractSample>,
		<http://www.opengis.net/spec/OMS/3.0/conf/sam-core/AbstractSampler>,
		<http://www.opengis.net/spec/OMS/3.0/conf/sam-core/AbstractSampling>,
		<http://www.opengis.net/spec/OMS/3.0/conf/sam-core/AbstractSamplingProcedure>,
		<http://www.opengis.net/spec/OMS/3.0/conf/sam-cpt>,
		<http://www.opengis.net/spec/OMS/3.0/conf/sam-cpt/PreparationProcedure>,
		<http://www.opengis.net/spec/OMS/3.0/conf/sam-cpt/PreparationStep>,
		<http://www.opengis.net/spec/OMS/3.0/conf/sam-cpt/Sample>,
		<http://www.opengis.net/spec/OMS/3.0/conf/sam-cpt/Sampler>,
		<http://www.opengis.net/spec/OMS/3.0/conf/sam-cpt/Sampling>,
		<http://www.opengis.net/spec/OMS/3.0/conf/sam-cpt/SamplingProcedure> ;
    spec:date "2021-12-20"^^xsd:date ;
    specrel:implementation <http://www.opengis.net/def/docs/20-082r2> ;
    skos:notation "20-082r2"^^na:doc_no ;
    skos:prefLabel "OGCÂ® Abstract Specification Topic 20 - Observations and measurements" ;
    adms:version "3.0" ;
    dcat:landingPage <http://docs.opengeospatial.org/is/20-082r2/20-082r2.html> .

<http://www.opengis.net/spec/OMS/3.0/conf/obs-basic/GenericDomainFeature/GenericDomainFeature-sem> a spec:ConformanceTest,
        skos:Concept ;
    spec:method "Inspect the documentation of the application, schema or profile." ;
    spec:purpose "Verify that all requirements from the requirements class have been fulfilled." ;
    spec:requirement <http://www.opengis.net/spec/OMS/3.0/req/obs-basic/GenericDomainFeature/GenericDomainFeature-sem> ;
    spec:testType spec:Capabilities ;
    skos:broader <http://www.opengis.net/spec/OMS/3.0/conf/obs-basic/GenericDomainFeature> ;
    skos:definition "Verify that all requirements from the requirements class have been fulfilled." ;
    skos:inScheme <http://www.opengis.net/spec/OMS/3.0> ;
    skos:prefLabel "Conformance Test http://www.opengis.net/spec/OMS/3.0/req/obs-basic/GenericDomainFeature/GenericDomainFeature-sem" .

<http://www.opengis.net/spec/OMS/3.0/conf/obs-basic/ObservationCollection/AbstractObservationCollectionTypeCodeListValue-sem> a spec:ConformanceTest,
        skos:Concept ;
    spec:method "Inspect the documentation of the application, schema or profile." ;
    spec:purpose "Verify that all requirements from the requirements class have been fulfilled." ;
    spec:requirement <http://www.opengis.net/spec/OMS/3.0/req/obs-basic/ObservationCollection/AbstractObservationCollectionTypeCodeListValue-sem> ;
    spec:testType spec:Capabilities ;
    skos:definition "Verify that all requirements from the requirements class have been fulfilled." ;
    skos:inScheme <http://www.opengis.net/spec/OMS/3.0> ;
    skos:prefLabel "Conformance Test http://www.opengis.net/spec/OMS/3.0/req/obs-basic/ObservationCollection/AbstractObservationCollectionTypeCodeListValue-sem" .

<http://www.opengis.net/spec/OMS/3.0/conf/obs-basic/ObservationCollection/CollectionTypeByMemberCharacteristicsSemantics-sem> a spec:ConformanceTest,
        skos:Concept ;
    spec:method "Inspect the documentation of the application, schema or profile." ;
    spec:purpose "Verify that all requirements from the requirements class have been fulfilled." ;
    spec:requirement <http://www.opengis.net/spec/OMS/3.0/req/obs-basic/ObservationCollection/CollectionTypeByMemberCharacteristicsSemantics-sem> ;
    spec:testType spec:Capabilities ;
    skos:broader <http://www.opengis.net/spec/OMS/3.0/conf/obs-basic/ObservationCollection> ;
    skos:definition "Verify that all requirements from the requirements class have been fulfilled." ;
    skos:inScheme <http://www.opengis.net/spec/OMS/3.0> ;
    skos:prefLabel "Conformance Test http://www.opengis.net/spec/OMS/3.0/req/obs-basic/ObservationCollection/CollectionTypeByMemberCharacteristicsSemantics-sem" .

<http://www.opengis.net/spec/OMS/3.0/conf/obs-basic/ObservationCollection/ObservationCollection-sem> a spec:ConformanceTest,
        skos:Concept ;
    spec:method "Inspect the documentation of the application, schema or profile." ;
    spec:purpose "Verify that all requirements from the requirements class have been fulfilled." ;
    spec:requirement <http://www.opengis.net/spec/OMS/3.0/req/obs-basic/ObservationCollection/ObservationCollection-sem> ;
    spec:testType spec:Capabilities ;
    skos:broader <http://www.opengis.net/spec/OMS/3.0/conf/obs-basic/ObservationCollection> ;
    skos:definition "Verify that all requirements from the requirements class have been fulfilled." ;
    skos:inScheme <http://www.opengis.net/spec/OMS/3.0> ;
    skos:prefLabel "Conformance Test http://www.opengis.net/spec/OMS/3.0/req/obs-basic/ObservationCollection/ObservationCollection-sem" .

<http://www.opengis.net/spec/OMS/3.0/conf/obs-basic/ObservationCollection/collectionType-homogenous-con> a spec:ConformanceTest,
        skos:Concept ;
    spec:method "Inspect the documentation of the application, schema or profile." ;
    spec:purpose "Verify that all requirements from the requirements class have been fulfilled." ;
    spec:requirement <http://www.opengis.net/spec/OMS/3.0/req/obs-basic/ObservationCollection/collectionType-homogenous-con> ;
    spec:testType spec:Capabilities ;
    skos:broader <http://www.opengis.net/spec/OMS/3.0/conf/obs-basic/ObservationCollection> ;
    skos:definition "Verify that all requirements from the requirements class have been fulfilled." ;
    skos:inScheme <http://www.opengis.net/spec/OMS/3.0> ;
    skos:prefLabel "Conformance Test http://www.opengis.net/spec/OMS/3.0/req/obs-basic/ObservationCollection/collectionType-homogenous-con" .

<http://www.opengis.net/spec/OMS/3.0/conf/obs-basic/ObservationCollection/collectionType-sem> a spec:ConformanceTest,
        skos:Concept ;
    spec:method "Inspect the documentation of the application, schema or profile." ;
    spec:purpose "Verify that all requirements from the requirements class have been fulfilled." ;
    spec:requirement <http://www.opengis.net/spec/OMS/3.0/req/obs-basic/ObservationCollection/collectionType-sem> ;
    spec:testType spec:Capabilities ;
    skos:broader <http://www.opengis.net/spec/OMS/3.0/conf/obs-basic/ObservationCollection> ;
    skos:definition "Verify that all requirements from the requirements class have been fulfilled." ;
    skos:inScheme <http://www.opengis.net/spec/OMS/3.0> ;
    skos:prefLabel "Conformance Test http://www.opengis.net/spec/OMS/3.0/req/obs-basic/ObservationCollection/collectionType-sem" .

<http://www.opengis.net/spec/OMS/3.0/conf/obs-basic/ObservationCollection/collectionType-summarizing-con> a spec:ConformanceTest,
        skos:Concept ;
    spec:method "Inspect the documentation of the application, schema or profile." ;
    spec:purpose "Verify that all requirements from the requirements class have been fulfilled." ;
    spec:requirement <http://www.opengis.net/spec/OMS/3.0/req/obs-basic/ObservationCollection/collectionType-summarizing-con> ;
    spec:testType spec:Capabilities ;
    skos:broader <http://www.opengis.net/spec/OMS/3.0/conf/obs-basic/ObservationCollection> ;
    skos:definition "Verify that all requirements from the requirements class have been fulfilled." ;
    skos:inScheme <http://www.opengis.net/spec/OMS/3.0> ;
    skos:prefLabel "Conformance Test http://www.opengis.net/spec/OMS/3.0/req/obs-basic/ObservationCollection/collectionType-summarizing-con" .

<http://www.opengis.net/spec/OMS/3.0/conf/obs-basic/ObservationCollection/member-sem> a spec:ConformanceTest,
        skos:Concept ;
    spec:method "Inspect the documentation of the application, schema or profile." ;
    spec:purpose "Verify that all requirements from the requirements class have been fulfilled." ;
    spec:requirement <http://www.opengis.net/spec/OMS/3.0/req/obs-basic/ObservationCollection/member-sem> ;
    spec:testType spec:Capabilities ;
    skos:broader <http://www.opengis.net/spec/OMS/3.0/conf/obs-basic/ObservationCollection> ;
    skos:definition "Verify that all requirements from the requirements class have been fulfilled." ;
    skos:inScheme <http://www.opengis.net/spec/OMS/3.0> ;
    skos:prefLabel "Conformance Test http://www.opengis.net/spec/OMS/3.0/req/obs-basic/ObservationCollection/member-sem" .

<http://www.opengis.net/spec/OMS/3.0/conf/obs-basic/ObservationCollection/memberCharacteristics-sem> a spec:ConformanceTest,
        skos:Concept ;
    spec:method "Inspect the documentation of the application, schema or profile." ;
    spec:purpose "Verify that all requirements from the requirements class have been fulfilled." ;
    spec:requirement <http://www.opengis.net/spec/OMS/3.0/req/obs-basic/ObservationCollection/memberCharacteristics-sem> ;
    spec:testType spec:Capabilities ;
    skos:broader <http://www.opengis.net/spec/OMS/3.0/conf/obs-basic/ObservationCollection> ;
    skos:definition "Verify that all requirements from the requirements class have been fulfilled." ;
    skos:inScheme <http://www.opengis.net/spec/OMS/3.0> ;
    skos:prefLabel "Conformance Test http://www.opengis.net/spec/OMS/3.0/req/obs-basic/ObservationCollection/memberCharacteristics-sem" .

<http://www.opengis.net/spec/OMS/3.0/conf/obs-basic/ObservationCollection/relatedCollection-sem> a spec:ConformanceTest,
        skos:Concept ;
    spec:method "Inspect the documentation of the application, schema or profile." ;
    spec:purpose "Verify that all requirements from the requirements class have been fulfilled." ;
    spec:requirement <http://www.opengis.net/spec/OMS/3.0/req/obs-basic/ObservationCollection/relatedCollection-sem> ;
    spec:testType spec:Capabilities ;
    skos:broader <http://www.opengis.net/spec/OMS/3.0/conf/obs-basic/ObservationCollection> ;
    skos:definition "Verify that all requirements from the requirements class have been fulfilled." ;
    skos:inScheme <http://www.opengis.net/spec/OMS/3.0> ;
    skos:prefLabel "Conformance Test http://www.opengis.net/spec/OMS/3.0/req/obs-basic/ObservationCollection/relatedCollection-sem" .

<http://www.opengis.net/spec/OMS/3.0/conf/obs-basic/ObservingCapability/ObservingCapability-sem> a spec:ConformanceTest,
        skos:Concept ;
    spec:method "Inspect the documentation of the application, schema or profile." ;
    spec:purpose "Verify that all requirements from the requirements class have been fulfilled." ;
    spec:requirement <http://www.opengis.net/spec/OMS/3.0/req/obs-basic/ObservingCapability/ObservingCapability-sem> ;
    spec:testType spec:Capabilities ;
    skos:broader <http://www.opengis.net/spec/OMS/3.0/conf/obs-basic/ObservingCapability> ;
    skos:definition "Verify that all requirements from the requirements class have been fulfilled." ;
    skos:inScheme <http://www.opengis.net/spec/OMS/3.0> ;
    skos:prefLabel "Conformance Test http://www.opengis.net/spec/OMS/3.0/req/obs-basic/ObservingCapability/ObservingCapability-sem" .

<http://www.opengis.net/spec/OMS/3.0/conf/obs-basic/gen/link-sem> a spec:ConformanceTest,
        skos:Concept ;
    spec:method "Inspect the documentation of the application, schema or profile." ;
    spec:purpose "Verify that all requirements from the requirements class have been fulfilled." ;
    spec:requirement <http://www.opengis.net/spec/OMS/3.0/req/obs-basic/gen/link-sem> ;
    spec:testType spec:Capabilities ;
    skos:broader <http://www.opengis.net/spec/OMS/3.0/conf/obs-basic/Host> ;
    skos:broader <http://www.opengis.net/spec/OMS/3.0/conf/obs-basic/ObservableProperty> ;
    skos:broader <http://www.opengis.net/spec/OMS/3.0/conf/obs-basic/ObservingProcedure> ;
    skos:broader <http://www.opengis.net/spec/OMS/3.0/conf/obs-basic/GenericDomainFeature> ;
    skos:broader <http://www.opengis.net/spec/OMS/3.0/conf/obs-basic/Deployment> ;
    skos:broader <http://www.opengis.net/spec/OMS/3.0/conf/obs-basic/Observer> ;
    skos:definition "Verify that all requirements from the requirements class have been fulfilled." ;
    skos:inScheme <http://www.opengis.net/spec/OMS/3.0> ;
    skos:prefLabel "Conformance Test http://www.opengis.net/spec/OMS/3.0/req/obs-basic/gen/link-sem" .

<http://www.opengis.net/spec/OMS/3.0/conf/obs-basic/gen/location-sem> a spec:ConformanceTest,
        skos:Concept ;
    spec:method "Inspect the documentation of the application, schema or profile." ;
    spec:purpose "Verify that all requirements from the requirements class have been fulfilled." ;
    spec:requirement <http://www.opengis.net/spec/OMS/3.0/req/obs-basic/gen/location-sem> ;
    spec:testType spec:Capabilities ;
    skos:broader <http://www.opengis.net/spec/OMS/3.0/conf/obs-basic/Host> ;
    skos:broader <http://www.opengis.net/spec/OMS/3.0/conf/obs-basic/GenericDomainFeature> ;
    skos:broader <http://www.opengis.net/spec/OMS/3.0/conf/obs-basic/Observer> ;
    skos:definition "Verify that all requirements from the requirements class have been fulfilled." ;
    skos:inScheme <http://www.opengis.net/spec/OMS/3.0> ;
    skos:prefLabel "Conformance Test http://www.opengis.net/spec/OMS/3.0/req/obs-basic/gen/location-sem" .

<http://www.opengis.net/spec/OMS/3.0/conf/obs-core/AbstractDeployment/deploymentReason-sem> a spec:ConformanceTest,
        skos:Concept ;
    spec:method "Inspect the documentation of the application, schema or profile." ;
    spec:purpose "Verify that all requirements from the requirements class have been fulfilled." ;
    spec:requirement <http://www.opengis.net/spec/OMS/3.0/req/obs-core/AbstractDeployment/deploymentReason-sem> ;
    spec:testType spec:Capabilities ;
    skos:broader <http://www.opengis.net/spec/OMS/3.0/conf/obs-core/AbstractDeployment> ;
    skos:definition "Verify that all requirements from the requirements class have been fulfilled." ;
    skos:inScheme <http://www.opengis.net/spec/OMS/3.0> ;
    skos:prefLabel "Conformance Test http://www.opengis.net/spec/OMS/3.0/req/obs-core/AbstractDeployment/deploymentReason-sem" .

<http://www.opengis.net/spec/OMS/3.0/conf/obs-core/AbstractDeployment/deploymentTime-sem> a spec:ConformanceTest,
        skos:Concept ;
    spec:method "Inspect the documentation of the application, schema or profile." ;
    spec:purpose "Verify that all requirements from the requirements class have been fulfilled." ;
    spec:requirement <http://www.opengis.net/spec/OMS/3.0/req/obs-core/AbstractDeployment/deploymentTime-sem> ;
    spec:testType spec:Capabilities ;
    skos:broader <http://www.opengis.net/spec/OMS/3.0/conf/obs-core/AbstractDeployment> ;
    skos:definition "Verify that all requirements from the requirements class have been fulfilled." ;
    skos:inScheme <http://www.opengis.net/spec/OMS/3.0> ;
    skos:prefLabel "Conformance Test http://www.opengis.net/spec/OMS/3.0/req/obs-core/AbstractDeployment/deploymentTime-sem" .

<http://www.opengis.net/spec/OMS/3.0/conf/obs-core/AbstractObservation/FoI-con> a spec:ConformanceTest,
        skos:Concept ;
    spec:method "Inspect the documentation of the application, schema or profile." ;
    spec:purpose "Verify that all requirements from the requirements class have been fulfilled." ;
    spec:requirement <http://www.opengis.net/spec/OMS/3.0/req/obs-core/AbstractObservation/FoI-con> ;
    spec:testType spec:Capabilities ;
    skos:broader <http://www.opengis.net/spec/OMS/3.0/conf/obs-core/AbstractObservation> ;
    skos:definition "Verify that all requirements from the requirements class have been fulfilled." ;
    skos:inScheme <http://www.opengis.net/spec/OMS/3.0> ;
    skos:prefLabel "Conformance Test http://www.opengis.net/spec/OMS/3.0/req/obs-core/AbstractObservation/FoI-con" .

<http://www.opengis.net/spec/OMS/3.0/conf/obs-core/AbstractObservation/parameterName-card> a spec:ConformanceTest,
        skos:Concept ;
    spec:method "Inspect the documentation of the application, schema or profile." ;
    spec:purpose "Verify that all requirements from the requirements class have been fulfilled." ;
    spec:requirement <http://www.opengis.net/spec/OMS/3.0/req/obs-core/AbstractObservation/parameterName-card> ;
    spec:testType spec:Capabilities ;
    skos:broader <http://www.opengis.net/spec/OMS/3.0/conf/obs-core/AbstractObservation> ;
    skos:definition "Verify that all requirements from the requirements class have been fulfilled." ;
    skos:inScheme <http://www.opengis.net/spec/OMS/3.0> ;
    skos:prefLabel "Conformance Test http://www.opengis.net/spec/OMS/3.0/req/obs-core/AbstractObservation/parameterName-card" .

<http://www.opengis.net/spec/OMS/3.0/conf/obs-core/AbstractObservation/resultTime-type> a spec:ConformanceTest,
        skos:Concept ;
    spec:method "Inspect the documentation of the application, schema or profile." ;
    spec:purpose "Verify that all requirements from the requirements class have been fulfilled." ;
    spec:requirement <http://www.opengis.net/spec/OMS/3.0/req/obs-core/AbstractObservation/resultTime-type> ;
    spec:testType spec:Capabilities ;
    skos:broader <http://www.opengis.net/spec/OMS/3.0/conf/obs-core/AbstractObservation> ;
    skos:definition "Verify that all requirements from the requirements class have been fulfilled." ;
    skos:inScheme <http://www.opengis.net/spec/OMS/3.0> ;
    skos:prefLabel "Conformance Test http://www.opengis.net/spec/OMS/3.0/req/obs-core/AbstractObservation/resultTime-type" .

<http://www.opengis.net/spec/OMS/3.0/conf/obs-core/AbstractObservation/validTime-type> a spec:ConformanceTest,
        skos:Concept ;
    spec:method "Inspect the documentation of the application, schema or profile." ;
    spec:purpose "Verify that all requirements from the requirements class have been fulfilled." ;
    spec:requirement <http://www.opengis.net/spec/OMS/3.0/req/obs-core/AbstractObservation/validTime-type> ;
    spec:testType spec:Capabilities ;
    skos:broader <http://www.opengis.net/spec/OMS/3.0/conf/obs-core/AbstractObservation> ;
    skos:definition "Verify that all requirements from the requirements class have been fulfilled." ;
    skos:inScheme <http://www.opengis.net/spec/OMS/3.0> ;
    skos:prefLabel "Conformance Test http://www.opengis.net/spec/OMS/3.0/req/obs-core/AbstractObservation/validTime-type" .

<http://www.opengis.net/spec/OMS/3.0/conf/obs-core/AbstractObservationCharacteristics/AbstractObservationCharacteristics-sem> a spec:ConformanceTest,
        skos:Concept ;
    spec:method "Inspect the documentation of the application, schema or profile." ;
    spec:purpose "Verify that all requirements from the requirements class have been fulfilled." ;
    spec:requirement <http://www.opengis.net/spec/OMS/3.0/req/obs-core/AbstractObservationCharacteristics/AbstractObservationCharacteristics-sem> ;
    spec:testType spec:Capabilities ;
    skos:broader <http://www.opengis.net/spec/OMS/3.0/conf/obs-core/AbstractObservationCharacteristics> ;
    skos:definition "Verify that all requirements from the requirements class have been fulfilled." ;
    skos:inScheme <http://www.opengis.net/spec/OMS/3.0> ;
    skos:prefLabel "Conformance Test http://www.opengis.net/spec/OMS/3.0/req/obs-core/AbstractObservationCharacteristics/AbstractObservationCharacteristics-sem" .

<http://www.opengis.net/spec/OMS/3.0/conf/obs-core/AbstractObservationCharacteristics/pFoI-sem> a spec:ConformanceTest,
        skos:Concept ;
    spec:method "Inspect the documentation of the application, schema or profile." ;
    spec:purpose "Verify that all requirements from the requirements class have been fulfilled." ;
    spec:requirement <http://www.opengis.net/spec/OMS/3.0/req/obs-core/AbstractObservationCharacteristics/pFoI-sem> ;
    spec:testType spec:Capabilities ;
    skos:broader <http://www.opengis.net/spec/OMS/3.0/conf/obs-core/AbstractObservationCharacteristics> ;
    skos:definition "Verify that all requirements from the requirements class have been fulfilled." ;
    skos:inScheme <http://www.opengis.net/spec/OMS/3.0> ;
    skos:prefLabel "Conformance Test http://www.opengis.net/spec/OMS/3.0/req/obs-core/AbstractObservationCharacteristics/pFoI-sem" .

<http://www.opengis.net/spec/OMS/3.0/conf/obs-core/AbstractObservationCharacteristics/parameter-sem> a spec:ConformanceTest,
        skos:Concept ;
    spec:method "Inspect the documentation of the application, schema or profile." ;
    spec:purpose "Verify that all requirements from the requirements class have been fulfilled." ;
    spec:requirement <http://www.opengis.net/spec/OMS/3.0/req/obs-core/AbstractObservationCharacteristics/parameter-sem> ;
    spec:testType spec:Capabilities ;
    skos:broader <http://www.opengis.net/spec/OMS/3.0/conf/obs-core/AbstractObservationCharacteristics> ;
    skos:definition "Verify that all requirements from the requirements class have been fulfilled." ;
    skos:inScheme <http://www.opengis.net/spec/OMS/3.0> ;
    skos:prefLabel "Conformance Test http://www.opengis.net/spec/OMS/3.0/req/obs-core/AbstractObservationCharacteristics/parameter-sem" .

<http://www.opengis.net/spec/OMS/3.0/conf/obs-core/AbstractObservationCharacteristics/resultQuality-sem> a spec:ConformanceTest,
        skos:Concept ;
    spec:method "Inspect the documentation of the application, schema or profile." ;
    spec:purpose "Verify that all requirements from the requirements class have been fulfilled." ;
    spec:requirement <http://www.opengis.net/spec/OMS/3.0/req/obs-core/AbstractObservationCharacteristics/resultQuality-sem> ;
    spec:testType spec:Capabilities ;
    skos:broader <http://www.opengis.net/spec/OMS/3.0/conf/obs-core/AbstractObservationCharacteristics> ;
    skos:definition "Verify that all requirements from the requirements class have been fulfilled." ;
    skos:inScheme <http://www.opengis.net/spec/OMS/3.0> ;
    skos:prefLabel "Conformance Test http://www.opengis.net/spec/OMS/3.0/req/obs-core/AbstractObservationCharacteristics/resultQuality-sem" .

<http://www.opengis.net/spec/OMS/3.0/conf/obs-core/AbstractObservationCharacteristics/type-sem> a spec:ConformanceTest,
        skos:Concept ;
    spec:method "Inspect the documentation of the application, schema or profile." ;
    spec:purpose "Verify that all requirements from the requirements class have been fulfilled." ;
    spec:requirement <http://www.opengis.net/spec/OMS/3.0/req/obs-core/AbstractObservationCharacteristics/type-sem> ;
    spec:testType spec:Capabilities ;
    skos:broader <http://www.opengis.net/spec/OMS/3.0/conf/obs-core/AbstractObservationCharacteristics> ;
    skos:definition "Verify that all requirements from the requirements class have been fulfilled." ;
    skos:inScheme <http://www.opengis.net/spec/OMS/3.0> ;
    skos:prefLabel "Conformance Test http://www.opengis.net/spec/OMS/3.0/req/obs-core/AbstractObservationCharacteristics/type-sem" .

<http://www.opengis.net/spec/OMS/3.0/conf/obs-core/AbstractObservationCharacteristics/uFoI-sem> a spec:ConformanceTest,
        skos:Concept ;
    spec:method "Inspect the documentation of the application, schema or profile." ;
    spec:purpose "Verify that all requirements from the requirements class have been fulfilled." ;
    spec:requirement <http://www.opengis.net/spec/OMS/3.0/req/obs-core/AbstractObservationCharacteristics/uFoI-sem> ;
    spec:testType spec:Capabilities ;
    skos:broader <http://www.opengis.net/spec/OMS/3.0/conf/obs-core/AbstractObservationCharacteristics> ;
    skos:definition "Verify that all requirements from the requirements class have been fulfilled." ;
    skos:inScheme <http://www.opengis.net/spec/OMS/3.0> ;
    skos:prefLabel "Conformance Test http://www.opengis.net/spec/OMS/3.0/req/obs-core/AbstractObservationCharacteristics/uFoI-sem" .

<http://www.opengis.net/spec/OMS/3.0/conf/obs-core/NamedValue/NamedValue-sem> a spec:ConformanceTest,
        skos:Concept ;
    spec:method "Inspect the documentation of the application, schema or profile." ;
    spec:purpose "Verify that all requirements from the requirements class have been fulfilled." ;
    spec:requirement <http://www.opengis.net/spec/OMS/3.0/req/obs-core/NamedValue/NamedValue-sem> ;
    spec:testType spec:Capabilities ;
    skos:broader <http://www.opengis.net/spec/OMS/3.0/conf/obs-core/NamedValue> ;
    skos:definition "Verify that all requirements from the requirements class have been fulfilled." ;
    skos:inScheme <http://www.opengis.net/spec/OMS/3.0> ;
    skos:prefLabel "Conformance Test http://www.opengis.net/spec/OMS/3.0/req/obs-core/NamedValue/NamedValue-sem" .

<http://www.opengis.net/spec/OMS/3.0/conf/obs-core/NamedValue/name-sem> a spec:ConformanceTest,
        skos:Concept ;
    spec:method "Inspect the documentation of the application, schema or profile." ;
    spec:purpose "Verify that all requirements from the requirements class have been fulfilled." ;
    spec:requirement <http://www.opengis.net/spec/OMS/3.0/req/obs-core/NamedValue/name-sem> ;
    spec:testType spec:Capabilities ;
    skos:broader <http://www.opengis.net/spec/OMS/3.0/conf/obs-core/NamedValue> ;
    skos:definition "Verify that all requirements from the requirements class have been fulfilled." ;
    skos:inScheme <http://www.opengis.net/spec/OMS/3.0> ;
    skos:prefLabel "Conformance Test http://www.opengis.net/spec/OMS/3.0/req/obs-core/NamedValue/name-sem" .

<http://www.opengis.net/spec/OMS/3.0/conf/obs-core/NamedValue/value-sem> a spec:ConformanceTest,
        skos:Concept ;
    spec:method "Inspect the documentation of the application, schema or profile." ;
    spec:purpose "Verify that all requirements from the requirements class have been fulfilled." ;
    spec:requirement <http://www.opengis.net/spec/OMS/3.0/req/obs-core/NamedValue/value-sem> ;
    spec:testType spec:Capabilities ;
    skos:broader <http://www.opengis.net/spec/OMS/3.0/conf/obs-core/NamedValue> ;
    skos:definition "Verify that all requirements from the requirements class have been fulfilled." ;
    skos:inScheme <http://www.opengis.net/spec/OMS/3.0> ;
    skos:prefLabel "Conformance Test http://www.opengis.net/spec/OMS/3.0/req/obs-core/NamedValue/value-sem" .

<http://www.opengis.net/spec/OMS/3.0/conf/obs-core/gen/metadata-sem> a spec:ConformanceTest,
        skos:Concept ;
    spec:method "Inspect the documentation of the application, schema or profile." ;
    spec:purpose "Verify that all requirements from the requirements class have been fulfilled." ;
    spec:requirement <http://www.opengis.net/spec/OMS/3.0/req/obs-core/gen/metadata-sem> ;
    spec:testType spec:Capabilities ;
    skos:broader <http://www.opengis.net/spec/OMS/3.0/conf/sam-basic/SampleCollection> ;
    skos:broader <http://www.opengis.net/spec/OMS/3.0/conf/sam-core/AbstractSamplingProcedure> ;
    skos:broader <http://www.opengis.net/spec/OMS/3.0/conf/sam-core/AbstractSampler> ;
    skos:broader <http://www.opengis.net/spec/OMS/3.0/conf/sam-core/AbstractSampling> ;
    skos:broader <http://www.opengis.net/spec/OMS/3.0/conf/sam-core/AbstractPreparationProcedure> ;
    skos:broader <http://www.opengis.net/spec/OMS/3.0/conf/obs-core/AbstractObservationCharacteristics> ;
    skos:broader <http://www.opengis.net/spec/OMS/3.0/conf/sam-core/AbstractSample> ;
    skos:broader <http://www.opengis.net/spec/OMS/3.0/conf/obs-core/AbstractObserver> ;
    skos:broader <http://www.opengis.net/spec/OMS/3.0/conf/obs-core/AbstractDeployment> ;
    skos:broader <http://www.opengis.net/spec/OMS/3.0/conf/obs-core/AbstractHost> ;
    skos:broader <http://www.opengis.net/spec/OMS/3.0/conf/sam-core/AbstractPreparationStep> ;
    skos:broader <http://www.opengis.net/spec/OMS/3.0/conf/obs-core/AbstractObservingProcedure> ;
    skos:broader <http://www.opengis.net/spec/OMS/3.0/conf/obs-core/AbstractObservableProperty> ;
    skos:definition "Verify that all requirements from the requirements class have been fulfilled." ;
    skos:inScheme <http://www.opengis.net/spec/OMS/3.0> ;
    skos:prefLabel "Conformance Test http://www.opengis.net/spec/OMS/3.0/req/obs-core/gen/metadata-sem" .

<http://www.opengis.net/spec/OMS/3.0/conf/obs-cpt/Deployment/Deployment-sem> a spec:ConformanceTest,
        skos:Concept ;
    spec:method "Inspect the documentation of the application, schema or profile." ;
    spec:purpose "Verify that all requirements from the requirements class have been fulfilled." ;
    spec:requirement <http://www.opengis.net/spec/OMS/3.0/req/obs-cpt/Deployment/Deployment-sem> ;
    spec:testType spec:Capabilities ;
    skos:broader <http://www.opengis.net/spec/OMS/3.0/conf/obs-cpt/Deployment> ;
    skos:definition "Verify that all requirements from the requirements class have been fulfilled." ;
    skos:inScheme <http://www.opengis.net/spec/OMS/3.0> ;
    skos:prefLabel "Conformance Test http://www.opengis.net/spec/OMS/3.0/req/obs-cpt/Deployment/Deployment-sem" .

<http://www.opengis.net/spec/OMS/3.0/conf/obs-cpt/Deployment/host-sem> a spec:ConformanceTest,
        skos:Concept ;
    spec:method "Inspect the documentation of the application, schema or profile." ;
    spec:purpose "Verify that all requirements from the requirements class have been fulfilled." ;
    spec:requirement <http://www.opengis.net/spec/OMS/3.0/req/obs-cpt/Deployment/host-sem> ;
    spec:testType spec:Capabilities ;
    skos:broader <http://www.opengis.net/spec/OMS/3.0/conf/obs-cpt/Deployment> ;
    skos:definition "Verify that all requirements from the requirements class have been fulfilled." ;
    skos:inScheme <http://www.opengis.net/spec/OMS/3.0> ;
    skos:prefLabel "Conformance Test http://www.opengis.net/spec/OMS/3.0/req/obs-cpt/Deployment/host-sem" .

<http://www.opengis.net/spec/OMS/3.0/conf/obs-cpt/Deployment/observer-sem> a spec:ConformanceTest,
        skos:Concept ;
    spec:method "Inspect the documentation of the application, schema or profile." ;
    spec:purpose "Verify that all requirements from the requirements class have been fulfilled." ;
    spec:requirement <http://www.opengis.net/spec/OMS/3.0/req/obs-cpt/Deployment/observer-sem> ;
    spec:testType spec:Capabilities ;
    skos:broader <http://www.opengis.net/spec/OMS/3.0/conf/obs-cpt/Deployment> ;
    skos:definition "Verify that all requirements from the requirements class have been fulfilled." ;
    skos:inScheme <http://www.opengis.net/spec/OMS/3.0> ;
    skos:prefLabel "Conformance Test http://www.opengis.net/spec/OMS/3.0/req/obs-cpt/Deployment/observer-sem" .

<http://www.opengis.net/spec/OMS/3.0/conf/obs-cpt/Host/Host-sem> a spec:ConformanceTest,
        skos:Concept ;
    spec:method "Inspect the documentation of the application, schema or profile." ;
    spec:purpose "Verify that all requirements from the requirements class have been fulfilled." ;
    spec:requirement <http://www.opengis.net/spec/OMS/3.0/req/obs-cpt/Host/Host-sem> ;
    spec:testType spec:Capabilities ;
    skos:broader <http://www.opengis.net/spec/OMS/3.0/conf/obs-cpt/Host> ;
    skos:definition "Verify that all requirements from the requirements class have been fulfilled." ;
    skos:inScheme <http://www.opengis.net/spec/OMS/3.0> ;
    skos:prefLabel "Conformance Test http://www.opengis.net/spec/OMS/3.0/req/obs-cpt/Host/Host-sem" .

<http://www.opengis.net/spec/OMS/3.0/conf/obs-cpt/Host/deployment-sem> a spec:ConformanceTest,
        skos:Concept ;
    spec:method "Inspect the documentation of the application, schema or profile." ;
    spec:purpose "Verify that all requirements from the requirements class have been fulfilled." ;
    spec:requirement <http://www.opengis.net/spec/OMS/3.0/req/obs-cpt/Host/deployment-sem> ;
    spec:testType spec:Capabilities ;
    skos:broader <http://www.opengis.net/spec/OMS/3.0/conf/obs-cpt/Host> ;
    skos:definition "Verify that all requirements from the requirements class have been fulfilled." ;
    skos:inScheme <http://www.opengis.net/spec/OMS/3.0> ;
    skos:prefLabel "Conformance Test http://www.opengis.net/spec/OMS/3.0/req/obs-cpt/Host/deployment-sem" .

<http://www.opengis.net/spec/OMS/3.0/conf/obs-cpt/Host/relatedHost-sem> a spec:ConformanceTest,
        skos:Concept ;
    spec:method "Inspect the documentation of the application, schema or profile." ;
    spec:purpose "Verify that all requirements from the requirements class have been fulfilled." ;
    spec:requirement <http://www.opengis.net/spec/OMS/3.0/req/obs-cpt/Host/relatedHost-sem> ;
    spec:testType spec:Capabilities ;
    skos:broader <http://www.opengis.net/spec/OMS/3.0/conf/obs-cpt/Host> ;
    skos:definition "Verify that all requirements from the requirements class have been fulfilled." ;
    skos:inScheme <http://www.opengis.net/spec/OMS/3.0> ;
    skos:prefLabel "Conformance Test http://www.opengis.net/spec/OMS/3.0/req/obs-cpt/Host/relatedHost-sem" .

<http://www.opengis.net/spec/OMS/3.0/conf/obs-cpt/ObservableProperty/ObservableProperty-sem> a spec:ConformanceTest,
        skos:Concept ;
    spec:method "Inspect the documentation of the application, schema or profile." ;
    spec:purpose "Verify that all requirements from the requirements class have been fulfilled." ;
    spec:requirement <http://www.opengis.net/spec/OMS/3.0/req/obs-cpt/ObservableProperty/ObservableProperty-sem> ;
    spec:testType spec:Capabilities ;
    skos:broader <http://www.opengis.net/spec/OMS/3.0/conf/obs-cpt/ObservableProperty> ;
    skos:definition "Verify that all requirements from the requirements class have been fulfilled." ;
    skos:inScheme <http://www.opengis.net/spec/OMS/3.0> ;
    skos:prefLabel "Conformance Test http://www.opengis.net/spec/OMS/3.0/req/obs-cpt/ObservableProperty/ObservableProperty-sem" .

<http://www.opengis.net/spec/OMS/3.0/conf/obs-cpt/ObservableProperty/observer-sem> a spec:ConformanceTest,
        skos:Concept ;
    spec:method "Inspect the documentation of the application, schema or profile." ;
    spec:purpose "Verify that all requirements from the requirements class have been fulfilled." ;
    spec:requirement <http://www.opengis.net/spec/OMS/3.0/req/obs-cpt/ObservableProperty/observer-sem> ;
    spec:testType spec:Capabilities ;
    skos:broader <http://www.opengis.net/spec/OMS/3.0/conf/obs-cpt/ObservableProperty> ;
    skos:definition "Verify that all requirements from the requirements class have been fulfilled." ;
    skos:inScheme <http://www.opengis.net/spec/OMS/3.0> ;
    skos:prefLabel "Conformance Test http://www.opengis.net/spec/OMS/3.0/req/obs-cpt/ObservableProperty/observer-sem" .

<http://www.opengis.net/spec/OMS/3.0/conf/obs-cpt/Observation/Observation-sem> a spec:ConformanceTest,
        skos:Concept ;
    spec:method "Inspect the documentation of the application, schema or profile." ;
    spec:purpose "Verify that all requirements from the requirements class have been fulfilled." ;
    spec:requirement <http://www.opengis.net/spec/OMS/3.0/req/obs-cpt/Observation/Observation-sem> ;
    spec:testType spec:Capabilities ;
    skos:broader <http://www.opengis.net/spec/OMS/3.0/conf/obs-cpt/Observation> ;
    skos:definition "Verify that all requirements from the requirements class have been fulfilled." ;
    skos:inScheme <http://www.opengis.net/spec/OMS/3.0> ;
    skos:prefLabel "Conformance Test http://www.opengis.net/spec/OMS/3.0/req/obs-cpt/Observation/Observation-sem" .

<http://www.opengis.net/spec/OMS/3.0/conf/obs-cpt/Observation/featureOfInterest-card> a spec:ConformanceTest,
        skos:Concept ;
    spec:method "Inspect the documentation of the application, schema or profile." ;
    spec:purpose "Verify that all requirements from the requirements class have been fulfilled." ;
    spec:requirement <http://www.opengis.net/spec/OMS/3.0/req/obs-cpt/Observation/featureOfInterest-card> ;
    spec:testType spec:Capabilities ;
    skos:broader <http://www.opengis.net/spec/OMS/3.0/conf/obs-cpt/Observation> ;
    skos:definition "Verify that all requirements from the requirements class have been fulfilled." ;
    skos:inScheme <http://www.opengis.net/spec/OMS/3.0> ;
    skos:prefLabel "Conformance Test http://www.opengis.net/spec/OMS/3.0/req/obs-cpt/Observation/featureOfInterest-card" .

<http://www.opengis.net/spec/OMS/3.0/conf/obs-cpt/Observation/featureOfInterest-sem> a spec:ConformanceTest,
        skos:Concept ;
    spec:method "Inspect the documentation of the application, schema or profile." ;
    spec:purpose "Verify that all requirements from the requirements class have been fulfilled." ;
    spec:requirement <http://www.opengis.net/spec/OMS/3.0/req/obs-cpt/Observation/featureOfInterest-sem> ;
    spec:testType spec:Capabilities ;
    skos:broader <http://www.opengis.net/spec/OMS/3.0/conf/obs-cpt/Observation> ;
    skos:broader <http://www.opengis.net/spec/OMS/3.0/conf/obs-core/AbstractObservationCharacteristics> ;
    skos:definition "Verify that all requirements from the requirements class have been fulfilled." ;
    skos:inScheme <http://www.opengis.net/spec/OMS/3.0> ;
    skos:prefLabel "Conformance Test http://www.opengis.net/spec/OMS/3.0/req/obs-cpt/Observation/featureOfInterest-sem" .

<http://www.opengis.net/spec/OMS/3.0/conf/obs-cpt/Observation/host-sem> a spec:ConformanceTest,
        skos:Concept ;
    spec:method "Inspect the documentation of the application, schema or profile." ;
    spec:purpose "Verify that all requirements from the requirements class have been fulfilled." ;
    spec:requirement <http://www.opengis.net/spec/OMS/3.0/req/obs-cpt/Observation/host-sem> ;
    spec:testType spec:Capabilities ;
    skos:broader <http://www.opengis.net/spec/OMS/3.0/conf/obs-cpt/Observation> ;
    skos:broader <http://www.opengis.net/spec/OMS/3.0/conf/obs-core/AbstractObservationCharacteristics> ;
    skos:definition "Verify that all requirements from the requirements class have been fulfilled." ;
    skos:inScheme <http://www.opengis.net/spec/OMS/3.0> ;
    skos:prefLabel "Conformance Test http://www.opengis.net/spec/OMS/3.0/req/obs-cpt/Observation/host-sem" .

<http://www.opengis.net/spec/OMS/3.0/conf/obs-cpt/Observation/observedProperty-card> a spec:ConformanceTest,
        skos:Concept ;
    spec:method "Inspect the documentation of the application, schema or profile." ;
    spec:purpose "Verify that all requirements from the requirements class have been fulfilled." ;
    spec:requirement <http://www.opengis.net/spec/OMS/3.0/req/obs-cpt/Observation/observedProperty-card> ;
    spec:testType spec:Capabilities ;
    skos:broader <http://www.opengis.net/spec/OMS/3.0/conf/obs-cpt/Observation> ;
    skos:broader <http://www.opengis.net/spec/OMS/3.0/conf/obs-core/AbstractObservation> ;
    skos:definition "Verify that all requirements from the requirements class have been fulfilled." ;
    skos:inScheme <http://www.opengis.net/spec/OMS/3.0> ;
    skos:prefLabel "Conformance Test http://www.opengis.net/spec/OMS/3.0/req/obs-cpt/Observation/observedProperty-card" .

<http://www.opengis.net/spec/OMS/3.0/conf/obs-cpt/Observation/observedProperty-sem> a spec:ConformanceTest,
        skos:Concept ;
    spec:method "Inspect the documentation of the application, schema or profile." ;
    spec:purpose "Verify that all requirements from the requirements class have been fulfilled." ;
    spec:requirement <http://www.opengis.net/spec/OMS/3.0/req/obs-cpt/Observation/observedProperty-sem> ;
    spec:testType spec:Capabilities ;
    skos:broader <http://www.opengis.net/spec/OMS/3.0/conf/obs-cpt/Observation> ;
    skos:broader <http://www.opengis.net/spec/OMS/3.0/conf/obs-core/AbstractObservationCharacteristics> ;
    skos:definition "Verify that all requirements from the requirements class have been fulfilled." ;
    skos:inScheme <http://www.opengis.net/spec/OMS/3.0> ;
    skos:prefLabel "Conformance Test http://www.opengis.net/spec/OMS/3.0/req/obs-cpt/Observation/observedProperty-sem" .

<http://www.opengis.net/spec/OMS/3.0/conf/obs-cpt/Observation/observer-sem> a spec:ConformanceTest,
        skos:Concept ;
    spec:method "Inspect the documentation of the application, schema or profile." ;
    spec:purpose "Verify that all requirements from the requirements class have been fulfilled." ;
    spec:requirement <http://www.opengis.net/spec/OMS/3.0/req/obs-cpt/Observation/observer-sem> ;
    spec:testType spec:Capabilities ;
    skos:broader <http://www.opengis.net/spec/OMS/3.0/conf/obs-cpt/Observation> ;
    skos:broader <http://www.opengis.net/spec/OMS/3.0/conf/obs-core/AbstractObservationCharacteristics> ;
    skos:definition "Verify that all requirements from the requirements class have been fulfilled." ;
    skos:inScheme <http://www.opengis.net/spec/OMS/3.0> ;
    skos:prefLabel "Conformance Test http://www.opengis.net/spec/OMS/3.0/req/obs-cpt/Observation/observer-sem" .

<http://www.opengis.net/spec/OMS/3.0/conf/obs-cpt/Observation/observingProcedure-card> a spec:ConformanceTest,
        skos:Concept ;
    spec:method "Inspect the documentation of the application, schema or profile." ;
    spec:purpose "Verify that all requirements from the requirements class have been fulfilled." ;
    spec:requirement <http://www.opengis.net/spec/OMS/3.0/req/obs-cpt/Observation/observingProcedure-card> ;
    spec:testType spec:Capabilities ;
    skos:broader <http://www.opengis.net/spec/OMS/3.0/conf/obs-cpt/Observation> ;
    skos:definition "Verify that all requirements from the requirements class have been fulfilled." ;
    skos:inScheme <http://www.opengis.net/spec/OMS/3.0> ;
    skos:prefLabel "Conformance Test http://www.opengis.net/spec/OMS/3.0/req/obs-cpt/Observation/observingProcedure-card" .

<http://www.opengis.net/spec/OMS/3.0/conf/obs-cpt/Observation/observingProcedure-sem> a spec:ConformanceTest,
        skos:Concept ;
    spec:method "Inspect the documentation of the application, schema or profile." ;
    spec:purpose "Verify that all requirements from the requirements class have been fulfilled." ;
    spec:requirement <http://www.opengis.net/spec/OMS/3.0/req/obs-cpt/Observation/observingProcedure-sem> ;
    spec:testType spec:Capabilities ;
    skos:broader <http://www.opengis.net/spec/OMS/3.0/conf/obs-cpt/Observation> ;
    skos:definition "Verify that all requirements from the requirements class have been fulfilled." ;
    skos:inScheme <http://www.opengis.net/spec/OMS/3.0> ;
    skos:prefLabel "Conformance Test http://www.opengis.net/spec/OMS/3.0/req/obs-cpt/Observation/observingProcedure-sem" .

<http://www.opengis.net/spec/OMS/3.0/conf/obs-cpt/Observation/phenomenonTime-card> a spec:ConformanceTest,
        skos:Concept ;
    spec:method "Inspect the documentation of the application, schema or profile." ;
    spec:purpose "Verify that all requirements from the requirements class have been fulfilled." ;
    spec:requirement <http://www.opengis.net/spec/OMS/3.0/req/obs-cpt/Observation/phenomenonTime-card> ;
    spec:testType spec:Capabilities ;
    skos:broader <http://www.opengis.net/spec/OMS/3.0/conf/obs-cpt/Observation> ;
    skos:broader <http://www.opengis.net/spec/OMS/3.0/conf/obs-core/AbstractObservation> ;
    skos:definition "Verify that all requirements from the requirements class have been fulfilled." ;
    skos:inScheme <http://www.opengis.net/spec/OMS/3.0> ;
    skos:prefLabel "Conformance Test http://www.opengis.net/spec/OMS/3.0/req/obs-cpt/Observation/phenomenonTime-card" .

<http://www.opengis.net/spec/OMS/3.0/conf/obs-cpt/Observation/phenomenonTime-sem> a spec:ConformanceTest,
        skos:Concept ;
    spec:method "Inspect the documentation of the application, schema or profile." ;
    spec:purpose "Verify that all requirements from the requirements class have been fulfilled." ;
    spec:requirement <http://www.opengis.net/spec/OMS/3.0/req/obs-cpt/Observation/phenomenonTime-sem> ;
    spec:testType spec:Capabilities ;
    skos:broader <http://www.opengis.net/spec/OMS/3.0/conf/obs-cpt/Observation> ;
    skos:broader <http://www.opengis.net/spec/OMS/3.0/conf/obs-core/AbstractObservationCharacteristics> ;
    skos:definition "Verify that all requirements from the requirements class have been fulfilled." ;
    skos:inScheme <http://www.opengis.net/spec/OMS/3.0> ;
    skos:prefLabel "Conformance Test http://www.opengis.net/spec/OMS/3.0/req/obs-cpt/Observation/phenomenonTime-sem" .

<http://www.opengis.net/spec/OMS/3.0/conf/obs-cpt/Observation/procedure-card> a spec:ConformanceTest,
        skos:Concept ;
    spec:method "Inspect the documentation of the application, schema or profile." ;
    spec:purpose "Verify that all requirements from the requirements class have been fulfilled." ;
    spec:requirement <http://www.opengis.net/spec/OMS/3.0/req/obs-cpt/Observation/procedure-card> ;
    spec:testType spec:Capabilities ;
    skos:broader <http://www.opengis.net/spec/OMS/3.0/conf/obs-core/AbstractObservation> ;
    skos:definition "Verify that all requirements from the requirements class have been fulfilled." ;
    skos:inScheme <http://www.opengis.net/spec/OMS/3.0> ;
    skos:prefLabel "Conformance Test http://www.opengis.net/spec/OMS/3.0/req/obs-cpt/Observation/procedure-card" .

<http://www.opengis.net/spec/OMS/3.0/conf/obs-cpt/Observation/procedure-sem> a spec:ConformanceTest,
        skos:Concept ;
    spec:method "Inspect the documentation of the application, schema or profile." ;
    spec:purpose "Verify that all requirements from the requirements class have been fulfilled." ;
    spec:requirement <http://www.opengis.net/spec/OMS/3.0/req/obs-cpt/Observation/procedure-sem> ;
    spec:testType spec:Capabilities ;
    skos:broader <http://www.opengis.net/spec/OMS/3.0/conf/obs-core/AbstractObservationCharacteristics> ;
    skos:definition "Verify that all requirements from the requirements class have been fulfilled." ;
    skos:inScheme <http://www.opengis.net/spec/OMS/3.0> ;
    skos:prefLabel "Conformance Test http://www.opengis.net/spec/OMS/3.0/req/obs-cpt/Observation/procedure-sem" .

<http://www.opengis.net/spec/OMS/3.0/conf/obs-cpt/Observation/result-card> a spec:ConformanceTest,
        skos:Concept ;
    spec:method "Inspect the documentation of the application, schema or profile." ;
    spec:purpose "Verify that all requirements from the requirements class have been fulfilled." ;
    spec:requirement <http://www.opengis.net/spec/OMS/3.0/req/obs-cpt/Observation/result-card> ;
    spec:testType spec:Capabilities ;
    skos:broader <http://www.opengis.net/spec/OMS/3.0/conf/obs-cpt/Observation> ;
    skos:broader <http://www.opengis.net/spec/OMS/3.0/conf/obs-core/AbstractObservation> ;
    skos:definition "Verify that all requirements from the requirements class have been fulfilled." ;
    skos:inScheme <http://www.opengis.net/spec/OMS/3.0> ;
    skos:prefLabel "Conformance Test http://www.opengis.net/spec/OMS/3.0/req/obs-cpt/Observation/result-card" .

<http://www.opengis.net/spec/OMS/3.0/conf/obs-cpt/Observation/result-sem> a spec:ConformanceTest,
        skos:Concept ;
    spec:method "Inspect the documentation of the application, schema or profile." ;
    spec:purpose "Verify that all requirements from the requirements class have been fulfilled." ;
    spec:requirement <http://www.opengis.net/spec/OMS/3.0/req/obs-cpt/Observation/result-sem> ;
    spec:testType spec:Capabilities ;
    skos:broader <http://www.opengis.net/spec/OMS/3.0/conf/obs-cpt/Observation> ;
    skos:broader <http://www.opengis.net/spec/OMS/3.0/conf/obs-core/AbstractObservationCharacteristics> ;
    skos:definition "Verify that all requirements from the requirements class have been fulfilled." ;
    skos:inScheme <http://www.opengis.net/spec/OMS/3.0> ;
    skos:prefLabel "Conformance Test http://www.opengis.net/spec/OMS/3.0/req/obs-cpt/Observation/result-sem" .

<http://www.opengis.net/spec/OMS/3.0/conf/obs-cpt/Observation/resultTime-card> a spec:ConformanceTest,
        skos:Concept ;
    spec:method "Inspect the documentation of the application, schema or profile." ;
    spec:purpose "Verify that all requirements from the requirements class have been fulfilled." ;
    spec:requirement <http://www.opengis.net/spec/OMS/3.0/req/obs-cpt/Observation/resultTime-card> ;
    spec:testType spec:Capabilities ;
    skos:broader <http://www.opengis.net/spec/OMS/3.0/conf/obs-cpt/Observation> ;
    skos:broader <http://www.opengis.net/spec/OMS/3.0/conf/obs-core/AbstractObservation> ;
    skos:definition "Verify that all requirements from the requirements class have been fulfilled." ;
    skos:inScheme <http://www.opengis.net/spec/OMS/3.0> ;
    skos:prefLabel "Conformance Test http://www.opengis.net/spec/OMS/3.0/req/obs-cpt/Observation/resultTime-card" .

<http://www.opengis.net/spec/OMS/3.0/conf/obs-cpt/Observation/resultTime-sem> a spec:ConformanceTest,
        skos:Concept ;
    spec:method "Inspect the documentation of the application, schema or profile." ;
    spec:purpose "Verify that all requirements from the requirements class have been fulfilled." ;
    spec:requirement <http://www.opengis.net/spec/OMS/3.0/req/obs-cpt/Observation/resultTime-sem> ;
    spec:testType spec:Capabilities ;
    skos:broader <http://www.opengis.net/spec/OMS/3.0/conf/obs-cpt/Observation> ;
    skos:broader <http://www.opengis.net/spec/OMS/3.0/conf/obs-core/AbstractObservationCharacteristics> ;
    skos:definition "Verify that all requirements from the requirements class have been fulfilled." ;
    skos:inScheme <http://www.opengis.net/spec/OMS/3.0> ;
    skos:prefLabel "Conformance Test http://www.opengis.net/spec/OMS/3.0/req/obs-cpt/Observation/resultTime-sem" .

<http://www.opengis.net/spec/OMS/3.0/conf/obs-cpt/Observation/validTime-sem> a spec:ConformanceTest,
        skos:Concept ;
    spec:method "Inspect the documentation of the application, schema or profile." ;
    spec:purpose "Verify that all requirements from the requirements class have been fulfilled." ;
    spec:requirement <http://www.opengis.net/spec/OMS/3.0/req/obs-cpt/Observation/validTime-sem> ;
    spec:testType spec:Capabilities ;
    skos:broader <http://www.opengis.net/spec/OMS/3.0/conf/obs-cpt/Observation> ;
    skos:broader <http://www.opengis.net/spec/OMS/3.0/conf/obs-core/AbstractObservationCharacteristics> ;
    skos:definition "Verify that all requirements from the requirements class have been fulfilled." ;
    skos:inScheme <http://www.opengis.net/spec/OMS/3.0> ;
    skos:prefLabel "Conformance Test http://www.opengis.net/spec/OMS/3.0/req/obs-cpt/Observation/validTime-sem" .

<http://www.opengis.net/spec/OMS/3.0/conf/obs-cpt/Observer/Observer-sem> a spec:ConformanceTest,
        skos:Concept ;
    spec:method "Inspect the documentation of the application, schema or profile." ;
    spec:purpose "Verify that all requirements from the requirements class have been fulfilled." ;
    spec:requirement <http://www.opengis.net/spec/OMS/3.0/req/obs-cpt/Observer/Observer-sem> ;
    spec:testType spec:Capabilities ;
    skos:broader <http://www.opengis.net/spec/OMS/3.0/conf/obs-cpt/Observer> ;
    skos:definition "Verify that all requirements from the requirements class have been fulfilled." ;
    skos:inScheme <http://www.opengis.net/spec/OMS/3.0> ;
    skos:prefLabel "Conformance Test http://www.opengis.net/spec/OMS/3.0/req/obs-cpt/Observer/Observer-sem" .

<http://www.opengis.net/spec/OMS/3.0/conf/obs-cpt/Observer/deployment-sem> a spec:ConformanceTest,
        skos:Concept ;
    spec:method "Inspect the documentation of the application, schema or profile." ;
    spec:purpose "Verify that all requirements from the requirements class have been fulfilled." ;
    spec:requirement <http://www.opengis.net/spec/OMS/3.0/req/obs-cpt/Observer/deployment-sem> ;
    spec:testType spec:Capabilities ;
    skos:broader <http://www.opengis.net/spec/OMS/3.0/conf/obs-cpt/Observer> ;
    skos:definition "Verify that all requirements from the requirements class have been fulfilled." ;
    skos:inScheme <http://www.opengis.net/spec/OMS/3.0> ;
    skos:prefLabel "Conformance Test http://www.opengis.net/spec/OMS/3.0/req/obs-cpt/Observer/deployment-sem" .

<http://www.opengis.net/spec/OMS/3.0/conf/obs-cpt/Observer/observableProperty-sem> a spec:ConformanceTest,
        skos:Concept ;
    spec:method "Inspect the documentation of the application, schema or profile." ;
    spec:purpose "Verify that all requirements from the requirements class have been fulfilled." ;
    spec:requirement <http://www.opengis.net/spec/OMS/3.0/req/obs-cpt/Observer/observableProperty-sem> ;
    spec:testType spec:Capabilities ;
    skos:broader <http://www.opengis.net/spec/OMS/3.0/conf/obs-cpt/Observer> ;
    skos:definition "Verify that all requirements from the requirements class have been fulfilled." ;
    skos:inScheme <http://www.opengis.net/spec/OMS/3.0> ;
    skos:prefLabel "Conformance Test http://www.opengis.net/spec/OMS/3.0/req/obs-cpt/Observer/observableProperty-sem" .

<http://www.opengis.net/spec/OMS/3.0/conf/obs-cpt/Observer/observingProcedure-sem> a spec:ConformanceTest,
        skos:Concept ;
    spec:method "Inspect the documentation of the application, schema or profile." ;
    spec:purpose "Verify that all requirements from the requirements class have been fulfilled." ;
    spec:requirement <http://www.opengis.net/spec/OMS/3.0/req/obs-cpt/Observer/observingProcedure-sem> ;
    spec:testType spec:Capabilities ;
    skos:broader <http://www.opengis.net/spec/OMS/3.0/conf/obs-cpt/Observer> ;
    skos:definition "Verify that all requirements from the requirements class have been fulfilled." ;
    skos:inScheme <http://www.opengis.net/spec/OMS/3.0> ;
    skos:prefLabel "Conformance Test http://www.opengis.net/spec/OMS/3.0/req/obs-cpt/Observer/observingProcedure-sem" .

<http://www.opengis.net/spec/OMS/3.0/conf/obs-cpt/ObservingProcedure/ObservingProcedure-sem> a spec:ConformanceTest,
        skos:Concept ;
    spec:method "Inspect the documentation of the application, schema or profile." ;
    spec:purpose "Verify that all requirements from the requirements class have been fulfilled." ;
    spec:requirement <http://www.opengis.net/spec/OMS/3.0/req/obs-cpt/ObservingProcedure/ObservingProcedure-sem> ;
    spec:testType spec:Capabilities ;
    skos:broader <http://www.opengis.net/spec/OMS/3.0/conf/obs-cpt/ObservingProcedure> ;
    skos:definition "Verify that all requirements from the requirements class have been fulfilled." ;
    skos:inScheme <http://www.opengis.net/spec/OMS/3.0> ;
    skos:prefLabel "Conformance Test http://www.opengis.net/spec/OMS/3.0/req/obs-cpt/ObservingProcedure/ObservingProcedure-sem" .

<http://www.opengis.net/spec/OMS/3.0/conf/obs-cpt/ObservingProcedure/observer-sem> a spec:ConformanceTest,
        skos:Concept ;
    spec:method "Inspect the documentation of the application, schema or profile." ;
    spec:purpose "Verify that all requirements from the requirements class have been fulfilled." ;
    spec:requirement <http://www.opengis.net/spec/OMS/3.0/req/obs-cpt/ObservingProcedure/observer-sem> ;
    spec:testType spec:Capabilities ;
    skos:broader <http://www.opengis.net/spec/OMS/3.0/conf/obs-cpt/ObservingProcedure> ;
    skos:definition "Verify that all requirements from the requirements class have been fulfilled." ;
    skos:inScheme <http://www.opengis.net/spec/OMS/3.0> ;
    skos:prefLabel "Conformance Test http://www.opengis.net/spec/OMS/3.0/req/obs-cpt/ObservingProcedure/observer-sem" .

<http://www.opengis.net/spec/OMS/3.0/conf/obs-cpt/Procedure/Procedure-sem> a spec:ConformanceTest,
        skos:Concept ;
    spec:method "Inspect the documentation of the application, schema or profile." ;
    spec:purpose "Verify that all requirements from the requirements class have been fulfilled." ;
    spec:requirement <http://www.opengis.net/spec/OMS/3.0/req/obs-cpt/Procedure/Procedure-sem> ;
    spec:testType spec:Capabilities ;
    skos:broader <http://www.opengis.net/spec/OMS/3.0/conf/obs-cpt/Procedure> ;
    skos:definition "Verify that all requirements from the requirements class have been fulfilled." ;
    skos:inScheme <http://www.opengis.net/spec/OMS/3.0> ;
    skos:prefLabel "Conformance Test http://www.opengis.net/spec/OMS/3.0/req/obs-cpt/Procedure/Procedure-sem" .

<http://www.opengis.net/spec/OMS/3.0/conf/obs-cpt/gen/relatedObservation-sem> a spec:ConformanceTest,
        skos:Concept ;
    spec:method "Inspect the documentation of the application, schema or profile." ;
    spec:purpose "Verify that all requirements from the requirements class have been fulfilled." ;
    spec:requirement <http://www.opengis.net/spec/OMS/3.0/req/obs-cpt/gen/relatedObservation-sem> ;
    spec:testType spec:Capabilities ;
    skos:broader <http://www.opengis.net/spec/OMS/3.0/conf/obs-cpt/Host> ;
    skos:broader <http://www.opengis.net/spec/OMS/3.0/conf/obs-cpt/ObservingProcedure> ;
    skos:broader <http://www.opengis.net/spec/OMS/3.0/conf/obs-cpt/Observation> ;
    skos:broader <http://www.opengis.net/spec/OMS/3.0/conf/obs-cpt/ObservableProperty> ;
    skos:broader <http://www.opengis.net/spec/OMS/3.0/conf/obs-cpt/Observer> ;
    skos:broader <http://www.opengis.net/spec/OMS/3.0/conf/obs-core/AbstractObservationCharacteristics> ;
    skos:broader <http://www.opengis.net/spec/OMS/3.0/conf/sam-cpt/Sample> ;
    skos:broader <http://www.opengis.net/spec/OMS/3.0/conf/obs-basic/ObservationCollection> ;
    skos:definition "Verify that all requirements from the requirements class have been fulfilled." ;
    skos:inScheme <http://www.opengis.net/spec/OMS/3.0> ;
    skos:prefLabel "Conformance Test http://www.opengis.net/spec/OMS/3.0/req/obs-cpt/gen/relatedObservation-sem" .

<http://www.opengis.net/spec/OMS/3.0/conf/sam-basic/MaterialSample/MaterialSample-sem> a spec:ConformanceTest,
        skos:Concept ;
    spec:method "Inspect the documentation of the application, schema or profile." ;
    spec:purpose "Verify that all requirements from the requirements class have been fulfilled." ;
    spec:requirement <http://www.opengis.net/spec/OMS/3.0/req/sam-basic/MaterialSample/MaterialSample-sem> ;
    spec:testType spec:Capabilities ;
    skos:broader <http://www.opengis.net/spec/OMS/3.0/conf/sam-basic/MaterialSample> ;
    skos:definition "Verify that all requirements from the requirements class have been fulfilled." ;
    skos:inScheme <http://www.opengis.net/spec/OMS/3.0> ;
    skos:prefLabel "Conformance Test http://www.opengis.net/spec/OMS/3.0/req/sam-basic/MaterialSample/MaterialSample-sem" .

<http://www.opengis.net/spec/OMS/3.0/conf/sam-basic/MaterialSample/size-sem> a spec:ConformanceTest,
        skos:Concept ;
    spec:method "Inspect the documentation of the application, schema or profile." ;
    spec:purpose "Verify that all requirements from the requirements class have been fulfilled." ;
    spec:requirement <http://www.opengis.net/spec/OMS/3.0/req/sam-basic/MaterialSample/size-sem> ;
    spec:testType spec:Capabilities ;
    skos:broader <http://www.opengis.net/spec/OMS/3.0/conf/sam-basic/MaterialSample> ;
    skos:definition "Verify that all requirements from the requirements class have been fulfilled." ;
    skos:inScheme <http://www.opengis.net/spec/OMS/3.0> ;
    skos:prefLabel "Conformance Test http://www.opengis.net/spec/OMS/3.0/req/sam-basic/MaterialSample/size-sem" .

<http://www.opengis.net/spec/OMS/3.0/conf/sam-basic/MaterialSample/sourceLocation-sem> a spec:ConformanceTest,
        skos:Concept ;
    spec:method "Inspect the documentation of the application, schema or profile." ;
    spec:purpose "Verify that all requirements from the requirements class have been fulfilled." ;
    spec:requirement <http://www.opengis.net/spec/OMS/3.0/req/sam-basic/MaterialSample/sourceLocation-sem> ;
    spec:testType spec:Capabilities ;
    skos:broader <http://www.opengis.net/spec/OMS/3.0/conf/sam-basic/MaterialSample> ;
    skos:definition "Verify that all requirements from the requirements class have been fulfilled." ;
    skos:inScheme <http://www.opengis.net/spec/OMS/3.0> ;
    skos:prefLabel "Conformance Test http://www.opengis.net/spec/OMS/3.0/req/sam-basic/MaterialSample/sourceLocation-sem" .

<http://www.opengis.net/spec/OMS/3.0/conf/sam-basic/MaterialSample/storageLocation-sem> a spec:ConformanceTest,
        skos:Concept ;
    spec:method "Inspect the documentation of the application, schema or profile." ;
    spec:purpose "Verify that all requirements from the requirements class have been fulfilled." ;
    spec:requirement <http://www.opengis.net/spec/OMS/3.0/req/sam-basic/MaterialSample/storageLocation-sem> ;
    spec:testType spec:Capabilities ;
    skos:broader <http://www.opengis.net/spec/OMS/3.0/conf/sam-basic/MaterialSample> ;
    skos:definition "Verify that all requirements from the requirements class have been fulfilled." ;
    skos:inScheme <http://www.opengis.net/spec/OMS/3.0> ;
    skos:prefLabel "Conformance Test http://www.opengis.net/spec/OMS/3.0/req/sam-basic/MaterialSample/storageLocation-sem" .

<http://www.opengis.net/spec/OMS/3.0/conf/sam-basic/NamedLocation/NamedLocation-sem> a spec:ConformanceTest,
        skos:Concept ;
    spec:method "Inspect the documentation of the application, schema or profile." ;
    spec:purpose "Verify that all requirements from the requirements class have been fulfilled." ;
    spec:requirement <http://www.opengis.net/spec/OMS/3.0/req/sam-basic/NamedLocation/NamedLocation-sem> ;
    spec:testType spec:Capabilities ;
    skos:broader <http://www.opengis.net/spec/OMS/3.0/conf/sam-basic/NamedLocation> ;
    skos:definition "Verify that all requirements from the requirements class have been fulfilled." ;
    skos:inScheme <http://www.opengis.net/spec/OMS/3.0> ;
    skos:prefLabel "Conformance Test http://www.opengis.net/spec/OMS/3.0/req/sam-basic/NamedLocation/NamedLocation-sem" .

<http://www.opengis.net/spec/OMS/3.0/conf/sam-basic/NamedLocation/address-sem> a spec:ConformanceTest,
        skos:Concept ;
    spec:method "Inspect the documentation of the application, schema or profile." ;
    spec:purpose "Verify that all requirements from the requirements class have been fulfilled." ;
    spec:requirement <http://www.opengis.net/spec/OMS/3.0/req/sam-basic/NamedLocation/address-sem> ;
    spec:testType spec:Capabilities ;
    skos:broader <http://www.opengis.net/spec/OMS/3.0/conf/sam-basic/NamedLocation> ;
    skos:definition "Verify that all requirements from the requirements class have been fulfilled." ;
    skos:inScheme <http://www.opengis.net/spec/OMS/3.0> ;
    skos:prefLabel "Conformance Test http://www.opengis.net/spec/OMS/3.0/req/sam-basic/NamedLocation/address-sem" .

<http://www.opengis.net/spec/OMS/3.0/conf/sam-basic/NamedLocation/name-sem> a spec:ConformanceTest,
        skos:Concept ;
    spec:method "Inspect the documentation of the application, schema or profile." ;
    spec:purpose "Verify that all requirements from the requirements class have been fulfilled." ;
    spec:requirement <http://www.opengis.net/spec/OMS/3.0/req/sam-basic/NamedLocation/name-sem> ;
    spec:testType spec:Capabilities ;
    skos:broader <http://www.opengis.net/spec/OMS/3.0/conf/sam-basic/NamedLocation> ;
    skos:definition "Verify that all requirements from the requirements class have been fulfilled." ;
    skos:inScheme <http://www.opengis.net/spec/OMS/3.0> ;
    skos:prefLabel "Conformance Test http://www.opengis.net/spec/OMS/3.0/req/sam-basic/NamedLocation/name-sem" .

<http://www.opengis.net/spec/OMS/3.0/conf/sam-basic/NamedLocation/representativeGeometry-sem> a spec:ConformanceTest,
        skos:Concept ;
    spec:method "Inspect the documentation of the application, schema or profile." ;
    spec:purpose "Verify that all requirements from the requirements class have been fulfilled." ;
    spec:requirement <http://www.opengis.net/spec/OMS/3.0/req/sam-basic/NamedLocation/representativeGeometry-sem> ;
    spec:testType spec:Capabilities ;
    skos:broader <http://www.opengis.net/spec/OMS/3.0/conf/sam-basic/NamedLocation> ;
    skos:definition "Verify that all requirements from the requirements class have been fulfilled." ;
    skos:inScheme <http://www.opengis.net/spec/OMS/3.0> ;
    skos:prefLabel "Conformance Test http://www.opengis.net/spec/OMS/3.0/req/sam-basic/NamedLocation/representativeGeometry-sem" .

<http://www.opengis.net/spec/OMS/3.0/conf/sam-basic/PhysicalDimension/PhysicalDimension-sem> a spec:ConformanceTest,
        skos:Concept ;
    spec:method "Inspect the documentation of the application, schema or profile." ;
    spec:purpose "Verify that all requirements from the requirements class have been fulfilled." ;
    spec:requirement <http://www.opengis.net/spec/OMS/3.0/req/sam-basic/PhysicalDimension/PhysicalDimension-sem> ;
    spec:testType spec:Capabilities ;
    skos:broader <http://www.opengis.net/spec/OMS/3.0/conf/sam-basic/PhysicalDimension> ;
    skos:definition "Verify that all requirements from the requirements class have been fulfilled." ;
    skos:inScheme <http://www.opengis.net/spec/OMS/3.0> ;
    skos:prefLabel "Conformance Test http://www.opengis.net/spec/OMS/3.0/req/sam-basic/PhysicalDimension/PhysicalDimension-sem" .

<http://www.opengis.net/spec/OMS/3.0/conf/sam-basic/PhysicalDimension/dimension-sem> a spec:ConformanceTest,
        skos:Concept ;
    spec:method "Inspect the documentation of the application, schema or profile." ;
    spec:purpose "Verify that all requirements from the requirements class have been fulfilled." ;
    spec:requirement <http://www.opengis.net/spec/OMS/3.0/req/sam-basic/PhysicalDimension/dimension-sem> ;
    spec:testType spec:Capabilities ;
    skos:broader <http://www.opengis.net/spec/OMS/3.0/conf/sam-basic/PhysicalDimension> ;
    skos:definition "Verify that all requirements from the requirements class have been fulfilled." ;
    skos:inScheme <http://www.opengis.net/spec/OMS/3.0> ;
    skos:prefLabel "Conformance Test http://www.opengis.net/spec/OMS/3.0/req/sam-basic/PhysicalDimension/dimension-sem" .

<http://www.opengis.net/spec/OMS/3.0/conf/sam-basic/PhysicalDimension/value-sem> a spec:ConformanceTest,
        skos:Concept ;
    spec:method "Inspect the documentation of the application, schema or profile." ;
    spec:purpose "Verify that all requirements from the requirements class have been fulfilled." ;
    spec:requirement <http://www.opengis.net/spec/OMS/3.0/req/sam-basic/PhysicalDimension/value-sem> ;
    spec:testType spec:Capabilities ;
    skos:broader <http://www.opengis.net/spec/OMS/3.0/conf/sam-basic/PhysicalDimension> ;
    skos:definition "Verify that all requirements from the requirements class have been fulfilled." ;
    skos:inScheme <http://www.opengis.net/spec/OMS/3.0> ;
    skos:prefLabel "Conformance Test http://www.opengis.net/spec/OMS/3.0/req/sam-basic/PhysicalDimension/value-sem" .

<http://www.opengis.net/spec/OMS/3.0/conf/sam-basic/SampleCollection/SampleCollection-sem> a spec:ConformanceTest,
        skos:Concept ;
    spec:method "Inspect the documentation of the application, schema or profile." ;
    spec:purpose "Verify that all requirements from the requirements class have been fulfilled." ;
    spec:requirement <http://www.opengis.net/spec/OMS/3.0/req/sam-basic/SampleCollection/SampleCollection-sem> ;
    spec:testType spec:Capabilities ;
    skos:broader <http://www.opengis.net/spec/OMS/3.0/conf/sam-basic/SampleCollection> ;
    skos:definition "Verify that all requirements from the requirements class have been fulfilled." ;
    skos:inScheme <http://www.opengis.net/spec/OMS/3.0> ;
    skos:prefLabel "Conformance Test http://www.opengis.net/spec/OMS/3.0/req/sam-basic/SampleCollection/SampleCollection-sem" .

<http://www.opengis.net/spec/OMS/3.0/conf/sam-basic/SampleCollection/member-sem> a spec:ConformanceTest,
        skos:Concept ;
    spec:method "Inspect the documentation of the application, schema or profile." ;
    spec:purpose "Verify that all requirements from the requirements class have been fulfilled." ;
    spec:requirement <http://www.opengis.net/spec/OMS/3.0/req/sam-basic/SampleCollection/member-sem> ;
    spec:testType spec:Capabilities ;
    skos:broader <http://www.opengis.net/spec/OMS/3.0/conf/sam-basic/SampleCollection> ;
    skos:definition "Verify that all requirements from the requirements class have been fulfilled." ;
    skos:inScheme <http://www.opengis.net/spec/OMS/3.0> ;
    skos:prefLabel "Conformance Test http://www.opengis.net/spec/OMS/3.0/req/sam-basic/SampleCollection/member-sem" .

<http://www.opengis.net/spec/OMS/3.0/conf/sam-basic/SampleCollection/relatedCollection-sem> a spec:ConformanceTest,
        skos:Concept ;
    spec:method "Inspect the documentation of the application, schema or profile." ;
    spec:purpose "Verify that all requirements from the requirements class have been fulfilled." ;
    spec:requirement <http://www.opengis.net/spec/OMS/3.0/req/sam-basic/SampleCollection/relatedCollection-sem> ;
    spec:testType spec:Capabilities ;
    skos:broader <http://www.opengis.net/spec/OMS/3.0/conf/sam-basic/SampleCollection> ;
    skos:definition "Verify that all requirements from the requirements class have been fulfilled." ;
    skos:inScheme <http://www.opengis.net/spec/OMS/3.0> ;
    skos:prefLabel "Conformance Test http://www.opengis.net/spec/OMS/3.0/req/sam-basic/SampleCollection/relatedCollection-sem" .

<http://www.opengis.net/spec/OMS/3.0/conf/sam-basic/SpatialSample/SpatialSample-sem> a spec:ConformanceTest,
        skos:Concept ;
    spec:method "Inspect the documentation of the application, schema or profile." ;
    spec:purpose "Verify that all requirements from the requirements class have been fulfilled." ;
    spec:requirement <http://www.opengis.net/spec/OMS/3.0/req/sam-basic/SpatialSample/SpatialSample-sem> ;
    spec:testType spec:Capabilities ;
    skos:broader <http://www.opengis.net/spec/OMS/3.0/conf/sam-basic/SpatialSample> ;
    skos:definition "Verify that all requirements from the requirements class have been fulfilled." ;
    skos:inScheme <http://www.opengis.net/spec/OMS/3.0> ;
    skos:prefLabel "Conformance Test http://www.opengis.net/spec/OMS/3.0/req/sam-basic/SpatialSample/SpatialSample-sem" .

<http://www.opengis.net/spec/OMS/3.0/conf/sam-basic/SpatialSample/horizontalPositionalAccuracy-sem> a spec:ConformanceTest,
        skos:Concept ;
    spec:method "Inspect the documentation of the application, schema or profile." ;
    spec:purpose "Verify that all requirements from the requirements class have been fulfilled." ;
    spec:requirement <http://www.opengis.net/spec/OMS/3.0/req/sam-basic/SpatialSample/horizontalPositionalAccuracy-sem> ;
    spec:testType spec:Capabilities ;
    skos:broader <http://www.opengis.net/spec/OMS/3.0/conf/sam-basic/SpatialSample> ;
    skos:definition "Verify that all requirements from the requirements class have been fulfilled." ;
    skos:inScheme <http://www.opengis.net/spec/OMS/3.0> ;
    skos:prefLabel "Conformance Test http://www.opengis.net/spec/OMS/3.0/req/sam-basic/SpatialSample/horizontalPositionalAccuracy-sem" .

<http://www.opengis.net/spec/OMS/3.0/conf/sam-basic/SpatialSample/shape-sem> a spec:ConformanceTest,
        skos:Concept ;
    spec:method "Inspect the documentation of the application, schema or profile." ;
    spec:purpose "Verify that all requirements from the requirements class have been fulfilled." ;
    spec:requirement <http://www.opengis.net/spec/OMS/3.0/req/sam-basic/SpatialSample/shape-sem> ;
    spec:testType spec:Capabilities ;
    skos:broader <http://www.opengis.net/spec/OMS/3.0/conf/sam-basic/SpatialSample> ;
    skos:definition "Verify that all requirements from the requirements class have been fulfilled." ;
    skos:inScheme <http://www.opengis.net/spec/OMS/3.0> ;
    skos:prefLabel "Conformance Test http://www.opengis.net/spec/OMS/3.0/req/sam-basic/SpatialSample/shape-sem" .

<http://www.opengis.net/spec/OMS/3.0/conf/sam-basic/SpatialSample/verticalPositionalAccuracy-sem> a spec:ConformanceTest,
        skos:Concept ;
    spec:method "Inspect the documentation of the application, schema or profile." ;
    spec:purpose "Verify that all requirements from the requirements class have been fulfilled." ;
    spec:requirement <http://www.opengis.net/spec/OMS/3.0/req/sam-basic/SpatialSample/verticalPositionalAccuracy-sem> ;
    spec:testType spec:Capabilities ;
    skos:broader <http://www.opengis.net/spec/OMS/3.0/conf/sam-basic/SpatialSample> ;
    skos:definition "Verify that all requirements from the requirements class have been fulfilled." ;
    skos:inScheme <http://www.opengis.net/spec/OMS/3.0> ;
    skos:prefLabel "Conformance Test http://www.opengis.net/spec/OMS/3.0/req/sam-basic/SpatialSample/verticalPositionalAccuracy-sem" .

<http://www.opengis.net/spec/OMS/3.0/conf/sam-basic/StatisticalClassification/StatisticalClassification-sem> a spec:ConformanceTest,
        skos:Concept ;
    spec:method "Inspect the documentation of the application, schema or profile." ;
    spec:purpose "Verify that all requirements from the requirements class have been fulfilled." ;
    spec:requirement <http://www.opengis.net/spec/OMS/3.0/req/sam-basic/StatisticalClassification/StatisticalClassification-sem> ;
    spec:testType spec:Capabilities ;
    skos:broader <http://www.opengis.net/spec/OMS/3.0/conf/sam-basic/StatisticalClassification> ;
    skos:definition "Verify that all requirements from the requirements class have been fulfilled." ;
    skos:inScheme <http://www.opengis.net/spec/OMS/3.0> ;
    skos:prefLabel "Conformance Test http://www.opengis.net/spec/OMS/3.0/req/sam-basic/StatisticalClassification/StatisticalClassification-sem" .

<http://www.opengis.net/spec/OMS/3.0/conf/sam-basic/StatisticalClassification/classification-sem> a spec:ConformanceTest,
        skos:Concept ;
    spec:method "Inspect the documentation of the application, schema or profile." ;
    spec:purpose "Verify that all requirements from the requirements class have been fulfilled." ;
    spec:requirement <http://www.opengis.net/spec/OMS/3.0/req/sam-basic/StatisticalClassification/classification-sem> ;
    spec:testType spec:Capabilities ;
    skos:broader <http://www.opengis.net/spec/OMS/3.0/conf/sam-basic/StatisticalClassification> ;
    skos:definition "Verify that all requirements from the requirements class have been fulfilled." ;
    skos:inScheme <http://www.opengis.net/spec/OMS/3.0> ;
    skos:prefLabel "Conformance Test http://www.opengis.net/spec/OMS/3.0/req/sam-basic/StatisticalClassification/classification-sem" .

<http://www.opengis.net/spec/OMS/3.0/conf/sam-basic/StatisticalClassification/concept-sem> a spec:ConformanceTest,
        skos:Concept ;
    spec:method "Inspect the documentation of the application, schema or profile." ;
    spec:purpose "Verify that all requirements from the requirements class have been fulfilled." ;
    spec:requirement <http://www.opengis.net/spec/OMS/3.0/req/sam-basic/StatisticalClassification/concept-sem> ;
    spec:testType spec:Capabilities ;
    skos:broader <http://www.opengis.net/spec/OMS/3.0/conf/sam-basic/StatisticalClassification> ;
    skos:definition "Verify that all requirements from the requirements class have been fulfilled." ;
    skos:inScheme <http://www.opengis.net/spec/OMS/3.0> ;
    skos:prefLabel "Conformance Test http://www.opengis.net/spec/OMS/3.0/req/sam-basic/StatisticalClassification/concept-sem" .

<http://www.opengis.net/spec/OMS/3.0/conf/sam-basic/StatisticalSample/StatisticalSample-sem> a spec:ConformanceTest,
        skos:Concept ;
    spec:method "Inspect the documentation of the application, schema or profile." ;
    spec:purpose "Verify that all requirements from the requirements class have been fulfilled." ;
    spec:requirement <http://www.opengis.net/spec/OMS/3.0/req/sam-basic/StatisticalSample/StatisticalSample-sem> ;
    spec:testType spec:Capabilities ;
    skos:broader <http://www.opengis.net/spec/OMS/3.0/conf/sam-basic/StatisticalSample> ;
    skos:definition "Verify that all requirements from the requirements class have been fulfilled." ;
    skos:inScheme <http://www.opengis.net/spec/OMS/3.0> ;
    skos:prefLabel "Conformance Test http://www.opengis.net/spec/OMS/3.0/req/sam-basic/StatisticalSample/StatisticalSample-sem" .

<http://www.opengis.net/spec/OMS/3.0/conf/sam-basic/StatisticalSample/classification-sem> a spec:ConformanceTest,
        skos:Concept ;
    spec:method "Inspect the documentation of the application, schema or profile." ;
    spec:purpose "Verify that all requirements from the requirements class have been fulfilled." ;
    spec:requirement <http://www.opengis.net/spec/OMS/3.0/req/sam-basic/StatisticalSample/classification-sem> ;
    spec:testType spec:Capabilities ;
    skos:broader <http://www.opengis.net/spec/OMS/3.0/conf/sam-basic/StatisticalSample> ;
    skos:definition "Verify that all requirements from the requirements class have been fulfilled." ;
    skos:inScheme <http://www.opengis.net/spec/OMS/3.0> ;
    skos:prefLabel "Conformance Test http://www.opengis.net/spec/OMS/3.0/req/sam-basic/StatisticalSample/classification-sem" .

<http://www.opengis.net/spec/OMS/3.0/conf/sam-core/AbstractPreparationStep/description-sem> a spec:ConformanceTest,
        skos:Concept ;
    spec:method "Inspect the documentation of the application, schema or profile." ;
    spec:purpose "Verify that all requirements from the requirements class have been fulfilled." ;
    spec:requirement <http://www.opengis.net/spec/OMS/3.0/req/sam-core/AbstractPreparationStep/description-sem> ;
    spec:testType spec:Capabilities ;
    skos:broader <http://www.opengis.net/spec/OMS/3.0/conf/sam-core/AbstractPreparationStep> ;
    skos:definition "Verify that all requirements from the requirements class have been fulfilled." ;
    skos:inScheme <http://www.opengis.net/spec/OMS/3.0> ;
    skos:prefLabel "Conformance Test http://www.opengis.net/spec/OMS/3.0/req/sam-core/AbstractPreparationStep/description-sem" .

<http://www.opengis.net/spec/OMS/3.0/conf/sam-core/AbstractPreparationStep/time-sem> a spec:ConformanceTest,
        skos:Concept ;
    spec:method "Inspect the documentation of the application, schema or profile." ;
    spec:purpose "Verify that all requirements from the requirements class have been fulfilled." ;
    spec:requirement <http://www.opengis.net/spec/OMS/3.0/req/sam-core/AbstractPreparationStep/time-sem> ;
    spec:testType spec:Capabilities ;
    skos:broader <http://www.opengis.net/spec/OMS/3.0/conf/sam-core/AbstractPreparationStep> ;
    skos:definition "Verify that all requirements from the requirements class have been fulfilled." ;
    skos:inScheme <http://www.opengis.net/spec/OMS/3.0> ;
    skos:prefLabel "Conformance Test http://www.opengis.net/spec/OMS/3.0/req/sam-core/AbstractPreparationStep/time-sem" .

<http://www.opengis.net/spec/OMS/3.0/conf/sam-core/AbstractSample/parameter-sem> a spec:ConformanceTest,
        skos:Concept ;
    spec:method "Inspect the documentation of the application, schema or profile." ;
    spec:purpose "Verify that all requirements from the requirements class have been fulfilled." ;
    spec:requirement <http://www.opengis.net/spec/OMS/3.0/req/sam-core/AbstractSample/parameter-sem> ;
    spec:testType spec:Capabilities ;
    skos:broader <http://www.opengis.net/spec/OMS/3.0/conf/sam-core/AbstractSample> ;
    skos:definition "Verify that all requirements from the requirements class have been fulfilled." ;
    skos:inScheme <http://www.opengis.net/spec/OMS/3.0> ;
    skos:prefLabel "Conformance Test http://www.opengis.net/spec/OMS/3.0/req/sam-core/AbstractSample/parameter-sem" .

<http://www.opengis.net/spec/OMS/3.0/conf/sam-core/AbstractSample/sampleType-sem> a spec:ConformanceTest,
        skos:Concept ;
    spec:method "Inspect the documentation of the application, schema or profile." ;
    spec:purpose "Verify that all requirements from the requirements class have been fulfilled." ;
    spec:requirement <http://www.opengis.net/spec/OMS/3.0/req/sam-core/AbstractSample/sampleType-sem> ;
    spec:testType spec:Capabilities ;
    skos:broader <http://www.opengis.net/spec/OMS/3.0/conf/sam-core/AbstractSample> ;
    skos:definition "Verify that all requirements from the requirements class have been fulfilled." ;
    skos:inScheme <http://www.opengis.net/spec/OMS/3.0> ;
    skos:prefLabel "Conformance Test http://www.opengis.net/spec/OMS/3.0/req/sam-core/AbstractSample/sampleType-sem" .

<http://www.opengis.net/spec/OMS/3.0/conf/sam-core/AbstractSampler/samplerType-sem> a spec:ConformanceTest,
        skos:Concept ;
    spec:method "Inspect the documentation of the application, schema or profile." ;
    spec:purpose "Verify that all requirements from the requirements class have been fulfilled." ;
    spec:requirement <http://www.opengis.net/spec/OMS/3.0/req/sam-core/AbstractSampler/samplerType-sem> ;
    spec:testType spec:Capabilities ;
    skos:broader <http://www.opengis.net/spec/OMS/3.0/conf/sam-core/AbstractSampler> ;
    skos:definition "Verify that all requirements from the requirements class have been fulfilled." ;
    skos:inScheme <http://www.opengis.net/spec/OMS/3.0> ;
    skos:prefLabel "Conformance Test http://www.opengis.net/spec/OMS/3.0/req/sam-core/AbstractSampler/samplerType-sem" .

<http://www.opengis.net/spec/OMS/3.0/conf/sam-core/AbstractSampling/parameter-sem> a spec:ConformanceTest,
        skos:Concept ;
    spec:method "Inspect the documentation of the application, schema or profile." ;
    spec:purpose "Verify that all requirements from the requirements class have been fulfilled." ;
    spec:requirement <http://www.opengis.net/spec/OMS/3.0/req/sam-core/AbstractSampling/parameter-sem> ;
    spec:testType spec:Capabilities ;
    skos:broader <http://www.opengis.net/spec/OMS/3.0/conf/sam-core/AbstractSampling> ;
    skos:definition "Verify that all requirements from the requirements class have been fulfilled." ;
    skos:inScheme <http://www.opengis.net/spec/OMS/3.0> ;
    skos:prefLabel "Conformance Test http://www.opengis.net/spec/OMS/3.0/req/sam-core/AbstractSampling/parameter-sem" .

<http://www.opengis.net/spec/OMS/3.0/conf/sam-core/AbstractSampling/samplingLocation-sem> a spec:ConformanceTest,
        skos:Concept ;
    spec:method "Inspect the documentation of the application, schema or profile." ;
    spec:purpose "Verify that all requirements from the requirements class have been fulfilled." ;
    spec:requirement <http://www.opengis.net/spec/OMS/3.0/req/sam-core/AbstractSampling/samplingLocation-sem> ;
    spec:testType spec:Capabilities ;
    skos:broader <http://www.opengis.net/spec/OMS/3.0/conf/sam-core/AbstractSampling> ;
    skos:definition "Verify that all requirements from the requirements class have been fulfilled." ;
    skos:inScheme <http://www.opengis.net/spec/OMS/3.0> ;
    skos:prefLabel "Conformance Test http://www.opengis.net/spec/OMS/3.0/req/sam-core/AbstractSampling/samplingLocation-sem" .

<http://www.opengis.net/spec/OMS/3.0/conf/sam-core/AbstractSampling/time-sem> a spec:ConformanceTest,
        skos:Concept ;
    spec:method "Inspect the documentation of the application, schema or profile." ;
    spec:purpose "Verify that all requirements from the requirements class have been fulfilled." ;
    spec:requirement <http://www.opengis.net/spec/OMS/3.0/req/sam-core/AbstractSampling/time-sem> ;
    spec:testType spec:Capabilities ;
    skos:broader <http://www.opengis.net/spec/OMS/3.0/conf/sam-core/AbstractSampling> ;
    skos:definition "Verify that all requirements from the requirements class have been fulfilled." ;
    skos:inScheme <http://www.opengis.net/spec/OMS/3.0> ;
    skos:prefLabel "Conformance Test http://www.opengis.net/spec/OMS/3.0/req/sam-core/AbstractSampling/time-sem" .

<http://www.opengis.net/spec/OMS/3.0/conf/sam-cpt/PreparationProcedure/PreparationProcedure-sem> a spec:ConformanceTest,
        skos:Concept ;
    spec:method "Inspect the documentation of the application, schema or profile." ;
    spec:purpose "Verify that all requirements from the requirements class have been fulfilled." ;
    spec:requirement <http://www.opengis.net/spec/OMS/3.0/req/sam-cpt/PreparationProcedure/PreparationProcedure-sem> ;
    spec:testType spec:Capabilities ;
    skos:broader <http://www.opengis.net/spec/OMS/3.0/conf/sam-cpt/PreparationProcedure> ;
    skos:definition "Verify that all requirements from the requirements class have been fulfilled." ;
    skos:inScheme <http://www.opengis.net/spec/OMS/3.0> ;
    skos:prefLabel "Conformance Test http://www.opengis.net/spec/OMS/3.0/req/sam-cpt/PreparationProcedure/PreparationProcedure-sem" .

<http://www.opengis.net/spec/OMS/3.0/conf/sam-cpt/PreparationProcedure/samplePreparationStep-sem> a spec:ConformanceTest,
        skos:Concept ;
    spec:method "Inspect the documentation of the application, schema or profile." ;
    spec:purpose "Verify that all requirements from the requirements class have been fulfilled." ;
    spec:requirement <http://www.opengis.net/spec/OMS/3.0/req/sam-cpt/PreparationProcedure/samplePreparationStep-sem> ;
    spec:testType spec:Capabilities ;
    skos:broader <http://www.opengis.net/spec/OMS/3.0/conf/sam-cpt/PreparationProcedure> ;
    skos:definition "Verify that all requirements from the requirements class have been fulfilled." ;
    skos:inScheme <http://www.opengis.net/spec/OMS/3.0> ;
    skos:prefLabel "Conformance Test http://www.opengis.net/spec/OMS/3.0/req/sam-cpt/PreparationProcedure/samplePreparationStep-sem" .

<http://www.opengis.net/spec/OMS/3.0/conf/sam-cpt/PreparationStep/PreparationStep-sem> a spec:ConformanceTest,
        skos:Concept ;
    spec:method "Inspect the documentation of the application, schema or profile." ;
    spec:purpose "Verify that all requirements from the requirements class have been fulfilled." ;
    spec:requirement <http://www.opengis.net/spec/OMS/3.0/req/sam-cpt/PreparationStep/PreparationStep-sem> ;
    spec:testType spec:Capabilities ;
    skos:broader <http://www.opengis.net/spec/OMS/3.0/conf/sam-cpt/PreparationStep> ;
    skos:definition "Verify that all requirements from the requirements class have been fulfilled." ;
    skos:inScheme <http://www.opengis.net/spec/OMS/3.0> ;
    skos:prefLabel "Conformance Test http://www.opengis.net/spec/OMS/3.0/req/sam-cpt/PreparationStep/PreparationStep-sem" .

<http://www.opengis.net/spec/OMS/3.0/conf/sam-cpt/PreparationStep/preparedSample-sem> a spec:ConformanceTest,
        skos:Concept ;
    spec:method "Inspect the documentation of the application, schema or profile." ;
    spec:purpose "Verify that all requirements from the requirements class have been fulfilled." ;
    spec:requirement <http://www.opengis.net/spec/OMS/3.0/req/sam-cpt/PreparationStep/preparedSample-sem> ;
    spec:testType spec:Capabilities ;
    skos:broader <http://www.opengis.net/spec/OMS/3.0/conf/sam-cpt/PreparationStep> ;
    skos:definition "Verify that all requirements from the requirements class have been fulfilled." ;
    skos:inScheme <http://www.opengis.net/spec/OMS/3.0> ;
    skos:prefLabel "Conformance Test http://www.opengis.net/spec/OMS/3.0/req/sam-cpt/PreparationStep/preparedSample-sem" .

<http://www.opengis.net/spec/OMS/3.0/conf/sam-cpt/PreparationStep/processingDetails-sem> a spec:ConformanceTest,
        skos:Concept ;
    spec:method "Inspect the documentation of the application, schema or profile." ;
    spec:purpose "Verify that all requirements from the requirements class have been fulfilled." ;
    spec:requirement <http://www.opengis.net/spec/OMS/3.0/req/sam-cpt/PreparationStep/processingDetails-sem> ;
    spec:testType spec:Capabilities ;
    skos:broader <http://www.opengis.net/spec/OMS/3.0/conf/sam-cpt/PreparationStep> ;
    skos:definition "Verify that all requirements from the requirements class have been fulfilled." ;
    skos:inScheme <http://www.opengis.net/spec/OMS/3.0> ;
    skos:prefLabel "Conformance Test http://www.opengis.net/spec/OMS/3.0/req/sam-cpt/PreparationStep/processingDetails-sem" .

<http://www.opengis.net/spec/OMS/3.0/conf/sam-cpt/Sample/Sample-sem> a spec:ConformanceTest,
        skos:Concept ;
    spec:method "Inspect the documentation of the application, schema or profile." ;
    spec:purpose "Verify that all requirements from the requirements class have been fulfilled." ;
    spec:requirement <http://www.opengis.net/spec/OMS/3.0/req/sam-cpt/Sample/Sample-sem> ;
    spec:testType spec:Capabilities ;
    skos:broader <http://www.opengis.net/spec/OMS/3.0/conf/sam-cpt/Sample> ;
    skos:definition "Verify that all requirements from the requirements class have been fulfilled." ;
    skos:inScheme <http://www.opengis.net/spec/OMS/3.0> ;
    skos:prefLabel "Conformance Test http://www.opengis.net/spec/OMS/3.0/req/sam-cpt/Sample/Sample-sem" .

<http://www.opengis.net/spec/OMS/3.0/conf/sam-cpt/Sample/preparationStep-sem> a spec:ConformanceTest,
        skos:Concept ;
    spec:method "Inspect the documentation of the application, schema or profile." ;
    spec:purpose "Verify that all requirements from the requirements class have been fulfilled." ;
    spec:requirement <http://www.opengis.net/spec/OMS/3.0/req/sam-cpt/Sample/preparationStep-sem> ;
    spec:testType spec:Capabilities ;
    skos:broader <http://www.opengis.net/spec/OMS/3.0/conf/sam-cpt/Sample> ;
    skos:definition "Verify that all requirements from the requirements class have been fulfilled." ;
    skos:inScheme <http://www.opengis.net/spec/OMS/3.0> ;
    skos:prefLabel "Conformance Test http://www.opengis.net/spec/OMS/3.0/req/sam-cpt/Sample/preparationStep-sem" .

<http://www.opengis.net/spec/OMS/3.0/conf/sam-cpt/Sample/relatedSample-sem> a spec:ConformanceTest,
        skos:Concept ;
    spec:method "Inspect the documentation of the application, schema or profile." ;
    spec:purpose "Verify that all requirements from the requirements class have been fulfilled." ;
    spec:requirement <http://www.opengis.net/spec/OMS/3.0/req/sam-cpt/Sample/relatedSample-sem> ;
    spec:testType spec:Capabilities ;
    skos:broader <http://www.opengis.net/spec/OMS/3.0/conf/sam-cpt/Sample> ;
    skos:definition "Verify that all requirements from the requirements class have been fulfilled." ;
    skos:inScheme <http://www.opengis.net/spec/OMS/3.0> ;
    skos:prefLabel "Conformance Test http://www.opengis.net/spec/OMS/3.0/req/sam-cpt/Sample/relatedSample-sem" .

<http://www.opengis.net/spec/OMS/3.0/conf/sam-cpt/Sample/sampledFeature-card> a spec:ConformanceTest,
        skos:Concept ;
    spec:method "Inspect the documentation of the application, schema or profile." ;
    spec:purpose "Verify that all requirements from the requirements class have been fulfilled." ;
    spec:requirement <http://www.opengis.net/spec/OMS/3.0/req/sam-cpt/Sample/sampledFeature-card> ;
    spec:testType spec:Capabilities ;
    skos:broader <http://www.opengis.net/spec/OMS/3.0/conf/sam-cpt/Sample> ;
    skos:definition "Verify that all requirements from the requirements class have been fulfilled." ;
    skos:inScheme <http://www.opengis.net/spec/OMS/3.0> ;
    skos:prefLabel "Conformance Test http://www.opengis.net/spec/OMS/3.0/req/sam-cpt/Sample/sampledFeature-card" .

<http://www.opengis.net/spec/OMS/3.0/conf/sam-cpt/Sample/sampledFeature-sem> a spec:ConformanceTest,
        skos:Concept ;
    spec:method "Inspect the documentation of the application, schema or profile." ;
    spec:purpose "Verify that all requirements from the requirements class have been fulfilled." ;
    spec:requirement <http://www.opengis.net/spec/OMS/3.0/req/sam-cpt/Sample/sampledFeature-sem> ;
    spec:testType spec:Capabilities ;
    skos:broader <http://www.opengis.net/spec/OMS/3.0/conf/sam-cpt/Sample> ;
    skos:definition "Verify that all requirements from the requirements class have been fulfilled." ;
    skos:inScheme <http://www.opengis.net/spec/OMS/3.0> ;
    skos:prefLabel "Conformance Test http://www.opengis.net/spec/OMS/3.0/req/sam-cpt/Sample/sampledFeature-sem" .

<http://www.opengis.net/spec/OMS/3.0/conf/sam-cpt/Sample/sampling-sem> a spec:ConformanceTest,
        skos:Concept ;
    spec:method "Inspect the documentation of the application, schema or profile." ;
    spec:purpose "Verify that all requirements from the requirements class have been fulfilled." ;
    spec:requirement <http://www.opengis.net/spec/OMS/3.0/req/sam-cpt/Sample/sampling-sem> ;
    spec:testType spec:Capabilities ;
    skos:broader <http://www.opengis.net/spec/OMS/3.0/conf/sam-cpt/Sample> ;
    skos:definition "Verify that all requirements from the requirements class have been fulfilled." ;
    skos:inScheme <http://www.opengis.net/spec/OMS/3.0> ;
    skos:prefLabel "Conformance Test http://www.opengis.net/spec/OMS/3.0/req/sam-cpt/Sample/sampling-sem" .

<http://www.opengis.net/spec/OMS/3.0/conf/sam-cpt/Sampler/Sampler-sem> a spec:ConformanceTest,
        skos:Concept ;
    spec:method "Inspect the documentation of the application, schema or profile." ;
    spec:purpose "Verify that all requirements from the requirements class have been fulfilled." ;
    spec:requirement <http://www.opengis.net/spec/OMS/3.0/req/sam-cpt/Sampler/Sampler-sem> ;
    spec:testType spec:Capabilities ;
    skos:broader <http://www.opengis.net/spec/OMS/3.0/conf/sam-cpt/Sampler> ;
    skos:definition "Verify that all requirements from the requirements class have been fulfilled." ;
    skos:inScheme <http://www.opengis.net/spec/OMS/3.0> ;
    skos:prefLabel "Conformance Test http://www.opengis.net/spec/OMS/3.0/req/sam-cpt/Sampler/Sampler-sem" .

<http://www.opengis.net/spec/OMS/3.0/conf/sam-cpt/Sampler/implementedProcedure-sem> a spec:ConformanceTest,
        skos:Concept ;
    spec:method "Inspect the documentation of the application, schema or profile." ;
    spec:purpose "Verify that all requirements from the requirements class have been fulfilled." ;
    spec:requirement <http://www.opengis.net/spec/OMS/3.0/req/sam-cpt/Sampler/implementedProcedure-sem> ;
    spec:testType spec:Capabilities ;
    skos:broader <http://www.opengis.net/spec/OMS/3.0/conf/sam-cpt/Sampler> ;
    skos:definition "Verify that all requirements from the requirements class have been fulfilled." ;
    skos:inScheme <http://www.opengis.net/spec/OMS/3.0> ;
    skos:prefLabel "Conformance Test http://www.opengis.net/spec/OMS/3.0/req/sam-cpt/Sampler/implementedProcedure-sem" .

<http://www.opengis.net/spec/OMS/3.0/conf/sam-cpt/Sampler/sampling-sem> a spec:ConformanceTest,
        skos:Concept ;
    spec:method "Inspect the documentation of the application, schema or profile." ;
    spec:purpose "Verify that all requirements from the requirements class have been fulfilled." ;
    spec:requirement <http://www.opengis.net/spec/OMS/3.0/req/sam-cpt/Sampler/sampling-sem> ;
    spec:testType spec:Capabilities ;
    skos:broader <http://www.opengis.net/spec/OMS/3.0/conf/sam-cpt/Sampler> ;
    skos:definition "Verify that all requirements from the requirements class have been fulfilled." ;
    skos:inScheme <http://www.opengis.net/spec/OMS/3.0> ;
    skos:prefLabel "Conformance Test http://www.opengis.net/spec/OMS/3.0/req/sam-cpt/Sampler/sampling-sem" .

<http://www.opengis.net/spec/OMS/3.0/conf/sam-cpt/Sampling/Sampling-sem> a spec:ConformanceTest,
        skos:Concept ;
    spec:method "Inspect the documentation of the application, schema or profile." ;
    spec:purpose "Verify that all requirements from the requirements class have been fulfilled." ;
    spec:requirement <http://www.opengis.net/spec/OMS/3.0/req/sam-cpt/Sampling/Sampling-sem> ;
    spec:testType spec:Capabilities ;
    skos:broader <http://www.opengis.net/spec/OMS/3.0/conf/sam-cpt/Sampling> ;
    skos:definition "Verify that all requirements from the requirements class have been fulfilled." ;
    skos:inScheme <http://www.opengis.net/spec/OMS/3.0> ;
    skos:prefLabel "Conformance Test http://www.opengis.net/spec/OMS/3.0/req/sam-cpt/Sampling/Sampling-sem" .

<http://www.opengis.net/spec/OMS/3.0/conf/sam-cpt/Sampling/featureOfInterest-card> a spec:ConformanceTest,
        skos:Concept ;
    spec:method "Inspect the documentation of the application, schema or profile." ;
    spec:purpose "Verify that all requirements from the requirements class have been fulfilled." ;
    spec:requirement <http://www.opengis.net/spec/OMS/3.0/req/sam-cpt/Sampling/featureOfInterest-card> ;
    spec:testType spec:Capabilities ;
    skos:broader <http://www.opengis.net/spec/OMS/3.0/conf/sam-cpt/Sampling> ;
    skos:definition "Verify that all requirements from the requirements class have been fulfilled." ;
    skos:inScheme <http://www.opengis.net/spec/OMS/3.0> ;
    skos:prefLabel "Conformance Test http://www.opengis.net/spec/OMS/3.0/req/sam-cpt/Sampling/featureOfInterest-card" .

<http://www.opengis.net/spec/OMS/3.0/conf/sam-cpt/Sampling/featureOfInterest-sem> a spec:ConformanceTest,
        skos:Concept ;
    spec:method "Inspect the documentation of the application, schema or profile." ;
    spec:purpose "Verify that all requirements from the requirements class have been fulfilled." ;
    spec:requirement <http://www.opengis.net/spec/OMS/3.0/req/sam-cpt/Sampling/featureOfInterest-sem> ;
    spec:testType spec:Capabilities ;
    skos:broader <http://www.opengis.net/spec/OMS/3.0/conf/sam-cpt/Sampling> ;
    skos:definition "Verify that all requirements from the requirements class have been fulfilled." ;
    skos:inScheme <http://www.opengis.net/spec/OMS/3.0> ;
    skos:prefLabel "Conformance Test http://www.opengis.net/spec/OMS/3.0/req/sam-cpt/Sampling/featureOfInterest-sem" .

<http://www.opengis.net/spec/OMS/3.0/conf/sam-cpt/Sampling/relatedSampling-sem> a spec:ConformanceTest,
        skos:Concept ;
    spec:method "Inspect the documentation of the application, schema or profile." ;
    spec:purpose "Verify that all requirements from the requirements class have been fulfilled." ;
    spec:requirement <http://www.opengis.net/spec/OMS/3.0/req/sam-cpt/Sampling/relatedSampling-sem> ;
    spec:testType spec:Capabilities ;
    skos:broader <http://www.opengis.net/spec/OMS/3.0/conf/sam-cpt/Sampling> ;
    skos:definition "Verify that all requirements from the requirements class have been fulfilled." ;
    skos:inScheme <http://www.opengis.net/spec/OMS/3.0> ;
    skos:prefLabel "Conformance Test http://www.opengis.net/spec/OMS/3.0/req/sam-cpt/Sampling/relatedSampling-sem" .

<http://www.opengis.net/spec/OMS/3.0/conf/sam-cpt/Sampling/sample-sem> a spec:ConformanceTest,
        skos:Concept ;
    spec:method "Inspect the documentation of the application, schema or profile." ;
    spec:purpose "Verify that all requirements from the requirements class have been fulfilled." ;
    spec:requirement <http://www.opengis.net/spec/OMS/3.0/req/sam-cpt/Sampling/sample-sem> ;
    spec:testType spec:Capabilities ;
    skos:broader <http://www.opengis.net/spec/OMS/3.0/conf/sam-cpt/Sampling> ;
    skos:definition "Verify that all requirements from the requirements class have been fulfilled." ;
    skos:inScheme <http://www.opengis.net/spec/OMS/3.0> ;
    skos:prefLabel "Conformance Test http://www.opengis.net/spec/OMS/3.0/req/sam-cpt/Sampling/sample-sem" .

<http://www.opengis.net/spec/OMS/3.0/conf/sam-cpt/Sampling/sampler-sem> a spec:ConformanceTest,
        skos:Concept ;
    spec:method "Inspect the documentation of the application, schema or profile." ;
    spec:purpose "Verify that all requirements from the requirements class have been fulfilled." ;
    spec:requirement <http://www.opengis.net/spec/OMS/3.0/req/sam-cpt/Sampling/sampler-sem> ;
    spec:testType spec:Capabilities ;
    skos:broader <http://www.opengis.net/spec/OMS/3.0/conf/sam-cpt/Sampling> ;
    skos:definition "Verify that all requirements from the requirements class have been fulfilled." ;
    skos:inScheme <http://www.opengis.net/spec/OMS/3.0> ;
    skos:prefLabel "Conformance Test http://www.opengis.net/spec/OMS/3.0/req/sam-cpt/Sampling/sampler-sem" .

<http://www.opengis.net/spec/OMS/3.0/conf/sam-cpt/Sampling/samplingProcedure-sem> a spec:ConformanceTest,
        skos:Concept ;
    spec:method "Inspect the documentation of the application, schema or profile." ;
    spec:purpose "Verify that all requirements from the requirements class have been fulfilled." ;
    spec:requirement <http://www.opengis.net/spec/OMS/3.0/req/sam-cpt/Sampling/samplingProcedure-sem> ;
    spec:testType spec:Capabilities ;
    skos:broader <http://www.opengis.net/spec/OMS/3.0/conf/sam-cpt/Sampling> ;
    skos:definition "Verify that all requirements from the requirements class have been fulfilled." ;
    skos:inScheme <http://www.opengis.net/spec/OMS/3.0> ;
    skos:prefLabel "Conformance Test http://www.opengis.net/spec/OMS/3.0/req/sam-cpt/Sampling/samplingProcedure-sem" .

<http://www.opengis.net/spec/OMS/3.0/conf/sam-cpt/SamplingProcedure/SamplingProcedure-sem> a spec:ConformanceTest,
        skos:Concept ;
    spec:method "Inspect the documentation of the application, schema or profile." ;
    spec:purpose "Verify that all requirements from the requirements class have been fulfilled." ;
    spec:requirement <http://www.opengis.net/spec/OMS/3.0/req/sam-cpt/SamplingProcedure/SamplingProcedure-sem> ;
    spec:testType spec:Capabilities ;
    skos:broader <http://www.opengis.net/spec/OMS/3.0/conf/sam-cpt/SamplingProcedure> ;
    skos:definition "Verify that all requirements from the requirements class have been fulfilled." ;
    skos:inScheme <http://www.opengis.net/spec/OMS/3.0> ;
    skos:prefLabel "Conformance Test http://www.opengis.net/spec/OMS/3.0/req/sam-cpt/SamplingProcedure/SamplingProcedure-sem" .

<http://www.opengis.net/spec/OMS/3.0/conf/sam-cpt/SamplingProcedure/sampler-sem> a spec:ConformanceTest,
        skos:Concept ;
    spec:method "Inspect the documentation of the application, schema or profile." ;
    spec:purpose "Verify that all requirements from the requirements class have been fulfilled." ;
    spec:requirement <http://www.opengis.net/spec/OMS/3.0/req/sam-cpt/SamplingProcedure/sampler-sem> ;
    spec:testType spec:Capabilities ;
    skos:broader <http://www.opengis.net/spec/OMS/3.0/conf/sam-cpt/SamplingProcedure> ;
    skos:definition "Verify that all requirements from the requirements class have been fulfilled." ;
    skos:inScheme <http://www.opengis.net/spec/OMS/3.0> ;
    skos:prefLabel "Conformance Test http://www.opengis.net/spec/OMS/3.0/req/sam-cpt/SamplingProcedure/sampler-sem" .

<http://www.opengis.net/spec/OMS/3.0/conf/sam-cpt/SamplingProcedure/sampling-sem> a spec:ConformanceTest,
        skos:Concept ;
    spec:method "Inspect the documentation of the application, schema or profile." ;
    spec:purpose "Verify that all requirements from the requirements class have been fulfilled." ;
    spec:requirement <http://www.opengis.net/spec/OMS/3.0/req/sam-cpt/SamplingProcedure/sampling-sem> ;
    spec:testType spec:Capabilities ;
    skos:broader <http://www.opengis.net/spec/OMS/3.0/conf/sam-cpt/SamplingProcedure> ;
    skos:definition "Verify that all requirements from the requirements class have been fulfilled." ;
    skos:inScheme <http://www.opengis.net/spec/OMS/3.0> ;
    skos:prefLabel "Conformance Test http://www.opengis.net/spec/OMS/3.0/req/sam-cpt/SamplingProcedure/sampling-sem" .




<http://www.opengis.net/spec/OMS/3.0/req/obs-basic> a spec:RequirementClass,
        skos:Concept ;
    skos:broader <http://www.opengis.net/spec/OMS/3.0/req/obs-basic/Observation> ;
    skos:broader <http://www.opengis.net/spec/OMS/3.0/req/obs-basic/ObservationCharacteristics> ;
    skos:broader <http://www.opengis.net/spec/OMS/3.0/req/obs-basic/ObservationCollection> ;
    skos:broader <http://www.opengis.net/spec/OMS/3.0/req/obs-basic/ObservingCapability> ;
    skos:broader <http://www.opengis.net/spec/OMS/3.0/req/obs-basic/ObservableProperty> ;
    skos:broader <http://www.opengis.net/spec/OMS/3.0/req/obs-basic/ObservingProcedure> ;
    skos:broader <http://www.opengis.net/spec/OMS/3.0/req/obs-basic/Observer> ;
    skos:broader <http://www.opengis.net/spec/OMS/3.0/req/obs-basic/Host> ;
    skos:broader <http://www.opengis.net/spec/OMS/3.0/req/obs-basic/Deployment> ;
    skos:broader <http://www.opengis.net/spec/OMS/3.0/req/obs-basic/GenericDomainFeature> ;
    skos:definition "/req/obs-basic" ;
    skos:inScheme <http://www.opengis.net/spec/OMS/3.0> ;
    skos:prefLabel "Requirement Class /req/obs-basic" .

<http://www.opengis.net/spec/OMS/3.0/req/obs-basic/Deployment> a spec:RequirementClass,
        skos:Concept ;
    spec:normativeStatement <http://www.opengis.net/spec/OMS/3.0/req/obs-basic/gen/link-sem> ;
    skos:broader <http://www.opengis.net/spec/OMS/3.0/req/obs-core/AbstractDeployment> ;
    skos:definition "/req/obs-basic/Deployment" ;
    skos:inScheme <http://www.opengis.net/spec/OMS/3.0> ;
    skos:prefLabel "Requirement Class /req/obs-basic/Deployment" .

<http://www.opengis.net/spec/OMS/3.0/req/obs-basic/GenericDomainFeature> a spec:RequirementClass,
        skos:Concept ;
    spec:normativeStatement <http://www.opengis.net/spec/OMS/3.0/req/obs-basic/GenericDomainFeature/GenericDomainFeature-sem> ;
    spec:normativeStatement <http://www.opengis.net/spec/OMS/3.0/req/obs-basic/gen/link-sem> ;
    spec:normativeStatement <http://www.opengis.net/spec/OMS/3.0/req/obs-basic/gen/location-sem> ;
    skos:definition "/req/obs-basic/GenericDomainFeature" ;
    skos:inScheme <http://www.opengis.net/spec/OMS/3.0> ;
    skos:prefLabel "Requirement Class /req/obs-basic/GenericDomainFeature" .

<http://www.opengis.net/spec/OMS/3.0/req/obs-basic/Host> a spec:RequirementClass,
        skos:Concept ;
    spec:normativeStatement <http://www.opengis.net/spec/OMS/3.0/req/obs-basic/gen/link-sem> ;
    spec:normativeStatement <http://www.opengis.net/spec/OMS/3.0/req/obs-basic/gen/location-sem> ;
    skos:broader <http://www.opengis.net/spec/OMS/3.0/req/obs-core/AbstractHost> ;
    skos:definition "/req/obs-basic/Host" ;
    skos:inScheme <http://www.opengis.net/spec/OMS/3.0> ;
    skos:prefLabel "Requirement Class /req/obs-basic/Host" .

<http://www.opengis.net/spec/OMS/3.0/req/obs-basic/ObservableProperty> a spec:RequirementClass,
        skos:Concept ;
    spec:normativeStatement <http://www.opengis.net/spec/OMS/3.0/req/obs-basic/gen/link-sem> ;
    skos:broader <http://www.opengis.net/spec/OMS/3.0/req/obs-core/AbstractObservableProperty> ;
    skos:definition "/req/obs-basic/ObservableProperty" ;
    skos:inScheme <http://www.opengis.net/spec/OMS/3.0> ;
    skos:prefLabel "Requirement Class /req/obs-basic/ObservableProperty" .

<http://www.opengis.net/spec/OMS/3.0/req/obs-basic/Observation> a spec:RequirementClass,
        skos:Concept ;
    skos:broader <http://www.opengis.net/spec/OMS/3.0/req/obs-core/AbstractObservation> ;
    skos:definition "/req/obs-basic/Observation" ;
    skos:inScheme <http://www.opengis.net/spec/OMS/3.0> ;
    skos:prefLabel "Requirement Class /req/obs-basic/Observation" .

<http://www.opengis.net/spec/OMS/3.0/req/obs-basic/ObservationCharacteristics> a spec:RequirementClass,
        skos:Concept ;
    skos:broader <http://www.opengis.net/spec/OMS/3.0/req/obs-core/AbstractObservationCharacteristics> ;
    skos:definition "/req/obs-basic/ObservationCharacteristics" ;
    skos:inScheme <http://www.opengis.net/spec/OMS/3.0> ;
    skos:prefLabel "Requirement Class /req/obs-basic/ObservationCharacteristics" .

<http://www.opengis.net/spec/OMS/3.0/req/obs-basic/ObservationCollection> a spec:RequirementClass,
        skos:Concept ;
    spec:normativeStatement <http://www.opengis.net/spec/OMS/3.0/req/obs-basic/ObservationCollection/ObservationCollection-sem> ;
    spec:normativeStatement <http://www.opengis.net/spec/OMS/3.0/req/obs-basic/ObservationCollection/collectionType-sem> ;
    spec:normativeStatement <http://www.opengis.net/spec/OMS/3.0/req/obs-basic/ObservationCollection/collectionType-homogenous-con> ;
    spec:normativeStatement <http://www.opengis.net/spec/OMS/3.0/req/obs-basic/ObservationCollection/collectionType-summarizing-con> ;
    spec:normativeStatement <http://www.opengis.net/spec/OMS/3.0/req/obs-basic/ObservationCollection/member-sem> ;
    spec:normativeStatement <http://www.opengis.net/spec/OMS/3.0/req/obs-basic/ObservationCollection/memberCharacteristics-sem> ;
    spec:normativeStatement <http://www.opengis.net/spec/OMS/3.0/req/obs-basic/ObservationCollection/relatedCollection-sem> ;
    spec:normativeStatement <http://www.opengis.net/spec/OMS/3.0/req/obs-basic/ObservationCollection/CollectionTypeByMemberCharacteristicsSemantics-sem> ;
    spec:normativeStatement <http://www.opengis.net/spec/OMS/3.0/req/obs-cpt/gen/relatedObservation-sem> ;
    skos:definition "/req/obs-basic/ObservationCollection" ;
    skos:inScheme <http://www.opengis.net/spec/OMS/3.0> ;
    skos:prefLabel "Requirement Class /req/obs-basic/ObservationCollection" .

<http://www.opengis.net/spec/OMS/3.0/req/obs-basic/Observer> a spec:RequirementClass,
        skos:Concept ;
    spec:normativeStatement <http://www.opengis.net/spec/OMS/3.0/req/obs-basic/gen/link-sem> ;
    spec:normativeStatement <http://www.opengis.net/spec/OMS/3.0/req/obs-basic/gen/location-sem> ;
    skos:broader <http://www.opengis.net/spec/OMS/3.0/req/obs-core/AbstractObserver> ;
    skos:definition "/req/obs-basic/Observer" ;
    skos:inScheme <http://www.opengis.net/spec/OMS/3.0> ;
    skos:prefLabel "Requirement Class /req/obs-basic/Observer" .

<http://www.opengis.net/spec/OMS/3.0/req/obs-basic/ObservingCapability> a spec:RequirementClass,
        skos:Concept ;
    spec:normativeStatement <http://www.opengis.net/spec/OMS/3.0/req/obs-basic/ObservingCapability/ObservingCapability-sem> ;
    skos:broader <http://www.opengis.net/spec/OMS/3.0/req/obs-basic/ObservationCharacteristics> ;
    skos:definition "/req/obs-basic/ObservingCapability" ;
    skos:inScheme <http://www.opengis.net/spec/OMS/3.0> ;
    skos:prefLabel "Requirement Class /req/obs-basic/ObservingCapability" .

<http://www.opengis.net/spec/OMS/3.0/req/obs-basic/ObservingProcedure> a spec:RequirementClass,
        skos:Concept ;
    spec:normativeStatement <http://www.opengis.net/spec/OMS/3.0/req/obs-basic/gen/link-sem> ;
    skos:broader <http://www.opengis.net/spec/OMS/3.0/req/obs-core/AbstractObservingProcedure> ;
    skos:definition "/req/obs-basic/ObservingProcedure" ;
    skos:inScheme <http://www.opengis.net/spec/OMS/3.0> ;
    skos:prefLabel "Requirement Class /req/obs-basic/ObservingProcedure" .

<http://www.opengis.net/spec/OMS/3.0/req/obs-core> a spec:RequirementClass,
        skos:Concept ;
    skos:broader <http://www.opengis.net/spec/OMS/3.0/req/obs-core/AbstractObservationCharacteristics> ;
    skos:broader <http://www.opengis.net/spec/OMS/3.0/req/obs-core/AbstractObservation> ;
    skos:broader <http://www.opengis.net/spec/OMS/3.0/req/obs-core/AbstractObservableProperty> ;
    skos:broader <http://www.opengis.net/spec/OMS/3.0/req/obs-core/AbstractObservingProcedure> ;
    skos:broader <http://www.opengis.net/spec/OMS/3.0/req/obs-core/AbstractObserver> ;
    skos:broader <http://www.opengis.net/spec/OMS/3.0/req/obs-core/AbstractHost> ;
    skos:broader <http://www.opengis.net/spec/OMS/3.0/req/obs-core/AbstractDeployment> ;
    skos:definition "/req/obs-core" ;
    skos:inScheme <http://www.opengis.net/spec/OMS/3.0> ;
    skos:prefLabel "Requirement Class /req/obs-core" .

<http://www.opengis.net/spec/OMS/3.0/req/obs-core/AbstractDeployment> a spec:RequirementClass,
        skos:Concept ;
    spec:normativeStatement <http://www.opengis.net/spec/OMS/3.0/req/obs-core/AbstractDeployment/deploymentReason-sem> ;
    spec:normativeStatement <http://www.opengis.net/spec/OMS/3.0/req/obs-core/AbstractDeployment/deploymentTime-sem> ;
    spec:normativeStatement <http://www.opengis.net/spec/OMS/3.0/req/obs-core/gen/metadata-sem> ;
    skos:broader <http://www.opengis.net/spec/OMS/3.0/req/obs-cpt/Deployment> ;
    skos:definition "/req/obs-core/AbstractDeployment" ;
    skos:inScheme <http://www.opengis.net/spec/OMS/3.0> ;
    skos:prefLabel "Requirement Class /req/obs-core/AbstractDeployment" .

<http://www.opengis.net/spec/OMS/3.0/req/obs-core/AbstractHost> a spec:RequirementClass,
        skos:Concept ;
    spec:normativeStatement <http://www.opengis.net/spec/OMS/3.0/req/obs-core/gen/metadata-sem> ;
    skos:broader <http://www.opengis.net/spec/OMS/3.0/req/obs-cpt/Host> ;
    skos:definition "/req/obs-core/AbstractHost" ;
    skos:inScheme <http://www.opengis.net/spec/OMS/3.0> ;
    skos:prefLabel "Requirement Class /req/obs-core/AbstractHost" .

<http://www.opengis.net/spec/OMS/3.0/req/obs-core/AbstractObservableProperty> a spec:RequirementClass,
        skos:Concept ;
    spec:normativeStatement <http://www.opengis.net/spec/OMS/3.0/req/obs-core/gen/metadata-sem> ;
    skos:broader <http://www.opengis.net/spec/OMS/3.0/req/obs-cpt/ObservableProperty> ;
    skos:definition "/req/obs-core/AbstractObservableProperty" ;
    skos:inScheme <http://www.opengis.net/spec/OMS/3.0> ;
    skos:prefLabel "Requirement Class /req/obs-core/AbstractObservableProperty" .

<http://www.opengis.net/spec/OMS/3.0/req/obs-core/AbstractObservation> a spec:RequirementClass,
        skos:Concept ;
    spec:normativeStatement <http://www.opengis.net/spec/OMS/3.0/req/obs-core/AbstractObservation/resultTime-type> ;
    spec:normativeStatement <http://www.opengis.net/spec/OMS/3.0/req/obs-core/AbstractObservation/validTime-type> ;
    spec:normativeStatement <http://www.opengis.net/spec/OMS/3.0/req/obs-cpt/Observation/phenomenonTime-card> ;
    spec:normativeStatement <http://www.opengis.net/spec/OMS/3.0/req/obs-cpt/Observation/resultTime-card> ;
    spec:normativeStatement <http://www.opengis.net/spec/OMS/3.0/req/obs-core/AbstractObservation/FoI-con> ;
    spec:normativeStatement <http://www.opengis.net/spec/OMS/3.0/req/obs-cpt/Observation/observedProperty-card> ;
    spec:normativeStatement <http://www.opengis.net/spec/OMS/3.0/req/obs-cpt/Observation/procedure-card> ;
    spec:normativeStatement <http://www.opengis.net/spec/OMS/3.0/req/obs-cpt/Observation/result-card> ;
    spec:normativeStatement <http://www.opengis.net/spec/OMS/3.0/req/obs-core/AbstractObservation/parameterName-card> ;
    skos:broader <http://www.opengis.net/spec/OMS/3.0/req/obs-core/AbstractObservationCharacteristics> ;
    skos:definition "/req/obs-core/AbstractObservation" ;
    skos:inScheme <http://www.opengis.net/spec/OMS/3.0> ;
    skos:prefLabel "Requirement Class /req/obs-core/AbstractObservation" .

<http://www.opengis.net/spec/OMS/3.0/req/obs-core/AbstractObservationCharacteristics> a spec:RequirementClass,
        skos:Concept ;
    spec:normativeStatement <http://www.opengis.net/spec/OMS/3.0/req/obs-core/AbstractObservationCharacteristics/AbstractObservationCharacteristics-sem> ;
    spec:normativeStatement <http://www.opengis.net/spec/OMS/3.0/req/obs-core/AbstractObservationCharacteristics/type-sem> ;
    spec:normativeStatement <http://www.opengis.net/spec/OMS/3.0/req/obs-core/AbstractObservationCharacteristics/parameter-sem> ;
    spec:normativeStatement <http://www.opengis.net/spec/OMS/3.0/req/obs-core/AbstractObservationCharacteristics/resultQuality-sem> ;
    spec:normativeStatement <http://www.opengis.net/spec/OMS/3.0/req/obs-cpt/Observation/phenomenonTime-sem> ;
    spec:normativeStatement <http://www.opengis.net/spec/OMS/3.0/req/obs-cpt/Observation/resultTime-sem> ;
    spec:normativeStatement <http://www.opengis.net/spec/OMS/3.0/req/obs-cpt/Observation/validTime-sem> ;
    spec:normativeStatement <http://www.opengis.net/spec/OMS/3.0/req/obs-cpt/Observation/featureOfInterest-sem> ;
    spec:normativeStatement <http://www.opengis.net/spec/OMS/3.0/req/obs-core/AbstractObservationCharacteristics/pFoI-sem> ;
    spec:normativeStatement <http://www.opengis.net/spec/OMS/3.0/req/obs-core/AbstractObservationCharacteristics/uFoI-sem> ;
    spec:normativeStatement <http://www.opengis.net/spec/OMS/3.0/req/obs-cpt/Observation/observedProperty-sem> ;
    spec:normativeStatement <http://www.opengis.net/spec/OMS/3.0/req/obs-cpt/Observation/result-sem> ;
    spec:normativeStatement <http://www.opengis.net/spec/OMS/3.0/req/obs-cpt/Observation/procedure-sem> ;
    spec:normativeStatement <http://www.opengis.net/spec/OMS/3.0/req/obs-cpt/Observation/observer-sem> ;
    spec:normativeStatement <http://www.opengis.net/spec/OMS/3.0/req/obs-cpt/Observation/host-sem> ;
    spec:normativeStatement <http://www.opengis.net/spec/OMS/3.0/req/obs-cpt/gen/relatedObservation-sem> ;
    spec:normativeStatement <http://www.opengis.net/spec/OMS/3.0/req/obs-core/gen/metadata-sem> ;
    skos:broader <http://www.opengis.net/spec/OMS/3.0/req/obs-core/NamedValue> ;
    skos:definition "/req/obs-core/AbstractObservationCharacteristics" ;
    skos:inScheme <http://www.opengis.net/spec/OMS/3.0> ;
    skos:prefLabel "Requirement Class /req/obs-core/AbstractObservationCharacteristics" .

<http://www.opengis.net/spec/OMS/3.0/req/obs-core/AbstractObserver> a spec:RequirementClass,
        skos:Concept ;
    spec:normativeStatement <http://www.opengis.net/spec/OMS/3.0/req/obs-core/gen/metadata-sem> ;
    skos:broader <http://www.opengis.net/spec/OMS/3.0/req/obs-cpt/Observer> ;
    skos:definition "/req/obs-core/AbstractObserver" ;
    skos:inScheme <http://www.opengis.net/spec/OMS/3.0> ;
    skos:prefLabel "Requirement Class /req/obs-core/AbstractObserver" .

<http://www.opengis.net/spec/OMS/3.0/req/obs-core/AbstractObservingProcedure> a spec:RequirementClass,
        skos:Concept ;
    spec:normativeStatement <http://www.opengis.net/spec/OMS/3.0/req/obs-core/gen/metadata-sem> ;
    skos:broader <http://www.opengis.net/spec/OMS/3.0/req/obs-cpt/ObservingProcedure> ;
    skos:definition "/req/obs-core/AbstractObservingProcedure" ;
    skos:inScheme <http://www.opengis.net/spec/OMS/3.0> ;
    skos:prefLabel "Requirement Class /req/obs-core/AbstractObservingProcedure" .

<http://www.opengis.net/spec/OMS/3.0/req/obs-core/NamedValue> a spec:RequirementClass,
        skos:Concept ;
    spec:normativeStatement <http://www.opengis.net/spec/OMS/3.0/req/obs-core/NamedValue/NamedValue-sem> ;
    spec:normativeStatement <http://www.opengis.net/spec/OMS/3.0/req/obs-core/NamedValue/name-sem> ;
    spec:normativeStatement <http://www.opengis.net/spec/OMS/3.0/req/obs-core/NamedValue/value-sem> ;
    skos:definition "/req/obs-core/NamedValue" ;
    skos:inScheme <http://www.opengis.net/spec/OMS/3.0> ;
    skos:prefLabel "Requirement Class /req/obs-core/NamedValue" .

<http://www.opengis.net/spec/OMS/3.0/req/obs-cpt> a spec:RequirementClass,
        skos:Concept ;
    skos:broader <http://www.opengis.net/spec/OMS/3.0/req/obs-cpt/Observation> ;
    skos:broader <http://www.opengis.net/spec/OMS/3.0/req/obs-cpt/ObservableProperty> ;
    skos:broader <http://www.opengis.net/spec/OMS/3.0/req/obs-cpt/Procedure> ;
    skos:broader <http://www.opengis.net/spec/OMS/3.0/req/obs-cpt/ObservingProcedure> ;
    skos:broader <http://www.opengis.net/spec/OMS/3.0/req/obs-cpt/Observer> ;
    skos:broader <http://www.opengis.net/spec/OMS/3.0/req/obs-cpt/Host> ;
    skos:broader <http://www.opengis.net/spec/OMS/3.0/req/obs-cpt/Deployment> ;
    skos:definition "/req/obs-cpt" ;
    skos:inScheme <http://www.opengis.net/spec/OMS/3.0> ;
    skos:prefLabel "Requirement Class /req/obs-cpt" .

<http://www.opengis.net/spec/OMS/3.0/req/obs-cpt/Deployment> a spec:RequirementClass,
        skos:Concept ;
    spec:normativeStatement <http://www.opengis.net/spec/OMS/3.0/req/obs-cpt/Deployment/Deployment-sem> ;
    spec:normativeStatement <http://www.opengis.net/spec/OMS/3.0/req/obs-cpt/Deployment/observer-sem> ;
    spec:normativeStatement <http://www.opengis.net/spec/OMS/3.0/req/obs-cpt/Deployment/host-sem> ;
    skos:definition "/req/obs-cpt/Deployment" ;
    skos:inScheme <http://www.opengis.net/spec/OMS/3.0> ;
    skos:prefLabel "Requirement Class /req/obs-cpt/Deployment" .

<http://www.opengis.net/spec/OMS/3.0/req/obs-cpt/Host> a spec:RequirementClass,
        skos:Concept ;
    spec:normativeStatement <http://www.opengis.net/spec/OMS/3.0/req/obs-cpt/Host/Host-sem> ;
    spec:normativeStatement <http://www.opengis.net/spec/OMS/3.0/req/obs-cpt/Host/deployment-sem> ;
    spec:normativeStatement <http://www.opengis.net/spec/OMS/3.0/req/obs-cpt/Host/relatedHost-sem> ;
    spec:normativeStatement <http://www.opengis.net/spec/OMS/3.0/req/obs-cpt/gen/relatedObservation-sem> ;
    skos:definition "/req/obs-cpt/Host" ;
    skos:inScheme <http://www.opengis.net/spec/OMS/3.0> ;
    skos:prefLabel "Requirement Class /req/obs-cpt/Host" .

<http://www.opengis.net/spec/OMS/3.0/req/obs-cpt/ObservableProperty> a spec:RequirementClass,
        skos:Concept ;
    spec:normativeStatement <http://www.opengis.net/spec/OMS/3.0/req/obs-cpt/ObservableProperty/ObservableProperty-sem> ;
    spec:normativeStatement <http://www.opengis.net/spec/OMS/3.0/req/obs-cpt/ObservableProperty/observer-sem> ;
    spec:normativeStatement <http://www.opengis.net/spec/OMS/3.0/req/obs-cpt/gen/relatedObservation-sem> ;
    skos:definition "/req/obs-cpt/ObservableProperty" ;
    skos:inScheme <http://www.opengis.net/spec/OMS/3.0> ;
    skos:prefLabel "Requirement Class /req/obs-cpt/ObservableProperty" .

<http://www.opengis.net/spec/OMS/3.0/req/obs-cpt/Observation> a spec:RequirementClass,
        skos:Concept ;
    spec:normativeStatement <http://www.opengis.net/spec/OMS/3.0/req/obs-cpt/Observation/Observation-sem> ;
    spec:normativeStatement <http://www.opengis.net/spec/OMS/3.0/req/obs-cpt/Observation/phenomenonTime-sem> ;
    spec:normativeStatement <http://www.opengis.net/spec/OMS/3.0/req/obs-cpt/Observation/phenomenonTime-card> ;
    spec:normativeStatement <http://www.opengis.net/spec/OMS/3.0/req/obs-cpt/Observation/resultTime-sem> ;
    spec:normativeStatement <http://www.opengis.net/spec/OMS/3.0/req/obs-cpt/Observation/resultTime-card> ;
    spec:normativeStatement <http://www.opengis.net/spec/OMS/3.0/req/obs-cpt/Observation/validTime-sem> ;
    spec:normativeStatement <http://www.opengis.net/spec/OMS/3.0/req/obs-cpt/Observation/featureOfInterest-sem> ;
    spec:normativeStatement <http://www.opengis.net/spec/OMS/3.0/req/obs-cpt/Observation/featureOfInterest-card> ;
    spec:normativeStatement <http://www.opengis.net/spec/OMS/3.0/req/obs-cpt/Observation/observedProperty-sem> ;
    spec:normativeStatement <http://www.opengis.net/spec/OMS/3.0/req/obs-cpt/Observation/observedProperty-card> ;
    spec:normativeStatement <http://www.opengis.net/spec/OMS/3.0/req/obs-cpt/Observation/result-sem> ;
    spec:normativeStatement <http://www.opengis.net/spec/OMS/3.0/req/obs-cpt/Observation/result-card> ;
    spec:normativeStatement <http://www.opengis.net/spec/OMS/3.0/req/obs-cpt/Observation/observingProcedure-sem> ;
    spec:normativeStatement <http://www.opengis.net/spec/OMS/3.0/req/obs-cpt/Observation/observingProcedure-card> ;
    spec:normativeStatement <http://www.opengis.net/spec/OMS/3.0/req/obs-cpt/Observation/observer-sem> ;
    spec:normativeStatement <http://www.opengis.net/spec/OMS/3.0/req/obs-cpt/Observation/host-sem> ;
    spec:normativeStatement <http://www.opengis.net/spec/OMS/3.0/req/obs-cpt/gen/relatedObservation-sem> ;
    skos:definition "/req/obs-cpt/Observation" ;
    skos:inScheme <http://www.opengis.net/spec/OMS/3.0> ;
    skos:prefLabel "Requirement Class /req/obs-cpt/Observation" .

<http://www.opengis.net/spec/OMS/3.0/req/obs-cpt/Observer> a spec:RequirementClass,
        skos:Concept ;
    spec:normativeStatement <http://www.opengis.net/spec/OMS/3.0/req/obs-cpt/Observer/Observer-sem> ;
    spec:normativeStatement <http://www.opengis.net/spec/OMS/3.0/req/obs-cpt/Observer/observableProperty-sem> ;
    spec:normativeStatement <http://www.opengis.net/spec/OMS/3.0/req/obs-cpt/Observer/observingProcedure-sem> ;
    spec:normativeStatement <http://www.opengis.net/spec/OMS/3.0/req/obs-cpt/Observer/deployment-sem> ;
    spec:normativeStatement <http://www.opengis.net/spec/OMS/3.0/req/obs-cpt/gen/relatedObservation-sem> ;
    skos:definition "/req/obs-cpt/Observer" ;
    skos:inScheme <http://www.opengis.net/spec/OMS/3.0> ;
    skos:prefLabel "Requirement Class /req/obs-cpt/Observer" .

<http://www.opengis.net/spec/OMS/3.0/req/obs-cpt/ObservingProcedure> a spec:RequirementClass,
        skos:Concept ;
    spec:normativeStatement <http://www.opengis.net/spec/OMS/3.0/req/obs-cpt/ObservingProcedure/ObservingProcedure-sem> ;
    spec:normativeStatement <http://www.opengis.net/spec/OMS/3.0/req/obs-cpt/ObservingProcedure/observer-sem> ;
    spec:normativeStatement <http://www.opengis.net/spec/OMS/3.0/req/obs-cpt/gen/relatedObservation-sem> ;
    skos:broader <http://www.opengis.net/spec/OMS/3.0/req/obs-cpt/Procedure> ;
    skos:definition "/req/obs-cpt/ObservingProcedure" ;
    skos:inScheme <http://www.opengis.net/spec/OMS/3.0> ;
    skos:prefLabel "Requirement Class /req/obs-cpt/ObservingProcedure" .

<http://www.opengis.net/spec/OMS/3.0/req/obs-cpt/Procedure> a spec:RequirementClass,
        skos:Concept ;
    spec:normativeStatement <http://www.opengis.net/spec/OMS/3.0/req/obs-cpt/Procedure/Procedure-sem> ;
    skos:definition "/req/obs-cpt/Procedure" ;
    skos:inScheme <http://www.opengis.net/spec/OMS/3.0> ;
    skos:prefLabel "Requirement Class /req/obs-cpt/Procedure" .

<http://www.opengis.net/spec/OMS/3.0/req/sam-basic> a spec:RequirementClass,
        skos:Concept ;
    skos:broader <http://www.opengis.net/spec/OMS/3.0/req/sam-basic/Sample> ;
    skos:broader <http://www.opengis.net/spec/OMS/3.0/req/sam-basic/SpatialSample> ;
    skos:broader <http://www.opengis.net/spec/OMS/3.0/req/sam-basic/MaterialSample> ;
    skos:broader <http://www.opengis.net/spec/OMS/3.0/req/sam-basic/StatisticalSample> ;
    skos:broader <http://www.opengis.net/spec/OMS/3.0/req/sam-basic/Sampling> ;
    skos:broader <http://www.opengis.net/spec/OMS/3.0/req/sam-basic/Sampler> ;
    skos:broader <http://www.opengis.net/spec/OMS/3.0/req/sam-basic/SampleCollection> ;
    skos:definition "/req/sam-basic" ;
    skos:inScheme <http://www.opengis.net/spec/OMS/3.0> ;
    skos:prefLabel "Requirement Class /req/sam-basic" .

<http://www.opengis.net/spec/OMS/3.0/req/sam-basic/MaterialSample> a spec:RequirementClass,
        skos:Concept ;
    spec:normativeStatement <http://www.opengis.net/spec/OMS/3.0/req/sam-basic/MaterialSample/MaterialSample-sem> ;
    spec:normativeStatement <http://www.opengis.net/spec/OMS/3.0/req/sam-basic/MaterialSample/size-sem> ;
    spec:normativeStatement <http://www.opengis.net/spec/OMS/3.0/req/sam-basic/MaterialSample/storageLocation-sem> ;
    spec:normativeStatement <http://www.opengis.net/spec/OMS/3.0/req/sam-basic/MaterialSample/sourceLocation-sem> ;
    skos:broader <http://www.opengis.net/spec/OMS/3.0/req/sam-basic/Sample> ;
    skos:broader <http://www.opengis.net/spec/OMS/3.0/req/sam-basic/PhysicalDimension> ;
    skos:broader <http://www.opengis.net/spec/OMS/3.0/req/sam-basic/NamedLocation> ;
    skos:definition "/req/sam-basic/MaterialSample" ;
    skos:inScheme <http://www.opengis.net/spec/OMS/3.0> ;
    skos:prefLabel "Requirement Class /req/sam-basic/MaterialSample" .

<http://www.opengis.net/spec/OMS/3.0/req/sam-basic/NamedLocation> a spec:RequirementClass,
        skos:Concept ;
    spec:normativeStatement <http://www.opengis.net/spec/OMS/3.0/req/sam-basic/NamedLocation/NamedLocation-sem> ;
    spec:normativeStatement <http://www.opengis.net/spec/OMS/3.0/req/sam-basic/NamedLocation/address-sem> ;
    spec:normativeStatement <http://www.opengis.net/spec/OMS/3.0/req/sam-basic/NamedLocation/name-sem> ;
    spec:normativeStatement <http://www.opengis.net/spec/OMS/3.0/req/sam-basic/NamedLocation/representativeGeometry-sem> ;
    skos:definition "/req/sam-basic/NamedLocation" ;
    skos:inScheme <http://www.opengis.net/spec/OMS/3.0> ;
    skos:prefLabel "Requirement Class /req/sam-basic/NamedLocation" .

<http://www.opengis.net/spec/OMS/3.0/req/sam-basic/PhysicalDimension> a spec:RequirementClass,
        skos:Concept ;
    spec:normativeStatement <http://www.opengis.net/spec/OMS/3.0/req/sam-basic/PhysicalDimension/PhysicalDimension-sem> ;
    spec:normativeStatement <http://www.opengis.net/spec/OMS/3.0/req/sam-basic/PhysicalDimension/dimension-sem> ;
    spec:normativeStatement <http://www.opengis.net/spec/OMS/3.0/req/sam-basic/PhysicalDimension/value-sem> ;
    skos:definition "/req/sam-basic/PhysicalDimension" ;
    skos:inScheme <http://www.opengis.net/spec/OMS/3.0> ;
    skos:prefLabel "Requirement Class /req/sam-basic/PhysicalDimension" .

<http://www.opengis.net/spec/OMS/3.0/req/sam-basic/Sample> a spec:RequirementClass,
        skos:Concept ;
    skos:broader <http://www.opengis.net/spec/OMS/3.0/req/sam-core/AbstractSample> ;
    skos:definition "/req/sam-basic/Sample" ;
    skos:inScheme <http://www.opengis.net/spec/OMS/3.0> ;
    skos:prefLabel "Requirement Class /req/sam-basic/Sample" .

<http://www.opengis.net/spec/OMS/3.0/req/sam-basic/SampleCollection> a spec:RequirementClass,
        skos:Concept ;
    spec:normativeStatement <http://www.opengis.net/spec/OMS/3.0/req/sam-basic/SampleCollection/SampleCollection-sem> ;
    spec:normativeStatement <http://www.opengis.net/spec/OMS/3.0/req/sam-basic/SampleCollection/member-sem> ;
    spec:normativeStatement <http://www.opengis.net/spec/OMS/3.0/req/sam-basic/SampleCollection/relatedCollection-sem> ;
    spec:normativeStatement <http://www.opengis.net/spec/OMS/3.0/req/obs-core/gen/metadata-sem> ;
    skos:definition "/req/sam-basic/SampleCollection" ;
    skos:inScheme <http://www.opengis.net/spec/OMS/3.0> ;
    skos:prefLabel "Requirement Class /req/sam-basic/SampleCollection" .

<http://www.opengis.net/spec/OMS/3.0/req/sam-basic/Sampler> a spec:RequirementClass,
        skos:Concept ;
    skos:broader <http://www.opengis.net/spec/OMS/3.0/req/sam-core/AbstractSampler> ;
    skos:definition "/req/sam-basic/Sampler" ;
    skos:inScheme <http://www.opengis.net/spec/OMS/3.0> ;
    skos:prefLabel "Requirement Class /req/sam-basic/Sampler" .

<http://www.opengis.net/spec/OMS/3.0/req/sam-basic/Sampling> a spec:RequirementClass,
        skos:Concept ;
    skos:broader <http://www.opengis.net/spec/OMS/3.0/req/sam-core/AbstractSampling> ;
    skos:definition "/req/sam-basic/Sampling" ;
    skos:inScheme <http://www.opengis.net/spec/OMS/3.0> ;
    skos:prefLabel "Requirement Class /req/sam-basic/Sampling" .

<http://www.opengis.net/spec/OMS/3.0/req/sam-basic/SpatialSample> a spec:RequirementClass,
        skos:Concept ;
    spec:normativeStatement <http://www.opengis.net/spec/OMS/3.0/req/sam-basic/SpatialSample/SpatialSample-sem> ;
    spec:normativeStatement <http://www.opengis.net/spec/OMS/3.0/req/sam-basic/SpatialSample/shape-sem> ;
    spec:normativeStatement <http://www.opengis.net/spec/OMS/3.0/req/sam-basic/SpatialSample/horizontalPositionalAccuracy-sem> ;
    spec:normativeStatement <http://www.opengis.net/spec/OMS/3.0/req/sam-basic/SpatialSample/verticalPositionalAccuracy-sem> ;
    skos:broader <http://www.opengis.net/spec/OMS/3.0/req/sam-basic/Sample> ;
    skos:definition "/req/sam-basic/SpatialSample" ;
    skos:inScheme <http://www.opengis.net/spec/OMS/3.0> ;
    skos:prefLabel "Requirement Class /req/sam-basic/SpatialSample" .

<http://www.opengis.net/spec/OMS/3.0/req/sam-basic/StatisticalClassification> a spec:RequirementClass,
        skos:Concept ;
    spec:normativeStatement <http://www.opengis.net/spec/OMS/3.0/req/sam-basic/StatisticalClassification/StatisticalClassification-sem> ;
    spec:normativeStatement <http://www.opengis.net/spec/OMS/3.0/req/sam-basic/StatisticalClassification/concept-sem> ;
    spec:normativeStatement <http://www.opengis.net/spec/OMS/3.0/req/sam-basic/StatisticalClassification/classification-sem> ;
    skos:definition "/req/sam-basic/StatisticalClassification" ;
    skos:inScheme <http://www.opengis.net/spec/OMS/3.0> ;
    skos:prefLabel "Requirement Class /req/sam-basic/StatisticalClassification" .

<http://www.opengis.net/spec/OMS/3.0/req/sam-basic/StatisticalSample> a spec:RequirementClass,
        skos:Concept ;
    spec:normativeStatement <http://www.opengis.net/spec/OMS/3.0/req/sam-basic/StatisticalSample/StatisticalSample-sem> ;
    spec:normativeStatement <http://www.opengis.net/spec/OMS/3.0/req/sam-basic/StatisticalSample/classification-sem> ;
    skos:broader <http://www.opengis.net/spec/OMS/3.0/req/sam-basic/Sample> ;
    skos:broader <http://www.opengis.net/spec/OMS/3.0/req/sam-basic/StatisticalClassification> ;
    skos:definition "/req/sam-basic/StatisticalSample" ;
    skos:inScheme <http://www.opengis.net/spec/OMS/3.0> ;
    skos:prefLabel "Requirement Class /req/sam-basic/StatisticalSample" .

<http://www.opengis.net/spec/OMS/3.0/req/sam-core> a spec:RequirementClass,
        skos:Concept ;
    skos:broader <http://www.opengis.net/spec/OMS/3.0/req/sam-core/AbstractSample> ;
    skos:broader <http://www.opengis.net/spec/OMS/3.0/req/sam-core/AbstractSampling> ;
    skos:broader <http://www.opengis.net/spec/OMS/3.0/req/sam-core/AbstractSampler> ;
    skos:broader <http://www.opengis.net/spec/OMS/3.0/req/sam-core/AbstractSamplingProcedure> ;
    skos:broader <http://www.opengis.net/spec/OMS/3.0/req/sam-core/AbstractPreparationProcedure> ;
    skos:broader <http://www.opengis.net/spec/OMS/3.0/req/sam-core/AbstractPreparationStep> ;
    skos:definition "/req/sam-core" ;
    skos:inScheme <http://www.opengis.net/spec/OMS/3.0> ;
    skos:prefLabel "Requirement Class /req/sam-core" .

<http://www.opengis.net/spec/OMS/3.0/req/sam-core/AbstractPreparationProcedure> a spec:RequirementClass,
        skos:Concept ;
    spec:normativeStatement <http://www.opengis.net/spec/OMS/3.0/req/obs-core/gen/metadata-sem> ;
    skos:broader <http://www.opengis.net/spec/OMS/3.0/req/sam-cpt/PreparationProcedure> ;
    skos:definition "/req/sam-core/AbstractPreparationProcedure" ;
    skos:inScheme <http://www.opengis.net/spec/OMS/3.0> ;
    skos:prefLabel "Requirement Class /req/sam-core/AbstractPreparationProcedure" .

<http://www.opengis.net/spec/OMS/3.0/req/sam-core/AbstractPreparationStep> a spec:RequirementClass,
        skos:Concept ;
    spec:normativeStatement <http://www.opengis.net/spec/OMS/3.0/req/sam-core/AbstractPreparationStep/description-sem> ;
    spec:normativeStatement <http://www.opengis.net/spec/OMS/3.0/req/sam-core/AbstractPreparationStep/time-sem> ;
    spec:normativeStatement <http://www.opengis.net/spec/OMS/3.0/req/obs-core/gen/metadata-sem> ;
    skos:broader <http://www.opengis.net/spec/OMS/3.0/req/sam-cpt/PreparationStep> ;
    skos:definition "/req/sam-core/AbstractPreparationStep" ;
    skos:inScheme <http://www.opengis.net/spec/OMS/3.0> ;
    skos:prefLabel "Requirement Class /req/sam-core/AbstractPreparationStep" .

<http://www.opengis.net/spec/OMS/3.0/req/sam-core/AbstractSample> a spec:RequirementClass,
        skos:Concept ;
    spec:normativeStatement <http://www.opengis.net/spec/OMS/3.0/req/sam-core/AbstractSample/sampleType-sem> ;
    spec:normativeStatement <http://www.opengis.net/spec/OMS/3.0/req/sam-core/AbstractSample/parameter-sem> ;
    spec:normativeStatement <http://www.opengis.net/spec/OMS/3.0/req/obs-core/gen/metadata-sem> ;
    skos:broader <http://www.opengis.net/spec/OMS/3.0/req/sam-cpt/Sample> ;
    skos:broader <http://www.opengis.net/spec/OMS/3.0/req/obs-core/NamedValue> ;
    skos:definition "/req/sam-core/AbstractSample" ;
    skos:inScheme <http://www.opengis.net/spec/OMS/3.0> ;
    skos:prefLabel "Requirement Class /req/sam-core/AbstractSample" .

<http://www.opengis.net/spec/OMS/3.0/req/sam-core/AbstractSampler> a spec:RequirementClass,
        skos:Concept ;
    spec:normativeStatement <http://www.opengis.net/spec/OMS/3.0/req/sam-core/AbstractSampler/samplerType-sem> ;
    spec:normativeStatement <http://www.opengis.net/spec/OMS/3.0/req/obs-core/gen/metadata-sem> ;
    skos:broader <http://www.opengis.net/spec/OMS/3.0/req/sam-cpt/Sampler> ;
    skos:definition "/req/sam-core/AbstractSampler" ;
    skos:inScheme <http://www.opengis.net/spec/OMS/3.0> ;
    skos:prefLabel "Requirement Class /req/sam-core/AbstractSampler" .

<http://www.opengis.net/spec/OMS/3.0/req/sam-core/AbstractSampling> a spec:RequirementClass,
        skos:Concept ;
    spec:normativeStatement <http://www.opengis.net/spec/OMS/3.0/req/sam-core/AbstractSampling/samplingLocation-sem> ;
    spec:normativeStatement <http://www.opengis.net/spec/OMS/3.0/req/sam-core/AbstractSampling/time-sem> ;
    spec:normativeStatement <http://www.opengis.net/spec/OMS/3.0/req/sam-core/AbstractSampling/parameter-sem> ;
    spec:normativeStatement <http://www.opengis.net/spec/OMS/3.0/req/obs-core/gen/metadata-sem> ;
    skos:broader <http://www.opengis.net/spec/OMS/3.0/req/sam-cpt/Sampling> ;
    skos:broader <http://www.opengis.net/spec/OMS/3.0/req/obs-core/NamedValue> ;
    skos:definition "/req/sam-core/AbstractSampling" ;
    skos:inScheme <http://www.opengis.net/spec/OMS/3.0> ;
    skos:prefLabel "Requirement Class /req/sam-core/AbstractSampling" .

<http://www.opengis.net/spec/OMS/3.0/req/sam-core/AbstractSamplingProcedure> a spec:RequirementClass,
        skos:Concept ;
    spec:normativeStatement <http://www.opengis.net/spec/OMS/3.0/req/obs-core/gen/metadata-sem> ;
    skos:broader <http://www.opengis.net/spec/OMS/3.0/req/sam-cpt/SamplingProcedure> ;
    skos:definition "/req/sam-core/AbstractSamplingProcedure" ;
    skos:inScheme <http://www.opengis.net/spec/OMS/3.0> ;
    skos:prefLabel "Requirement Class /req/sam-core/AbstractSamplingProcedure" .

<http://www.opengis.net/spec/OMS/3.0/req/sam-cpt> a spec:RequirementClass,
        skos:Concept ;
    skos:broader <http://www.opengis.net/spec/OMS/3.0/req/sam-cpt/Sample> ;
    skos:broader <http://www.opengis.net/spec/OMS/3.0/req/sam-cpt/Sampling> ;
    skos:broader <http://www.opengis.net/spec/OMS/3.0/req/sam-cpt/Sampler> ;
    skos:broader <http://www.opengis.net/spec/OMS/3.0/req/sam-cpt/PreparationStep> ;
    skos:broader <http://www.opengis.net/spec/OMS/3.0/req/sam-cpt/PreparationProcedure> ;
    skos:broader <http://www.opengis.net/spec/OMS/3.0/req/sam-cpt/SamplingProcedure> ;
    skos:definition "/req/sam-cpt" ;
    skos:inScheme <http://www.opengis.net/spec/OMS/3.0> ;
    skos:prefLabel "Requirement Class /req/sam-cpt" .

<http://www.opengis.net/spec/OMS/3.0/req/sam-cpt/PreparationProcedure> a spec:RequirementClass,
        skos:Concept ;
    spec:normativeStatement <http://www.opengis.net/spec/OMS/3.0/req/sam-cpt/PreparationProcedure/PreparationProcedure-sem> ;
    spec:normativeStatement <http://www.opengis.net/spec/OMS/3.0/req/sam-cpt/PreparationProcedure/samplePreparationStep-sem> ;
    skos:broader <http://www.opengis.net/spec/OMS/3.0/req/obs-cpt/Procedure> ;
    skos:definition "/req/sam-cpt/PreparationProcedure" ;
    skos:inScheme <http://www.opengis.net/spec/OMS/3.0> ;
    skos:prefLabel "Requirement Class /req/sam-cpt/PreparationProcedure" .

<http://www.opengis.net/spec/OMS/3.0/req/sam-cpt/PreparationStep> a spec:RequirementClass,
        skos:Concept ;
    spec:normativeStatement <http://www.opengis.net/spec/OMS/3.0/req/sam-cpt/PreparationStep/PreparationStep-sem> ;
    spec:normativeStatement <http://www.opengis.net/spec/OMS/3.0/req/sam-cpt/PreparationStep/processingDetails-sem> ;
    spec:normativeStatement <http://www.opengis.net/spec/OMS/3.0/req/sam-cpt/PreparationStep/preparedSample-sem> ;
    skos:definition "/req/sam-cpt/PreparationStep" ;
    skos:inScheme <http://www.opengis.net/spec/OMS/3.0> ;
    skos:prefLabel "Requirement Class /req/sam-cpt/PreparationStep" .

<http://www.opengis.net/spec/OMS/3.0/req/sam-cpt/Sample> a spec:RequirementClass,
        skos:Concept ;
    spec:normativeStatement <http://www.opengis.net/spec/OMS/3.0/req/sam-cpt/Sample/Sample-sem> ;
    spec:normativeStatement <http://www.opengis.net/spec/OMS/3.0/req/sam-cpt/Sample/sampling-sem> ;
    spec:normativeStatement <http://www.opengis.net/spec/OMS/3.0/req/sam-cpt/Sample/preparationStep-sem> ;
    spec:normativeStatement <http://www.opengis.net/spec/OMS/3.0/req/sam-cpt/Sample/sampledFeature-sem> ;
    spec:normativeStatement <http://www.opengis.net/spec/OMS/3.0/req/sam-cpt/Sample/sampledFeature-card> ;
    spec:normativeStatement <http://www.opengis.net/spec/OMS/3.0/req/sam-cpt/Sample/relatedSample-sem> ;
    spec:normativeStatement <http://www.opengis.net/spec/OMS/3.0/req/obs-cpt/gen/relatedObservation-sem> ;
    skos:definition "/req/sam-cpt/Sample" ;
    skos:inScheme <http://www.opengis.net/spec/OMS/3.0> ;
    skos:prefLabel "Requirement Class /req/sam-cpt/Sample" .

<http://www.opengis.net/spec/OMS/3.0/req/sam-cpt/Sampler> a spec:RequirementClass,
        skos:Concept ;
    spec:normativeStatement <http://www.opengis.net/spec/OMS/3.0/req/sam-cpt/Sampler/Sampler-sem> ;
    spec:normativeStatement <http://www.opengis.net/spec/OMS/3.0/req/sam-cpt/Sampler/sampling-sem> ;
    spec:normativeStatement <http://www.opengis.net/spec/OMS/3.0/req/sam-cpt/Sampler/implementedProcedure-sem> ;
    skos:definition "/req/sam-cpt/Sampler" ;
    skos:inScheme <http://www.opengis.net/spec/OMS/3.0> ;
    skos:prefLabel "Requirement Class /req/sam-cpt/Sampler" .

<http://www.opengis.net/spec/OMS/3.0/req/sam-cpt/Sampling> a spec:RequirementClass,
        skos:Concept ;
    spec:normativeStatement <http://www.opengis.net/spec/OMS/3.0/req/sam-cpt/Sampling/Sampling-sem> ;
    spec:normativeStatement <http://www.opengis.net/spec/OMS/3.0/req/sam-cpt/Sampling/sample-sem> ;
    spec:normativeStatement <http://www.opengis.net/spec/OMS/3.0/req/sam-cpt/Sampling/featureOfInterest-sem> ;
    spec:normativeStatement <http://www.opengis.net/spec/OMS/3.0/req/sam-cpt/Sampling/featureOfInterest-card> ;
    spec:normativeStatement <http://www.opengis.net/spec/OMS/3.0/req/sam-cpt/Sampling/sampler-sem> ;
    spec:normativeStatement <http://www.opengis.net/spec/OMS/3.0/req/sam-cpt/Sampling/samplingProcedure-sem> ;
    spec:normativeStatement <http://www.opengis.net/spec/OMS/3.0/req/sam-cpt/Sampling/relatedSampling-sem> ;
    skos:definition "/req/sam-cpt/Sampling" ;
    skos:inScheme <http://www.opengis.net/spec/OMS/3.0> ;
    skos:prefLabel "Requirement Class /req/sam-cpt/Sampling" .

<http://www.opengis.net/spec/OMS/3.0/req/sam-cpt/SamplingProcedure> a spec:RequirementClass,
        skos:Concept ;
    spec:normativeStatement <http://www.opengis.net/spec/OMS/3.0/req/sam-cpt/SamplingProcedure/SamplingProcedure-sem> ;
    spec:normativeStatement <http://www.opengis.net/spec/OMS/3.0/req/sam-cpt/SamplingProcedure/sampling-sem> ;
    spec:normativeStatement <http://www.opengis.net/spec/OMS/3.0/req/sam-cpt/SamplingProcedure/sampler-sem> ;
    skos:broader <http://www.opengis.net/spec/OMS/3.0/req/obs-cpt/Procedure> ;
    skos:definition "/req/sam-cpt/SamplingProcedure" ;
    skos:inScheme <http://www.opengis.net/spec/OMS/3.0> ;
    skos:prefLabel "Requirement Class /req/sam-cpt/SamplingProcedure" .




<http://www.opengis.net/spec/OMS/3.0/req/obs-basic/GenericDomainFeature/GenericDomainFeature-sem> a spec:Requirement,
        skos:Concept ;
    dcterms:description "A concrete featureType to be utilized as featureOfInterest of an Observation." ;
    skos:broader <http://www.opengis.net/spec/OMS/3.0/req/obs-basic/GenericDomainFeature> ;
    skos:definition "A concrete featureType to be utilized as featureOfInterest of an Observation." ;
    skos:inScheme <http://www.opengis.net/spec/OMS/3.0> ;
    skos:prefLabel "Requirement: /req/obs-basic/GenericDomainFeature/GenericDomainFeature-sem" .

<http://www.opengis.net/spec/OMS/3.0/req/obs-basic/ObservationCollection/AbstractObservationCollectionTypeCodeListValue-sem> a spec:Requirement,
        skos:Concept ;
    dcterms:description "A codelist detailing the semantics of collection types. A concrete realization must be created for the application." ;
    skos:definition "A codelist detailing the semantics of collection types. A concrete realization must be created for the application." ;
    skos:inScheme <http://www.opengis.net/spec/OMS/3.0> ;
    skos:prefLabel "Requirement: /req/obs-basic/ObservationCollection/AbstractObservationCollectionTypeCodeListValue-sem" .

<http://www.opengis.net/spec/OMS/3.0/req/obs-basic/ObservationCollection/CollectionTypeByMemberCharacteristicsSemantics-sem> a spec:Requirement,
        skos:Concept ;
    dcterms:description "The following entries SHALL be provided: â Â Â Â Â Â Â  homogenous: all observations contained are of a similar nature â Â Â Â Â Â Â  summarizing: a wider grab-bag type of collection" ;
    skos:broader <http://www.opengis.net/spec/OMS/3.0/req/obs-basic/ObservationCollection> ;
    skos:definition "The following entries SHALL be provided: â Â Â Â Â Â Â  homogenous: all observations contained are of a similar nature â Â Â Â Â Â Â  summarizing: a wider grab-bag type of collection" ;
    skos:inScheme <http://www.opengis.net/spec/OMS/3.0> ;
    skos:prefLabel "Requirement: /req/obs-basic/ObservationCollection/CollectionTypeByMemberCharacteristicsSemantics-sem" .

<http://www.opengis.net/spec/OMS/3.0/req/obs-basic/ObservationCollection/ObservationCollection-sem> a spec:Requirement,
        skos:Concept ;
    dcterms:description "A collection of similar Observation s" ;
    skos:broader <http://www.opengis.net/spec/OMS/3.0/req/obs-basic/ObservationCollection> ;
    skos:definition "A collection of similar Observation s" ;
    skos:inScheme <http://www.opengis.net/spec/OMS/3.0> ;
    skos:prefLabel "Requirement: /req/obs-basic/ObservationCollection/ObservationCollection-sem" .

<http://www.opengis.net/spec/OMS/3.0/req/obs-basic/ObservationCollection/collectionType-homogenous-con> a spec:Requirement,
        skos:Concept ;
    dcterms:description "" ;
    skos:broader <http://www.opengis.net/spec/OMS/3.0/req/obs-basic/ObservationCollection> ;
    skos:definition "" ;
    skos:inScheme <http://www.opengis.net/spec/OMS/3.0> ;
    skos:prefLabel "Requirement: /req/obs-basic/ObservationCollection/collectionType-homogenous-con" .

<http://www.opengis.net/spec/OMS/3.0/req/obs-basic/ObservationCollection/collectionType-sem> a spec:Requirement,
        skos:Concept ;
    dcterms:description "" ;
    skos:broader <http://www.opengis.net/spec/OMS/3.0/req/obs-basic/ObservationCollection> ;
    skos:definition "" ;
    skos:inScheme <http://www.opengis.net/spec/OMS/3.0> ;
    skos:prefLabel "Requirement: /req/obs-basic/ObservationCollection/collectionType-sem" .

<http://www.opengis.net/spec/OMS/3.0/req/obs-basic/ObservationCollection/collectionType-summarizing-con> a spec:Requirement,
        skos:Concept ;
    dcterms:description "If collectionType is specified as summarizingObservationCollection from the CollectionTypeByMemberCharacteristicsSemantics Codelist , the following constraints apply to the associated ObservationCharacteristics and all Observation instances referenced via the member association. If multiple values for a property are available in the contained observations, ALL values for this attribute (or the range of values contained in all Observations) are provided in the ObservationCharacteristics. A property may also be empty in the ObservationCharacteristics - in this case any value can be provided for this attribute within the contained Observations: â Â Â Â Â Â  property not provided - values may be provided by the observations but a summary is not provided at this level â Â Â Â Â Â Â  property provided but with no content - no observation within the collection provides this property â Â Â Â Â Â  property = value - this value applies to all observations within the collection â Â Â Â Â Â  property = value set/range - all observations provide a value within this set/range" ;
    skos:broader <http://www.opengis.net/spec/OMS/3.0/req/obs-basic/ObservationCollection> ;
    skos:definition "If collectionType is specified as summarizingObservationCollection from the CollectionTypeByMemberCharacteristicsSemantics Codelist , the following constraints apply to the associated ObservationCharacteristics and all Observation instances referenced via the member association. If multiple values for a property are available in the contained observations, ALL values for this attribute (or the range of values contained in all Observations) are provided in the ObservationCharacteristics. A property may also be empty in the ObservationCharacteristics - in this case any value can be provided for this attribute within the contained Observations: â Â Â Â Â Â  property not provided - values may be provided by the observations but a summary is not provided at this level â Â Â Â Â Â Â  property provided but with no content - no observation within the collection provides this property â Â Â Â Â Â  property = value - this value applies to all observations within the collection â Â Â Â Â Â  property = value set/range - all observations provide a value within this set/range" ;
    skos:inScheme <http://www.opengis.net/spec/OMS/3.0> ;
    skos:prefLabel "Requirement: /req/obs-basic/ObservationCollection/collectionType-summarizing-con" .

<http://www.opengis.net/spec/OMS/3.0/req/obs-basic/ObservationCollection/member-sem> a spec:Requirement,
        skos:Concept ;
    dcterms:description "An Observation that is part of this ObservationCollection . If a reference to a member Observation is provided, the association with the role member SHALL be used." ;
    skos:broader <http://www.opengis.net/spec/OMS/3.0/req/obs-basic/ObservationCollection> ;
    skos:definition "An Observation that is part of this ObservationCollection . If a reference to a member Observation is provided, the association with the role member SHALL be used." ;
    skos:inScheme <http://www.opengis.net/spec/OMS/3.0> ;
    skos:prefLabel "Requirement: /req/obs-basic/ObservationCollection/member-sem" .

<http://www.opengis.net/spec/OMS/3.0/req/obs-basic/ObservationCollection/memberCharacteristics-sem> a spec:Requirement,
        skos:Concept ;
    dcterms:description "Information on ObservationCharacteristics of Observations contained within the ObservationCollection . If a reference to ObservationCharacteristics pertaining to the collection members is provided, the association with the role memberCharacteristics SHALL be used." ;
    skos:broader <http://www.opengis.net/spec/OMS/3.0/req/obs-basic/ObservationCollection> ;
    skos:definition "Information on ObservationCharacteristics of Observations contained within the ObservationCollection . If a reference to ObservationCharacteristics pertaining to the collection members is provided, the association with the role memberCharacteristics SHALL be used." ;
    skos:inScheme <http://www.opengis.net/spec/OMS/3.0> ;
    skos:prefLabel "Requirement: /req/obs-basic/ObservationCollection/memberCharacteristics-sem" .

<http://www.opengis.net/spec/OMS/3.0/req/obs-basic/ObservationCollection/relatedCollection-sem> a spec:Requirement,
        skos:Concept ;
    dcterms:description "A ObservationCollection the ObservationCollection is related to. If a reference to a related ObservationCollection is provided, the association with role relatedCollection SHALL be used. The context:GenericName qualifier of this association may be used to provide further information as to the nature of the relation." ;
    skos:broader <http://www.opengis.net/spec/OMS/3.0/req/obs-basic/ObservationCollection> ;
    skos:definition "A ObservationCollection the ObservationCollection is related to. If a reference to a related ObservationCollection is provided, the association with role relatedCollection SHALL be used. The context:GenericName qualifier of this association may be used to provide further information as to the nature of the relation." ;
    skos:inScheme <http://www.opengis.net/spec/OMS/3.0> ;
    skos:prefLabel "Requirement: /req/obs-basic/ObservationCollection/relatedCollection-sem" .

<http://www.opengis.net/spec/OMS/3.0/req/obs-basic/ObservingCapability/ObservingCapability-sem> a spec:Requirement,
        skos:Concept ;
    dcterms:description "Information on Observation (s) that could potentially be provided." ;
    skos:broader <http://www.opengis.net/spec/OMS/3.0/req/obs-basic/ObservingCapability> ;
    skos:definition "Information on Observation (s) that could potentially be provided." ;
    skos:inScheme <http://www.opengis.net/spec/OMS/3.0> ;
    skos:prefLabel "Requirement: /req/obs-basic/ObservingCapability/ObservingCapability-sem" .

<http://www.opengis.net/spec/OMS/3.0/req/obs-basic/gen/link-sem> a spec:Requirement,
        skos:Concept ;
    dcterms:description "Additional descriptive resources pertaining to a feature. If a link to a descriptive resource is provided, the attribute link:URI SHALL be used." ;
    skos:broader <http://www.opengis.net/spec/OMS/3.0/req/obs-basic/Host> ;
    skos:broader <http://www.opengis.net/spec/OMS/3.0/req/obs-basic/ObservableProperty> ;
    skos:broader <http://www.opengis.net/spec/OMS/3.0/req/obs-basic/ObservingProcedure> ;
    skos:broader <http://www.opengis.net/spec/OMS/3.0/req/obs-basic/GenericDomainFeature> ;
    skos:broader <http://www.opengis.net/spec/OMS/3.0/req/obs-basic/Deployment> ;
    skos:broader <http://www.opengis.net/spec/OMS/3.0/req/obs-basic/Observer> ;
    skos:definition "Additional descriptive resources pertaining to a feature. If a link to a descriptive resource is provided, the attribute link:URI SHALL be used." ;
    skos:inScheme <http://www.opengis.net/spec/OMS/3.0> ;
    skos:prefLabel "Requirement: /req/obs-basic/gen/link-sem" .

<http://www.opengis.net/spec/OMS/3.0/req/obs-basic/gen/location-sem> a spec:Requirement,
        skos:Concept ;
    dcterms:description "Location information pertaining to a feature . If location information is provided, the attribute location:Geometry SHALL be used." ;
    skos:broader <http://www.opengis.net/spec/OMS/3.0/req/obs-basic/Host> ;
    skos:broader <http://www.opengis.net/spec/OMS/3.0/req/obs-basic/GenericDomainFeature> ;
    skos:broader <http://www.opengis.net/spec/OMS/3.0/req/obs-basic/Observer> ;
    skos:definition "Location information pertaining to a feature . If location information is provided, the attribute location:Geometry SHALL be used." ;
    skos:inScheme <http://www.opengis.net/spec/OMS/3.0> ;
    skos:prefLabel "Requirement: /req/obs-basic/gen/location-sem" .

<http://www.opengis.net/spec/OMS/3.0/req/obs-core/AbstractDeployment/deploymentReason-sem> a spec:Requirement,
        skos:Concept ;
    dcterms:description "A human readable description of the reason for the Deployment . If the reason for the Deployment is provided, the property deploymentReason:CharacterString SHALL be used." ;
    skos:broader <http://www.opengis.net/spec/OMS/3.0/req/obs-core/AbstractDeployment> ;
    skos:definition "A human readable description of the reason for the Deployment . If the reason for the Deployment is provided, the property deploymentReason:CharacterString SHALL be used." ;
    skos:inScheme <http://www.opengis.net/spec/OMS/3.0> ;
    skos:prefLabel "Requirement: /req/obs-core/AbstractDeployment/deploymentReason-sem" .

<http://www.opengis.net/spec/OMS/3.0/req/obs-core/AbstractDeployment/deploymentTime-sem> a spec:Requirement,
        skos:Concept ;
    dcterms:description "The time that the Deployment pertains to. If the time of the Deployment is provided, property deploymentTime:TM_Period SHALL be used." ;
    skos:broader <http://www.opengis.net/spec/OMS/3.0/req/obs-core/AbstractDeployment> ;
    skos:definition "The time that the Deployment pertains to. If the time of the Deployment is provided, property deploymentTime:TM_Period SHALL be used." ;
    skos:inScheme <http://www.opengis.net/spec/OMS/3.0> ;
    skos:prefLabel "Requirement: /req/obs-core/AbstractDeployment/deploymentTime-sem" .

<http://www.opengis.net/spec/OMS/3.0/req/obs-core/AbstractObservation/FoI-con> a spec:Requirement,
        skos:Concept ;
    dcterms:description "at least one proximateFeatureOfInterest or ultimateFeatureOfInterest SHALL be given." ;
    skos:broader <http://www.opengis.net/spec/OMS/3.0/req/obs-core/AbstractObservation> ;
    skos:definition "at least one proximateFeatureOfInterest or ultimateFeatureOfInterest SHALL be given." ;
    skos:inScheme <http://www.opengis.net/spec/OMS/3.0> ;
    skos:prefLabel "Requirement: /req/obs-core/AbstractObservation/FoI-con" .

<http://www.opengis.net/spec/OMS/3.0/req/obs-core/AbstractObservation/parameterName-card> a spec:Requirement,
        skos:Concept ;
    dcterms:description "The name attribute of a parameter NamedValue SHALL be unique within an Observation ." ;
    skos:broader <http://www.opengis.net/spec/OMS/3.0/req/obs-core/AbstractObservation> ;
    skos:definition "The name attribute of a parameter NamedValue SHALL be unique within an Observation ." ;
    skos:inScheme <http://www.opengis.net/spec/OMS/3.0> ;
    skos:prefLabel "Requirement: /req/obs-core/AbstractObservation/parameterName-card" .

<http://www.opengis.net/spec/OMS/3.0/req/obs-core/AbstractObservation/resultTime-type> a spec:Requirement,
        skos:Concept ;
    dcterms:description "If the result time of the Observation is provided, the resultTime attribute SHALL be of type TM_Instant ." ;
    skos:broader <http://www.opengis.net/spec/OMS/3.0/req/obs-core/AbstractObservation> ;
    skos:definition "If the result time of the Observation is provided, the resultTime attribute SHALL be of type TM_Instant ." ;
    skos:inScheme <http://www.opengis.net/spec/OMS/3.0> ;
    skos:prefLabel "Requirement: /req/obs-core/AbstractObservation/resultTime-type" .

<http://www.opengis.net/spec/OMS/3.0/req/obs-core/AbstractObservation/validTime-type> a spec:Requirement,
        skos:Concept ;
    dcterms:description "If the result time of the Observation is provided, the validTime attribute SHALL be of type TM_Period ." ;
    skos:broader <http://www.opengis.net/spec/OMS/3.0/req/obs-core/AbstractObservation> ;
    skos:definition "If the result time of the Observation is provided, the validTime attribute SHALL be of type TM_Period ." ;
    skos:inScheme <http://www.opengis.net/spec/OMS/3.0> ;
    skos:prefLabel "Requirement: /req/obs-core/AbstractObservation/validTime-type" .

<http://www.opengis.net/spec/OMS/3.0/req/obs-core/AbstractObservationCharacteristics/AbstractObservationCharacteristics-sem> a spec:Requirement,
        skos:Concept ;
    dcterms:description "Set of common characteristics used for describing an Observation or a collection of Observations." ;
    skos:broader <http://www.opengis.net/spec/OMS/3.0/req/obs-core/AbstractObservationCharacteristics> ;
    skos:definition "Set of common characteristics used for describing an Observation or a collection of Observations." ;
    skos:inScheme <http://www.opengis.net/spec/OMS/3.0> ;
    skos:prefLabel "Requirement: /req/obs-core/AbstractObservationCharacteristics/AbstractObservationCharacteristics-sem" .

<http://www.opengis.net/spec/OMS/3.0/req/obs-core/AbstractObservationCharacteristics/pFoI-sem> a spec:Requirement,
        skos:Concept ;
    dcterms:description "The entity that is directly of interest in the act of observing. If a reference to the entity being directly observed is provided, the association with the role proximateFeatureOfInterest SHALL be used. This association is a specialization of the featureOfInterest role." ;
    skos:broader <http://www.opengis.net/spec/OMS/3.0/req/obs-core/AbstractObservationCharacteristics> ;
    skos:definition "The entity that is directly of interest in the act of observing. If a reference to the entity being directly observed is provided, the association with the role proximateFeatureOfInterest SHALL be used. This association is a specialization of the featureOfInterest role." ;
    skos:inScheme <http://www.opengis.net/spec/OMS/3.0> ;
    skos:prefLabel "Requirement: /req/obs-core/AbstractObservationCharacteristics/pFoI-sem" .

<http://www.opengis.net/spec/OMS/3.0/req/obs-core/AbstractObservationCharacteristics/parameter-sem> a spec:Requirement,
        skos:Concept ;
    dcterms:description "Arbitrary event-specific parameter relevant to the AbstractObservationCharacteristics . If additional parameter information is provided, the property parameter:NamedValue SHALL be used." ;
    skos:broader <http://www.opengis.net/spec/OMS/3.0/req/obs-core/AbstractObservationCharacteristics> ;
    skos:definition "Arbitrary event-specific parameter relevant to the AbstractObservationCharacteristics . If additional parameter information is provided, the property parameter:NamedValue SHALL be used." ;
    skos:inScheme <http://www.opengis.net/spec/OMS/3.0> ;
    skos:prefLabel "Requirement: /req/obs-core/AbstractObservationCharacteristics/parameter-sem" .

<http://www.opengis.net/spec/OMS/3.0/req/obs-core/AbstractObservationCharacteristics/resultQuality-sem> a spec:Requirement,
        skos:Concept ;
    dcterms:description "Information pertaining to the data quality of the Result ( ref ). If additional data quality information is provided, the property resultQuality:Any SHALL be used." ;
    skos:broader <http://www.opengis.net/spec/OMS/3.0/req/obs-core/AbstractObservationCharacteristics> ;
    skos:definition "Information pertaining to the data quality of the Result ( ref ). If additional data quality information is provided, the property resultQuality:Any SHALL be used." ;
    skos:inScheme <http://www.opengis.net/spec/OMS/3.0> ;
    skos:prefLabel "Requirement: /req/obs-core/AbstractObservationCharacteristics/resultQuality-sem" .

<http://www.opengis.net/spec/OMS/3.0/req/obs-core/AbstractObservationCharacteristics/type-sem> a spec:Requirement,
        skos:Concept ;
    dcterms:description "Information providing further detail on the type of Observations being described by the AbstractObservationCharacteristics . If information on the type of Observation is provided, the property observationType:AbstractObservationTypeCodeListValue SHALL be used." ;
    skos:broader <http://www.opengis.net/spec/OMS/3.0/req/obs-core/AbstractObservationCharacteristics> ;
    skos:definition "Information providing further detail on the type of Observations being described by the AbstractObservationCharacteristics . If information on the type of Observation is provided, the property observationType:AbstractObservationTypeCodeListValue SHALL be used." ;
    skos:inScheme <http://www.opengis.net/spec/OMS/3.0> ;
    skos:prefLabel "Requirement: /req/obs-core/AbstractObservationCharacteristics/type-sem" .

<http://www.opengis.net/spec/OMS/3.0/req/obs-core/AbstractObservationCharacteristics/uFoI-sem> a spec:Requirement,
        skos:Concept ;
    dcterms:description "The entity that is ultimately of interest in the act of observing. If a reference to the entity ultimately being observed is provided, the association with the role ultimateFeatureOfInterest SHALL be used. This association is a specialization of the featureOfInterest role." ;
    skos:broader <http://www.opengis.net/spec/OMS/3.0/req/obs-core/AbstractObservationCharacteristics> ;
    skos:definition "The entity that is ultimately of interest in the act of observing. If a reference to the entity ultimately being observed is provided, the association with the role ultimateFeatureOfInterest SHALL be used. This association is a specialization of the featureOfInterest role." ;
    skos:inScheme <http://www.opengis.net/spec/OMS/3.0> ;
    skos:prefLabel "Requirement: /req/obs-core/AbstractObservationCharacteristics/uFoI-sem" .

<http://www.opengis.net/spec/OMS/3.0/req/obs-core/NamedValue/NamedValue-sem> a spec:Requirement,
        skos:Concept ;
    dcterms:description "The class NamedValue provides for a generic soft-typed parameter value." ;
    skos:broader <http://www.opengis.net/spec/OMS/3.0/req/obs-core/NamedValue> ;
    skos:definition "The class NamedValue provides for a generic soft-typed parameter value." ;
    skos:inScheme <http://www.opengis.net/spec/OMS/3.0> ;
    skos:prefLabel "Requirement: /req/obs-core/NamedValue/NamedValue-sem" .

<http://www.opengis.net/spec/OMS/3.0/req/obs-core/NamedValue/name-sem> a spec:Requirement,
        skos:Concept ;
    dcterms:description "The attribute name:GenericName SHALL indicate the meaning of the named value." ;
    skos:broader <http://www.opengis.net/spec/OMS/3.0/req/obs-core/NamedValue> ;
    skos:definition "The attribute name:GenericName SHALL indicate the meaning of the named value." ;
    skos:inScheme <http://www.opengis.net/spec/OMS/3.0> ;
    skos:prefLabel "Requirement: /req/obs-core/NamedValue/name-sem" .

<http://www.opengis.net/spec/OMS/3.0/req/obs-core/NamedValue/value-sem> a spec:Requirement,
        skos:Concept ;
    dcterms:description "The attribute value:Any SHALL provide the value." ;
    skos:broader <http://www.opengis.net/spec/OMS/3.0/req/obs-core/NamedValue> ;
    skos:definition "The attribute value:Any SHALL provide the value." ;
    skos:inScheme <http://www.opengis.net/spec/OMS/3.0> ;
    skos:prefLabel "Requirement: /req/obs-core/NamedValue/value-sem" .

<http://www.opengis.net/spec/OMS/3.0/req/obs-core/gen/metadata-sem> a spec:Requirement,
        skos:Concept ;
    dcterms:description "If descriptive metadata is provided, the association role metadata SHALL link to descriptive metadata as commonly understood by communities." ;
    skos:broader <http://www.opengis.net/spec/OMS/3.0/req/sam-basic/SampleCollection> ;
    skos:broader <http://www.opengis.net/spec/OMS/3.0/req/sam-core/AbstractSamplingProcedure> ;
    skos:broader <http://www.opengis.net/spec/OMS/3.0/req/sam-core/AbstractSampler> ;
    skos:broader <http://www.opengis.net/spec/OMS/3.0/req/sam-core/AbstractSampling> ;
    skos:broader <http://www.opengis.net/spec/OMS/3.0/req/sam-core/AbstractPreparationProcedure> ;
    skos:broader <http://www.opengis.net/spec/OMS/3.0/req/obs-core/AbstractObservationCharacteristics> ;
    skos:broader <http://www.opengis.net/spec/OMS/3.0/req/sam-core/AbstractSample> ;
    skos:broader <http://www.opengis.net/spec/OMS/3.0/req/obs-core/AbstractObserver> ;
    skos:broader <http://www.opengis.net/spec/OMS/3.0/req/obs-core/AbstractDeployment> ;
    skos:broader <http://www.opengis.net/spec/OMS/3.0/req/obs-core/AbstractHost> ;
    skos:broader <http://www.opengis.net/spec/OMS/3.0/req/sam-core/AbstractPreparationStep> ;
    skos:broader <http://www.opengis.net/spec/OMS/3.0/req/obs-core/AbstractObservingProcedure> ;
    skos:broader <http://www.opengis.net/spec/OMS/3.0/req/obs-core/AbstractObservableProperty> ;
    skos:definition "If descriptive metadata is provided, the association role metadata SHALL link to descriptive metadata as commonly understood by communities." ;
    skos:inScheme <http://www.opengis.net/spec/OMS/3.0> ;
    skos:prefLabel "Requirement: /req/obs-core/gen/metadata-sem" .

<http://www.opengis.net/spec/OMS/3.0/req/obs-cpt/Deployment/Deployment-sem> a spec:Requirement,
        skos:Concept ;
    dcterms:description "Information on the assignment of an Observer to a Host." ;
    skos:broader <http://www.opengis.net/spec/OMS/3.0/req/obs-cpt/Deployment> ;
    skos:definition "Information on the assignment of an Observer to a Host." ;
    skos:inScheme <http://www.opengis.net/spec/OMS/3.0> ;
    skos:prefLabel "Requirement: /req/obs-cpt/Deployment/Deployment-sem" .

<http://www.opengis.net/spec/OMS/3.0/req/obs-cpt/Deployment/host-sem> a spec:Requirement,
        skos:Concept ;
    dcterms:description "The Host to which this Deployment pertains. If a reference to a Host is provided, the association with the role host SHALL be used" ;
    skos:broader <http://www.opengis.net/spec/OMS/3.0/req/obs-cpt/Deployment> ;
    skos:definition "The Host to which this Deployment pertains. If a reference to a Host is provided, the association with the role host SHALL be used" ;
    skos:inScheme <http://www.opengis.net/spec/OMS/3.0> ;
    skos:prefLabel "Requirement: /req/obs-cpt/Deployment/host-sem" .

<http://www.opengis.net/spec/OMS/3.0/req/obs-cpt/Deployment/observer-sem> a spec:Requirement,
        skos:Concept ;
    dcterms:description "The Observer associated with this Deployment . If a reference to an Observer is provided, the association with the role observer SHALL be used." ;
    skos:broader <http://www.opengis.net/spec/OMS/3.0/req/obs-cpt/Deployment> ;
    skos:definition "The Observer associated with this Deployment . If a reference to an Observer is provided, the association with the role observer SHALL be used." ;
    skos:inScheme <http://www.opengis.net/spec/OMS/3.0> ;
    skos:prefLabel "Requirement: /req/obs-cpt/Deployment/observer-sem" .

<http://www.opengis.net/spec/OMS/3.0/req/obs-cpt/Host/Host-sem> a spec:Requirement,
        skos:Concept ;
    dcterms:description "ï¿½ A grouping of Observer s for a specific reason." ;
    skos:broader <http://www.opengis.net/spec/OMS/3.0/req/obs-cpt/Host> ;
    skos:definition "ï¿½ A grouping of Observer s for a specific reason." ;
    skos:inScheme <http://www.opengis.net/spec/OMS/3.0> ;
    skos:prefLabel "Requirement: /req/obs-cpt/Host/Host-sem" .

<http://www.opengis.net/spec/OMS/3.0/req/obs-cpt/Host/deployment-sem> a spec:Requirement,
        skos:Concept ;
    dcterms:description "A Deployment at this Host . If a reference to a Deployment is provided, the association with the role host SHALL be used." ;
    skos:broader <http://www.opengis.net/spec/OMS/3.0/req/obs-cpt/Host> ;
    skos:definition "A Deployment at this Host . If a reference to a Deployment is provided, the association with the role host SHALL be used." ;
    skos:inScheme <http://www.opengis.net/spec/OMS/3.0> ;
    skos:prefLabel "Requirement: /req/obs-cpt/Host/deployment-sem" .

<http://www.opengis.net/spec/OMS/3.0/req/obs-cpt/Host/relatedHost-sem> a spec:Requirement,
        skos:Concept ;
    dcterms:description "A Host the Host is related to. If a reference to a related Host is provided, the association with role relatedHost SHALL be used. The context:GenericName qualifier of this association may be used to provide further information as to the nature of the relation." ;
    skos:broader <http://www.opengis.net/spec/OMS/3.0/req/obs-cpt/Host> ;
    skos:definition "A Host the Host is related to. If a reference to a related Host is provided, the association with role relatedHost SHALL be used. The context:GenericName qualifier of this association may be used to provide further information as to the nature of the relation." ;
    skos:inScheme <http://www.opengis.net/spec/OMS/3.0> ;
    skos:prefLabel "Requirement: /req/obs-cpt/Host/relatedHost-sem" .

<http://www.opengis.net/spec/OMS/3.0/req/obs-cpt/ObservableProperty/ObservableProperty-sem> a spec:Requirement,
        skos:Concept ;
    dcterms:description "An observable quality (property, characteristic) of the feature of interest that can be observed." ;
    skos:broader <http://www.opengis.net/spec/OMS/3.0/req/obs-cpt/ObservableProperty> ;
    skos:definition "An observable quality (property, characteristic) of the feature of interest that can be observed." ;
    skos:inScheme <http://www.opengis.net/spec/OMS/3.0> ;
    skos:prefLabel "Requirement: /req/obs-cpt/ObservableProperty/ObservableProperty-sem" .

<http://www.opengis.net/spec/OMS/3.0/req/obs-cpt/ObservableProperty/observer-sem> a spec:Requirement,
        skos:Concept ;
    dcterms:description "An Observer capable of observing this ObservableProperty . If a reference to the Observer is provided, the association with the role observer SHALL be used." ;
    skos:broader <http://www.opengis.net/spec/OMS/3.0/req/obs-cpt/ObservableProperty> ;
    skos:definition "An Observer capable of observing this ObservableProperty . If a reference to the Observer is provided, the association with the role observer SHALL be used." ;
    skos:inScheme <http://www.opengis.net/spec/OMS/3.0> ;
    skos:prefLabel "Requirement: /req/obs-cpt/ObservableProperty/observer-sem" .

<http://www.opengis.net/spec/OMS/3.0/req/obs-cpt/Observation/Observation-sem> a spec:Requirement,
        skos:Concept ;
    dcterms:description "An observation is an act carried out by an Observer to determine the value of an ObservableProperty of an object ( featureOfInterest) by using a Procedure ; the value is provided as the result ." ;
    skos:broader <http://www.opengis.net/spec/OMS/3.0/req/obs-cpt/Observation> ;
    skos:definition "An observation is an act carried out by an Observer to determine the value of an ObservableProperty of an object ( featureOfInterest) by using a Procedure ; the value is provided as the result ." ;
    skos:inScheme <http://www.opengis.net/spec/OMS/3.0> ;
    skos:prefLabel "Requirement: /req/obs-cpt/Observation/Observation-sem" .

<http://www.opengis.net/spec/OMS/3.0/req/obs-cpt/Observation/featureOfInterest-card> a spec:Requirement,
        skos:Concept ;
    dcterms:description "An Observation SHALL have at least 1 featureOfInterest and MAY have more than 1 in cases objects are created with the intention to sample the real-world object The cardinality of the featureOfInterest association SHALL be 1 at minimum." ;
    skos:broader <http://www.opengis.net/spec/OMS/3.0/req/obs-cpt/Observation> ;
    skos:definition "An Observation SHALL have at least 1 featureOfInterest and MAY have more than 1 in cases objects are created with the intention to sample the real-world object The cardinality of the featureOfInterest association SHALL be 1 at minimum." ;
    skos:inScheme <http://www.opengis.net/spec/OMS/3.0> ;
    skos:prefLabel "Requirement: /req/obs-cpt/Observation/featureOfInterest-card" .

<http://www.opengis.net/spec/OMS/3.0/req/obs-cpt/Observation/featureOfInterest-sem> a spec:Requirement,
        skos:Concept ;
    dcterms:description "The subject of the Observation . The reference(s) to featureOfInterest(s) SHALL be provided using the association Domain with the role featureOfInterest ." ;
    skos:broader <http://www.opengis.net/spec/OMS/3.0/req/obs-cpt/Observation> ;
    skos:broader <http://www.opengis.net/spec/OMS/3.0/req/obs-core/AbstractObservationCharacteristics> ;
    skos:definition "The subject of the Observation . The reference(s) to featureOfInterest(s) SHALL be provided using the association Domain with the role featureOfInterest ." ;
    skos:inScheme <http://www.opengis.net/spec/OMS/3.0> ;
    skos:prefLabel "Requirement: /req/obs-cpt/Observation/featureOfInterest-sem" .

<http://www.opengis.net/spec/OMS/3.0/req/obs-cpt/Observation/host-sem> a spec:Requirement,
        skos:Concept ;
    dcterms:description "A Host that is involved in the creation of this Observation If a reference to a Host is provided, the association with the role host SHALL be used." ;
    skos:broader <http://www.opengis.net/spec/OMS/3.0/req/obs-cpt/Observation> ;
    skos:broader <http://www.opengis.net/spec/OMS/3.0/req/obs-core/AbstractObservationCharacteristics> ;
    skos:definition "A Host that is involved in the creation of this Observation If a reference to a Host is provided, the association with the role host SHALL be used." ;
    skos:inScheme <http://www.opengis.net/spec/OMS/3.0> ;
    skos:prefLabel "Requirement: /req/obs-cpt/Observation/host-sem" .

<http://www.opengis.net/spec/OMS/3.0/req/obs-cpt/Observation/observedProperty-card> a spec:Requirement,
        skos:Concept ;
    dcterms:description "An Observation SHALL have exactly 1 observedProperty ." ;
    skos:broader <http://www.opengis.net/spec/OMS/3.0/req/obs-cpt/Observation> ;
    skos:broader <http://www.opengis.net/spec/OMS/3.0/req/obs-core/AbstractObservation> ;
    skos:definition "An Observation SHALL have exactly 1 observedProperty ." ;
    skos:inScheme <http://www.opengis.net/spec/OMS/3.0> ;
    skos:prefLabel "Requirement: /req/obs-cpt/Observation/observedProperty-card" .

<http://www.opengis.net/spec/OMS/3.0/req/obs-cpt/Observation/observedProperty-sem> a spec:Requirement,
        skos:Concept ;
    dcterms:description "The ObservableProperty that is the subject of the Observation . If a reference to an ObservableProperty is provided, the association with the role observedProperty SHALL be used." ;
    skos:broader <http://www.opengis.net/spec/OMS/3.0/req/obs-cpt/Observation> ;
    skos:broader <http://www.opengis.net/spec/OMS/3.0/req/obs-core/AbstractObservationCharacteristics> ;
    skos:definition "The ObservableProperty that is the subject of the Observation . If a reference to an ObservableProperty is provided, the association with the role observedProperty SHALL be used." ;
    skos:inScheme <http://www.opengis.net/spec/OMS/3.0> ;
    skos:prefLabel "Requirement: /req/obs-cpt/Observation/observedProperty-sem" .

<http://www.opengis.net/spec/OMS/3.0/req/obs-cpt/Observation/observer-sem> a spec:Requirement,
        skos:Concept ;
    dcterms:description "An Observer (ref) that is involved in the creation of this Observation . If a reference to an Observer is provided, the association with the role observer SHALL be used." ;
    skos:broader <http://www.opengis.net/spec/OMS/3.0/req/obs-cpt/Observation> ;
    skos:broader <http://www.opengis.net/spec/OMS/3.0/req/obs-core/AbstractObservationCharacteristics> ;
    skos:definition "An Observer (ref) that is involved in the creation of this Observation . If a reference to an Observer is provided, the association with the role observer SHALL be used." ;
    skos:inScheme <http://www.opengis.net/spec/OMS/3.0> ;
    skos:prefLabel "Requirement: /req/obs-cpt/Observation/observer-sem" .

<http://www.opengis.net/spec/OMS/3.0/req/obs-cpt/Observation/observingProcedure-card> a spec:Requirement,
        skos:Concept ;
    dcterms:description "" ;
    skos:broader <http://www.opengis.net/spec/OMS/3.0/req/obs-cpt/Observation> ;
    skos:definition "" ;
    skos:inScheme <http://www.opengis.net/spec/OMS/3.0> ;
    skos:prefLabel "Requirement: /req/obs-cpt/Observation/observingProcedure-card" .

<http://www.opengis.net/spec/OMS/3.0/req/obs-cpt/Observation/observingProcedure-sem> a spec:Requirement,
        skos:Concept ;
    dcterms:description "The ObservingProcedure used by the Observation to determine the value of the ObservableProperty provided by the Result. If a reference to an ObservingProcedure is provided, the association with the role procedure SHALL be used." ;
    skos:broader <http://www.opengis.net/spec/OMS/3.0/req/obs-cpt/Observation> ;
    skos:definition "The ObservingProcedure used by the Observation to determine the value of the ObservableProperty provided by the Result. If a reference to an ObservingProcedure is provided, the association with the role procedure SHALL be used." ;
    skos:inScheme <http://www.opengis.net/spec/OMS/3.0> ;
    skos:prefLabel "Requirement: /req/obs-cpt/Observation/observingProcedure-sem" .

<http://www.opengis.net/spec/OMS/3.0/req/obs-cpt/Observation/phenomenonTime-card> a spec:Requirement,
        skos:Concept ;
    dcterms:description "An Observation SHALL have exactly 1 phenomenonTime." ;
    skos:broader <http://www.opengis.net/spec/OMS/3.0/req/obs-cpt/Observation> ;
    skos:broader <http://www.opengis.net/spec/OMS/3.0/req/obs-core/AbstractObservation> ;
    skos:definition "An Observation SHALL have exactly 1 phenomenonTime." ;
    skos:inScheme <http://www.opengis.net/spec/OMS/3.0> ;
    skos:prefLabel "Requirement: /req/obs-cpt/Observation/phenomenonTime-card" .

<http://www.opengis.net/spec/OMS/3.0/req/obs-cpt/Observation/phenomenonTime-sem> a spec:Requirement,
        skos:Concept ;
    dcterms:description "The time that the Result applies to the characteristic of the FeatureOfInterest being observed. If the phenomenonTime is described, this SHALL be provided by the attribute phenomenonTime:TM_Object" ;
    skos:broader <http://www.opengis.net/spec/OMS/3.0/req/obs-cpt/Observation> ;
    skos:broader <http://www.opengis.net/spec/OMS/3.0/req/obs-core/AbstractObservationCharacteristics> ;
    skos:definition "The time that the Result applies to the characteristic of the FeatureOfInterest being observed. If the phenomenonTime is described, this SHALL be provided by the attribute phenomenonTime:TM_Object" ;
    skos:inScheme <http://www.opengis.net/spec/OMS/3.0> ;
    skos:prefLabel "Requirement: /req/obs-cpt/Observation/phenomenonTime-sem" .

<http://www.opengis.net/spec/OMS/3.0/req/obs-cpt/Observation/procedure-card> a spec:Requirement,
        skos:Concept ;
    dcterms:description "" ;
    skos:broader <http://www.opengis.net/spec/OMS/3.0/req/obs-core/AbstractObservation> ;
    skos:definition "" ;
    skos:inScheme <http://www.opengis.net/spec/OMS/3.0> ;
    skos:prefLabel "Requirement: /req/obs-cpt/Observation/procedure-card" .

<http://www.opengis.net/spec/OMS/3.0/req/obs-cpt/Observation/procedure-sem> a spec:Requirement,
        skos:Concept ;
    dcterms:description "" ;
    skos:broader <http://www.opengis.net/spec/OMS/3.0/req/obs-core/AbstractObservationCharacteristics> ;
    skos:definition "" ;
    skos:inScheme <http://www.opengis.net/spec/OMS/3.0> ;
    skos:prefLabel "Requirement: /req/obs-cpt/Observation/procedure-sem" .

<http://www.opengis.net/spec/OMS/3.0/req/obs-cpt/Observation/result-card> a spec:Requirement,
        skos:Concept ;
    dcterms:description "An Observation SHALL have exactly 1 result ." ;
    skos:broader <http://www.opengis.net/spec/OMS/3.0/req/obs-cpt/Observation> ;
    skos:broader <http://www.opengis.net/spec/OMS/3.0/req/obs-core/AbstractObservation> ;
    skos:definition "An Observation SHALL have exactly 1 result ." ;
    skos:inScheme <http://www.opengis.net/spec/OMS/3.0> ;
    skos:prefLabel "Requirement: /req/obs-cpt/Observation/result-card" .

<http://www.opengis.net/spec/OMS/3.0/req/obs-cpt/Observation/result-sem> a spec:Requirement,
        skos:Concept ;
    dcterms:description "The Result of the Observation . If a reference to a result is provided, the association Range with the role result SHALL be used." ;
    skos:broader <http://www.opengis.net/spec/OMS/3.0/req/obs-cpt/Observation> ;
    skos:broader <http://www.opengis.net/spec/OMS/3.0/req/obs-core/AbstractObservationCharacteristics> ;
    skos:definition "The Result of the Observation . If a reference to a result is provided, the association Range with the role result SHALL be used." ;
    skos:inScheme <http://www.opengis.net/spec/OMS/3.0> ;
    skos:prefLabel "Requirement: /req/obs-cpt/Observation/result-sem" .

<http://www.opengis.net/spec/OMS/3.0/req/obs-cpt/Observation/resultTime-card> a spec:Requirement,
        skos:Concept ;
    dcterms:description "An Observation SHALL have exactly 1 resultTime ." ;
    skos:broader <http://www.opengis.net/spec/OMS/3.0/req/obs-cpt/Observation> ;
    skos:broader <http://www.opengis.net/spec/OMS/3.0/req/obs-core/AbstractObservation> ;
    skos:definition "An Observation SHALL have exactly 1 resultTime ." ;
    skos:inScheme <http://www.opengis.net/spec/OMS/3.0> ;
    skos:prefLabel "Requirement: /req/obs-cpt/Observation/resultTime-card" .

<http://www.opengis.net/spec/OMS/3.0/req/obs-cpt/Observation/resultTime-sem> a spec:Requirement,
        skos:Concept ;
    dcterms:description "The instant of time when the result of the Observation became available. If the resultTime is described, this SHALL be provided by the attribute resultTime:TM_Object" ;
    skos:broader <http://www.opengis.net/spec/OMS/3.0/req/obs-cpt/Observation> ;
    skos:broader <http://www.opengis.net/spec/OMS/3.0/req/obs-core/AbstractObservationCharacteristics> ;
    skos:definition "The instant of time when the result of the Observation became available. If the resultTime is described, this SHALL be provided by the attribute resultTime:TM_Object" ;
    skos:inScheme <http://www.opengis.net/spec/OMS/3.0> ;
    skos:prefLabel "Requirement: /req/obs-cpt/Observation/resultTime-sem" .

<http://www.opengis.net/spec/OMS/3.0/req/obs-cpt/Observation/validTime-sem> a spec:Requirement,
        skos:Concept ;
    dcterms:description "The time interval during which the result is assumed to be applicable for use. If validTime(s) are described they SHALL be provided by the attribute validTime:TM_Period" ;
    skos:broader <http://www.opengis.net/spec/OMS/3.0/req/obs-cpt/Observation> ;
    skos:broader <http://www.opengis.net/spec/OMS/3.0/req/obs-core/AbstractObservationCharacteristics> ;
    skos:definition "The time interval during which the result is assumed to be applicable for use. If validTime(s) are described they SHALL be provided by the attribute validTime:TM_Period" ;
    skos:inScheme <http://www.opengis.net/spec/OMS/3.0> ;
    skos:prefLabel "Requirement: /req/obs-cpt/Observation/validTime-sem" .

<http://www.opengis.net/spec/OMS/3.0/req/obs-cpt/Observer/Observer-sem> a spec:Requirement,
        skos:Concept ;
    dcterms:description "An identifiable entity that can generate Observations pertaining to an observableProperty by implementing a Procedure ." ;
    skos:broader <http://www.opengis.net/spec/OMS/3.0/req/obs-cpt/Observer> ;
    skos:definition "An identifiable entity that can generate Observations pertaining to an observableProperty by implementing a Procedure ." ;
    skos:inScheme <http://www.opengis.net/spec/OMS/3.0> ;
    skos:prefLabel "Requirement: /req/obs-cpt/Observer/Observer-sem" .

<http://www.opengis.net/spec/OMS/3.0/req/obs-cpt/Observer/deployment-sem> a spec:Requirement,
        skos:Concept ;
    dcterms:description "A Deployment to which this Observer is either physically or organizationally attached. If a reference to Deployment (s) is provided, the association with the role deployment SHALL be used." ;
    skos:broader <http://www.opengis.net/spec/OMS/3.0/req/obs-cpt/Observer> ;
    skos:definition "A Deployment to which this Observer is either physically or organizationally attached. If a reference to Deployment (s) is provided, the association with the role deployment SHALL be used." ;
    skos:inScheme <http://www.opengis.net/spec/OMS/3.0> ;
    skos:prefLabel "Requirement: /req/obs-cpt/Observer/deployment-sem" .

<http://www.opengis.net/spec/OMS/3.0/req/obs-cpt/Observer/observableProperty-sem> a spec:Requirement,
        skos:Concept ;
    dcterms:description "An ObservableProperty that this Observer can observe. If a reference to ObservableProperty (s) is provided, the association with the role observableProperty SHALL be used." ;
    skos:broader <http://www.opengis.net/spec/OMS/3.0/req/obs-cpt/Observer> ;
    skos:definition "An ObservableProperty that this Observer can observe. If a reference to ObservableProperty (s) is provided, the association with the role observableProperty SHALL be used." ;
    skos:inScheme <http://www.opengis.net/spec/OMS/3.0> ;
    skos:prefLabel "Requirement: /req/obs-cpt/Observer/observableProperty-sem" .

<http://www.opengis.net/spec/OMS/3.0/req/obs-cpt/Observer/observingProcedure-sem> a spec:Requirement,
        skos:Concept ;
    dcterms:description "An ObservingProcedure that this Observer can perform. If a reference to ObservingProcedure (s) is provided, the association with the role observingProcedure SHALL be used." ;
    skos:broader <http://www.opengis.net/spec/OMS/3.0/req/obs-cpt/Observer> ;
    skos:definition "An ObservingProcedure that this Observer can perform. If a reference to ObservingProcedure (s) is provided, the association with the role observingProcedure SHALL be used." ;
    skos:inScheme <http://www.opengis.net/spec/OMS/3.0> ;
    skos:prefLabel "Requirement: /req/obs-cpt/Observer/observingProcedure-sem" .

<http://www.opengis.net/spec/OMS/3.0/req/obs-cpt/ObservingProcedure/ObservingProcedure-sem> a spec:Requirement,
        skos:Concept ;
    dcterms:description "The description of steps performed in order to determine the value of an observableProperty by an Observer ." ;
    skos:broader <http://www.opengis.net/spec/OMS/3.0/req/obs-cpt/ObservingProcedure> ;
    skos:definition "The description of steps performed in order to determine the value of an observableProperty by an Observer ." ;
    skos:inScheme <http://www.opengis.net/spec/OMS/3.0> ;
    skos:prefLabel "Requirement: /req/obs-cpt/ObservingProcedure/ObservingProcedure-sem" .

<http://www.opengis.net/spec/OMS/3.0/req/obs-cpt/ObservingProcedure/observer-sem> a spec:Requirement,
        skos:Concept ;
    dcterms:description "An Observer capable of performing this ObservingProcedure . If a reference to an Observer is provided, the association with the role observer SHALL be used." ;
    skos:broader <http://www.opengis.net/spec/OMS/3.0/req/obs-cpt/ObservingProcedure> ;
    skos:definition "An Observer capable of performing this ObservingProcedure . If a reference to an Observer is provided, the association with the role observer SHALL be used." ;
    skos:inScheme <http://www.opengis.net/spec/OMS/3.0> ;
    skos:prefLabel "Requirement: /req/obs-cpt/ObservingProcedure/observer-sem" .

<http://www.opengis.net/spec/OMS/3.0/req/obs-cpt/Procedure/Procedure-sem> a spec:Requirement,
        skos:Concept ;
    dcterms:description "A description of steps performed." ;
    skos:broader <http://www.opengis.net/spec/OMS/3.0/req/obs-cpt/Procedure> ;
    skos:definition "A description of steps performed." ;
    skos:inScheme <http://www.opengis.net/spec/OMS/3.0> ;
    skos:prefLabel "Requirement: /req/obs-cpt/Procedure/Procedure-sem" .

<http://www.opengis.net/spec/OMS/3.0/req/obs-cpt/gen/relatedObservation-sem> a spec:Requirement,
        skos:Concept ;
    dcterms:description "An Observation the Observation is related to. If a reference to a related Observation is provided, the association with role relatedObservation SHALL be used. The context:GenericName qualifier of this association may be used to provide further information as to the nature of the relation." ;
    skos:broader <http://www.opengis.net/spec/OMS/3.0/req/obs-cpt/Host> ;
    skos:broader <http://www.opengis.net/spec/OMS/3.0/req/obs-cpt/ObservingProcedure> ;
    skos:broader <http://www.opengis.net/spec/OMS/3.0/req/obs-cpt/Observation> ;
    skos:broader <http://www.opengis.net/spec/OMS/3.0/req/obs-cpt/ObservableProperty> ;
    skos:broader <http://www.opengis.net/spec/OMS/3.0/req/obs-cpt/Observer> ;
    skos:broader <http://www.opengis.net/spec/OMS/3.0/req/obs-core/AbstractObservationCharacteristics> ;
    skos:broader <http://www.opengis.net/spec/OMS/3.0/req/sam-cpt/Sample> ;
    skos:broader <http://www.opengis.net/spec/OMS/3.0/req/obs-basic/ObservationCollection> ;
    skos:definition "An Observation the Observation is related to. If a reference to a related Observation is provided, the association with role relatedObservation SHALL be used. The context:GenericName qualifier of this association may be used to provide further information as to the nature of the relation." ;
    skos:inScheme <http://www.opengis.net/spec/OMS/3.0> ;
    skos:prefLabel "Requirement: /req/obs-cpt/gen/relatedObservation-sem" .

<http://www.opengis.net/spec/OMS/3.0/req/sam-basic/MaterialSample/MaterialSample-sem> a spec:Requirement,
        skos:Concept ;
    dcterms:description "A MaterialSample is a physical, tangible Sample ." ;
    skos:broader <http://www.opengis.net/spec/OMS/3.0/req/sam-basic/MaterialSample> ;
    skos:definition "A MaterialSample is a physical, tangible Sample ." ;
    skos:inScheme <http://www.opengis.net/spec/OMS/3.0> ;
    skos:prefLabel "Requirement: /req/sam-basic/MaterialSample/MaterialSample-sem" .

<http://www.opengis.net/spec/OMS/3.0/req/sam-basic/MaterialSample/size-sem> a spec:Requirement,
        skos:Concept ;
    dcterms:description "The size describes a physical extent of the specimen. If size information pertaining to the MaterialSample is provided, the attribute size:PhysicalDimension SHALL be used." ;
    skos:broader <http://www.opengis.net/spec/OMS/3.0/req/sam-basic/MaterialSample> ;
    skos:definition "The size describes a physical extent of the specimen. If size information pertaining to the MaterialSample is provided, the attribute size:PhysicalDimension SHALL be used." ;
    skos:inScheme <http://www.opengis.net/spec/OMS/3.0> ;
    skos:prefLabel "Requirement: /req/sam-basic/MaterialSample/size-sem" .

<http://www.opengis.net/spec/OMS/3.0/req/sam-basic/MaterialSample/sourceLocation-sem> a spec:Requirement,
        skos:Concept ;
    dcterms:description "The sourceLocation is the location from where the MaterialSample was obtained. If information pertaining to the source location of the MaterialSample is provided, the attribute sourceLocation:Geometry SHALL be used." ;
    skos:broader <http://www.opengis.net/spec/OMS/3.0/req/sam-basic/MaterialSample> ;
    skos:definition "The sourceLocation is the location from where the MaterialSample was obtained. If information pertaining to the source location of the MaterialSample is provided, the attribute sourceLocation:Geometry SHALL be used." ;
    skos:inScheme <http://www.opengis.net/spec/OMS/3.0> ;
    skos:prefLabel "Requirement: /req/sam-basic/MaterialSample/sourceLocation-sem" .

<http://www.opengis.net/spec/OMS/3.0/req/sam-basic/MaterialSample/storageLocation-sem> a spec:Requirement,
        skos:Concept ;
    dcterms:description "The storageLocation is the location of a MaterialSample . If information pertaining to the storage location of the MaterialSample is provided, the attribute storageLocation:NamedLocation SHALL be used." ;
    skos:broader <http://www.opengis.net/spec/OMS/3.0/req/sam-basic/MaterialSample> ;
    skos:definition "The storageLocation is the location of a MaterialSample . If information pertaining to the storage location of the MaterialSample is provided, the attribute storageLocation:NamedLocation SHALL be used." ;
    skos:inScheme <http://www.opengis.net/spec/OMS/3.0> ;
    skos:prefLabel "Requirement: /req/sam-basic/MaterialSample/storageLocation-sem" .

<http://www.opengis.net/spec/OMS/3.0/req/sam-basic/NamedLocation/NamedLocation-sem> a spec:Requirement,
        skos:Concept ;
    dcterms:description "A location identified by its name, address, spatial geometry or a combination of any of these three." ;
    skos:broader <http://www.opengis.net/spec/OMS/3.0/req/sam-basic/NamedLocation> ;
    skos:definition "A location identified by its name, address, spatial geometry or a combination of any of these three." ;
    skos:inScheme <http://www.opengis.net/spec/OMS/3.0> ;
    skos:prefLabel "Requirement: /req/sam-basic/NamedLocation/NamedLocation-sem" .

<http://www.opengis.net/spec/OMS/3.0/req/sam-basic/NamedLocation/address-sem> a spec:Requirement,
        skos:Concept ;
    dcterms:description "An address used for identifying a NamedLocation. If address information is provided, the attribute address:Any SHALL be used." ;
    skos:broader <http://www.opengis.net/spec/OMS/3.0/req/sam-basic/NamedLocation> ;
    skos:definition "An address used for identifying a NamedLocation. If address information is provided, the attribute address:Any SHALL be used." ;
    skos:inScheme <http://www.opengis.net/spec/OMS/3.0> ;
    skos:prefLabel "Requirement: /req/sam-basic/NamedLocation/address-sem" .

<http://www.opengis.net/spec/OMS/3.0/req/sam-basic/NamedLocation/name-sem> a spec:Requirement,
        skos:Concept ;
    dcterms:description "A name used for identifying a NamedLocation. If name information is provided, the attribute name:GenericName SHALL be used." ;
    skos:broader <http://www.opengis.net/spec/OMS/3.0/req/sam-basic/NamedLocation> ;
    skos:definition "A name used for identifying a NamedLocation. If name information is provided, the attribute name:GenericName SHALL be used." ;
    skos:inScheme <http://www.opengis.net/spec/OMS/3.0> ;
    skos:prefLabel "Requirement: /req/sam-basic/NamedLocation/name-sem" .

<http://www.opengis.net/spec/OMS/3.0/req/sam-basic/NamedLocation/representativeGeometry-sem> a spec:Requirement,
        skos:Concept ;
    dcterms:description "A geometry used for providing a representative spatial location of a NamedLocation. If geometry is provided, the attribute representativeGeometry:Geometry SHALL be used." ;
    skos:broader <http://www.opengis.net/spec/OMS/3.0/req/sam-basic/NamedLocation> ;
    skos:definition "A geometry used for providing a representative spatial location of a NamedLocation. If geometry is provided, the attribute representativeGeometry:Geometry SHALL be used." ;
    skos:inScheme <http://www.opengis.net/spec/OMS/3.0> ;
    skos:prefLabel "Requirement: /req/sam-basic/NamedLocation/representativeGeometry-sem" .

<http://www.opengis.net/spec/OMS/3.0/req/sam-basic/PhysicalDimension/PhysicalDimension-sem> a spec:Requirement,
        skos:Concept ;
    dcterms:description "A dataType for the provision of various size quantities." ;
    skos:broader <http://www.opengis.net/spec/OMS/3.0/req/sam-basic/PhysicalDimension> ;
    skos:definition "A dataType for the provision of various size quantities." ;
    skos:inScheme <http://www.opengis.net/spec/OMS/3.0> ;
    skos:prefLabel "Requirement: /req/sam-basic/PhysicalDimension/PhysicalDimension-sem" .

<http://www.opengis.net/spec/OMS/3.0/req/sam-basic/PhysicalDimension/dimension-sem> a spec:Requirement,
        skos:Concept ;
    dcterms:description "The PhysicalDimension about which a value is provided. The name of the physical dimension, the quantity being provided in the value SHALL be provided in the attribute dimension:URI." ;
    skos:broader <http://www.opengis.net/spec/OMS/3.0/req/sam-basic/PhysicalDimension> ;
    skos:definition "The PhysicalDimension about which a value is provided. The name of the physical dimension, the quantity being provided in the value SHALL be provided in the attribute dimension:URI." ;
    skos:inScheme <http://www.opengis.net/spec/OMS/3.0> ;
    skos:prefLabel "Requirement: /req/sam-basic/PhysicalDimension/dimension-sem" .

<http://www.opengis.net/spec/OMS/3.0/req/sam-basic/PhysicalDimension/value-sem> a spec:Requirement,
        skos:Concept ;
    dcterms:description "The value of the PhysicalDimension . The measure of the quantity being provided SHALL be provided in the attribute value:Measure" ;
    skos:broader <http://www.opengis.net/spec/OMS/3.0/req/sam-basic/PhysicalDimension> ;
    skos:definition "The value of the PhysicalDimension . The measure of the quantity being provided SHALL be provided in the attribute value:Measure" ;
    skos:inScheme <http://www.opengis.net/spec/OMS/3.0> ;
    skos:prefLabel "Requirement: /req/sam-basic/PhysicalDimension/value-sem" .

<http://www.opengis.net/spec/OMS/3.0/req/sam-basic/SampleCollection/SampleCollection-sem> a spec:Requirement,
        skos:Concept ;
    dcterms:description "A collection of Sample s." ;
    skos:broader <http://www.opengis.net/spec/OMS/3.0/req/sam-basic/SampleCollection> ;
    skos:definition "A collection of Sample s." ;
    skos:inScheme <http://www.opengis.net/spec/OMS/3.0> ;
    skos:prefLabel "Requirement: /req/sam-basic/SampleCollection/SampleCollection-sem" .

<http://www.opengis.net/spec/OMS/3.0/req/sam-basic/SampleCollection/member-sem> a spec:Requirement,
        skos:Concept ;
    dcterms:description "A member of the SampleCollection . If the SampleCollection has members, the association with the role member SHALL be used." ;
    skos:broader <http://www.opengis.net/spec/OMS/3.0/req/sam-basic/SampleCollection> ;
    skos:definition "A member of the SampleCollection . If the SampleCollection has members, the association with the role member SHALL be used." ;
    skos:inScheme <http://www.opengis.net/spec/OMS/3.0> ;
    skos:prefLabel "Requirement: /req/sam-basic/SampleCollection/member-sem" .

<http://www.opengis.net/spec/OMS/3.0/req/sam-basic/SampleCollection/relatedCollection-sem> a spec:Requirement,
        skos:Concept ;
    dcterms:description "A SampleCollection the SampleCollection is related to. If a reference to a related SampleCollection is provided, the association with role relatedCollection SHALL be used. The context:GenericName qualifier of this association may be used to provide further information as to the nature of the relation." ;
    skos:broader <http://www.opengis.net/spec/OMS/3.0/req/sam-basic/SampleCollection> ;
    skos:definition "A SampleCollection the SampleCollection is related to. If a reference to a related SampleCollection is provided, the association with role relatedCollection SHALL be used. The context:GenericName qualifier of this association may be used to provide further information as to the nature of the relation." ;
    skos:inScheme <http://www.opengis.net/spec/OMS/3.0> ;
    skos:prefLabel "Requirement: /req/sam-basic/SampleCollection/relatedCollection-sem" .

<http://www.opengis.net/spec/OMS/3.0/req/sam-basic/SpatialSample/SpatialSample-sem> a spec:Requirement,
        skos:Concept ;
    dcterms:description "A SpatialSample is a geospatial Sample ." ;
    skos:broader <http://www.opengis.net/spec/OMS/3.0/req/sam-basic/SpatialSample> ;
    skos:definition "A SpatialSample is a geospatial Sample ." ;
    skos:inScheme <http://www.opengis.net/spec/OMS/3.0> ;
    skos:prefLabel "Requirement: /req/sam-basic/SpatialSample/SpatialSample-sem" .

<http://www.opengis.net/spec/OMS/3.0/req/sam-basic/SpatialSample/horizontalPositionalAccuracy-sem> a spec:Requirement,
        skos:Concept ;
    dcterms:description "The PositionalAccuracy of the horizontal component of the Geometry of the SpatialSample . If horizontal PositionalAccuracy information pertaining to the SpatialSample is provided, the attribute horizontalPositionalAccuracy:Any SHALL be used." ;
    skos:broader <http://www.opengis.net/spec/OMS/3.0/req/sam-basic/SpatialSample> ;
    skos:definition "The PositionalAccuracy of the horizontal component of the Geometry of the SpatialSample . If horizontal PositionalAccuracy information pertaining to the SpatialSample is provided, the attribute horizontalPositionalAccuracy:Any SHALL be used." ;
    skos:inScheme <http://www.opengis.net/spec/OMS/3.0> ;
    skos:prefLabel "Requirement: /req/sam-basic/SpatialSample/horizontalPositionalAccuracy-sem" .

<http://www.opengis.net/spec/OMS/3.0/req/sam-basic/SpatialSample/shape-sem> a spec:Requirement,
        skos:Concept ;
    dcterms:description "The shape is the Geometry of the SpatialSample . If location information pertaining to the SpatialSample is provided, the attribute shape:Geometry SHALL be used." ;
    skos:broader <http://www.opengis.net/spec/OMS/3.0/req/sam-basic/SpatialSample> ;
    skos:definition "The shape is the Geometry of the SpatialSample . If location information pertaining to the SpatialSample is provided, the attribute shape:Geometry SHALL be used." ;
    skos:inScheme <http://www.opengis.net/spec/OMS/3.0> ;
    skos:prefLabel "Requirement: /req/sam-basic/SpatialSample/shape-sem" .

<http://www.opengis.net/spec/OMS/3.0/req/sam-basic/SpatialSample/verticalPositionalAccuracy-sem> a spec:Requirement,
        skos:Concept ;
    dcterms:description "The PositionalAccuracy of the vertical component of the Geometry of the SpatialSample . If horizontal PositionalAccuracy information pertaining to the SpatialSample is provided, the attribute verticalPositionalAccuracy:Any SHALL be used." ;
    skos:broader <http://www.opengis.net/spec/OMS/3.0/req/sam-basic/SpatialSample> ;
    skos:definition "The PositionalAccuracy of the vertical component of the Geometry of the SpatialSample . If horizontal PositionalAccuracy information pertaining to the SpatialSample is provided, the attribute verticalPositionalAccuracy:Any SHALL be used." ;
    skos:inScheme <http://www.opengis.net/spec/OMS/3.0> ;
    skos:prefLabel "Requirement: /req/sam-basic/SpatialSample/verticalPositionalAccuracy-sem" .

<http://www.opengis.net/spec/OMS/3.0/req/sam-basic/StatisticalClassification/StatisticalClassification-sem> a spec:Requirement,
        skos:Concept ;
    dcterms:description "A dataType for the provision of information on statistical classifications." ;
    skos:broader <http://www.opengis.net/spec/OMS/3.0/req/sam-basic/StatisticalClassification> ;
    skos:definition "A dataType for the provision of information on statistical classifications." ;
    skos:inScheme <http://www.opengis.net/spec/OMS/3.0> ;
    skos:prefLabel "Requirement: /req/sam-basic/StatisticalClassification/StatisticalClassification-sem" .

<http://www.opengis.net/spec/OMS/3.0/req/sam-basic/StatisticalClassification/classification-sem> a spec:Requirement,
        skos:Concept ;
    dcterms:description "The explicit classification class pertaining to the classification concept described by the StatisticalClassification . The classification class of the StatisticalClassification SHALL be provided in the attribute classification:URI." ;
    skos:broader <http://www.opengis.net/spec/OMS/3.0/req/sam-basic/StatisticalClassification> ;
    skos:definition "The explicit classification class pertaining to the classification concept described by the StatisticalClassification . The classification class of the StatisticalClassification SHALL be provided in the attribute classification:URI." ;
    skos:inScheme <http://www.opengis.net/spec/OMS/3.0> ;
    skos:prefLabel "Requirement: /req/sam-basic/StatisticalClassification/classification-sem" .

<http://www.opengis.net/spec/OMS/3.0/req/sam-basic/StatisticalClassification/concept-sem> a spec:Requirement,
        skos:Concept ;
    dcterms:description "The concept by which a StatisticalClassification is to be performed. The name of the concept by which the statistical classification is performed SHALL be provided in the attribute concept:URI." ;
    skos:broader <http://www.opengis.net/spec/OMS/3.0/req/sam-basic/StatisticalClassification> ;
    skos:definition "The concept by which a StatisticalClassification is to be performed. The name of the concept by which the statistical classification is performed SHALL be provided in the attribute concept:URI." ;
    skos:inScheme <http://www.opengis.net/spec/OMS/3.0> ;
    skos:prefLabel "Requirement: /req/sam-basic/StatisticalClassification/concept-sem" .

<http://www.opengis.net/spec/OMS/3.0/req/sam-basic/StatisticalSample/StatisticalSample-sem> a spec:Requirement,
        skos:Concept ;
    dcterms:description "A StatisticalSample is a statistical subset of a feature-of-interest, defined for the purpose of creating Observation (s)." ;
    skos:broader <http://www.opengis.net/spec/OMS/3.0/req/sam-basic/StatisticalSample> ;
    skos:definition "A StatisticalSample is a statistical subset of a feature-of-interest, defined for the purpose of creating Observation (s)." ;
    skos:inScheme <http://www.opengis.net/spec/OMS/3.0> ;
    skos:prefLabel "Requirement: /req/sam-basic/StatisticalSample/StatisticalSample-sem" .

<http://www.opengis.net/spec/OMS/3.0/req/sam-basic/StatisticalSample/classification-sem> a spec:Requirement,
        skos:Concept ;
    dcterms:description "The classification describes a criterion by which the subset was defined. If information pertaining to the subsetting criteria by which a StatisticalSample has been defined is provided, the attribute classification:StatisticalClassification SHALL be used." ;
    skos:broader <http://www.opengis.net/spec/OMS/3.0/req/sam-basic/StatisticalSample> ;
    skos:definition "The classification describes a criterion by which the subset was defined. If information pertaining to the subsetting criteria by which a StatisticalSample has been defined is provided, the attribute classification:StatisticalClassification SHALL be used." ;
    skos:inScheme <http://www.opengis.net/spec/OMS/3.0> ;
    skos:prefLabel "Requirement: /req/sam-basic/StatisticalSample/classification-sem" .

<http://www.opengis.net/spec/OMS/3.0/req/sam-core/AbstractPreparationStep/description-sem> a spec:Requirement,
        skos:Concept ;
    dcterms:description "Description of the preparationStep . If a description pertaining to the preparationStep is provided, the attribute description:CharacterString SHALL be used." ;
    skos:broader <http://www.opengis.net/spec/OMS/3.0/req/sam-core/AbstractPreparationStep> ;
    skos:definition "Description of the preparationStep . If a description pertaining to the preparationStep is provided, the attribute description:CharacterString SHALL be used." ;
    skos:inScheme <http://www.opengis.net/spec/OMS/3.0> ;
    skos:prefLabel "Requirement: /req/sam-core/AbstractPreparationStep/description-sem" .

<http://www.opengis.net/spec/OMS/3.0/req/sam-core/AbstractPreparationStep/time-sem> a spec:Requirement,
        skos:Concept ;
    dcterms:description "Time of the preparationStep . If information on the time of the preparationStep of the Sampling is provided, the attribute time:TM_Object SHALL be used." ;
    skos:broader <http://www.opengis.net/spec/OMS/3.0/req/sam-core/AbstractPreparationStep> ;
    skos:definition "Time of the preparationStep . If information on the time of the preparationStep of the Sampling is provided, the attribute time:TM_Object SHALL be used." ;
    skos:inScheme <http://www.opengis.net/spec/OMS/3.0> ;
    skos:prefLabel "Requirement: /req/sam-core/AbstractPreparationStep/time-sem" .

<http://www.opengis.net/spec/OMS/3.0/req/sam-core/AbstractSample/parameter-sem> a spec:Requirement,
        skos:Concept ;
    dcterms:description "Arbitrary event-specific parameter relevant to the Sample . If additional parameter information is provided, the property parameter : NamedValue SHALL be used." ;
    skos:broader <http://www.opengis.net/spec/OMS/3.0/req/sam-core/AbstractSample> ;
    skos:definition "Arbitrary event-specific parameter relevant to the Sample . If additional parameter information is provided, the property parameter : NamedValue SHALL be used." ;
    skos:inScheme <http://www.opengis.net/spec/OMS/3.0> ;
    skos:prefLabel "Requirement: /req/sam-core/AbstractSample/parameter-sem" .

<http://www.opengis.net/spec/OMS/3.0/req/sam-core/AbstractSample/sampleType-sem> a spec:Requirement,
        skos:Concept ;
    dcterms:description "The type of Sample according to a community agreed typology. If information on the type of AbstractSample is provided, the attribute sampleType:AbstractSampleTypeCodeListValue shall be used." ;
    skos:broader <http://www.opengis.net/spec/OMS/3.0/req/sam-core/AbstractSample> ;
    skos:definition "The type of Sample according to a community agreed typology. If information on the type of AbstractSample is provided, the attribute sampleType:AbstractSampleTypeCodeListValue shall be used." ;
    skos:inScheme <http://www.opengis.net/spec/OMS/3.0> ;
    skos:prefLabel "Requirement: /req/sam-core/AbstractSample/sampleType-sem" .

<http://www.opengis.net/spec/OMS/3.0/req/sam-core/AbstractSampler/samplerType-sem> a spec:Requirement,
        skos:Concept ;
    dcterms:description "The type of Sampler according to a community agreed typology. If information on the type of AbstractSampler is provided, the attribute samplerType:AbstractSamplerTypeCodeListValue shall be used." ;
    skos:broader <http://www.opengis.net/spec/OMS/3.0/req/sam-core/AbstractSampler> ;
    skos:definition "The type of Sampler according to a community agreed typology. If information on the type of AbstractSampler is provided, the attribute samplerType:AbstractSamplerTypeCodeListValue shall be used." ;
    skos:inScheme <http://www.opengis.net/spec/OMS/3.0> ;
    skos:prefLabel "Requirement: /req/sam-core/AbstractSampler/samplerType-sem" .

<http://www.opengis.net/spec/OMS/3.0/req/sam-core/AbstractSampling/parameter-sem> a spec:Requirement,
        skos:Concept ;
    dcterms:description "Arbitrary event-specific parameter relevant to the Sampling . If additional parameter information is provided, the property parameter : NamedValue SHALL be used." ;
    skos:broader <http://www.opengis.net/spec/OMS/3.0/req/sam-core/AbstractSampling> ;
    skos:definition "Arbitrary event-specific parameter relevant to the Sampling . If additional parameter information is provided, the property parameter : NamedValue SHALL be used." ;
    skos:inScheme <http://www.opengis.net/spec/OMS/3.0> ;
    skos:prefLabel "Requirement: /req/sam-core/AbstractSampling/parameter-sem" .

<http://www.opengis.net/spec/OMS/3.0/req/sam-core/AbstractSampling/samplingLocation-sem> a spec:Requirement,
        skos:Concept ;
    dcterms:description "If location information pertaining to the Sampling is provided, the attribute samplingLocation:Geometry SHALL be used." ;
    skos:broader <http://www.opengis.net/spec/OMS/3.0/req/sam-core/AbstractSampling> ;
    skos:definition "If location information pertaining to the Sampling is provided, the attribute samplingLocation:Geometry SHALL be used." ;
    skos:inScheme <http://www.opengis.net/spec/OMS/3.0> ;
    skos:prefLabel "Requirement: /req/sam-core/AbstractSampling/samplingLocation-sem" .

<http://www.opengis.net/spec/OMS/3.0/req/sam-core/AbstractSampling/time-sem> a spec:Requirement,
        skos:Concept ;
    dcterms:description "If information on the time of the Sampling is provided, the attribute time:TM_Object SHALL be used." ;
    skos:broader <http://www.opengis.net/spec/OMS/3.0/req/sam-core/AbstractSampling> ;
    skos:definition "If information on the time of the Sampling is provided, the attribute time:TM_Object SHALL be used." ;
    skos:inScheme <http://www.opengis.net/spec/OMS/3.0> ;
    skos:prefLabel "Requirement: /req/sam-core/AbstractSampling/time-sem" .

<http://www.opengis.net/spec/OMS/3.0/req/sam-cpt/PreparationProcedure/PreparationProcedure-sem> a spec:Requirement,
        skos:Concept ;
    dcterms:description "The description of preparation steps performed on a Sample ." ;
    skos:broader <http://www.opengis.net/spec/OMS/3.0/req/sam-cpt/PreparationProcedure> ;
    skos:definition "The description of preparation steps performed on a Sample ." ;
    skos:inScheme <http://www.opengis.net/spec/OMS/3.0> ;
    skos:prefLabel "Requirement: /req/sam-cpt/PreparationProcedure/PreparationProcedure-sem" .

<http://www.opengis.net/spec/OMS/3.0/req/sam-cpt/PreparationProcedure/samplePreparationStep-sem> a spec:Requirement,
        skos:Concept ;
    dcterms:description "If the PreparingProcedure provides information on the PreparationStep where this procedure has been used, the association with the role samplePreparationStep SHALL be used." ;
    skos:broader <http://www.opengis.net/spec/OMS/3.0/req/sam-cpt/PreparationProcedure> ;
    skos:definition "If the PreparingProcedure provides information on the PreparationStep where this procedure has been used, the association with the role samplePreparationStep SHALL be used." ;
    skos:inScheme <http://www.opengis.net/spec/OMS/3.0> ;
    skos:prefLabel "Requirement: /req/sam-cpt/PreparationProcedure/samplePreparationStep-sem" .

<http://www.opengis.net/spec/OMS/3.0/req/sam-cpt/PreparationStep/PreparationStep-sem> a spec:Requirement,
        skos:Concept ;
    dcterms:description "A PreparationStep is an individual step pertaining to a PreparationProcedure ." ;
    skos:broader <http://www.opengis.net/spec/OMS/3.0/req/sam-cpt/PreparationStep> ;
    skos:definition "A PreparationStep is an individual step pertaining to a PreparationProcedure ." ;
    skos:inScheme <http://www.opengis.net/spec/OMS/3.0> ;
    skos:prefLabel "Requirement: /req/sam-cpt/PreparationStep/PreparationStep-sem" .

<http://www.opengis.net/spec/OMS/3.0/req/sam-cpt/PreparationStep/preparedSample-sem> a spec:Requirement,
        skos:Concept ;
    dcterms:description "The Sample on which the PreparationProcedure is performed. The Sample SHALL be referred to using the association with the role preparedSample ." ;
    skos:broader <http://www.opengis.net/spec/OMS/3.0/req/sam-cpt/PreparationStep> ;
    skos:definition "The Sample on which the PreparationProcedure is performed. The Sample SHALL be referred to using the association with the role preparedSample ." ;
    skos:inScheme <http://www.opengis.net/spec/OMS/3.0> ;
    skos:prefLabel "Requirement: /req/sam-cpt/PreparationStep/preparedSample-sem" .

<http://www.opengis.net/spec/OMS/3.0/req/sam-cpt/PreparationStep/processingDetails-sem> a spec:Requirement,
        skos:Concept ;
    dcterms:description "A PreparationProcedure step performed on the Sample the PreparationStep pertains to. If PreparationProcedure (s) are described they SHALL be referred to using the association with the role processingDetails ." ;
    skos:broader <http://www.opengis.net/spec/OMS/3.0/req/sam-cpt/PreparationStep> ;
    skos:definition "A PreparationProcedure step performed on the Sample the PreparationStep pertains to. If PreparationProcedure (s) are described they SHALL be referred to using the association with the role processingDetails ." ;
    skos:inScheme <http://www.opengis.net/spec/OMS/3.0> ;
    skos:prefLabel "Requirement: /req/sam-cpt/PreparationStep/processingDetails-sem" .

<http://www.opengis.net/spec/OMS/3.0/req/sam-cpt/Sample/Sample-sem> a spec:Requirement,
        skos:Concept ;
    dcterms:description "A Sample is an object that is representative of a concept, real-world object or phenomenon." ;
    skos:broader <http://www.opengis.net/spec/OMS/3.0/req/sam-cpt/Sample> ;
    skos:definition "A Sample is an object that is representative of a concept, real-world object or phenomenon." ;
    skos:inScheme <http://www.opengis.net/spec/OMS/3.0> ;
    skos:prefLabel "Requirement: /req/sam-cpt/Sample/Sample-sem" .

<http://www.opengis.net/spec/OMS/3.0/req/sam-cpt/Sample/preparationStep-sem> a spec:Requirement,
        skos:Concept ;
    dcterms:description "The PreparationStep (s) applied to prepare the Sample . If PreparationSteps are described they SHALL be referred to using the association with the role preparationStep ." ;
    skos:broader <http://www.opengis.net/spec/OMS/3.0/req/sam-cpt/Sample> ;
    skos:definition "The PreparationStep (s) applied to prepare the Sample . If PreparationSteps are described they SHALL be referred to using the association with the role preparationStep ." ;
    skos:inScheme <http://www.opengis.net/spec/OMS/3.0> ;
    skos:prefLabel "Requirement: /req/sam-cpt/Sample/preparationStep-sem" .

<http://www.opengis.net/spec/OMS/3.0/req/sam-cpt/Sample/relatedSample-sem> a spec:Requirement,
        skos:Concept ;
    dcterms:description "A Sample the Sample is related to. If a reference to a related Sample is provided, the association with role relatedSample SHALL be used. The context:GenericName qualifier of this association may be used to provide further information as to the nature of the relation." ;
    skos:broader <http://www.opengis.net/spec/OMS/3.0/req/sam-cpt/Sample> ;
    skos:definition "A Sample the Sample is related to. If a reference to a related Sample is provided, the association with role relatedSample SHALL be used. The context:GenericName qualifier of this association may be used to provide further information as to the nature of the relation." ;
    skos:inScheme <http://www.opengis.net/spec/OMS/3.0> ;
    skos:prefLabel "Requirement: /req/sam-cpt/Sample/relatedSample-sem" .

<http://www.opengis.net/spec/OMS/3.0/req/sam-cpt/Sample/sampledFeature-card> a spec:Requirement,
        skos:Concept ;
    dcterms:description "" ;
    skos:broader <http://www.opengis.net/spec/OMS/3.0/req/sam-cpt/Sample> ;
    skos:definition "" ;
    skos:inScheme <http://www.opengis.net/spec/OMS/3.0> ;
    skos:prefLabel "Requirement: /req/sam-cpt/Sample/sampledFeature-card" .

<http://www.opengis.net/spec/OMS/3.0/req/sam-cpt/Sample/sampledFeature-sem> a spec:Requirement,
        skos:Concept ;
    dcterms:description "The sampledFeature is the feature the Sample is intended to be representative of. References to the sampled feature SHALL be provided using the association with the role sampledFeature ." ;
    skos:broader <http://www.opengis.net/spec/OMS/3.0/req/sam-cpt/Sample> ;
    skos:definition "The sampledFeature is the feature the Sample is intended to be representative of. References to the sampled feature SHALL be provided using the association with the role sampledFeature ." ;
    skos:inScheme <http://www.opengis.net/spec/OMS/3.0> ;
    skos:prefLabel "Requirement: /req/sam-cpt/Sample/sampledFeature-sem" .

<http://www.opengis.net/spec/OMS/3.0/req/sam-cpt/Sample/sampling-sem> a spec:Requirement,
        skos:Concept ;
    dcterms:description "The Sampling the Sample is the result of. If Sampling (s) are described they SHALL be referred to using the association with the role sampling ." ;
    skos:broader <http://www.opengis.net/spec/OMS/3.0/req/sam-cpt/Sample> ;
    skos:definition "The Sampling the Sample is the result of. If Sampling (s) are described they SHALL be referred to using the association with the role sampling ." ;
    skos:inScheme <http://www.opengis.net/spec/OMS/3.0> ;
    skos:prefLabel "Requirement: /req/sam-cpt/Sample/sampling-sem" .

<http://www.opengis.net/spec/OMS/3.0/req/sam-cpt/Sampler/Sampler-sem> a spec:Requirement,
        skos:Concept ;
    dcterms:description "A Sampler is a device or entity (including humans) that is used by, or implements, a SamplingProcedure to create or transform one or more Sample (s)." ;
    skos:broader <http://www.opengis.net/spec/OMS/3.0/req/sam-cpt/Sampler> ;
    skos:definition "A Sampler is a device or entity (including humans) that is used by, or implements, a SamplingProcedure to create or transform one or more Sample (s)." ;
    skos:inScheme <http://www.opengis.net/spec/OMS/3.0> ;
    skos:prefLabel "Requirement: /req/sam-cpt/Sampler/Sampler-sem" .

<http://www.opengis.net/spec/OMS/3.0/req/sam-cpt/Sampler/implementedProcedure-sem> a spec:Requirement,
        skos:Concept ;
    dcterms:description "The Procedure implemented by the Sampler . If Procedure (s) are described they SHALL be referred to using the association with the role implementedProcedure ." ;
    skos:broader <http://www.opengis.net/spec/OMS/3.0/req/sam-cpt/Sampler> ;
    skos:definition "The Procedure implemented by the Sampler . If Procedure (s) are described they SHALL be referred to using the association with the role implementedProcedure ." ;
    skos:inScheme <http://www.opengis.net/spec/OMS/3.0> ;
    skos:prefLabel "Requirement: /req/sam-cpt/Sampler/implementedProcedure-sem" .

<http://www.opengis.net/spec/OMS/3.0/req/sam-cpt/Sampler/sampling-sem> a spec:Requirement,
        skos:Concept ;
    dcterms:description "The Sampling act performed by the Sampler . If Sampling (s) are described they SHALL be referred to using the association with the role sampling ." ;
    skos:broader <http://www.opengis.net/spec/OMS/3.0/req/sam-cpt/Sampler> ;
    skos:definition "The Sampling act performed by the Sampler . If Sampling (s) are described they SHALL be referred to using the association with the role sampling ." ;
    skos:inScheme <http://www.opengis.net/spec/OMS/3.0> ;
    skos:prefLabel "Requirement: /req/sam-cpt/Sampler/sampling-sem" .

<http://www.opengis.net/spec/OMS/3.0/req/sam-cpt/Sampling/Sampling-sem> a spec:Requirement,
        skos:Concept ;
    dcterms:description "Sampling is an act applying a Sampling Procedure to create or transform one or more Sample (s)." ;
    skos:broader <http://www.opengis.net/spec/OMS/3.0/req/sam-cpt/Sampling> ;
    skos:definition "Sampling is an act applying a Sampling Procedure to create or transform one or more Sample (s)." ;
    skos:inScheme <http://www.opengis.net/spec/OMS/3.0> ;
    skos:prefLabel "Requirement: /req/sam-cpt/Sampling/Sampling-sem" .

<http://www.opengis.net/spec/OMS/3.0/req/sam-cpt/Sampling/featureOfInterest-card> a spec:Requirement,
        skos:Concept ;
    dcterms:description "Reference to the feature-of-interest SHALL be done using the association with the role featureOfInterest ." ;
    skos:broader <http://www.opengis.net/spec/OMS/3.0/req/sam-cpt/Sampling> ;
    skos:definition "Reference to the feature-of-interest SHALL be done using the association with the role featureOfInterest ." ;
    skos:inScheme <http://www.opengis.net/spec/OMS/3.0> ;
    skos:prefLabel "Requirement: /req/sam-cpt/Sampling/featureOfInterest-card" .

<http://www.opengis.net/spec/OMS/3.0/req/sam-cpt/Sampling/featureOfInterest-sem> a spec:Requirement,
        skos:Concept ;
    dcterms:description "The concept, real-world object or phenomenon (feature-of-interest) the Sample (s) of the Sampling represent ." ;
    skos:broader <http://www.opengis.net/spec/OMS/3.0/req/sam-cpt/Sampling> ;
    skos:definition "The concept, real-world object or phenomenon (feature-of-interest) the Sample (s) of the Sampling represent ." ;
    skos:inScheme <http://www.opengis.net/spec/OMS/3.0> ;
    skos:prefLabel "Requirement: /req/sam-cpt/Sampling/featureOfInterest-sem" .

<http://www.opengis.net/spec/OMS/3.0/req/sam-cpt/Sampling/relatedSampling-sem> a spec:Requirement,
        skos:Concept ;
    dcterms:description "Related Sampling (s). If a reference to a related Sampling is provided, the association with role relatedSampling SHALL be used. The context:GenericName qualifier of this association may be used to provide further information as to the nature of the relation." ;
    skos:broader <http://www.opengis.net/spec/OMS/3.0/req/sam-cpt/Sampling> ;
    skos:definition "Related Sampling (s). If a reference to a related Sampling is provided, the association with role relatedSampling SHALL be used. The context:GenericName qualifier of this association may be used to provide further information as to the nature of the relation." ;
    skos:inScheme <http://www.opengis.net/spec/OMS/3.0> ;
    skos:prefLabel "Requirement: /req/sam-cpt/Sampling/relatedSampling-sem" .

<http://www.opengis.net/spec/OMS/3.0/req/sam-cpt/Sampling/sample-sem> a spec:Requirement,
        skos:Concept ;
    dcterms:description "The Sample generated by the Sampling. If Samples are described they SHALL be referred to using the association with the role sample ." ;
    skos:broader <http://www.opengis.net/spec/OMS/3.0/req/sam-cpt/Sampling> ;
    skos:definition "The Sample generated by the Sampling. If Samples are described they SHALL be referred to using the association with the role sample ." ;
    skos:inScheme <http://www.opengis.net/spec/OMS/3.0> ;
    skos:prefLabel "Requirement: /req/sam-cpt/Sampling/sample-sem" .

<http://www.opengis.net/spec/OMS/3.0/req/sam-cpt/Sampling/sampler-sem> a spec:Requirement,
        skos:Concept ;
    dcterms:description "The Sampler that performed the Sampling . If Sampler (s) are described they SHALL be referred to using the association with the role sampler ." ;
    skos:broader <http://www.opengis.net/spec/OMS/3.0/req/sam-cpt/Sampling> ;
    skos:definition "The Sampler that performed the Sampling . If Sampler (s) are described they SHALL be referred to using the association with the role sampler ." ;
    skos:inScheme <http://www.opengis.net/spec/OMS/3.0> ;
    skos:prefLabel "Requirement: /req/sam-cpt/Sampling/sampler-sem" .

<http://www.opengis.net/spec/OMS/3.0/req/sam-cpt/Sampling/samplingProcedure-sem> a spec:Requirement,
        skos:Concept ;
    dcterms:description "The SamplingProcedure used by the Sampling. If SamplingProcedures are described they SHALL be referred to using the association with the role samplingProcedure ." ;
    skos:broader <http://www.opengis.net/spec/OMS/3.0/req/sam-cpt/Sampling> ;
    skos:definition "The SamplingProcedure used by the Sampling. If SamplingProcedures are described they SHALL be referred to using the association with the role samplingProcedure ." ;
    skos:inScheme <http://www.opengis.net/spec/OMS/3.0> ;
    skos:prefLabel "Requirement: /req/sam-cpt/Sampling/samplingProcedure-sem" .

<http://www.opengis.net/spec/OMS/3.0/req/sam-cpt/SamplingProcedure/SamplingProcedure-sem> a spec:Requirement,
        skos:Concept ;
    dcterms:description "The description of steps performed by a Sampler in order to extract a Sample from its sampledFeature in the frame of a Sampling." ;
    skos:broader <http://www.opengis.net/spec/OMS/3.0/req/sam-cpt/SamplingProcedure> ;
    skos:definition "The description of steps performed by a Sampler in order to extract a Sample from its sampledFeature in the frame of a Sampling." ;
    skos:inScheme <http://www.opengis.net/spec/OMS/3.0> ;
    skos:prefLabel "Requirement: /req/sam-cpt/SamplingProcedure/SamplingProcedure-sem" .

<http://www.opengis.net/spec/OMS/3.0/req/sam-cpt/SamplingProcedure/sampler-sem> a spec:Requirement,
        skos:Concept ;
    dcterms:description "If the SamplingProcedure provides information on the Sampler that implements this procedure has been used, the association with the role sampler SHALL be used." ;
    skos:broader <http://www.opengis.net/spec/OMS/3.0/req/sam-cpt/SamplingProcedure> ;
    skos:definition "If the SamplingProcedure provides information on the Sampler that implements this procedure has been used, the association with the role sampler SHALL be used." ;
    skos:inScheme <http://www.opengis.net/spec/OMS/3.0> ;
    skos:prefLabel "Requirement: /req/sam-cpt/SamplingProcedure/sampler-sem" .

<http://www.opengis.net/spec/OMS/3.0/req/sam-cpt/SamplingProcedure/sampling-sem> a spec:Requirement,
        skos:Concept ;
    dcterms:description "If the SamplingProcedure provides information on the Sampling where this procedure has been used, the association with the role sampling SHALL be used." ;
    skos:broader <http://www.opengis.net/spec/OMS/3.0/req/sam-cpt/SamplingProcedure> ;
    skos:definition "If the SamplingProcedure provides information on the Sampling where this procedure has been used, the association with the role sampling SHALL be used." ;
    skos:inScheme <http://www.opengis.net/spec/OMS/3.0> ;
    skos:prefLabel "Requirement: /req/sam-cpt/SamplingProcedure/sampling-sem" .




<http://www.opengis.net/spec/OMS/3.0/conf/obs-basic> a spec:ConformanceClass,
        skos:Concept ;
    skos:definition "/conf/obs-basic" ;
    skos:inScheme <http://www.opengis.net/spec/OMS/3.0> ;
    skos:prefLabel "Conformance Class /conf/obs-basic" ;
    skos:topConceptOf <http://www.opengis.net/spec/OMS/3.0> .

<http://www.opengis.net/spec/OMS/3.0/conf/obs-basic/Deployment> a spec:ConformanceClass,
        skos:Concept ;
    skos:definition "/conf/obs-basic/Deployment" ;
    skos:inScheme <http://www.opengis.net/spec/OMS/3.0> ;
    skos:prefLabel "Conformance Class /conf/obs-basic/Deployment" ;
    skos:topConceptOf <http://www.opengis.net/spec/OMS/3.0> .

<http://www.opengis.net/spec/OMS/3.0/conf/obs-basic/GenericDomainFeature> a spec:ConformanceClass,
        skos:Concept ;
    skos:definition "/conf/obs-basic/GenericDomainFeature" ;
    skos:inScheme <http://www.opengis.net/spec/OMS/3.0> ;
    skos:prefLabel "Conformance Class /conf/obs-basic/GenericDomainFeature" ;
    skos:topConceptOf <http://www.opengis.net/spec/OMS/3.0> .

<http://www.opengis.net/spec/OMS/3.0/conf/obs-basic/Host> a spec:ConformanceClass,
        skos:Concept ;
    skos:definition "/conf/obs-basic/Host" ;
    skos:inScheme <http://www.opengis.net/spec/OMS/3.0> ;
    skos:prefLabel "Conformance Class /conf/obs-basic/Host" ;
    skos:topConceptOf <http://www.opengis.net/spec/OMS/3.0> .

<http://www.opengis.net/spec/OMS/3.0/conf/obs-basic/ObservableProperty> a spec:ConformanceClass,
        skos:Concept ;
    skos:definition "/conf/obs-basic/ObservableProperty" ;
    skos:inScheme <http://www.opengis.net/spec/OMS/3.0> ;
    skos:prefLabel "Conformance Class /conf/obs-basic/ObservableProperty" ;
    skos:topConceptOf <http://www.opengis.net/spec/OMS/3.0> .

<http://www.opengis.net/spec/OMS/3.0/conf/obs-basic/Observation> a spec:ConformanceClass,
        skos:Concept ;
    skos:definition "/conf/obs-basic/Observation" ;
    skos:inScheme <http://www.opengis.net/spec/OMS/3.0> ;
    skos:prefLabel "Conformance Class /conf/obs-basic/Observation" ;
    skos:topConceptOf <http://www.opengis.net/spec/OMS/3.0> .

<http://www.opengis.net/spec/OMS/3.0/conf/obs-basic/ObservationCharacteristics> a spec:ConformanceClass,
        skos:Concept ;
    skos:definition "/conf/obs-basic/ObservationCharacteristics" ;
    skos:inScheme <http://www.opengis.net/spec/OMS/3.0> ;
    skos:prefLabel "Conformance Class /conf/obs-basic/ObservationCharacteristics" ;
    skos:topConceptOf <http://www.opengis.net/spec/OMS/3.0> .

<http://www.opengis.net/spec/OMS/3.0/conf/obs-basic/ObservationCollection> a spec:ConformanceClass,
        skos:Concept ;
    skos:definition "/conf/obs-basic/ObservationCollection" ;
    skos:inScheme <http://www.opengis.net/spec/OMS/3.0> ;
    skos:prefLabel "Conformance Class /conf/obs-basic/ObservationCollection" ;
    skos:topConceptOf <http://www.opengis.net/spec/OMS/3.0> .

<http://www.opengis.net/spec/OMS/3.0/conf/obs-basic/Observer> a spec:ConformanceClass,
        skos:Concept ;
    skos:definition "/conf/obs-basic/Observer" ;
    skos:inScheme <http://www.opengis.net/spec/OMS/3.0> ;
    skos:prefLabel "Conformance Class /conf/obs-basic/Observer" ;
    skos:topConceptOf <http://www.opengis.net/spec/OMS/3.0> .

<http://www.opengis.net/spec/OMS/3.0/conf/obs-basic/ObservingCapability> a spec:ConformanceClass,
        skos:Concept ;
    skos:definition "/conf/obs-basic/ObservingCapability" ;
    skos:inScheme <http://www.opengis.net/spec/OMS/3.0> ;
    skos:prefLabel "Conformance Class /conf/obs-basic/ObservingCapability" ;
    skos:topConceptOf <http://www.opengis.net/spec/OMS/3.0> .

<http://www.opengis.net/spec/OMS/3.0/conf/obs-basic/ObservingProcedure> a spec:ConformanceClass,
        skos:Concept ;
    skos:definition "/conf/obs-basic/ObservingProcedure" ;
    skos:inScheme <http://www.opengis.net/spec/OMS/3.0> ;
    skos:prefLabel "Conformance Class /conf/obs-basic/ObservingProcedure" ;
    skos:topConceptOf <http://www.opengis.net/spec/OMS/3.0> .

<http://www.opengis.net/spec/OMS/3.0/conf/obs-core> a spec:ConformanceClass,
        skos:Concept ;
    skos:definition "/conf/obs-core" ;
    skos:inScheme <http://www.opengis.net/spec/OMS/3.0> ;
    skos:prefLabel "Conformance Class /conf/obs-core" ;
    skos:topConceptOf <http://www.opengis.net/spec/OMS/3.0> .

<http://www.opengis.net/spec/OMS/3.0/conf/obs-core/AbstractDeployment> a spec:ConformanceClass,
        skos:Concept ;
    skos:definition "/conf/obs-core/AbstractDeployment" ;
    skos:inScheme <http://www.opengis.net/spec/OMS/3.0> ;
    skos:prefLabel "Conformance Class /conf/obs-core/AbstractDeployment" ;
    skos:topConceptOf <http://www.opengis.net/spec/OMS/3.0> .

<http://www.opengis.net/spec/OMS/3.0/conf/obs-core/AbstractHost> a spec:ConformanceClass,
        skos:Concept ;
    skos:definition "/conf/obs-core/AbstractHost" ;
    skos:inScheme <http://www.opengis.net/spec/OMS/3.0> ;
    skos:prefLabel "Conformance Class /conf/obs-core/AbstractHost" ;
    skos:topConceptOf <http://www.opengis.net/spec/OMS/3.0> .

<http://www.opengis.net/spec/OMS/3.0/conf/obs-core/AbstractObservableProperty> a spec:ConformanceClass,
        skos:Concept ;
    skos:definition "/conf/obs-core/AbstractObservableProperty" ;
    skos:inScheme <http://www.opengis.net/spec/OMS/3.0> ;
    skos:prefLabel "Conformance Class /conf/obs-core/AbstractObservableProperty" ;
    skos:topConceptOf <http://www.opengis.net/spec/OMS/3.0> .

<http://www.opengis.net/spec/OMS/3.0/conf/obs-core/AbstractObservation> a spec:ConformanceClass,
        skos:Concept ;
    skos:definition "/conf/obs-core/AbstractObservation" ;
    skos:inScheme <http://www.opengis.net/spec/OMS/3.0> ;
    skos:prefLabel "Conformance Class /conf/obs-core/AbstractObservation" ;
    skos:topConceptOf <http://www.opengis.net/spec/OMS/3.0> .

<http://www.opengis.net/spec/OMS/3.0/conf/obs-core/AbstractObservationCharacteristics> a spec:ConformanceClass,
        skos:Concept ;
    skos:definition "/conf/obs-core/AbstractObservationCharacteristics" ;
    skos:inScheme <http://www.opengis.net/spec/OMS/3.0> ;
    skos:prefLabel "Conformance Class /conf/obs-core/AbstractObservationCharacteristics" ;
    skos:topConceptOf <http://www.opengis.net/spec/OMS/3.0> .

<http://www.opengis.net/spec/OMS/3.0/conf/obs-core/AbstractObserver> a spec:ConformanceClass,
        skos:Concept ;
    skos:definition "/conf/obs-core/AbstractObserver" ;
    skos:inScheme <http://www.opengis.net/spec/OMS/3.0> ;
    skos:prefLabel "Conformance Class /conf/obs-core/AbstractObserver" ;
    skos:topConceptOf <http://www.opengis.net/spec/OMS/3.0> .

<http://www.opengis.net/spec/OMS/3.0/conf/obs-core/AbstractObservingProcedure> a spec:ConformanceClass,
        skos:Concept ;
    skos:definition "/conf/obs-core/AbstractObservingProcedure" ;
    skos:inScheme <http://www.opengis.net/spec/OMS/3.0> ;
    skos:prefLabel "Conformance Class /conf/obs-core/AbstractObservingProcedure" ;
    skos:topConceptOf <http://www.opengis.net/spec/OMS/3.0> .

<http://www.opengis.net/spec/OMS/3.0/conf/obs-core/NamedValue> a spec:ConformanceClass,
        skos:Concept ;
    skos:definition "/conf/obs-core/NamedValue" ;
    skos:inScheme <http://www.opengis.net/spec/OMS/3.0> ;
    skos:prefLabel "Conformance Class /conf/obs-core/NamedValue" ;
    skos:topConceptOf <http://www.opengis.net/spec/OMS/3.0> .

<http://www.opengis.net/spec/OMS/3.0/conf/obs-cpt> a spec:ConformanceClass,
        skos:Concept ;
    skos:definition "/conf/obs-cpt" ;
    skos:inScheme <http://www.opengis.net/spec/OMS/3.0> ;
    skos:prefLabel "Conformance Class /conf/obs-cpt" ;
    skos:topConceptOf <http://www.opengis.net/spec/OMS/3.0> .

<http://www.opengis.net/spec/OMS/3.0/conf/obs-cpt/Deployment> a spec:ConformanceClass,
        skos:Concept ;
    skos:definition "/conf/obs-cpt/Deployment" ;
    skos:inScheme <http://www.opengis.net/spec/OMS/3.0> ;
    skos:prefLabel "Conformance Class /conf/obs-cpt/Deployment" ;
    skos:topConceptOf <http://www.opengis.net/spec/OMS/3.0> .

<http://www.opengis.net/spec/OMS/3.0/conf/obs-cpt/Host> a spec:ConformanceClass,
        skos:Concept ;
    skos:definition "/conf/obs-cpt/Host" ;
    skos:inScheme <http://www.opengis.net/spec/OMS/3.0> ;
    skos:prefLabel "Conformance Class /conf/obs-cpt/Host" ;
    skos:topConceptOf <http://www.opengis.net/spec/OMS/3.0> .

<http://www.opengis.net/spec/OMS/3.0/conf/obs-cpt/ObservableProperty> a spec:ConformanceClass,
        skos:Concept ;
    skos:definition "/conf/obs-cpt/ObservableProperty" ;
    skos:inScheme <http://www.opengis.net/spec/OMS/3.0> ;
    skos:prefLabel "Conformance Class /conf/obs-cpt/ObservableProperty" ;
    skos:topConceptOf <http://www.opengis.net/spec/OMS/3.0> .

<http://www.opengis.net/spec/OMS/3.0/conf/obs-cpt/Observation> a spec:ConformanceClass,
        skos:Concept ;
    skos:definition "/conf/obs-cpt/Observation" ;
    skos:inScheme <http://www.opengis.net/spec/OMS/3.0> ;
    skos:prefLabel "Conformance Class /conf/obs-cpt/Observation" ;
    skos:topConceptOf <http://www.opengis.net/spec/OMS/3.0> .

<http://www.opengis.net/spec/OMS/3.0/conf/obs-cpt/Observer> a spec:ConformanceClass,
        skos:Concept ;
    skos:definition "/conf/obs-cpt/Observer" ;
    skos:inScheme <http://www.opengis.net/spec/OMS/3.0> ;
    skos:prefLabel "Conformance Class /conf/obs-cpt/Observer" ;
    skos:topConceptOf <http://www.opengis.net/spec/OMS/3.0> .

<http://www.opengis.net/spec/OMS/3.0/conf/obs-cpt/ObservingProcedure> a spec:ConformanceClass,
        skos:Concept ;
    skos:definition "/conf/obs-cpt/ObservingProcedure" ;
    skos:inScheme <http://www.opengis.net/spec/OMS/3.0> ;
    skos:prefLabel "Conformance Class /conf/obs-cpt/ObservingProcedure" ;
    skos:topConceptOf <http://www.opengis.net/spec/OMS/3.0> .

<http://www.opengis.net/spec/OMS/3.0/conf/obs-cpt/Procedure> a spec:ConformanceClass,
        skos:Concept ;
    skos:definition "/conf/obs-cpt/Procedure" ;
    skos:inScheme <http://www.opengis.net/spec/OMS/3.0> ;
    skos:prefLabel "Conformance Class /conf/obs-cpt/Procedure" ;
    skos:topConceptOf <http://www.opengis.net/spec/OMS/3.0> .

<http://www.opengis.net/spec/OMS/3.0/conf/sam-basic> a spec:ConformanceClass,
        skos:Concept ;
    skos:definition "/conf/sam-basic" ;
    skos:inScheme <http://www.opengis.net/spec/OMS/3.0> ;
    skos:prefLabel "Conformance Class /conf/sam-basic" ;
    skos:topConceptOf <http://www.opengis.net/spec/OMS/3.0> .

<http://www.opengis.net/spec/OMS/3.0/conf/sam-basic/MaterialSample> a spec:ConformanceClass,
        skos:Concept ;
    skos:definition "/conf/sam-basic/MaterialSample" ;
    skos:inScheme <http://www.opengis.net/spec/OMS/3.0> ;
    skos:prefLabel "Conformance Class /conf/sam-basic/MaterialSample" ;
    skos:topConceptOf <http://www.opengis.net/spec/OMS/3.0> .

<http://www.opengis.net/spec/OMS/3.0/conf/sam-basic/NamedLocation> a spec:ConformanceClass,
        skos:Concept ;
    skos:definition "/conf/sam-basic/NamedLocation" ;
    skos:inScheme <http://www.opengis.net/spec/OMS/3.0> ;
    skos:prefLabel "Conformance Class /conf/sam-basic/NamedLocation" ;
    skos:topConceptOf <http://www.opengis.net/spec/OMS/3.0> .

<http://www.opengis.net/spec/OMS/3.0/conf/sam-basic/PhysicalDimension> a spec:ConformanceClass,
        skos:Concept ;
    skos:definition "/conf/sam-basic/PhysicalDimension" ;
    skos:inScheme <http://www.opengis.net/spec/OMS/3.0> ;
    skos:prefLabel "Conformance Class /conf/sam-basic/PhysicalDimension" ;
    skos:topConceptOf <http://www.opengis.net/spec/OMS/3.0> .

<http://www.opengis.net/spec/OMS/3.0/conf/sam-basic/Sample> a spec:ConformanceClass,
        skos:Concept ;
    skos:definition "/conf/sam-basic/Sample" ;
    skos:inScheme <http://www.opengis.net/spec/OMS/3.0> ;
    skos:prefLabel "Conformance Class /conf/sam-basic/Sample" ;
    skos:topConceptOf <http://www.opengis.net/spec/OMS/3.0> .

<http://www.opengis.net/spec/OMS/3.0/conf/sam-basic/SampleCollection> a spec:ConformanceClass,
        skos:Concept ;
    skos:definition "/conf/sam-basic/SampleCollection" ;
    skos:inScheme <http://www.opengis.net/spec/OMS/3.0> ;
    skos:prefLabel "Conformance Class /conf/sam-basic/SampleCollection" ;
    skos:topConceptOf <http://www.opengis.net/spec/OMS/3.0> .

<http://www.opengis.net/spec/OMS/3.0/conf/sam-basic/Sampler> a spec:ConformanceClass,
        skos:Concept ;
    skos:definition "/conf/sam-basic/Sampler" ;
    skos:inScheme <http://www.opengis.net/spec/OMS/3.0> ;
    skos:prefLabel "Conformance Class /conf/sam-basic/Sampler" ;
    skos:topConceptOf <http://www.opengis.net/spec/OMS/3.0> .

<http://www.opengis.net/spec/OMS/3.0/conf/sam-basic/Sampling> a spec:ConformanceClass,
        skos:Concept ;
    skos:definition "/conf/sam-basic/Sampling" ;
    skos:inScheme <http://www.opengis.net/spec/OMS/3.0> ;
    skos:prefLabel "Conformance Class /conf/sam-basic/Sampling" ;
    skos:topConceptOf <http://www.opengis.net/spec/OMS/3.0> .

<http://www.opengis.net/spec/OMS/3.0/conf/sam-basic/SpatialSample> a spec:ConformanceClass,
        skos:Concept ;
    skos:definition "/conf/sam-basic/SpatialSample" ;
    skos:inScheme <http://www.opengis.net/spec/OMS/3.0> ;
    skos:prefLabel "Conformance Class /conf/sam-basic/SpatialSample" ;
    skos:topConceptOf <http://www.opengis.net/spec/OMS/3.0> .

<http://www.opengis.net/spec/OMS/3.0/conf/sam-basic/StatisticalClassification> a spec:ConformanceClass,
        skos:Concept ;
    skos:definition "/conf/sam-basic/StatisticalClassification" ;
    skos:inScheme <http://www.opengis.net/spec/OMS/3.0> ;
    skos:prefLabel "Conformance Class /conf/sam-basic/StatisticalClassification" ;
    skos:topConceptOf <http://www.opengis.net/spec/OMS/3.0> .

<http://www.opengis.net/spec/OMS/3.0/conf/sam-basic/StatisticalSample> a spec:ConformanceClass,
        skos:Concept ;
    skos:definition "/conf/sam-basic/StatisticalSample" ;
    skos:inScheme <http://www.opengis.net/spec/OMS/3.0> ;
    skos:prefLabel "Conformance Class /conf/sam-basic/StatisticalSample" ;
    skos:topConceptOf <http://www.opengis.net/spec/OMS/3.0> .

<http://www.opengis.net/spec/OMS/3.0/conf/sam-core> a spec:ConformanceClass,
        skos:Concept ;
    skos:definition "/conf/sam-core" ;
    skos:inScheme <http://www.opengis.net/spec/OMS/3.0> ;
    skos:prefLabel "Conformance Class /conf/sam-core" ;
    skos:topConceptOf <http://www.opengis.net/spec/OMS/3.0> .

<http://www.opengis.net/spec/OMS/3.0/conf/sam-core/AbstractPreparationProcedure> a spec:ConformanceClass,
        skos:Concept ;
    skos:definition "/conf/sam-core/AbstractPreparationProcedure" ;
    skos:inScheme <http://www.opengis.net/spec/OMS/3.0> ;
    skos:prefLabel "Conformance Class /conf/sam-core/AbstractPreparationProcedure" ;
    skos:topConceptOf <http://www.opengis.net/spec/OMS/3.0> .

<http://www.opengis.net/spec/OMS/3.0/conf/sam-core/AbstractPreparationStep> a spec:ConformanceClass,
        skos:Concept ;
    skos:definition "/conf/sam-core/AbstractPreparationStep" ;
    skos:inScheme <http://www.opengis.net/spec/OMS/3.0> ;
    skos:prefLabel "Conformance Class /conf/sam-core/AbstractPreparationStep" ;
    skos:topConceptOf <http://www.opengis.net/spec/OMS/3.0> .

<http://www.opengis.net/spec/OMS/3.0/conf/sam-core/AbstractSample> a spec:ConformanceClass,
        skos:Concept ;
    skos:definition "/conf/sam-core/AbstractSample" ;
    skos:inScheme <http://www.opengis.net/spec/OMS/3.0> ;
    skos:prefLabel "Conformance Class /conf/sam-core/AbstractSample" ;
    skos:topConceptOf <http://www.opengis.net/spec/OMS/3.0> .

<http://www.opengis.net/spec/OMS/3.0/conf/sam-core/AbstractSampler> a spec:ConformanceClass,
        skos:Concept ;
    skos:definition "/conf/sam-core/AbstractSampler" ;
    skos:inScheme <http://www.opengis.net/spec/OMS/3.0> ;
    skos:prefLabel "Conformance Class /conf/sam-core/AbstractSampler" ;
    skos:topConceptOf <http://www.opengis.net/spec/OMS/3.0> .

<http://www.opengis.net/spec/OMS/3.0/conf/sam-core/AbstractSampling> a spec:ConformanceClass,
        skos:Concept ;
    skos:definition "/conf/sam-core/AbstractSampling" ;
    skos:inScheme <http://www.opengis.net/spec/OMS/3.0> ;
    skos:prefLabel "Conformance Class /conf/sam-core/AbstractSampling" ;
    skos:topConceptOf <http://www.opengis.net/spec/OMS/3.0> .

<http://www.opengis.net/spec/OMS/3.0/conf/sam-core/AbstractSamplingProcedure> a spec:ConformanceClass,
        skos:Concept ;
    skos:definition "/conf/sam-core/AbstractSamplingProcedure" ;
    skos:inScheme <http://www.opengis.net/spec/OMS/3.0> ;
    skos:prefLabel "Conformance Class /conf/sam-core/AbstractSamplingProcedure" ;
    skos:topConceptOf <http://www.opengis.net/spec/OMS/3.0> .

<http://www.opengis.net/spec/OMS/3.0/conf/sam-cpt> a spec:ConformanceClass,
        skos:Concept ;
    skos:definition "/conf/sam-cpt" ;
    skos:inScheme <http://www.opengis.net/spec/OMS/3.0> ;
    skos:prefLabel "Conformance Class /conf/sam-cpt" ;
    skos:topConceptOf <http://www.opengis.net/spec/OMS/3.0> .

<http://www.opengis.net/spec/OMS/3.0/conf/sam-cpt/PreparationProcedure> a spec:ConformanceClass,
        skos:Concept ;
    skos:definition "/conf/sam-cpt/PreparationProcedure" ;
    skos:inScheme <http://www.opengis.net/spec/OMS/3.0> ;
    skos:prefLabel "Conformance Class /conf/sam-cpt/PreparationProcedure" ;
    skos:topConceptOf <http://www.opengis.net/spec/OMS/3.0> .

<http://www.opengis.net/spec/OMS/3.0/conf/sam-cpt/PreparationStep> a spec:ConformanceClass,
        skos:Concept ;
    skos:definition "/conf/sam-cpt/PreparationStep" ;
    skos:inScheme <http://www.opengis.net/spec/OMS/3.0> ;
    skos:prefLabel "Conformance Class /conf/sam-cpt/PreparationStep" ;
    skos:topConceptOf <http://www.opengis.net/spec/OMS/3.0> .

<http://www.opengis.net/spec/OMS/3.0/conf/sam-cpt/Sample> a spec:ConformanceClass,
        skos:Concept ;
    skos:definition "/conf/sam-cpt/Sample" ;
    skos:inScheme <http://www.opengis.net/spec/OMS/3.0> ;
    skos:prefLabel "Conformance Class /conf/sam-cpt/Sample" ;
    skos:topConceptOf <http://www.opengis.net/spec/OMS/3.0> .

<http://www.opengis.net/spec/OMS/3.0/conf/sam-cpt/Sampler> a spec:ConformanceClass,
        skos:Concept ;
    skos:definition "/conf/sam-cpt/Sampler" ;
    skos:inScheme <http://www.opengis.net/spec/OMS/3.0> ;
    skos:prefLabel "Conformance Class /conf/sam-cpt/Sampler" ;
    skos:topConceptOf <http://www.opengis.net/spec/OMS/3.0> .

<http://www.opengis.net/spec/OMS/3.0/conf/sam-cpt/Sampling> a spec:ConformanceClass,
        skos:Concept ;
    skos:definition "/conf/sam-cpt/Sampling" ;
    skos:inScheme <http://www.opengis.net/spec/OMS/3.0> ;
    skos:prefLabel "Conformance Class /conf/sam-cpt/Sampling" ;
    skos:topConceptOf <http://www.opengis.net/spec/OMS/3.0> .

<http://www.opengis.net/spec/OMS/3.0/conf/sam-cpt/SamplingProcedure> a spec:ConformanceClass,
        skos:Concept ;
    skos:definition "/conf/sam-cpt/SamplingProcedure" ;
    skos:inScheme <http://www.opengis.net/spec/OMS/3.0> ;
    skos:prefLabel "Conformance Class /conf/sam-cpt/SamplingProcedure" ;
    skos:topConceptOf <http://www.opengis.net/spec/OMS/3.0> .




<http://www.opengis.net/spec/OMS/3.0> a skos:ConceptScheme ;
    dcterms:created "2021-07-08"^^xsd:date ;
    dcterms:modified "2021-07-08"^^xsd:date ;
    dcterms:source <http://www.opengis.net/def/docs/20-082r2> ;
    skos:definition "A convenience hierarchy for navigating the elements of a specification using the SKOS model" ;
    skos:hasTopConcept <http://www.opengis.net/spec/OMS/3.0/conf/obs-cpt>,
		<http://www.opengis.net/spec/OMS/3.0/conf/obs-core>,
		<http://www.opengis.net/spec/OMS/3.0/conf/obs-basic>,
		<http://www.opengis.net/spec/OMS/3.0/conf/obs-cpt/Observation>,
		<http://www.opengis.net/spec/OMS/3.0/conf/obs-core/AbstractObservationCharacteristics>,
		<http://www.opengis.net/spec/OMS/3.0/conf/obs-core/AbstractObservation>,
		<http://www.opengis.net/spec/OMS/3.0/conf/obs-basic/ObservationCharacteristics>,
		<http://www.opengis.net/spec/OMS/3.0/conf/obs-basic/Observation>,
		<http://www.opengis.net/spec/OMS/3.0/conf/obs-basic/ObservingCapability> ;
    skos:prefLabel "Specification elements for OGC 20-082r2 Observations, Measurements and Samples" .