@prefix dc: <http://purl.org/dc/elements/1.1/> .
@prefix dct: <http://purl.org/dc/terms/> .
@prefix owl: <http://www.w3.org/2002/07/owl#> .
@prefix policy: <http://www.opengis.net/def/metamodel/ogc-na/> .
@prefix rdfs: <http://www.w3.org/2000/01/rdf-schema#> .
@prefix skos: <http://www.w3.org/2004/02/skos/core#> .
@prefix status: <http://www.opengis.net/def/status/> .
@prefix xsd: <http://www.w3.org/2001/XMLSchema#> .

<http://www.opengis.net/def/netcdf> a owl:Ontology ;
    rdfs:comment "Definitions from OGC netCDF standards"^^xsd:string ;
    rdfs:seeAlso <http://www.opengeospatial.org/standards/netcdf>,
        <http://www.opengis.net/def/property/netcdf/> ;
    owl:imports <http://www.opengis.net/def/ogc-na> ;
    owl:versionIRI <https://svn.opengeospatial.org/ogc-projects/sp/ogc-na/tags/2012-10/definitions/netcdf.rdf> .

<http://www.opengis.net/def/ogc-netcdf> a skos:ConceptScheme ;
    rdfs:label "OGC NetCDF definitions" ;
    dct:source "OGC Naming Authority on behalf of relevant OGC Working Group" ;
    skos:prefLabel "OGC NetCDF definitions" .

<http://www.opengis.net/def/property> skos:member <http://www.opengis.net/def/property/netcdf/> .

<http://www.opengis.net/def/property/> skos:member <http://www.opengis.net/def/property/netcdf/> .

<http://www.opengis.net/def/property/netcdf> owl:sameAs <http://www.opengis.net/def/property/netcdf/> .

<http://www.opengis.net/def/property/netcdf/1.0> rdfs:label ""^^xsd:string ;
    owl:sameAs <http://www.opengis.net/def/property/netcdf/1.0/> ;
    skos:prefLabel ""^^xsd:string .

<http://www.opengis.net/def/property/netcdf/1.0/byte> a skos:Concept ;
    rdfs:label "byte"^^xsd:string,
        "byte"@en ;
    dc:source <http://www.opengis.net/doc/netcdf#clause-4.1>,
        "OGC netCDF Clause 4.1"^^xsd:string ;
    dct:created "2012-03-27"^^xsd:date ;
    policy:status status:valid ;
    rdfs:seeAlso <http://www.opengis.net/doc/netcdf#clause-4.1>,
        <http://www.opengis.net/doc/netcdf/1.0#clause-4.1>,
        "OGC netCDF Clause 4.1"^^xsd:string ;
    skos:definition "A byte is an eight-bit integer.  The byte type differs from the char type in that it is intended for eight-bit data, and the zero byte has no special significance, as it may for character data."^^xsd:string ;
    skos:inScheme <http://www.opengis.net/def/scheme> ;
    skos:prefLabel "byte"@en .

<http://www.opengis.net/def/property/netcdf/1.0/char> a skos:Concept ;
    rdfs:label "character"^^xsd:string,
        "character"@en ;
    dc:source <http://www.opengis.net/doc/netcdf#clause-4.2>,
        "OGC netCDF Clause 4.2"^^xsd:string ;
    policy:status status:valid ;
    rdfs:seeAlso <http://www.opengis.net/doc/netcdf#clause-4.2>,
        <http://www.opengis.net/doc/netcdf/1.0#clause-4.2>,
        "OGC netCDF Clause 4.2"^^xsd:string ;
    skos:definition "A char is a single Unicode character, and may use up to 32 bits. (Note that ASCII characters are represented in Unicode using 8 bits.)"^^xsd:string ;
    skos:inScheme <http://www.opengis.net/def/scheme> ;
    skos:prefLabel "character"@en .

<http://www.opengis.net/def/property/netcdf/1.0/compound-type> a skos:Concept ;
    policy:status status:valid .

<http://www.opengis.net/def/property/netcdf/1.0/compoundType> a skos:Concept ;
    rdfs:label "compound type"^^xsd:string,
        "compound type"@en ;
    dc:source <http://www.opengis.net/doc/netcdf#clause-4.3>,
        "OGC netCDF Clause 4.3"^^xsd:string ;
    policy:status status:valid ;
    rdfs:seeAlso <http://www.opengis.net/doc/netcdf#clause-4.3>,
        <http://www.opengis.net/doc/netcdf/1.0#clause-4.3>,
        "OGC netCDF Clause 4.3"^^xsd:string ;
    owl:sameAs <http://www.opengis.net/def/property/netcdf/1.0/compound-type> ;
    skos:definition """Compound types are like C structures, grouping together named fields (also called "members"), that may be of different types, into a structure that may be accessed as a unit. It has a fixed total size. It consists of zero or more named members that do not overlap with other members.\r
\r
    Each member has a name distinct from other members.\r
    Each member has its own datatype.\r
    Each member is referenced by an index number between zero and N-1, where N is the number of members in the compound datatype.\r
    Each member has a fixed byte offset, which is the first byte (smallest byte address) of that member in the compound datatype.\r
    In addition to other other user-defined data types or atomic datatypes, a member can be a small fixed-size array of any type with up to four fixed-size “dimensions” (not associated with named netCDF dimensions)."""^^xsd:string ;
    skos:inScheme <http://www.opengis.net/def/scheme> ;
    skos:prefLabel "compound type"@en .

<http://www.opengis.net/def/property/netcdf/1.0/double> a skos:Concept ;
    rdfs:label "Double-precision floating point number"^^xsd:string,
        "Double-precision floating point number"@en ;
    dc:source <http://www.opengis.net/doc/netcdf#clause-4.4>,
        "OGC netCDF Clause 4.4"^^xsd:string ;
    policy:status status:valid ;
    rdfs:seeAlso <http://www.opengis.net/doc/netcdf#clause-4.4>,
        <http://www.opengis.net/doc/netcdf/1.0#clause-4.4>,
        "OGC netCDF Clause 4.4"^^xsd:string ;
    skos:definition "A double is an IEEE double-precision floating point (64 bits.).  The double type can hold values between about -1.7+308 and 1.7+308, with external representation as 64-bit IEEE standard normalized double-precision, floating-point numbers"^^xsd:string ;
    skos:inScheme <http://www.opengis.net/def/scheme> ;
    skos:prefLabel "Double-precision floating point number"@en .

<http://www.opengis.net/def/property/netcdf/1.0/enumerated-type> a skos:Concept ;
    policy:status status:valid .

<http://www.opengis.net/def/property/netcdf/1.0/enumeratedType> a skos:Concept ;
    rdfs:label "Enumeration"^^xsd:string,
        "Enumeration"@en ;
    dc:source <http://www.opengis.net/doc/netcdf#clause-4.5>,
        "OGC netCDF Clause 4.5"^^xsd:string ;
    policy:status status:valid ;
    rdfs:seeAlso <http://www.opengis.net/doc/netcdf#clause-4.5>,
        <http://www.opengis.net/doc/netcdf/1.0#clause-4.5>,
        "OGC netCDF Clause 4.5"^^xsd:string ;
    owl:sameAs <http://www.opengis.net/def/property/netcdf/1.0/enumerated-type> ;
    skos:definition "Enumerated types are used to represent a small number of named values more concisely than strings"^^xsd:string ;
    skos:inScheme <http://www.opengis.net/def/scheme> ;
    skos:prefLabel "Enumeration"@en .

<http://www.opengis.net/def/property/netcdf/1.0/float> a skos:Concept ;
    rdfs:label "Single-precision floating point number"^^xsd:string,
        "Single-precision floating point number"@en ;
    dc:source <http://www.opengis.net/doc/netcdf#clause-4.6>,
        "OGC netCDF Clause 4.6"^^xsd:string ;
    policy:status status:valid ;
    rdfs:seeAlso <http://www.opengis.net/doc/netcdf#clause-4.6>,
        <http://www.opengis.net/doc/netcdf/1.0#clause-4.6>,
        "OGC netCDF Clause 4.6"^^xsd:string ;
    skos:definition "A float is an IEEE single-precision floating point (32 bits).  The float type can hold values between about -3.4+38 and 3.4+38, with external representation as 32-bit IEEE normalized single-precision floating-point numbers"^^xsd:string ;
    skos:inScheme <http://www.opengis.net/def/scheme> ;
    skos:prefLabel "Single-precision floating point number"@en .

<http://www.opengis.net/def/property/netcdf/1.0/group> a skos:Concept ;
    rdfs:label "Group"^^xsd:string ;
    dc:source <http://www.opengis.net/doc/netcdf#clause-4.7>,
        "OGC netCDF Clause 4.7"^^xsd:string ;
    policy:status status:valid ;
    rdfs:seeAlso <http://www.opengis.net/doc/netcdf#clause-4.7>,
        <http://www.opengis.net/doc/netcdf/1.0#clause-4.7>,
        "OGC netCDF Clause 4.7"^^xsd:string ;
    skos:definition "A group provides a nested scope for names"^^xsd:string ;
    skos:inScheme <http://www.opengis.net/def/scheme> ;
    skos:prefLabel "Group"@en .

<http://www.opengis.net/def/property/netcdf/1.0/int> a skos:Concept ;
    rdfs:label "32-bit signed integer"^^xsd:string,
        "32-bit signed integer"@en ;
    dc:source <http://www.opengis.net/doc/netcdf#clause-4.8>,
        "OGC netCDF Clause 4.8"^^xsd:string ;
    policy:status status:valid ;
    rdfs:seeAlso <http://www.opengis.net/doc/netcdf#clause-4.8>,
        <http://www.opengis.net/doc/netcdf/1.0#clause-4.8>,
        "OGC netCDF Clause 4.8"^^xsd:string ;
    skos:definition "An int is a 32-bit signed integer.  An int can hold values between -2147483648 and 2147483647"^^xsd:string ;
    skos:inScheme <http://www.opengis.net/def/scheme> ;
    skos:prefLabel "32-bit signed integer"@en .

<http://www.opengis.net/def/property/netcdf/1.0/int64> a skos:Concept ;
    rdfs:label "8-byte signed integer"^^xsd:string,
        "8-byte signed integer"@en ;
    dc:source <http://www.opengis.net/doc/netcdf#clause-4.9>,
        "OGC netCDF Clause 4.9"^^xsd:string ;
    policy:status status:valid ;
    rdfs:seeAlso <http://www.opengis.net/doc/netcdf#clause-4.9>,
        <http://www.opengis.net/doc/netcdf/1.0#clause-4.9>,
        "OGC netCDF Clause 4.9"^^xsd:string ;
    skos:definition "An int64 is an eight-byte signed integer.   An int64 can hold values between -9223372036854775808 and 9223372036854775807"^^xsd:string ;
    skos:inScheme <http://www.opengis.net/def/scheme> ;
    skos:prefLabel "8-byte signed integer"@en .

<http://www.opengis.net/def/property/netcdf/1.0/long> a skos:Concept ;
    rdfs:label "Long integer"^^xsd:string,
        "Long integer"@en ;
    dc:source <http://www.opengis.net/doc/netcdf#clause-4.10>,
        "OGC netCDF Clause 4.10"^^xsd:string ;
    policy:status status:valid ;
    rdfs:seeAlso <http://www.opengis.net/doc/netcdf#clause-4.10>,
        <http://www.opengis.net/doc/netcdf/1.0#clause-4.10>,
        "OGC netCDF Clause 4.10"^^xsd:string ;
    skos:definition "The long type is deprecated.  It is synonymous with int"^^xsd:string ;
    skos:inScheme <http://www.opengis.net/def/scheme> ;
    skos:prefLabel "Long integer"@en .

<http://www.opengis.net/def/property/netcdf/1.0/opaque-type> a skos:Concept ;
    policy:status status:valid ;
    owl:sameAs <http://www.opengis.net/def/property/netcdf/1.0/opaqueType> .

<http://www.opengis.net/def/property/netcdf/1.0/real> a skos:Concept ;
    rdfs:label "Real number"^^xsd:string,
        "Real number"@en ;
    dc:source <http://www.opengis.net/doc/netcdf#clause-4.12>,
        "OGC netCDF Clause 4.12"^^xsd:string ;
    policy:status status:valid ;
    rdfs:seeAlso <http://www.opengis.net/doc/netcdf#clause-4.12>,
        <http://www.opengis.net/doc/netcdf/1.0#clause-4.12>,
        "OGC netCDF Clause 4.12"^^xsd:string ;
    skos:definition "The real type is synonymous with float"^^xsd:string ;
    skos:inScheme <http://www.opengis.net/def/scheme> ;
    skos:prefLabel "Real number"@en .

<http://www.opengis.net/def/property/netcdf/1.0/short> a skos:Concept ;
    rdfs:label "Short integer"^^xsd:string,
        "Short integer"@en ;
    dc:source <http://www.opengis.net/doc/netcdf#clause-4.13>,
        "OGC netCDF Clause 4.13"^^xsd:string ;
    policy:status status:valid ;
    rdfs:seeAlso <http://www.opengis.net/doc/netcdf#clause-4.13>,
        <http://www.opengis.net/doc/netcdf/1.0#clause-4.13>,
        "OGC netCDF Clause 4.13"^^xsd:string ;
    skos:definition "A short is a 16-bit signed integer.  A short holds values between -32768 and 32767"^^xsd:string ;
    skos:inScheme <http://www.opengis.net/def/scheme> ;
    skos:prefLabel "Short integer"@en .

<http://www.opengis.net/def/property/netcdf/1.0/string> a skos:Concept ;
    rdfs:label "Character string"^^xsd:string,
        "Character string"@en ;
    dc:source <http://www.opengis.net/doc/netcdf#clause-4.14>,
        "OGC netCDF Clause 4.14"^^xsd:string ;
    policy:status status:valid ;
    rdfs:seeAlso <http://www.opengis.net/doc/netcdf#clause-4.14>,
        <http://www.opengis.net/doc/netcdf/1.0#clause-4.14>,
        "OGC netCDF Clause 4.14"^^xsd:string ;
    skos:definition "A string is a variable length string of characters"^^xsd:string ;
    skos:inScheme <http://www.opengis.net/def/scheme> ;
    skos:prefLabel "Character string"@en .

<http://www.opengis.net/def/property/netcdf/1.0/unsigned-int> a skos:Concept ;
    policy:status status:valid ;
    owl:sameAs <http://www.opengis.net/def/property/netcdf/1.0/unsignedInt> .

<http://www.opengis.net/def/property/netcdf/1.0/unsigned-int-64> a skos:Concept ;
    policy:status status:valid ;
    owl:sameAs <http://www.opengis.net/def/property/netcdf/1.0/unsignedInt64> .

<http://www.opengis.net/def/property/netcdf/1.0/unsigned-short> a skos:Concept ;
    policy:status status:valid ;
    owl:sameAs <http://www.opengis.net/def/property/netcdf/1.0/unsignedShort> .

<http://www.opengis.net/def/property/netcdf/1.0/user-defined-type> a skos:Concept ;
    policy:status status:valid ;
    owl:sameAs <http://www.opengis.net/def/property/netcdf/1.0/userDefinedType> .

<http://www.opengis.net/def/property/netcdf/1.0/variable-length-type> a skos:Concept ;
    policy:status status:valid ;
    owl:sameAs <http://www.opengis.net/def/property/netcdf/1.0/variableLengthType> .

<http://www.opengis.net/def/property/netcdf/1.0/> a skos:Collection ;
    rdfs:label "netCDF properties 1.0" ;
    skos:member <http://www.opengis.net/def/property/netcdf/1.0/byte>,
        <http://www.opengis.net/def/property/netcdf/1.0/char>,
        <http://www.opengis.net/def/property/netcdf/1.0/compoundType>,
        <http://www.opengis.net/def/property/netcdf/1.0/double>,
        <http://www.opengis.net/def/property/netcdf/1.0/enumeratedType>,
        <http://www.opengis.net/def/property/netcdf/1.0/float>,
        <http://www.opengis.net/def/property/netcdf/1.0/group>,
        <http://www.opengis.net/def/property/netcdf/1.0/int>,
        <http://www.opengis.net/def/property/netcdf/1.0/int64>,
        <http://www.opengis.net/def/property/netcdf/1.0/long>,
        <http://www.opengis.net/def/property/netcdf/1.0/opaqueType>,
        <http://www.opengis.net/def/property/netcdf/1.0/real>,
        <http://www.opengis.net/def/property/netcdf/1.0/short>,
        <http://www.opengis.net/def/property/netcdf/1.0/string>,
        <http://www.opengis.net/def/property/netcdf/1.0/unsignedInt>,
        <http://www.opengis.net/def/property/netcdf/1.0/unsignedInt64>,
        <http://www.opengis.net/def/property/netcdf/1.0/unsignedShort>,
        <http://www.opengis.net/def/property/netcdf/1.0/userDefinedType>,
        <http://www.opengis.net/def/property/netcdf/1.0/variableLengthType> .

<http://www.opengis.net/def/property/netcdf/1.0/opaqueType> a skos:Concept ;
    rdfs:label "Opaque collection"^^xsd:string,
        "Opaque collection"@en ;
    dc:source <http://www.opengis.net/doc/netcdf#clause-4.11>,
        "OGC netCDF Clause 4.11"^^xsd:string ;
    policy:status status:valid ;
    rdfs:seeAlso <http://www.opengis.net/doc/netcdf#clause-4.11>,
        <http://www.opengis.net/doc/netcdf/1.0#clause-4.11>,
        "OGC netCDF Clause 4.11"^^xsd:string ;
    owl:sameAs <http://www.opengis.net/def/property/netcdf/1.0/opaque-type> ;
    skos:definition "Opaque is a collection of objects of a known size.  Each object is the same size.  Nothing is known to netCDF about the contents of these blobs of data, except their size in bytes, and the name of the type"^^xsd:string ;
    skos:inScheme <http://www.opengis.net/def/scheme> ;
    skos:prefLabel "Opaque collection"@en .

<http://www.opengis.net/def/property/netcdf/1.0/unsignedInt> a skos:Concept ;
    rdfs:label "Unsigned 32-bit Integer"^^xsd:string,
        "Unsigned 32-bit Integer"@en ;
    dc:source <http://www.opengis.net/doc/netcdf#clause-4.15>,
        "OGC netCDF Clause 4.15"^^xsd:string ;
    policy:status status:valid ;
    rdfs:seeAlso <http://www.opengis.net/doc/netcdf#clause-4.15>,
        <http://www.opengis.net/doc/netcdf/1.0#clause-4.15>,
        "OGC netCDF Clause 4.15"^^xsd:string ;
    owl:sameAs <http://www.opengis.net/def/property/netcdf/1.0/unsigned-int> ;
    skos:definition "An unsigned int is a 32-bit unsigned integer.  An unsigned int holds values between 0 and 4294967296"^^xsd:string ;
    skos:inScheme <http://www.opengis.net/def/scheme> ;
    skos:prefLabel "Unsigned 32-bit Integer"@en .

<http://www.opengis.net/def/property/netcdf/1.0/unsignedInt64> a skos:Concept ;
    rdfs:label "Unsigned 64-bit Integer"^^xsd:string,
        "Unsigned 64-bit Integer"@en ;
    dc:source <http://www.opengis.net/doc/netcdf#clause-4.16>,
        "OGC netCDF Clause 4.16"^^xsd:string ;
    policy:status status:valid ;
    rdfs:seeAlso <http://www.opengis.net/doc/netcdf#clause-4.16>,
        <http://www.opengis.net/doc/netcdf/1.0#clause-4.16>,
        "OGC netCDF Clause 4.16"^^xsd:string ;
    owl:sameAs <http://www.opengis.net/def/property/netcdf/1.0/unsigned-int-64> ;
    skos:definition "An unsigned int64 is an unsigned 8-byte integer type. An unsigned int64 can hold values between 0 and 18446744073709551616"^^xsd:string ;
    skos:inScheme <http://www.opengis.net/def/scheme> ;
    skos:prefLabel "Unsigned 64-bit Integer"@en .

<http://www.opengis.net/def/property/netcdf/1.0/unsignedShort> a skos:Concept ;
    rdfs:label "Unsigned Short"^^xsd:string ;
    dc:source <http://www.opengis.net/doc/netcdf#clause-4.17>,
        "OGC netCDF Clause 4.17"^^xsd:string ;
    policy:status status:valid ;
    rdfs:seeAlso <http://www.opengis.net/doc/netcdf#clause-4.17>,
        <http://www.opengis.net/doc/netcdf/1.0#clause-4.17>,
        "OGC netCDF Clause 4.17"^^xsd:string ;
    owl:sameAs <http://www.opengis.net/def/property/netcdf/1.0/unsigned-short> ;
    skos:definition "An unsigned short is a 16-bit unsigned integer.  An unsigned short holds values between 0 and 65536"^^xsd:string ;
    skos:inScheme <http://www.opengis.net/def/scheme> ;
    skos:prefLabel "Unsigned Short"@en .

<http://www.opengis.net/def/property/netcdf/1.0/userDefinedType> a skos:Concept ;
    rdfs:label "User Defined Type"^^xsd:string,
        "User Defined Type"@en ;
    dc:source <http://www.opengis.net/doc/netcdf#clause-4.18>,
        "OGC netCDF Clause 4.18"^^xsd:string ;
    policy:status status:valid ;
    rdfs:seeAlso <http://www.opengis.net/doc/netcdf#clause-4.18>,
        <http://www.opengis.net/doc/netcdf/1.0#clause-4.18>,
        "OGC netCDF Clause 4.18"^^xsd:string ;
    owl:sameAs <http://www.opengis.net/def/property/netcdf/1.0/user-defined-type> ;
    skos:definition "User defined types are: compound, enumerated, variable-length, and opaque"^^xsd:string ;
    skos:inScheme <http://www.opengis.net/def/scheme> ;
    skos:prefLabel "User Defined Type"@en .

<http://www.opengis.net/def/property/netcdf/1.0/variableLengthType> a skos:Concept ;
    rdfs:label "Variable Length Type"^^xsd:string,
        "Variable Length Type"@en ;
    dc:source <http://www.opengis.net/doc/netcdf#clause-4.19>,
        "OGC netCDF Clause 4.19"^^xsd:string ;
    policy:status status:valid ;
    rdfs:seeAlso <http://www.opengis.net/doc/netcdf#clause-4.19>,
        <http://www.opengis.net/doc/netcdf/1.0#clause-4.19>,
        "OGC netCDF Clause 4.19"^^xsd:string ;
    owl:sameAs <http://www.opengis.net/def/property/netcdf/1.0/variable-length-type> ;
    skos:definition "The variable length type represents a one-dimensional array of variable length"^^xsd:string ;
    skos:inScheme <http://www.opengis.net/def/scheme> ;
    skos:prefLabel "Variable Length Type"@en .

<http://www.opengis.net/def/property/netcdf/> a skos:Collection ;
    rdfs:label "netCDF properties" ;
    skos:member <http://www.opengis.net/def/property/netcdf/1.0/> .

